@prefix owl: <http://www.w3.org/2002/07/owl#> .
@prefix rdf: <http://www.w3.org/1999/02/22-rdf-syntax-ns#> .
@prefix xsd: <http://www.w3.org/2001/XMLSchema#> .
@prefix rdfs: <http://www.w3.org/2000/01/rdf-schema#> .
@prefix cc: <http://creativecommons.org/ns#> .
@prefix oa: <https://www.w3.org/ns/oa> .
@prefix schema: <http://schema.org/> .
@prefix dcterms: <http://purl.org/dc/terms/> .
@prefix dc: <http://purl.org/dc/elements/1.1/> .
@prefix skos: <http://www.w3.org/2004/02/skos/core#> .
@prefix vann: <http://purl.org/vocab/vann/> .
@prefix dbo: <http://dbpedia.org/ontology/> .
@prefix dbr: <http://dbpedia.org/resource/> .
@prefix deo: <http://purl.org/spar/deo/> .
@prefix dul: <http://www.ontologydesignpatterns.org/ont/dul/DUL.owl#> .
@prefix geo: <http://www.geonames.org/ontology#> .
@prefix om2: <http://www.ontology-of-units-of-measure.org/resource/om-2/> .
@prefix doap: <http://usefulinc.com/ns/doap#> .
@prefix foaf: <http://xmlns.com/foaf/0.1/> .
@prefix lvont:<http://lexvo.org/ontology> .
@prefix void:<http://www.w3.org/TR/void/> .
@prefix lang: <http://lexvo.org/id/iso639-3/> .
@prefix muto: <http://purl.org/muto/core#> .
@prefix obda: <https://w3id.org/obda/vocabulary#> .
@prefix prov: <http://www.w3.org/ns/prov#> .
@prefix sto: <https://w3id.org/i40/sto#> .
@prefix sto_iot: <https://w3id.org/i40/sto/iot#> .

<https://w3id.org/i40/sto#> rdf:type owl:Ontology ;
                            dcterms:modified "2017-09-08"^^xsd:date ,
                                             "2019-01-23"^^xsd:date ,                                        
                                             "2019-01-23"^^xsd:date ,
                                             "2019-12-04"^^xsd:date ;     
                            void:sparqlEndpoint <https://dydra.com/mtasnim/stoviz/sparql>;
                            void:dataDump <https://dydra.com/mtasnim/stoviz.ttl>;
                            owl:versionInfo "0.9"^^xsd:double ;
                            rdfs:label "Industry 4.0 Knowledge Graph"@en ;
                            dcterms:title "Industry 4.0 Knowledge Graph"@en ;
                            rdfs:comment "A Knowledge Graph to describe standards and standardization frameworks related to Industry 4.0 and Smart Manufacturing"@en ;
                            dcterms:rights "This work is distributed under a Creative Commons Attribution License (http://creativecommons.org/licenses/by/3.0/)."@en ;
                            dcterms:license <https://creativecommons.org/licenses/by-nc/3.0/legalcode> ;
                            dcterms:publisher <http://de.dbpedia.org/resource/Fraunhofer-Gesellschaft> ;
                            doap:repository <https://github.com/i40-Tools/StandardsOntology> ;
                            vann:preferredNamespaceUri "https://w3id.org/i40/sto#"^^xsd:anyURI ;
                            vann:preferredNamespacePrefix "sto"^^xsd:string ;
                            dcterms:created "2017-01-25"^^xsd:date ;
                            dcterms:creator sto:irlan,
                                            sto:sebastian ,  
                                             <http://data.semanticweb.org/person/steffen-lohmann> ,
                                            <https://www.linkedin.com/in/paul-baptista-601177b2> ;
                           .


#################################################################
#    Annotation properties
#################################################################

###  http://creativecommons.org/ns#attributionURL
cc:attributionURL rdf:type owl:AnnotationProperty .


###  http://purl.org/dc/elements/1.1/date
dc:date rdf:type owl:AnnotationProperty .


###  http://purl.org/dc/elements/1.1/description
dc:description rdf:type owl:AnnotationProperty ;
                 dcterms:description "Description may include but is not limited to: an abstract, a table of contents, a graphical representation, or a free-text account of the resource."@en ;
                 dcterms:hasVersion <http://dublincore.org/usage/terms/history/#description-006> ;
                 dcterms:issued "1999-07-02"^^xsd:date ;
                 dcterms:modified "2008-01-14"^^xsd:date ;
                 rdfs:comment "An account of the resource."@en ;
                 rdfs:isDefinedBy dc: ;
                 rdfs:label "Description"@en ;
                 skos:note "A second property with the same name as this property has been declared in the dcterms: namespace (http://purl.org/dc/terms/).  See the Introduction to the document \"DCMI Metadata Terms\" (http://dublincore.org/documents/dcmi-terms/) for an explanation."@en .


###  http://purl.org/dc/elements/1.1/relation
dc:relation rdf:type owl:AnnotationProperty .


###  http://purl.org/dc/elements/1.1/title
dc:title rdf:type owl:AnnotationProperty ;
           dcterms:hasVersion <http://dublincore.org/usage/terms/history/#title-006> ;
           dcterms:issued "1999-07-02"^^xsd:date ;
           dcterms:modified "2008-01-14"^^xsd:date ;
           rdfs:comment "A name given to the resource."@en ;
           rdfs:isDefinedBy dc: ;
           rdfs:label "Title"@en ;
           skos:note "A second property with the same name as this property has been declared in the dcterms: namespace (http://purl.org/dc/terms/).  See the Introduction to the document \"DCMI Metadata Terms\" (http://dublincore.org/documents/dcmi-terms/) for an explanation."@en .


###  http://purl.org/dc/terms/description
dcterms:description rdf:type owl:AnnotationProperty ;
                    dcterms:description "Description may include but is not limited to: an abstract, a table of contents, a graphical representation, or a free-text account of the resource."@en ;
                    dcterms:hasVersion <http://dublincore.org/usage/terms/history/#descriptionT-001> ;
                    dcterms:issued "2008-01-14"^^xsd:date ;
                    dcterms:modified "2008-01-14"^^xsd:date ;
                    rdfs:comment "An account of the resource."@en ;
                    rdfs:isDefinedBy dcterms: ;
                    rdfs:label "Description"@en .


###  http://purl.org/dc/terms/format
dcterms:format rdf:type owl:AnnotationProperty .


###  http://purl.org/dc/terms/license
dcterms:license rdf:type owl:AnnotationProperty ;
                   dcterms:hasVersion <http://dublincore.org/usage/terms/history/#license-002> ;
                   dcterms:issued "2004-06-14"^^xsd:date ;
                   dcterms:modified "2017-12-19"^^xsd:date ;
                   rdfs:comment "A legal document giving official permission to do something with the resource."@en ,
                                "Represent the license document for a given Standard"@en ;
                   rdfs:label "has License"@en .

###  http://purl.org/dc/terms/hasVersion
dcterms:hasVersion rdf:type owl:AnnotationProperty ;
                   dcterms:hasVersion <http://dublincore.org/usage/terms/history/#hasVersion-003> ;
                   dcterms:issued "2000-07-11"^^xsd:date ;
                   dcterms:modified "2008-01-14"^^xsd:date ;
                   rdfs:comment "A related resource that is a version, edition, or adaptation of the described resource."@en ;
                   rdfs:isDefinedBy dcterms: ;
                   rdfs:label "Has Version"@en ;
                   skos:note "This term is intended to be used with non-literal values as defined in the DCMI Abstract Model (http://dublincore.org/documents/abstract-model/).  As of December 2007, the DCMI Usage Board is seeking a way to express this intention with a formal range declaration."@en .

###  http://purl.org/dc/terms/issued
dcterms:issued rdf:type owl:AnnotationProperty ;
               dcterms:hasVersion <http://dublincore.org/usage/terms/history/#issued-003> ;
               dcterms:issued "2000-07-11"^^xsd:date ;
               dcterms:modified "2008-01-14"^^xsd:date ;
               rdfs:comment "Date of formal issuance (e.g., publication) of the resource."@en ;
               rdfs:isDefinedBy dcterms: ;
               rdfs:label "Date Issued"@en .

###  http://purl.org/dc/terms/license
dcterms:license rdf:type owl:AnnotationProperty ;
                dcterms:hasVersion <http://dublincore.org/usage/terms/history/#license-002> ;
                dcterms:issued "2004-06-14"^^xsd:date ;
                dcterms:modified "2017-12-19"^^xsd:date ;
                rdfs:comment "A legal document giving official permission to do something with the resource."@en ,
                             "A legal document giving official permission to do something with the resource. In this ontology denotes the license of a Standard."@en ,
                             "Represent the license document for a given Standard"@en ;
                rdfs:isDefinedBy dcterms: ;
                rdfs:label "has License"@en .


###  http://purl.org/dc/terms/modified
dcterms:modified rdf:type owl:AnnotationProperty ;
                 dcterms:hasVersion <http://dublincore.org/usage/terms/history/#modified-003> ;
                 dcterms:issued "2000-07-11"^^xsd:date ;
                 dcterms:modified "2008-01-14"^^xsd:date ;
                 rdfs:comment "Date on which the resource was changed."@en ;
                 rdfs:isDefinedBy dcterms: ;
                 rdfs:label "Date Modified"@en .


###  http://purl.org/dc/terms/title
dcterms:title rdf:type owl:AnnotationProperty ;
              dcterms:hasVersion <http://dublincore.org/usage/terms/history/#titleT-002> ;
              dcterms:issued "2008-01-14"^^xsd:date ;
              dcterms:modified "2010-10-11"^^xsd:date ;
              rdfs:comment "A name given to the resource."@en ;
              rdfs:isDefinedBy dcterms: ;
              rdfs:label "Title"@en .


###  http://swrl.stanford.edu/ontologies/3.3/swrla.owl#isRuleEnabled
<http://swrl.stanford.edu/ontologies/3.3/swrla.owl#isRuleEnabled> rdf:type owl:AnnotationProperty .



###  http://www.w3.org/1999/02/22-rdf-syntax-ns#value
rdf:value rdf:type owl:AnnotationProperty .


###  http://www.w3.org/2004/02/skos/core#altLabel
skos:altLabel rdf:type owl:AnnotationProperty ;
              rdfs:label "alternative label"@en .


###  http://www.w3.org/2004/02/skos/core#definition
skos:definition rdf:type owl:AnnotationProperty ;
                rdfs:label "definition"@en .


###  https://w3id.org/i40/sto#hasDomain
sto:hasDomain rdf:type owl:ObjectProperty ;
              rdfs:domain sto:Publication ;
              rdfs:range sto:Domain ;
              rdfs:comment "Describes the domain, in which the Publication is used, particularly, standards."@en ;
              rdfs:label "has Domain"@en ;
              .

###  https://w3id.org/i40/sto#hasStakeholder
sto:hasStakeholder rdf:type owl:ObjectProperty ;
                   rdfs:comment "This property links entities to the typical stakeholder which is interested in the topic."@en ;
                   rdfs:label "has Stakeholder" ;
                   skos:note "Subproperty of http://voag.linkedmodel.org/voag#hasStakeholder (vocabulary not accessible)."@en ;
                   rdfs:range sto_iot:StakeholderGroup .

###  http://www.w3.org/2004/02/skos/core#note
skos:note rdf:type owl:AnnotationProperty ;
          rdfs:label "note"@en .


###  http://www.w3.org/2004/02/skos/core#prefLabel
skos:prefLabel rdf:type owl:AnnotationProperty ;
               rdfs:label "preferred label"@en .


###  http://www.w3.org/ns/prov#wasRevisionOf
prov:wasRevisionOf rdf:type owl:AnnotationProperty .


###  http://xmlns.com/foaf/0.1/familyName
foaf:familyName rdf:type owl:AnnotationProperty ;
                rdfs:label "Family Name"@en .


###  http://xmlns.com/foaf/0.1/mbox
foaf:mbox rdf:type owl:AnnotationProperty ;
          rdfs:label "mbox"@en .


###  http://xmlns.com/foaf/0.1/name
foaf:name rdf:type owl:AnnotationProperty ;
          rdfs:label "name"@en .


###  https://w3id.org/i40/sto#Tag
sto:Tag rdf:type owl:AnnotationProperty .


###  https://w3id.org/i40/sto#alignsWith
sto:alignsWith rdf:type owl:ObjectProperty .


###  https://w3id.org/i40/sto#hasDBpediaResource
sto:hasDBpediaResource rdf:type owl:AnnotationProperty ;
                       rdfs:comment "Instance's DBpedia Resource"@en ;
                       rdfs:label "has DBpedia Resource"@en .


###  https://w3id.org/i40/sto#hasStakeholder
sto:hasStakeholder rdf:type owl:AnnotationProperty ;
                   rdfs:comment "This property links entities to the typical stakeholder which is interested in the topic."@en ;
                   rdfs:label "has Stakeholder" ;
                   skos:note "Subproperty of http://voag.linkedmodel.org/voag#hasStakeholder (vocabulary not accessible)."@en ;
                   rdfs:range sto_iot:hasStakeholder .



###  http://www.w3.org/2004/02/skos/core#prefLabel
skos:prefLabel rdf:type owl:AnnotationProperty ;
               rdfs:label "preferred label"@en .

###  https://w3id.org/i40/sto#hasWikipediaArticle
sto:hasWikipediaArticle rdf:type owl:AnnotationProperty .

###  http://www.w3.org/ns/prov#wasRevisionOf
prov:wasRevisionOf rdf:type owl:AnnotationProperty .

###  https://w3id.org/i40/sto#publisher
sto:publisher rdf:type owl:AnnotationProperty .

###  http://xmlns.com/foaf/0.1/familyName
foaf:familyName rdf:type owl:AnnotationProperty ;
                rdfs:label "Family Name"@en .

###  https://w3id.org/i40/sto#seeAlso
sto:seeAlso rdf:type owl:AnnotationProperty .

###  http://xmlns.com/foaf/0.1/mbox
foaf:mbox rdf:type owl:AnnotationProperty ;
          rdfs:label "mbox"@en .


###  http://xmlns.com/foaf/0.1/name
foaf:name rdf:type owl:AnnotationProperty ;
          rdfs:label "name"@en .

###  https://www.w3.org/ns/oahasBody
oa:hasBody rdf:type owl:AnnotationProperty .


###  https://www.w3.org/ns/oahasEndSelector
oa:hasEndSelector rdf:type owl:AnnotationProperty .


###  https://www.w3.org/ns/oahasSelector
oa:hasSelector rdf:type owl:AnnotationProperty .


###  https://www.w3.org/ns/oahasSource
oa:hasSource rdf:type owl:AnnotationProperty .


###  https://www.w3.org/ns/oahasStartSelector
oa:hasStartSelector rdf:type owl:AnnotationProperty .


###  https://www.w3.org/ns/oahasTarget
oa:hasTarget rdf:type owl:AnnotationProperty .


#################################################################
#    Datatypes
#################################################################

###  http://purl.org/muto/core#Tag
muto:Tag rdf:type rdfs:Datatype .


###  http://www.w3.org/2001/XMLSchema#date
xsd:date rdf:type rdfs:Datatype .


###  http://www.w3.org/2001/XMLSchema#gYear
xsd:gYear rdf:type rdfs:Datatype .


#################################################################
#    Object Properties
#################################################################

###  http://purl.org/dc/terms/creator
dcterms:creator rdf:type owl:ObjectProperty ;
                owl:equivalentProperty foaf:maker ;
                rdfs:comment "An entity primarily responsible for making the resource."@en ;
                dcterms:hasVersion <http://dublincore.org/usage/terms/history/#creatorT-002> ;
                rdfs:isDefinedBy dcterms: ;
                dcterms:modified "2010-10-11"^^xsd:date ;
                rdfs:label "has Creator"@en ;
                dcterms:issued "2008-01-14"^^xsd:date ;
                dcterms:description "Examples of a Creator include a person, an organization, or a service."@en .


###  https://w3id.org/i40/sto#isImplementationOf
sto:isImplementationOf rdf:type owl:ObjectProperty ;
                       dcterms:creator sto:irlan .


###  http://purl.org/dc/terms/language
dcterms:language rdf:type owl:ObjectProperty .


###  http://www.ontology-of-units-of-measure.org/resource/om-2/hasUnit
om2:hasUnit rdf:type owl:ObjectProperty ;
            rdfs:range om2:Unit ;
            rdfs:label "has unit"@en .


###  http://www.ontologydesignpatterns.org/ont/dul/DUL.owl#associatedWith
dul:associatedWith rdf:type owl:ObjectProperty .


###  http://www.ontologydesignpatterns.org/ont/dul/DUL.owl#isComponentOf
dul:isComponentOf rdf:type owl:ObjectProperty ;
                  rdfs:subPropertyOf sto:relatedTo ;
                  rdfs:domain sto:Standard ;
                  rdfs:range [ rdf:type owl:Class ;
                               owl:unionOf ( sto:Standard
                                             sto:StandardPart
                                           )
                             ] ;
                  rdfs:comment "Represents Standards that are component of other Standards. This relation is not transitive"@en ;
                  rdfs:isDefinedBy <http://www.ontologydesignpatterns.org/ont/dul/DUL.owl> ;
                  rdfs:label "is Component Of"@en .


###  http://www.ontologydesignpatterns.org/ont/dul/DUL.owl#isMemberOf
dul:isMemberOf rdf:type owl:ObjectProperty ;
               rdfs:subPropertyOf dul:associatedWith ;
               rdfs:range dul:Collection ;
               rdfs:comment "A relation between collections and entities, e.g. 'the Night Watch by Rembrandt is in the Rijksmuseum collection'; 'Davide is member of the Pen Club', 'Igor is one the subjects chosen for the experiment'."@en ;
               rdfs:isDefinedBy <http://www.ontologydesignpatterns.org/ont/dul/DUL.owl> ;
               rdfs:label "is member of"@en ,
                          "è membro di"@it .


###  http://www.ontologydesignpatterns.org/ont/dul/DUL.owl#isPartOf
dul:isPartOf rdf:type owl:ObjectProperty ;
             rdfs:label "isPartOf"@en .



###  https://w3id.org/i40/sto#isPartOf
sto:isPartOf rdf:type owl:ObjectProperty ;
             rdfs:subPropertyOf dul:isPartOf ;
             rdfs:domain sto:Publication ;
             rdfs:range sto:Publication ;
			 rdfs:comment "specifies that one publication is a part or a section of another publication. Mostly used to indicate that a sto:Standard is a part of standard familiy or group of standards."@en ;
             rdfs:label "is part of"@en .



###  http://www.w3.org/ns/prov#wasGeneratedBy
prov:wasGeneratedBy rdf:type owl:ObjectProperty ;
                    rdfs:subPropertyOf sto:relatedTo ;
                    rdfs:comment "Standard A has influences in Standard B. For example, IEC_61499 hasInfluenceIn IEC_61804-2(EDDL)"@en ;
                    rdfs:isDefinedBy <https://www.w3.org/TR/prov-o/#wasGeneratedBy> ;
                    rdfs:label "was Generated By"@en .


###  http://xmlns.com/foaf/0.1/maker
foaf:maker rdf:type owl:ObjectProperty .


###  https://w3id.org/i40/sto#alignsWith
sto:alignsWith rdf:type owl:ObjectProperty ;
               rdfs:subPropertyOf dul:associatedWith ;
               rdf:type owl:SymmetricProperty ;
               rdfs:domain sto:StandardClassification ;
               rdfs:range sto:StandardClassification ;
               rdfs:comment "indicates that some Standard Classification entity has a similar scope as another. This property most probably is symmetric but not transitive."@en ;
               rdfs:label "alignes With"@en .


###  https://w3id.org/i40/sto#belongsTo
sto:belongsTo rdf:type owl:ObjectProperty ;
              rdfs:domain sto:StandardOrganization ;
              rdfs:range dbo:Country ;
              dcterms:creator sto:irlan;
              rdfs:label "belongs To"@en ;
              rdfs:comment "A Standard Organization that belongs to the country"@en ;
              .



###  https://w3id.org/i40/sto#hasAvailableLanguage
sto:hasAvailableLanguage rdf:type owl:ObjectProperty ;
                         rdfs:range lvont:Language;
                         rdfs:domain foaf:Document ;
                         rdfs:label "hasAvailableLanguage"@en ;
                         rdfs:comment "Points to Languages in which the standard document is available, e.g., English, French, etc. Defined as subProperty of dcterms:language"@en ,
                                      "Languages in which the document of the Standard is available, e.g., English, French, Spanish"@en .


###  https://w3id.org/i40/sto#hasClassification
sto:hasClassification rdf:type owl:ObjectProperty ;
                      rdfs:domain sto:Publication ;
                      rdfs:range sto:StandardClassification ;
                      dcterms:creator sto:irlan .


###  https://w3id.org/i40/sto#hasDeveloper
sto:hasDeveloper rdf:type owl:ObjectProperty ;
                 rdfs:subPropertyOf foaf:maker ;
                 rdfs:label "has Developer"@en;
                 rdfs:comment "Links the Standard Organization that developed the Publication with the specific type of publication, e.g., Standard, Technical Report"@en;
                 rdfs:domain sto:Publication ;
                 rdfs:range sto:StandardOrganization ;
                 dcterms:creator sto:irlan ;                 
                 .


###  https://w3id.org/i40/sto#hasDimension
sto:hasDimension rdf:type owl:ObjectProperty ;
                 rdfs:domain sto:StandardizationFramework ;
                 rdfs:range sto:Dimension ;
                 rdfs:comment "Links the Standardization Frameworks with the Dimensions."@en ;
                 rdfs:label "has Dimension"@en .


###  https://w3id.org/i40/sto#hasDimensionLayer
sto:hasDimensionLayer rdf:type owl:ObjectProperty ;
                      rdfs:domain sto:Dimension ;
                      rdfs:range sto:Layer ;
                      rdfs:comment "Links the Dimensions with Layers."@en ;
                      rdfs:label "has Dimension Layer"@en .


###  https://w3id.org/i40/sto#hasDomain
sto:hasDomain rdf:type owl:ObjectProperty ;
              rdfs:domain sto:Publication ;
              rdfs:range sto:Domain ;
              rdfs:comment "Describes the domain, in which the Publication is used, particularly, standards."@en ;
              rdfs:label "has Domain"@en .


###  https://w3id.org/i40/sto#hasFileSize
sto:hasFileSize rdf:type owl:ObjectProperty,
                         owl:FunctionalProperty ;
                rdfs:domain foaf:Document ;
                rdfs:range om2:Measure .


###  https://w3id.org/i40/sto#hasHeadquaterIn
sto:hasHeadquaterIn rdf:type owl:ObjectProperty ;
                    rdfs:domain sto:StandardOrganization ;
                    rdfs:range dbo:Place .


###  https://w3id.org/i40/sto#hasICS
sto:hasICS rdf:type owl:ObjectProperty;
           rdfs:domain sto:Publication ;
           rdfs:range sto:InternationalClassificationForStandards ;
           rdfs:comment "Serves as a catalogue of International Classification For Standards"@en ;
           rdfs:label "has ICS"@en .


###  https://w3id.org/i40/sto#hasLayer
sto:hasLayer rdf:type owl:ObjectProperty ;
             rdfs:domain sto:StandardizationFramework ;
             rdfs:range sto:Layer ;
             rdfs:comment "Links the Standardization Frameworks with the Layers "@en ;
             rdfs:label "has Layer"@en .


###  https://w3id.org/i40/sto#hasPreviousVersion
sto:hasPreviousVersion rdf:type owl:ObjectProperty ;
                       rdfs:subPropertyOf sto:relatedTo ;
                       rdfs:comment "Indicates the list of Standards that are previous versions of a Standard. For example,IEC 60038:2009 has IEC 60038:1983+AMD1:1994+AMD2:1997,IEC 60038:1983/AMD2:1997,IEC 60038:1983/AMD1:1994,IEC 60038:1983,IEC 60038:1975/AMD1:1977,IEC 60038:1975,IEC 60038:1967,IEC 60038:1954,IEC 60038:1938,IEC 60038:1927 as previous versions."@en ;
                       rdfs:label "has Previous Version"@en .


###  https://w3id.org/i40/sto#hasPublisher
sto:hasPublisher rdf:type owl:ObjectProperty ;
                 rdfs:subPropertyOf foaf:maker ;
                 rdfs:domain sto:Publication ;
                 rdfs:range sto:StandardOrganization .


###  https://w3id.org/i40/sto#hasTag
sto:hasTag rdf:type owl:ObjectProperty ;
           rdfs:range [ rdf:type owl:Class ;
                        owl:unionOf ( muto:Tag
                                      rdfs:Literal
                                    )
                      ] .


###  https://w3id.org/i40/sto#hasTechnicalCommittee
sto:hasTechnicalCommittee rdf:type owl:ObjectProperty ;
                          rdfs:domain sto:Publication ;
                          rdfs:range sto:TechnicalCommittee ;
                          rdfs:comment "Specifies the Technical Committee or a Sub-Committee that is responsible for creation and maintenance of a standard"@en ;
                          rdfs:label "has Technical Committee"@en .


###  https://w3id.org/i40/sto#identifies
sto:identifies rdf:type owl:ObjectProperty ;
               rdfs:subPropertyOf dul:associatedWith ;
               rdfs:comment "ISO 42010 relation between an architecture description on the on hand and stakeholders and concerns on the other."@en ;
               rdfs:label "identifies"@en .


###  https://w3id.org/i40/sto#isDescribedin
sto:isDescribedin rdf:type owl:ObjectProperty ;
                  rdfs:domain sto:StandardClassification ;
                  rdfs:range sto:StandardizationFramework ;
                  rdfs:comment "Links the Standarization Frameworks with the Classification of Standards"@en ;
                  rdfs:label "is Described in"@en .


###  https://w3id.org/i40/sto#isImplementationOf
sto:isImplementationOf rdf:type owl:ObjectProperty ;
                       rdfs:subPropertyOf sto:relatedTo .


###  https://w3id.org/i40/sto#isPartOf
sto:isPartOf rdf:type owl:ObjectProperty ;
             rdfs:domain sto:Publication ;
             rdfs:range sto:Publication ;
             rdfs:comment "specifies that one publication is a part or a section of another publication. Mostly used to indicate that a sto:Standard is a part of standard familiy or group of standards."@en ;
             rdfs:label "is part of"@en .


###  https://w3id.org/i40/sto#isRelevantFor
sto:isRelevantFor rdf:type owl:ObjectProperty ;
                  rdfs:domain sto:Standard ;
                  rdfs:range sto:RelevantSubject ;
                  rdfs:comment "An Standard is concerned with Relevant Subjects"@en ;
                  rdfs:label "is Relevant for"@en .


###  https://w3id.org/i40/sto#relatedTo
sto:relatedTo rdf:type owl:ObjectProperty ;
              rdf:type owl:SymmetricProperty ,
                       owl:TransitiveProperty ;
              rdfs:domain sto:Standard ;
              rdfs:range sto:Standard ;
              skos:altLabel "has Associated Standard"@en ;
              rdfs:comment "General property to represent any type of relation that connects two standards."@en ;
              rdfs:label "related To"@en .


###  https://w3id.org/i40/sto#useStructureOf
sto:useStructureOf rdf:type owl:ObjectProperty ;
                   rdfs:subPropertyOf sto:relatedTo ;
                   rdfs:comment "Standard A uses the structure of Standard B. For example, OPC UA uses Structure Of IEC_61804 (EDDL)"@en ;
                   rdfs:label "use Structure Of"@en .


###  https://w3id.org/i40/sto#uses
sto:uses rdf:type owl:ObjectProperty ;
         rdfs:subPropertyOf sto:relatedTo .

###  https://w3id.org/i40/sto#hasDeveloper
sto:hasDeveloper rdf:type owl:ObjectProperty ;
                 dcterms:creator sto:irlan .

###  https://w3id.org/i40/sto#hasFileSize
sto:hasFileSize rdf:type owl:ObjectProperty,
                        owl:FunctionalProperty ;
                dcterms:creator sto:irlan .


###  https://w3id.org/i40/sto#hasHeadquaterIn
sto:hasHeadquaterIn rdf:type owl:ObjectProperty ;
                    dcterms:creator sto:irlan .


###  https://w3id.org/i40/sto#hasPublisher
sto:hasPublisher rdf:type owl:ObjectProperty ;
                 dcterms:creator sto:irlan .




sto:hasClassification rdf:type owl:ObjectProperty ;
                      rdfs:comment "An Standard is isCategorizedBy a given Categorization Area which is connected to a specific Standarization Initiative"@en ;
                      rdfs:label "has Classification"@en;
                      rdfs:domain sto:Publication ;
                      rdfs:range sto:StandardClassification ;
                      dcterms:creator sto:irlan. 


sto:hasDeveloper rdfs:label "has Developer"@en ;
                 rdfs:comment "The organization that developed this Standard"@en .




sto:hasFileSize skos:note """1. Reference for om2:Measure <http://www.ontology-of-units-of-measure.org/page/om-2/Measure>
                         2. om2:Measure om2:hasNumericalValue xsd:float;
                         3. om2:Measure om2:hasUnit om2:Unit;
                         4. om2:hasUnit om2:InformationCapacityUnit; is another possibility for range that could not be verified.
                         5. rdfs:seeAlso <http://www.ontology-of-units-of-measure.org/page/om-2/kilobyte> 
                         6. Documentation on Measure <https://github.com/HajoRijgersberg/OM>"""@en ;
                rdfs:seeAlso <https://webstore.iec.ch/webstore/webstore.nsf/xpFAQ.xsp?Open&id=ADMN-7NALM5> ;
                rdfs:label "has File Size"@en ;
                rdfs:comment "The size of document file in some unit, e.g., 104 Kilobyte."@en .


sto:hasHeadquaterIn rdfs:label "has Headquater In"@en ;
                    rdfs:comment "Denotes the countries in which the Headquarter of the organization who publishes the Standart"@en .


sto:hasOfficialResource rdf:type owl:DatatypeProperty ;
                        rdfs:range xsd:anyURI ;
                        rdfs:comment "Points to the URL of the official website from which published the document"@en ;
                        rdfs:label "has Official Resource"@en .


sto:hasOpenResource rdfs:label "has Open Resource"@en ;
                    rdfs:comment "points to the URLs of the resources(documents) openly available for the standard"@en .


sto:hasPublisher rdfs:label "has Publisher"@en ;
                 rdfs:comment "The organization that published this Standard"@en .

###  https://w3id.org/i40/sto/iot#alignsWith
sto_iot:alignsWith rdf:type owl:ObjectProperty ;
                   rdfs:subPropertyOf dul:associatedWith ;
                   owl:inverseOf sto_iot:alignsWith ;
                   rdf:type owl:SymmetricProperty ;
                   rdfs:domain sto:StandardClassification ;
                   rdfs:range sto:StandardClassification ;
                   rdfs:comment "indicates that some Standard Classification entity has a similar scope as another. This property most probably is symmetric but not transitive."@en ;
                   rdfs:label "alignes With"@en .

sto:hasWikipediaArticle rdfs:label "has Wikipedia Article"@en ;
                        rdfs:range xsd:anyURI ;
                        rdfs:comment "Wikipedia Article about the Standard"@en .

###  https://w3id.org/i40/sto/iot#frames
sto_iot:frames rdf:type owl:ObjectProperty ;
               rdfs:subPropertyOf dul:associatedWith ;
               rdfs:domain sto:StandardClassification ;
               rdfs:range sto_iot:Concern ;
               rdfs:comment "A relation specifying that a vewpoint regards a Concern."@en ;
               rdfs:label "frames"@en ;
               sto:hasOfficialResource <http://www.iso-architecture.org/42010/> .

sto:isImplementationOf rdfs:label "is Implementation Of"@en ;
                       rdfs:comment "Represent the relation that connects two standards when standard A is the implementation of standard B, e.g., B2MML isImplementationOf ISA-95."@en .

###  https://w3id.org/i40/sto/iot#hasTargetConcern
sto_iot:hasTargetConcern rdf:type owl:ObjectProperty ;
                         rdfs:subPropertyOf dul:associatedWith ;
                         rdfs:domain [ rdf:type owl:Class ;
                                       owl:unionOf ( sto:Standard
                                                     sto:StandardizationFramework
                                                   )
                                     ] .

sto:useStructureOf rdfs:comment "Standard A uses the structure of Standard B. For example, OPC UA uses Structure Of IEC_61804 (EDDL)"@en ;
                   rdfs:label "use Structure Of"@en .

###  https://w3id.org/i40/sto/iot#supports
sto_iot:supports rdf:type owl:ObjectProperty ;
                 rdfs:domain sto_iot:Concern ;
                 rdfs:range sto_iot:Concern ;
                 rdfs:comment "A relation between two different concerns where dealing with the subject Concern supports in achieving the object concern"@en ;
                 rdfs:label "supports" .

sto:uses rdfs:comment "Defines that Standard A uses Standard B. For example, IEC_62714(AML) uses MathML."@en ;
         rdfs:label "uses"@en .


#################################################################
#    Data properties
#################################################################

###  http://creativecommons.org/ns#attributionName
cc:attributionName rdf:type owl:DatatypeProperty .


###  http://creativecommons.org/ns#attributionURL
cc:attributionURL rdf:type owl:DatatypeProperty .


###  http://www.ontology-of-units-of-measure.org/resource/om-2/hasNumericalValue
om2:hasNumericalValue rdf:type owl:DatatypeProperty ;
                      rdfs:label "has numerical value"@en .


###  https://w3id.org/i40/sto#abbreviation
sto:abbreviation rdf:type owl:DatatypeProperty ;
                 rdfs:range rdf:PlainLiteral ;
                 rdfs:comment "Abbreviated name of the thing."@en ;
                 rdfs:label "has Abbreviated Name"@en .


###  https://w3id.org/i40/sto#domainName
sto:domainName rdf:type owl:DatatypeProperty ;
               rdfs:domain sto:RelevantDomain;
               rdfs:range rdf:PlainLiteral ;
               rdfs:comment "Points the Standard with the name of the Industrial Domain"@en ;
               rdfs:label "has Domain Name"@en .


###  https://w3id.org/i40/sto#formationDate
sto:formationDate rdf:type owl:DatatypeProperty ,
                           owl:FunctionalProperty ;
                  rdfs:domain sto:StandardOrganization ;
                  rdfs:range xsd:date ;
                  rdfs:comment "Formation date of the Organization"@en ;
                  rdfs:label "has Formation Date"@en .


###  https://w3id.org/i40/sto#hasEdition
sto:hasEdition rdf:type owl:DatatypeProperty ;
               rdfs:domain foaf:Document ;
               rdfs:range xsd:float ;
               rdfs:comment "Indicates the current Edition/Version number of the document."@en ;
               rdfs:label "has Edition"@en .


###  https://w3id.org/i40/sto#hasImplementationFormat
sto:hasImplementationFormat rdf:type owl:DatatypeProperty ;
                            rdfs:domain sto:Publication ;
                            rdfs:range rdfs:Literal ;
                            rdfs:comment "Describes the name of the implementation or serialization format of the Publication, e.g., XML, Document, binary, batch"@en ;
                            rdfs:label "has Implementation Format"@en .


###  https://w3id.org/i40/sto#hasMotivation
sto:hasMotivation rdf:type owl:DatatypeProperty ;
                  rdfs:domain sto:Publication ;
                  rdfs:range rdfs:Literal ;
                  rdfs:label "has Motivation"@en .


###  https://w3id.org/i40/sto#hasObjective
sto:hasObjective rdf:type owl:DatatypeProperty ;
                 rdfs:domain sto:ISA95Level ;
                 rdfs:range xsd:string ;
                 rdfs:comment "Specifies the objectives for the different ISA 95 levels."@en ;
                 rdfs:label "has Objective"@en .


###  https://w3id.org/i40/sto#hasOfficialResource
sto:hasOfficialResource rdf:type owl:DatatypeProperty ;
                        rdfs:domain sto:Publication ;
                        rdfs:range xsd:anyURI .


###  https://w3id.org/i40/sto#hasOntology
sto:hasOntology rdf:type owl:DatatypeProperty ;
                rdfs:domain sto:Publication ;
                rdfs:range xsd:anyURI ;
                rdfs:comment "Point to the URL of a recognized Ontology representation of the Standard"@en ;
                rdfs:label "has Ontology"@en .


###  https://w3id.org/i40/sto#hasOpenResource
sto:hasOpenResource rdf:type owl:DatatypeProperty ;
                    rdfs:domain sto:Publication ;
                    rdfs:range xsd:anyURI .


###  https://w3id.org/i40/sto#hasPages
sto:hasPages rdf:type owl:DatatypeProperty ;
             rdfs:domain foaf:Document ;
             rdfs:range xsd:integer ;
             rdfs:comment "Indicates the number of pages in the document."@en ;
             rdfs:label "has Pages"@en .


###  https://w3id.org/i40/sto#hasPublicationDate
sto:hasPublicationDate rdf:type owl:DatatypeProperty ;
                       rdfs:domain sto:Publication ;
                       rdfs:range xsd:date ;
                       rdfs:comment "Publication date of the Publication"@en ;
                       rdfs:label "has Publication Date"@en .


###  https://w3id.org/i40/sto#hasStabilityDate
sto:hasStabilityDate rdf:type owl:DatatypeProperty ;
                     rdfs:domain sto:Publication ;
                     rdfs:range xsd:gYear ;
                     rdfs:comment "Stability date of a publication. Publications are valid for a certain period, i.e., the Stability Period. This property defines the end of the stability period."@en ;
                     rdfs:label "has Stability Date"@en ;
                     rdfs:seeAlso <https://webstore.iec.ch/webstore/webstore.nsf/xpFAQ.xsp?Open&id=ADMN-7NALM5> ;
                     skos:note "The data specified is not actually a Date but an Year"@en .


###  https://w3id.org/i40/sto#hasStatus
sto:hasStatus rdf:type owl:DatatypeProperty ;
              rdfs:domain sto:Publication ;
              rdfs:range rdfs:Literal ;
              rdfs:comment "Publication status of the Standard, e.g., Valid, Revised, Published, under preparation, Released"@en ;
              rdfs:label "has Status"@en .


###  https://w3id.org/i40/sto#hasTag
sto:hasTag rdf:type owl:DatatypeProperty ;
           rdfs:range [ owl:unionOf ( muto:Tag
                                      rdfs:Literal
                                    )
                      ] ;
           rdfs:comment "Points to the identification of the standards"@en ;
           rdfs:label "has Tag"@en .

###  https://w3id.org/i40/sto#hasTargetConcern
sto_iot:hasTargetConcern rdf:type owl:ObjectProperty ;
                     rdfs:subPropertyOf dul:associatedWith ;
                     rdfs:domain  sto:Standard;
                     rdfs:range sto_iot:Concern ;
                     rdfs:comment "The relation declaring that a standard is relevant for a certain concern."@en ;
                     rdfs:label "has Target Concern"@en .


###  https://w3id.org/i40/sto#hasTask
sto:hasTask rdf:type owl:DatatypeProperty ;
            rdfs:domain sto:ISA95Level ;
            rdfs:range xsd:string ;
            rdfs:comment "Specifies the tasks for the different ISA 95 levels."@en ;
            rdfs:label "has Task"@en .


###  https://w3id.org/i40/sto#hasWikipediaArticle
sto:hasWikipediaArticle rdf:type owl:DatatypeProperty .


###  https://w3id.org/i40/sto#orgName
sto:orgName rdf:type owl:DatatypeProperty ;
            rdfs:domain sto:StandardOrganization ;
            rdfs:range rdf:PlainLiteral ;
            rdfs:comment "Name of the Organization"@en ;
            rdfs:label "Org Name"@en .


###  https://w3id.org/i40/sto#stoPartName
sto:stoPartName rdf:type owl:DatatypeProperty ;
                rdfs:domain sto:StandardPart ;
                rdfs:range xsd:string ;
                rdfs:comment "Name of the standard part."@en ;
                rdfs:label "std Part Name"@en .


#################################################################
#    Classes
#################################################################

###  http://dbpedia.org/ontology/Country
dbo:Country rdf:type owl:Class .


###  http://dbpedia.org/ontology/Place
dbo:Place rdf:type owl:Class .


###  http://purl.org/dc/terms/LicenseDocument
dcterms:LicenseDocument rdf:type owl:Class ;
                        rdfs:comment "A legal document giving official permission to do something with a Resource."@en ;
                        rdfs:isDefinedBy dcterms: ;
                        rdfs:label "License Document"@en .


###  http://purl.org/dc/terms/LinguisticSystem
dcterms:LinguisticSystem rdf:type owl:Class .


###  http://purl.org/spar/deo/Motivation
deo:Motivation rdf:type owl:Class .


###  http://www.ontology-of-units-of-measure.org/resource/om-2/Measure
om2:Measure rdf:type owl:Class .


###  http://www.ontology-of-units-of-measure.org/resource/om-2/Unit
om2:Unit rdf:type owl:Class .


###  http://www.ontologydesignpatterns.org/ont/dul/DUL.owl#Collection
dul:Collection rdf:type owl:Class .


###  http://www.w3.org/2002/07/owl#class
owl:class rdf:type owl:Class .


###  http://xmlns.com/foaf/0.1/Document
foaf:Document rdf:type owl:Class .


###  http://xmlns.com/foaf/0.1/Organization
foaf:Organization rdf:type owl:Class .


###  http://xmlns.com/foaf/0.1/Person
foaf:Person rdf:type owl:Class .


###  https://w3id.org/i40/sto#AdminShellSubmodel
sto:RamiAdminShellSubmodel rdf:type owl:Class ;
                        rdfs:subClassOf sto:StandardClassification ;
                        rdfs:comment "Describes the Administration Shell concept to organize/classify standards into submodels"@en ;
                        rdfs:isDefinedBy <https://www.plattform-i40.de/I40/Redaktion/EN/Downloads/Publikation/structure-of-the-administration-shell.pdf?__blob=publicationFile&v=7> ;
                        rdfs:label "Admin Shell Sub Model"@en .


###  https://w3id.org/i40/sto#RamiControlDevice
sto:RamiControlDevice rdf:type owl:Class ;
                        rdfs:subClassOf sto:StandardClassification ;
                        rdfs:label "RAMI Control Device"@en ;
                        dcterms:creator sto:sebastian ;
                        rdfs:isDefinedBy sto:Rami ;
                        .


###  https://w3id.org/i40/sto#RamiHierarchyLevel
sto:RamiHierarchyLevel rdf:type owl:Class ;
                        owl:equivalentClass [ rdf:type owl:Class ;
                                              owl:oneOf ( sto:RamiConnectedWorld
                                                          sto:RamiControlDevice
                                                          sto:RamiEnterprise
                                                          sto:RamiFieldDevice
                                                          sto:RamiProduct
                                                          sto:RamiStation
                                                          sto:RamiWorkCenter
                                                        )
                                            ] ;
                        rdfs:subClassOf sto:StandardClassification ;
                        rdfs:label "RAMI Hierarchy Level"@en .


###  https://w3id.org/i40/sto#RamiITLayer
sto:RamiITLayer rdf:type owl:Class ;
                 owl:equivalentClass [ rdf:type owl:Class ;
                                       owl:oneOf ( sto:RamiAssetlayer
                                                   sto:RamiBusinessLayer
                                                   sto:RamiCommunicationlayer
                                                   sto:RamiFunctionalLayer
                                                   sto:RamiInformationLayer
                                                   sto:RamiIntegrationLayer
                                                 )
                                     ] ;
                 rdfs:subClassOf sto:StandardClassification ;
                 rdfs:label "RAMI IT Layer"@en .


###  https://w3id.org/i40/sto#RamiLifeCycleLayer
sto:RamiLifeCycleLayer rdf:type owl:Class ;
                        rdfs:subClassOf sto:StandardClassification ;
                        rdfs:label "RAMI Life Cycle Layer"@en ;
                        rdfs:seeAlso <http://www.zvei.org/en/subjects/Industry-40/Pages/The-Reference-Architectural-Model-RAMI-40-and-the-Industrie-40-Component.aspx> ;
                        skos:definition "It describes the different Life Cycle and Value Stream layers for the RAMI model according to the IEC 62890 Standard."@en ;
                        skos:prefLabel "RAMI Life Cycle Layer"@en .


###  https://w3id.org/i40/sto#AiiClassification
sto:AiiClassification rdf:type owl:Class ;
                      rdfs:subClassOf sto:StandardClassification .


###  https://w3id.org/i40/sto#ArchitectureDescription
sto:ArchitectureDescription rdf:type owl:Class ;
                            rdfs:subClassOf sto:StandardizationFramework ;
                            rdfs:comment """A Reference Architecture describes the structure of a system with its element types and their structures, as well as their interaction types, among each other and with their environment. Describing this, a Reference Architecture defines restrictions for an instantiation (concrete architecture). Through abstraction from individual details, a Reference Architecture is universally valid within a specific domain. Further architectures with the same functional requirements can be constructed based on the reference architecture. Along with reference architectures comes a recommendation, based on experiences from existing developments as well as from a wide acceptance and recognition by its users or per definition. [ISO/IEC42010]
Note: It is important to distinguish the Reference Architecture from a Reference Architecture Description. While the first refers to a mental model or shared concept, the second is potentially only one of several different documents describing this model."""@en ,
                                         "ISO 42010 definition of an Architecture Description"@en ;
                            rdfs:label "Architecture Description" ;
                            rdfs:seeAlso <https://www.iso.org/standard/50508.html> .


###  https://w3id.org/i40/sto#BdvaConcern
sto:BdvaConcern rdf:type owl:Class ;
                rdfs:subClassOf sto:StandardClassification .


###  https://w3id.org/i40/sto#BusinessCycleSCM
sto:BusinessCycleSCM rdf:type owl:Class ;
                     rdfs:subClassOf sto:StandardClassification ;
                     rdfs:comment "Suply Chain Management Business Cycle."@en ;
                     rdfs:isDefinedBy <http://nvlpubs.nist.gov/nistpubs/ir/2016/NIST.IR.8107.pdf> ;
                     rdfs:label "Business Cycle SCM"@en ;
                     rdfs:seeAlso <https://en.wikipedia.org/wiki/Supply_chain_management> .


###  https://w3id.org/i40/sto#DataSharingInitiative
sto:DataSharingInitiative rdf:type owl:Class ;
                          rdfs:subClassOf foaf:Organization .


###  https://w3id.org/i40/sto#Dimension
sto:Dimension rdf:type owl:Class ;
              rdfs:comment "Links the Standardization Frameworks with the Layers"@en ;
              rdfs:label "Dimension"@en .


###  https://w3id.org/i40/sto#Domain
sto:RelevantDomain rdf:type owl:Class ;
           rdfs:comment "Represents the Domains in which the Standards can be used"@en ;
           rdfs:label "RelevantDomain"@en .


###  https://w3id.org/i40/sto#EdgecrossLayer
sto:EdgecrossLayer rdf:type owl:Class ;
                   rdfs:subClassOf sto:StandardClassification ,
                                   [ rdf:type owl:Restriction ;
                                     owl:onProperty sto:isDescribedin ;
                                     owl:hasValue sto:EdgecrossArchitecture
                                   ] ;
                   rdfs:label "Edgecross Layer"@en .


###  https://w3id.org/i40/sto#FiwareChapter
sto:FiwareChapter rdf:type owl:Class ;
                  rdfs:subClassOf sto:StandardClassification .


###  https://w3id.org/i40/sto#IDSRAMLayer
sto:IDSRAMLayer rdf:type owl:Class ;
                owl:equivalentClass [ rdf:type owl:Class ;
                                      owl:oneOf ( sto:IDSRAMBusinessLayer
                                                  sto:IDSRAMFunctionalLayer
                                                  sto:IDSRAMInformationLayer
                                                  sto:IDSRAMProcessLayer
                                                  sto:IDSRAMSystemLayer
                                                )
                                    ] ;
                rdfs:subClassOf sto:StandardClassification .


###  https://w3id.org/i40/sto#IIRACrosscuttingFunction
sto:IIRACrosscuttingFunction rdf:type owl:Class ;
                             rdfs:subClassOf sto:StandardClassification ,
                                             [ rdf:type owl:Restriction ;
                                               owl:onProperty dul:isPartOf ;
                                               owl:hasValue sto:IIRAFunctionalViewpoint
                                             ] .


###  https://w3id.org/i40/sto#IIRAFunctionalDomain
sto:IIRAFunctionalDomain rdf:type owl:Class ;
                         rdfs:subClassOf sto:StandardClassification ,
                                         [ rdf:type owl:Restriction ;
                                           owl:onProperty dul:isPartOf ;
                                           owl:hasValue sto:IIRAFunctionalViewpoint
                                         ] ,
                                         [ rdf:type owl:Restriction ;
                                           owl:onProperty sto:isDescribedin ;
                                           owl:hasValue sto:IIRA
                                         ] .


###  https://w3id.org/i40/sto#IIRASystemCharacteristics
sto:IIRASystemCharacteristics rdf:type owl:Class ;
                              rdfs:subClassOf sto:StandardClassification ,
                                              [ rdf:type owl:Restriction ;
                                                owl:onProperty dul:isPartOf ;
                                                owl:hasValue sto:IIRAFunctionalViewpoint
                                              ] ,
                                              [ rdf:type owl:Restriction ;
                                                owl:onProperty sto:isDescribedin ;
                                                owl:hasValue sto:IIRA
                                              ] .


###  https://w3id.org/i40/sto#IIoTConsortium
sto:IIoTConsortium rdf:type owl:Class ;
                   rdfs:subClassOf foaf:Organization .


###  https://w3id.org/i40/sto#ISA95Level
sto:ISA95Level rdf:type owl:Class ;
               rdfs:subClassOf sto:StandardClassification ;
               rdfs:comment "Describes the ISA95 levels to classify the industry Standards according to those levels. Eg., Device, SCADA, etc. It has strong relation to the RAMI Hierarchy levels"@en ;
               rdfs:label "ISA 95 Level"@en .


###  https://w3id.org/i40/sto#IdsPerspective
sto:IdsPerspective rdf:type owl:Class ;
                   owl:equivalentClass [ rdf:type owl:Class ;
                                         owl:oneOf ( sto:IDSRAMCertification
                                                     sto:IDSRAMGovernance
                                                     sto:IDSRAMSecurity
                                                   )
                                       ] ;
                   rdfs:subClassOf sto:StandardClassification .


###  https://w3id.org/i40/sto#IicfConnectivityLayer
sto:IicfConnectivityLayer rdf:type owl:Class ;
                          rdfs:subClassOf sto:StandardClassification ,
                                          [ rdf:type owl:Restriction ;
                                            owl:onProperty dul:isPartOf ;
                                            owl:hasValue sto:IIRAConnectivity
                                          ] .


###  https://w3id.org/i40/sto#InternationalClassificationForStandards
sto:InternationalClassificationForStandards rdf:type owl:Class .


###  https://w3id.org/i40/sto#IotaPerspective
sto:IotaPerspective rdf:type owl:Class ;
                    rdfs:subClassOf sto:StandardClassification .


###  https://w3id.org/i40/sto#IviLayer
sto:IviLayer rdf:type owl:Class ;
             rdfs:subClassOf sto:StandardClassification .


###  https://w3id.org/i40/sto#Layer
sto:Layer rdf:type owl:Class ;
          rdfs:comment "Describes the layers of the standardization frameworks. In some cases, the layers are connected to dimensions of the frameworks. "@en ;
          rdfs:label "Layer"@en .


###  https://w3id.org/i40/sto#NGSI_Context_Information_Management_API
sto:NGSI_Context_Information_Management_API rdf:type owl:Class ;
                                            rdfs:subClassOf sto:StandardClassification ,
                                                            [ rdf:type owl:Restriction ;
                                                              owl:onProperty sto:isDescribedin ;
                                                              owl:hasValue sto:FIWARE
                                                            ] .


###  https://w3id.org/i40/sto#OcfBlock
sto:OcfBlock rdf:type owl:Class ;
             rdfs:subClassOf sto:StandardClassification .


###  https://w3id.org/i40/sto#ProductDevelopmentLifeCycle
sto:ProductDevelopmentLifeCycle rdf:type owl:Class ;
                                rdfs:subClassOf sto:StandardClassification ;
                                rdfs:comment "PLM is the process of managing the entire lifecycle of a product from inception, through engineering design and manufacture, to service and disposal of manufactured products. Related areas are PLMManagement, Modeling Practice, Product Model Data exchange, Manufacturing Model Data, Product Catalog Data."@en ,
                                             "Product Development Life-Cycle Phase"@en ;
                                rdfs:isDefinedBy <https://en.wikipedia.org/wiki/Product_lifecycle> ;
                                rdfs:label "Product Development Life Cycle"@en .


###  https://w3id.org/i40/sto#ProductionSystemLifeCycle
sto:ProductionSystemLifeCycle rdf:type owl:Class ;
                              rdfs:subClassOf sto:StandardClassification ;
                              rdfs:comment "Collections of machines, equipment, and auxiliary systems organized to create goods and services from various resources."@en ;
                              rdfs:isDefinedBy <http://nvlpubs.nist.gov/nistpubs/ir/2016/NIST.IR.8107.pdf> ;
                              rdfs:label "Production System Life Cycle"@en .


###  https://w3id.org/i40/sto#Publication
sto:Publication rdf:type owl:Class ;
                rdfs:subClassOf foaf:Document ;
                rdfs:comment """Specifies a Publication. E.g., International Standards,Technical Specifications,Publicly Available Specifications,Amendments
                Technical Corrigenda,Interpretation Sheets,Technical Reports,Guides"""@en ;
                rdfs:isDefinedBy sto:IEC ;
                rdfs:label "Publication"@en ;
                rdfs:seeAlso <http://www.iec.ch/standardsdev/publications/> .


###  https://w3id.org/i40/sto#RelevantSubject
sto:RelevantSubject rdf:type owl:Class ;
                    rdfs:comment "A subject that is relevant in the context of a standard (IEC standards in specific). As specified in IEC Website ."@en ;
                    rdfs:label "Relevant Subject"@en .

###  https://w3id.org/i40/sto#StandardClassification
sto:StandardClassification rdf:type owl:Class;
                 rdfs:comment "Describes categorization areas that the different Standardizations Initiatives use to category Standards."@en ;
                           rdfs:label "Standard Classification"@en ;
                 rdfs:comment "A category or section of a standard or reference framework. StandardClassification reflects views and viewpoints as defined by ISO 42010."@en ;
                 rdfs:label "Standard Classification"@en ;
                 rdfs:isDefinedBy <http://cabibbo.dia.uniroma3.it/asw/altrui/iso-iec-ieee-42010-2011.pdf>;
                 sto:hasOfficialResource <http://www.iso-architecture.org/42010/>.

###  https://w3id.org/i40/sto#Stakeholder
sto:Stakeholder rdf:type owl:Class ;
                rdfs:subClassOf foaf:Person ;
                rdfs:comment "A stakeholder is an individual, team, organization or classes thereof,having an interest in a concern and by extension an interest in the viewpoint and system."@en ;
                rdfs:label "Layer"@en ;
                rdfs:seeAlso "IIC:PUB:G1:V1.80:20170131" ;
                skos:note "Publications referred: 'IIC:PUB:G1:V1.80:20170131' '4.1 STAKEHOLDERS' 'Page 20' " ;
                sto:hasWikipediaArticle <https://en.wikipedia.org/wiki/Stakeholder> .



###  https://w3id.org/i40/sto#InternationalClassificationForStandards
sto:InternationalClassificationForStandards rdf:type owl:Class ;
                                            rdfs:seeAlso <https://www.iso.org/publication/PUB100033.html> ;
                                            rdfs:label "International Classification For Standards"@en ;
                                            sto:hasOfficialResource <https://www.iso.org/publication/PUB100033.html> ;
                                            rdfs:comment "Serves as a structure for catalogues of international, regional and national standards and other normative documents, and as a basis for standing-order systems."@en .


###  https://w3id.org/i40/sto#Standard
sto:Standard rdf:type owl:Class ;
             rdfs:subClassOf sto:Publication ;
             rdfs:label "Standard"@en ;
             rdfs:comment "A document, established by consensus and approved by a recognized body, that provides, for common and repeated use, rules, guidelines or characteristics for activities or their results, aimed at the achievement of the optimum degree of order in a given context."@en ;
             cc:attributionURL <http://www.iec.ch> ;
            cc:attributionName "Copyright © 2016 IEC Geneva, Switzerland."@en ;
             rdfs:isDefinedBy sto:IEC ;
             rdfs:seeAlso <http://www.iec.ch/standardsdev/publications/is.htm> ;
.             




###  https://w3id.org/i40/sto#StandardOrganization
sto:StandardOrganization rdf:type owl:Class ;
                         rdfs:subClassOf foaf:Organization ;
                         rdfs:comment "Define the standards organizations that develop and publish industry standards"@en ;
                         rdfs:label "StandardOrganization"@en .


###  https://w3id.org/i40/sto#StandardPart
sto:StandardPart rdf:type owl:Class ;
                 rdfs:subClassOf sto:Publication ;
                 rdfs:comment "Typically Standards are divided into parts. E.g., ISA 95 has part Part 1: Models and Terminology, Part 2: Object Model Attributes, etc."@en ;
                 rdfs:label "StandardPart"^^xsd:string .


###  https://w3id.org/i40/sto#StandardizationFramework
sto:StandardizationFramework rdf:type owl:Class ;
                 rdfs:comment "A framework is conventions, principles and practices for the description of architectures established within a specific domain of application and/or community of stakeholders."@en ;
                 rdfs:label "Standardization Framework";
                 rdfs:isDefinedBy <http://cabibbo.dia.uniroma3.it/asw/altrui/iso-iec-ieee-42010-2011.pdf>;
                 sto:hasOfficialResource <http://www.iso-architecture.org/42010/>; 
                 skos:altLabel "Reference Architecture"@en ;
                 rdfs:comment "Describes existings Standardizations Initiatives, e.g, RAMI, NIST."@en ;
.


###  https://w3id.org/i40/sto#TechnicalCommittee
sto:TechnicalCommittee rdf:type owl:Class ;
                       rdfs:subClassOf foaf:Organization .


###  https://w3id.org/i40/sto#TechnicalReport
sto:TechnicalReport rdf:type owl:Class ;
                    rdfs:subClassOf sto:Publication ;
                    sto:abbreviation "TR"^^xsd:string ;
                    .


###  https://w3id.org/i40/sto#TechnicalSpecification
sto:TechnicalSpecification rdf:type owl:Class ;
                           rdfs:subClassOf sto:Publication ;
                           cc:attributionURL <http://www.iec.ch> ;
                           rdfs:comment "Specifies that a given Publication is a Technical Specification"@en ,
                                        "Technical Specifications are often published when the subject under question is still under development or when insufficient consensus for approval of an International Standard is available.Technical Specifications approach International Standards in terms of detail and completeness, but have not yet passed through all approval stages either because consensus has not been reached or because standardization is seen to be premature."@en ;
                           rdfs:isDefinedBy sto:IEC ;
                           rdfs:label "Technical Specification"@en ;
                           rdfs:seeAlso <http://www.iec.ch/standardsdev/publications/ts.htm> .


###  https://w3id.org/i40/sto#Technology
sto:Technology rdf:type owl:Class ;
               rdfs:subClassOf sto:Publication .


###  https://w3id.org/i40/sto#Viewpoint
sto:Viewpoint rdf:type owl:Class ;
              rdfs:subClassOf sto:StandardClassification .


###  https://w3id.org/i40/sto#standard
sto:standard rdf:type owl:Class .


###  https://w3id.org/i40/sto#xRoadSection
sto:xRoadSection rdf:type owl:Class ;
                 rdfs:subClassOf sto:StandardClassification ,
                                 [ rdf:type owl:Restriction ;
                                   owl:onProperty sto:isDescribedin ;
                                   owl:hasValue sto:xTee
                                 ] .


###  https://w3id.org/i40/sto/iot#Concern
sto_iot:Concern rdf:type owl:Class .


###  https://w3id.org/i40/sto/iot#StakeholderGroup
sto_iot:StakeholderGroup rdf:type owl:Class ;
                         rdfs:comment "A Stakeholder Group is a party of people who have common interests and concerns."@en ,
                                      "A stakeholder is everyone with an interest in a system."@en ,
                                      "This class contains types of stakeholders who share a common interest or task."@en ;
                         rdfs:label "Stakeholder Group"@en ;
                         skos:note "Stakeholders are interpreted in the same manner as outlined by ISO 42010: '<system> individual, team, organization, or classes thereof, having an interest in a system'"@en ,
                                   "Subclass of http://voag.linkedmodel.org/voag#StakeholderGroup (vocabulary not accessible)." .


###  https://w3id.org/i40/sto/iot#hasStakeholder
sto_iot:hasStakeholder rdf:type owl:Class .


###  https://www.w3.org/ns/oaAnnotation
oa:Annotation rdf:type owl:Class .


###  https://www.w3.org/ns/oaRangeSelector
oa:RangeSelector rdf:type owl:Class .


###  https://www.w3.org/ns/oaSpecificResource
oa:SpecificResource rdf:type owl:Class .


###  https://www.w3.org/ns/oaXPathSelector
oa:XPathSelector rdf:type owl:Class .


#################################################################
#    Individuals
#################################################################

###  http://data.semanticweb.org/person/steffen-lohmann
<http://data.semanticweb.org/person/steffen-lohmann> rdf:type owl:NamedIndividual ,
                                                              foaf:Person .


###  http://dbpedia.org/resource#Beijing
dbr:Beijing rdf:type owl:NamedIndividual ,
                     dbo:Place ;
            rdfs:comment "Refers to a place called Beijing."@en ;
            rdfs:label "Beijing"@en .


###  http://dbpedia.org/resource#Berlin
dbr:Berlin rdf:type owl:NamedIndividual ,
                    dbo:Place ;
           rdfs:comment "Refers to a place called Berlin."@en ;
           rdfs:label "Berlin"@en .


###  http://dbpedia.org/resource#Boston
dbr:Boston rdf:type owl:NamedIndividual ,
                    dbo:Place ;
           rdfs:comment "Refers to a place called Boston."@en ;
           rdfs:label "Boston"@en .


###  http://dbpedia.org/resource#Chicago
dbr:Chicago rdf:type owl:NamedIndividual ,
                     dbo:Place ;
            rdfs:comment "Refers to a place called Chicago."@en ;
            rdfs:label "Chicago"@en .


###  http://dbpedia.org/resource#China
dbr:China rdf:type owl:NamedIndividual ,
                   dbo:Country ;
          rdfs:comment "Refers to a Country called China."@en ;
          rdfs:label "China"@en .


###  http://dbpedia.org/resource#Cologne
dbr:Cologne rdf:type owl:NamedIndividual ,
                     dbo:Place ;
            rdfs:comment "Refers to a place called Cologne."@en ;
            rdfs:label "Cologne"@en .


###  http://dbpedia.org/resource#Eumseong
dbr:Eumseong rdf:type owl:NamedIndividual ,
                      dbo:Place ;
             rdfs:comment "Refers to a place called Eumseong."@en ;
             rdfs:label "Eumseong"@en .


###  http://dbpedia.org/resource#Frankfurt
dbr:Frankfurt rdf:type owl:NamedIndividual ,
                       dbo:Place ;
              rdfs:comment "Refers to a place called Frankfurt."@en ;
              rdfs:label "Frankfurt"@en .


###  http://dbpedia.org/resource#Geneva
dbr:Geneva rdf:type owl:NamedIndividual ,
                    dbo:Place ;
           rdfs:comment "Refers to a place called Geneva."@en ;
           rdfs:label "Geneva"@en .


###  http://dbpedia.org/resource#Germany
dbr:Germany rdf:type owl:NamedIndividual ,
                     dbo:Country ;
            rdfs:comment "Refers to a Country called Germany."@en ;
            rdfs:label "Germany"@en .


###  http://dbpedia.org/resource#Hoehenkirchen-Siegertsbrunn
dbr:Hoehenkirchen-Siegertsbrunn rdf:type owl:NamedIndividual ,
                                         dbo:Place ;
                                rdfs:comment "Refers to a place called Berlin."@en ;
                                rdfs:label "Berlin"@en .


###  http://dbpedia.org/resource#Hoehenkirchen_Siegertsbrunn
dbr:Hoehenkirchen_Siegertsbrunn rdf:type owl:NamedIndividual ,
                                         dbo:Place ;
                                rdfs:comment "Refers to a place called Hoehenkirchen-Siegertsbrunn."@en ;
                                rdfs:label "Hoehenkirchen-Siegertsbrunn"@en .


###  http://dbpedia.org/resource#New_York_City
dbr:New_York_City rdf:type owl:NamedIndividual ,
                           dbo:Place ;
                  rdfs:comment "Refers to a place called New York City."@en ;
                  rdfs:label "New_York_City"@en .


###  http://dbpedia.org/resource#Paris
dbr:Paris rdf:type owl:NamedIndividual ,
                   dbo:Place ;
          rdfs:comment "Refers to a place called Paris."@en ;
          rdfs:label "Paris"@en .


###  http://dbpedia.org/resource#South_Korea
dbr:South_Korea rdf:type owl:NamedIndividual ,
                         dbo:Country ;
                rdfs:comment "Refers to a Country called South Korea."@en ;
                rdfs:label "South Korea"@en .


###  http://dbpedia.org/resource#Switzerland
dbr:Switzerland rdf:type owl:NamedIndividual ,
                         dbo:Country ;
                rdfs:comment "Refers to a Country called Switzerland."@en ;
                rdfs:label "Switzerland"@en .


###  http://dbpedia.org/resource#United_States
dbr:United_States rdf:type owl:NamedIndividual ,
                           dbo:Country ;
                  rdfs:comment "Refers to a Country called United_States."@en ;
                  rdfs:label "United States"@en .


###  http://dbpedia.org/resource#Valbonne
dbr:Valbonne rdf:type owl:NamedIndividual ,
                      dbo:Place ;
             rdfs:comment "Refers to a place called Valbonne."@en ;
             rdfs:label "Valbonne"@en .


###  http://dbpedia.org/resource#_Arizona
dbr:_Arizona rdf:type owl:NamedIndividual ,
                      dbo:Place ;
             rdfs:comment "Refers to a place called Arizona."@en ;
             rdfs:label "Arizona"@en .


###  http://dbpedia.org/resource#_California
dbr:_California rdf:type owl:NamedIndividual ,
                         dbo:Place ;
                rdfs:comment "Refers to a place called California."@en ;
                rdfs:label "_California"@en .


###  http://dbpedia.org/resource#_Georgia
dbr:_Georgia rdf:type owl:NamedIndividual ,
                      dbo:Place ;
             rdfs:comment "Refers to a place called Georgia."@en ;
             rdfs:label "Georgia"@en .


###  http://dbpedia.org/resource#_Maryland
dbr:_Maryland rdf:type owl:NamedIndividual ,
                       dbo:Place ;
              rdfs:comment "Refers to a place called Maryland."@en ;
              rdfs:label "Maryland"@en .


###  http://dbpedia.org/resource#_Massachusetts
dbr:_Massachusetts rdf:type owl:NamedIndividual ,
                            dbo:Place ;
                   rdfs:comment "Refers to a place called Massachusetts."@en ;
                   rdfs:label "Massachusetts"@en .


###  http://dbpedia.org/resource#_Michigan
dbr:_Michigan rdf:type owl:NamedIndividual ,
                       dbo:Place ;
              rdfs:comment "Refers to a place called Michigan."@en ;
              rdfs:label "Michigan"@en .


###  http://dbpedia.org/resource#_New_York
dbr:_New_York rdf:type owl:NamedIndividual ,
                       dbo:Place ;
              rdfs:comment "Refers to a place called New York."@en ;
              rdfs:label "New York"@en .


###  http://dbpedia.org/resource#_North_Carolina
dbr:_North_Carolina rdf:type owl:NamedIndividual ,
                             dbo:Place ;
                    rdfs:comment "Refers to a place called North Carolina."@en ;
                    rdfs:label "North Carolina"@en .


###  http://dbpedia.org/resource#_Texas
dbr:_Texas rdf:type owl:NamedIndividual ,
                    dbo:Place ;
           rdfs:comment "Refers to a place called Texas."@en ;
           rdfs:label "_Texas"@en .


###  http://dbpedia.org/resource#Washington,_D.C.
<http://dbpedia.org/resource#Washington,_D.C.> rdf:type owl:NamedIndividual ,
                                                        dbo:Place ;
                                               rdfs:comment "Refers to a place called Washington D.C."@en ;
                                               rdfs:label "Washington D.C"@en .


###  http://http://sda.cs.uni-bonn.de/people/irlan-grangel-gonzalez/
<http://http://sda.cs.uni-bonn.de/people/irlan-grangel-gonzalez/> rdf:type owl:NamedIndividual .


###  http://lexvo.org/id/iso639-3/deu
lang:deu rdf:type owl:NamedIndividual ,
                  dcterms:LinguisticSystem ;
         rdfs:label "Deu"@en .


###  http://lexvo.org/id/iso639-3/eng
lang:eng rdf:type owl:NamedIndividual ,
                  dcterms:LinguisticSystem .


###  http://lexvo.org/id/iso639-3/fra
lang:fra rdf:type owl:NamedIndividual ,
                  dcterms:LinguisticSystem .


###  http://lexvo.org/id/iso639-3/rus
lang:rus rdf:type owl:NamedIndividual ,
                  dcterms:LinguisticSystem .


###  http://lexvo.org/id/iso639-3/spa
lang:spa rdf:type owl:NamedIndividual ,
                  dcterms:LinguisticSystem .


###  http://purl.oclc.org/NET/mvco.owl#EndUser
<http://purl.oclc.org/NET/mvco.owl#EndUser> rdf:type owl:NamedIndividual ,
                                                     sto_iot:StakeholderGroup .


###  http://www.ontology-of-units-of-measure.org/resource/om-2/kilobyte
om2:kilobyte rdf:type owl:NamedIndividual ,
                      om2:Unit .


###  https://doi.org/10.1016/j.compind.2018.04.015
<https://doi.org/10.1016/j.compind.2018.04.015> rdf:type owl:NamedIndividual ,
                                                         sto:Publication ;
                                                rdfs:label "The industrial internet of things (IIoT): An analysis framework"@en .


###  https://doi.org/10.1016/j.jksuci.2016.10.003
<https://doi.org/10.1016/j.jksuci.2016.10.003> rdf:type owl:NamedIndividual ,
                                                        sto:Publication ;
                                               dc:title "A survey on Internet of Things architectures"@en ;
                                               rdfs:label "A survey on Internet of Things architectures"@en .


###  https://w3id.org/i40/sto#AdminShellGeneral
sto:AdminShellGeneral rdf:type owl:NamedIndividual ,
                                sto:RamiAdminShellSubmodel ,
                                sto:StandardClassification ;
                       sto:isDescribedin sto:AdministrationShell .


###  https://w3id.org/i40/sto#AsConditionMonitoring
sto:AsConditionMonitoring rdf:type owl:NamedIndividual ,
                                  sto:RamiAdminShellSubmodel ,
                                  sto:StandardClassification ;
                         sto:isDescribedin sto:AdministrationShell .


###  https://w3id.org/i40/sto#AsConfiguration
sto:AsConfiguration rdf:type owl:NamedIndividual ,
                           sto:RamiAdminShellSubmodel ,
                            sto:StandardClassification ;
                   sto:isDescribedin sto:AdministrationShell ;
                   skos:note "Publications referred: '<https://doi.org/10.1016/j.jksuci.2016.10.003>' '2.2.2. Middleware enablement' 'Page 300'"@en .


###  https://w3id.org/i40/sto#AsEngineering
sto:AsEngineering rdf:type owl:NamedIndividual ,
                          sto:RamiAdminShellSubmodel ,
                          sto:StandardClassification ;
                 dul:associatedWith sto:IviActivityLayer ,
                                    sto:IviActivityView ,
                                    sto:IviSpecificationLayer ;
                 sto:isDescribedin sto:AdministrationShell ;
                 sto:alignsWith sto:IviActivityLayer ,
                                sto:IviActivityView ,
                                sto:IviSpecificationLayer .



###  https://w3id.org/i40/sto#AsIdentification
sto:AsIdentification rdf:type owl:NamedIndividual ,
                             sto:RamiAdminShellSubmodel ,
                             sto:StandardClassification ;
                    sto_iot:frames sto:IdentityManagement;
                    dul:associatedWith sto:AsIdentification ;
                    sto:alignsWith sto:AsIdentification ;
                    sto:isDescribedin sto:AdministrationShell ;
                    rdfs:label "RAMI Identification"@en .



###  https://w3id.org/i40/sto#RamiInstanceMaintenance
sto:RamiInstanceMaintenance rdf:type owl:NamedIndividual ,
                                  sto:RamiLifeCycleLayer ,
                                  sto:StandardClassification ;
                         sto:isDescribedin sto:Rami;
                         rdfs:label "Instance Maintenance"@en .


###  https://w3id.org/i40/sto#RamiInstanceProduction
sto:RamiInstanceProduction rdf:type owl:NamedIndividual ,
                                 sto:RamiLifeCycleLayer ,
                                 sto:StandardClassification ;
                        sto:isDescribedin sto:Rami;
                        rdfs:label "Instance Production"@en .



###  https://w3id.org/i40/sto#AsLifecycle_Status
sto:AsLifecycle_Status rdf:type owl:NamedIndividual ,
                               sto:RamiAdminShellSubmodel ,
                               sto:StandardClassification ;
                      sto:isDescribedin sto:AdministrationShell ;
                      rdfs:label "Lifecycle Status"@en .



###  https://w3id.org/i40/sto#AsProcessPlanning
sto:AsProcessPlanning rdf:type owl:NamedIndividual ,
                              sto:RamiAdminShellSubmodel ,
                              sto:StandardClassification ;
                     sto:isDescribedin sto:AdministrationShell ;
                     rdfs:comment "Process planning frames everything related to model, plan and manage business workflows and processes."@en ;
                     rdfs:label "Process planning"@en .



###  https://w3id.org/i40/sto#AsSafety
sto:AsSafety rdf:type owl:NamedIndividual ,
                     sto:RamiAdminShellSubmodel ,
                     sto:StandardClassification ;
            sto:isDescribedin sto:AdministrationShell ;
            rdfs:label "RAMI Safety"@en .


###  https://w3id.org/i40/sto#AsSecurity
sto:AsSecurity rdf:type owl:NamedIndividual ,
                       sto:RamiAdminShellSubmodel ,
                       sto:StandardClassification ;
              dul:associatedWith sto:BdvaCyberSecurityTrust ,
                                 sto:DtpSecurityPrivacy ,
                                 sto:FiwareSecurity ;
              sto:isDescribedin sto:AdministrationShell ;
              rdfs:label "RAMI Security"@en ;
              sto:alignsWith sto:BdvaCyberSecurityTrust ,
                             sto:DtpSecurityPrivacy ,
                             sto:FiwareSecurity ,
                             sto:OcfSecurity .


###  https://w3id.org/i40/rami#Station
sto:RamiStation rdf:type owl:NamedIndividual ,
                       sto:StandardClassification ;
              rdfs:label "RAMI Station"@en ;
              dcterms:creator sto:sebastian ;
              sto:isDescribedin sto:AdministrationShell ;
.


###  https://w3id.org/i40/sto#RamiTypeDevelopment
sto:RamiTypeDevelopment rdf:type owl:NamedIndividual ,
                              sto:RamiLifeCycleLayer ,
                              sto:StandardClassification ;
                     dul:associatedWith sto:IviSpecificationLayer ;
                     sto:alignsWith sto:IviSpecificationLayer ;
                     sto:isDescribedin sto:Rami;
                     rdfs:label "Type Development"@en .


###  https://w3id.org/i40/sto#RamiTypeMaintenance
sto:RamiTypeMaintenance rdf:type owl:NamedIndividual ,
                              sto:StandardClassification ;
                              sto:isDescribedin sto:Rami;
                     rdfs:label "Type Maintenance"@en .


###  https://w3id.org/i40/sto#RamiWorkCenter
sto:RamiWorkCenter rdf:type owl:NamedIndividual ,
                       sto:StandardClassification ;
              rdfs:label "RAMI Work Center"@en ;
              dcterms:creator sto:sebastian ;
              sto:isDescribedin sto:AdministrationShell ;
.

###  https://w3id.org/i40/sto#AI
sto:AI rdf:type owl:NamedIndividual ,
                sto_iot:Concern ;
       dcterms:creator sto:sebastian ;
       sto_iot:supports sto:DataAnalytics ;
       rdfs:comment "Artificial intelligence (AI) is intelligence exhibited by machines. In computer science, an ideal \"intelligent\" machine is a flexible rational agent that perceives its environment and takes actions that maximize its chance of success at some goal. Colloquially, the term \"artificial intelligence\" is applied when a machine mimics \"cognitive\" functions that humans associate with other human minds, such as \"learning\" and \"problem solving\". (source: wikipedia)"@en ;
       rdfs:label "Artificial Intelligence"@en ;
       sto:hasDBpediaResource <http://dbpedia.org/resource/Artificial_intelligence> ,
                              ""@en .


###  https://w3id.org/i40/sto#AMQP
sto:AMQP rdf:type owl:NamedIndividual ,
                  foaf:Document ,
                  sto:Publication ,
                  sto:TechnicalSpecification ;
         dcterms:creator sto:sebastian ;
         rdfs:comment "AMQP (Advanced Message Queuing Protocol): An open standard application layer protocol for message-oriented middleware. The defining features of AMQP are message orientation, queuing, routing (including point-to-point and publish-and-subscribe), reliability and security. (source: https://www.postscapes.com/internet-of-things-protocols/)"@en ;
         rdfs:label "AMQP"@en ;
         sto:hasOfficialResource <http://www.amqp.org/> .


###  https://w3id.org/i40/sto#ANSI
sto:ANSI rdf:type owl:NamedIndividual ,
                  sto:StandardOrganization ;
         sto:hasHeadquaterIn <http://dbpedia.org/resource#Washington,_D.C.> ;
         sto:abbreviation "ANSI"@en ;
         sto:formationDate "1918-05-14"^^xsd:date ;
         sto:orgName "American National Standards Institute"@en ;
         rdfs:comment "The American National Standards Institute is a private non-profit organization that oversees the development of voluntary consensus standards for products, services, processes, systems, and personnel in the United States. The organization also coordinates U.S. standards with international standards so that American products can be used worldwide. ANSI accredits standards that are developed by representatives of other standards organizations, government agencies, consumer groups, companies, and others. These standards ensure that the characteristics and performance of products are consistent, that people use the same definitions and terms, and that products are tested the same way. ANSI also accredits organizations that carry out product or personnel certification in accordance with requirements defined in international standards."@en ;
         rdfs:label "ANSI"@en ;
         sto:hasDBpediaResource <http://dbpedia.org/resource/American_National_Standards_Institute> ;
         sto:hasOfficialResource <https://www.ansi.org/> ;
         sto:hasWikipediaArticle <https://en.wikipedia.org/wiki/American_National_Standards_Institute?oldformat=true> .


###  https://w3id.org/i40/sto#ANT
sto:ANT rdf:type owl:NamedIndividual ,
                 sto:TechnicalSpecification ;
        dcterms:creator sto:sebastian ;
        rdfs:comment "ANT is a proprietary wireless sensor network technology featuring a wireless communications protocol stack that enables semiconductor radios operating in the 2.4 GHz Industrial, Scientific and Medical allocation of the RF spectrum (ISM band) to communicate by establishing standard rules for co-existence, data representation, signalling, authentication and error detection.  (source: https://www.postscapes.com/internet-of-things-protocols/)"@en ;
        rdfs:label "ANT"@en ;
        sto:hasWikipediaArticle <https://en.wikipedia.org/wiki/ANT_(network)> .


###  https://w3id.org/i40/sto#APICS
sto:APICS rdf:type owl:NamedIndividual ,
                   sto:StandardOrganization ;
          sto:hasHeadquaterIn dbr:Chicago ;
          sto:formationDate "1957-01-01"^^xsd:date ;
          sto:orgName "American Production and Inventory Control Society"@en ;
          rdfs:comment "American Production and Inventory Control Society."@en ;
          rdfs:label "APICS"@en ;
          sto:hasDBpediaResource <http://dbpedia.org/page/APICS> ;
          sto:hasOfficialResource <http://www.apics.org/apics> ;
          sto:hasWikipediaArticle <https://en.wikipedia.org/wiki/APICS> .


###  https://w3id.org/i40/sto#AsAM
sto:AsAM rdf:type owl:NamedIndividual ,
                  sto:StandardOrganization ;
         sto:belongsTo dbr:Germany ;
         sto:hasHeadquaterIn dbr:Hoehenkirchen_Siegertsbrunn ;
         sto:abbreviation "ASAM"^^xsd:string ;
         sto:formationDate "1998-12-01"^^xsd:date ;
         sto:orgName "Association for Standardization of Automation and Measuring Systems"@en ;
         rdfs:comment "Association for Standardization of Automation and Measuring Systems or ASAM is an incorporated association under German law. Its members are primarily international car manufacturers, suppliers and engineering service providers from the automotive industry. The association coordinates the development of technical standards, which are developed by working groups composed of experts from its member companies. ASAM pursues the vision that the tools of a development process chain can be freely interconnected and allow a seamless exchange of data. The standards define protocols, data models, file formats and application programming interfaces (APIs) for the use in the development and testing of automotive electronic control units. A large amount of popular tools in the areas of simulation, measurement, calibration and test automation are compliant to ASAM standards. Compliance shall guarantee interoperability of tools from different vendors, allow data exchange without the need for converters, and facilitate the exchange of unambiguous specification between customers and suppliers."@en ;
         rdfs:label "ASAM"^^xsd:string ;
         sto:hasDBpediaResource <http://dbpedia.org/page/Association_for_Standardisation_of_Automation_and_Measuring_Systems> ;
         sto:hasOfficialResource <https://www.asam.net/> ;
         sto:hasWikipediaArticle <https://en.wikipedia.org/wiki/Association_for_Standardisation_of_Automation_and_Measuring_Systems> .


###  https://w3id.org/i40/sto#AsAM_ODS
sto:AsAM_ODS rdf:type owl:NamedIndividual ,
                      sto:Standard ;
             dcterms:creator sto:irlan ;
             sto:hasPublisher sto:AsAM ;
             rdfs:comment "Set up a test data management system on top of test systems that produce measured or calculated data from testing activities"@en ;
             rdfs:label "ASAM ODS"@en ;
             sto:hasOfficialResource <https://wiki.asam.net/display/STANDARDS/ASAM+ODS> .


###  https://w3id.org/i40/sto#AsME
sto:AsME rdf:type owl:NamedIndividual ,
                  sto:StandardOrganization ;
         sto:hasHeadquaterIn dbr:New_York_City ;
         sto:abbreviation "ASME"^^xsd:string ;
         sto:formationDate "1880-01-01"^^xsd:date ;
         sto:orgName "American Society of Mechanical Engineers"@en ;
         rdfs:comment "The American Society of Mechanical Engineers (ASME) is a professional association that, promotes the art, science, and practice of multidisciplinary engineering and allied sciences around the globe via continuing education, training and professional development, codes and standards, research, conferences and publications, government relations, and other forms of outreach."@en ;
         sto:hasDBpediaResource <http://dbpedia.org/resource/ASME> ;
         sto:hasOfficialResource <https://www.asme.org/> ;
         sto:hasWikipediaArticle <https://en.wikipedia.org/wiki/ASME> .


###  https://w3id.org/i40/sto#AsME_Y1441
sto:AsME_Y1441 rdf:type owl:NamedIndividual ,
                        sto:Standard ;
               dcterms:creator sto:irlan ;
               foaf:maker sto:AsME ;
               sto:hasClassification sto:ModelingPractice ;
               sto:hasPublisher sto:AsME ;
               rdfs:comment "ASME Y14.41 establishs requirements for model-based definition upon CAD software and those who use CAD software to create product definition within the 3D model."@en ;
               rdfs:label "ASME Y14.41"@en ;
               sto:hasDBpediaResource <http://dbpedia.org/resource/ASME_Y14.41> ;
               sto:hasOfficialResource <https://www.asme.org/products/codes-standards/y1441-2012-digital-product-definition-data> ;
               sto:hasWikipediaArticle <https://en.wikipedia.org/wiki/ASME_Y14.41> .


###  https://w3id.org/i40/sto#AdministrationShell
sto:AdministrationShell rdf:type owl:NamedIndividual ,
                                 sto:StandardizationFramework ;
                        sto:hasPublisher sto:PlatformIndustry40 ;
                        rdfs:comment "Represents the classifications of the standards according to the submodels of the administration shell."@en ;
                        rdfs:label "Administration Shell"@en .


###  https://w3id.org/i40/sto#Automation
sto:Automation rdf:type owl:NamedIndividual ,
                        sto:RelevantDomain ;
               rdfs:comment "Technology with which a process or procedure is performed with minimal human intervention "@en ;
               rdfs:label "Automation"@en ;
               sto:hasWikipediaArticle <https://en.wikipedia.org/wiki/Automation> .


###  https://w3id.org/i40/sto#B2MML
sto:B2MML rdf:type owl:NamedIndividual ,
                   sto:Standard ;
          dcterms:creator sto:irlan ;
          sto:hasClassification sto:NISTBusinessProcessExecution ,
                                sto:EnterpriseLevel ;
          sto:hasDeveloper sto:MESA ;
          sto:hasPublisher sto:MESA ;
          sto:isImplementationOf sto:ISA-95 ;
          sto:relatedTo sto:B2MML ,
                        sto:IEC_62264 ,
                        sto:ISA-95 ;
          rdfs:comment "B2MML or Business To Manufacturing Markup Language is an XML implementation of the ANSI/ISA-95 family of standards (ISA-95)"@en ;
          rdfs:label "Business To Manufacturing Markup Language"@en ;
          skos:altLabel "IEC 62264"@en ;
          sto:hasDBpediaResource <http://dbpedia.org/resource/B2MML> ;
          sto:hasOfficialResource <https://services.mesa.org/ResourceLibrary/ShowResource/0f47758b-60f0-40c6-a71b-fa7b2363fb3a> ;
          sto:hasWikipediaArticle <https://en.wikipedia.org/wiki/B2MML> .


###  https://w3id.org/i40/sto#BBF
sto:BBF rdf:type owl:NamedIndividual ,
                 sto:StandardOrganization ;
        sto:hasHeadquaterIn dbr:_California ;
        sto:abbreviation "BBF"^^xsd:string ;
        sto:formationDate "2008-01-01"^^xsd:date ;
        sto:orgName "Broadband Forum"@en ;
        rdfs:comment "The Broadband Forum is a non-profit industry consortium dedicated to developing broadband network specifications. Members include telecommunications networking and service provider companies, broadband device and equipment vendors, consultants and independent testing labs (ITLs). Service provider members are primarily wire-line service providers (non-mobile) telephone companies."@en ;
        rdfs:label "Broadband Forum"@en ;
        sto:hasDBpediaResource <http://dbpedia.org/resource/Broadband_Forum> ;
        sto:hasOfficialResource <https://www.broadband-forum.org/> ;
        sto:hasWikipediaArticle <https://en.wikipedia.org/wiki/Broadband_Forum> .


###  https://w3id.org/i40/sto#BBF_TR-069
sto:BBF_TR-069 rdf:type owl:NamedIndividual ,
                        sto:Standard ;
               dcterms:creator sto:irlan ;
               sto:hasDeveloper sto:BBF ;
               sto:hasPublisher sto:BBF ;
               sto:hasTag "CPE WAN Management Protocol"@en ;
               rdfs:comment "Digital Enhanced Cordless Telecommunications (DECT) is the ETSI standard for short-range cordless communications, which can be adapted for many applications and can be used over unlicensed frequency allocations world-wide."@en ;
               rdfs:label "BBF TR-069"@en ;
               sto:hasDBpediaResource <http://dbpedia.org/resource/TR-069> ;
               sto:hasOfficialResource <https://www.broadband-forum.org/standards-and-software/technical-specifications/tr-069-files-tools> ;
               sto:hasWikipediaArticle <https://en.wikipedia.org/wiki/TR-069> .


###  https://w3id.org/i40/sto#BDI
sto:BDI rdf:type owl:NamedIndividual ,
                 sto:StandardOrganization ;
        dcterms:creator sto:sebastian ;
        dcterms:title "The Federation of German Industries"@en ;
        rdfs:comment "The Federation of German Industries represents a large proportion of the German manufacturing industry."@en ;
        sto:hasOfficialResource <https://english.bdi.eu/> .


###  https://w3id.org/i40/sto#BDVA
sto:BDVA rdf:type owl:NamedIndividual ,
                  foaf:Organization ;
         rdfs:label "Big Data Value Association" ;
         skos:altLabel "BDVA" .


###  https://w3id.org/i40/sto#BPEL
sto:BPEL rdf:type owl:NamedIndividual ,
                  sto:Standard ;
         dcterms:creator sto:irlan ;
         sto:hasClassification sto:NISTBusinessProcessExecution ;
         sto:hasPublisher sto:OASIS ;
         sto:hasTag "BPEL"@en ;
         rdfs:comment "The Web Services Business Process Execution Language (WS-BPEL), commonly known as BPEL Business Process Execution Language, is a standard executable language for specifying actions within business processes with web services."@en ;
         rdfs:label "Business Process Execution Language"@en ;
         sto:hasDBpediaResource <http://dbpedia.org/resource/Business_Process_Execution_Language> ;
         sto:hasOfficialResource <https://www.oasis-open.org/committees/tc_home.php?wg_abbrev=wsbpel> ;
         sto:hasWikipediaArticle <https://en.wikipedia.org/wiki/Business_Process_Execution_Language> .


###  https://w3id.org/i40/sto#BPMN
sto:BPMN rdf:type owl:NamedIndividual ,
                  sto:TechnicalSpecification ;
         dcterms:creator sto:irlan ;
         sto:hasClassification sto:SCM ;
         sto:hasDeveloper sto:OMG ;
         sto:hasTag "BPMN"@en ;
         rdfs:comment "Business Process Model and Notation is a graphical representation for specifying business processes in a business process model."@en ;
         rdfs:label "Business Process Model Notation"@en ;
         sto:hasDBpediaResource <http://dbpedia.org/page/Business_Process_Model_and_Notation> ;
         sto:hasOfficialResource <http://www.bpmn.org/> ;
         sto:hasWikipediaArticle <https://en.wikipedia.org/wiki/Business_Process_Model_and_Notation> .


###  https://w3id.org/i40/sto#BusinessProcessExecution
sto:NISTBusinessProcessExecution rdf:type owl:NamedIndividual ,
                                      sto:BusinessCycleSCM ,
                                      sto:StandardClassification ;
                             sto:isDescribedin sto:NISTInitiative ;
                             rdfs:comment "Describes Business Process Execution concept."@en ;
                             rdfs:label "Business Process Execution"@en .


###  https://w3id.org/i40/sto#CAD
sto:CAD rdf:type owl:NamedIndividual ,
                 sto:RelevantDomain;
        sto:domainName "Computer-Aided Design"@en ;
        rdfs:comment "Computer-Aided Design"@en ;
        rdfs:isDefinedBy <https://en.wikipedia.org/wiki/Computer-aided_design> ;
        rdfs:label "CAD"@en ;
        sto:hasDBpediaResource <http://dbpedia.org/resource/Computer-aided_design> .


###  https://w3id.org/i40/sto#CASAGRAS
sto:CASAGRAS rdf:type owl:NamedIndividual ,
                      sto:IIoTConsortium ;
             dcterms:creator sto:sebastian ;
             rdfs:comment "A key group of international partners representing Europe, the USA, China, Japan and Korea who has joined a strategic EU funded 7th Framework initiative that will look at global standards, regulatory and other issues concerning RFID and its role in realising an Internet of Things.  (source: https://www.postscapes.com/internet-of-things-protocols/)"@en ;
             rdfs:label "CASAGRAS"@en ;
             sto:hasOfficialResource <http://www.iot-casagras.org/page/standards-and-regulations> .


###  https://w3id.org/i40/sto#Enterprise_Control
sto:Enterprise_Control
   a owl:NamedIndividual ;
   a sto:RelevantDomain;
rdfs:label "Enterprise Control"@en;   
sto:domainName "Enterprise Control"@en ;
rdfs:comment "Enterprise Control Domain"@en .


###  https://w3id.org/i40/sto#CCN
sto:CCN rdf:type owl:NamedIndividual ,
                 sto:TechnicalSpecification ;
        dcterms:creator sto:sebastian ;
        rdfs:comment "Content-Centric Networking (CCN). Next-gen network architecture to solve challenges in content distribution scalability, mobility, and security. CCN directly routes and delivers named pieces of content at the packet level of the network, enabling automatic and application-neutral caching in memory wherever it’s located in the network. The result? Efficient and effective delivery of content wherever and whenever it is needed. Since the architecture enables these caching effects as an automatic side effect of packet delivery, memory can be used without building expensive application-level caching services. (source: https://www.postscapes.com/internet-of-things-protocols/)"@en ;
        rdfs:label "CCN"@en ;
        sto:hasOfficialResource <http://www.ccnx.org/> .


###  https://w3id.org/i40/sto#CGMES
sto:CGMES rdf:type owl:NamedIndividual ,
                   sto:RelevantDomain ;
          rdfs:comment "Specification for Energy Management"@en ;
          rdfs:label "CGMES: Common Grid Model Exchange Specification"@en ;
          sto:hasOpenResource <https://docstore.entsoe.eu/Documents/CIM_documents/IOP/CGMES_2_5_TechnicalSpecification_61970-600_Part%201_Ed2.pdf> ;
          sto:seeAlso <https://docstore.entsoe.eu/major-projects/common-information-model-cim/cim-for-grid-models-exchange/standards/Pages/default.aspx> .


###  https://w3id.org/i40/sto#CrossLevel
sto:ISA95CrossLevel rdf:type owl:NamedIndividual ,
                        sto:ISA95Level ,
                        sto:StandardClassification ;
               sto:isDescribedin sto:ISA95 ;
               rdfs:comment "Describes the cross-level according to the ISA95 level classification. It means standards that are used at more than one level, e.g., manufacturing system security, etc"@en ;
               rdfs:label "Cross Level"@en .


###  https://w3id.org/i40/sto#CyberSecurity
sto:CyberSecurity rdf:type owl:NamedIndividual ,
                           sto:RelevantDomain ;
                  rdfs:comment "Protection of Computer Systems from damage of all kinds "@en ;
                  rdfs:label "Cyber Security"@en ;
                  sto:hasWikipediaArticle <https://en.wikipedia.org/wiki/Computer_security> .


###  https://w3id.org/i40/sto#DDS
sto:DDS rdf:type owl:NamedIndividual ,
                 sto:TechnicalSpecification ;
        dcterms:creator sto:sebastian ;
        rdfs:comment "DDS (Data-Distribution Service for Real-Time Systems): The first open international middleware standard directly addressing publish-subscribe communications for real-time and embedded systems. (source: https://www.postscapes.com/internet-of-things-protocols/)"@en ;
        rdfs:label "DDS"@en ;
        sto:hasOfficialResource <http://portals.omg.org/dds/> .


###  https://w3id.org/i40/sto#DIN
sto:DIN rdf:type owl:NamedIndividual ,
                 sto:StandardOrganization ;
        sto:belongsTo dbr:Germany ;
        sto:hasHeadquaterIn dbr:Berlin ;
        sto:abbreviation "DIN"@de ;
        sto:formationDate "1918-01-01"^^xsd:date ;
        sto:orgName "Deutsches Institut für Normung"@en ;
        rdfs:comment "Deutsches Institut für Normung e.V. (DIN; in English, the German Institute for Standardization) is the German national organization for standardization and is the German ISO member body. DIN is a German Registered Association (e.V.) headquartered in Berlin. There are currently around thirty thousand DIN Standards, covering nearly every field of technology"@en ;
        rdfs:label "DIN"@en ,
                   "Deutsches Institut für Normung"@de ,
                   "German Institute for Standardization"@en ;
        sto:hasDBpediaResource <http://dbpedia.org/page/Deutsches_Institut_f%C3%BCr_Normung> ;
        sto:hasOfficialResource <http://www.din.de/en/about-standards/din-standards> ;
        sto:hasWikipediaArticle <https://en.wikipedia.org/wiki/Deutsches_Institut_f%C3%BCr_Normung> .



###  https://w3id.org/i40/sto#DIN_77005_P1
sto:DIN_77005_P1 rdf:type owl:NamedIndividual ,
                          sto:Standard ;
                 dcterms:creator sto:irlan ;
                 sto:hasAvailableLanguage lang:deu ;
                 sto:hasPublisher sto:DIN ;
                 sto:hasAvailableLanguage lang:deu;
                 sto_iot:hasTargetConcern sto:DataLifecycleManagment ;
                 sto:hasPublicationDate "2018-09-01"^^xsd:date ;
                 sto:hasTag "DIN 77005-1:2018-09"^^xsd:string ;
                 rdfs:comment "Lifecycle record of technical objects - Part 1: Structural and content-related specifications"@en ;
                 rdfs:label "DIN 77005-1:2018-09"@en ;
                 sto:hasOfficialResource <https://www.beuth.de/en/standard/din-77005-1/290281150> .


###  https://w3id.org/i40/sto#DIN_EN_50128
sto:DIN_EN_50128 rdf:type owl:NamedIndividual ,
                          sto:Standard ;
                 dcterms:creator sto:irlan ,
                                 sto:sebastian ;
                 sto:hasAvailableLanguage lang:deu ;
                 sto:hasClassification sto:IDSRAMCertification ;
                 sto:hasPublisher sto:DIN ;
                 sto_iot:hasTargetConcern sto:Safety ;
                 sto:hasAvailableLanguage lang:deu;
                 sto:hasPublicationDate "2012-03-01"^^xsd:date ;
                 rdfs:comment "Die EN 50128 ist eine Europäische Norm für sicherheitsrelevante Software der Eisenbahn, sowohl strecken- als auch zugseitig. Zusammen mit der EN 50129 für die Hardware und den Zulassungsprozessen ist die EN 50128 eine Spezialisierung der EN 61508. Die EN 50128 ist eine Prozessnorm. Sie stellt dar, welche Verfahren, Prinzipien und Maßnahmen anzuwenden sind, damit die Software als sicher gilt."@de ;
                 rdfs:label "DIN EN 50128"@en ;
                 sto:hasOfficialResource <https://www.beuth.de/de/norm/din-en-50128/148018416> .


###  https://w3id.org/i40/sto#DIN_EN_50129
sto:DIN_EN_50129 rdf:type owl:NamedIndividual ,
                          sto:Standard ;
                 dcterms:creator sto:irlan ,
                                 sto:sebastian ;
                 sto:hasClassification sto:IDSRAMCertification ;
                 sto:hasPublisher sto:DIN ;
                  sto:hasClassification sto:IDSRAMCertification ;
                  sto_iot:hasTargetConcern sto:Safety;
                 dcterms:title "Railway applications - Communications, signalling and processing systems - Safety related electronic systems for signalling"@en ;
                 rdfs:comment "Für alle Eisenbahnsignalsysteme, -Teilsysteme und -Einrichtungen sind jedoch Gefährdungsanalyse und Risikobewertungsprozesse, wie in DIN EN 50126 und in dieser Norm definiert, notwendig, um die Sicherheitsanforderungen zu identifizieren."@de ,
                              "Specifies risk analysis for railway systems"@en ;
                 rdfs:label "DIN EN 50129"@en ;
                 sto:hasOfficialResource <https://www.beuth.de/de/norm/din-en-50129/67478433> ;
                 sto_iot:hasTargetConcern sto:Safety .


###  https://w3id.org/i40/sto#DIN_EN_50155
sto:DIN_EN_50155 rdf:type owl:NamedIndividual ,
                          sto:Standard ;
                 dcterms:title "Railway applications - Rolling stock - Electronic equipment"@en ;
                 rdfs:comment "Diese Norm wird bei der Konstruktion, Fertigung und Prüfung von auf Schienenfahrzeugen eingebauten elektronischen Betriebsmitteln verwendet. Sie beschreibt außerdem die elektrischen sowie die Umweltbedingungen für den Betrieb. Die Norm gilt für alle elektronischen Betriebsmittel für die Steuerung, die Regelung, den Schutz, die Diagnose, die Versorgung und so weiter, die auf Schienenfahrzeugen installiert sind. Als ein elektronisches Betriebsmittel gilt dabei ein Betriebsmittel, das hauptsächlich aus Halbleiterbauelementen und üblicherweise zugehörigen Bauelementen aufgebaut ist. Auch Sensoren (Strom, Spannung, Geschwindigkeit und so weiter) und bestückte Leiterplatten von Zündeinheiten für leistungselektronische Geräte sind von dieser Norm umfasst. Vollständige Zündeinheiten und leistungselektronische Schaltkreise sind in EN 61287-1 enthalten. Die Norm umfasst die Betriebsbedingungen, die Konstruktionsanforderungen, die Dokumentation und die Prüfung der elektronischen Betriebsmittel sowie die grundlegenden Hardware- und Softwareanforderungen, die für ein leistungsfähiges, zuverlässiges Betriebsmittel als erforderlich erachtet werden. Zuständig ist das DKE/UK 351.1 \"Fahrzeuge\" der DKE Deutsche Kommission Elektrotechnik Elektronik Informationstechnik in DIN und VDE."@de ,
                              "EN 50155:2017 is an international standard covering electronic equipment used on rolling stock for railway applications. The standard covers aspects of this electronic equipment, including temperature, humidity, shock, vibration, and other parameters. A copy of the standard may be purchased from authorised standards agencies, e.g. BSI in the UK."@en ;
                 rdfs:label "DIN EN 50155"@en ;
                 sto:hasClassification sto:IDSRAMCertification;
                 sto:hasPublisher sto:DIN ;
                 sto_iot:hasTargetConcern sto:Safety;
                 sto:hasDBpediaResource <http://dbpedia.org/resource/EN_50155> ;
                 sto:hasOfficialResource <https://www.beuth.de/de/norm/din-en-50155/275256249> ;
                 sto:hasWikipediaArticle <https://en.wikipedia.org/wiki/EN_50155> .


###  https://w3id.org/i40/sto#DIN_EN_50159
sto:DIN_EN_50159 rdf:type owl:NamedIndividual ,
                          sto:Standard ;
                 sto:hasAvailableLanguage lang:deu ;
                 sto:hasClassification sto:IDSRAMCertification ;
                 sto:hasPublicationDate "2011-04-01"^^xsd:date ;
                 dcterms:title "Railway applications - Communication, signalling and processing systems - Safety-related communication in transmission systems"@en ;
                 rdfs:comment "This European Standard is applicable for safety-relevant electronic systems which use a transmission system for digital communication purposes which has not been necessarily designed for safety-relevant applications and which - remains under the control of the designer and does not change during the life cycle, or - which is partly unknown and also does not remain constant, for which unauthorized access can be excluded, however, or - which is not under control of the designer and where unauthorized access shall also be considered. The responsible Committee is Subcommittee UK 351.3 \"Bahn-Signalanlagen\" (\"Signalling systems for railways\") of the DKE (German Commission for Electrical, Electronic and Information Technologies) at DIN and VDE."@en ;
                 rdfs:label "DIN EN 50159"@en ;
                 sto:hasPublisher sto:DIN ;
                 sto:hasAvailableLanguage lang:deu;
                 sto:hasClassification sto:IDSRAMCertification ;
                 sto_iot:hasTargetConcern sto:Safety;
                 sto:hasPublicationDate "2011-04-01"^^xsd:date;
                 sto:hasPublisher sto:DIN ;
                 sto:hasOfficialResource <https://www.beuth.de/de/norm/din-en-50159/137853742> .


###  https://w3id.org/i40/sto#DIN_EN_61511
sto:DIN_EN_61511 rdf:type owl:NamedIndividual ,
                          sto:Standard ;
                 dcterms:creator sto:irlan ,
                                 sto:sebastian ;
                 sto:hasAvailableLanguage lang:deu ;
                 sto:hasClassification sto:IDSRAMCertification ;
                 sto:hasPublisher sto:DIN ;
                 owl:sameAs sto:IEC_61511;
                 sto:hasAvailableLanguage lang:deu;
                 sto:hasPublicationDate "2019-02-01"^^xsd:date;
                 dcterms:title "Functional safety - Safety instrumented systems for the process industry sector - Part 1: Framework, definitions, system, hardware and software requirements"@en ;
                 rdfs:comment "This standard gives requirements for the specification, design, installation, operation and maintenance of a safety instrumented system (SIS), so that it can be confidently entrusted to achieve or maintain a safe state of the process. This standard has been developed as a process sector implementation of IEC 61508."@en ;
                 rdfs:label "DIN EN 61511"@en ;
                 sto_iot:hasTargetConcern sto:Safety .



###  https://w3id.org/i40/sto#DIN_EN_ISO_13849
sto:DIN_EN_ISO_13849 rdf:type owl:NamedIndividual ,
                              sto:Standard ;
                     dcterms:creator sto:irlan ,
                                     sto:sebastian ;
                     sto:hasClassification sto:IDSRAMCertification ;
                     sto:hasPublisher sto:DIN ,
                                      sto:ISO ;
                     owl:sameAs sto:ISO_13849;
                     sto:hasClassification sto:IDSRAMCertification ,
                                    sto:IIRASecurity;
                     sto_iot:hasTargetConcern sto:Safety;
                     rdfs:comment """ISO 13849 is a safety standard which deals with safety-related design principles of employed control systems to establish different safety Performance Levels (PL). It replaced EN 954-1 in December 2011.  Part 1 defines the general principles for design. Part 2 describes the validation."""@en ;
                     rdfs:label "DIN EN ISO 13849"@en ;
                     sto:hasDBpediaResource <http://dbpedia.org/resource/ISO_13849> ;
                     sto:hasWikipediaArticle <https://en.wikipedia.org/wiki/ISO_13849> ;
                     sto_iot:hasTargetConcern sto:Safety .

###  https://w3id.org/i40/sto#ISO_13849
sto:ISO_13849 rdf:type owl:NamedIndividual ,
                       sto:Standard ;
              dcterms:creator sto:irlan ;
              sto:hasClassification sto:AsSafety  ;
              sto:hasPublisher sto:ISO ;
              sto:relatedTo sto:IEC_61508 ,
                            sto:IEC_61511 ,
                            sto:IEC_62061 ,
                            sto:ISO_13849 ;
              rdfs:comment "Provides safety requirements and guidance on the principles for the design and integration of safety-related parts of control systems (SRP/CS), including the design of software."@en ;
              rdfs:label "ISO 13849"@en ;
              sto:hasDBpediaResource <http://dbpedia.org/resource/ISO_13849> ;
              sto:hasRelevantDomain sto:Safety_Machinery ;
              sto:hasOfficialResource <http://www.iso.org/iso/home/store/catalogue_tc/catalogue_detail.htm?csnumber=69883> ;
              sto:hasWikipediaArticle <https://en.wikipedia.org/wiki/ISO_13849> .


###  https://w3id.org/i40/sto#DIN_EN_ISO_IEC_17025
sto:DIN_EN_ISO_IEC_17025 rdf:type owl:NamedIndividual ,
                                  sto:Standard ;
                         dcterms:creator sto:irlan ,
                                         sto:sebastian ;
                         sto:hasAvailableLanguage lang:deu ,
                                                  lang:eng ;
                         sto:hasClassification sto:IDSRAMCertification ;
                         sto:hasPublisher sto:DIN ,
                                          sto:IEC ,
                                          sto:ISO ;
                         sto:hasPublicationDate "2018-03-01"^^xsd:date ;
                         dcterms:title "General requirements for the competence of testing and calibration laboratories"@en ;
                         rdfs:comment "DIN EN ISO/IEC 17025 legt allgemeine Anforderungen an die Kompetenz, an die Unparteilichkeit und für die einheitliche Arbeitsweise von Laboratorien fest. Die Norm ist auf alle Organisationen anwendbar, die Labortätigkeiten durchführen, unabhängig von der Anzahl der Mitarbeiter. Sie reiht sich in die Normenreihe DIN EN ISO/IEC 17000 ein. Kunden von Laboratorien, Behörden, Organisationen und Programme, die eine Begutachtung unter Gleichrangigen anwenden, Akkreditierungsstellen und andere können diese Norm zur Bestätigung oder Anerkennung der Kompetenz von Laboratorien nutzen."@de ,
                                      "ISO 17025 specifies general requirements for laboratories."@en ;
                         rdfs:label "DIN EN ISO/IEC 17025"@en ;
                         sto:hasAvailableLanguage lang:eng, 
                                                  lang:deu;
                         sto:hasPublicationDate "2018-03-01"^^xsd:date;
                         sto:hasOfficialResource <https://www.beuth.de/de/norm/din-en-iso-iec-17025/278030106> .


###  https://w3id.org/i40/sto#DIN_ISO_14638
sto:DIN_ISO_14638 rdf:type owl:NamedIndividual ,
                           sto:Standard ;
                  dcterms:creator sto:irlan ,
                                  sto:sebastian ;
                  sto:hasAvailableLanguage lang:deu ;
                  sto:hasPublisher sto:DIN ;
                  sto:hasPublicationDate "2015-12-01"^^xsd:date ;
                  sto:hasTag "ISO GPS"^^xsd:string ;
                  rdfs:comment "Geometrical product specifications (GPS) - Matrix model (ISO 14638:2015); German version EN ISO 14638:2015"@en ;
                  rdfs:label "DIN EN ISO 14638:2015-12"@en ;
                  sto:hasAvailableLanguage lang:deu;
                  sto_iot:hasTargetConcern sto:ThingDescription;
                  sto:hasPublicationDate "2015-12-01"^^xsd:date;
                  sto:hasOfficialResource <https://www.beuth.de/en/standard/din-en-iso-14638/208096393> .


###  https://w3id.org/i40/sto#DIN_SPEC_16592
sto:DIN_SPEC_16592 rdf:type owl:NamedIndividual ,
                            sto:Standard ;
                   dcterms:creator sto:irlan ,
                                   sto:sebastian ;
                   prov:wasGeneratedBy sto:IEC_62541 ,
                                       sto:IEC_62714 ;
                   sto:hasDeveloper sto:DIN ;
                   sto:hasPublisher sto:DIN ;
                   sto:relatedTo sto:DIN_SPEC_16592 ,
                                 sto:IEC_61131 ,
                                 sto:IEC_61360 ,
                                 sto:IEC_61499 ,
                                 sto:IEC_61804 ,
                                 sto:IEC_61850 ,
                                 sto:IEC_61987_X ,
                                 sto:IEC_62424 ,
                                 sto:IEC_62453 ,
                                 sto:IEC_62541 ,
                                 sto:IEC_62714 ,
                                 sto:ISO_13584 ,
                                 sto:ISO_14306 ,
                                 sto:ISO_15746 ,
                                 sto:ISO_15926 ,
                                 sto:ISO_18629 ,
                                 sto:ISO_18828-2 ,
                                 sto:ISO_20922 ,
                                 sto:ISO_22400 ,
                                 sto:ISO_29002 ,
                                 sto:ISO_ASTM_52915 ,
                                 sto:ISO_PAS_17506 ,
                                 sto:MathML ,
                                 sto:SysML ,
                                 sto:eClass ;
                   rdfs:comment "Combining OPC Unified Architecture and Automation Markup Language."@en ;
                   rdfs:label "DIN SPEC 16592"@en ;
                   sto:hasAvailableLanguage lang:eng;
                   sto:hasPublicationDate "2016-12-01"^^xsd:date;
                   sto:hasOfficialResource <https://www.beuth.de/de/technische-regel/din-spec-16592/265597431> .


###  https://w3id.org/i40/sto#DIN_SPEC_16593_P1
sto:DIN_SPEC_16593_P1 rdf:type owl:NamedIndividual ,
                               sto:Standard ;
                      dcterms:creator sto:irlan ,
                                      sto:sebastian ;
                      sto:hasAvailableLanguage lang:eng ;
                      sto:hasPublisher sto:DIN ;
                      sto_iot:frames sto:ServiceDescription ;
                      sto:hasPublicationDate "2018-04-01"^^xsd:date ;
                      sto:hasTag "DIN SPEC 16593-1:2018-04"^^xsd:string ;
                      rdfs:comment "RM-SA - Reference Model for Industrie 4.0 Service Architectures - Part 1: Basic Concepts of an Interaction-based Architecture; Text in English"@en ;
                      rdfs:label "DIN SPEC 16593-1:2018-04"@en ;
                      sto:hasOfficialResource <https://www.beuth.de/en/technical-rule/din-spec-16593-1/287632675> .


###  https://w3id.org/i40/sto#DIN_SPEC_27070
sto:DIN_SPEC_27070 rdf:type owl:NamedIndividual ,
                            sto:Standard ;
                   dcterms:creator sto:sebastian ,
                                   sto:irlan ;
                   dul:associatedWith sto:TrustedConnector ;
                   sto:hasClassification sto:IDSRAMSecurity ;
                   sto:hasPublisher sto:DIN ;
                   dcterms:title "Reference architecture of a security gateway for the exchange of industry data and services"@en ;
                   rdfs:comment "security gateway for data protection of personal data"@en ;
                   rdfs:label "DIN SPEC 27070"@en ;
                   sto:alignsWith sto:TrustedConnector ;
                   sto:hasOfficialResource <https://www.beuth.de/de/publikation/din-spec-27070-din-spec-27072/289649579> .


###  https://w3id.org/i40/sto#DIN_SPEC_91345
sto:DIN_SPEC_91345 rdf:type owl:NamedIndividual ,
                            sto:Standard ,
                            oa:SpecificResource ;
                   dcterms:creator sto:irlan ,
                                   sto:sebastian ;
                   sto:hasAvailableLanguage lang:eng ;
                   sto:hasICS sto:ICS_03_100_01 ,
                              sto:ICS_25_040_01 ,
                              sto:ICS_35_240_50 ;
                   sto:hasPublisher sto:DIN ;
                   sto:hasImplementationFormat "Document"@en ;
                   sto:hasPages "40"^^xsd:int ;
                   sto:hasPublicationDate "2016-04-01"^^xsd:date ;
                   rdfs:comment "Reference Architecture Model Industrie 4.0 (RAMI4.0) English translation of DIN SPEC 91345:2016-04"@en ;
                   rdfs:label "DIN SPEC 91345:2016-04"@en ;
                   sto:hasOfficialResource <https://www.beuth.de/en/technical-rule/din-spec-91345/250940128> .


###  https://w3id.org/i40/sto#DIN_SPEC_92222
sto:DIN_SPEC_92222 rdf:type owl:NamedIndividual ,
                            sto:Standard ;
                   dcterms:creator sto:irlan ,
                                   sto:sebastian ;
                   sto:hasClassification sto:IDSRAMSecurity ;
                   sto:hasDeveloper sto:DIN ;
                   sto:hasPublisher sto:DIN ;
                   sto_iot:frames sto:CloudComputing ,
                                  sto:communication ,
                                  sto:interoperability ;
                   dcterms:title "Reference Model for Industrial Cloud Federation"@en ;
                   rdfs:comment "ensuring interoperability and communication of IT systems in cloud scenarios"@en ;
                   rdfs:label "DIN SPEC 92222"@en ;
                   sto:hasOfficialResource <https://www.beuth.de/de/publikation/referenzmodell-industrielle-cloud-federation/296675641> .


###  https://w3id.org/i40/sto#DMA
sto:DMA rdf:type owl:NamedIndividual ,
                 sto:StandardOrganization ;
        dcterms:creator sto:sebastian ;
        dcterms:title "Data & Marketing Association"@en ;
        rdfs:comment "The Data & Marketing Association (formerly, Direct Marketing Association), also known as the DMA, is a trade organization for marketers which seeks to advance and protect responsible data-driven marketing."@en ;
        rdfs:label "DMA"@en ;
        sto:hasWikipediaArticle <https://en.wikipedia.org/wiki/Data_%26_Marketing_Association> ;
.

###  https://w3id.org/i40/sto#DMSC
sto:DMSC rdf:type owl:NamedIndividual ,
                  sto:StandardOrganization ;
         dcterms:creator sto:irlan ,
                         sto:sebastian ;
         sto:hasHeadquaterIn dbr:_Texas ;
         rdfs:comment "Dimensional Metrology Standards Consortium (DMSC) is to identify urgently needed standards in the field of dimensional metrology, and to promote, foster, and encourage the development and interoperability of these standards, along with related and supporting standards that will benefit the industry as a whole."@en ;
         rdfs:label "Dimensional Metrology Standards Consortium"@en ;
         sto:hasOfficialResource <http://www.dmis.org/> .


###  https://w3id.org/i40/sto#DTLS
sto:DTLS rdf:type owl:NamedIndividual ,
                  sto:TechnicalSpecification ;
         dcterms:creator sto:irlan ,
                         sto:sebastian ;
         rdfs:comment "Datagram Transport Layer - The DTLS protocol provides communications privacy for datagram protocols. The protocol allows client/server applications to communicate in a way that is designed to prevent eavesdropping, tampering, or message forgery. The DTLS protocol is based on the Transport Layer Security (TLS) protocol and provides equivalent security guarantees. (source: https://www.postscapes.com/internet-of-things-protocols/)"@en ;
         rdfs:label "DTLS"@en ;
         sto:hasOfficialResource <https://tools.ietf.org/html/rfc4347> .


###  https://w3id.org/i40/sto#DeviceLevel
sto:ISA95DeviceLevel rdf:type owl:NamedIndividual ,
                         sto:ISA95Level ,
                         sto:StandardClassification ;
                rdfs:comment "Describes the device level according to the ISA95 level classification."@en ;
                sto:isDescribedin sto:ISA95 ;
                rdfs:label "Device Level"@en .


###  https://w3id.org/i40/sto#DigiMesh
sto:DigiMesh rdf:type owl:NamedIndividual ,
                      sto:TechnicalSpecification ;
             dcterms:creator sto:sebastian ;
             rdfs:comment "DigiMesh is a proprietary peer-to-peer networking topology for use in wireless end-point connectivity solutions. (source: https://www.postscapes.com/internet-of-things-protocols/)"@en ;
             rdfs:label "DigiMesh"@en ;
             sto:hasOfficialResource <http://www.digi.com/technology/digimesh/> .


###  https://w3id.org/i40/sto#ENISA
sto:ENISA rdf:type owl:NamedIndividual ,
                   sto:StandardOrganization ;
          dcterms:title "European Union Agency for Network and Information Security"@en ;
          rdfs:comment "ENISA provides recommendations on cybersecurity, supports policy development and its implementation, and collaborates with operational teams throughout Europe."@en ;
          rdfs:label "ENISA"@en ;
          sto:hasOfficialResource <https://www.enisa.europa.eu/> .


###  https://w3id.org/i40/sto#ENISA_CloudComputing
sto:ENISA_CloudComputing rdf:type owl:NamedIndividual ,
                                  sto:RelevantDomain,
                                  sto:Standard ;
                         dcterms:creator sto:ENISA ;
                         foaf:maker sto:ENISA ;
                         sto:hasClassification sto:IIRASecurity ;
                         sto:hasPublisher sto:ENISA ;
                         sto:domainName "Cloud Computing"@en ;
                         sto:hasPublicationDate "2012-12-01"^^xsd:date ;
                         dcterms:title "Cloud Computing - Benefits, risks and recommendations for information security"@en ;
                         rdfs:comment "ENISA, supported by a group of subject matter expert comprising representatives from Industries, Academia and Governmental Organizations, has conducted, in the context of the Emerging and Future Risk Framework project, an risks assessment on cloud computing business model and technologies. The result is an in-depth and independent analysis that outlines some of the information security benefits and key security risks of cloud computing. The report provide also a set of practical recommendations.Produced by ENISA with contributions from a group of subject matter expert comprising representatives from Industry, Academia and Governmental Organizations, a risk assessment of cloud computing business model and technologies. This is an in-depth and independent analysis that outlines some of the information security benefits and key security risks of cloud computing. The report provide also a set of practical recommendations. It is produced in the context of the Emerging and Future Risk Framework project."@en ;
                         rdfs:label "ENISA Cloud Computing"@en ;
                         sto:hasOfficialResource <https://resilience.enisa.europa.eu/cloud-security-and-resilience/publications/cloud-computing-benefits-risks-and-recommendations-for-information-security> .


###  https://w3id.org/i40/sto#ETSI
sto:ETSI rdf:type owl:NamedIndividual ,
                  sto:StandardOrganization ;
         sto:hasHeadquaterIn dbr:Valbonne ;
         sto:abbreviation "ETSI"@en ;
         sto:formationDate "1988-01-01"^^xsd:date ;
         sto:orgName "European Telecommunications Standards Institute"@en ;
         rdfs:comment "The European Telecommunications Standards Institute (ETSI) is an independent, not-for-profit, standardization organization in the telecommunications industry (equipment makers and network operators) in Europe, headquartered in Sophia-Antipolis, France, with worldwide projection. ETSI produces globally-applicable standards for Information and Communications Technologies (ICT), including fixed, mobile, radio, converged, broadcast and internet technologies."@en ;
         rdfs:label "ETSI"@en ;
         sto:hasDBpediaResource <http://dbpedia.org/resource/ETSI> ;
         sto:hasOfficialResource <http://www.etsi.org/> ;
         sto:hasWikipediaArticle <https://en.wikipedia.org/wiki/ETSI> .


###  https://w3id.org/i40/sto#ETSI_DECT
sto:ETSI_DECT rdf:type owl:NamedIndividual ,
                       sto:Standard ;
              dcterms:creator sto:irlan ,
                              sto:sebastian ;
              sto:hasDeveloper sto:ETSI ;
              sto:hasPublisher sto:ETSI ;
              sto:hasTag "Digital Enhanced Cordless Telecommunications"@en ;
              rdfs:comment "Digital Enhanced Cordless Telecommunications (DECT) is the ETSI standard for short-range cordless communications, which can be adapted for many applications and can be used over unlicensed frequency allocations world-wide."@en ;
              rdfs:label "ETSI DECT"^^xsd:string ;
              sto:hasDBpediaResource <http://dbpedia.org/resource/Digital_Enhanced_Cordless_Telecommunications> ;
              sto:hasOfficialResource <http://www.etsi.org/technologies-clusters/technologies/dect> ;
              sto:hasWikipediaArticle <https://en.wikipedia.org/wiki/Digital_Enhanced_Cordless_Telecommunications> .


###  https://w3id.org/i40/sto#ETSI_LTN
sto:ETSI_LTN rdf:type owl:NamedIndividual ,
                      sto:Standard ;
             dcterms:creator sto:irlan ,
                             sto:sebastian ;
             sto:hasDeveloper sto:ETSI ;
             sto:hasDomain sto:M2M ;
             sto:hasPublisher sto:ETSI ;
             sto:relatedTo sto:ETSI_DECT ,
                           sto:ETSI_LTN ,
                           sto:ETSI_ULE ;
             sto:hasTag "Low Throughput Networks"@en ;
             rdfs:comment "Machine-to-Machine communications and the Internet of Things (IoT) involve the connection of potentially billions of connected objects which need only low throughput connectivity. The anticipated benefits of creating new dedicated IoT Low Throughput Networks (LTN) include lower costs, the creation of new applications, a reduction in electromagnetic radiation by improving data transmission efficiency LTN are expected to be crucial to the success of IoT standardization and implementation, and to provide the basis for many new and innovative applications. "@en ;
             rdfs:label "ETSI LTN"@en ;
             sto:hasOfficialResource <http://www.etsi.org/technologies-clusters/technologies/low-throughput-networks> .


###  https://w3id.org/i40/sto#ETSI_ULE
sto:ETSI_ULE rdf:type owl:NamedIndividual ,
                      sto:Standard ;
             dcterms:creator sto:irlan ,
                             sto:sebastian ;
             sto:hasDeveloper sto:ETSI ;
             sto:hasPublisher sto:ETSI ;
             sto:relatedTo sto:ETSI_DECT ,
                           sto:ETSI_LTN ,
                           sto:ETSI_ULE ;
             sto:hasTag "ETSI ULE"@en ;
             rdfs:comment "DECT Ultra Low Energy (DECT ULE) is a technology based on DECT, and intended for Machine-to-Machine communications such as Home and Industrial automation. The main characteristics of the technology are ultra-low power consumption (much lower than IEEE 802.11) and wider coverage (much wider than IEEE 802.15 and Bluetooth Low Energy)."@en ;
             rdfs:label "Ultra Low Energy"@en ;
             sto:hasDBpediaResource <http://dbpedia.org/resource/ULE_-_Ultra_Low_Energy> ;
             sto:hasOfficialResource <http://www.etsi.org/technologies-clusters/technologies/dect/dect-ule> ;
             sto:hasWikipediaArticle <https://en.wikipedia.org/wiki/DECT_Ultra_Low_Energy> .


###  https://w3id.org/i40/sto#EcGsmIoT
sto:EcGsmIoT rdf:type owl:NamedIndividual ,
                      sto:TechnicalSpecification ;
             dcterms:creator sto:sebastian ;
             rdfs:comment "EC-GSM-IoT (Extended Coverage-GSM-IoT): Enables new capabilities of existing cellular networks for LPWA (Low Power Wide Area) IoT applications. EC-GSM-IoT can be activated through new software deployed over a very large GSM footprint, adding even more coverage to serve IoT devices. (source: https://www.postscapes.com/internet-of-things-protocols/)"@en ;
             rdfs:label "EC-GSM-IoT"@en ;
             sto:hasOfficialResource <https://www.ericsson.com/news/1987789> .


###  https://w3id.org/i40/sto#EclipsePaho
sto:EclipsePaho rdf:type owl:NamedIndividual ,
                         sto:TechnicalSpecification ;
                dcterms:creator sto:sebastian ;
                rdfs:comment "The scope of the Paho project is to provide open source implementations of open and standard messaging protocols that support current and emerging requirements of M2M integration with Web and Enterprise middleware and applications. It will include client implementations for use on embedded platforms along with corresponding server support as determined by the community. (source: https://www.postscapes.com/internet-of-things-protocols/)"@en ;
                rdfs:label "Eclipse Paho Project"@en ;
                sto:hasOfficialResource <https://www.eclipse.org/proposals/technology.paho/> .


###  https://w3id.org/i40/sto#Eddystone
sto:Eddystone rdf:type owl:NamedIndividual ,
                       sto:TechnicalSpecification ;
              dcterms:creator sto:irlan ,
                              sto:sebastian ;
              rdfs:comment "Eddystone - A protocol specification that defines a Bluetooth low energy (BLE) message format for proximity beacon messages. (source: https://www.postscapes.com/internet-of-things-protocols/)"@en ;
              rdfs:label "Eddystone"@en ;
              sto:hasOfficialResource <https://github.com/google/eddystone> .


###  https://w3id.org/i40/sto#EnOcean
sto:EnOcean rdf:type owl:NamedIndividual ,
                     sto:TechnicalSpecification ;
            dcterms:creator sto:sebastian ;
            rdfs:comment "EnOcean is a an energy harvesting wireless technology which works in the frequencies of 868 MHz for europe and 315 MHz for North America. The transmit range goes up to 30 meter in buildings and up to 300 meter outdoor. (source: https://www.postscapes.com/internet-of-things-protocols/)"@en ;
            rdfs:label "EnOcean"@en ;
            sto:hasOfficialResource <http://www.enocean.com/en/home/> .

###  https://w3id.org/i40/sto#EnterpriseIntegration
sto:EnterpriseIntegration rdf:type owl:NamedIndividual ,
                                   sto:RelevantDomain;
                          sto:domainName "EnterpriseIntegration"@en ;
                          rdfs:comment "Enterprise Integration deals primarily with system interconnection, electronic data interchange, product data exchange and distributed computing environments."@en ;
                          rdfs:label "EnterpriseIntegration"@en ;
                          sto:hasWikipediaArticle <https://en.wikipedia.org/wiki/Enterprise_integration> ;
                          sto:hasDBpediaResource <http://dbpedia.org/page/Enterprise_integration>;
                          .

sto:CloudComputing rdf:type owl:NamedIndividual ,
                                   sto:RelevantDomain;
                          sto:domainName "Cloud Computing"@en ;
                          rdfs:comment "Cloud computing is the on-demand availability of computer system resources, especially data storage and computing power, without direct active management by the user."@en ;
                          rdfs:label "Cloud Computing"@en ;
                          sto:hasWikipediaArticle <https://en.wikipedia.org/wiki/Cloud_computing> ;
                          sto:hasDBpediaResource <http://dbpedia.org/page/Cloud_computing>;
                          .


###  https://w3id.org/i40/sto#EnterpriseLevel
sto:ISA95EnterpriseLevel rdf:type owl:NamedIndividual ,
                             sto:ISA95Level ,
                             sto:StandardClassification ;
                    rdfs:comment "Describes the Enterprise level according to the ISA95 level classification."@en ;
                    sto:isDescribedin sto:ISA95 ;
                    rdfs:label "Enterprise Level"@en .


###  https://w3id.org/i40/sto#Enterprise_Control
sto:Enterprise_Control rdf:type owl:NamedIndividual ,
                                sto:Domain ;
                       sto:domainName "Enterprise Control"@en ;
                       rdfs:comment "Enterprise Control Domain"@en ;
                       rdfs:label "Enterprise Control"@en .


###  https://w3id.org/i40/sto#EstonianInformationSystemAuthority
sto:EstonianInformationSystemAuthority rdf:type owl:NamedIndividual ,
                                                sto:StandardOrganization ;
                                       rdfs:label "Information System Authority of Estonia"@en ;
                                       sto:hasOfficialResource <https://www.ria.ee/en.html> .


###  https://w3id.org/i40/sto#FileSizeIEC_60027_P6
sto:FileSizeIEC_60027_P6 rdf:type owl:NamedIndividual ,
                                  om2:Measure ;
                         om2:hasUnit om2:kilobyte ;
                         om2:hasNumericalValue "661.0"^^xsd:float ;
                         rdfs:comment "Specifies the file size of the document for standard IEC 60027:2006"@en ;
                         rdfs:label "FileSize IEC 60027-6:2006"@en .


###  https://w3id.org/i40/sto#FileSizeIEC_60038
sto:FileSizeIEC_60038 rdf:type owl:NamedIndividual ,
                               om2:Measure ;
                      om2:hasUnit om2:kilobyte ;
                      om2:hasNumericalValue "946.0"^^xsd:float ;
                      rdfs:comment "Specifies the file size of the document for standard IEC 60038:2009"@en ;
                      rdfs:label "FileSize IEC 60038:2009"@en .


###  https://w3id.org/i40/sto#FileSizeIEC_60038_2009
sto:FileSizeIEC_60038_2009 rdf:type owl:NamedIndividual ,
                                    om2:Measure ;
                           om2:hasUnit om2:kilobyte ;
                           om2:hasNumericalValue "946.0"^^xsd:float ;
                           rdfs:comment "Specifies the file size of the document for standard IEC 60038:2009"@en ;
                           rdfs:label "FileSize IEC 60038:2009"@en .


###  https://w3id.org/i40/sto#FileSizeIEC_60050_P101
sto:FileSizeIEC_60050_P101 rdf:type owl:NamedIndividual ,
                                    om2:Measure ;
                           om2:hasUnit om2:kilobyte ;
                           om2:hasNumericalValue "1712.0"^^xsd:float ;
                           rdfs:comment "Specifies the file size of the document for standard IEC 60050-101:1998 "@en ;
                           rdfs:label "FileSize IEC 60050-101:1998"@en .


###  https://w3id.org/i40/sto#FileSizeIEC_60050_P351
sto:FileSizeIEC_60050_P351 rdf:type owl:NamedIndividual ,
                                    om2:Measure ;
                           om2:hasUnit om2:kilobyte ;
                           om2:hasNumericalValue "3999.0"^^xsd:float ;
                           rdfs:comment "Specifies the file size of the document for standard IEC 60050-351:2013 "@en ;
                           rdfs:label "FileSize IEC 60050-351:2013"@en .


###  https://w3id.org/i40/sto#FileSizeIEC_60050_P371
sto:FileSizeIEC_60050_P371 rdf:type owl:NamedIndividual ,
                                    om2:Measure ;
                           om2:hasUnit om2:kilobyte ;
                           om2:hasNumericalValue "2485.0"^^xsd:float ;
                           rdfs:comment "Specifies the file size of the document for standard IEC 60050-101:1998 "@en ;
                           rdfs:label "FileSize IEC 60050-371:1984"@en .


###  https://w3id.org/i40/sto#FileSizeIEC_60073
sto:FileSizeIEC_60073 rdf:type owl:NamedIndividual ,
                               om2:Measure ;
                      om2:hasUnit om2:kilobyte ;
                      om2:hasNumericalValue "525.0"^^xsd:float ;
                      rdfs:comment "Specifies the file size of the document for standard IEC 60073:2002"@en ;
                      rdfs:label "FileSize IEC 60073:2002"@en .


###  https://w3id.org/i40/sto#FileSizeIEC_60204
sto:FileSizeIEC_60204 rdf:type owl:NamedIndividual ,
                               om2:Measure ;
                      om2:hasUnit om2:kilobyte ;
                      om2:hasNumericalValue "494.0"^^xsd:float ;
                      rdfs:comment "Specifies the file size of the document for standard IEC 60204:2000"@en ;
                      rdfs:label "FileSize IEC 60204:2000"@en .


###  https://w3id.org/i40/sto#FileSizeIEC_60204_P11
sto:FileSizeIEC_60204_P11 rdf:type owl:NamedIndividual .


###  https://w3id.org/i40/sto#FileSizeIEC_60255_149_2013
sto:FileSizeIEC_60255_149_2013 rdf:type owl:NamedIndividual ,
                                        om2:Measure ;
                               om2:hasUnit om2:kilobyte ;
                               om2:hasNumericalValue "1722.0"^^xsd:float ;
                               rdfs:comment "Specifies the file size of the document for standard IEC 60255-149:2013 "@en ;
                               rdfs:label "FileSize 60255-149:2013"@en .


###  https://w3id.org/i40/sto#FileSizeIEC_60255_2009
sto:FileSizeIEC_60255_2009 rdf:type owl:NamedIndividual ,
                                    om2:Measure ;
                           om2:hasUnit om2:kilobyte ;
                           om2:hasNumericalValue "1411.0"^^xsd:float ;
                           rdfs:comment "Specifies the file size of the document for standard 60255-1:2009"@en ;
                           rdfs:label "FileSize IEC 60255-1:2009"@en .


###  https://w3id.org/i40/sto#FileSizeIEC_60255_2010
sto:FileSizeIEC_60255_2010 rdf:type owl:NamedIndividual ,
                                    om2:Measure ;
                           om2:hasUnit om2:kilobyte ;
                           om2:hasNumericalValue "1215.0"^^xsd:float ;
                           rdfs:comment "Specifies the file size of the document for standard IEC 60255-127:2010 "@en ;
                           rdfs:label "FileSize 60255-127:2010"@en .


###  https://w3id.org/i40/sto#FileSizeIEC_60255_P1
sto:FileSizeIEC_60255_P1 rdf:type owl:NamedIndividual ,
                                  om2:Measure ;
                         om2:hasUnit om2:kilobyte ;
                         om2:hasNumericalValue "1411.0"^^xsd:float ;
                         rdfs:comment "Specifies the file size of the document for standard 60255-1:2009"@en ;
                         rdfs:label "FileSize IEC 60255-1:2009"@en .


###  https://w3id.org/i40/sto#FileSizeIEC_60255_P127
sto:FileSizeIEC_60255_P127 rdf:type owl:NamedIndividual ,
                                    om2:Measure ;
                           om2:hasUnit om2:kilobyte ;
                           om2:hasNumericalValue "1215.0"^^xsd:float ;
                           rdfs:comment "Specifies the file size of the document for standard IEC 60255-127:2010 "@en ;
                           rdfs:label "FileSize 60255-127:2010"@en .


###  https://w3id.org/i40/sto#FileSizeIEC_60255_P149
sto:FileSizeIEC_60255_P149 rdf:type owl:NamedIndividual ,
                                    om2:Measure ;
                           om2:hasUnit om2:kilobyte ;
                           om2:hasNumericalValue "1722.0"^^xsd:float ;
                           rdfs:comment "Specifies the file size of the document for standard IEC 60255-149:2013 "@en ;
                           rdfs:label "FileSize 60255-149:2013"@en .


###  https://w3id.org/i40/sto#FileSizeIEC_60255_P151
sto:FileSizeIEC_60255_P151 rdf:type owl:NamedIndividual ,
                                    om2:Measure ;
                           om2:hasUnit om2:kilobyte ;
                           om2:hasNumericalValue "1341.0"^^xsd:float ;
                           rdfs:comment "Specifies the file size of the document for standard IEC IEC 60255-151:2009"@en ;
                           rdfs:label "FileSize IEC 60255-151:2009 "@en .


###  https://w3id.org/i40/sto#FileSizeIEC_60255_P27
sto:FileSizeIEC_60255_P27 rdf:type owl:NamedIndividual ,
                                   om2:Measure ;
                          om2:hasUnit om2:kilobyte ;
                          om2:hasNumericalValue "2520.0"^^xsd:float ;
                          rdfs:comment "Specifies the file size of the document for standard IEC 60255-27:2013"@en ;
                          rdfs:label "FileSize IEC 60255-27:2013"@en .


###  https://w3id.org/i40/sto#FileSizeIEC_60286_P3
sto:FileSizeIEC_60286_P3 rdf:type owl:NamedIndividual ,
                                  om2:Measure ;
                         om2:hasUnit om2:kilobyte ;
                         om2:hasNumericalValue "1764.0"^^xsd:float ;
                         rdfs:comment "Specifies the file size of the document for standard IEC IEC 60286-3:2013 "@en ;
                         rdfs:label "FileSize IEC 60286-3:2013  "@en .


###  https://w3id.org/i40/sto#FileSizeIEC_60286_P4
sto:FileSizeIEC_60286_P4 rdf:type owl:NamedIndividual ,
                                  om2:Measure ;
                         om2:hasUnit om2:kilobyte ;
                         om2:hasNumericalValue "1129.0"^^xsd:float ;
                         rdfs:comment "Specifies the file size of the document for standard IEC IEC 60286-4:2013 "@en ;
                         rdfs:label "FileSize IEC 60286-4:2013  "@en .


###  https://w3id.org/i40/sto#FileSizeIEC_60286_P5
sto:FileSizeIEC_60286_P5 rdf:type owl:NamedIndividual ,
                                  om2:Measure ;
                         om2:hasUnit om2:kilobyte ;
                         om2:hasNumericalValue "3481.0"^^xsd:float ;
                         rdfs:comment "Specifies the file size of the document for standard IEC IEC 60286-5:2018 "@en ;
                         rdfs:label "FileSize IEC 60286-5:2018  "@en .


###  https://w3id.org/i40/sto#FileSizeIEC_60381_P1
sto:FileSizeIEC_60381_P1 rdf:type owl:NamedIndividual ,
                                  om2:Measure ;
                         om2:hasUnit om2:kilobyte ;
                         om2:hasNumericalValue "507.0"^^xsd:float ;
                         rdfs:comment "Specifies the file size of the document for standard IEC 60381-1:1982 "@en ;
                         rdfs:label "FileSize IEC 60381-1:1982"@en .


###  https://w3id.org/i40/sto#FileSizeIEC_60381_P2
sto:FileSizeIEC_60381_P2 rdf:type owl:NamedIndividual ,
                                  om2:Measure ;
                         om2:hasUnit om2:kilobyte ;
                         om2:hasNumericalValue "483.0"^^xsd:float ;
                         rdfs:comment "Specifies the file size of the document for standard IEC 60381-2:1978"@en ;
                         rdfs:label "FileSize IEC 60381-2:1978"@en .


###  https://w3id.org/i40/sto#FileSizeIEC_60382
sto:FileSizeIEC_60382 rdf:type owl:NamedIndividual ,
                               om2:Measure ;
                      om2:hasUnit om2:kilobyte ;
                      om2:hasNumericalValue "1460.0"^^xsd:float ,
                                            "557.0"^^xsd:float ;
                      rdfs:comment "Specifies the file size of the document for standard  IEC 60382:1991."@en ;
                      rdfs:label "FileSize IEC 60382:1991"@en ;
                      skos:note "todo"@en .


###  https://w3id.org/i40/sto#FileSizeIEC_60382_1991
sto:FileSizeIEC_60382_1991 rdf:type owl:NamedIndividual ,
                                    om2:Measure ;
                           om2:hasUnit om2:kilobyte ;
                           om2:hasNumericalValue "557.0"^^xsd:float ;
                           rdfs:comment "Specifies the file size of the document for standard IEC 60382:1991"@en ;
                           rdfs:label "FileSize IEC 60382:1991"@en .


###  https://w3id.org/i40/sto#FileSizeIEC_60839_P5_S2
sto:FileSizeIEC_60839_P5_S2 rdf:type owl:NamedIndividual ,
                                     om2:Measure ;
                            om2:hasUnit om2:kilobyte ;
                            om2:hasNumericalValue "1137.0"^^xsd:float ;
                            rdfs:comment "Specifies the file size of the document for standard IEC 60839-5-2:2016"@en ;
                            rdfs:label "FileSize IEC 60839-5-2:2016"@en .


###  https://w3id.org/i40/sto#FileSizeIEC_60839_P7_S1
sto:FileSizeIEC_60839_P7_S1 rdf:type owl:NamedIndividual ,
                                     om2:Measure ;
                            om2:hasUnit om2:kilobyte ;
                            om2:hasNumericalValue "1137.0"^^xsd:float ;
                            rdfs:comment "Specifies the file size of the document for standard IEC 60839-7-1:2001"@en ;
                            rdfs:label "FileSize IEC 60839-7-1:2001"@en .


###  https://w3id.org/i40/sto#FileSizeIEC_60839_P7_S2
sto:FileSizeIEC_60839_P7_S2 rdf:type owl:NamedIndividual ,
                                     om2:Measure ;
                            om2:hasUnit om2:kilobyte ;
                            om2:hasNumericalValue "1047.0"^^xsd:float ;
                            rdfs:comment "Specifies the file size of the document for standard IEC 60839-7-2:2001"@en ;
                            rdfs:label "FileSize IEC 60839-7-2:2001"@en .


###  https://w3id.org/i40/sto#FileSizeIEC_60839_P7_S3
sto:FileSizeIEC_60839_P7_S3 rdf:type owl:NamedIndividual ,
                                     om2:Measure ;
                            om2:hasUnit om2:kilobyte ;
                            om2:hasNumericalValue "975.0"^^xsd:float ;
                            rdfs:comment "Specifies the file size of the document for standard IEC 60839-7-3:2001"@en ;
                            rdfs:label "FileSize IEC 60839-7-3:2001"@en .


###  https://w3id.org/i40/sto#FileSizeIEC_60839_P7_S4
sto:FileSizeIEC_60839_P7_S4 rdf:type owl:NamedIndividual ,
                                     om2:Measure ;
                            om2:hasUnit om2:kilobyte ;
                            om2:hasNumericalValue "967.0"^^xsd:float ;
                            rdfs:comment "Specifies the file size of the document for standard IEC 60839-7-4:2001"@en ;
                            rdfs:label "FileSize IEC 60839-7-4:2001"@en .


###  https://w3id.org/i40/sto#FileSizeIEC_60839_P7_S5
sto:FileSizeIEC_60839_P7_S5 rdf:type owl:NamedIndividual ,
                                     om2:Measure ;
                            om2:hasUnit om2:kilobyte ;
                            om2:hasNumericalValue "939.0"^^xsd:float ;
                            rdfs:comment "Specifies the file size of the document for standard IEC 60839-7-5:2001"@en ;
                            rdfs:label "FileSize IEC 60839-7-5:2001"@en .


###  https://w3id.org/i40/sto#FileSizeIEC_60839_P7_S6
sto:FileSizeIEC_60839_P7_S6 rdf:type owl:NamedIndividual ,
                                     om2:Measure ;
                            om2:hasUnit om2:kilobyte ;
                            om2:hasNumericalValue "926.0"^^xsd:float ;
                            rdfs:comment "Specifies the file size of the document for standard IEC 60839-7-6:2001"@en ;
                            rdfs:label "FileSize IEC 60839-7-6:2001"@en .


###  https://w3id.org/i40/sto#FileSizeIEC_60839_P7_S7
sto:FileSizeIEC_60839_P7_S7 rdf:type owl:NamedIndividual ,
                                     om2:Measure ;
                            om2:hasUnit om2:kilobyte ;
                            om2:hasNumericalValue "964.0"^^xsd:float ;
                            rdfs:comment "Specifies the file size of the document for standard IEC 60839-7-7:2001"@en ;
                            rdfs:label "FileSize IEC 60839-7-7:2001"@en .


###  https://w3id.org/i40/sto#FileSizeIEC_60848
sto:FileSizeIEC_60848 rdf:type owl:NamedIndividual ,
                               om2:Measure ;
                      om2:hasUnit om2:kilobyte ;
                      om2:hasNumericalValue "1784.0"^^xsd:float ;
                      rdfs:comment "Specifies the file size of the document for standard IEC 60848:2013"@en ;
                      rdfs:label "FileSize IEC 60848:2013"@en .


###  https://w3id.org/i40/sto#FileSizeIEC_60864_P1
sto:FileSizeIEC_60864_P1 rdf:type owl:NamedIndividual ,
                                  om2:Measure ;
                         om2:hasUnit om2:kilobyte ;
                         om2:hasNumericalValue "1540.0"^^xsd:float ;
                         rdfs:comment "Specifies the file size of the document for standard IEC 60864-1:1986 "@en ;
                         rdfs:label "FileSizeIEC 60864-1:1986"@en .


###  https://w3id.org/i40/sto#FileSizeIEC_60864_P2
sto:FileSizeIEC_60864_P2 rdf:type owl:NamedIndividual ,
                                  om2:Measure ;
                         om2:hasUnit om2:kilobyte ;
                         om2:hasNumericalValue "283.0"^^xsd:float ;
                         rdfs:comment "Specifies the file size of the document for standard IEC 60864-2:1997"@en ;
                         rdfs:label "FileSize IEC 60864-2:1997"@en .


###  https://w3id.org/i40/sto#FileSizeIEC_60870_1990_P5_S1
sto:FileSizeIEC_60870_1990_P5_S1 rdf:type owl:NamedIndividual ,
                                          om2:Measure ;
                                 om2:hasUnit om2:kilobyte ;
                                 om2:hasNumericalValue "2954.0"^^xsd:float ;
                                 rdfs:comment "Specifies the file size of the document for standard IEC 60870-5-1:1990"@en ;
                                 rdfs:label "FileSize IEC 60870-5-1:1990"@en .


###  https://w3id.org/i40/sto#FileSizeIEC_60870_1992_P5_S2
sto:FileSizeIEC_60870_1992_P5_S2 rdf:type owl:NamedIndividual ,
                                          om2:Measure ;
                                 om2:hasUnit om2:kilobyte ;
                                 om2:hasNumericalValue "3658.0"^^xsd:float ;
                                 rdfs:comment "Specifies the file size of the document for standard IEC 60870-5-2:1992"@en ;
                                 rdfs:label "FileSize IEC 60870-5-2:1992"@en .


###  https://w3id.org/i40/sto#FileSizeIEC_60870_1992_P5_S3
sto:FileSizeIEC_60870_1992_P5_S3 rdf:type owl:NamedIndividual ,
                                          om2:Measure ;
                                 om2:hasUnit om2:kilobyte ;
                                 om2:hasNumericalValue "1629.0"^^xsd:float ;
                                 rdfs:comment "Specifies the file size of the document for standard IEC 60870-5-3:1992"@en ;
                                 rdfs:label "FileSize IEC 60870-5-3:1992"@en .


###  https://w3id.org/i40/sto#FileSizeIEC_60870_1995_P2_S1
sto:FileSizeIEC_60870_1995_P2_S1 rdf:type owl:NamedIndividual ,
                                          om2:Measure ;
                                 om2:hasUnit om2:kilobyte ;
                                 om2:hasNumericalValue "1674.0"^^xsd:float ;
                                 rdfs:comment "Specifies the file size of the document for standard IEC 60870-2-1:1995"@en ;
                                 rdfs:label "FileSize IEC 60870-2-1:1995"@en .


###  https://w3id.org/i40/sto#FileSizeIEC_60870_1996_P2_S2
sto:FileSizeIEC_60870_1996_P2_S2 rdf:type owl:NamedIndividual ,
                                          om2:Measure ;
                                 om2:hasUnit om2:kilobyte ;
                                 om2:hasNumericalValue "1705.0"^^xsd:float ;
                                 rdfs:comment "Specifies the file size of the document for standard IEC 60870-2-2:1996"@en ;
                                 rdfs:label "FileSize IEC 60870-2-2:1996"@en .


###  https://w3id.org/i40/sto#FileSizeIEC_60870_P2_S1
sto:FileSizeIEC_60870_P2_S1 rdf:type owl:NamedIndividual .


###  https://w3id.org/i40/sto#FileSizeIEC_60870_P2_S2
sto:FileSizeIEC_60870_P2_S2 rdf:type owl:NamedIndividual .


###  https://w3id.org/i40/sto#FileSizeIEC_60870_P5_S1
sto:FileSizeIEC_60870_P5_S1 rdf:type owl:NamedIndividual .


###  https://w3id.org/i40/sto#FileSizeIEC_60870_P5_S101
sto:FileSizeIEC_60870_P5_S101 rdf:type owl:NamedIndividual .


###  https://w3id.org/i40/sto#FileSizeIEC_60870_P5_S101_2003
sto:FileSizeIEC_60870_P5_S101_2003 rdf:type owl:NamedIndividual ,
                                            om2:Measure ;
                                   om2:hasUnit om2:kilobyte ;
                                   om2:hasNumericalValue "2651.0"^^xsd:float ;
                                   rdfs:comment "Specifies the file size of the document for standard IEC 60870-5-101:2003"@en ;
                                   rdfs:label "FileSize IEC 60870-5-101:2003"@en .


###  https://w3id.org/i40/sto#FileSizeIEC_60870_P5_S102
sto:FileSizeIEC_60870_P5_S102 rdf:type owl:NamedIndividual ,
                                       om2:Measure ;
                              om2:hasUnit om2:kilobyte ;
                              om2:hasNumericalValue "505.0"^^xsd:float ;
                              rdfs:comment "Specifies the file size of the document for standard IEC 60870-5-102:1996"@en ;
                              rdfs:label "FileSize IEC 60870-5-102:1996"@en .


###  https://w3id.org/i40/sto#FileSizeIEC_60870_P5_S103
sto:FileSizeIEC_60870_P5_S103 rdf:type owl:NamedIndividual ,
                                       om2:Measure ;
                              om2:hasUnit om2:kilobyte ;
                              om2:hasNumericalValue "964.0"^^xsd:float ;
                              rdfs:comment "Specifies the file size of the document for standard IEC 60870-5-103:1997"@en ;
                              rdfs:label "FileSize IEC 60870-5-103:1997"@en .


###  https://w3id.org/i40/sto#FileSizeIEC_60870_P5_S104
sto:FileSizeIEC_60870_P5_S104 rdf:type owl:NamedIndividual ,
                                       om2:Measure ;
                              om2:hasUnit om2:kilobyte ;
                              om2:hasNumericalValue "2994.0"^^xsd:float ;
                              rdfs:comment "Specifies the file size of the document for standard IEC 60870-5-104:2006"@en ;
                              rdfs:label "FileSize IEC 60870-5-104:2006"@en .


###  https://w3id.org/i40/sto#FileSizeIEC_60870_P5_S2
sto:FileSizeIEC_60870_P5_S2 rdf:type owl:NamedIndividual .


###  https://w3id.org/i40/sto#FileSizeIEC_60870_P5_S3
sto:FileSizeIEC_60870_P5_S3 rdf:type owl:NamedIndividual .


###  https://w3id.org/i40/sto#FileSizeIEC_60870_P5_S4
sto:FileSizeIEC_60870_P5_S4 rdf:type owl:NamedIndividual ,
                                     om2:Measure ;
                            om2:hasUnit om2:kilobyte ;
                            om2:hasNumericalValue "1776.0"^^xsd:float ;
                            rdfs:comment "Specifies the file size of the document for standard IEC 60870-5-4:1993"@en ;
                            rdfs:label "FileSize IEC 60870-5-4:1993"@en .


###  https://w3id.org/i40/sto#FileSizeIEC_60870_P5_S5
sto:FileSizeIEC_60870_P5_S5 rdf:type owl:NamedIndividual ,
                                     om2:Measure ;
                            om2:hasUnit om2:kilobyte ;
                            om2:hasNumericalValue "3347.0"^^xsd:float ;
                            rdfs:comment "Specifies the file size of the document for standard IEC 60870-5-5:1995"@en ;
                            rdfs:label "FileSize IEC 60870-5-5:1995"@en .


###  https://w3id.org/i40/sto#FileSizeIEC_60870_P5_S6
sto:FileSizeIEC_60870_P5_S6 rdf:type owl:NamedIndividual ,
                                     om2:Measure ;
                            om2:hasUnit om2:kilobyte ;
                            om2:hasNumericalValue "1342.0"^^xsd:float ;
                            rdfs:comment "Specifies the file size of the document for standard IEC 60870-5-6::2006."@en ;
                            rdfs:label "FileSize IEC 60870-5-6:2006"@en .


###  https://w3id.org/i40/sto#FileSizeIEC_60870_P6_S2
sto:FileSizeIEC_60870_P6_S2 rdf:type owl:NamedIndividual ,
                                     om2:Measure ;
                            om2:hasUnit om2:kilobyte ;
                            om2:hasNumericalValue "3524.0"^^xsd:float ;
                            rdfs:comment "Specifies the file size of the document for standard IEC 60870-6-2:1995"@en ;
                            rdfs:label "FileSize IEC 60870-6-2:1995"@en .


###  https://w3id.org/i40/sto#FileSizeIEC_60870_P6_S2_1995
sto:FileSizeIEC_60870_P6_S2_1995 rdf:type owl:NamedIndividual .


###  https://w3id.org/i40/sto#FileSizeIEC_60870_P6_S501
sto:FileSizeIEC_60870_P6_S501 rdf:type owl:NamedIndividual ,
                                       om2:Measure ;
                              om2:hasUnit om2:kilobyte ;
                              om2:hasNumericalValue "578.0"^^xsd:float ;
                              rdfs:comment "Specifies the file size of the document for standard IEC 60870-6-501:1995"@en ;
                              rdfs:label "FileSize IEC 60870-6-501:1995"@en .


###  https://w3id.org/i40/sto#FileSizeIEC_60870_P6_S501_1995
sto:FileSizeIEC_60870_P6_S501_1995 rdf:type owl:NamedIndividual .


###  https://w3id.org/i40/sto#FileSizeIEC_60870_P6_S502
sto:FileSizeIEC_60870_P6_S502 rdf:type owl:NamedIndividual ,
                                       om2:Measure ;
                              om2:hasUnit om2:kilobyte ;
                              om2:hasNumericalValue "1963.0"^^xsd:float ;
                              rdfs:comment "Specifies the file size of the document for standard IEC 60870-6-502:1995"@en ;
                              rdfs:label "FileSize IEC 60870-6-502:1995"@en .


###  https://w3id.org/i40/sto#FileSizeIEC_60870_P6_S502_1995
sto:FileSizeIEC_60870_P6_S502_1995 rdf:type owl:NamedIndividual .


###  https://w3id.org/i40/sto#FileSizeIEC_60870_P6_S503
sto:FileSizeIEC_60870_P6_S503 rdf:type owl:NamedIndividual ,
                                       om2:Measure ;
                              om2:hasUnit om2:kilobyte ;
                              om2:hasNumericalValue "2630.0"^^xsd:float ;
                              rdfs:comment "Specifies the file size of the document for standard IEC 60870-6-503:2014"@en ;
                              rdfs:label "FileSize IEC 60870-6-503:2014"@en .


###  https://w3id.org/i40/sto#FileSizeIEC_60870_P6_S503_2014
sto:FileSizeIEC_60870_P6_S503_2014 rdf:type owl:NamedIndividual .


###  https://w3id.org/i40/sto#FileSizeIEC_60870_P6_S601
sto:FileSizeIEC_60870_P6_S601 rdf:type owl:NamedIndividual ,
                                       om2:Measure ;
                              om2:hasUnit om2:kilobyte ;
                              om2:hasNumericalValue "1112.0"^^xsd:float ;
                              rdfs:comment "Specifies the file size of the document for standard IEC 60870-6-601:1994"@en ;
                              rdfs:label "FileSize IEC 60870-6-601:1994"@en .


###  https://w3id.org/i40/sto#FileSizeIEC_60870_P6_S701
sto:FileSizeIEC_60870_P6_S701 rdf:type owl:NamedIndividual ,
                                       om2:Measure ;
                              om2:hasUnit om2:kilobyte ;
                              om2:hasNumericalValue "130.0"^^xsd:float ;
                              rdfs:comment "Specifies the file size of the document for standard IEC 60870-6-701:1998"@en ;
                              rdfs:label "FileSize IEC 60870-6-701:1998"@en .


###  https://w3id.org/i40/sto#FileSizeIEC_60870_P6_S702
sto:FileSizeIEC_60870_P6_S702 rdf:type owl:NamedIndividual ,
                                       om2:Measure ;
                              om2:hasUnit om2:kilobyte ;
                              om2:hasNumericalValue "1374.0"^^xsd:float ;
                              rdfs:comment "Specifies the file size of the document for standard IEC 60870-6-702:2014"@en ;
                              rdfs:label "FileSize IEC 60870-6-702:2014"@en .


###  https://w3id.org/i40/sto#FileSizeIEC_60870_P6_S802
sto:FileSizeIEC_60870_P6_S802 rdf:type owl:NamedIndividual ,
                                       om2:Measure ;
                              om2:hasUnit om2:kilobyte ;
                              om2:hasNumericalValue "1678.0"^^xsd:float ;
                              rdfs:comment "Specifies the file size of the document for standard IEC 60870-6-802:2014"@en ;
                              rdfs:label "FileSize IEC 60870-6-802:2014"@en .


###  https://w3id.org/i40/sto#FileSizeIEC_60946
sto:FileSizeIEC_60946 rdf:type owl:NamedIndividual ,
                               om2:Measure ;
                      om2:hasUnit om2:kilobyte ;
                      om2:hasNumericalValue "546.0"^^xsd:float ;
                      rdfs:comment "Specifies the file size of the document for standard IEC 60946"@en ;
                      rdfs:label "FileSize IEC 60946"@en .


###  https://w3id.org/i40/sto#FileSizeIEC_61000_P6_S2
sto:FileSizeIEC_61000_P6_S2 rdf:type owl:NamedIndividual ,
                                     om2:Measure ;
                            om2:hasUnit om2:kilobyte ;
                            om2:hasNumericalValue "2028.0"^^xsd:float ;
                            rdfs:comment "Specifies the file size of the document for standard IEC 61000-6-2:2016."@en ;
                            rdfs:label "FileSize IEC 61000-6-2:2016"@en .


###  https://w3id.org/i40/sto#FileSizeIEC_61010_P2_S012
sto:FileSizeIEC_61010_P2_S012 rdf:type owl:NamedIndividual ,
                                       om2:Measure ;
                              om2:hasUnit om2:kilobyte ;
                              om2:hasNumericalValue "2717.0"^^xsd:float ;
                              rdfs:comment "Specifies the file size of the document for standard IEC 61010-2-012:2016."@en ;
                              rdfs:label "FileSize IEC 61010-2-012:2016"@en .


###  https://w3id.org/i40/sto#FileSizeIEC_61010_P2_S201
sto:FileSizeIEC_61010_P2_S201 rdf:type owl:NamedIndividual ,
                                       om2:Measure ;
                              om2:hasUnit om2:kilobyte ;
                              om2:hasNumericalValue "5743.0"^^xsd:float ;
                              rdfs:comment "Specifies the file size of the document for standard IEC 61010-2-201:2017."@en ;
                              rdfs:label "FileSize IEC 61010-2-201:2017"@en .


###  https://w3id.org/i40/sto#FileSizeIEC_61010_P2_S202
sto:FileSizeIEC_61010_P2_S202 rdf:type owl:NamedIndividual ,
                                       om2:Measure ;
                              om2:hasUnit om2:kilobyte ;
                              om2:hasNumericalValue "1027.0"^^xsd:float ;
                              rdfs:comment "Specifies the file size of the document for standard IEC 61010-2-202:2016."@en ;
                              rdfs:label "FileSize IEC 61010-2-202:2016"@en .


###  https://w3id.org/i40/sto#FileSizeIEC_61160
sto:FileSizeIEC_61160 rdf:type owl:NamedIndividual ,
                               om2:Measure ;
                      om2:hasUnit om2:kilobyte ;
                      om2:hasNumericalValue "69.0"^^xsd:float ;
                      rdfs:comment "Specifies the file size of the document for standard  IEC 61160:2005."@en ;
                      rdfs:label "FileSize IEC 61160:2005"@en .


###  https://w3id.org/i40/sto#FileSizeIEC_61310_P1
sto:FileSizeIEC_61310_P1 rdf:type owl:NamedIndividual ,
                                  om2:Measure ;
                         om2:hasUnit om2:kilobyte ;
                         om2:hasNumericalValue "763.0"^^xsd:float ;
                         rdfs:comment "Specifies the file size of the document for standard IEC 61310-1:2007."@en ;
                         rdfs:label "FileSize IEC 61310-1:2007"@en .


###  https://w3id.org/i40/sto#FileSizeIEC_61310_P2
sto:FileSizeIEC_61310_P2 rdf:type owl:NamedIndividual ,
                                  om2:Measure ;
                         om2:hasUnit om2:kilobyte ;
                         om2:hasNumericalValue "724.0"^^xsd:float ;
                         rdfs:comment "Specifies the file size of the document for standard IEC 61310-2:2007."@en ;
                         rdfs:label "FileSize IEC 61310-2:2007"@en .


###  https://w3id.org/i40/sto#FileSizeIEC_61310_P3
sto:FileSizeIEC_61310_P3 rdf:type owl:NamedIndividual ,
                                  om2:Measure ;
                         om2:hasUnit om2:kilobyte ;
                         om2:hasNumericalValue "716.0"^^xsd:float ;
                         rdfs:comment "Specifies the file size of the document for standard IEC 61310-3:2007."@en ;
                         rdfs:label "FileSize IEC 61310-3:2007"@en .


###  https://w3id.org/i40/sto#FileSizeIEC_61334_1996_P4_S32
sto:FileSizeIEC_61334_1996_P4_S32 rdf:type owl:NamedIndividual ,
                                           om2:Measure ;
                                  om2:hasUnit om2:kilobyte ;
                                  om2:hasNumericalValue "869.0"^^xsd:float ;
                                  rdfs:comment "Specifies the file size of the document for standard IEC 61334-4-32:1996 "@en ;
                                  rdfs:label "FileSize IEC 61334-4-32:1996 "@en .


###  https://w3id.org/i40/sto#FileSizeIEC_61334_1998_P3_S1
sto:FileSizeIEC_61334_1998_P3_S1 rdf:type owl:NamedIndividual ,
                                          om2:Measure ;
                                 om2:hasUnit om2:kilobyte ;
                                 om2:hasNumericalValue "147.0"^^xsd:float ;
                                 rdfs:comment "Specifies the file size of the document for standard IEC 61334-3-1:1998 "@en ;
                                 rdfs:label "FileSize IEC 61334-3-1:1998 "@en .


###  https://w3id.org/i40/sto#FileSizeIEC_61334_1998_P4_S3
sto:FileSizeIEC_61334_1998_P4_S3 rdf:type owl:NamedIndividual ,
                                          om2:Measure ;
                                 om2:hasUnit om2:kilobyte ;
                                 om2:hasNumericalValue "135.0"^^xsd:float ;
                                 rdfs:comment "Specifies the file size of the document for standard IEC 61334-4-33:1998 "@en ;
                                 rdfs:label "FileSize IEC 61334-4-33:1998"@en .


###  https://w3id.org/i40/sto#FileSizeIEC_61334_1998_P4_S61
sto:FileSizeIEC_61334_1998_P4_S61 rdf:type owl:NamedIndividual ,
                                           om2:Measure ;
                                  om2:hasUnit om2:kilobyte ;
                                  om2:hasNumericalValue "753.0"^^xsd:float ;
                                  rdfs:comment "Specifies the file size of the document for standard IEC 61334-4-61:1998"@en ;
                                  rdfs:label "FileSize IEC 61334-4-61:1998"@en .


###  https://w3id.org/i40/sto#FileSizeIEC_61334_2001_P4_S512
sto:FileSizeIEC_61334_2001_P4_S512 rdf:type owl:NamedIndividual ,
                                            om2:Measure ;
                                   om2:hasUnit om2:kilobyte ;
                                   om2:hasNumericalValue "459.0"^^xsd:float ;
                                   rdfs:comment "Specifies the file size of the document for standard IEC 61334-4-512:2001"@en ;
                                   rdfs:label "FileSize IEC 61334-4-512:2001"@en .


###  https://w3id.org/i40/sto#FileSizeIEC_61334_2001_P5_S1
sto:FileSizeIEC_61334_2001_P5_S1 rdf:type owl:NamedIndividual ,
                                          om2:Measure ;
                                 om2:hasUnit om2:kilobyte ;
                                 om2:hasNumericalValue "723.0"^^xsd:float ;
                                 rdfs:comment "Specifies the file size of the document for standard IEC 61334-5-1:2001"@en ;
                                 rdfs:label "FileSize IEC 61334-5-1:2001"@en .


###  https://w3id.org/i40/sto#FileSizeIEC_61334_P3_S1
sto:FileSizeIEC_61334_P3_S1 rdf:type owl:NamedIndividual ,
                                     om2:Measure ;
                            om2:hasUnit om2:kilobyte ;
                            om2:hasNumericalValue "147.0"^^xsd:float ;
                            rdfs:comment "Specifies the file size of the document for standard IEC 61334-3-1:1998 "@en ;
                            rdfs:label "FileSize IEC 61334-3-1:1998 "@en .


###  https://w3id.org/i40/sto#FileSizeIEC_61334_P3_S21
sto:FileSizeIEC_61334_P3_S21 rdf:type owl:NamedIndividual ,
                                      om2:Measure ;
                             om2:hasUnit om2:kilobyte ;
                             om2:hasNumericalValue "1112.0"^^xsd:float ;
                             rdfs:comment "Specifies the file size of the document for standard IEC 61334-3-21:1996 "@en ;
                             rdfs:label "FileSize IEC 61334-3-21:1996 "@en .


###  https://w3id.org/i40/sto#FileSizeIEC_61334_P3_S22
sto:FileSizeIEC_61334_P3_S22 rdf:type owl:NamedIndividual ,
                                      om2:Measure ;
                             om2:hasUnit om2:kilobyte ;
                             om2:hasNumericalValue "165.0"^^xsd:float ;
                             rdfs:comment "Specifies the file size of the document for standard IEC 61334-3-22:2001"@en ;
                             rdfs:label "FileSize IEC 61334-3-22:2001"@en .


###  https://w3id.org/i40/sto#FileSizeIEC_61334_P4_S1
sto:FileSizeIEC_61334_P4_S1 rdf:type owl:NamedIndividual ,
                                     om2:Measure ;
                            om2:hasUnit om2:kilobyte ;
                            om2:hasNumericalValue "1707.0"^^xsd:float ;
                            rdfs:comment "Specifies the file size of the document for standard IEC 61334-4-1:1996"@en ;
                            rdfs:label "FileSize IEC 61334-3-22:2000"@en .


###  https://w3id.org/i40/sto#FileSizeIEC_61334_P4_S3
sto:FileSizeIEC_61334_P4_S3 rdf:type owl:NamedIndividual .


###  https://w3id.org/i40/sto#FileSizeIEC_61334_P4_S32
sto:FileSizeIEC_61334_P4_S32 rdf:type owl:NamedIndividual ,
                                      om2:Measure ;
                             om2:hasUnit om2:kilobyte ;
                             om2:hasNumericalValue "869.0"^^xsd:float ;
                             rdfs:comment "Specifies the file size of the document for standard IEC 61334-4-32:1996 "@en ;
                             rdfs:label "FileSize IEC 61334-4-32:1996 "@en .


###  https://w3id.org/i40/sto#FileSizeIEC_61334_P4_S33
sto:FileSizeIEC_61334_P4_S33 rdf:type owl:NamedIndividual ,
                                      om2:Measure ;
                             om2:hasUnit om2:kilobyte ;
                             om2:hasNumericalValue "135.0"^^xsd:float ;
                             rdfs:comment "Specifies the file size of the document for standard IEC 61334-4-33:1998 "@en ;
                             rdfs:label "FileSize IEC 61334-4-33:1998"@en .


###  https://w3id.org/i40/sto#FileSizeIEC_61334_P4_S41
sto:FileSizeIEC_61334_P4_S41 rdf:type owl:NamedIndividual ,
                                      om2:Measure ;
                             om2:hasUnit om2:kilobyte ;
                             om2:hasNumericalValue "834.0"^^xsd:float ;
                             rdfs:comment "Specifies the file size of the document for standard IEC 61334-4-41:1996"@en ;
                             rdfs:label "FileSize IEC 61334-4-41:1996"@en .


###  https://w3id.org/i40/sto#FileSizeIEC_61334_P4_S42
sto:FileSizeIEC_61334_P4_S42 rdf:type owl:NamedIndividual ,
                                      om2:Measure ;
                             om2:hasUnit om2:kilobyte ;
                             om2:hasNumericalValue "305.0"^^xsd:float ;
                             rdfs:comment "Specifies the file size of the document for standard IEC 61334-4-42:1996"@en ;
                             rdfs:label "FileSize IEC 61334-4-42:1996"@en .


###  https://w3id.org/i40/sto#FileSizeIEC_61334_P4_S511
sto:FileSizeIEC_61334_P4_S511 rdf:type owl:NamedIndividual ,
                                       om2:Measure ;
                              om2:hasUnit om2:kilobyte ;
                              om2:hasNumericalValue "203.0"^^xsd:float ;
                              rdfs:comment "Specifies the file size of the document for standard IEC 61334-4-511:2000"@en ;
                              rdfs:label "FileSize IEC 61334-4-511:2000"@en .


###  https://w3id.org/i40/sto#FileSizeIEC_61334_P4_S512
sto:FileSizeIEC_61334_P4_S512 rdf:type owl:NamedIndividual ,
                                       om2:Measure ;
                              om2:hasUnit om2:kilobyte ;
                              om2:hasNumericalValue "459.0"^^xsd:float ;
                              rdfs:comment "Specifies the file size of the document for standard IEC 61334-4-512:2001"@en ;
                              rdfs:label "FileSize IEC 61334-4-512:2001"@en .


###  https://w3id.org/i40/sto#FileSizeIEC_61334_P4_S61
sto:FileSizeIEC_61334_P4_S61 rdf:type owl:NamedIndividual ,
                                      om2:Measure ;
                             om2:hasUnit om2:kilobyte ;
                             om2:hasNumericalValue "753.0"^^xsd:float ;
                             rdfs:comment "Specifies the file size of the document for standard IEC 61334-4-61:1998"@en ;
                             rdfs:label "FileSize IEC 61334-4-61:1998"@en .


###  https://w3id.org/i40/sto#FileSizeIEC_61334_P5_S1
sto:FileSizeIEC_61334_P5_S1 rdf:type owl:NamedIndividual ,
                                     om2:Measure ;
                            om2:hasUnit om2:kilobyte ;
                            om2:hasNumericalValue "723.0"^^xsd:float ;
                            rdfs:comment "Specifies the file size of the document for standard IEC 61334-5-1:2001"@en ;
                            rdfs:label "FileSize IEC 61334-5-1:2001"@en .


###  https://w3id.org/i40/sto#FileSizeIEC_61334_P6
sto:FileSizeIEC_61334_P6 rdf:type owl:NamedIndividual ,
                                  om2:Measure ;
                         om2:hasUnit om2:kilobyte ;
                         om2:hasNumericalValue "294.0"^^xsd:float ;
                         rdfs:comment "Specifies the file size of the document for standard IEC 61334-6:2000"@en ;
                         rdfs:label "FileSize IEC 61334-6:2000"@en .


###  https://w3id.org/i40/sto#FileSizeIEC_61400_P25_S1
sto:FileSizeIEC_61400_P25_S1 rdf:type owl:NamedIndividual ,
                                      om2:Measure ;
                             om2:hasUnit om2:kilobyte ;
                             om2:hasNumericalValue "3644.0"^^xsd:float ;
                             rdfs:comment "Specifies the file size of the document for standard  IEC 61400-25-1:2017."@en ;
                             rdfs:label "FileSize IEC 61400-25-1:2017"@en .


###  https://w3id.org/i40/sto#FileSizeIEC_61400_P25_S2
sto:FileSizeIEC_61400_P25_S2 rdf:type owl:NamedIndividual ,
                                      om2:Measure ;
                             om2:hasUnit om2:kilobyte ;
                             om2:hasNumericalValue "3707.0"^^xsd:float ;
                             rdfs:comment "Specifies the file size of the document for standard IEC 61400-25-2:2015."@en ;
                             rdfs:label "FileSize IEC 61400-25-2:2015"@en .


###  https://w3id.org/i40/sto#FileSizeIEC_61400_P25_S3
sto:FileSizeIEC_61400_P25_S3 rdf:type owl:NamedIndividual ,
                                      om2:Measure ;
                             om2:hasUnit om2:kilobyte ;
                             om2:hasNumericalValue "2027.0"^^xsd:float ;
                             rdfs:comment "Specifies the file size of the document for standard IEC 61400-25-3:2015."@en ;
                             rdfs:label "FileSize IEC 61400-25-3:2015"@en .


###  https://w3id.org/i40/sto#FileSizeIEC_61400_P25_S4
sto:FileSizeIEC_61400_P25_S4 rdf:type owl:NamedIndividual ,
                                      om2:Measure ;
                             om2:hasUnit om2:kilobyte ;
                             om2:hasNumericalValue "7800.0"^^xsd:float ;
                             rdfs:comment "Specifies the file size of the document for standard IEC 61400-25-4:2016."@en ;
                             rdfs:label "FileSize IEC 61400-25-4:2016"@en .


###  https://w3id.org/i40/sto#FileSizeIEC_61400_P25_S5
sto:FileSizeIEC_61400_P25_S5 rdf:type owl:NamedIndividual ,
                                      om2:Measure ;
                             om2:hasUnit om2:kilobyte ;
                             om2:hasNumericalValue "1567.0"^^xsd:float ;
                             rdfs:comment "Specifies the file size of the document for standard IEC 61400-25-5:2017."@en ;
                             rdfs:label "FileSize IEC 61400-25-5:2017"@en .


###  https://w3id.org/i40/sto#FileSizeIEC_61400_P25_S6
sto:FileSizeIEC_61400_P25_S6 rdf:type owl:NamedIndividual ,
                                      om2:Measure ;
                             om2:hasUnit om2:kilobyte ;
                             om2:hasNumericalValue "1673.0"^^xsd:float ;
                             rdfs:comment "Specifies the file size of the document for standard IEC 61400-25-5:2017."@en ;
                             rdfs:label "FileSize IEC 61400-25-6:2016"@en .


###  https://w3id.org/i40/sto#FileSizeIEC_61506
sto:FileSizeIEC_61506 rdf:type owl:NamedIndividual ,
                               om2:Measure ;
                      om2:hasUnit om2:kilobyte ;
                      om2:hasNumericalValue "294.0"^^xsd:float ;
                      rdfs:comment "Specifies the file size of the document for standard  IEC 61506:1997."@en ;
                      rdfs:label "FileSize IEC 61506:1997"@en .


###  https://w3id.org/i40/sto#FileSizeIEC_61690_P1
sto:FileSizeIEC_61690_P1 rdf:type owl:NamedIndividual ,
                                  om2:Measure ;
                         om2:hasUnit om2:kilobyte ;
                         om2:hasNumericalValue "1676.0"^^xsd:float ;
                         rdfs:comment "Specifies the file size of the document for standard IEC 61690-1:2000 ."@en ;
                         rdfs:label "FileSize IEC 61690-1:2000 "@en .


###  https://w3id.org/i40/sto#FileSizeIEC_61690_P2
sto:FileSizeIEC_61690_P2 rdf:type owl:NamedIndividual ,
                                  om2:Measure ;
                         om2:hasUnit om2:kilobyte ;
                         om2:hasNumericalValue "6700.0"^^xsd:float ;
                         rdfs:comment "Specifies the file size of the document for standard IEC 61690-2:2000 ."@en ;
                         rdfs:label "FileSize IEC 61690-2:2000 "@en .


###  https://w3id.org/i40/sto#FileSizeIEC_61691_P6
sto:FileSizeIEC_61691_P6 rdf:type owl:NamedIndividual ,
                                  om2:Measure ;
                         om2:hasUnit om2:kilobyte ;
                         om2:hasNumericalValue "5004.0"^^xsd:float ;
                         rdfs:comment "Specifies the file size of the document for standard IEC 61691-6:2009."@en ;
                         rdfs:label "FileSize IEC 61691-6:2009"@en .


###  https://w3id.org/i40/sto#FileSizeIEC_61804_P1
sto:FileSizeIEC_61804_P1 rdf:type owl:NamedIndividual ,
                                  om2:Measure ;
                         om2:hasUnit om2:kilobyte ;
                         om2:hasNumericalValue "977.0"^^xsd:float ;
                         rdfs:comment "Specifies the file size of the document for standard IEC 61804-6:2012 "@en ;
                         rdfs:label "FileSize IEC 61804-6:2012  "@en .


###  https://w3id.org/i40/sto#FileSizeIEC_61804_P3
sto:FileSizeIEC_61804_P3 rdf:type owl:NamedIndividual ,
                                  om2:Measure ;
                         om2:hasUnit om2:kilobyte ;
                         om2:hasNumericalValue "9306.0"^^xsd:float ;
                         rdfs:comment "Specifies the file size of the document for standard IEC 61804-3:2015"@en ;
                         rdfs:label "FileSize IEC 61804-3:2015"@en .


###  https://w3id.org/i40/sto#FileSizeIEC_61804_P4
sto:FileSizeIEC_61804_P4 rdf:type owl:NamedIndividual ,
                                  om2:Measure ;
                         om2:hasUnit om2:kilobyte ;
                         om2:hasNumericalValue "3514.0"^^xsd:float ;
                         rdfs:comment "Specifies the file size of the document for standard IEC 61804-4:2015"@en ;
                         rdfs:label "FileSize IEC 61804-4:2015"@en .


###  https://w3id.org/i40/sto#FileSizeIEC_61804_P5
sto:FileSizeIEC_61804_P5 rdf:type owl:NamedIndividual ,
                                  om2:Measure ;
                         om2:hasUnit om2:kilobyte ;
                         om2:hasNumericalValue "7931.0"^^xsd:float ;
                         rdfs:comment "Specifies the file size of the document for standard IEC 61804-5:2015 "@en ;
                         rdfs:label "FileSize IEC 61804-5:2015 "@en .


###  https://w3id.org/i40/sto#FileSizeIEC_61804_P6
sto:FileSizeIEC_61804_P6 rdf:type owl:NamedIndividual .


###  https://w3id.org/i40/sto#FileSizeIEC_61810_P2
sto:FileSizeIEC_61810_P2 rdf:type owl:NamedIndividual ,
                                  om2:Measure ;
                         om2:hasUnit om2:kilobyte ;
                         om2:hasNumericalValue "4364.0"^^xsd:float ;
                         rdfs:comment "Specifies the file size of the document for standard IEC 61810-2:2017."@en ;
                         rdfs:label "FileSize IEC 61810-2:2017"@en .


###  https://w3id.org/i40/sto#FileSizeIEC_61810_P7
sto:FileSizeIEC_61810_P7 rdf:type owl:NamedIndividual ,
                                  om2:Measure ;
                         om2:hasUnit om2:kilobyte ;
                         om2:hasNumericalValue "2204.0"^^xsd:float ;
                         rdfs:comment "Specifies the file size of the document for standard IEC 61810-7:2006."@en ;
                         rdfs:label "FileSize IEC 61810-7:2006"@en .


###  https://w3id.org/i40/sto#FileSizeIEC_61850_P10_E1
sto:FileSizeIEC_61850_P10_E1 rdf:type owl:NamedIndividual ,
                                      om2:Measure ;
                             om2:hasUnit om2:kilobyte ;
                             om2:hasNumericalValue "452.0"^^xsd:float ;
                             rdfs:comment "Specifies the file size of the document for standard IEC 61850-10:2005 ."@en ;
                             rdfs:label "FileSize IEC 61850-10:2005 "@en .


###  https://w3id.org/i40/sto#FileSizeIEC_61850_P10_E2
sto:FileSizeIEC_61850_P10_E2 rdf:type owl:NamedIndividual ,
                                      om2:Measure ;
                             om2:hasUnit om2:kilobyte ;
                             om2:hasNumericalValue "2121.0"^^xsd:float ;
                             rdfs:comment "Specifies the file size of the document for standard IEC 61850-10:2012."@en ;
                             rdfs:label "FileSize IEC 61850-10:2012 "@en .


###  https://w3id.org/i40/sto#FileSizeIEC_61850_P4_E1
sto:FileSizeIEC_61850_P4_E1 rdf:type owl:NamedIndividual ,
                                     om2:Measure ;
                            om2:hasUnit om2:kilobyte ;
                            om2:hasNumericalValue "444.0"^^xsd:float ;
                            rdfs:comment "Specifies the file size of the document for standard IEC 61850-4:2002 ."@en ;
                            rdfs:label "FileSize IEC 61850-4:2002 "@en .


###  https://w3id.org/i40/sto#FileSizeIEC_61850_P4_E2
sto:FileSizeIEC_61850_P4_E2 rdf:type owl:NamedIndividual ,
                                     om2:Measure ;
                            om2:hasUnit om2:kilobyte ;
                            om2:hasNumericalValue "1250.0"^^xsd:float ;
                            rdfs:comment "Specifies the file size of the document for standard IEC 61850-4:2011 ."@en ;
                            rdfs:label "FileSize IEC 61850-4:2011 "@en .


###  https://w3id.org/i40/sto#FileSizeIEC_61850_P7_S1_E1
sto:FileSizeIEC_61850_P7_S1_E1 rdf:type owl:NamedIndividual ,
                                        om2:Measure ;
                               om2:hasUnit om2:kilobyte ;
                               om2:hasNumericalValue "4106.0"^^xsd:float ;
                               rdfs:comment "Specifies the file size of the document for standard IEC 61850-7-1:2003 ."@en ;
                               rdfs:label "FileSize IEC 61850-7-1:2003 "@en .


###  https://w3id.org/i40/sto#FileSizeIEC_61850_P7_S1_E2
sto:FileSizeIEC_61850_P7_S1_E2 rdf:type owl:NamedIndividual ,
                                        om2:Measure ;
                               om2:hasUnit om2:kilobyte ;
                               om2:hasNumericalValue "8338.0"^^xsd:float ;
                               rdfs:comment "Specifies the file size of the document for standard IEC 61850-7-1:2011 ."@en ;
                               rdfs:label "FileSize IEC 61850-7-1:2011 "@en .


###  https://w3id.org/i40/sto#FileSizeIEC_61850_P7_S2_E1
sto:FileSizeIEC_61850_P7_S2_E1 rdf:type owl:NamedIndividual ,
                                        om2:Measure ;
                               om2:hasUnit om2:kilobyte ;
                               om2:hasNumericalValue "3596.0"^^xsd:float ;
                               rdfs:comment "Specifies the file size of the document for standard IEC 61850-7-2:2003 ."@en ;
                               rdfs:label "FileSize IEC 61850-7-2:2003 "@en .


###  https://w3id.org/i40/sto#FileSizeIEC_61850_P7_S2_E2
sto:FileSizeIEC_61850_P7_S2_E2 rdf:type owl:NamedIndividual ,
                                        om2:Measure ;
                               om2:hasUnit om2:kilobyte ;
                               om2:hasNumericalValue "2286.0"^^xsd:float ;
                               rdfs:comment "Specifies the file size of the document for standard IEC 61850-7-2:2010."@en ;
                               rdfs:label "FileSize IEC 61850-7-2:2010 "@en .


###  https://w3id.org/i40/sto#FileSizeIEC_61850_P7_S3_E1
sto:FileSizeIEC_61850_P7_S3_E1 rdf:type owl:NamedIndividual ,
                                        om2:Measure ;
                               om2:hasUnit om2:kilobyte ;
                               om2:hasNumericalValue "3236.0"^^xsd:float ;
                               rdfs:comment "Specifies the file size of the document for standard IEC 61850-7-3:2003 ."@en ;
                               rdfs:label "FileSize IEC 61850-7-3:2003 "@en .


###  https://w3id.org/i40/sto#FileSizeIEC_61850_P7_S3_E2
sto:FileSizeIEC_61850_P7_S3_E2 rdf:type owl:NamedIndividual ,
                                        om2:Measure ;
                               om2:hasUnit om2:kilobyte ;
                               om2:hasNumericalValue "2043.0"^^xsd:float ;
                               rdfs:comment "Specifies the file size of the document for standard IEC 61850-7-3:2010."@en ;
                               rdfs:label "FileSize IEC 61850-7-3:2010 "@en .


###  https://w3id.org/i40/sto#FileSizeIEC_61850_P7_S420_E1
sto:FileSizeIEC_61850_P7_S420_E1 rdf:type owl:NamedIndividual ,
                                          om2:Measure ;
                                 om2:hasUnit om2:kilobyte ;
                                 om2:hasNumericalValue "2026.0"^^xsd:float ;
                                 rdfs:comment "Specifies the file size of the document for standard IEC 61850-7-420:2009."@en ;
                                 rdfs:label "FileSize IEC 61850-7-420:2009 "@en .


###  https://w3id.org/i40/sto#FileSizeIEC_61850_P7_S4_E1
sto:FileSizeIEC_61850_P7_S4_E1 rdf:type owl:NamedIndividual ,
                                        om2:Measure ;
                               om2:hasUnit om2:kilobyte ;
                               om2:hasNumericalValue "3475.0"^^xsd:float ;
                               rdfs:comment "Specifies the file size of the document for standard IEC 61850-7-4:2003 ."@en ;
                               rdfs:label "FileSize IEC 61850-7-4:2003 "@en .


###  https://w3id.org/i40/sto#FileSizeIEC_61850_P7_S4_E2
sto:FileSizeIEC_61850_P7_S4_E2 rdf:type owl:NamedIndividual ,
                                        om2:Measure ;
                               om2:hasUnit om2:kilobyte ;
                               om2:hasNumericalValue "4326.0"^^xsd:float ;
                               rdfs:comment "Specifies the file size of the document for standard IEC 61850-7-4:2010."@en ;
                               rdfs:label "FileSize IEC 61850-7-4:2010 "@en .

sto:FileSizeIEC_61850_P8_S1_E2 rdf:type owl:NamedIndividual ,
                                        om2:Measure ;
                               om2:hasUnit om2:kilobyte ;
                               om2:hasNumericalValue "3365.0"^^xsd:float ;
                               rdfs:comment "Specifies the file size of the document for standard IEC 61850-8-1:2011."@en ;
                               rdfs:label "FileSize IEC 61850-8-1:2011 "@en .


###  https://w3id.org/i40/sto#FileSizeIEC_61968_P3_E1
sto:FileSizeIEC_61968_P3_E1 rdf:type owl:NamedIndividual ,
                                     om2:Measure ;
                            om2:hasUnit om2:kilobyte ;
                            om2:hasNumericalValue "601.0"^^xsd:float ;
                            rdfs:comment "Specifies the file size of the document for standard IEC 61968-3:2004 ."@en ;
                            rdfs:label "FileSize IEC 61968-3:2004 "@en .


###  https://w3id.org/i40/sto#FileSizeIEC_61968_P3_E2
sto:FileSizeIEC_61968_P3_E2 rdf:type owl:NamedIndividual ,
                                     om2:Measure ;
                            om2:hasUnit om2:kilobyte ;
                            om2:hasNumericalValue "8270.0"^^xsd:float ;
                            rdfs:comment "Specifies the file size of the document for standard IEC 61968-3:2017."@en ;
                            rdfs:label "FileSize IEC 61968-3:2017 "@en .


###  https://w3id.org/i40/sto#FileSizeIEC_61968_P4_E1
sto:FileSizeIEC_61968_P4_E1 rdf:type owl:NamedIndividual ,
                                     om2:Measure ;
                            om2:hasUnit om2:kilobyte ;
                            om2:hasNumericalValue "3106.0"^^xsd:float ;
                            rdfs:comment "Specifies the file size of the document for standard IEC 61968-4:2007."@en ;
                            rdfs:label "FileSize IEC 61968-4:2007 "@en .


###  https://w3id.org/i40/sto#FileSizeIEC_61968_P4_E2
sto:FileSizeIEC_61968_P4_E2 rdf:type owl:NamedIndividual ,
                                     om2:Measure ;
                            om2:hasUnit om2:kilobyte ;
                            om2:hasNumericalValue "8173.0"^^xsd:float ;
                            rdfs:comment "Specifies the file size of the document for standard IEC 61968-4:2018 PRV."@en ;
                            rdfs:label "FileSize IEC 61968-4:2018 PRV "@en .


###  https://w3id.org/i40/sto#FileSizeIEC_61968_P6_E1
sto:FileSizeIEC_61968_P6_E1 rdf:type owl:NamedIndividual ,
                                     om2:Measure ;
                            om2:hasUnit om2:kilobyte ;
                            om2:hasNumericalValue "4059.0"^^xsd:float ;
                            rdfs:comment "Specifies the file size of the document for standard IEC 61968-6:2015."@en ;
                            rdfs:label "FileSize IEC 61968-6:2015 "@en .


###  https://w3id.org/i40/sto#FileSizeIEC_61968_P8_E1
sto:FileSizeIEC_61968_P8_E1 rdf:type owl:NamedIndividual ,
                                     om2:Measure ;
                            om2:hasUnit om2:kilobyte ;
                            om2:hasNumericalValue "2555.0"^^xsd:float ;
                            rdfs:comment "Specifies the file size of the document for standard IEC 61968-8:2015 ."@en ;
                            rdfs:label "FileSize IEC 61968-8:2015  "@en .


###  https://w3id.org/i40/sto#FileSizeIEC_61968_P9_E1
sto:FileSizeIEC_61968_P9_E1 rdf:type owl:NamedIndividual ,
                                     om2:Measure ;
                            om2:hasUnit om2:kilobyte ;
                            om2:hasNumericalValue "2745.0"^^xsd:float ;
                            rdfs:comment "Specifies the file size of the document for standard IEC 61968-9:2009."@en ;
                            rdfs:label "FileSize IEC 61968-9:2009 "@en .


###  https://w3id.org/i40/sto#FileSizeIEC_61968_P9_E2
sto:FileSizeIEC_61968_P9_E2 rdf:type owl:NamedIndividual ,
                                     om2:Measure ;
                            om2:hasUnit om2:kilobyte ;
                            om2:hasNumericalValue "6943.0"^^xsd:float ;
                            rdfs:comment "Specifies the file size of the document for standard IEC 61968-9:2013."@en ;
                            rdfs:label "FileSize IEC 61968-9:2013 "@en .


###  https://w3id.org/i40/sto#FileSizeIEC_61970_P1_E1
sto:FileSizeIEC_61970_P1_E1 rdf:type owl:NamedIndividual ,
                                     om2:Measure ;
                            om2:hasUnit om2:kilobyte ;
                            om2:hasNumericalValue "707.0"^^xsd:float ;
                            rdfs:comment "Specifies the file size of the document for standard IEC 61970-1:2005 ."@en ;
                            rdfs:label "FileSize IEC 61970-1:2005  "@en .


###  https://w3id.org/i40/sto#FileSizeIEC_61970_P301_E1
sto:FileSizeIEC_61970_P301_E1 rdf:type owl:NamedIndividual ,
                                       om2:Measure ;
                              om2:hasUnit om2:kilobyte ;
                              om2:hasNumericalValue "2709.0"^^xsd:float ;
                              rdfs:comment "Specifies the file size of the document for standard IEC 61970-301:2003."@en ;
                              rdfs:label "FileSize IEC 61970-301:2003 "@en .


###  https://w3id.org/i40/sto#FileSizeIEC_61970_P301_E2
sto:FileSizeIEC_61970_P301_E2 rdf:type owl:NamedIndividual ,
                                       om2:Measure ;
                              om2:hasUnit om2:kilobyte ;
                              om2:hasNumericalValue "2348.0"^^xsd:float ;
                              rdfs:comment "Specifies the file size of the document for standard IEC 61970-301:2009."@en ;
                              rdfs:label "FileSize IEC 61970-301:2009 "@en .


###  https://w3id.org/i40/sto#FileSizeIEC_61970_P301_E3
sto:FileSizeIEC_61970_P301_E3 rdf:type owl:NamedIndividual ,
                                       om2:Measure ;
                              om2:hasUnit om2:kilobyte ;
                              om2:hasNumericalValue "4841.0"^^xsd:float ;
                              rdfs:comment "Specifies the file size of the document for standard IEC 61970-301:2011."@en ;
                              rdfs:label "FileSize IEC 61970-301:2011 "@en .


###  https://w3id.org/i40/sto#FileSizeIEC_61970_P301_E4
sto:FileSizeIEC_61970_P301_E4 rdf:type owl:NamedIndividual ,
                                       om2:Measure ;
                              om2:hasUnit om2:kilobyte ;
                              om2:hasNumericalValue "5466.0"^^xsd:float ;
                              rdfs:comment "Specifies the file size of the document for standard IEC 61970-301:2013."@en ;
                              rdfs:label "FileSize IEC 61970-301:2013 "@en .


###  https://w3id.org/i40/sto#FileSizeIEC_61970_P301_E5
sto:FileSizeIEC_61970_P301_E5 rdf:type owl:NamedIndividual ,
                                       om2:Measure ;
                              om2:hasUnit om2:kilobyte ;
                              om2:hasNumericalValue "8022.0"^^xsd:float ;
                              rdfs:comment "Specifies the file size of the document for standard IEC 61970-301:2013."@en ;
                              rdfs:label "FileSize IEC 61970-301:2013 "@en .


###  https://w3id.org/i40/sto#FileSizeIEC_61970_P301_E6
sto:FileSizeIEC_61970_P301_E6 rdf:type owl:NamedIndividual ,
                                       om2:Measure ;
                              om2:hasUnit om2:kilobyte ;
                              om2:hasNumericalValue "17830.0"^^xsd:float ;
                              rdfs:comment "Specifies the file size of the document for standard IEC 61970-301:2016."@en ;
                              rdfs:label "FileSize IEC 61970-301:2016 "@en .


###  https://w3id.org/i40/sto#FileSizeIEC_61970_P301_E6_RLV
sto:FileSizeIEC_61970_P301_E6_RLV rdf:type owl:NamedIndividual ,
                                           om2:Measure ;
                                  om2:hasUnit om2:kilobyte ;
                                  om2:hasNumericalValue "24554.0"^^xsd:float ;
                                  rdfs:comment "Specifies the file size of the document for standard IEC 61970-301:2016 RLV Redline version."@en ;
                                  rdfs:label "FileSize IEC 61970-301:2016 RLV Redline version "@en .


###  https://w3id.org/i40/sto#FileSizeIEC_61970_P452_E1
sto:FileSizeIEC_61970_P452_E1 rdf:type owl:NamedIndividual ,
                                       om2:Measure ;
                              om2:hasUnit om2:kilobyte ;
                              om2:hasNumericalValue "2015.0"^^xsd:float ;
                              rdfs:comment "Specifies the file size of the document for standard IEC 61970-452:2013."@en ;
                              rdfs:label "FileSize IEC 61970-452:2013 "@en .


###  https://w3id.org/i40/sto#FileSizeIEC_61970_P452_E2
sto:FileSizeIEC_61970_P452_E2 rdf:type owl:NamedIndividual ,
                                       om2:Measure ;
                              om2:hasUnit om2:kilobyte ;
                              om2:hasNumericalValue "2238.0"^^xsd:float ;
                              rdfs:comment "Specifies the file size of the document for standard IEC 61970-452:2015."@en ;
                              rdfs:label "FileSize IEC 61970-452:2015 "@en .


###  https://w3id.org/i40/sto#FileSizeIEC_61970_P452_E3
sto:FileSizeIEC_61970_P452_E3 rdf:type owl:NamedIndividual ,
                                       om2:Measure ;
                              om2:hasUnit om2:kilobyte ;
                              om2:hasNumericalValue "1533.0"^^xsd:float ,
                                                    "4157.0"^^xsd:float ;
                              rdfs:comment "Specifies the file size of the document for standard IEC 61970-452:2017."@en ,
                                           "Specifies the file size of the document for standard IEC IEC PAS 62264-6:2016."@en ;
                              rdfs:label "FileSize IEC 61970-452:2017 "@en ,
                                         "FileSize IEC PAS 62264-6:2016 "@en .


###  https://w3id.org/i40/sto#FileSizeIEC_62264_P6
sto:FileSizeIEC_62264_P6 rdf:type owl:NamedIndividual .


###  https://w3id.org/i40/sto#FileSizeIEC_62769_P1
sto:FileSizeIEC_62769_P1 rdf:type owl:NamedIndividual ,
                                  om2:Measure ;
                         om2:hasUnit om2:kilobyte ;
                         om2:hasNumericalValue "1259.0"^^xsd:float ;
                         rdfs:comment "Specifies the file size of the document for standard IECIEC 62769-1:2015 "@en ;
                         rdfs:label "FileSize IEC 62769-1:2015   "@en .


###  https://w3id.org/i40/sto#FileSizeIEC_62832
sto:FileSizeIEC_62832 rdf:type owl:NamedIndividual ,
                               om2:Measure ;
                      om2:hasUnit om2:kilobyte ;
                      om2:hasNumericalValue "2722.0"^^xsd:float .





###  https://w3id.org/i40/sto#France
sto:France rdf:type owl:NamedIndividual ,
                    dbo:Country .


###  https://w3id.org/i40/sto#FunctionalSafety
sto:FunctionalSafety rdf:type owl:NamedIndividual ,
                              sto:RelevantDomain;
                     rdfs:comment "Functional Safety"@en ;
                     rdfs:label "Functional Safety"@en .


###  https://w3id.org/i40/sto#GPLv2
sto:GPLv2 rdf:type owl:NamedIndividual ,
                   dcterms:LicenseDocument ;
          rdfs:comment "Published under Open Content License."@en ;
          rdfs:label "GNU General Public License"@en ;
          rdfs:seeAlso <https://opcfoundation.org/license/gpl.htm> ;
          skos:note "todo"@en ;
          skos:prefLabel "OCL 1.0"^^xsd:string .


###  https://w3id.org/i40/sto#HTML
sto:HTML rdf:type owl:NamedIndividual ,
                  sto:TechnicalSpecification ;
         dcterms:creator sto:irlan ;
         sto:hasDeveloper sto:IETF ;
         sto:hasPublisher sto:IETF ;
         rdfs:label "HTML"@en .


###  https://w3id.org/i40/sto#HTTP
sto:HTTP rdf:type owl:NamedIndividual ,
                  sto:TechnicalSpecification ;
         dcterms:creator sto:irlan ,
                         sto:sebastian ;
         sto:hasDeveloper sto:IETF ;
         sto:hasPublisher sto:IETF ;
         rdfs:comment "HTTP is the most widely used protocol for internet communication."@en ;
         rdfs:label "HTTP"@en ;
         sto:hasDBpediaResource <http://dbpedia.org/resource/Hypertext_Transfer_Protocol> ;
         sto:hasOfficialResource <https://tools.ietf.org/html/rfc7230> ,
                                 <https://tools.ietf.org/html/rfc7231> ,
                                 <https://tools.ietf.org/html/rfc7232> ,
                                 <https://tools.ietf.org/html/rfc7233> ,
                                 <https://tools.ietf.org/html/rfc7234> ,
                                 <https://tools.ietf.org/html/rfc7235> ;
         sto:hasWikipediaArticle <https://en.wikipedia.org/wiki/Hypertext_Transfer_Protocol> .


###  https://w3id.org/i40/sto#HTTP2
sto:HTTP2 rdf:type owl:NamedIndividual ,
                   sto:TechnicalSpecification ;
          dcterms:creator sto:irlan ,
                          sto:sebastian ;
          sto:hasDeveloper sto:IETF ;
          sto:hasPublisher sto:IETF ;
          rdfs:comment "HTTP/2 - Enables a more efficient use of network resources and a reduced perception of latency by introducing header field compression and allowing multiple concurrent exchanges on the same connection. (source: https://www.postscapes.com/internet-of-things-protocols/)"@en ;
          rdfs:label "HTTP/2"@en ;
          sto:hasOfficialResource <http://httpwg.org/specs/rfc7540.html> .


###  https://w3id.org/i40/sto#HyperCat
sto:HyperCat rdf:type owl:NamedIndividual ,
                      sto:TechnicalSpecification ;
             dcterms:creator sto:sebastian ;
             rdfs:comment "HyperCat - An open, lightweight JSON-based hypermedia catalogue format for exposing collections of URIs. (source: https://www.postscapes.com/internet-of-things-protocols/)"@en ;
             rdfs:label "HyperCat"@en ;
             sto:hasOfficialResource <http://www.hypercat.io/standard.html> .


###  https://w3id.org/i40/sto#IBM
sto:IBM rdf:type owl:NamedIndividual ,
                 foaf:Organization ;
        sto:hasHeadquaterIn dbr:_New_York ;
        sto:abbreviation "IBM"^^xsd:string ;
        sto:formationDate "1911-06-16"^^xsd:date ;
        sto:orgName "International Business Machines Corporation"@en ;
        rdfs:comment "International Business Machines Corporation (commonly referred to as IBM) is an American multinational technology and consulting corporation, with corporate headquarters in Armonk, New York. IBM manufactures and markets computer hardware, middleware and software, and offers infrastructure, hosting and consulting services in areas ranging from mainframe computers to nanotechnology.On August 6, 2015, IBM announced that it will buy Merge Healthcare Inc for $1 billion."@en ;
        sto:hasDBpediaResource <http://dbpedia.org/resource/IBM> ;
        sto:hasOfficialResource <http://www.ibm.com> ;
        sto:hasWikipediaArticle <https://en.wikipedia.org/wiki/IBM> .


###  https://w3id.org/i40/sto#ICS_01_040_07
sto:ICS_01_040_07 rdf:type owl:NamedIndividual ,
                           sto:InternationalClassificationForStandards ;
                  dcterms:title "Natural and applied sciences (Vocabularies)"@en ;
                  rdfs:comment "This is ICS for Natural and applied sciences (Vocabularies)"@en ;
                  rdfs:label "ICS 01.040.07"@en .


###  https://w3id.org/i40/sto#ICS_01_040_35
sto:ICS_01_040_35 rdf:type owl:NamedIndividual ,
                           sto:InternationalClassificationForStandards ;
                  dcterms:title " Information technology. Office machines (Vocabularies)"@en ;
                  rdfs:comment "This is ICS for  Information technology. Office machines (Vocabularies)"@en ;
                  rdfs:label "ICS 01.040.35"@en .


###  https://w3id.org/i40/sto#ICS_01_060
sto:ICS_01_060 rdf:type owl:NamedIndividual ,
                        sto:InternationalClassificationForStandards ;
               dcterms:title "Quantities and units "@en ;
               rdfs:comment "This is ICS for Quantities and units"@en ;
               rdfs:label "ICS 01.060"@en .


###  https://w3id.org/i40/sto#ICS_01_070
sto:ICS_01_070 rdf:type owl:NamedIndividual ,
                        sto:InternationalClassificationForStandards ;
               dcterms:title "Colour coding  "@en ;
               rdfs:comment "This is ICS for Colour coding "@en ;
               rdfs:label "ICS 01.070"@en .


###  https://w3id.org/i40/sto#ICS_03_100_01
sto:ICS_03_100_01 rdf:type owl:NamedIndividual .


###  https://w3id.org/i40/sto#ICS_03_100_40
sto:ICS_03_100_40 rdf:type owl:NamedIndividual ,
                           sto:InternationalClassificationForStandards ;
                  dcterms:title "Research and development"@en ;
                  rdfs:comment "This is ICS for “Research and development  ”"@en ;
                  rdfs:label "ICS 03.100.40"@en .


###  https://w3id.org/i40/sto#ICS_03_120_01
sto:ICS_03_120_01 rdf:type owl:NamedIndividual ,
                           sto:InternationalClassificationForStandards ;
                  dcterms:title "Quality in general "@en ;
                  rdfs:comment "This is ICS for “Quality in general  ”"@en ;
                  rdfs:label "ICS 03.120.01"@en .


###  https://w3id.org/i40/sto#ICS_13_110
sto:ICS_13_110 rdf:type owl:NamedIndividual ,
                        sto:InternationalClassificationForStandards ;
               dcterms:title "Safety of machinery"@en ;
               rdfs:comment "This is ICS for Safety of machinery "@en ;
               rdfs:label "ICS 13.110"@en .


###  https://w3id.org/i40/sto#ICS_13_320
sto:ICS_13_320 rdf:type owl:NamedIndividual ,
                        sto:InternationalClassificationForStandards ;
               dcterms:title "Alarm and warning systems"@en ;
               rdfs:comment "This is ICS for Alarm and warning systems"@en ;
               rdfs:label "ICS 13.320"@en .


###  https://w3id.org/i40/sto#ICS_17_020
sto:ICS_17_020 rdf:type owl:NamedIndividual ,
                        sto:InternationalClassificationForStandards ;
               dcterms:title "Metrology and measurement in general "@en ;
               rdfs:comment "This is ICS for “Metrology and measurement in general ”"@en ;
               rdfs:label "ICS 17.020"@en .


###  https://w3id.org/i40/sto#ICS_19_020
sto:ICS_19_020 rdf:type owl:NamedIndividual ,
                        sto:InternationalClassificationForStandards ;
               dcterms:title "Test conditions and procedures in general"@en ;
               rdfs:comment "This is ICS for “Test conditions and procedures in general"@en ;
               rdfs:label "ICS 19.020"@en .


###  https://w3id.org/i40/sto#ICS_19_08
sto:ICS_19_08 rdf:type owl:NamedIndividual ,
                       sto:InternationalClassificationForStandards ;
              dcterms:title "Electrical and electronic testing"@en ;
              rdfs:comment "This is ICS for “Electrical and electronic testing”"@en ;
              rdfs:label "ICS 19.08"@en .


###  https://w3id.org/i40/sto#ICS_25_040_01
sto:ICS_25_040_01 rdf:type owl:NamedIndividual ,
                           sto:InternationalClassificationForStandards ;
                  dcterms:title "Industrial automation systems in general"@en ;
                  rdfs:comment "This is ICS for Industrial automation systems in general"@en ;
                  rdfs:label "ICS 25.040.01"@en .


###  https://w3id.org/i40/sto#ICS_25_040_40
sto:ICS_25_040_40 rdf:type owl:NamedIndividual ,
                           sto:InternationalClassificationForStandards ;
                  dcterms:title "Industrial process measurement and control"@en ;
                  rdfs:comment "This is ICS for industrial process measurement and control"@en ;
                  rdfs:label "ICS 25.040.40"@en .


###  https://w3id.org/i40/sto#ICS_25_040_99
sto:ICS_25_040_99 rdf:type owl:NamedIndividual .


###  https://w3id.org/i40/sto#ICS_27_180
sto:ICS_27_180 rdf:type owl:NamedIndividual ,
                        sto:InternationalClassificationForStandards ;
               dcterms:title "Wind turbine energy systems"@en ;
               rdfs:comment "This is ICS for “Wind turbine energy systems”"@en ;
               rdfs:label "ICS 27.180"@en .


###  https://w3id.org/i40/sto#ICS_29_020
sto:ICS_29_020 rdf:type owl:NamedIndividual ,
                        sto:InternationalClassificationForStandards ;
               dcterms:title "Electrical engineering in general "@en ;
               rdfs:comment "This is ICS for Electrical engineering in general"@en ;
               rdfs:label "ICS 29.020"@en .


###  https://w3id.org/i40/sto#ICS_29_120_70
sto:ICS_29_120_70 rdf:type owl:NamedIndividual ,
                           sto:InternationalClassificationForStandards ;
                  dcterms:title "Relays"@en ;
                  rdfs:comment "This is ICS for Relays"@en ,
                               "This is ICS for “Relays”"@en ;
                  rdfs:label "ICS 29.120.70"@en .


###  https://w3id.org/i40/sto#ICS_29_240_20
sto:ICS_29_240_20 rdf:type owl:NamedIndividual ,
                           sto:InternationalClassificationForStandards ;
                  dcterms:title "Power transmission and distribution lines"@en ;
                  rdfs:comment "This is ICS for “Power transmission and distribution lines”"@en ;
                  rdfs:label "ICS 29.240.20"@en .


###  https://w3id.org/i40/sto#ICS_31_020
sto:ICS_31_020 rdf:type owl:NamedIndividual ,
                        sto:InternationalClassificationForStandards ;
               dcterms:title "Electronic components in general "@en ;
               rdfs:comment "This is ICS for Electronic components in general "@en ;
               rdfs:label "ICS 31.020"@en .


###  https://w3id.org/i40/sto#ICS_31_240
sto:ICS_31_240 rdf:type owl:NamedIndividual ,
                        sto:InternationalClassificationForStandards ;
               dcterms:title "Mechanical structures for electronic equipment"@en ;
               rdfs:comment "This is ICS for  Mechanical structures for electronic equipment"@en ;
               rdfs:label "ICS 31.240"@en .


###  https://w3id.org/i40/sto#ICS_33_040_40
sto:ICS_33_040_40 rdf:type owl:NamedIndividual ,
                           sto:InternationalClassificationForStandards ;
                  dcterms:title "Data communication networks "@en ;
                  rdfs:comment "This is ICS for “Data communication networks”"@en ;
                  rdfs:label "ICS 33.040.40"@en .


###  https://w3id.org/i40/sto#ICS_33_060_20
sto:ICS_33_060_20 rdf:type owl:NamedIndividual ,
                           sto:InternationalClassificationForStandards ;
                  dcterms:title "Receiving and transmitting equipment"@en ;
                  rdfs:comment "This is ICS for Receiving and transmitting equipment"@en ;
                  rdfs:label "ICS 33.060.20"@en .


###  https://w3id.org/i40/sto#ICS_33_100_10
sto:ICS_33_100_10 rdf:type owl:NamedIndividual ,
                           sto:InternationalClassificationForStandards ;
                  dcterms:title "Emission"@en ;
                  rdfs:comment "This is ICS for “Emission”"@en ;
                  rdfs:label "ICS 33.100.10"@en .


###  https://w3id.org/i40/sto#ICS_33_100_20
sto:ICS_33_100_20 rdf:type owl:NamedIndividual ,
                           sto:InternationalClassificationForStandards ;
                  dcterms:title "Immunity"@en ;
                  rdfs:comment "This is ICS for “Immunity”"@en ;
                  rdfs:label "ICS 33.100.20"@en .


###  https://w3id.org/i40/sto#ICS_33_200
sto:ICS_33_200 rdf:type owl:NamedIndividual ,
                        sto:InternationalClassificationForStandards ;
               dcterms:title "Telecontrol. Telemetering Including Supervising, Control and Data Acquisition System (SCADA)"@en ;
               rdfs:comment "This is ICS for Telecontrol. Telemetering Including Supervising, Control and Data Acquisition System (SCADA)"@en ;
               rdfs:label "ICS 33.200"@en .


###  https://w3id.org/i40/sto#ICS_35_060
sto:ICS_35_060 rdf:type owl:NamedIndividual ,
                        sto:InternationalClassificationForStandards ;
               dcterms:title "Languages used in information technology"@en ;
               rdfs:comment "This is ICS for “Languages used in information technology”"@en ;
               rdfs:label "ICS 35.060"@en .


###  https://w3id.org/i40/sto#ICS_35_100
sto:ICS_35_100 rdf:type owl:NamedIndividual .


###  https://w3id.org/i40/sto#ICS_35_100_05
sto:ICS_35_100_05 rdf:type owl:NamedIndividual .


###  https://w3id.org/i40/sto#ICS_35_100_50
sto:ICS_35_100_50 rdf:type owl:NamedIndividual .


###  https://w3id.org/i40/sto#ICS_35_240_50
sto:ICS_35_240_50 rdf:type owl:NamedIndividual ,
                           sto:InternationalClassificationForStandards ;
                  dcterms:title "IT applications in industry"@en ;
                  rdfs:comment "This is ICS for IT applications in industry"@en ;
                  rdfs:label "ICS 35.240.50"@en .


###  https://w3id.org/i40/sto#ID4me
sto:ID4me rdf:type owl:NamedIndividual ,
                   sto:TechnicalSpecification ;
          dcterms:creator sto:sebastian ;
          rdfs:comment "ID4me is a federated digital identity service that aims to provide two main functions: (1) Authorization of a user for access to any third party accepting ID4me identifiers (“single sign-on” on an Internet scale); (2) Controlled communication of the user’s personal information to the third parties accessed by the user."@en ;
          rdfs:label "ID4me"@en ;
          sto:hasOfficialResource <https://id4me.org/files/ID4me_Technical_Overview_v1.3.pdf> ;
          sto_iot:hasTargetConcern sto:Identification ,
                                   sto:IdentityManagement .


###  https://w3id.org/i40/sto#IEC
sto:IEC rdf:type owl:NamedIndividual ,
                 dul:Collection ,
                 foaf:Organization ,
                 sto:StandardOrganization ;
        sto:hasHeadquaterIn dbr:Geneva ;
        sto:abbreviation "IEC"^^xsd:string ;
        rdfs:label "IEC"^^xsd:string ;
        sto:formationDate "1906-06-26"^^xsd:date ;
        sto:orgName "Commission électrotechnique internationale"@fr ,
                    "International Electrotechnical Commission"@en ;
        rdfs:comment "Is a non-profit, non-governmental international standards organization that prepares and publishes International Standards for all electrical, electronic and related technologies – collectively known as \"electrotechnology\". IEC standards cover a vast range of technologies from power generation, transmission and distribution to home appliances and office equipment, semiconductors, fiber optics, batteries, solar energy, nanotechnology and marine energy as well as many others. The IEC also manages three global conformity assessment systems that certify whether equipment, system or components conform to its International Standards."@en ;
        sto:hasDBpediaResource <http://dbpedia.org/resource/International_Electrotechnical_Commission> ;
        sto:hasOfficialResource <http://www.iec.ch/> ;
        sto:hasWikipediaArticle <https://en.wikipedia.org/wiki/International_Electrotechnical_Commission> .


###  https://w3id.org/i40/sto#IEC_11404
sto:IEC_11404 rdf:type owl:NamedIndividual ,
                       sto:Standard ;
              owl:sameAs sto:ISO_11404 ;
              rdfs:comment "Information technology -- General-Purpose Datatypes (GPD)"@en ;
              rdfs:label "ISO/IEC 11404"@en ;
              dcterms:creator sto:irlan ,
                              sto:sebastian ; 
              sto:hasDeveloper sto:IEC ,
                               sto:ISO ;
              sto:hasPublisher sto:ISO ;
              sto:hasPublicationDate "2007-12-01"^^xsd:date .


###  https://w3id.org/i40/sto#IEC_14443
sto:IEC_14443 rdf:type owl:NamedIndividual ,
                       sto:Standard ;
              owl:sameAs sto:ISO_14443 ;
              dcterms:creator sto:irlan;
              sto:hasPublisher sto:IEC ,
                               sto:ISO ;
              sto:hasTag "IEC 14443"@en ;
              rdfs:comment "The ISO/IEC 14443 standard is a four-part international standard for contact-less smart cards operating at 13.56 MHz in close proximity (~10cm) with a reader antenna. This ISO standard describes the modulation and transmission protocols between card and reader to create interoperability for contact-less smart card products. There are two main communication protocols supported by the ISO/IEC 14443 standard, they are addressed as Type A and Type B. Most High Frequency (13.56 MHz) proximity tags are using these guidelines for their communication."@en ;
              rdfs:label "ISO/IEC 14443"@en ;
              sto:hasDBpediaResource <http://dbpedia.org/resource/ISO/IEC_14443> ;
              sto:hasOfficialResource <https://webstore.iec.ch/publication/62997> ,
                                      <https://www.iso.org/standard/73596.html> ;
              sto:hasOpenResource <http://www.icedev.se/proxmark3/docs/ISO-14443-3.pdf> ,
                                  <https://webstore.iec.ch/preview/info_isoiec14443-2%7Bed3.0%7Den.pdf> ,
                                  <https://www.sis.se/api/document/preview/912600/> ;
              sto:hasWikipediaArticle <https://en.wikipedia.org/wiki/ISO/IEC_14443> .


###  https://w3id.org/i40/sto#IEC_15408
sto:IEC_15408 rdf:type owl:NamedIndividual ,
                       sto:Standard ;  
              dcterms:creator sto:irlan ;
              rdfs:label "IEC 15408"@en ;
              sto:hasClassification sto:IIRASecurity ;
              sto:hasPublisher sto:ISO ;
              sto:Tag "Common Criteria"@en,
                      "CC"^^xsd:string ;
              rdfs:comment "The Common Criteria for Information Technology Security Evaluation (referred to as Common Criteria or CC) is an international standard (ISO/IEC 15408) for computer security certification"@en;
              sto:hasDBpediaResource <http://dbpedia.org/page/Common_Criteria>;
              sto:hasOfficialResource <https://www.iso.org/standard/40612.html> ;
              .


###  https://w3id.org/i40/sto#IEC_15459
sto:IEC_15459 rdf:type owl:NamedIndividual ,
                       sto:Standard ;
              owl:sameAs sto:ISO_15459 ;
              dcterms:creator sto:irlan ;
              sto:hasPublisher sto:IEC ,
                               sto:ISO ;
              sto:hasTag "Information technology -- Automatic identification and data capture techniques -- Unique identification"@en ;
              rdfs:comment "ISO/IEC 15459-1:2014 specifies a unique string of characters for the identification of individual transport units. The character string is intended to be represented in a bar code label or other AIDC media attached to the entity to meet management needs. To address management needs, different types of entities are recognized in the various parts of ISO/IEC 15459, which allows different requirements to be met by the identities associated with each type. The rules for the unique identification for individual transport units, to identify physical logistical transfers, with the identity relevant for the duration of one or more items in the load being held or transported as part of that load, are defined and supported by example."@en ;
              rdfs:label "IEC 15459"@en ;
              sto:hasOfficialResource <https://webstore.iec.ch/publication/10334> ,
                                      <https://www.iso.org/standard/54779.html> .


###  https://w3id.org/i40/sto#IEC_24760
sto:IEC_24760 rdf:type owl:NamedIndividual ,
                       sto:Standard ;
              dcterms:creator sto:irlan ;
              sto_iot:hasTargetConcern sto:IdentityManagement;
              sto:hasClassification sto:AsSafety  ,
                                    sto:AsSecurity ,
                                    sto:IIRASecurity ,
                                    sto:NISTProductModelDataExchange ,
                                    sto:RamiControlDevice ,
                                    sto:RamiFieldDevice ,
                                    sto:RamiInformationLayer ,
                                    sto:RamiProduct ,
                                    sto:RamiStation ;
              sto:hasPublisher sto:IEC ;
              sto:relatedTo sto:IEC_24760 ,
                            sto:IEC_62443 ,
                            sto:ISO_24760 ;
              sto:hasPublicationDate "2011-01-12"^^xsd:date ;
              rdfs:comment "ISO/IEC 24760: it defines terms for identity management, and also specifies core concepts of identity and identity management and their relationships. It is applicable to any information system that processes identity information. A bibliography of documents describing various aspects of identity information management is provided."@en ;
              rdfs:label "IEC 24760"@en ;
              sto:hasRelevantDomain sto:ITSecurity ;
              sto:hasOfficialResource <https://webstore.iec.ch/publication/11190> ,
                                      <https://www.iso.org/standard/57914.html> .


###  https://w3id.org/i40/sto#IEC_27018
sto:IEC_27018 rdf:type owl:NamedIndividual ,
                       sto:Standard ;
              owl:sameAs sto:ISO_27018 ;
              rdfs:label "IEC 27018" ;
              rdfs:comment "ISO/IEC 27018:2014 establishes commonly accepted control objectives, controls and guidelines for implementing measures to protect Personally Identifiable Information (PII) in accordance with the privacy principles in ISO/IEC 29100 for the public cloud computing environment."@en ;
              dcterms:creator sto:irlan;
              sto:hasClassification sto:IIRAPrivacy ,
                                    sto:IIRASecurity ;
              sto:hasPublisher sto:IEC ,
                               sto:ISO ;
              sto:hasPublicationDate "2014-08-01"^^xsd:date .


###  https://w3id.org/i40/sto#IEC_27031
sto:IEC_27031 rdf:type owl:NamedIndividual ,
                       sto:Standard ;
              owl:sameAs sto:ISO_27031 ;
              rdfs:comment "ISO/IEC 27031:2011 describes the concepts and principles of information and comunication technology (ICT) readiness for business continuity, and provides a framework of methods and processes to identify and specify all aspects (such as performance criteria, design, and implementation) for improving an organization's ICT readiness to ensure business continuity."@en ;
              rdfs:label "ISO/IEC 27031"@en ;
              dcterms:creator sto:irlan;
              sto:hasClassification sto:IIRAPrivacy ,
                                    sto:IIRASecurity ;
              sto:hasPublisher sto:IEC ,
                               sto:ISO ;
              sto:domainName "Business Continuity"@en ;
              sto:hasPublicationDate "2011-03-01"^^xsd:date  .


###  https://w3id.org/i40/sto#IEC_27036
sto:IEC_27036 rdf:type owl:NamedIndividual ,
                       sto:Standard ;
              owl:sameAs sto:ISO_27036 ;
              rdfs:comment """ISO/IEC 27036-4:2016 provides cloud service customers and cloud service providers with guidance on

a) gaining visibility into the information security risks associated with the use of cloud services and managing those risks effectively, and

b) responding to risks specific to the acquisition or provision of cloud services that can have an information security impact on organizations using these services."""@en ;
              rdfs:label "ISO/IEC 27036"@en ;
              dcterms:creator sto:irlan;
              sto:hasClassification sto:IIRASecurity ;
              sto:hasPublisher sto:IEC ,
                               sto:ISO ;
              sto:hasPublicationDate "2016-10-01"^^xsd:date .


###  https://w3id.org/i40/sto#IEC_29100
sto:IEC_29100 rdf:type owl:NamedIndividual ,
                       sto:Standard ;
              owl:sameAs sto:ISO_29100 ;
              rdfs:comment """‘Privacy framework’1 provides a guideline that specifies a common privacy terminology, defines actors and roles in processing PII, describes privacy safeguarding considerations, and includes references to known privacy principles for Information technology.
source: IIC SF"""@en ;
              rdfs:label "ISO/IEC 29100"@en ;
              dcterms:creator sto:irlan ;
              sto:hasClassification sto:IIRAPrivacy ,
                                    sto:IIRASecurity ;
              sto:hasPublisher sto:IEC ,
                               sto:ISO ;
              sto:hasPublicationDate "2011-12-01"^^xsd:date .


###  https://w3id.org/i40/sto#ISO_29115
sto:ISO_29115 rdf:type owl:NamedIndividual ,
                       foaf:Document ,
                       sto:Publication ,
                       sto:Standard ;
              dcterms:creator sto:irlan ,
                              sto:ISO ;
              foaf:maker sto:IEC ,
                         sto:ISO ;
              sto_iot:hasTargetConcern sto:Authentication ,
                                   sto:Identification ;
              sto:hasClassification sto:IIRASecurity ;
              sto:hasPublisher sto:IEC ,
                               sto:ISO ;
              rdfs:comment """ISO/IEC 29115:2013 provides a framework for managing entity authentication assurance in a given context. In particular, it:

- specifies four levels of entity authentication assurance;

- specifies criteria and guidelines for achieving each of the four levels of entity authentication assurance;

- provides guidance for mapping other authentication assurance schemes to the four LoAs;

- provides guidance for exchanging the results of authentication that are based on the four LoAs; and

- provides guidance concerning controls that should be used to mitigate authentication threats."""@en ;
              rdfs:label "ISO/IEC 29115"@en .

###  https://w3id.org/i40/sto#IEC_29115
sto:IEC_29115 rdf:type owl:NamedIndividual ,
                       sto:Standard ;
              owl:sameAs sto:ISO_29115 ;
              dcterms:creator sto:irlan;
              sto:hasPublisher sto:IEC ,
                               sto:ISO ;
              dcterms:title "Information technology -- Security techniques -- Entity authentication assurance framework"@en ;
              rdfs:comment """ISO/IEC 29115:2013 provides a framework for managing entity authentication assurance in a given context. In particular, it:

- specifies four levels of entity authentication assurance;

- specifies criteria and guidelines for achieving each of the four levels of entity authentication assurance;

- provides guidance for mapping other authentication assurance schemes to the four LoAs;

- provides guidance for exchanging the results of authentication that are based on the four LoAs; and

- provides guidance concerning controls that should be used to mitigate authentication threats."""@en ;
              rdfs:label "IEC 29115"@en ;
              sto:hasOfficialResource <https://webstore.iec.ch/publication/11351> ,
                                      <https://www.iso.org/standard/45138.html> .


###  https://w3id.org/i40/sto#IEC_29161
sto:IEC_29161 rdf:type owl:NamedIndividual ,
                       sto:Standard ;
              owl:sameAs sto:ISO_29161 ;
              dcterms:creator sto:irlan ;
              sto:hasDomain sto:Automatic_Id_Data_Capture_Techniques ;
              sto:hasPublisher sto:IEC ,
                               sto:ISO ;
              sto:hasPublicationDate "2016-08-01"^^xsd:date ;
              sto:hasTag "Information technology -- Data structure -- Unique identification for the Internet of Things"@en ;
              rdfs:comment "ISO/IEC 29161:2016 establishes a unique identification scheme for the Internet of Things (IoT), based on existing and evolving data structures. This International Standard specifies the common rules applicable for unique identification that are required to ensure full compatibility across different identities. The unique identification is a universal construct for any physical object, virtual object, or person. It is used in IoT information systems that need to track or otherwise refer to entities. It is intended for use with any IoT media."@en ;
              rdfs:label "IEC 29161"@en ;
              sto:hasOfficialResource <https://webstore.iec.ch/publication/60834> ,
                                      <https://www.iso.org/standard/45240.html> .





###  https://w3id.org/i40/sto#IEC_29182_P1
sto:IEC_29182_P1 rdf:type owl:NamedIndividual ,
                          sto:Standard ;
                 dcterms:creator sto:irlan ;
                 sto:hasClassification sto:ProductionSystemModelData ,
                                       sto:RamiCommunicationlayer ,
                                       sto:RamiControlDevice ,
                                       sto:RamiFieldDevice ;
                 sto:hasPublisher sto:IEC ,
                                  sto:ISO ;
                 sto:relatedTo sto:IEC_61158 ,
                               sto:IEC_61784 ,
                               sto:OMG_DDS ;
                 sto:hasPublicationDate "2013-06-01"^^xsd:date ;
                 rdfs:comment "ISO/IEC 29182-1: provides a general overview of the characteristics of a sensor network and the organization of the entities that comprise such a network. It also describes the general requirements that are identified for sensor networks."@en ;
                 rdfs:label "IEC 29182-1"@en ;
                 sto:hasOfficialResource <https://webstore.iec.ch/publication/11411> ,
                                         <https://www.iso.org/standard/45261.html> .


###  https://w3id.org/i40/sto#IEC_29190
sto:IEC_29190 rdf:type owl:NamedIndividual ,
                       sto:Standard ;
              owl:sameAs sto:ISO_29190 ;
              dcterms:creator sto:irlan ;
              sto:hasClassification sto:IIRAPrivacy ,
                                    sto:IIRASecurity ;
              sto:hasPublisher sto:IEC ,
                               sto:ISO ;
              sto:hasPublicationDate "2015-08-01"^^xsd:date ;
              rdfs:comment "‘Privacy capability assessment model’ provides high-level guidance to organizations about assessing their capability to manage privacy-related processes."@en ;
              rdfs:label "IEC 29190"@en .


###  https://w3id.org/i40/sto#IEC_42010
sto:IEC_42010 rdf:type owl:NamedIndividual ,
                       sto:Standard ;
              rdfs:label "IEC 42010" ;
              owl:sameAs sto:ISO_42010 ;
              dcterms:creator sto:irlan ,
                              sto:sebastian ;
              sto:hasPublisher sto:IEC ,
                               sto:IEEE ,
                               sto:ISO ;
              sto:hasTag "ISO/IEC/IEEE 42010"@en ;
              rdfs:comment "ISO/IEC/IEEE 42010:2011 defines requirements on the description of system, software and enterprise architectures. It aims to standardise the practice of architecture description by defining standard terms, presenting a conceptual foundation for expressing, communicating and reviewing architectures and specifying requirements that apply to architecture descriptions, architecture frameworks and architecture description languages."@en ;
              rdfs:label "IEC 42010"@en ;
              skos:note "The IIRA is based on this standards"@en ;
              sto:hasDBpediaResource <http://dbpedia.org/page/ISO/IEC_42010> ;
              sto:hasOfficialResource <http://www.iso-architecture.org/ieee-1471/> ,
                                      <https://standards.ieee.org/standard/42010-2011.html> ,
                                      <https://webstore.iec.ch/publication/11978> ,
                                      <https://www.iso.org/standard/50508.html> ;
              sto:hasOpenResource <http://cabibbo.dia.uniroma3.it/asw/altrui/iso-iec-ieee-42010-2011.pdf> ;
              sto:hasWikipediaArticle <https://en.wikipedia.org/wiki/ISO/IEC_42010> .

sto:IEC_60027 rdf:type owl:NamedIndividual ,
                             sto:Standard ;
                    sto:hasAvailableLanguage lang:eng ,
                                             lang:fra ,
                                             lang:spa ;
                    sto:hasImplementationFormat "Document"@en ;
                    rdfs:comment "IEC 60027 (formerly IEC 27) is a technical international standard for letter symbols."@en ;
                    rdfs:label "IEC 60027"@en ;
              sto:hasPublisher sto:IEC ;
                    sto:hasDBpediaResource <http://dbpedia.org/page/IEC_60027> ;
                    sto:hasWikipediaArticle <https://en.wikipedia.org/wiki/IEC_60027> .



###  https://w3id.org/i40/sto#IEC_60027_P6_E1
sto:IEC_60027_P6_E1 rdf:type owl:NamedIndividual ,
                             sto:Standard ;
                    dcterms:creator sto:irlan ;
                    sto:hasAvailableLanguage lang:eng ,
                                             lang:fra ,
                                             lang:spa ;
                    sto:hasFileSize sto:FileSizeIEC_60027_P6 ;
                    sto:isPartOf sto:IEC_60027;
                    sto:hasICS sto:ICS_01_060 ;
                    sto:hasPublisher sto:IEC ;
                    sto:hasTechnicalCommittee sto:TC_25 ;
                    sto:hasEdition "1.0"^^xsd:float ;
                    sto:hasImplementationFormat "Document"@en ;
                    sto:hasPages "29"^^xsd:int ;
                    sto:hasPublicationDate "2006-12-14"^^xsd:date ;
                    sto:hasStabilityDate "2019"^^xsd:gYear ;
                    dcterms:title "Letter symbols to be used in electrical technology - Part 6: Control technology"@en ;
                    rdfs:comment "This part of IEC 60027 is applicable to control technology. It gives names and symbols for quantities, signals and functions, and their units."@en ;
                    rdfs:label "IEC 60027-6:2006"@en ;
                    sto:hasDBpediaResource <http://dbpedia.org/page/IEC_60027> ;
                    sto:hasOfficialResource <https://webstore.iec.ch/publication/96> ;
                    sto:hasStatus "Valid"@en ;
                    sto:hasWikipediaArticle <https://en.wikipedia.org/wiki/IEC_60027> .



sto:IEC_60038 rdf:type owl:NamedIndividual ,
                          sto:Standard ;
                 sto:hasAvailableLanguage lang:eng ,
                                          lang:fra ,
                                          lang:spa ;
                 sto:hasPublisher sto:IEC ;
                 sto:hasImplementationFormat "Document"@en ;
                 rdfs:comment "IEC 60038 specifies standard voltage values which are intended to serve as preferential values for the nominal voltage of electrical supply systems, and as reference values for equipment and system design. "@en ;
                 rdfs:label "IEC 60038"@en ;
                 sto:hasDBpediaResource <http://dbpedia.org/page/IEC_60038> ;
                 sto:hasWikipediaArticle <https://en.wikipedia.org/wiki/IEC_60038> .


###  https://w3id.org/i40/sto#IEC_60038_E7
sto:IEC_60038_E7 rdf:type owl:NamedIndividual ,
                          sto:Standard ;
                 dcterms:creator sto:irlan ,
                                 sto:sebastian ;
                 sto:hasAvailableLanguage lang:eng ,
                                          lang:fra ,
                                          lang:spa ;
                 sto:hasFileSize sto:FileSizeIEC_60038 ;
                 sto:hasICS sto:ICS_29_020 ;
                 sto:hasPublisher sto:IEC ;
                 sto:hasTechnicalCommittee sto:TC_8 ;
                 sto:hasRelevantDomain sto:RuralElectrification ;
                 sto:hasEdition "7.0"^^xsd:float ;
                 sto:hasImplementationFormat "Document"@en ;
                 sto:hasPages "26"^^xsd:int ;
                 sto:hasPublicationDate "2009-06-17"^^xsd:date ;
                 sto:hasStabilityDate "2020"^^xsd:gYear ;
                 dcterms:title " IEC standard voltages "@en ;
                 rdfs:comment "IEC 60038:2009 specifies standard voltage values which are intended to serve as preferential values for the nominal voltage of electrical supply systems, and as reference values for equipment and system design. This seventh edition supersedes the sixth edition (1993), its Amendment 1 (1994) and its Amendment 2 (1997). It constitutes a technical revision. The significant technical changes are: -the addition of the values of 230 V (50 Hz) and 230/400 V (60 Hz) to Table 1;-the replacement of the utilization voltage range at LV by a reference to the relevant standard and an informative annex;- the addition of the value of 30 kV to Table 3;- the replacement of the value of 1 050 kV by 1 100 kV in Table 5. It has the status of a horizontal standard in accordance with IEC Guide 108."@en ;
                 rdfs:label "IEC 60038:2009"@en ;
                 sto:hasDBpediaResource <http://dbpedia.org/page/IEC_60038> ;
                 sto:hasOfficialResource <https://webstore.iec.ch/publication/153> ;
                 sto:hasStatus "Valid"@en ;
                 sto:hasWikipediaArticle <https://en.wikipedia.org/wiki/IEC_60038> .


###  https://w3id.org/i40/sto#IEC_60050
sto:IEC_60050 rdf:type owl:NamedIndividual ,
                       sto:Standard ;
              sto:relatedTo sto:IEC_60050_P101_E2,
                           sto:IEC_60050_P351_E4,
                           sto:IEC_60050_P371_E1 ;
              rdfs:comment "The International Electrotechnical Vocabulary (IEV) serves to promote the global unification of terminology in the field of electrotechnology, electronics and telecommunications."@en ;
              rdfs:label "IEC 60050"@en ;
              skos:altLabel "Electropedia"@en ;
                 sto:hasPublisher sto:IEC ;
              sto:hasDBpediaResource <http://dbpedia.org/page/International_Electrotechnical_Vocabulary> ;
              sto:hasWikipediaArticle <https://en.wikipedia.org/wiki/International_Electrotechnical_Vocabulary> .



###  https://w3id.org/i40/sto#IEC_60050_P101_E2
sto:IEC_60050_P101_E2 rdf:type owl:NamedIndividual ,
                               sto:StandardPart ;
                      dcterms:creator sto:irlan ;
                      dul:isComponentOf sto:IEC_60050 ;
                      sto:hasAvailableLanguage lang:eng ,
                                               lang:fra ,
                                               lang:spa ;
                      sto:hasFileSize sto:FileSizeIEC_60050_P101 ;
                      sto:hasICS sto:ICS_01_040_07 ;
                      sto:hasPublisher sto:IEC ;
                      sto:hasTechnicalCommittee sto:TC_1 ;
                      sto:isPartOf sto:IEC_60050;
                      sto:relatedTo sto:IEC_60050 ,
                                    sto:IEC_60050_P351_E4,
                                    sto:IEC_60050_P371_E1 ;
                      sto:hasEdition "2.0"^^xsd:float ;
                      sto:hasImplementationFormat "Document"@en ;
                      sto:hasPages "129"^^xsd:int ;
                      sto:hasPublicationDate "1998-04-30"^^xsd:date ;
                      sto:hasStatus "Replaced"@en ;
                      dcterms:title "International Electrotechnical Vocabulary - Part 101: Mathematics"@en ;
                      rdfs:comment "It has the status of a horizontal standard in accordance with IEC Guide 108."@en ;
                      rdfs:label "IEC 60050-101:1998"@en ;
                      sto:hasDBpediaResource <http://dbpedia.org/page/International_Electrotechnical_Vocabulary> ;
                      sto:hasOfficialResource <https://webstore.iec.ch/publication/159> ;
                      sto:hasWikipediaArticle <https://en.wikipedia.org/wiki/International_Electrotechnical_Vocabulary> .


###  https://w3id.org/i40/sto#IEC_60050_P351_E4
sto:IEC_60050_P351_E4 rdf:type owl:NamedIndividual ,
                               sto:StandardPart ;
                      dcterms:creator sto:irlan ;
                      dul:isComponentOf sto:IEC_60050 ;
                      sto:hasAvailableLanguage lang:eng ,
                                               lang:fra ;
                      sto:hasFileSize sto:FileSizeIEC_60050_P351 ;
                      sto:hasICS sto:ICS_01_040_07 ,
                                 sto:ICS_25_040_40 ;
                      sto:hasPublisher sto:IEC ;
                      sto:hasTechnicalCommittee sto:TC_1 ;
                      sto:isPartOf sto:IEC_60050;
                      sto:relatedTo sto:IEC_60050 ,
                                    sto:IEC_60050_P101_E2,
                                    sto:IEC_60050_P371_E1 ;
                      sto:hasEdition "4.0"^^xsd:float ;
                      sto:hasImplementationFormat "Document"@en ;
                      sto:hasPages "457"^^xsd:int ;
                      sto:hasPublicationDate "2013-11-25"^^xsd:date ;
                      sto:hasStatus "Valid"@en ;
                      dcterms:title "International Electrotechnical Vocabulary - Part 351: Control technology"@en ;
                      rdfs:comment "IEC 60050-351:2013 gives the general terminology used in control technology, as well as general terms pertaining to specific applications and associated technologies. This new edition reviews and complements the previous one. It has the status of a horizontal standard in accordance with IEC Guide 108."@en ;
                      rdfs:label "IEC 60050-351:2013"@en ;
                      sto:hasOfficialResource <https://webstore.iec.ch/publication/194> .


###  https://w3id.org/i40/sto#IEC_60050_P371_E1
sto:IEC_60050_P371_E1 rdf:type owl:NamedIndividual ,
                               sto:StandardPart ;
                      dcterms:creator sto:irlan ;
                      dul:isComponentOf sto:IEC_60050 ;
                      sto:hasAvailableLanguage lang:eng ,
                                               lang:fra ,
                                               lang:rus ;
                      sto:hasFileSize sto:FileSizeIEC_60050_P371 ;
                      sto:hasICS sto:ICS_01_040_35 ,
                                 sto:ICS_35_240_50 ;
                      sto:hasPublisher sto:IEC ;
                      sto:hasTechnicalCommittee sto:TC_1 ;
                      sto:isPartOf sto:IEC_60050;
                      sto:relatedTo sto:IEC_60050 ,
                                    sto:IEC_60050_P101_E2,
                                    sto:IEC_60050_P351_E4;
                      sto:hasEdition "1.0"^^xsd:float ;
                      sto:hasImplementationFormat "Document"@en ;
                      sto:hasPages "44"^^xsd:int ;
                      sto:hasPublicationDate "1984-11-30"^^xsd:date ;
                      sto:hasStatus "Valid"@en ;
                      dcterms:title "International Electrotechnical Vocabulary. Chapter 371: Telecontrol"@en ;
                      rdfs:comment "Terms on telecontrol, teleprotection and associated telecommunications for electric power systems. It has the status of a horizontal standard in accordance with IEC Guide 108."@en ;
                      rdfs:label "IEC 60050-371:1984"@en ;
                      sto:hasOfficialResource <https://webstore.iec.ch/publication/196> .


###  https://w3id.org/i40/sto#IEC_60073_E6
sto:IEC_60073_E6 rdf:type owl:NamedIndividual ,
                          sto:Standard ;
                 dcterms:creator sto:irlan;
                 sto:hasAvailableLanguage lang:eng ,
                                          lang:fra ,
                                          lang:spa ;
                 sto:hasFileSize sto:FileSizeIEC_60073 ;
                 sto:hasICS sto:ICS_01_070 ,
                            sto:ICS_29_020 ;
                 sto:hasPublisher sto:IEC ;
                 sto:hasTechnicalCommittee sto:TC_3 ;
                 sto:hasEdition "6.0"^^xsd:float ;
                 sto:hasImplementationFormat "Document"@en ;
                 sto:hasPages "61"^^xsd:int ;
                 sto:hasPublicationDate "2002-05-22"^^xsd:date ;
                 sto:hasStabilityDate "2025"^^xsd:gYear ;
                 sto:hasStatus "Valid"@en ;
                 sto:hasTag "IEC_60073:2002"@en ;
                 dcterms:title "Basic and safety principles for man-machine interface, marking and identification - Coding principles for indicators and actuators"@en ;
                 rdfs:comment "Establishes general rules for assigning particular meanings to certain visual, acoustsic and tactile indications. It has the status of a Basic Safety Publication in accordance with IEC Guide 104."@en ;
                 rdfs:label "IEC 60073:2002 "@en ;
                 sto:hasOfficialResource <https://webstore.iec.ch/publication/587> .


###  https://w3id.org/i40/sto#IEC_60086
sto:IEC_60086 rdf:type owl:NamedIndividual ,
                       sto:Standard ;
              dcterms:creator sto:irlan;
              sto:hasPublisher sto:IEC ;
              rdfs:comment "Standard battery nomenclature describes portable dry cell batteries that have physical dimensions and electrical characteristics interchangeable between manufacturers."@en ;
              rdfs:label "IEC 60086"@en ;
              sto:hasDBpediaResource <http://dbpedia.org/page/Battery_nomenclature#IEC_60086> ;
              sto:hasOfficialResource <https://webstore.iec.ch/publication/22991> ;
              sto:hasWikipediaArticle <https://en.wikipedia.org/wiki/Battery_nomenclature#IEC_60086> .

sto:IEC_60204 rdf:type owl:NamedIndividual ,
                              sto:Standard ;
                     sto:hasPublisher sto:IEC ;
                     dcterms:title "IEC 60204-1 / EN 60204 Safety of machinery – Electrical equipment of machines"@en ;
                     rdfs:comment "Applies to the electrical and electronic equipment and systems of machines, including a group of machines working together in a coordinated manner, but excluding higher level system aspects (i.e. communications between systems)."@en ;
                     rdfs:label "IEC 60204"@en ;
                     sto:hasWikipediaArticle <https://en.wikipedia.org/wiki/IEC_60204> .


###  https://w3id.org/i40/sto#IEC_60204_P11_E1
sto:IEC_60204_P11_E1 rdf:type owl:NamedIndividual ,
                              sto:Standard ;
                     dcterms:creator sto:irlan ;
                     sto:hasAvailableLanguage lang:eng ,
                                              lang:fra ,
                                              lang:spa ;
                     sto:hasFileSize sto:FileSizeIEC_60204_P11 ;
                     sto:hasICS sto:ICS_13_110 ,
                                sto:ICS_29_020 ;
                     sto:hasPublisher sto:IEC ;
                     sto:hasTechnicalCommittee sto:TC_44 ;
                     sto:isPartOf sto:IEC_60204;
                     sto:hasEdition "1.0"^^xsd:float ;
                     sto:hasImplementationFormat "Document"@en ;
                     sto:hasPages "111"^^xsd:int ;
                     sto:hasPublicationDate "2000-07-31"^^xsd:date ;
                     sto:hasStabilityDate "2018"^^xsd:gYear ;
                     sto:hasStatus "Withdrawn"@en ;
                     dcterms:title "Safety of machinery - Electrical equipment of machines - Part 11: Requirements for HV equipment for voltages above 1 000 V a.c. or 1 500 V d.c. and not exceeding 36 kV"@en ;
                     rdfs:comment "Applies to the electrical and electronic equipment and systems of machines, including a group of machines working together in a coordinated manner, but excluding higher level system aspects (i.e. communications between systems)."@en ;
                     rdfs:label "IEC 60204-11:2000"@en ;
                     sto:hasOfficialResource <https://webstore.iec.ch/publication/1022> .


sto:IEC_60255 rdf:type owl:NamedIndividual ,
                            sto:Standard ;
                   sto:hasPublisher sto:IEC ;
                   sto:hasTag "IEC 60255"@en ;
                   dcterms:title "Measuring relays and protection equipment "@en ;
                   rdfs:comment "Rules and requirements applicable to measuring relays and protection equipment."@en ;
                   rdfs:label "IEC 60255"@en  .


###  https://w3id.org/i40/sto#IEC_60255_2010
sto:IEC_60255_P127_E1 rdf:type owl:NamedIndividual ,
                            sto:Standard ;
                   sto:hasAvailableLanguage lang:eng ,
                                            lang:fra ;
                   sto:hasFileSize sto:FileSizeIEC_60255_2010 ;
                   sto:hasICS sto:ICS_29_120_70 ;
                   sto:hasPublisher sto:IEC ;
                   sto:hasTechnicalCommittee sto:TC_95 ;
                   sto:relatedTo sto:IEC_60255_P149_E1 ;
                   sto:isPartOf sto:IEC_60255;
                   sto:hasEdition "1.0"^^xsd:float ;
                   sto:hasImplementationFormat "Document"@en ;
                   sto:hasPages "93"^^xsd:int ;
                   sto:hasPublicationDate "2010-04-27"^^xsd:date ;
                   sto:hasStatus "Valid"@en ;
                   sto:hasTag "IEC 60255-127:2010"@en ;
                   dcterms:title "Measuring relays and protection equipment - Part 127: Functional requirements for over/under voltage protection"@en ;
                   rdfs:comment "IEC 60255-127:2010 specifies minimum requirements for over/under voltage relays. The standard includes specification of the protection function, measurement characteristics and time delay characteristics."@en ;
                   rdfs:label "IEC 60255-127:2010"@en ;
                   sto:hasOfficialResource <https://webstore.iec.ch/publication/1165> .


###  https://w3id.org/i40/sto#IEC_60255_P149_E1
sto:IEC_60255_P149_E1 rdf:type owl:NamedIndividual ,
                               sto:Standard ;
                      dcterms:creator sto:irlan ;
                      sto:hasAvailableLanguage lang:eng ,
                                               lang:fra ;
                      sto:hasFileSize sto:FileSizeIEC_60255_P149 ;
                      sto:hasICS sto:ICS_29_120_70 ;
                      sto:hasPublisher sto:IEC ;
                      sto:hasTechnicalCommittee sto:TC_95 ;
                      sto:isPartOf sto:IEC_60255;
                      sto:hasEdition "1.0"^^xsd:float ;
                      sto:hasImplementationFormat "Document"@en ;
                      sto:hasPages "93"^^xsd:int ;
                      sto:hasPublicationDate "2013-07-30"^^xsd:date ;
                      sto:hasStatus "Valid"@en ;
                      sto:hasTag "IEC 60255-149:2013 "@en ;
                      dcterms:title "Measuring relays and protection equipment - Part 149: Functional requirements for thermal electrical relays"@en ;
                      rdfs:comment "IEC 60255-149:2013 specifies minimum requirements for thermal protection relays. This standard includes specification of the protection function, measurement characteristics and test methodologies. The object is to establish a common and reproducible reference for evaluating dependent time relays which protect equipment from thermal damage by measuring a.c. current flowing through the equipment. Complementary input energizing quantities such as ambient, coolant, top oil and winding temperature may be applicable for the thermal protection specification set forth in this standard. This standard covers protection relays based on a thermal model with memory function."@en ;
                      rdfs:label "IEC 60255-149:2013 "@en ;
                      sto:hasOfficialResource <https://webstore.iec.ch/publication/1165> .


###  https://w3id.org/i40/sto#IEC_60255_P151_E1
sto:IEC_60255_P151_E1 rdf:type owl:NamedIndividual ,
                               sto:Standard ;
                      dcterms:creator sto:irlan ;
                      sto:hasAvailableLanguage lang:eng ,
                                               lang:fra ;
                      sto:hasFileSize sto:FileSizeIEC_60255_P151 ;
                      sto:hasICS sto:ICS_29_120_70 ;
                      sto:hasPublisher sto:IEC ;
                      sto:hasTechnicalCommittee sto:TC_95 ;
                      sto:relatedTo sto:IEC_60255_P149_E1 ;
                      sto:isPartOf sto:IEC_60255;
                      sto:hasEdition "1.0"^^xsd:float ;
                      sto:hasImplementationFormat "Document"@en ;
                      sto:hasPages "63"^^xsd:int ;
                      sto:hasPublicationDate "2009-08-28"^^xsd:date ;
                      sto:hasStatus "Valid"@en ;
                      sto:hasTag "IEC 60255-151:2009 "@en ;
                      dcterms:title "Measuring relays and protection equipment - Part 151: Functional requirements for over/under current protection"@en ;
                      rdfs:comment "IEC 60255-151:2009 specifies minimum requirements for over/under current relays. It includes a specification of the protection function, measurement characteristics and time delay characteristics. Defines the influencing factors that affect the accuracy under steady state conditions and performance characteristics during dynamic conditions."@en ;
                      rdfs:label "IEC 60255-151:2009 "@en ;
                      sto:hasOfficialResource <https://webstore.iec.ch/publication/1166> .


###  https://w3id.org/i40/sto#IEC_60255_P1_E1
sto:IEC_60255_P1_E1 rdf:type owl:NamedIndividual ,
                             sto:Standard ;
                    dcterms:creator sto:irlan ;
                    sto:hasAvailableLanguage lang:eng ,
                                             lang:fra ,
                                             lang:spa ;
                    sto:hasFileSize sto:FileSizeIEC_60255_P1 ;
                    sto:hasICS sto:ICS_29_120_70 ;
                    sto:hasPublisher sto:IEC ;
                    sto:hasTechnicalCommittee sto:TC_95 ;
                    sto:isPartOf sto:IEC_60255;
                    sto:hasEdition "1.0"^^xsd:float ;
                    sto:hasImplementationFormat "Document"@en ;
                    sto:hasPages "89"^^xsd:int ;
                    sto:hasPublicationDate "2009-08-18"^^xsd:date ;
                    sto:hasStabilityDate "2018"^^xsd:gYear ;
                    sto:hasStatus "Valid"@en ;
                    sto:hasTag "IEC 60255-1:2009 "@en ;
                    dcterms:title "Measuring relays and protection equipment - Part 1: Common requirements"@en ;
                    rdfs:comment "IEC 60255-1:2009 specifies common rules and requirements applicable to measuring relays and protection equipment including any combination of devices to form schemes for power system protection such as control, monitoring and process interface equipment in order to obtain uniformity of requirements and tests. Covers all measuring relays and protection equipment used for protection within the power system environment."@en ;
                    rdfs:label "IEC 60255-1:2009 "@en ;
                    sto:hasOfficialResource <https://webstore.iec.ch/publication/1160> .


###  https://w3id.org/i40/sto#IEC_60255_P27_E2
sto:IEC_60255_P27_E2 rdf:type owl:NamedIndividual ,
                              sto:Standard ;
                     dcterms:creator sto:irlan ;
                     sto:hasAvailableLanguage lang:eng ,
                                              lang:fra ;
                     sto:hasFileSize sto:FileSizeIEC_60255_P27 ;
                     sto:hasICS sto:ICS_29_120_70 ;
                     sto:hasPublisher sto:IEC ;
                     sto:hasTechnicalCommittee sto:TC_95 ;
                     sto:isPartOf sto:IEC_60255;
                     sto:hasEdition "2.0"^^xsd:float ;
                     sto:hasImplementationFormat "Document"@en ;
                     sto:hasPages "197"^^xsd:int ;
                     sto:hasPublicationDate "2013-10-15"^^xsd:date ;
                     sto:hasStabilityDate "2018"^^xsd:gYear ;
                     sto:hasStatus "Valid"@en ;
                     sto:hasTag "IEC 60255-27:2013 "@en ;
                     dcterms:title "Measuring relays and protection equipment - Part 27: Product safety requirements"@en ;
                     rdfs:comment "IEC 60255-27:2013 describes the product safety requirements for measuring relays and protection equipment having a rated a.c. voltage up to 1 000 V with a rated frequency up to 65 Hz, or a rated d.c. voltage up to 1 500 V. Above these limits, IEC 60664-1 is applicable for the determination of clearance, creepage distance and withstand test voltage. This standard details essential safety requirements to minimize the risk of fire and hazards caused by electric shock or injury to the user. This new edition includes the following significant technical changes with respect to the previous edition:- the removal of tables and diagrams which are from other standards and referring instead directly to the source standard;- all aspects of IEC 60255-5 have been covered and this standard will be withdrawn."@en ;
                     rdfs:label "IEC 60255-27:2013 "@en ;
                     sto:hasOfficialResource <https://webstore.iec.ch/publication/1172> .

sto:IEC_60286 rdf:type owl:NamedIndividual ,
                             sto:Standard ;
                    sto:hasPublisher sto:IEC ;
                    dcterms:title "Packaging of components for automatic handling."@en ;
                    rdfs:comment "In electrical engineering, IEC 60269 is a set of technical standards for low-voltage power fuses."@en ;
                    rdfs:label "IEC 60286"@en.                  

###  https://w3id.org/i40/sto#IEC_60286_P3_E5
sto:IEC_60286_P3_E5 rdf:type owl:NamedIndividual ,
                             sto:Standard ;
                    dcterms:creator sto:irlan ;
                    sto:hasAvailableLanguage lang:eng ,
                                             lang:fra ;
                    sto:hasFileSize sto:FileSizeIEC_60286_P3 ;
                    sto:hasICS sto:ICS_31_020 ,
                               sto:ICS_31_240 ;
                    sto:hasPublisher sto:IEC ;
                    sto:hasTechnicalCommittee sto:TC_40 ;
                    sto:isPartOf sto:IEC_60286;
                    sto:hasEdition "5.0"^^xsd:float ;
                    sto:hasImplementationFormat "Document"@en ;
                    sto:hasPages "77"^^xsd:int ;
                    sto:hasPublicationDate "2013-05-17"^^xsd:date ;
                    sto:hasStabilityDate "2024"^^xsd:gYear ;
                    sto:hasStatus "Valid"@en ;
                    sto:hasTag "IEC 60286-3:2013"@en ;
                    dcterms:title "Packaging of components for automatic handling - Part 3: Packaging of surface mount components on continuous tapes"@en ;
                    rdfs:comment "IEC 60286-3:2013 is applicable to the tape packaging of electronic components without leads or with lead stumps, intended to be connected to electronic circuits. It includes only those dimensions that are essential for the taping of components intended for the above-mentioned purposes. This standard also includes requirements related to the packaging of singulated die products including bare die and bumped die (flip chips). This fifth edition cancels and replaces the fourth edition, published in 2007, as well as IEC 60286-3-1, published in 2009 and IEC 60286-3-2, published in 2009. It constitutes a full layout revision. In addition, this edition includes the following significant technical changes with respect to the previous edition:a) IEC 60286-3:2013 is applicable to the tape packaging of electronic components without leads or with lead stumps, intended to be connected to electronic circuits. It includes only those dimensions that are essential for the taping of components intended for the above-mentioned purposes. This standard also includes requirements related to the packaging of singulated die products including bare die and bumped die (flip chips). This fifth edition cancels and replaces the fourth edition, published in 2007, as well as IEC 60286-3-1, published in 2009 and IEC 60286-3-2, published in 2009.It constitutes a full layout revision. In addition, this edition includes the following significant technical changes with respect to the previous edition:a) integration of IEC 60286-3-1:2009 as type 1b (Packaging of surface mount components on continuous pressed carrier tapes);b) integration of IEC 60286-3-2:2009 as type 2b (Packaging of surface mount components on blister carrier tapes 4 mm in width).ntegration of IEC 60286-3-1:2009 as type 1b (Packaging of surface mount components on continuous pressed carrier tapes);b) integration of IEC 60286-3-2:2009 as type 2b (Packaging of surface mount components on blister carrier tapes 4 mm in width)."@en ;
                    rdfs:label "IEC 60286-3:2013"@en ;
                    sto:hasOfficialResource <https://webstore.iec.ch/publication/1258> .


###  https://w3id.org/i40/sto#IEC_60286_P4_E3
sto:IEC_60286_P4_E3 rdf:type owl:NamedIndividual ,
                             sto:Standard ;
                    dcterms:creator sto:irlan ;
                    sto:hasAvailableLanguage lang:eng ,
                                             lang:fra ;
                    sto:hasFileSize sto:FileSizeIEC_60286_P4 ;
                    sto:hasICS sto:ICS_31_020 ,
                               sto:ICS_31_240 ;
                    sto:hasPublisher sto:IEC ;
                    sto:hasTechnicalCommittee sto:TC_40 ;
                    sto:isPartOf sto:IEC_60286;
                    sto:hasEdition "3.0"^^xsd:float ;
                    sto:hasImplementationFormat "Document"@en ;
                    sto:hasPages "32"^^xsd:int ;
                    sto:hasPublicationDate "2013-07-26"^^xsd:date ;
                    sto:hasStabilityDate "2022"^^xsd:gYear ;
                    sto:hasStatus "Valid"@en ;
                    sto:hasTag "IEC 60286-3:2013"@en ;
                    dcterms:title "Packaging of components for automatic handling - Part 4: Stick magazines for electronic components encapsulated in packages of different forms"@en ;
                    rdfs:comment "IEC 60286-4:2013 is applicable to stick magazines (including end stoppers) intended to be used for storage of electronic components, for transport from the manufacturer to the customer and for in-house use in the manufacturing plant. They are also used to feed automatic placement machines for surface mounting as well as for through-hole mounting of electronic components. This edition includes the following significant technical changes with respect to the previous edition: Clause 4 describes the guidelines for customer specific stick magazine design. It replaces the magazine design rules for IEC outlined components and rules for orientation of components in stick magazines which have been moved to Annexes A to D."@en ;
                    rdfs:label "IEC 60286-4:2013"@en ;
                    sto:hasOfficialResource <https://webstore.iec.ch/publication/1259> .


###  https://w3id.org/i40/sto#IEC_60286_P5_E3
sto:IEC_60286_P5_E3 rdf:type owl:NamedIndividual ,
                             sto:Standard ;
                    dcterms:creator sto:irlan;
                    sto:hasAvailableLanguage lang:eng ;
                    sto:hasFileSize sto:FileSizeIEC_60286_P5 ;
                    sto:hasICS sto:ICS_31_020 ;
                    sto:hasPublisher sto:IEC ;
                    sto:hasTechnicalCommittee sto:TC_40 ;
                    sto:isPartOf sto:IEC_60286;
                    sto:hasEdition "3.0"^^xsd:float ;
                    sto:hasImplementationFormat "Document"@en ;
                    sto:hasPages "71"^^xsd:int ;
                    sto:hasPublicationDate "2018-04-25"^^xsd:date ;
                    sto:hasStabilityDate "2024"^^xsd:gYear ;
                    sto:hasStatus "RLV-Redline version"@en ,
                                  "Valid"@en ;
                    sto:hasTag "IEC 60286-5:2018"@en ;
                    dcterms:title "Packaging of components for automatic handling - Part 5: Matrix trays"@en ;
                    rdfs:comment "IEC 60286-5:2018 RLV contains the International Standard and its Redline version. The Redline version is available in English only. The Redline version provides you with a quick and easy way to compare all the changes between this standard and its previous edition. The Redline version is not an official IEC Standard, only the current version of the standard is to be considered the official document.IEC 60286-5:2018 describes the common dimensions, tolerances and characteristics of the tray. It includes only those dimensions that are essential for the handling of the trays for the stated purpose and for placing or removing components from the trays. This edition includes the following significant technical changes with respect to the previous edition: - The generic rules for the design of matrix trays are given in this document. Newly developed trays which follow these rules will not be listed individually. Only those trays which conform to the design rules set forth herein are classified as 'standard trays' and are thus preferred for use.- An update of the matrix trays, which do not conform to the design rules set forth herein, are considered as 'non-standard trays' and are not preferred for use, is listed in Annex A."@en ;
                    rdfs:label "IEC 60286-5:2018"@en ;
                    sto:hasOfficialResource <https://webstore.iec.ch/publication/63037> .


###  https://w3id.org/i40/sto#IEC_60364
sto:IEC_60364 rdf:type owl:NamedIndividual ,
                       sto:Standard ;
              dcterms:creator sto:irlan;
              sto:hasPublisher sto:IEC ;
              rdfs:comment "Electrical Installations for Buildings is the International Electrotechnical Commission's international standard on electrical installations of buildings"@en ;
              rdfs:label "IEC 60364"@en ;
              sto:hasDBpediaResource <http://dbpedia.org/page/IEC_60364> ;
              sto:hasOfficialResource <https://webstore.iec.ch/publication/1865> ;
              sto:hasWikipediaArticle <https://en.wikipedia.org/wiki/IEC_60364> .

sto:IEC_60381 rdf:type owl:NamedIndividual ,
                             sto:Standard ;
                    sto:hasPublisher sto:IEC ;
                    dcterms:title "Analogue signals for process control systems. "@en ;
                    rdfs:comment "Applicable to analogue direct current signals used in industrial-process measurement and control systems to transmit information between elements of systems. Does not apply to signals used entirely within an element."@en ;
                    rdfs:label "IEC 60381"@en  .

###  https://w3id.org/i40/sto#IEC_60381_P1_E2
sto:IEC_60381_P1_E2 rdf:type owl:NamedIndividual ,
                             sto:Standard ;
                    dcterms:creator sto:irlan ;
                    sto:hasAvailableLanguage lang:eng ,
                                             lang:fra ;
                    sto:hasFileSize sto:FileSizeIEC_60381_P1 ;
                    sto:hasICS sto:ICS_33_200 ;
                    sto:hasPublisher sto:IEC ;
                    sto:hasTechnicalCommittee sto:TC_40 ;
                    sto:isPartOf sto:IEC_60381;
                    sto:hasEdition "2.0"^^xsd:float ;
                    sto:hasImplementationFormat "Document"@en ;
                    sto:hasPages "9"^^xsd:int ;
                    sto:hasPublicationDate "1982-01-01"^^xsd:date ;
                    sto:hasStabilityDate "2018"^^xsd:gYear ;
                    sto:hasStatus "Valid"@en ;
                    sto:hasTag "IEC 60381-1:1982"@en ;
                    dcterms:title "Analogue signals for process control systems. Part 1: Direct current signals"@en ;
                    rdfs:comment "Applicable to analogue direct current signals used in industrial-process measurement and control systems to transmit information between elements of systems. Does not apply to signals used entirely within an element."@en ;
                    rdfs:label "IEC 60381-1:1982"@en ;
                    sto:hasOfficialResource <https://webstore.iec.ch/publication/1948> .


###  https://w3id.org/i40/sto#IEC_60381_P2_E1
sto:IEC_60381_P2_E1 rdf:type owl:NamedIndividual ,
                             sto:Standard ;
                    dcterms:creator sto:irlan ;
                    sto:hasAvailableLanguage lang:eng ,
                                             lang:fra ,
                                             lang:rus ;
                    sto:hasFileSize sto:FileSizeIEC_60381_P2 ;
                    sto:hasICS sto:ICS_33_200 ,
                               sto:ICS_35_240_50 ;
                    sto:hasPublisher sto:IEC ;
                    sto:hasTechnicalCommittee sto:TC_65 ;
                    sto:isPartOf sto:IEC_60381;
                    sto:hasEdition "1.0"^^xsd:float ;
                    sto:hasImplementationFormat "Document"@en ;
                    sto:hasPages "9"^^xsd:int ;
                    sto:hasPublicationDate "1978-01-01"^^xsd:date ;
                    sto:hasStabilityDate "2018"^^xsd:gYear ;
                    sto:hasStatus "Valid"@en ;
                    sto:hasTag "IEC 60381-2:1978"@en ;
                    dcterms:title "Analogue signals for process control systems. Part 2: Direct voltage signals"@en ;
                    rdfs:comment "Applicable to analogue direct voltage signals used in industrial process measurement and control systems. lt specifies ranges of analogue direct voltage signals and the signal common; it also deals with ripple content. The analogue direct voltage signal, unlike the analogue direct current signal specified in IEC 60381-1, is not intended for transmission over long distances. This standard does not apply to signals used entirely within an element."@en ;
                    rdfs:label "IEC 60381-2:1978"@en ;
                    sto:hasOfficialResource <https://webstore.iec.ch/publication/1949> .



###  https://w3id.org/i40/sto#IEC_60382
sto:IEC_60382 rdf:type owl:NamedIndividual ,
                       sto:Standard ;
              dcterms:creator sto:sebastian, 
                              sto:irlan ;
              sto:hasAvailableLanguage lang:eng ,
                                       lang:fra ;
              sto:hasFileSize sto:FileSizeIEC_60382 ;
              sto:hasICS sto:ICS_25_040_40 ;
              sto:hasPublisher sto:IEC ;
              sto:hasTechnicalCommittee sto:TC_65 ;
              sto:hasEdition "2.0"^^xsd:float ;
              sto:hasPages "9"^^xsd:int ;
              sto:hasPublicationDate "1991-11-01"^^xsd:date ;
              sto:hasStabilityDate "2018"^^xsd:gYear ;
              sto:hasTag "IEC 60382:1991"@en ;
              dcterms:title "Analogue pneumatic signal for process control systems"@en ;
              rdfs:comment "Applies to analogue pneumatic signals used in process control systems to transmit information between the elements of systems and gives definitions, units and the recommended value of the range of the analogue pneumatic signal."@en ;
              rdfs:label "IEC 60382:1991"@en ;
              sto:hasOfficialResource <https://webstore.iec.ch/publication/1950> .


###  https://w3id.org/i40/sto#IEC_60382_E2
sto:IEC_60382_E2 rdf:type owl:NamedIndividual ,
                          sto:Standard ;
                 dcterms:creator sto:irlan, 
                                 sto:sebastian ;
                 sto:hasAvailableLanguage lang:eng ,
                                          lang:fra ;
                 sto:hasFileSize sto:FileSizeIEC_60382 ;
                 sto:hasICS sto:ICS_25_040_40 ;
                 sto:hasPublisher sto:IEC ;
                 sto:hasTechnicalCommittee sto:TC_65 ;
                 sto:hasEdition "2.0"^^xsd:float ;
                 sto:hasImplementationFormat "Document"@en ;
                 sto:hasPages "9"^^xsd:int ;
                 sto:hasPublicationDate "1991-11-01"^^xsd:date ;
                 sto:hasStabilityDate "2018"^^xsd:gYear ;
                 sto:hasStatus "Valid"@en ;
                 sto:hasTag "IEC 60382:1991"@en ;
                 dcterms:title "Analogue pneumatic signal for process control systems"@en ;
                 rdfs:comment "Applies to analogue pneumatic signals used in process control systems to transmit information between the elements of systems and gives definitions, units and the recommended value of the range of the analogue pneumatic signal."@en ;
                 rdfs:label "IEC 60382:1991"@en ;
                 sto:hasOfficialResource <https://webstore.iec.ch/publication/1950> .


sto:IEC_60839 rdf:type owl:NamedIndividual ,
                                sto:Standard ;
                       sto:hasPublisher sto:IEC ;
                       dcterms:title "Alarm and electronic security systems"@en ;
                       rdfs:comment "General equipment requirements for the performance, reliability, resilience, security and safety characteristics of supervised premises transceiver (SPT) installed in supervised premises and used in alarm transmission systems (ATS)."@en ;
                       rdfs:label "IEC 60839"@en  .

###  https://w3id.org/i40/sto#IEC_60839_P5_S2_E2
sto:IEC_60839_P5_S2_E2 rdf:type owl:NamedIndividual ,
                                sto:Standard ;
                       dcterms:creator sto:irlan;
                       sto:hasAvailableLanguage lang:eng ,
                                                lang:fra ;
                       sto:hasClassification sto:AsSecurity ,
                                             sto:RamiCommunicationlayer ,
                                             sto:RamiControlDevice ,
                                             sto:RamiFieldDevice ;
                       sto:hasFileSize sto:FileSizeIEC_60839_P5_S2 ;
                       sto:hasICS sto:ICS_13_320 ;
                       sto:hasPublisher sto:IEC ;
                       sto:hasTechnicalCommittee sto:TC_79 ;
                       sto:isPartOf sto:IEC_60839;
                       sto:hasEdition "2.0"^^xsd:float ;
                       sto:hasImplementationFormat "Document"@en ;
                       sto:hasPages "63"^^xsd:int ;
                       sto:hasPublicationDate "2016-02-03"^^xsd:date ;
                       sto:hasStabilityDate "2019"^^xsd:gYear ;
                       sto:hasStatus "Valid"@en ;
                       sto:hasTag "IEC 60839-5-2:2016"@en ;
                       dcterms:title "Alarm and electronic security systems - Part 5-2: Alarm transmission systems - Requirements for supervised premises transceiver (SPT)"@en ;
                       rdfs:comment "IEC 60839-5-2:2016 specifies the general equipment requirements for the performance, reliability, resilience, security and safety characteristics of supervised premises transceiver (SPT) installed in supervised premises and used in alarm transmission systems (ATS). A supervised premises transceiver can be a stand-alone device or an integrated part of an alarm system. These requirements also apply to the SPT sharing means of interconnection, control, communication and power supplies with other applications. The alarm transmission system requirements and classifications are defined within IEC 60839-5-1. This new edition includes the following significant technical changes with respect to the previous edition: reflects the current technological state of art (IP networks) ,harmonizes with the ATS categories introduced in IEC 60839-5-1:2014; introduces test requirements."@en ;
                       rdfs:label "IEC 60839-5-2:2016"@en ;
                       sto:hasOfficialResource <https://webstore.iec.ch/publication/24120> .


###  https://w3id.org/i40/sto#IEC_60839_P7_S1_E1
sto:IEC_60839_P7_S1_E1 rdf:type owl:NamedIndividual ,
                                sto:Standard ;
                       dcterms:creator sto:irlan;
                       sto:hasAvailableLanguage lang:eng ,
                                                lang:fra ;
                       sto:hasFileSize sto:FileSizeIEC_60839_P7_S1 ;
                       sto:hasICS sto:ICS_13_320 ;
                       sto:hasPublisher sto:IEC ;
                       sto:hasTechnicalCommittee sto:TC_79 ;
                       sto:isPartOf sto:IEC_60839;
                       sto:hasEdition "1.0"^^xsd:float ;
                       sto:hasPages "39"^^xsd:int ;
                       sto:hasPublicationDate "2001-03-09"^^xsd:date ;
                       sto:hasStabilityDate "2018"^^xsd:gYear ;
                       sto:hasTag "IEC 60839-7-1:2001"@en ;
                       dcterms:title "Alarm systems - Part 7-1: Message formats and protocols for serial data interfaces in alarm transmission systems – General"@en ;
                       rdfs:comment "Describes the requirements for standard serial data interfaces in alarm transmission systems. Gives an outline of how alarm transmission systems are connected and the various types of serial data interfaces that might be employed."@en ;
                       rdfs:label "IEC 60839-7-1:2001"@en ;
                       sto:hasOfficialResource <https://webstore.iec.ch/publication/3666> ;
                       sto:hasStatus "Valid"@en .


###  https://w3id.org/i40/sto#IEC_60839_P7_S2_E1
sto:IEC_60839_P7_S2_E1 rdf:type owl:NamedIndividual ,
                                sto:Standard ;
                       dcterms:creator sto:irlan;
                       sto:hasAvailableLanguage lang:eng ,
                                                lang:fra ;
                       sto:hasFileSize sto:FileSizeIEC_60839_P7_S2 ;
                       sto:hasICS sto:ICS_13_320 ;
                       sto:hasPublisher sto:IEC ;
                       sto:hasTechnicalCommittee sto:TC_79 ;
                       sto:isPartOf sto:IEC_60839;
                       sto:hasEdition "1.0"^^xsd:float ;
                       sto:hasPages "53"^^xsd:int ;
                       sto:hasPublicationDate "2001-03-09"^^xsd:date ;
                       sto:hasStabilityDate "2018"^^xsd:gYear ;
                       sto:hasTag "IEC 60839-7-2:2001"@en ;
                       dcterms:title "Alarm systems - Part 7-2: Message formats and protocols for serial data interfaces in alarm transmission systems - Common application layer protocol"@en ;
                       rdfs:comment "Specifies a common application layer protocol (message structure, formats and transmission procedures) to be used at standard interfaces in alarm transmission systems. Should be used at all such interfaces where equipment from one supplier is intended to inter-work with equipment from other suppliers."@en ;
                       rdfs:label "IEC 60839-7-2:2001"@en ;
                       sto:hasOfficialResource <https://webstore.iec.ch/publication/3669> ;
                       sto:hasStatus "Valid"@en .


###  https://w3id.org/i40/sto#IEC_60839_P7_S3_E1
sto:IEC_60839_P7_S3_E1 rdf:type owl:NamedIndividual ,
                                sto:Standard ;
                       dcterms:creator sto:irlan;
                       sto:hasAvailableLanguage lang:eng ,
                                                lang:fra ;
                       sto:hasFileSize sto:FileSizeIEC_60839_P7_S3 ;
                       sto:hasICS sto:ICS_13_320 ;
                       sto:hasPublisher sto:IEC ;
                       sto:hasTechnicalCommittee sto:TC_79 ;
                       sto:isPartOf sto:IEC_60839;
                       sto:hasEdition "1.0"^^xsd:float ;
                       sto:hasPages "29"^^xsd:int ;
                       sto:hasPublicationDate "2001-03-09"^^xsd:date ;
                       sto:hasStabilityDate "2018"^^xsd:gYear ;
                       sto:hasTag "IEC 60839-7-3:2001"@en ;
                       dcterms:title "Alarm systems - Part 7-3: Message formats and protocols for serial data interfaces in alarm transmission systems - Common data link layer protocol"@en ;
                       rdfs:comment "Specifies the data link layer message structure, formats and transmission procedures which should be used at standard serial data interfaces in alarm transmission systems where the transmission network employed does not offer a standard protocol. Is necessary in order to ensure compatibility of equipment from different suppliers."@en ;
                       rdfs:label "IEC 60839-7-3:2001"@en ;
                       sto:hasOfficialResource <https://webstore.iec.ch/publication/3671> ;
                       sto:hasStatus "Valid"@en .


###  https://w3id.org/i40/sto#IEC_60839_P7_S4_E1
sto:IEC_60839_P7_S4_E1 rdf:type owl:NamedIndividual ,
                                sto:Standard ;
                       dcterms:creator sto:irlan;
                       sto:hasAvailableLanguage lang:eng ,
                                                lang:fra ;
                       sto:hasFileSize sto:FileSizeIEC_60839_P7_S4 ;
                       sto:hasICS sto:ICS_13_320 ;
                       sto:hasPublisher sto:IEC ;
                       sto:hasTechnicalCommittee sto:TC_79 ;
                       sto:isPartOf sto:IEC_60839;
                       sto:hasEdition "1.0"^^xsd:float ;
                       sto:hasPages "23"^^xsd:int ;
                       sto:hasPublicationDate "2001-03-09"^^xsd:date ;
                       sto:hasStabilityDate "2018"^^xsd:gYear ;
                       sto:hasTag "IEC 60839-7-4:2001"@en ;
                       dcterms:title "Alarm systems - Part 7-4: Message formats and protocols for serial data interfaces in alarm transmission systems - Common transport layer protocol"@en ;
                       rdfs:comment "Specifies the transport layer message structure, formats and transmission procedures to be used at standard interfaces in alarm transmission systems. Should be used at all such interfaces where equipment from one supplier is intended to inter-work with equipment from other suppliers, and where the underlying system architecture does not provide the necessary facilities to support the common application layer."@en ;
                       rdfs:label "IEC 60839-7-4:2001"@en ;
                       sto:hasOfficialResource <https://webstore.iec.ch/publication/3672> ;
                       sto:hasStatus "Valid"@en .


###  https://w3id.org/i40/sto#IEC_60839_P7_S5_E1
sto:IEC_60839_P7_S5_E1 rdf:type owl:NamedIndividual ,
                                sto:Standard ;
                       dcterms:creator sto:irlan;
                       sto:hasAvailableLanguage lang:eng ,
                                                lang:fra ;
                       sto:hasFileSize sto:FileSizeIEC_60839_P7_S5 ;
                       sto:hasICS sto:ICS_13_320 ;
                       sto:hasPublisher sto:IEC ;
                       sto:hasTechnicalCommittee sto:TC_79 ;
                       sto:isPartOf sto:IEC_60839;
                       sto:hasEdition "1.0"^^xsd:float ;
                       sto:hasPages "13"^^xsd:int ;
                       sto:hasPublicationDate "2001-03-09"^^xsd:date ;
                       sto:hasStabilityDate "2018"^^xsd:gYear ;
                       sto:hasTag "IEC 60839-7-5:2001"@en ;
                       dcterms:title "Alarm systems - Part 7-5: Message formats and protocols for serial data interfaces in alarm transmission systems - Alarm system interfaces employing a two-wire configuration in accordance with ISO/IEC 8482"@en ;
                       rdfs:comment "Specifies the requirements for standard interfaces using a two-wire connection employing ISO/IEC 8482 signalling for use between the control and indicating equipment of an alarm system and one or more alarm system transceivers connected to alarm transmission systems."@en ;
                       rdfs:label "IEC 60839-7-5:2001"@en ;
                       sto:hasOfficialResource <https://webstore.iec.ch/publication/3673> ;
                       sto:hasStatus "Valid"@en .


###  https://w3id.org/i40/sto#IEC_60839_P7_S6_E1
sto:IEC_60839_P7_S6_E1 rdf:type owl:NamedIndividual ,
                                sto:Standard ;
                       dcterms:creator sto:irlan;
                       sto:hasAvailableLanguage lang:eng ,
                                                lang:fra ;
                       sto:hasFileSize sto:FileSizeIEC_60839_P7_S6 ;
                       sto:hasICS sto:ICS_13_320 ;
                       sto:hasPublisher sto:IEC ;
                       sto:hasTechnicalCommittee sto:TC_79 ;
                       sto:isPartOf sto:IEC_60839;
                       sto:hasEdition "1.0"^^xsd:float ;
                       sto:hasPages "9"^^xsd:int ;
                       sto:hasPublicationDate  "2001-03-09"^^xsd:date ;
                       sto:hasStabilityDate "2018"^^xsd:gYear ;
                       sto:hasTag "IEC 60839-7-6:2001"@en ;
                       dcterms:title "Alarm systems - Part 7-6: Message formats and protocols for serial data interfaces in alarm transmission systems - Alarm system interfaces employing ITU-T Recommendation V.24/V.28 signalling"@en ;
                       rdfs:comment "Specifies the requirements for standard interfaces employing ITU-T V.24/V.28 signalling for communications between the control and indicating equipment of an alarm system and transmission equipment used for remote communications, where the transmission equipment is general purpose equipment. Is intended to be used as interfacing to standard modems, packet switching networks, X.25 PADs, etc."@en ;
                       rdfs:label "IEC 60839-7-6:2001"@en ;
                       sto:hasOfficialResource <https://webstore.iec.ch/publication/3674> ;
                       sto:hasStatus "Valid"@en .


###  https://w3id.org/i40/sto#IEC_60839_P7_S7_E1
sto:IEC_60839_P7_S7_E1 rdf:type owl:NamedIndividual ,
                                sto:Standard ;
                       dcterms:creator sto:irlan;
                       sto:hasAvailableLanguage lang:eng ,
                                                lang:fra ;
                       sto:hasFileSize sto:FileSizeIEC_60839_P7_S7 ;
                       sto:hasICS sto:ICS_13_320 ;
                       sto:hasPublisher sto:IEC ;
                       sto:hasTechnicalCommittee sto:TC_79 ;
                       sto:isPartOf sto:IEC_60839;
                       sto:hasEdition "1.0"^^xsd:float ;
                       sto:hasPages "21"^^xsd:int ;
                       sto:hasPublicationDate "2001-03-09"^^xsd:date ;
                       sto:hasStabilityDate "2018"^^xsd:gYear ;
                       sto:hasTag "IEC 60839-7-7:2001"@en ;
                       dcterms:title "Alarm systems - Part 7-7: Message formats and protocols for serial data interfaces in alarm transmission systems - Alarm system interfaces for plug-in alarm system transceivers"@en ;
                       rdfs:comment "Specifies the requirements for standard interfaces between the control and indicating equipment (CIE) of an alarm system and an alarm system transceiver where the alarm system transceiver is intended to plug into a standard space inside the CIE of the alarm system."@en ;
                       rdfs:label "IEC 60839-7-7:2001"@en ;
                       sto:hasOfficialResource <https://webstore.iec.ch/publication/3675> ;
                       sto:hasStatus "Valid"@en .


###  https://w3id.org/i40/sto#IEC_60848_E3
sto:IEC_60848_E3 rdf:type owl:NamedIndividual ,
                          sto:Standard ;
                 dcterms:creator sto:irlan;
                 sto:hasAvailableLanguage lang:eng ,
                                          lang:fra ;
                 sto:hasFileSize sto:FileSizeIEC_60848 ;
                 sto:hasICS sto:ICS_29_020 ;
                 sto:hasPublisher sto:IEC ;
                 sto:hasTechnicalCommittee sto:TC_3 ;
                 sto:hasEdition "3.0"^^xsd:float ;
                 sto:hasPages "109"^^xsd:int ;
                 sto:hasPublicationDate "2013-02-27"^^xsd:date ;
                 sto:hasStabilityDate "2020"^^xsd:gYear ;
                 sto:hasTag "IEC 60848:2013"@en ;
                 dcterms:title "GRAFCET specification language for sequential function charts"@en ;
                 rdfs:comment "IEC 60848:2013 defines the GRAFCET specification language for the functional description of the behaviour of the sequential part of a control system. It specifies the symbols and rules for the graphical representation of this language, as well as for its interpretation and has been prepared for automated production systems of industrial applications. This third edition cancels and replaces the second edition published in 2002 and constitutes a global technical revision with the extended definition of the concept of variables introducing: internal variable, input variable and output variable."@en ;
                 rdfs:label "IEC 60848:2013"@en ;
                 sto:hasOfficialResource <https://webstore.iec.ch/publication/3684> ;
                 sto:hasStatus "Valid"@en .

sto:IEC_60864 rdf:type owl:NamedIndividual ,
                             sto:Standard ;
                    sto:hasPublisher sto:IEC ;
                    dcterms:title "Standardization of interconnections between broadcasting transmitters or transmitter systems and supervisory equipment. "@en ;
                    rdfs:comment "Applies to all classes of transmitters for sound and television broadcasting. Deals with the interface between a transmitter (or system of transmitters) and the supervisory equipment which is intended to remotely monitor and/or control the transmitter(s). "@en ;
                    rdfs:label "IEC 60864 "@en ;
                    sto:hasOfficialResource <https://webstore.iec.ch/publication/3727> ;
                    sto:hasStatus "Valid"@en .

###  https://w3id.org/i40/sto#IEC_60864_P1_E1
sto:IEC_60864_P1_E1 rdf:type owl:NamedIndividual ,
                             sto:Standard ;
                    dcterms:creator sto:irlan;
                    sto:hasAvailableLanguage lang:eng ,
                                             lang:fra ;
                    sto:hasFileSize sto:FileSizeIEC_60864_P1 ;
                    sto:hasICS sto:ICS_33_060_20 ,
                               sto:ICS_33_200 ;
                    sto:hasPublisher sto:IEC ;
                    sto:hasTechnicalCommittee sto:TC_103 ;
                    sto:isPartOf sto:IEC_60864;
                    sto:hasEdition "1.0"^^xsd:float ;
                    sto:hasPages "43"^^xsd:int ;
                    sto:hasPublicationDate "1986-01-01"^^xsd:date ;
                    sto:hasStabilityDate "2020"^^xsd:gYear ;
                    sto:hasTag "IEC 60864-1:1986 "@en ;
                    dcterms:title "Standardization of interconnections between broadcasting transmitters or transmitter systems and supervisory equipment. Part 1: Interface standards for systems using dedicated interconnections"@en ;
                    rdfs:comment "Applies to all classes of transmitters for sound and television broadcasting. Deals with the interface between a transmitter (or system of transmitters) and the supervisory equipment which is intended to remotely monitor and/or control the transmitter(s). Details the interconnections and facilities to be provided with a view to achieving compatibility between different types and makes of transmitters and supervisory equipment."@en ;
                    rdfs:label "IEC 60864-1:1986 "@en ;
                    sto:hasOfficialResource <https://webstore.iec.ch/publication/3727> ;
                    sto:hasStatus "Valid"@en .


###  https://w3id.org/i40/sto#IEC_60864_P2_E1
sto:IEC_60864_P2_E1 rdf:type owl:NamedIndividual ,
                             sto:Standard ;
                    dcterms:creator sto:sebastian , 
                                    sto:irlan ;
                    sto:hasAvailableLanguage lang:eng ,
                                             lang:fra ;
                    sto:hasFileSize sto:FileSizeIEC_60864_P2 ;
                    sto:hasICS sto:ICS_33_060_20 ,
                               sto:ICS_33_200 ;
                    sto:hasPublisher sto:IEC ;
                    sto:hasTechnicalCommittee sto:TC_103 ;
                    sto:isPartOf sto:IEC_60864;
                    sto:hasEdition "1.0"^^xsd:float ;
                    sto:hasPages "79"^^xsd:int ;
                    sto:hasPublicationDate "1997-06-17"^^xsd:date ;
                    sto:hasStabilityDate "2020"^^xsd:gYear ;
                    sto:hasTag "IEC 60864-2:1997"@en ;
                    dcterms:title "Standardization of interconnections between broadcasting transmitters or transmitter systems and supervisory equipment - Part 2: Interface standards for systems using data bus type interconnections"@en ;
                    rdfs:comment "Deals with the interface between a transmitter (or system of transmitters) and the supervisory equipment which is entended to remotely monitor and/or control the transmitter(s). It details the interconnections and facilities to be provided with a view to achieving compatibility between different types and makes of transmitters and supervisory equipement."@en ,
                                 "Deals with the itnerface between a transmitter (or system of transmitters) and the supervisory equipment which is entended to remotely monitor and/or control the transmitter(s). It details the interconnections and facilities to be provided with a view to achieving compatibility between different types and makes of transmitters and supervisory equipement."@en ;
                    rdfs:label "IEC 60864-2:1997"@en ;
                    sto:hasOfficialResource <https://webstore.iec.ch/publication/3728> ;
                    sto:hasStatus "Valid"@en .


###  https://w3id.org/i40/sto#IEC_60870
sto:IEC_60870 rdf:type owl:NamedIndividual ,
                       sto:Standard ;
              dcterms:creator sto:irlan ;
              sto:hasPublisher sto:IEC ;
              rdfs:comment "In electrical engineering and power system automation, the IEC 60870 series define systems used for telecontrol (supervisory control and data acquisition)"@en ;
              rdfs:label "IEC 60870"@en ;
              sto:hasDBpediaResource <http://dbpedia.org/page/IEC_60870> ;
              sto:hasWikipediaArticle <https://en.wikipedia.org/wiki/IEC_60870> .


###  https://w3id.org/i40/sto#IEC_60870_P2_S1_E2
sto:IEC_60870_P2_S1_E2 rdf:type owl:NamedIndividual ,
                                sto:Standard ;
                       dcterms:creator sto:irlan ;
                       sto:hasAvailableLanguage lang:eng ,
                                                lang:fra ,
                                                lang:spa ;
                       sto:hasFileSize sto:FileSizeIEC_60870_P2_S1 ;
                       sto:isPartOf sto:IEC_60870 ;
                       sto:hasICS sto:ICS_29_020 ,
                                  sto:ICS_33_100_10 ,
                                  sto:ICS_33_200 ;
                       sto:hasPublisher sto:IEC ;
                       sto:hasTechnicalCommittee sto:TC_57 ;
                       sto:hasEdition "2.0"^^xsd:float ;
                       sto:hasPages "43"^^xsd:int ;
                       sto:hasPublicationDate "1995-12-08"^^xsd:date ;
                       sto:hasStabilityDate "2018"^^xsd:gYear ;
                       sto:hasTag "IEC 60870-2-1:1995"@en ;
                       dcterms:title "Telecontrol equipment and systems - Part 2: Operating conditions - Section 1: Power supply and electromagnetic compatibility"@en ;
                       rdfs:comment "Specifies classes for environmental conditions under which telecontrol equipment has to operate."@en ;
                       rdfs:label "IEC 60870-2-1:1995"@en ;
                       sto:hasDBpediaResource <https://dbpedia.org/resource/IEC_60870> ;
                       sto:hasOfficialResource <https://webstore.iec.ch/publication/3738> ;
                       sto:hasWikipediaArticle <https://en.wikipedia.org/wiki/IEC_60870> ;
                       sto:hasStatus "Valid"@en .


###  https://w3id.org/i40/sto#IEC_60870_P2_S2_E1
sto:IEC_60870_P2_S2_E1 rdf:type owl:NamedIndividual ,
                                sto:Standard ;
                       dcterms:creator sto:irlan ,
                                       sto:sebastian ;
                       sto:hasAvailableLanguage lang:eng ,
                                                lang:fra ,
                                                lang:spa ;
                       sto:hasFileSize sto:FileSizeIEC_60870_P2_S2 ;
                       sto:hasICS sto:ICS_29_020 ,
                                  sto:ICS_33_200 ;
                       sto:hasPublisher sto:IEC ;
                       sto:hasTechnicalCommittee sto:TC_57 ;
                       sto:isPartOf sto:IEC_60870 ;
                       sto:relatedTo sto:IEC_60870_P2_S1_E2 ;
                       sto:hasEdition "1.0"^^xsd:float ;
                       sto:hasPages "33"^^xsd:int ;
                       sto:hasPublicationDate "1996-08-19"^^xsd:date ;
                       sto:hasStabilityDate "2018"^^xsd:gYear ;
                       sto:hasTag "IEC 60870-2-2:1996"@en ;
                       dcterms:title "Telecontrol equipment and systems - Part 2: Operating conditions -Section 2: Environmental conditions (climatic, mechanical and othernon electrical influences)"@en ;
                       rdfs:comment "Applies to telecontrol equipment and systems with coded bit serial data transmission for monitoring and control of geographically wides pread processes. Specifies classes for environmental conditions under which the various components of the systems have to operate."@en ;
                       rdfs:label "IEC 60870-2-2:1996"@en ;
                       sto:hasDBpediaResource <https://dbpedia.org/resource/IEC_60870> ;
                       sto:hasOfficialResource <https://webstore.iec.ch/publication/3739> ;
                       sto:hasWikipediaArticle <https://en.wikipedia.org/wiki/IEC_60870> ;
                       sto:hasStatus "Valid"@en .


###  https://w3id.org/i40/sto#IEC_60870_P5_S101_E2_1
sto:IEC_60870_P5_S101_E2_1 rdf:type owl:NamedIndividual ,
                                    sto:Standard ;
                           dcterms:creator sto:irlan ;
                           sto:hasAvailableLanguage lang:eng ;
                           sto:hasFileSize sto:FileSizeIEC_60870_P5_S101 ;
                           sto:hasICS sto:ICS_33_200 ;
                           sto:hasPublisher sto:IEC ;
                           sto:hasTechnicalCommittee sto:TC_57 ;
                           sto:isPartOf sto:IEC_60870 ;
                           sto:relatedTo sto:IEC_60870_P2_S1_E2 ;
                           sto:hasEdition "2.1"^^xsd:float ;
                           sto:hasPages "360"^^xsd:int ;
                           sto:hasPublicationDate "2015-11-30"^^xsd:date ;
                           sto:hasStabilityDate "2018"^^xsd:gYear ;
                           sto:hasTag "IEC 60870-5-101:2003"@en ;
                           dcterms:title "Telecontrol equipment and systems - Part 5-101: Transmissionprotocols - Companion standard for basic telecontrol tasks"@en ;
                           rdfs:comment """IEC 60870-5-101:2003+A1:2015 Applies to telecontrol equipment and systems with coded bit serial data transmission for monitoring and controlling geographically widespread processes. Defines a telecontrol companion standard that enables interoperability among compatible telecontrol equipment. The defined telecontrol companion standard utilizes standards of the IEC 60870-5 series of documents. 
This publication is of high relevance for Smart Grid. This consolidated version consists of the second edition (2003) and its amendment 1 (2015). Therefore, no need to order amendment in addition to this publication."""@en ,
                                        "IEC 60870-5-101:2003+A1:2015 Applies to telecontrol equipment and systems with coded bit serial data transmission for monitoring and controlling geographically widespread processes. Defines a telecontrol companion standard that enables interoperability among compatible telecontrol equipment. The defined telecontrol companion standard utilizes standards of the IEC 60870-5 series of documents. This publication is of high relevance for Smart Grid. This consolidated version consists of the second edition (2003) and its amendment 1 (2015). Therefore, no need to order amendment in addition to this publication."@en ,
                                        "IEC 60870-5-101:2003+A1:2015 Applies to telecontrol equipment and systems with coded bit serial data transmission for monitoring and controlling geographically widespread processes. Defines a telecontrol companion standard that enables interoperability among compatible telecontrol equipment. The defined telecontrol companion standard utilizes standards of the IEC 60870-5 series of documents. nThis publication is of high relevance for Smart Grid. This consolidated version consists of the second edition (2003) and its amendment 1 (2015). Therefore, no need to order amendment in addition to this publication."@en ;
                           rdfs:label "IEC 60870-5-101:2003"@en ;
                           sto:hasDBpediaResource <https://dbpedia.org/resource/IEC_60870> ;
                           sto:hasOfficialResource <https://webstore.iec.ch/publication/23822> ;
                           sto:hasWikipediaArticle <https://en.wikipedia.org/wiki/IEC_60870> ;
                           sto:hasStatus "Valid"@en .


###  https://w3id.org/i40/sto#IEC_60870_P5_S102_E1
sto:IEC_60870_P5_S102_E1 rdf:type owl:NamedIndividual ,
                                  sto:Standard ;
                         dcterms:creator sto:irlan ;
                         sto:hasAvailableLanguage lang:eng ,
                                                  lang:fra ;
                         sto:hasFileSize sto:FileSizeIEC_60870_P5_S102 ;
                         sto:hasICS sto:ICS_33_200 ;
                         sto:hasPublisher sto:IEC ;
                         sto:hasTechnicalCommittee sto:TC_57 ;
                         sto:isPartOf sto:IEC_60870 ;
                         sto:relatedTo sto:IEC_60870_P2_S1_E2 ;
                         sto:hasEdition "1.0"^^xsd:float ;
                         sto:hasPages "99"^^xsd:int ;
                         sto:hasPublicationDate "1996-06-18"^^xsd:date ;
                         sto:hasStabilityDate "2018"^^xsd:gYear ;
                         sto:hasTag "IEC 60870-5-102:1996"@en ;
                         dcterms:title "Telecontrol equipment and systems - Part 5: Transmission protocols - Section 102: Companion standard for the transmission of integrated totals in electric power systems"@en ;
                         rdfs:comment """Standardizes the transmission of integrated totals representing the amount of electrical energy transferred between power utilities, or between a power utility and independent producers on a high voltage or medium voltage network.
This publication is of high relevance for Smart Grid."""@en ,
                                      "Standardizes the transmission of integrated totals representing the amount of electrical energy transferred between power utilities, or between a power utility and independent producers on a high voltage or medium voltage network.nThis publication is of high relevance for Smart Grid."@en ;
                         rdfs:label "IEC 60870-5-102:1996"@en ;
                         sto:hasDBpediaResource <https://dbpedia.org/resource/IEC_60870> ;
                         sto:hasOfficialResource <https://webstore.iec.ch/publication/3744> ;
                         sto:hasWikipediaArticle <https://en.wikipedia.org/wiki/IEC_60870> ;
                         sto:hasStatus "Valid"@en .


###  https://w3id.org/i40/sto#IEC_60870_P5_S103_E1
sto:IEC_60870_P5_S103_E1 rdf:type owl:NamedIndividual ,
                                  sto:Standard ;
                         dcterms:creator sto:irlan ;
                         sto:hasAvailableLanguage lang:eng ,
                                                  lang:fra ;
                         sto:hasFileSize sto:FileSizeIEC_60870_P5_S103 ;
                         sto:hasICS sto:ICS_33_200 ;
                         sto:hasPublisher sto:IEC ;
                         sto:hasTechnicalCommittee sto:TC_57 ;
                         sto:isPartOf sto:IEC_60870 ;
                         sto:relatedTo sto:IEC_60870_P2_S1_E2 ;
                         sto:hasEdition "1.0"^^xsd:float ;
                         sto:hasPages "203"^^xsd:int ;
                         sto:hasPublicationDate "1997-12-11"^^xsd:date ;
                         sto:hasStabilityDate "2018"^^xsd:gYear ;
                         sto:hasTag "IEC 60870-5-103:1997"@en ;
                         dcterms:title "Telecontrol equipment and systems - Part 5-103: Transmission protocols - Companion standard for the informative interface of protection equipment"@en ;
                         rdfs:comment """Applies to protection equipment with coded bit serial data transmission for exchanging information with control systems. Defines a companion standard that enables interoperability between protection equipment and devices of a control system in a substation.
This publication is of high relevance for Smart Grid."""@en ,
                                      "Applies to protection equipment with coded bit serial data transmission for exchanging information with control systems. Defines a companion standard that enables interoperability between protection equipment and devices of a control system in a substation.nThis publication is of high relevance for Smart Grid."@en ;
                         rdfs:label "IEC 60870-5-103:1997"@en ;
                         sto:hasDBpediaResource <https://dbpedia.org/resource/IEC_60870> ;
                         sto:hasOfficialResource <https://webstore.iec.ch/publication/3745> ;
                         sto:hasWikipediaArticle <https://en.wikipedia.org/wiki/IEC_60870> ;
                         sto:hasStatus "Valid"@en .


###  https://w3id.org/i40/sto#IEC_60870_P5_S104_E2_1
sto:IEC_60870_P5_S104_E2_1 rdf:type owl:NamedIndividual ,
                                    sto:Standard ;
                           dcterms:creator sto:irlan ;
                           sto:hasAvailableLanguage lang:eng ,
                                                    lang:fra ;
                           sto:hasFileSize sto:FileSizeIEC_60870_P5_S104 ;
                           sto:hasICS sto:ICS_33_200 ;
                           sto:hasPublisher sto:IEC ;
                           sto:hasTechnicalCommittee sto:TC_57 ;
                           sto:isPartOf sto:IEC_60870 ;
                           sto:relatedTo sto:IEC_60870_P2_S1_E2 ;
                           sto:hasEdition "2.1"^^xsd:float ;
                           sto:hasPages "281"^^xsd:int ;
                           sto:hasPublicationDate "2016-06-07"^^xsd:date ;
                           sto:hasStabilityDate "2018"^^xsd:gYear ;
                           sto:hasTag "IEC 60870-5-104:2006"@en ;
                           dcterms:title "Telecontrol equipment and systems - Part 5-104: Transmission protocols - Network access for IEC 60870-5-101 using standardtransport profiles"@en ;
                           rdfs:comment """IEC 60870-5-104:2006+A1:2016 Defines a telecontrol companion standard that enables interoperability among compatible telecontrol equipment. Applies to telecontrol equipment and systems with coded bit serial data transmission for monitoring and controlling geographically widespread processes. 
This publication is of high relevance for Smart Grid. This consolidated version consists of the second edition (2006) and its amendment 1 (2012). Therefore, no need to order amendment in addition to this publication."""@en ,
                                        "IEC 60870-5-104:2006+A1:2016 Defines a telecontrol companion standard that enables interoperability among compatible telecontrol equipment. Applies to telecontrol equipment and systems with coded bit serial data transmission for monitoring and controlling geographically widespread processes. nThis publication is of high relevance for Smart Grid. This consolidated version consists of the second edition (2006) and its amendment 1 (2012). Therefore, no need to order amendment in addition to this publication."@en ;
                           rdfs:label "IEC 60870-5-104:2006"@en ;
                           sto:hasDBpediaResource <https://dbpedia.org/resource/IEC_60870> ;
                           sto:hasOfficialResource <https://webstore.iec.ch/publication/25035> ;
                           sto:hasWikipediaArticle <https://en.wikipedia.org/wiki/IEC_60870> ;
                           sto:hasStatus "Valid"@en .


###  https://w3id.org/i40/sto#IEC_60870_P5_S1_E1
sto:IEC_60870_P5_S1_E1 rdf:type owl:NamedIndividual ,
                                sto:Standard ;
                       dcterms:creator sto:irlan ;
                       sto:hasAvailableLanguage lang:eng ,
                                                lang:fra ;
                       sto:hasFileSize sto:FileSizeIEC_60870_P5_S1 ;
                       sto:hasICS sto:ICS_33_200 ;
                       sto:hasPublisher sto:IEC ;
                       sto:hasTechnicalCommittee sto:TC_57 ;
                       sto:isPartOf sto:IEC_60870 ;
                       sto:relatedTo sto:IEC_60870_P2_S1_E2 ;
                       sto:hasEdition "1.0"^^xsd:float ;
                       sto:hasPages "79"^^xsd:int ;
                       sto:hasPublicationDate "1990-02-01"^^xsd:date ;
                       sto:hasStabilityDate "2018"^^xsd:gYear ;
                       sto:hasTag "IEC 60870-5-1:1990"@en ;
                       dcterms:title "Telecontrol equipment and systems. Part 5: Transmission protocols - Section One: Transmission frame formats"@en ;
                       rdfs:comment "Covers asynchronous data transmission with half duplex and duplex link protocols operating with window size one for message transfers. Specifies the basic requirements for services to be provided by the link plus physical layers, for telecontrol applications. In particular it specifies standards on coding, formatting and synchronizing data frames of variable and filed lengths which meet specified data integrity requirements."@en ;
                       rdfs:label "IEC 60870-5-1:1990"@en ;
                       sto:hasDBpediaResource <https://dbpedia.org/resource/IEC_60870> ;
                       sto:hasOfficialResource <https://webstore.iec.ch/publication/3742> ;
                       sto:hasWikipediaArticle <https://en.wikipedia.org/wiki/IEC_60870> ;
                       sto:hasStatus "Valid"@en .


###  https://w3id.org/i40/sto#IEC_60870_P5_S2_E1
sto:IEC_60870_P5_S2_E1 rdf:type owl:NamedIndividual ,
                                sto:Standard ;
                       dcterms:creator sto:irlan ;
                       sto:hasAvailableLanguage lang:eng ,
                                                lang:fra ;
                       sto:hasFileSize sto:FileSizeIEC_60870_P5_S2 ;
                       sto:hasICS sto:ICS_33_200 ;
                       sto:hasPublisher sto:IEC ;
                       sto:hasTechnicalCommittee sto:TC_57 ;
                       sto:isPartOf sto:IEC_60870 ;
                       sto:relatedTo sto:IEC_60870_P2_S1_E2 ;
                       sto:hasEdition "1.0"^^xsd:float ;
                       sto:hasPages "99"^^xsd:int ;
                       sto:hasPublicationDate "1992-04-30"^^xsd:date ;
                       sto:hasStabilityDate "2018"^^xsd:gYear ;
                       sto:hasTag "IEC 60870-5-2:1992"@en ;
                       dcterms:title "Telecontrol equipment and systems - Part 5: Transmission protocols - Section 2: Link transmission procedures"@en ;
                       rdfs:comment """Applies to telecontrol equipment and systems with coded bit serial data transmission for monitoring and controlling geographically widespread processes. 
This publication is of high relevance for Smart Grid."""@en ,
                                    "Applies to telecontrol equipment and systems with coded bit serial data transmission for monitoring and controlling geographically widespread processes. nThis publication is of high relevance for Smart Grid."@en ;
                       rdfs:label "IEC 60870-5-2:1992"@en ;
                       sto:hasDBpediaResource <https://dbpedia.org/resource/IEC_60870> ;
                       sto:hasOfficialResource <https://webstore.iec.ch/publication/3747> ;
                       sto:hasWikipediaArticle <https://en.wikipedia.org/wiki/IEC_60870> ;
                       sto:hasStatus "Valid"@en .


###  https://w3id.org/i40/sto#IEC_60870_P5_S3_E1
sto:IEC_60870_P5_S3_E1 rdf:type owl:NamedIndividual ,
                                sto:Standard ;
                       dcterms:creator sto:irlan ;
                       sto:hasAvailableLanguage lang:eng ,
                                                lang:fra ;
                       sto:hasFileSize sto:FileSizeIEC_60870_P5_S3 ;
                       sto:hasICS sto:ICS_33_200 ;
                       sto:hasPublisher sto:IEC ;
                       sto:hasTechnicalCommittee sto:TC_57 ;
                       sto:isPartOf sto:IEC_60870 ;
                       sto:relatedTo sto:IEC_60870_P2_S1_E2 ;
                       sto:hasEdition "1.0"^^xsd:float ;
                       sto:hasPages "43"^^xsd:int ;
                       sto:hasPublicationDate "1992-09-29"^^xsd:date ;
                       sto:hasStabilityDate "2018"^^xsd:gYear ;
                       sto:hasTag "IEC 60870-5-3:1992"@en ;
                       dcterms:title "Telecontrol equipment and systems - Part 5: Transmission protocols - Section 3: General structure of application data"@en ;
                       rdfs:comment """Applies to telecontrol equipment and systems with coded bit serial data transmission for monitoring and controlling geographically widespread processes; specifies rules for structuring application data units in transmission frames of telecontrol systems.
This publication is of high relevance for Smart Grid."""@en ,
                                    "Applies to telecontrol equipment and systems with coded bit serial data transmission for monitoring and controlling geographically widespread processes; specifies rules for structuring application data units in transmission frames of telecontrol systems.nThis publication is of high relevance for Smart Grid."@en ;
                       rdfs:label "IEC 60870-5-3:1992"@en ;
                       sto:hasDBpediaResource <https://dbpedia.org/resource/IEC_60870> ;
                       sto:hasOfficialResource <https://webstore.iec.ch/publication/3748> ;
                       sto:hasWikipediaArticle <https://en.wikipedia.org/wiki/IEC_60870> ;
                       sto:hasStatus "Valid"@en .


###  https://w3id.org/i40/sto#IEC_60870_P5_S4_E1
sto:IEC_60870_P5_S4_E1 rdf:type owl:NamedIndividual ,
                                sto:Standard ;
                       dcterms:creator sto:irlan ;
                       sto:hasAvailableLanguage lang:eng ,
                                                lang:fra ;
                       sto:hasFileSize sto:FileSizeIEC_60870_P5_S4 ;
                       sto:hasICS sto:ICS_33_200 ;
                       sto:hasPublisher sto:IEC ;
                       sto:hasTechnicalCommittee sto:TC_57 ;
                       sto:isPartOf sto:IEC_60870 ;
                       sto:relatedTo sto:IEC_60870_P2_S1_E2 ;
                       sto:hasEdition "1.0"^^xsd:float ;
                       sto:hasPages "45"^^xsd:int ;
                       sto:hasPublicationDate "1993-08-06"^^xsd:date ;
                       sto:hasStabilityDate "2018"^^xsd:gYear ;
                       sto:hasTag "IEC 60870-5-4:1993"@en ;
                       dcterms:title "Telecontrol equipment and systems - Part 5: Transmission protocols - Section 4: Definition and coding of application information elements"@en ;
                       rdfs:comment """Gives rules for defining information elements and presents a set of information elements, in particular of digital and analog process variables frequently used in telecontrol applications. 
This publication is of high relevance for Smart Grid."""@en ,
                                    "Gives rules for defining information elements and presents a set of information elements, in particular of digital and analog process variables frequently used in telecontrol applications. nThis publication is of high relevance for Smart Grid."@en ;
                       rdfs:label "IEC 60870-5-4:1993"@en ;
                       sto:hasDBpediaResource <https://dbpedia.org/resource/IEC_60870> ;
                       sto:hasOfficialResource <https://webstore.iec.ch/publication/3749> ;
                       sto:hasWikipediaArticle <https://en.wikipedia.org/wiki/IEC_60870> ;
                       sto:hasStatus "Valid"@en .


###  https://w3id.org/i40/sto#IEC_60870_P5_S5_E1
sto:IEC_60870_P5_S5_E1 rdf:type owl:NamedIndividual ,
                                sto:Standard ;
                       dcterms:creator sto:irlan ;
                       sto:hasAvailableLanguage lang:eng ,
                                                lang:fra ;
                       sto:hasFileSize sto:FileSizeIEC_60870_P5_S5 ;
                       sto:hasICS sto:ICS_33_200 ;
                       sto:hasPublisher sto:IEC ;
                       sto:hasTechnicalCommittee sto:TC_57 ;
                       sto:isPartOf sto:IEC_60870 ;
                       sto:relatedTo sto:IEC_60870_P2_S1_E2 ;
                       sto:hasEdition "1.0"^^xsd:float ;
                       sto:hasPages "101"^^xsd:int ;
                       sto:hasPublicationDate "1995-06-04"^^xsd:date ;
                       sto:hasStabilityDate "2018"^^xsd:gYear ;
                       sto:hasTag "IEC 60870-5-5:1995"@en ;
                       dcterms:title "Telecontrol equipment and systems - Part 5: Transmission protocols - Section 5: Basic application functions"@en ;
                       rdfs:comment """Applies to telecontrol equipment and systems with coded bit serial data transmission for monitoring and controlling geographically widespread processes. It defines a telecontrol companion standard that enables interoperability among compatible telecontrol equipment. 
This publication is of high relevance for Smart Grid."""@en ,
                                    "Applies to telecontrol equipment and systems with coded bit serial data transmission for monitoring and controlling geographically widespread processes. It defines a telecontrol companion standard that enables interoperability among compatible telecontrol equipment. nThis publication is of high relevance for Smart Grid."@en ;
                       rdfs:label "IEC 60870-5-5:1995"@en ;
                       sto:hasDBpediaResource <https://dbpedia.org/resource/IEC_60870> ;
                       sto:hasOfficialResource <https://webstore.iec.ch/publication/3750> ;
                       sto:hasWikipediaArticle <https://en.wikipedia.org/wiki/IEC_60870> ;
                       sto:hasStatus "Valid"@en .


###  https://w3id.org/i40/sto#IEC_60870_P5_S6_E1
sto:IEC_60870_P5_S6_E1 rdf:type owl:NamedIndividual ,
                                sto:Standard ;
                       dcterms:creator sto:irlan ;
                       sto:hasAvailableLanguage lang:eng ,
                                                lang:fra ;
                       sto:hasFileSize sto:FileSizeIEC_60870_P5_S6 ;
                       sto:hasICS sto:ICS_33_200 ;
                       sto:hasPublisher sto:IEC ;
                       sto:hasTechnicalCommittee sto:TC_57 ;
                       sto:isPartOf sto:IEC_60870 ;
                       sto:relatedTo sto:IEC_60870_P2_S1_E2 ;
                       sto:hasEdition "1.0"^^xsd:float ;
                       sto:hasPages "46"^^xsd:int ;
                       sto:hasPublicationDate "2006-03-08"^^xsd:date ;
                       sto:hasStabilityDate "2018"^^xsd:gYear ;
                       sto:hasTag "IEC 60870-5-6:2006"@en ;
                       dcterms:title "Telecontrol equipment and systems - Part 5-6: Guidelines for conformance testing for the IEC 60870-5 companion standards"@en ;
                       rdfs:comment "IEC 60870-5-6:2006 Specifies methods for conformance testing of telecontrol equipment, amongst substation automation systems and telecontrol systems, including front-end functions of SCADA. Facilitates interoperability by providing a standard method of testing protocol implementations. Is expected to minimize the risk of non-interoperability."@en ;
                       rdfs:label "IEC 60870-5-6:2006"@en ;
                       sto:hasDBpediaResource <https://dbpedia.org/resource/IEC_60870> ;
                       sto:hasOfficialResource <https://webstore.iec.ch/publication/3751> ;
                       sto:hasWikipediaArticle <https://en.wikipedia.org/wiki/IEC_60870> ;
                       sto:hasStatus "Valid"@en .


###  https://w3id.org/i40/sto#IEC_60870_P6_S2_1995
sto:IEC_60870_P6_S2_1995 rdf:type owl:NamedIndividual ,
                                  sto:Standard ;
                         sto:hasAvailableLanguage lang:eng ,
                                                  lang:fra ;
                         sto:hasFileSize sto:FileSizeIEC_60870_P6_S2_1995 ;
                         sto:hasICS sto:ICS_33_200 ;
                         sto:hasPublisher sto:IEC ;
                         sto:hasTechnicalCommittee sto:TC_57 ;
                         sto:isPartOf sto:IEC_60870 ;
                         sto:relatedTo sto:IEC_60870_P2_S1_E2 ;
                         sto:hasEdition "1.0"^^xsd:float ;
                         sto:hasPages "83"^^xsd:int ;
                         sto:hasPublicationDate "1995-10-31"^^xsd:date ;
                         sto:hasStabilityDate "2018"^^xsd:gYear ;
                         sto:hasTag "IEC 60870-6-2:1995"@en ;
                         dcterms:title "Telecontrol equipment and systems - Part 6: Telecontrol protocols compatible with ISO standards and ITU-T recommendations - Section 2: Use of basic standards (OSI layers 1-4)"@en ;
                         rdfs:comment """Considers the standards related to layers 1-4 of the OSI reference model and describes the role and the functions carried out by each layer.
This publication is of high relevance for Smart Grid."""@en ;
                         rdfs:label "IEC 60870-6-2:1995"@en ;
                         sto:hasDBpediaResource <https://dbpedia.org/resource/IEC_60870> ;
                         sto:hasOfficialResource <https://webstore.iec.ch/publication/3757> ;
                         sto:hasWikipediaArticle <https://en.wikipedia.org/wiki/IEC_60870> .


###  https://w3id.org/i40/sto#IEC_60870_P6_S2_E1
sto:IEC_60870_P6_S2_E1 rdf:type owl:NamedIndividual ,
                                sto:Standard ;
                       dcterms:creator sto:irlan ;
                       sto:hasAvailableLanguage lang:eng ,
                                                lang:fra ;
                       sto:hasFileSize sto:FileSizeIEC_60870_P6_S2 ;
                       sto:hasICS sto:ICS_33_200 ;
                       sto:hasPublisher sto:IEC ;
                       sto:hasTechnicalCommittee sto:TC_57 ;
                       sto:isPartOf sto:IEC_60870 ;
                       sto:relatedTo sto:IEC_60870_P2_S1_E2 ;
                       sto:hasEdition "1.0"^^xsd:float ;
                       sto:hasPages "83"^^xsd:int ;
                       sto:hasPublicationDate "1995-10-31"^^xsd:date ;
                       sto:hasStabilityDate "2018"^^xsd:gYear ;
                       sto:hasTag "IEC 60870-6-2:1995"@en ;
                       dcterms:title "Telecontrol equipment and systems - Part 6: Telecontrol protocols compatible with ISO standards and ITU-T recommendations - Section 2: Use of basic standards (OSI layers 1-4)"@en ;
                       rdfs:comment """Considers the standards related to layers 1-4 of the OSI reference model and describes the role and the functions carried out by each layer.
This publication is of high relevance for Smart Grid."""@en ,
                                    "Considers the standards related to layers 1-4 of the OSI reference model and describes the role and the functions carried out by each layer.nThis publication is of high relevance for Smart Grid."@en ;
                       rdfs:label "IEC 60870-6-2:1995"@en ;
                       sto:hasDBpediaResource <https://dbpedia.org/resource/IEC_60870> ;
                       sto:hasOfficialResource <https://webstore.iec.ch/publication/3757> ;
                       sto:hasWikipediaArticle <https://en.wikipedia.org/wiki/IEC_60870> ;
                       sto:hasStatus "Valid"@en .


###  https://w3id.org/i40/sto#IEC_60870_P6_S501_1995
sto:IEC_60870_P6_S501_1995 rdf:type owl:NamedIndividual ,
                                    sto:Standard ;
                           sto:hasAvailableLanguage lang:eng ,
                                                    lang:fra ;
                           sto:hasFileSize sto:FileSizeIEC_60870_P6_S501_1995 ;
                           sto:hasICS sto:ICS_33_200 ;
                           sto:hasPublisher sto:IEC ;
                           sto:hasTechnicalCommittee sto:TC_57 ;
                           sto:isPartOf sto:IEC_60870 ;
                           sto:relatedTo sto:IEC_60870_P2_S1_E2 ;
                           sto:hasEdition "1.0"^^xsd:float ;
                           sto:hasPages "170"^^xsd:int ;
                           sto:hasPublicationDate "1995-12-18"^^xsd:date ;
                           sto:hasStabilityDate "2018"^^xsd:gYear ;
                           sto:hasTag "IEC 60870-6-501:1995"@en ;
                           dcterms:title "Telecontrol equipment and systems - Part 6: Telecontrol protocols compatible with ISO standards and ITU-T recommendations - Section 501: TASE.1 Service definitions"@en ;
                           rdfs:comment """Defines the services provided by a telecontrol specific application-service-element - the Telecontrol Application Service Element No. 1 (TASE.1) - for the exchange of process data in telecontrol systems.
This publication is of high relevance for Smart Grid."""@en ,
                                        "Defines the services provided by a telecontrol specific application-service-element - the Telecontrol Application Service Element No. 1 (TASE.1) - for the exchange of process data in telecontrol systems.nThis publication is of high relevance for Smart Grid."@en ;
                           rdfs:label "IEC 60870-6-501:1995"@en ;
                           sto:hasDBpediaResource <https://dbpedia.org/resource/IEC_60870> ;
                           sto:hasOfficialResource <https://webstore.iec.ch/publication/3758> ;
                           sto:hasWikipediaArticle <https://en.wikipedia.org/wiki/IEC_60870> .


###  https://w3id.org/i40/sto#IEC_60870_P6_S501_E1
sto:IEC_60870_P6_S501_E1 rdf:type owl:NamedIndividual ,
                                  sto:Standard ;
                         dcterms:creator sto:irlan ;
                         sto:hasAvailableLanguage lang:eng ,
                                                  lang:fra ;
                         sto:hasFileSize sto:FileSizeIEC_60870_P6_S501 ;
                         sto:hasICS sto:ICS_33_200 ;
                         sto:hasPublisher sto:IEC ;
                         sto:hasTechnicalCommittee sto:TC_57 ;
                         sto:isPartOf sto:IEC_60870 ;
                         sto:relatedTo sto:IEC_60870_P2_S1_E2 ;
                         sto:hasEdition "1.0"^^xsd:float ;
                         sto:hasPages "170"^^xsd:int ;
                         sto:hasPublicationDate "1995-12-18"^^xsd:date ;
                         sto:hasStabilityDate "2018"^^xsd:gYear ;
                         sto:hasTag "IEC 60870-6-501:1995"@en ;
                         dcterms:title "Telecontrol equipment and systems - Part 6: Telecontrol protocols compatible with ISO standards and ITU-T recommendations - Section 501: TASE.1 Service definitions"@en ;
                         rdfs:comment """Defines the services provided by a telecontrol specific application-service-element - the Telecontrol Application Service Element No. 1 (TASE.1) - for the exchange of process data in telecontrol systems.
This publication is of high relevance for Smart Grid."""@en ,
                                      "Defines the services provided by a telecontrol specific application-service-element - the Telecontrol Application Service Element No. 1 (TASE.1) - for the exchange of process data in telecontrol systems.nThis publication is of high relevance for Smart Grid."@en ;
                         rdfs:label "IEC 60870-6-501:1995"@en ;
                         sto:hasDBpediaResource <https://dbpedia.org/resource/IEC_60870> ;
                         sto:hasOfficialResource <https://webstore.iec.ch/publication/3758> ;
                         sto:hasWikipediaArticle <https://en.wikipedia.org/wiki/IEC_60870> ;
                         sto:hasStatus "Valid"@en .


###  https://w3id.org/i40/sto#IEC_60870_P6_S502_1995
sto:IEC_60870_P6_S502_1995 rdf:type owl:NamedIndividual ,
                                    sto:Standard ;
                           sto:hasAvailableLanguage lang:eng ,
                                                    lang:fra ;
                           sto:hasFileSize sto:FileSizeIEC_60870_P6_S502_1995 ;
                           sto:hasICS sto:ICS_33_200 ;
                           sto:hasPublisher sto:IEC ;
                           sto:hasTechnicalCommittee sto:TC_57 ;
                           sto:isPartOf sto:IEC_60870 ;
                           sto:relatedTo sto:IEC_60870_P2_S1_E2 ;
                           sto:hasEdition "1.0"^^xsd:float ;
                           sto:hasPages "57"^^xsd:int ;
                           sto:hasPublicationDate "1995-12-05"^^xsd:date ;
                           sto:hasStabilityDate "2018"^^xsd:gYear ;
                           sto:hasTag "IEC 60870-6-502:1995"@en ;
                           dcterms:title "Telecontrol equipment and systems - Part 6: Telecontrol protocols compatible with ISO standards and ITU-T recommendations - Section 502: TASE.1 Protocol definitions"@en ;
                           rdfs:comment """Specifies the protocol for the services provided by an application-service-element - the Telecontrol Application Service Element No. 1 (TASE.1) - to support the exchange of process data between telecontrol systems.
This publication is of high relevance for Smart Grid."""@en ,
                                        "Specifies the protocol for the services provided by an application-service-element - the Telecontrol Application Service Element No. 1 (TASE.1) - to support the exchange of process data between telecontrol systems.nThis publication is of high relevance for Smart Grid."@en ;
                           rdfs:label "IEC 60870-6-502:1995"@en ;
                           sto:hasDBpediaResource <https://dbpedia.org/resource/IEC_60870> ;
                           sto:hasOfficialResource <https://webstore.iec.ch/publication/3759> ;
                           sto:hasWikipediaArticle <https://en.wikipedia.org/wiki/IEC_60870> .


###  https://w3id.org/i40/sto#IEC_60870_P6_S502_E1
sto:IEC_60870_P6_S502_E1 rdf:type owl:NamedIndividual ,
                                  sto:Standard ;
                         dcterms:creator sto:irlan ;
                         sto:hasAvailableLanguage lang:eng ,
                                                  lang:fra ;
                         sto:hasFileSize sto:FileSizeIEC_60870_P6_S502 ;
                         sto:hasICS sto:ICS_33_200 ;
                         sto:hasPublisher sto:IEC ;
                         sto:hasTechnicalCommittee sto:TC_57 ;
                         sto:isPartOf sto:IEC_60870 ;
                         sto:relatedTo sto:IEC_60870_P2_S1_E2 ;
                         sto:hasEdition "1.0"^^xsd:float ;
                         sto:hasPages "57"^^xsd:int ;
                         sto:hasPublicationDate "1995-12-05"^^xsd:date ;
                         sto:hasStabilityDate "2018"^^xsd:gYear ;
                         sto:hasTag "IEC 60870-6-502:1995"@en ;
                         dcterms:title "Telecontrol equipment and systems - Part 6: Telecontrol protocols compatible with ISO standards and ITU-T recommendations - Section 502: TASE.1 Protocol definitions"@en ;
                         rdfs:comment """Specifies the protocol for the services provided by an application-service-element - the Telecontrol Application Service Element No. 1 (TASE.1) - to support the exchange of process data between telecontrol systems.
This publication is of high relevance for Smart Grid."""@en ,
                                      "Specifies the protocol for the services provided by an application-service-element - the Telecontrol Application Service Element No. 1 (TASE.1) - to support the exchange of process data between telecontrol systems.nThis publication is of high relevance for Smart Grid."@en ;
                         rdfs:label "IEC 60870-6-502:1995"@en ;
                         sto:hasDBpediaResource <https://dbpedia.org/resource/IEC_60870> ;
                         sto:hasOfficialResource <https://webstore.iec.ch/publication/3759> ;
                         sto:hasWikipediaArticle <https://en.wikipedia.org/wiki/IEC_60870> ;
                         sto:hasStatus "Valid"@en .


###  https://w3id.org/i40/sto#IEC_60870_P6_S503_2014
sto:IEC_60870_P6_S503_2014 rdf:type owl:NamedIndividual ,
                                    sto:Standard ;
                           sto:hasAvailableLanguage lang:eng ,
                                                    lang:fra ;
                           sto:hasFileSize sto:FileSizeIEC_60870_P6_S503_2014 ;
                           sto:hasICS sto:ICS_33_200 ;
                           sto:hasPublisher sto:IEC ;
                           sto:hasTechnicalCommittee sto:TC_57 ;
                           sto:isPartOf sto:IEC_60870 ;
                           sto:relatedTo sto:IEC_60870_P2_S1_E2 ;
                           sto:hasEdition "3.0"^^xsd:float ;
                           sto:hasPages "310"^^xsd:int ;
                           sto:hasPublicationDate "2014-07-15"^^xsd:date ;
                           sto:hasStabilityDate "2018"^^xsd:gYear ;
                           sto:hasTag "IEC 60870-6-503:2014"@en ;
                           dcterms:title "Telecontrol equipment and systems - Part 6-503: Telecontrol protocols compatible with ISO standards and ITU-T recommendations - TASE.2 Services and protocol"@en ;
                           rdfs:comment "IEC 60870-6-503:2014 specifies a method of exchanging time-critical control centre data through wide-area and local-area networks using a full ISO compliant protocol stack. It contains provisions for supporting both centralized and distributed architectures. This standard includes the exchange of real-time data indications, control operations, time-series data, scheduling and accounting information, remote program control and event notification. This new edition includes the following significant technical changes with respect to the previous edition: - certain objects were made informative; - services associated with the informative objects were made informative; - certain TASE.2 conformance blocks were made out-of-scope."@en ;
                           rdfs:label "IEC 60870-6-503:2014"@en ;
                           sto:hasDBpediaResource <https://dbpedia.org/resource/IEC_60870> ;
                           sto:hasOfficialResource <https://webstore.iec.ch/publication/3760> ;
                           sto:hasWikipediaArticle <https://en.wikipedia.org/wiki/IEC_60870> .


###  https://w3id.org/i40/sto#IEC_60870_P6_S503_E3
sto:IEC_60870_P6_S503_E3 rdf:type owl:NamedIndividual ,
                                  sto:Standard ;
                         dcterms:creator sto:irlan ;
                         sto:hasAvailableLanguage lang:eng ,
                                                  lang:fra ;
                         sto:hasFileSize sto:FileSizeIEC_60870_P6_S503 ;
                         sto:hasICS sto:ICS_33_200 ;
                         sto:hasPublisher sto:IEC ;
                         sto:hasTechnicalCommittee sto:TC_57 ;
                         sto:isPartOf sto:IEC_60870 ;
                         sto:relatedTo sto:IEC_60870_P2_S1_E2 ;
                         sto:hasEdition "3.0"^^xsd:float ;
                         sto:hasPages "310"^^xsd:int ;
                         sto:hasPublicationDate "2014-07-15"^^xsd:date ;
                         sto:hasStabilityDate "2018"^^xsd:gYear ;
                         sto:hasTag "IEC 60870-6-503:2014"@en ;
                         dcterms:title "Telecontrol equipment and systems - Part 6-503: Telecontrol protocols compatible with ISO standards and ITU-T recommendations - TASE.2 Services and protocol"@en ;
                         rdfs:comment "IEC 60870-6-503:2014 specifies a method of exchanging time-critical control centre data through wide-area and local-area networks using a full ISO compliant protocol stack. It contains provisions for supporting both centralized and distributed architectures. This standard includes the exchange of real-time data indications, control operations, time-series data, scheduling and accounting information, remote program control and event notification. This new edition includes the following significant technical changes with respect to the previous edition: - certain objects were made informative; - services associated with the informative objects were made informative; - certain TASE.2 conformance blocks were made out-of-scope."@en ,
                                      "IEC 60870-6-503:2014 specifies a method of exchanging time-critical control centre data through wide-area and local-area networks using a full ISO compliant protocol stack. It contains provisions for supporting both centralized and distributed architectures. This standard includes the exchange of real-time data indications, control operations, time-series data, scheduling and accounting information, remote program control and event notification. This new edition includes the following significant technical changes with respect to the previous edition:n- certain objects were made informative;n- services associated with the informative objects were made informative;n- certain TASE.2 conformance blocks were made out-of-scope."@en ;
                         rdfs:label "IEC 60870-6-503:2014"@en ;
                         sto:hasDBpediaResource <https://dbpedia.org/resource/IEC_60870> ;
                         sto:hasOfficialResource <https://webstore.iec.ch/publication/3760> ;
                         sto:hasWikipediaArticle <https://en.wikipedia.org/wiki/IEC_60870> ;
                         sto:hasStatus "Valid"@en .


###  https://w3id.org/i40/sto#IEC_60870_P6_S601_E1
sto:IEC_60870_P6_S601_E1 rdf:type owl:NamedIndividual ,
                                  sto:Standard ;
                         dcterms:creator sto:irlan ;
                         sto:hasAvailableLanguage lang:eng ,
                                                  lang:fra ;
                         sto:hasFileSize sto:FileSizeIEC_60870_P6_S601 ;
                         sto:hasICS sto:ICS_33_200 ;
                         sto:hasPublisher sto:IEC ;
                         sto:hasTechnicalCommittee sto:TC_57 ;
                         sto:isPartOf sto:IEC_60870 ;
                         sto:relatedTo sto:IEC_60870_P2_S1_E2 ;
                         sto:hasEdition "1.0"^^xsd:float ;
                         sto:hasPages "25"^^xsd:int ;
                         sto:hasPublicationDate "1994-12-21"^^xsd:date ;
                         sto:hasStabilityDate "2018"^^xsd:gYear ;
                         sto:hasTag "IEC 60870-6-601:1994"@en ;
                         dcterms:title "Telecontrol equipment and systems - Part 6: Telecontrol protocol s compatible with ISO standards and ITU-T recommendations - Sect ion 601: Functional profile for providing the connection-oriente d transport service in an end system connected via permanent acc ess to a packet switched data network"@en ;
                         rdfs:comment "Defines the functional profile which provides the connection-oriented transport service in an end system connected via permanent access to a packet switched data network.nThis publication is of high relevance for Smart Grid."@en ;
                         rdfs:label "IEC 60870-6-601:1994"@en ;
                         sto:hasDBpediaResource <https://dbpedia.org/resource/IEC_60870> ;
                         sto:hasOfficialResource <https://webstore.iec.ch/publication/3765> ;
                         sto:hasWikipediaArticle <https://en.wikipedia.org/wiki/IEC_60870> ;
                         sto:hasStatus "Valid"@en .


###  https://w3id.org/i40/sto#IEC_60870_P6_S701_E1
sto:IEC_60870_P6_S701_E1 rdf:type owl:NamedIndividual ,
                                  sto:Standard ;
                         dcterms:creator sto:irlan ;
                         sto:hasAvailableLanguage lang:eng ,
                                                  lang:fra ;
                         sto:hasFileSize sto:FileSizeIEC_60870_P6_S701 ;
                         sto:hasICS sto:ICS_33_200 ;
                         sto:hasPublisher sto:IEC ;
                         sto:hasTechnicalCommittee sto:TC_57 ;
                         sto:isPartOf sto:IEC_60870 ;
                         sto:relatedTo sto:IEC_60870_P2_S1_E2 ;
                         sto:hasEdition "1.0"^^xsd:float ;
                         sto:hasPages "37"^^xsd:int ;
                         sto:hasPublicationDate "1998-08-07"^^xsd:date ;
                         sto:hasStabilityDate "2018"^^xsd:gYear ;
                         sto:hasTag "IEC 60870-6-701:1998"@en ;
                         dcterms:title "Telecontrol equipment and systems - Part 6-701: Telecontrol protocols compatible with ISO standards and ITU-T recommendations - Functional profile for providing the TASE.1 application service in end systems"@en ;
                         rdfs:comment "Describes the functional profile which defines the provision of the TASE.1 communication services between two control centre end systems.nThis publication is of high relevance for Smart Grid"@en ;
                         rdfs:label "IEC 60870-6-701:1998"@en ;
                         sto:hasDBpediaResource <https://dbpedia.org/resource/IEC_60870> ;
                         sto:hasOfficialResource <https://webstore.iec.ch/publication/3767> ;
                         sto:hasWikipediaArticle <https://en.wikipedia.org/wiki/IEC_60870> ;
                         sto:hasStatus "Valid"@en .


###  https://w3id.org/i40/sto#IEC_60870_P6_S702_E2
sto:IEC_60870_P6_S702_E2 rdf:type owl:NamedIndividual ,
                                  sto:Standard ;
                         dcterms:creator sto:irlan ;
                         sto:hasAvailableLanguage lang:eng ,
                                                  lang:fra ;
                         sto:hasFileSize sto:FileSizeIEC_60870_P6_S702 ;
                         sto:hasICS sto:ICS_33_200 ;
                         sto:hasPublisher sto:IEC ;
                         sto:hasTechnicalCommittee sto:TC_57 ;
                         sto:hasPublisher sto:IEC ;
                         sto:isPartOf sto:IEC_60870 ;
                         sto:relatedTo sto:IEC_60870_P2_S1_E2 ;
                         sto:hasEdition "2.0"^^xsd:float ;
                         sto:hasPages "71"^^xsd:int ;
                         sto:hasPublicationDate "2014-07-15"^^xsd:date ;
                         sto:hasStabilityDate "2018"^^xsd:gYear ;
                         sto:hasTag "IEC 60870-6-702:2014"@en ;
                         dcterms:title "Telecontrol equipment and systems - Part 6-702: Telecontrol protocols compatible with ISO standards and ITU-T recommendations - Functional profile for providing the TASE.2 application service in end systems"@en ;
                         rdfs:comment """IEC 60870-6-702:2014 is a functional profile (FP) and defines the provision of the TASE.2 communications services between two control centre end systems. It is supported by the transport services implemented in accordance with transport-profiles defined for the type of network that interconnects the control centre end systems. The main changes with respect to the previous edition are listed below:
- certain objects were moved from being normative to informative - certain TASE.2 conformance blocks have been made out-of-scope."""@en ;
                         rdfs:label "IEC 60870-6-702:2014"@en ;
                         sto:hasDBpediaResource <https://dbpedia.org/resource/IEC_60870> ;
                         sto:hasOfficialResource <https://webstore.iec.ch/publication/3768> ;
                         sto:hasWikipediaArticle <https://en.wikipedia.org/wiki/IEC_60870> ;
                         sto:hasStatus "Valid"@en .


###  https://w3id.org/i40/sto#IEC_60870_P6_S802_E3
sto:IEC_60870_P6_S802_E3 rdf:type owl:NamedIndividual ,
                                  sto:Standard ;
                         dcterms:creator sto:irlan ;
                         sto:hasAvailableLanguage lang:eng ,
                                                  lang:fra ;
                         sto:hasFileSize sto:FileSizeIEC_60870_P6_S802 ;
                         sto:hasICS sto:ICS_33_200 ;
                         sto:hasPublisher sto:IEC ;
                         sto:hasTechnicalCommittee sto:TC_57 ;
                         sto:isPartOf sto:IEC_60870 ;
                         sto:relatedTo sto:IEC_60870_P2_S1_E2 ;
                         sto:hasEdition "3.0"^^xsd:float ;
                         sto:hasPages "188"^^xsd:int ;
                         sto:hasPublicationDate "2014-07-15"^^xsd:date ;
                         sto:hasStabilityDate "2019"^^xsd:gYear ;
                         sto:hasTag "IEC 60870-6-802:2014"@en ;
                         dcterms:title "Telecontrol equipment and systems - Part 6-802: Telecontrol protocols compatible with ISO standards and ITU-T recommendations - TASE.2 Object models"@en ;
                         rdfs:comment "IEC 60870-6-802:2014 specifies a method of exchanging time-critical control centre data through wide-area and local-area networks using a full ISO compliant protocol stack. It contains provisions for supporting both centralized and distributed architectures. The standard includes the exchange of real-time data indications, control operations, time series data, scheduling and accounting information, remote program control and event notification. This new edition includes the following significant technical changes with respect to the previous edition: -certain objects have been changed from informative to normative; - certain TASE.2 conformance blocks have been made out of scope."@en ;
                         rdfs:label "IEC 60870-6-802:2014"@en ;
                         sto:hasDBpediaResource <https://dbpedia.org/resource/IEC_60870> ;
                         sto:hasOfficialResource <https://webstore.iec.ch/publication/3769> ;
                         sto:hasWikipediaArticle <https://en.wikipedia.org/wiki/IEC_60870> ;
                         sto:hasStatus "Valid"@en .


###  https://w3id.org/i40/sto#IEC_60904
sto:IEC_60904 rdf:type owl:NamedIndividual ,
                       sto:Standard ;
              dcterms:creator sto:irlan ;
              sto:hasAvailableLanguage lang:eng ,
                                       lang:fra ;
              sto:hasPublisher sto:IEC ;
              sto:hasPublicationDate "2017-05-18"^^xsd:date ;
              rdfs:comment "Photovoltaic devices"@en ;
              rdfs:label "IEC 60904"@en ;
              sto:hasOfficialResource <https://webstore.iec.ch/publication/3881> .


###  https://w3id.org/i40/sto#IEC_60946_E1
sto:IEC_60946_E1 rdf:type owl:NamedIndividual ,
                          sto:Standard ;
                 dcterms:creator sto:irlan ,
                                 sto:sebastian ;
                 sto:hasAvailableLanguage lang:eng ,
                                          lang:fra ;
                 sto:hasFileSize sto:FileSizeIEC_60946 ;
                 sto:hasICS sto:ICS_25_040_40 ;
                 sto:hasPublisher sto:IEC ;
                 sto:hasTechnicalCommittee sto:TC_65 ;
                 sto:hasEdition "1.0"^^xsd:float ;
                 sto:hasPages "13"^^xsd:int ;
                 sto:hasPublicationDate "1988-09-29"^^xsd:date ;
                 sto:hasStabilityDate "2018"^^xsd:gYear ;
                 sto:hasTag "IEC 60946:1988"@en ;
                 dcterms:title "Binary direct voltage signals for process measurement and control systems"@en ;
                 rdfs:comment "Applies to non-multiplexed two wire binary direct voltage signals of nominal 24 V level that are used in industrial-process measurement and control systems to transmit information between elements of systems."@en ;
                 rdfs:label "IEC 60946:1988"@en ;
                 sto:hasOfficialResource <https://webstore.iec.ch/publication/3961> ;
                 sto:hasStatus "Valid"@en .

sto:IEC_61000 rdf:type owl:NamedIndividual ,
                                sto:Standard ;
                       sto:hasPublisher sto:IEC ;;
                       dcterms:title "Electromagnetic compatibility (EMC) "@en ;
                       rdfs:comment "Terms of basic importance to concepts and practical applications in the design and evaluation of electromagnetically compatible systems."@en ;
                       rdfs:label "IEC 61000"^^xsd:string .

###  https://w3id.org/i40/sto#IEC_61000_P6_S2_E3
sto:IEC_61000_P6_S2_E3 rdf:type owl:NamedIndividual ,
                                sto:Standard ;
                       dcterms:creator sto:irlan ,
                                       sto:sebastian ;
                       sto:hasAvailableLanguage lang:eng ;
                       sto:hasFileSize sto:FileSizeIEC_61000_P6_S2 ;
                       sto:hasICS sto:ICS_33_100_20 ;
                       sto:hasPublisher sto:IEC ;
                       sto:hasTechnicalCommittee sto:TC_77 ;
                       sto:isPartOf sto:IEC_61000;
                       sto:hasEdition "3.0"^^xsd:float ;
                       sto:hasPages "57"^^xsd:int ;
                       sto:hasPublicationDate "2016-08-10"^^xsd:date ;
                       sto:hasStabilityDate "2020"^^xsd:gYear ;
                       sto:hasTag "IEC 61000-6-2:2016"@en ;
                       dcterms:title "Electromagnetic compatibility (EMC) - Part 6-2: Generic standards - Immunity standard for industrial environments"@en ;
                       rdfs:comment "IEC 61000-6-2:2016 RLV contains the International Standard and its Redline version. The Redline version is available in English only. The Redline version provides you with a quick and easy way to compare all the changes between this standard and its previous edition. The Redline version is not an official IEC Standard, only the current version of the standard is to be considered the official document. IEC 61000-6-2:2016 for EMC immunity requirements applies to electrical and electronic equipment intended for use in industrial locations, as described below. Immunity requirements in the frequency range 0 Hz to 400 GHz are covered. No tests need to be performed at frequencies where no requirements are specified. This generic EMC immunity standard is applicable if no relevant dedicated product or product-family EMC immunity standard exists. This third edition cancels and replaces the second edition published in 2005. This edition constitutes a technical revision."@en ;
                       rdfs:label "IEC 61000-6-2:2016"@en ;
                       sto:hasOfficialResource <https://webstore.iec.ch/publication/25629> ;
                       sto:hasStatus "Redline version"@en ;
                       .

sto:IEC_61010 rdf:type owl:NamedIndividual ,
                                  sto:Standard ;
                         sto:hasPublisher sto:IEC ;
                         dcterms:title "Safety requirements for electrical equipment for measurement, control, and laboratory use "@en ;
                         rdfs:comment "IEC 61010 specifies safety requirements for electrical equipment and their accessories . "@en ;
                         rdfs:label "IEC 61010"@en .

###  https://w3id.org/i40/sto#IEC_61010_P2_S012_E1
sto:IEC_61010_P2_S012_E1 rdf:type owl:NamedIndividual ,
                                  sto:Standard ;
                         dcterms:creator sto:irlan ,
                                         sto:sebastian ;
                         sto:hasAvailableLanguage lang:eng ,
                                                  lang:fra ;
                         sto:hasFileSize sto:FileSizeIEC_61010_P2_S012 ;
                         sto:hasICS sto:ICS_19_08 ;
                         sto:hasPublisher sto:IEC ;
                         sto:hasTechnicalCommittee sto:TC_66 ;
                         sto:isPartOf sto:IEC_61010; 
                         sto:hasEdition "1.0"^^xsd:float ;
                         sto:hasPages "174"^^xsd:int ;
                         sto:hasPublicationDate "2016-07-12"^^xsd:date ;
                         sto:hasStabilityDate "2020"^^xsd:gYear ;
                         dcterms:title "Safety requirements for electrical equipment for measurement, control, and laboratory use - Part 2-012: Particular requirements for climatic and environmental testing and other temperature conditioning equipment"@en ;
                         rdfs:comment "IEC 61010-2-012:2016 specifies safety requirements for electrical equipment and their accessories within the categories a) through c), wherever they are intended to be used, whenever that equipment incorporates one or more of the following characteristics:- A REFRIGERATING SYSTEM that is acted on or impacted by an integral heating function such that the combined heating and cooling system generates additional and/or more severe HAZARDS than those for the two systems if treated separately.- The materials being treated in the intended application introduce significant heat into the REFRIGERATING SYSTEM that the cooling system in the application yield additional and/or more severe HAZARDS than those for the cooling system if operated at the maximum RATED ambient alone.- An irradiation function for the materials being treated presenting additional HAZARDS.- A function to expose the materials being treated to excessive humidity, carbon dioxide, salt mist, or other substances which may result in additional HAZARDS.- A function of MECHANICAL MOVEMENT presenting additional HAZARDS.- Provision for an OPERATOR to walk-in to the operating area to load or unload the materials being treated.It has the status of a group safety publication in accordance with IEC Guide 104. This publication is to be read in conjunction with IEC 61010-1:2010."@en ;
                         rdfs:label "IEC 61010-2-012:2016"@en ;
                         sto:hasOfficialResource <https://webstore.iec.ch/publication/25400> .


###  https://w3id.org/i40/sto#IEC_61010_P2_S201_E2
sto:IEC_61010_P2_S201_E2 rdf:type owl:NamedIndividual ,
                                  sto:Standard ;
                         dcterms:creator sto:sebastian , 
                                        sto:irlan ;
                         sto:hasAvailableLanguage lang:eng ;
                         sto:hasFileSize sto:FileSizeIEC_61010_P2_S201 ;
                         sto:hasICS sto:ICS_17_020 ,
                                    sto:ICS_19_020 ,
                                    sto:ICS_25_040_40 ;
                         sto:hasPublisher sto:IEC ;
                         sto:hasTechnicalCommittee sto:TC_65 ;
                         sto:relatedTo sto:IEC_61000_P6_S2_E3 ;
                         sto:isPartOf sto:IEC_61010; 
                         sto:hasEdition "2.0"^^xsd:float ;
                         sto:hasPages "235"^^xsd:int ;
                         sto:hasPublicationDate "2017-03-24"^^xsd:date ;
                         sto:hasStabilityDate "2020"^^xsd:gYear ;
                         sto:hasTag "IEC 61010-2-201:2017"@en ;
                         dcterms:title "Safety requirements for electrical equipment for measurement, control, and laboratory use - Part 2-201: Particular requirements for control equipment"@en ;
                         rdfs:comment "IEC 61010-2-201:2017 RLV contains the International Standard and its Redline version. The Redline version is available in English only. The Redline version provides you with a quick and easy way to compare all the changes between this standard and its previous edition. The Redline version is not an official IEC Standard, only the current version of the standard is to be considered the official document.IEC 61010-2-201:2017 specifies safety requirements and related verification tests for any product performing the function of control equipment and/or their associated peripherals. In addition, these products have as their intended use the command and control of machines, automated manufacturing and industrial processes, e.g. discrete and continuous control.This second edition cancels and replaces the first edition published in 2013. This edition constitutes a technical revision. This second edition includes the following significant technical changes with respect to the previous edition;a) clarify, change, delete definitions which were causing confusion,b) change and clarify the temperature testing methodology,c) change documentation methodologies allowed,d) change some terminal markings,e) add clarity to some of the informative annexes,f) add Annex E with changes,g) add Annexes AA – FF."@en ,
                                      "IEC 61010-2-201:2017 RLV contains the International Standard and its Redline version. The Redline version is available in English only. The Redline version provides you with a quick and easy way to compare all the changes between this standard and its previous edition. The Redline version is not an official IEC Standard, only the current version of the standard is to be considered the official document.nnIEC 61010-2-201:2017 specifies safety requirements and related verification tests for any product performing the function of control equipment and/or their associated peripherals. In addition, these products have as their intended use the command and control of machines, automated manufacturing and industrial processes, e.g. discrete and continuous control.nThis second edition cancels and replaces the first edition published in 2013. This edition constitutes a technical revision. This second edition includes the following significant technical changes with respect to the previous edition;na) clarify, change, delete definitions which were causing confusion,nb) change and clarify the temperature testing methodology,nc) change documentation methodologies allowed,nd) change some terminal markings,ne) add clarity to some of the informative annexes,nf) add Annex E with changes,ng) add Annexes AA – FF."@en ;
                         rdfs:label "IEC 61010-2-201:2017"@en ;
                         sto:hasOfficialResource <https://webstore.iec.ch/publication/60204> .


###  https://w3id.org/i40/sto#IEC_61010_P2_S202_E1
sto:IEC_61010_P2_S202_E1 rdf:type owl:NamedIndividual ,
                                  sto:Standard ;
                         dcterms:creator sto:sebastian , 
                                         sto:irlan ;
                         sto:hasAvailableLanguage lang:eng ,
                                                  lang:fra ;
                         sto:hasFileSize sto:FileSizeIEC_61010_P2_S202 ;
                         sto:hasICS sto:ICS_13_110 ,
                                    sto:ICS_17_020 ,
                                    sto:ICS_19_020 ;
                         sto:hasPublisher sto:IEC ;
                         sto:hasTechnicalCommittee sto:TC_65 ;
                         sto:relatedTo sto:IEC_61000_P6_S2_E3 ;
                         sto:isPartOf sto:IEC_61010; 
                         sto:hasEdition "1.0"^^xsd:float ;
                         sto:hasPages "25"^^xsd:int ;
                         sto:hasPublicationDate "2016-07-12"^^xsd:date ;
                         sto:hasStabilityDate "2019"^^xsd:gYear ;
                         sto:hasTag "IEC 61010-2-202:2016"@en ;
                         dcterms:title "Safety requirements for electrical equipment for measurement, control and laboratory use - Part 2-202: Particular requirements for electrically operated valve actuators"@en ;
                         rdfs:comment "IEC 61010-2-202:2016 specifies the safety requirements for electric ACTUATORs and SOLENOIDs, as applied to valves, intended to be installed in an industrial process or discrete control environment. This publication is to be read in conjunction with IEC 61010-1:2010."@en ;
                         rdfs:label "IEC 61010-2-202:2016"@en ;
                         sto:hasOfficialResource <https://webstore.iec.ch/publication/25399> .


###  https://w3id.org/i40/sto#IEC_61131
sto:IEC_61131 rdf:type owl:NamedIndividual ,
                       sto:Standard ;
              dcterms:creator sto:sebastian , 
                              sto:irlan ;
              dul:isComponentOf sto:IEC_62714 ;
              sto:hasClassification sto:RamiControlDevice ,
                                    sto:RamiStation ,
                                    sto:RamiWorkCenter ;
              sto:hasPublisher sto:IEC ;
              sto:relatedTo sto:DIN_SPEC_16592 ,
                            sto:IEC_61131 ,
                            sto:IEC_61360 ,
                            sto:IEC_61499 ,
                            sto:IEC_61804 ,
                            sto:IEC_61850 ,
                            sto:IEC_61987_X ,
                            sto:IEC_62424 ,
                            sto:IEC_62453 ,
                            sto:IEC_62541 ,
                            sto:IEC_62714 ,
                            sto:ISO_13584 ,
                            sto:ISO_14306 ,
                            sto:ISO_15746 ,
                            sto:ISO_15926 ,
                            sto:ISO_18629 ,
                            sto:ISO_18828-2 ,
                            sto:ISO_20922 ,
                            sto:ISO_22400 ,
                            sto:ISO_29002 ,
                            sto:ISO_ASTM_52915 ,
                            sto:ISO_PAS_17506 ,
                            sto:MathML ,
                            sto:SysML ,
                            sto:eClass ;
              rdfs:comment "IEC 61131 is an IEC standard for programmable controllers. It was known as IEC 1131 before the change in numbering system by IEC. The parts of the IEC 61131 standard are prepared and maintained working group 7, programmable control systems, of subcommittee SC 65B of Technical Committee TC65 of the IEC."@en ;
              rdfs:label "IEC 61131"@en ;
              sto:hasDBpediaResource <http://dbpedia.org/page/IEC_61131> ;
              sto:hasOfficialResource <https://webstore.iec.ch/publication/4550> ;
              sto:hasWikipediaArticle <https://en.wikipedia.org/wiki/IEC_61131> .


###  https://w3id.org/i40/sto#IEC_61158
sto:IEC_61158 rdf:type owl:NamedIndividual ,
                       sto:Standard ;
              dcterms:creator sto:sebastian , 
                              sto:irlan ;
              sto:hasPublisher sto:IEC ;
              sto:relatedTo sto:IEC_29182_P1 ,
                            sto:IEC_61158 ,
                            sto:IEC_61784 ,
                            sto:OMG_DDS ;
              sto:hasTag "Fieldbus"@en ;
              rdfs:comment "Fieldbus is the name of a family of industrial computer network protocols used for real-time distributed control, standardized as IEC 61158. A complex automated industrial system such as manufacturing assembly line usually needs a distributed control system an organized hierarchy of controller systems to function. In this hierarchy, there is usually a Human Machine Interface (HMI) at the top, where an operator can monitor or operate the system. This is typically linked to a middle layer of programmable logic controllers (PLC) via a non-time-critical communications system (e.g. Ethernet). At the bottom of the control chain is the fieldbus that links the PLCs to the components that actually do the work, such as sensors, actuators, electric motors, console lights, switches, valves and contactors"@en ;
              rdfs:label "IEC 61158"@en ;
              sto:hasDBpediaResource <http://dbpedia.org/page/Fieldbus> ;
              sto:hasOfficialResource <http://www.fieldbus.org/> ;
              sto:hasWikipediaArticle <https://en.wikipedia.org/wiki/Fieldbus> .


###  https://w3id.org/i40/sto#IEC_61160_E2
sto:IEC_61160_E2 rdf:type owl:NamedIndividual ,
                          sto:Standard ;
                 dcterms:creator sto:sebastian , 
                                 sto:irlan ;
                 sto:hasAvailableLanguage lang:eng ,
                                          lang:fra ,
                                          lang:spa ;
                 sto:hasFileSize sto:FileSizeIEC_61160 ;
                 sto:hasICS sto:ICS_03_100_40 ,
                            sto:ICS_03_120_01 ;
                 sto:hasPublisher sto:IEC ;
                 sto:hasTechnicalCommittee sto:TC_56 ;
                 sto:hasEdition "2.0"^^xsd:float ;
                 sto:hasPages "69"^^xsd:int ;
                 sto:hasPublicationDate "2005-09-27"^^xsd:date ;
                 sto:hasStabilityDate "2020"^^xsd:gYear ;
                 sto:hasTag "IEC 61160:2005"@en ;
                 dcterms:title "Design review"@en ;
                 rdfs:comment "This International Standard makes recommendations for the implementation of design review as a means of verifying that the design input requirements have been met and stimulating the improvement of the product's design. The intention is for it to be applied during the design and development phase of a product's life cycle."@en ;
                 rdfs:label "IEC 61160:2005"@en ;
                 sto:hasOfficialResource <https://webstore.iec.ch/publication/4707> .

sto:IEC_61310 rdf:type owl:NamedIndividual ,
                             sto:Standard ;
                    sto:hasPublisher sto:IEC ;
                    dcterms:title "Safety of machinery - Indication, marking and actuation "@en ;
                    rdfs:comment "Specifies requirements for visual, acoustic and tactile methods of indicating safety-related information"@en ;
                    rdfs:label "IEC 61310"@en .

###  https://w3id.org/i40/sto#IEC_61310_P1_E2
sto:IEC_61310_P1_E2 rdf:type owl:NamedIndividual ,
                             sto:Standard ;
                    dcterms:creator sto:sebastian , 
                                    sto:irlan ;
                    sto:hasAvailableLanguage lang:eng ,
                                             lang:fra ,
                                             lang:spa ;
                    sto:hasFileSize sto:FileSizeIEC_61310_P1 ;
                    sto:hasICS sto:ICS_13_110 ;
                    sto:hasPublisher sto:IEC ;
                    sto:hasTechnicalCommittee sto:TC_44 ;
                    sto:isPartOf sto:IEC_61310;
                    sto:hasEdition "2.0"^^xsd:float ;
                    sto:hasPages "43"^^xsd:int ;
                    sto:hasPublicationDate "2007-02-16"^^xsd:date ;
                    sto:hasStabilityDate "2021"^^xsd:gYear ;
                    sto:hasTag "IEC 61310-1:2007"@en ;
                    dcterms:title "Safety of machinery - Indication, marking and actuation - Part 1: Requirements for visual, acoustic and tactile signals"@en ;
                    rdfs:comment "Specifies requirements for visual, acoustic and tactile methods of indicating safety-related information, at the human-machine interface and to exposed persons. It specifies a system of colours, safety signs, markings and other warnings, intended for use in the indication of hazardous situations and health hazards and for meeting certain emergencies. It also specifies ways of coding visual, acoustic and tactile signals for indicators and actuators to facilitate the safe use and monitoring of the machinery. It includes the following significant technical changes with respect to the previous edition: Adapted to the basic standards IEC 60073, IEC 60417, ISO 3864-1, ISO 7000 and ISO 7010"@en ;
                    rdfs:label "IEC 61310-1:2007"@en ;
                    sto:hasOfficialResource <https://webstore.iec.ch/publication/5263> .


###  https://w3id.org/i40/sto#IEC_61310_P2_E2
sto:IEC_61310_P2_E2 rdf:type owl:NamedIndividual ,
                             sto:Standard ;
                    dcterms:creator sto:sebastian , 
                                 sto:irlan ;
                    sto:hasAvailableLanguage lang:eng ,
                                             lang:fra ,
                                             lang:spa ;
                    sto:hasFileSize sto:FileSizeIEC_61310_P2 ;
                    sto:hasICS sto:ICS_13_110 ;
                    sto:hasPublisher sto:IEC ;
                    sto:hasTechnicalCommittee sto:TC_44 ;
                    sto:relatedTo sto:IEC_61310_P1_E2 ;
                    sto:isPartOf sto:IEC_61310;
                    sto:hasEdition "2.0"^^xsd:float ;
                    sto:hasPages "25"^^xsd:int ;
                    sto:hasPublicationDate "2007-02-16"^^xsd:date ;
                    sto:hasStabilityDate "2021"^^xsd:gYear ;
                    sto:hasTag "IEC 61310-2:2007"@en ;
                    dcterms:title "Safety of machinery - Indication, marking and actuation - Part 2: Requirements for marking"@en ;
                    rdfs:comment "It gives general rules on marking for identification of machinery, for safe use related to mechanical and electrical hazards, and for the avoidance of hazards arising from incorrect connections. Includes the following significant technical changes with respect to the previous edition: Annex A: additional safety signs included and updated."@en ;
                    rdfs:label "IEC 61310-2:2007"@en ;
                    sto:hasOfficialResource <https://webstore.iec.ch/publication/5264> .


###  https://w3id.org/i40/sto#IEC_61310_P3_E2
sto:IEC_61310_P3_E2 rdf:type owl:NamedIndividual ,
                             sto:Standard ;
                    dcterms:creator sto:sebastian , 
                                 sto:irlan ;
                    sto:hasAvailableLanguage lang:eng ,
                                             lang:fra ,
                                             lang:spa ;
                    sto:hasFileSize sto:FileSizeIEC_61310_P3 ;
                    sto:hasICS sto:ICS_13_110 ;
                    sto:hasPublisher sto:IEC ;
                    sto:hasTechnicalCommittee sto:TC_44 ;
                    sto:relatedTo sto:IEC_61310_P1_E2 ;
                    sto:isPartOf sto:IEC_61310;
                    sto:hasEdition "2.0"^^xsd:float ;
                    sto:hasPages "25"^^xsd:int ;
                    sto:hasPublicationDate "2007-02-16"^^xsd:date ;
                    sto:hasStabilityDate "2021"^^xsd:gYear ;
                    sto:hasTag "IEC 61310-3:2007"@en ;
                    dcterms:title "Safety of machinery - Indication, marking and actuation - Part 3: Requirements for the location and operation of actuators"@en ;
                    rdfs:comment "Specifies safety-related requirements for actuators, operated by the hand or by other parts of the human body, at the human-machine interface. It gives general requirements for the standard direction of movement for actuators; the arrangement of an actuator in relation to other actuators; the correlation between an action and its final effects. It includes the following significant technical changes with respect to the previous edition: Table 1, Table 2 and Table A.1 have been revised editorially."@en ;
                    rdfs:label "IEC 61310-3:2007"@en ;
                    sto:hasOfficialResource <https://webstore.iec.ch/publication/5265> .


###  https://w3id.org/i40/sto#IEC_61334
sto:IEC_61334 rdf:type owl:NamedIndividual ,
                       sto:Standard ;
              dcterms:creator sto:sebastian , 
                                 sto:irlan ;
              sto:hasPublisher sto:IEC ;
              rdfs:comment "IEC 61334 , known as Distribution automation using distribution line carrier systems, is a standard for low-speed reliable power line communications by electricity meters, water meters and SCADA."@en ;
              rdfs:label "IEC 61334"@en ;
              sto:hasDBpediaResource <http://dbpedia.org/page/IEC_61334> ;
              sto:hasOfficialResource <https://webstore.iec.ch/publication/5308> .


###  https://w3id.org/i40/sto#IEC_61334_P3_S1_E1
sto:IEC_61334_P3_S1_E1 rdf:type owl:NamedIndividual ,
                                sto:Standard ;
                       dcterms:creator sto:sebastian , 
                                 sto:irlan ;
                       sto:hasAvailableLanguage lang:eng ,
                                                lang:fra ;
                       sto:hasFileSize sto:FileSizeIEC_61334_P3_S1 ;
                       sto:hasICS sto:ICS_29_240_20 ,
                                  sto:ICS_33_200 ;
                       sto:hasPublisher sto:IEC ;
                       sto:hasTechnicalCommittee sto:TC_57 ;
                       sto:relatedTo sto:IEC_61334 ;
                       sto:isPartOf sto:IEC_61334;
                       sto:hasEdition "1.0"^^xsd:float ;
                       sto:hasPages "27"^^xsd:int ;
                       sto:hasPublicationDate "1998-11-24"^^xsd:date ;
                       sto:hasStabilityDate "2018"^^xsd:gYear ;
                       sto:hasTag "IEC 61334-3-1:1998 "@en ;
                       dcterms:title "Distribution automation using distribution line carrier systems - Part 3-1: Mains signalling requirements - Frequency bands and output levels"@en ;
                       rdfs:comment "Applies to electrical equipment used in distribution line carrier systems on both medium-voltage and low-voltage distribution networks. Specifies requirements such as frequency bands, output levels, spurious emissions, etc. This publication is of high relevance for Smart Grid."@en ;
                       rdfs:label "IEC 61334-3-1:1998"@en ;
                       sto:hasDBpediaResource <https://dbpedia.org/resource/IEC_61334> ;
                       sto:hasOfficialResource <https://webstore.iec.ch/publication/5297> ;
                       sto:hasWikipediaArticle <https://en.wikipedia.org/wiki/IEC_61334> .


###  https://w3id.org/i40/sto#IEC_61334_P3_S21_E1
sto:IEC_61334_P3_S21_E1 rdf:type owl:NamedIndividual ,
                                 sto:Standard ;
                        dcterms:creator sto:sebastian , 
                                 sto:irlan ;
                        sto:hasAvailableLanguage lang:eng ,
                                                 lang:fra ;
                        sto:hasFileSize sto:FileSizeIEC_61334_P3_S21 ;
                        sto:hasICS sto:ICS_29_240_20 ,
                                   sto:ICS_33_200 ;
                        sto:hasPublisher sto:IEC ;
                        sto:hasTechnicalCommittee sto:TC_57 ;
                        sto:relatedTo sto:IEC_61334 ;
                        sto:isPartOf sto:IEC_61334;
                        sto:hasEdition "1.0"^^xsd:float ;
                        sto:hasPages "33"^^xsd:int ;
                        sto:hasPublicationDate "1996-03-27"^^xsd:date ;
                        sto:hasStabilityDate "2018"^^xsd:gYear ;
                        sto:hasTag "IEC 61334-3-21:1996"@en ;
                        dcterms:title "Distribution automation using distribution line carrier systems - Part 3: Mains signalling requirements - Section 21: MV phase-to-phase isolated capacitive coupling device"@en ;
                        rdfs:comment """Establishes definitions, requirements, methods of testing and rated values for phase-to-phase isolated capacitive coupling devices to be used in medium-voltage (MV) distribution line carrier systems.
This publication is of high relevance for Smart Grid."""@en ;
                        rdfs:label "IEC 61334-3-21:1996"@en ;
                        sto:hasDBpediaResource <https://dbpedia.org/resource/IEC_61334> ;
                        sto:hasOfficialResource <https://webstore.iec.ch/publication/5298> ;
                        sto:hasWikipediaArticle <https://en.wikipedia.org/wiki/IEC_61334> .


###  https://w3id.org/i40/sto#IEC_61334_P3_S22_E1
sto:IEC_61334_P3_S22_E1 rdf:type owl:NamedIndividual ,
                                 sto:Standard ;
                        dcterms:creator sto:sebastian , 
                                 sto:irlan ;
                        sto:hasAvailableLanguage lang:eng ,
                                                 lang:fra ;
                        sto:hasFileSize sto:FileSizeIEC_61334_P3_S22 ;
                        sto:hasICS sto:ICS_29_240_20 ,
                                   sto:ICS_33_200 ;
                        sto:hasPublisher sto:IEC ;
                        sto:hasTechnicalCommittee sto:TC_57 ;
                        sto:isPartOf sto:IEC_61334;
                        sto:hasEdition "1.0"^^xsd:float ;
                        sto:hasPages "35"^^xsd:int ;
                        sto:hasPublicationDate "2001-01-12"^^xsd:date ;
                        sto:hasStabilityDate "2018"^^xsd:gYear ;
                        sto:hasTag "IEC 61334-3-22:2001 "@en ;
                        dcterms:title "Distribution automation using distribution line carrier systems - Part 3-22: Mains signalling requirements - MV phase-to-earth and screen-to-earth intrusive coupling devices"@en ;
                        rdfs:comment """Establishes definitions, requirements, methods of testing and rated values for phase-to-earth capacitive and screen-to-earth intrusive inductive coupling devices to be used in medium voltage DLC systems.
This publication is of high relevance for Smart Grid."""@en ,
                                     "Establishes definitions, requirements, methods of testing and rated values for phase-to-earth capacitive and screen-to-earth intrusive inductive coupling devices to be used in medium voltage DLC systems.nThis publication is of high relevance for Smart Grid."@en ;
                        rdfs:label "IEC 61334-3-22:2001"@en ;
                        sto:hasDBpediaResource <https://dbpedia.org/resource/IEC_61334> ;
                        sto:hasOfficialResource <https://webstore.iec.ch/publication/5299> ;
                        sto:hasWikipediaArticle <https://en.wikipedia.org/wiki/IEC_61334> .


###  https://w3id.org/i40/sto#IEC_61334_P4_S1_E1
sto:IEC_61334_P4_S1_E1 rdf:type owl:NamedIndividual ,
                                sto:Standard ;
                       dcterms:creator sto:sebastian , 
                                 sto:irlan ;
                       sto:hasAvailableLanguage lang:eng ,
                                                lang:fra ;
                       sto:hasFileSize sto:FileSizeIEC_61334_P4_S1 ;
                       sto:hasICS sto:ICS_29_240_20 ,
                                  sto:ICS_33_200 ;
                       sto:hasPublisher sto:IEC ;
                       sto:hasTechnicalCommittee sto:TC_57 ;
                        sto:isPartOf sto:IEC_61334;
                       sto:hasEdition "1.0"^^xsd:float ;
                       sto:hasPages "43"^^xsd:int ;
                       sto:hasPublicationDate "1996-07-31"^^xsd:date ;
                       sto:hasStabilityDate "2018"^^xsd:gYear ;
                       sto:hasTag "IEC 61334-4-1:1996 "@en ;
                       dcterms:title "Distribution automation using distribution line carrier systems - Part 4: Data communication protocols - Section 1: Reference model of the communication system"@en ;
                       rdfs:comment """Provides a basic description of the communication system based on a three layer model. Application examples are control and monitoring of the distribution network, order broadcast, control of user interfaces, public lighting, automatic meter reading, etc.
This publication is of high relevance for Smart Grid."""@en ,
                                    "Provides a basic description of the communication system based on a three layer model. Application examples are control and monitoring of the distribution network, order broadcast, control of user interfaces, public lighting, automatic meter reading, etc.nThis publication is of high relevance for Smart Grid."@en ;
                       rdfs:label "IEC 61334-4-1:1996 "@en ;
                       sto:hasDBpediaResource <https://dbpedia.org/resource/IEC_61334> ;
                       sto:hasOfficialResource <https://webstore.iec.ch/publication/5300> ;
                       sto:hasWikipediaArticle <https://en.wikipedia.org/wiki/IEC_61334> .


###  https://w3id.org/i40/sto#IEC_61334_P4_S32_E1
sto:IEC_61334_P4_S32_E1 rdf:type owl:NamedIndividual ,
                                 sto:Standard ;
                        dcterms:creator sto:sebastian , 
                                 sto:irlan ;
                        sto:hasAvailableLanguage lang:eng ,
                                                 lang:fra ;
                        sto:hasFileSize sto:FileSizeIEC_61334_P4_S32 ;
                        sto:hasICS sto:ICS_29_240_20 ,
                                   sto:ICS_33_200 ;
                        sto:hasPublisher sto:IEC ;
                        sto:hasTechnicalCommittee sto:TC_57 ;
                        sto:isPartOf sto:IEC_61334;
                        sto:hasEdition "1.0"^^xsd:float ;
                        sto:hasPages "69"^^xsd:int ;
                        sto:hasPublicationDate "1996-09-26"^^xsd:date ;
                        sto:hasStabilityDate "2018"^^xsd:gYear ;
                        sto:hasTag "IEC 61334-4-32:1996 "@en ;
                        dcterms:title "Distribution automation using distribution line carrier systems - Part 4: Data communication protocols - Section 32: Data link layer - Logical link control (LLC)"@en ;
                        rdfs:comment """Covers the services required of, or by, the DCP Logical Link Control (LLC) sublayer entity at the logical interfaces with the application layer and the MAC sublayer.
This publication is of high relevance for Smart Grid."""@en ,
                                     "Covers the services required of, or by, the DCP Logical Link Control (LLC) sublayer entity at the logical interfaces with the application layer and the MAC sublayer.nThis publication is of high relevance for Smart Grid."@en ;
                        rdfs:label "IEC 61334-4-32:1996 "@en ;
                        sto:hasDBpediaResource <https://dbpedia.org/resource/IEC_61334> ;
                        sto:hasOfficialResource <https://webstore.iec.ch/publication/5301> ;
                        sto:hasWikipediaArticle <https://en.wikipedia.org/wiki/IEC_61334> .


###  https://w3id.org/i40/sto#IEC_61334_P4_S33_E1
sto:IEC_61334_P4_S33_E1 rdf:type owl:NamedIndividual ,
                                 sto:Standard ;
                        dcterms:creator sto:sebastian , 
                                 sto:irlan ;
                        sto:hasAvailableLanguage lang:eng ,
                                                 lang:fra ;
                        sto:hasFileSize sto:FileSizeIEC_61334_P4_S3 ;
                        sto:hasICS sto:ICS_29_240_20 ,
                                   sto:ICS_33_200 ;
                        sto:hasPublisher sto:IEC ;
                        sto:hasTechnicalCommittee sto:TC_57 ;
                        sto:isPartOf sto:IEC_61334;
                        sto:hasEdition "1.0"^^xsd:float ;
                        sto:hasPages "51"^^xsd:int ;
                        sto:hasPublicationDate "1998-07-10"^^xsd:date ;
                        sto:hasStabilityDate "2018"^^xsd:gYear ;
                        sto:hasTag "IEC 61334-4-33:1998 "@en ;
                        dcterms:title "Distribution automation using distribution line carrier systems - Part 4-33: Data communication protocols - Data link layer - Connection oriented protocol"@en ;
                        rdfs:comment "Covers the services required by the data communication protocol (DCP) logical link control (LLC) sublayer entity at the logical interfaces with the LLC -user layer and the MAC sublayer, using the connection-oriented LLC procedures.nThis publication is of high relevance for Smart Grid."@en ;
                        rdfs:label "IEC 61334-4-33:1998 "@en ;
                        sto:hasDBpediaResource <https://dbpedia.org/resource/IEC_61334> ;
                        sto:hasOfficialResource <https://webstore.iec.ch/publication/5302> ;
                        sto:hasWikipediaArticle <https://en.wikipedia.org/wiki/IEC_61334> .


###  https://w3id.org/i40/sto#IEC_61334_P4_S41_E1
sto:IEC_61334_P4_S41_E1 rdf:type owl:NamedIndividual ,
                                 sto:Standard ;
                        dcterms:creator sto:sebastian , 
                                 sto:irlan ;
                        sto:hasAvailableLanguage lang:eng ,
                                                 lang:fra ;
                        sto:hasFileSize sto:FileSizeIEC_61334_P4_S41 ;
                        sto:hasICS sto:ICS_29_240_20 ,
                                   sto:ICS_33_200 ;
                        sto:hasPublisher sto:IEC ;
                        sto:hasTechnicalCommittee sto:TC_57 ;
                        sto:isPartOf sto:IEC_61334;
                        sto:hasEdition "1.0"^^xsd:float ;
                        sto:hasPages "247"^^xsd:int ;
                        sto:hasPublicationDate "1996-08-13"^^xsd:date ;
                        sto:hasStabilityDate "2018"^^xsd:gYear ;
                        sto:hasTag "IEC 61334-4-41:1996"@en ;
                        dcterms:title "Distribution automation using distribution line carrier systems - Part 4: Data communication protocols - Section 41: Application protocol - Distribution line message specification"@en ;
                        rdfs:comment """Defines the distribution line message specification (DLMS) within the OSI application layer.
This publication is of high relevance for Smart Grid."""@en ,
                                     "Defines the distribution line message specification (DLMS) within the OSI application layer.nThis publication is of high relevance for Smart Grid."@en ;
                        rdfs:label "IEC 61334-4-41:1996"@en ;
                        sto:hasDBpediaResource <https://dbpedia.org/resource/IEC_61334> ;
                        sto:hasOfficialResource <https://webstore.iec.ch/publication/5303> ;
                        sto:hasWikipediaArticle <https://en.wikipedia.org/wiki/IEC_61334> .


###  https://w3id.org/i40/sto#IEC_61334_P4_S42_E1
sto:IEC_61334_P4_S42_E1 rdf:type owl:NamedIndividual ,
                                 sto:Standard ;
                        dcterms:creator sto:irlan;
                        sto:hasAvailableLanguage lang:eng ,
                                                 lang:fra ;
                        sto:hasFileSize sto:FileSizeIEC_61334_P4_S42 ;
                        sto:hasICS sto:ICS_29_240_20 ,
                                   sto:ICS_33_200 ;
                        sto:hasPublisher sto:IEC ;
                        sto:hasTechnicalCommittee sto:TC_57 ;
                        sto:isPartOf sto:IEC_61334;
                        sto:hasEdition "1.0"^^xsd:float ;
                        sto:hasPages "89"^^xsd:int ;
                        sto:hasPublicationDate "1996-10-09"^^xsd:date ;
                        sto:hasStabilityDate "2018"^^xsd:gYear ;
                        sto:hasTag "IEC 61334-4-42:1996"@en ;
                        dcterms:title "Distribution automation using distribution line carrier systems -Part 4: Data communication protocols - Section 42: Applicationprotocols - Application laye"@en ;
                        rdfs:comment """Describes the rules used to design an application service element, the ISO connectionless ACSE (Application Control Service Element), and the DLMS Application Service Element.
This publication is of high relevance for Smart Grid."""@en ,
                                     "Describes the rules used to design an application service element, the ISO connectionless ACSE (Application Control Service Element), and the DLMS Application Service Element.nThis publication is of high relevance for Smart Grid."@en ;
                        rdfs:label "IEC 61334-4-42:1996"@en ;
                        sto:hasDBpediaResource <https://dbpedia.org/resource/IEC_61334> ;
                        sto:hasOfficialResource <https://webstore.iec.ch/publication/5304> ;
                        sto:hasWikipediaArticle <https://en.wikipedia.org/wiki/IEC_61334> .


###  https://w3id.org/i40/sto#IEC_61334_P4_S511_E1
sto:IEC_61334_P4_S511_E1 rdf:type owl:NamedIndividual ,
                                  sto:Standard ;
                         dcterms:creator sto:irlan;
                         sto:hasAvailableLanguage lang:eng ,
                                                  lang:fra ;
                         sto:hasFileSize sto:FileSizeIEC_61334_P4_S511 ;
                         sto:hasICS sto:ICS_33_040_40 ,
                                    sto:ICS_33_200 ;
                         sto:hasPublisher sto:IEC ;
                         sto:hasTechnicalCommittee sto:TC_57 ;
                        sto:isPartOf sto:IEC_61334;
                         sto:hasEdition "1.0"^^xsd:float ;
                         sto:hasPages "65"^^xsd:int ;
                         sto:hasPublicationDate "2000-04-18"^^xsd:date ;
                         sto:hasStabilityDate "2018"^^xsd:gYear ;
                         sto:hasTag "IEC 61334-4-511:2000"@en ;
                         dcterms:title "Distribution automation using distribution line carrier systems - Part 4-511: Data communication protocols - Systems management - CIASE protocol"@en ;
                         rdfs:comment """Specifies the data communication protocol (DCP) management requirements. Describes the management services in an abstract way as well as the underlying protocol.
This publication is of high relevance for Smart Grid."""@en ,
                                      "Specifies the data communication protocol (DCP) management requirements. Describes the management services in an abstract way as well as the underlying protocol.nThis publication is of high relevance for Smart Grid."@en ;
                         rdfs:label "IEC 61334-4-511:2000"@en ;
                         sto:hasDBpediaResource <https://dbpedia.org/resource/IEC_61334> ;
                         sto:hasOfficialResource <https://webstore.iec.ch/publication/5305> ;
                         sto:hasWikipediaArticle <https://en.wikipedia.org/wiki/IEC_61334> .


###  https://w3id.org/i40/sto#IEC_61334_P4_S512_E1
sto:IEC_61334_P4_S512_E1 rdf:type owl:NamedIndividual ,
                                  sto:Standard ;
                         dcterms:creator sto:irlan;
                         sto:hasAvailableLanguage lang:eng ,
                                                  lang:fra ;
                         sto:hasFileSize sto:FileSizeIEC_61334_P4_S512 ;
                         sto:hasICS sto:ICS_33_200 ;
                         sto:hasPublisher sto:IEC ;
                         sto:hasTechnicalCommittee sto:TC_57 ;
                         sto:isPartOf sto:IEC_61334;
                         sto:hasEdition "1.0"^^xsd:float ;
                         sto:hasPages "47"^^xsd:int ;
                         sto:hasPublicationDate "2001-10-30"^^xsd:date ;
                         sto:hasStabilityDate "2018"^^xsd:gYear ;
                         sto:hasTag "IEC 61334-4-512:2001"@en ;
                         dcterms:title "Distribution automation using distribution line carrier systems - Part 4-512: Data communication protocols - System management using profile 61334-5-1 - Management Information Base (MIB)"@en ;
                         rdfs:comment """Specifies the Management Information Base (MIB), which is used for the management of the communication profile defined by the following standards: IEC 61334-5-1, IEC 61334-4-32, IEC 61334-4-42, and IEC 61334-4-41.
This publication is of high relevance for Smart Grid."""@en ,
                                      "Specifies the Management Information Base (MIB), which is used for the management of the communication profile defined by the following standards: IEC 61334-5-1, IEC 61334-4-32, IEC 61334-4-42, and IEC 61334-4-41.nThis publication is of high relevance for Smart Grid."@en ;
                         rdfs:label "IEC 61334-4-512:2001"@en ;
                         sto:hasDBpediaResource <https://dbpedia.org/resource/IEC_61334> ;
                         sto:hasOfficialResource <https://webstore.iec.ch/publication/5306> ;
                         sto:hasWikipediaArticle <https://en.wikipedia.org/wiki/IEC_61334> .


###  https://w3id.org/i40/sto#IEC_61334_P4_S61_E1
sto:IEC_61334_P4_S61_E1 rdf:type owl:NamedIndividual ,
                                 sto:Standard ;
                        dcterms:creator sto:irlan;
                        sto:hasAvailableLanguage lang:eng ,
                                                 lang:fra ;
                        sto:hasFileSize sto:FileSizeIEC_61334_P4_S61 ;
                        sto:hasICS sto:ICS_29_240_20 ,
                                   sto:ICS_33_200 ;
                        sto:hasPublisher sto:IEC ;
                        sto:hasTechnicalCommittee sto:TC_57 ;
                        sto:isPartOf sto:IEC_61334;
                        sto:hasEdition "1.0"^^xsd:float ;
                        sto:hasPages "63"^^xsd:int ;
                        sto:hasPublicationDate "1998-07-10"^^xsd:date ;
                        sto:hasStabilityDate "2018"^^xsd:gYear ;
                        sto:hasTag "IEC 61334-4-61:1998"@en ;
                        dcterms:title "Distribution automation using distribution line carrier systems - Part 4-61: Data communication protocols - Network layer - Connectionless protocol"@en ;
                        rdfs:comment """Covers the services required by the data communication protocol (DCP) network layer (N) sublayer entity at the logical interfaces with the N user layer and the LLC sublayer, using the connectionless N procedures.
This publication is of high relevance for Smart Grid."""@en ,
                                     "Covers the services required by the data communication protocol (DCP) network layer (N) sublayer entity at the logical interfaces with the N user layer and the LLC sublayer, using the connectionless N procedures.nThis publication is of high relevance for Smart Grid."@en ;
                        rdfs:label "IEC 61334-4-61:1998"@en ;
                        sto:hasDBpediaResource <https://dbpedia.org/resource/IEC_61334> ;
                        sto:hasOfficialResource <https://webstore.iec.ch/publication/5307> ;
                        sto:hasWikipediaArticle <https://en.wikipedia.org/wiki/IEC_61334> .


###  https://w3id.org/i40/sto#IEC_61334_P5_S1_E2
sto:IEC_61334_P5_S1_E2 rdf:type owl:NamedIndividual ,
                                sto:Standard ;
                       dcterms:creator sto:irlan;
                       sto:hasAvailableLanguage lang:eng ,
                                                lang:fra ;
                       sto:hasFileSize sto:FileSizeIEC_61334_P5_S1 ;
                       sto:hasICS sto:ICS_33_200 ;
                       sto:hasPublisher sto:IEC ;
                       sto:hasTechnicalCommittee sto:TC_57 ;
                        sto:isPartOf sto:IEC_61334;
                       sto:hasRelevantDomain sto:SmartCity ;
                       sto:hasEdition "2.0"^^xsd:float ;
                       sto:hasPages "123"^^xsd:int ;
                       sto:hasPublicationDate "2001-05-28"^^xsd:date ;
                       sto:hasStabilityDate "2018"^^xsd:gYear ;
                       sto:hasTag "IEC 61334-5-1:2001"@en ;
                       dcterms:title "Distribution automation using distribution line carrier systems - Part 5-1: Lower layer profiles - The spread frequency shift keying (S-FSK) profile"@en ;
                       rdfs:comment """Describes the requirements of S-FSK (frequency shift keying modulation) in conjunction with the services provided by the physical layer entity and the MAC sublayer. The transmission medium is assumed to be the distribution network on both MV or LV level. To be used in conjunction with IEC 61334-4-32.
This publication is of high relevance for Smart Grid."""@en ,
                                    "Describes the requirements of S-FSK (frequency shift keying modulation) in conjunction with the services provided by the physical layer entity and the MAC sublayer. The transmission medium is assumed to be the distribution network on both MV or LV level. To be used in conjunction with IEC 61334-4-32.nThis publication is of high relevance for Smart Grid."@en ;
                       rdfs:label "IEC 61334-5-1:2001"@en ;
                       sto:hasDBpediaResource <https://dbpedia.org/resource/IEC_61334> ;
                       sto:hasOfficialResource <https://webstore.iec.ch/publication/5308> ;
                       sto:hasWikipediaArticle <https://en.wikipedia.org/wiki/IEC_61334> .


###  https://w3id.org/i40/sto#IEC_61334_P6_E1
sto:IEC_61334_P6_E1 rdf:type owl:NamedIndividual ,
                             sto:Standard ;
                    dcterms:creator sto:irlan ;
                    sto:hasAvailableLanguage lang:eng ,
                                             lang:fra ;
                    sto:hasFileSize sto:FileSizeIEC_61334_P6 ;
                    sto:hasICS sto:ICS_29_240_20 ,
                               sto:ICS_33_200 ;
                    sto:hasPublisher sto:IEC ;
                    sto:hasTechnicalCommittee sto:TC_57 ;
                    sto:isPartOf sto:IEC_61334;
                    sto:hasEdition "1.0"^^xsd:float ;
                    sto:hasPages "75"^^xsd:int ;
                    sto:hasPublicationDate "2000-06-16"^^xsd:date ;
                    sto:hasStabilityDate "2018"^^xsd:gYear ;
                    sto:hasTag "IEC 61334-6:2000"@en ;
                    dcterms:title "Distribution automation using distribution line carrier systems - Part 6: A-XDR encoding rule"@en ;
                    rdfs:comment """Defines a set of encoding rules that may be used to derive the specification of a transfer syntax for values of types defined in the DLMS core standard using the ASN.1 notation (see IEC 61334-4-41).
This publication is of high relevance for Smart Grid."""@en ,
                                 "Defines a set of encoding rules that may be used to derive the specification of a transfer syntax for values of types defined in the DLMS core standard using the ASN.1 notation (see IEC 61334-4-41).nThis publication is of high relevance for Smart Grid."@en ;
                    rdfs:label "IEC 61334-6:2000"@en ;
                    sto:hasDBpediaResource <https://dbpedia.org/resource/IEC_61334> ;
                    sto:hasOfficialResource <https://webstore.iec.ch/publication/5313> ;
                    sto:hasWikipediaArticle <https://en.wikipedia.org/wiki/IEC_61334> .


###  https://w3id.org/i40/sto#IEC_61360
sto:IEC_61360 rdf:type owl:NamedIndividual ,
                       sto:Standard ;
              dcterms:creator sto:irlan;
              sto:hasClassification sto:AsEngineering ,
                                    sto:IDSRAMInformationLayer ,
                                    sto:NISTManufacturingModelData ,
                                    sto:RamiAssetlayer ;
              sto:hasPublisher sto:IEC ;
              sto:relatedTo sto:DIN_SPEC_16592 ,
                            sto:IEC_61131 ,
                            sto:IEC_61360 ,
                            sto:IEC_61499 ,
                            sto:IEC_61804 ,
                            sto:IEC_61850 ,
                            sto:IEC_61987_X ,
                            sto:IEC_62424 ,
                            sto:IEC_62453 ,
                            sto:IEC_62541 ,
                            sto:IEC_62714 ,
                            sto:ISO_13584 ,
                            sto:ISO_14306 ,
                            sto:ISO_15746 ,
                            sto:ISO_15926 ,
                            sto:ISO_18629 ,
                            sto:ISO_18828-2 ,
                            sto:ISO_20922 ,
                            sto:ISO_22400 ,
                            sto:ISO_29002 ,
                            sto:ISO_ASTM_52915 ,
                            sto:ISO_PAS_17506 ,
                            sto:MathML ,
                            sto:SysML ,
                            sto:eClass ;
              sto:hasMotivation "Standard data elements (properties) are used as elements in administration shell"@en ;
              sto:hasTag "IEC Common Data Dictionary"@en ;
              rdfs:comment "IEC Common Data Dictionary (IEC CDD) is a common repository of concepts for all electrotechnical domains based on the methodology and the information model of IEC 61360 series. Standard data elements types with associated classification scheme for electric items."@en ;
              rdfs:label "IEC 61360"@en ;
              sto:hasRelevantDomain sto:Electrotechnical ;
              sto:hasMotivation "Standard data elements (properties) are used as elements in administration shell"@en ;
              sto:hasOfficialResource <http://cdd.iec.ch/cdd/iec61360/iec61360.nsf> ,
                                      <https://webstore.iec.ch/publication/5380> .


###  https://w3id.org/i40/sto#IEC_61400
sto:IEC_61400 rdf:type owl:NamedIndividual ,
                       sto:Standard ;
              dcterms:creator sto:irlan ;
              sto:hasPublisher sto:IEC ;
              sto:hasPublicationDate "2017-03-03"^^xsd:date ;
              rdfs:comment "IEC 61334 , known as Distribution automation using distribution line carrier systems, is a standard for low-speed reliable power line communications by electricity meters, water meters and SCADA."@en ;
              rdfs:label "IEC 61400"@en ;
              sto:hasDBpediaResource <http://dbpedia.org/page/IEC_61400> ;
              sto:hasOfficialResource <https://webstore.iec.ch/publication/26603> .


###  https://w3id.org/i40/sto#IEC_61400_P25_S1_E2
sto:IEC_61400_P25_S1_E2 rdf:type owl:NamedIndividual ,
                                 sto:Standard ;
                        dcterms:creator sto:irlan ;
                        sto:hasAvailableLanguage lang:eng ;
                        sto:hasFileSize sto:FileSizeIEC_61400_P25_S1 ;
                        sto:hasICS sto:ICS_27_180 ;
                        sto:hasPublisher sto:IEC ;
                        sto:hasTechnicalCommittee sto:TC_88 ;
                        sto:relatedTo sto:IEC_61400_P25_S2_E2 ;
                        sto:isPartOf sto:IEC_61400;
                        sto:hasEdition "2.0"^^xsd:float ;
                        sto:hasPages "109"^^xsd:int ;
                        sto:hasPublicationDate "2017-07-20"^^xsd:date ;
                        sto:hasStabilityDate "2020"^^xsd:gYear ;
                        sto:hasTag "IEC 61400-25-1:2017"@en ;
                        dcterms:title "Wind energy generation systems - Part 25-1: Communications for monitoring and control of wind power plants - Overall description of principles and models"@en ;
                        rdfs:comment """IEC 61400-25-1:2017 RLV contains the International Standard and its Redline version. The Redline version is available in English only. The Redline version provides you with a quick and easy way to compare all the changes between this standard and its previous edition. The Redline version is not an official IEC Standard, only the current version of the standard is to be considered the official document. 
IEC 61400-25-1:2017 gives an overall description of the principles and models used in the IEC 61400-25 series, which is designed for a communication environment supported by a client-server model. Three areas are defined, that are modelled separately to ensure the scalability of implementations: wind power plant information models, information exchange model, and mapping of these two models to a standard communication profile. This new edition includes the following significant technical changes with respect to the previous edition: general harmonization of text and overview models with the other parts of the IEC 61400-25 series, harmonization of definitions in other related standards."""@en ,
                                     "IEC 61400-25-1:2017 RLV contains the International Standard and its Redline version. The Redline version is available in English only. The Redline version provides you with a quick and easy way to compare all the changes between this standard and its previous edition. The Redline version is not an official IEC Standard, only the current version of the standard is to be considered the official document.nnIEC 61400-25-1:2017 gives an overall description of the principles and models used in the IEC 61400�25 series, which is designed for a communication environment supported by a client-server model. Three areas are defined, that are modelled separately to ensure the scalability of implementations: wind power plant information models, information exchange model, and mapping of these two models to a standard communication profile. This new edition includes the following significant technical changes with respect to the previous edition: general harmonization of text and overview models with the other parts of the IEC 61400�25 series, harmonization of definitions in other related standards."@en ;
                        rdfs:label "IEC 61400-25-1:2017"@en ;
                        sto:hasOfficialResource <https://webstore.iec.ch/publication/61087> .


###  https://w3id.org/i40/sto#IEC_61400_P25_S2_E2
sto:IEC_61400_P25_S2_E2 rdf:type owl:NamedIndividual ,
                                 sto:Standard ;
                        dcterms:creator sto:irlan ;
                        sto:hasAvailableLanguage lang:eng ,
                                                 lang:fra ;
                        sto:hasFileSize sto:FileSizeIEC_61400_P25_S2 ;
                        sto:hasICS sto:ICS_27_180 ;
                        sto:hasPublisher sto:IEC ;
                        sto:hasTechnicalCommittee sto:TC_88 ;
                        sto:isPartOf sto:IEC_61400;
                        sto:hasEdition "2.0"^^xsd:float ;
                        sto:hasPages "221"^^xsd:int ;
                        sto:hasPublicationDate "2015-06-30"^^xsd:date ;
                        sto:hasStabilityDate "2018"^^xsd:gYear ;
                        sto:hasTag "IEC 61400-25-2:2015 "@en ;
                        dcterms:title "Wind turbines - Part 25-2: Communications for monitoring and control of wind power plants - Information models"@en ;
                        rdfs:comment """IEC 61400-25-2:2015 specifies the information model of devices and functions related to wind power plant applications. In particular, it specifies the compatible logical node names, and data names for communication between wind power plant components. This includes the relationship between logical devices, logical nodes and data. The names defined in the IEC 61400-25 series are used to build the hierarchical object references applied for communicating with components in wind power plants. Main changes with respect to the previous edition consist of:
- harmonization with newer editions of IEC 61850 standards;
- reduction of overlap between standards and simplification by increased referencing,
- extension of data objects for operation of smart grids,
- extended and enhanced semantics for existing data objects, etc."""@en ,
                                     "IEC 61400-25-2:2015 specifies the information model of devices and functions related to wind power plant applications. In particular, it specifies the compatible logical node names, and data names for communication between wind power plant components. This includes the relationship between logical devices, logical nodes and data. The names defined in the IEC 61400-25 series are used to build the hierarchical object references applied for communicating with components in wind power plants. Main changes with respect to the previous edition consist of:- harmonization with newer editions of IEC 61850 standards;- reduction of overlap between standards and simplification by increased referencing,- extension of data objects for operation of smart grids,- extended and enhanced semantics for existing data objects, etc."@en ;
                        rdfs:label "IEC 61400-25-2:2015 "@en ;
                        sto:hasOfficialResource <https://webstore.iec.ch/publication/22813> .


###  https://w3id.org/i40/sto#IEC_61400_P25_S3_E2
sto:IEC_61400_P25_S3_E2 rdf:type owl:NamedIndividual ,
                                 sto:Standard ;
                        dcterms:creator sto:irlan ;
                        sto:hasAvailableLanguage lang:eng ;
                        sto:hasFileSize sto:FileSizeIEC_61400_P25_S3 ;
                        sto:hasICS sto:ICS_27_180 ;
                        sto:hasPublisher sto:IEC ;
                        sto:hasTechnicalCommittee sto:TC_88 ;
                        sto:relatedTo sto:IEC_61400_P25_S2_E2 ;
                        sto:hasEdition "2.0"^^xsd:float ;
                        sto:hasPages "103"^^xsd:int ;
                        sto:hasPublicationDate "2015-06-30"^^xsd:date ;
                        sto:hasStabilityDate "2018"^^xsd:gYear ;
                        sto:hasTag "IEC 61400-25-3:2015"@en ;
                        dcterms:title "Wind turbines - Part 25-3: Communications for monitoring and control of wind power plants - Information exchange models"@en ;
                        rdfs:comment """IEC 61400-25-3:2015 RLV contains the International Standard and its Redline version. The Redline version is available in English only. The Redline version provides you with a quick and easy way to compare all the changes between this standard and its previous edition. The Redline version is not an official IEC Standard, only the current version of the standard is to be considered the official document.
IEC 61400-25-3:2015 specifies an abstract communication service interface describing the information exchange between a client and a server for:
- data access and retrieval,
- device control,
- event reporting and logging,
- self-description of devices (device data dictionary),
- data typing and discovery of data types.
Main changes with respect to the previous edition consist of:
- harmonization with newer editions of IEC 61850 standards;
- reduction of overlap between standards and simplification by increased referencing, etc."""@en ,
                                     "IEC 61400-25-3:2015 RLV contains the International Standard and its Redline version. The Redline version is available in English only. The Redline version provides you with a quick and easy way to compare all the changes between this standard and its previous edition. The Redline version is not an official IEC Standard, only the current version of the standard is to be considered the official document.nIEC 61400-25-3:2015 specifies an abstract communication service interface describing the information exchange between a client and a server for:n- data access and retrieval,n- device control,n- event reporting and logging,n- self-description of devices (device data dictionary),n- data typing and discovery of data types.nMain changes with respect to the previous edition consist of:n- harmonization with newer editions of IEC 61850 standards;n- reduction of overlap between standards and simplification by increased referencing, etc."@en ;
                        rdfs:label "IEC 61400-25-3:2015"@en ;
                        sto:hasOfficialResource <https://webstore.iec.ch/publication/22808> .

sto:OPC_XML-DA rdf:type owl:NamedIndividual ,
                           sto:TechnicalSpecification ;
                  dcterms:creator sto:priyanka ;
                  sto:hasPublisher sto:OPC_Foundation ;
                  sto:hasPublicationDate "2004-12-01"^^xsd:date ;
                  sto:hasTag "OPC XML-DA"^^xsd:string ;
                  rdfs:comment "OPC XML-DA builds on the OPC Data Access specifications to communicate data in XML. Incorporates SOAP and Web services"@en ;
                  rdfs:label "OPC_XML-DA"@en ;
                  sto:hasOfficialResource <https://www.opcconnect.com/xml.php#xmlspec>;
                  sto:hasOpenResource <http://www.diit.unict.it/users/scava/dispense/II/OPCDataAccessXMLSpecification.pdf> .

sto:SOAP rdf:type owl:NamedIndividual ,
                           sto:TechnicalSpecification ;
                           dcterms:creator sto:priyanka ;
                  sto:hasTag "SOAP"^^xsd:string ;
                  rdfs:comment "SOAP (abbreviation for Simple Object Access Protocol) is a messaging protocol specification for exchanging structured information in the implementation of web services in computer networks."@en ;
                  rdfs:label "SOAP"@en ;
                  sto:hasWikipediaArticle <https://en.wikipedia.org/wiki/SOAP>.

###  https://w3id.org/i40/sto#IEC_61400_P25_S4_E2
sto:IEC_61400_P25_S4_E2 rdf:type owl:NamedIndividual ,
                                 sto:Standard ;
                        dcterms:creator sto:irlan ;
                        sto:hasAvailableLanguage lang:eng ;
                        sto:hasFileSize sto:FileSizeIEC_61400_P25_S4 ;
                        sto:hasICS sto:ICS_27_180 ;
                        sto:hasPublisher sto:IEC ;
                        sto:relatedTo sto:SOAP,
                                      sto:OPC_XML-DA,
                                      sto:IEC_61850_P8_S1_E2,
                                      sto:IEC_60870_P5_S104_E2_1,
                                      sto:IEEE_1815-2012;
                        sto:hasTechnicalCommittee sto:TC_88 ;
                        sto:relatedTo sto:IEC_61400_P25_S2_E2 ;
                        sto:isPartOf sto:IEC_61400;
                        sto:hasEdition "2.0"^^xsd:float ;
                        sto:hasPages "829"^^xsd:int ;
                        sto:hasPublicationDate "2016-11-30"^^xsd:date ;
                        sto:hasStabilityDate "2018"^^xsd:gYear ;
                        sto:hasTag "IEC 61400-25-4:2016"@en ;
                        dcterms:title "Wind energy generation systems - Part 25-4: Communications for monitoring and control of wind power plants - Mapping to communication profile"@en ;
                        rdfs:comment """IEC 61400-25-4:2016 RLV contains the International Standard and its Redline version. The Redline version is available in English only. The Redline version provides you with a quick and easy way to compare all the changes between this standard and its previous edition. The Redline version is not an official IEC Standard, only the current version of the standard is to be considered the official document.
IEC 61400-25-4:2016 specifies the specific mappings to protocol stacks encoding the messages required for the information exchange between a client and a remote server for: data access and retrieval, device control, event reporting and logging, publisher/subscriber, self-description of devices (device data dictionary), data typing and discovery of data types. The mappings specified in this part of IEC 61400-25 comprise:
- a mapping to SOAP-based web services,
- a mapping to OPC/XML-DA,
- a mapping to IEC 61850-8-1 MMS,
- a mapping to IEC 60870-5-104,
- a mapping to DNP3.
The main technical changes with regard to the previous edition are as follows:
- general harmonization with information models in IEC 61400-25-2 and information exchange services in IEC 61400-25-3;
- reduction of overlap between standards and simplification by increased referencing."""@en ,
                                     "IEC 61400-25-4:2016 RLV contains the International Standard and its Redline version. The Redline version is available in English only. The Redline version provides you with a quick and easy way to compare all the changes between this standard and its previous edition. The Redline version is not an official IEC Standard, only the current version of the standard is to be considered the official document.nnIEC 61400-25-4:2016 specifies the specific mappings to protocol stacks encoding the messages required for the information exchange between a client and a remote server for: data access and retrieval, device control, event reporting and logging, publisher/subscriber, self-description of devices (device data dictionary), data typing and discovery of data types. The mappings specified in this part of IEC 61400-25 comprise:n- a mapping to SOAP-based web services,n- a mapping to OPC/XML-DA,n- a mapping to IEC 61850-8-1 MMS,n- a mapping to IEC 60870-5-104,n- a mapping to DNP3.nThe main technical changes with regard to the previous edition are as follows:n- general harmonization with information models in IEC 61400-25-2 and information exchange services in IEC 61400-25-3;n- reduction of overlap between standards and simplification by increased referencing."@en ;
                        rdfs:label "IEC 61400-25-4:2016"@en ;
                        sto:hasOfficialResource <https://webstore.iec.ch/publication/59497> .


###  https://w3id.org/i40/sto#IEC_61400_P25_S5_E2
sto:IEC_61400_P25_S5_E2 rdf:type owl:NamedIndividual ,
                                 sto:Standard ;
                        dcterms:creator sto:irlan ;
                        sto:hasAvailableLanguage lang:eng ;
                        sto:hasFileSize sto:FileSizeIEC_61400_P25_S5 ;
                        sto:hasICS sto:ICS_27_180 ;
                        sto:hasPublisher sto:IEC ;
                        sto:hasTechnicalCommittee sto:TC_88 ;
                        sto:relatedTo sto:IEC_61400_P25_S2_E2 ;
                        sto:isPartOf sto:IEC_61400;
                        sto:hasEdition "2.0"^^xsd:float ;
                        sto:hasPages "56"^^xsd:int ;
                        sto:hasPublicationDate "2017-09-20"^^xsd:date ;
                        sto:hasStabilityDate "2020"^^xsd:gYear ;
                        sto:hasTag "IEC 61400-25-5:2017"@en ;
                        dcterms:title "Wind energy generation systems - Part 25-5: Communications for monitoring and control of wind power plants - Compliance testing"@en ;
                        rdfs:comment """IEC 61400-25-5:2017 specifies standard techniques for testing of compliance of implementations, as well as specific measurement techniques to be applied when declaring performance parameters. The use of these techniques will enhance the ability of users to purchase systems that integrate easily, operate correctly, and support the applications as intended. This part of IEC 61400-25 defines: the methods and abstract test cases for compliance testing of server and client devices used in wind power plants; the metrics to be measured in said devices according to the communication requirements specified in IEC 61400-25 (all parts). This new edition includes the following significant technical changes with respect to the previous edition:
- harmonization with structure and test cases in IEC 61850-10:2012;
- reduction of overlap between standards and simplification by increased referencing to the IEC 61850 standard series."""@en ,
                                     "IEC 61400-25-5:2017 specifies standard techniques for testing of compliance of implementations, as well as specific measurement techniques to be applied when declaring performance parameters. The use of these techniques will enhance the ability of users to purchase systems that integrate easily, operate correctly, and support the applications as intended. This part of IEC 61400-25 defines: the methods and abstract test cases for compliance testing of server and client devices used in wind power plants; the metrics to be measured in said devices according to the communication requirements specified in IEC 61400-25 (all parts). This new edition includes the following significant technical changes with respect to the previous edition:n- harmonization with structure and test cases in IEC 61850-10:2012;n- reduction of overlap between standards and simplification by increased referencing to the IEC 61850 standard series."@en ;
                        rdfs:label "IEC 61400-25-5:2017"@en ;
                        sto:hasOfficialResource <https://webstore.iec.ch/publication/26560> .


###  https://w3id.org/i40/sto#IEC_61400_P25_S6_E2
sto:IEC_61400_P25_S6_E2 rdf:type owl:NamedIndividual ,
                                 sto:Standard ;
                        dcterms:creator sto:irlan ;
                        sto:hasAvailableLanguage lang:eng ;
                        sto:hasFileSize sto:FileSizeIEC_61400_P25_S6 ;
                        sto:hasICS sto:ICS_27_180 ;
                        sto:hasPublisher sto:IEC ;
                        sto:hasTechnicalCommittee sto:TC_88 ;
                        sto:relatedTo sto:IEC_61400_P25_S2_E2 ;
                        sto:isPartOf sto:IEC_61400;
                        sto:hasEdition "2.0"^^xsd:float ;
                        sto:hasPages "49"^^xsd:int ;
                        sto:hasPublicationDate "2016-12-16"^^xsd:date ;
                        sto:hasStabilityDate "2019"^^xsd:gYear ;
                        dcterms:title "Wind energy generation systems - Part 25-6: Communications for monitoring and control of wind power plants - Logical node classes and data classes for condition monitoring"@en ;
                        rdfs:comment """IEC 61400-25-6:2016(E) specifies the information models related to condition monitoring for wind power plants and the information exchange of data values related to these models. This standard is to be used with other standards of the IEC 61400-25 series. This new edition includes the following significant technical changes with respect to the previous edition:
- major restructuring of the data model to accommodate flexibility; removal of UFF58 format;
- access to data using the standard reporting and logging functions;
- recommendations for creating data names to accommodate flexibility."""@en ,
                                     "IEC 61400-25-6:2016(E) specifies the information models related to condition monitoring for wind power plants and the information exchange of data values related to these models. This standard is to be used with other standards of the IEC 61400-25 series. This new edition includes the following significant technical changes with respect to the previous edition:n- major restructuring of the data model to accommodate flexibility; removal of UFF58 format;n- access to data using the standard reporting and logging functions;n- recommendations for creating data names to accommodate flexibility."@en ;
                        rdfs:label "IEC 61400-25-6:2016"@en ;
                        sto:hasOfficialResource <https://webstore.iec.ch/publication/32580> .


###  https://w3id.org/i40/sto#IEC_61499
sto:IEC_61499 rdf:type owl:NamedIndividual ,
                       sto:Standard ;
              dcterms:creator sto:irlan ;
              sto:hasClassification sto:RamiControlDevice ,
                                    sto:RamiFieldDevice ;
              sto:hasPublisher sto:IEC ;
              sto:relatedTo sto:DIN_SPEC_16592 ,
                            sto:IEC_61131 ,
                            sto:IEC_61360 ,
                            sto:IEC_61499 ,
                            sto:IEC_61804 ,
                            sto:IEC_61850 ,
                            sto:IEC_61987_X ,
                            sto:IEC_62424 ,
                            sto:IEC_62453 ,
                            sto:IEC_62541 ,
                            sto:IEC_62714 ,
                            sto:ISO_13584 ,
                            sto:ISO_14306 ,
                            sto:ISO_15746 ,
                            sto:ISO_15926 ,
                            sto:ISO_18629 ,
                            sto:ISO_18828-2 ,
                            sto:ISO_20922 ,
                            sto:ISO_22400 ,
                            sto:ISO_29002 ,
                            sto:ISO_ASTM_52915 ,
                            sto:ISO_PAS_17506 ,
                            sto:MathML ,
                            sto:SysML ,
                            sto:eClass ;
              sto:hasMotivation "Functional description, informational representation and communication mapping of application functionality. This standard describes how a distributed control application is composed of functional units (FB), which are executed in different context. It may help to describe how functions are distributed between different I40-Components and how the execution of the functions between the different I40-Components is controled."@en ;
              sto:hasPublicationDate "2012-11-07"^^xsd:date ;
              sto:hasTag "FBs distributed systems"@en ;
              rdfs:comment "Function Blocks - Architecture Related Applications http://www.eclipse.org/4diac/ (sourceforge.net/projects/oooneida-fbench/) http://timeme.io/  not accepted by the Industry yet. http://www.holobloc.com/Proposed for IEC to overcome the restricctions of IEC 61131"@en ;
              rdfs:label "IEC 61499"@en ;
              sto:hasDBpediaResource <http://dbpedia.org/resource/IEC_61499> ;
              sto:hasOfficialResource <https://webstore.iec.ch/publication/5506> ;
              sto:hasWikipediaArticle <https://en.wikipedia.org/wiki/IEC_61499> .


###  https://w3id.org/i40/sto#IEC_61506
sto:IEC_61506 rdf:type owl:NamedIndividual ,
                       sto:Standard ;
              dcterms:creator sto:irlan ,
                              sto:sebastian ;
              sto:hasAvailableLanguage lang:eng ,
                                       lang:fra ;
              sto:hasFileSize sto:FileSizeIEC_61506 ;
              sto:hasICS sto:ICS_25_040_40 ;
              sto:hasPublisher sto:IEC ;
              sto:hasTechnicalCommittee sto:TC_65 ;
              sto:hasEdition "1.0"^^xsd:float ;
              sto:hasPages "119"^^xsd:int ;
              sto:hasPublicationDate "1997-02-28"^^xsd:date ;
              sto:hasStabilityDate "2018"^^xsd:gYear ;
              sto:hasTag "IEC 61506:1997"@en ;
              dcterms:title "Industrial-process measurement and control - Documentation ofapplication software"@en ;
              rdfs:comment "Defines the requirements for the documentation of software in industrial process measurement and control systems."@en ;
              rdfs:label "IEC 61506:1997"@en ;
              sto:hasOfficialResource <https://webstore.iec.ch/publication/5513> .


###  https://w3id.org/i40/sto#IEC_61508
sto:IEC_61508 rdf:type owl:NamedIndividual ,
                       sto:Standard ;
              owl:sameAs sto:ISO_61508 ;
              dcterms:creator sto:sebastian , 
                                 sto:irlan ;
              sto:hasClassification sto:AsSafety,
                                    sto:IDSRAMCertification  ;
              sto_iot:hasTargetConcern sto:Safety;
              sto:hasPublisher sto:IEC ,
                               sto:ISO ;
              sto:relatedTo sto:IEC_61508 ,
                            sto:IEC_61511 ,
                            sto:IEC_62061 ,
                            sto:ISO_13849 ;
              sto:hasMotivation "Defines the functional safety requirements established by IEC 61508 in process industry sector terminology"@en ;
              sto:hasPublicationDate "1997-02-28"^^xsd:date ;
              sto:hasTag "Functional Safety of Electrical/Electronic/Programmable Electronic Safety-related Systems"@en ;
              dcterms:license sto:PrivateLicenseDocument ;
              rdfs:comment "Functional safety is a concept applicable across all industry sectors. It is fundamental to the enabling of complex technology used for safety-related systems. It provides the assurance that the safety-related systems will offer the necessary risk reduction required to achieve safety for the equipment. The oil and gas industry, nuclear plants and the machinery sector, to name but a few, all rely heavily on functional safety to achieve safety for the equipment giving rise to the hazards."@en ;
              rdfs:label "IEC 61508"@en ;
              sto:hasDBpediaResource <http://dbpedia.org/resource/IEC_61508> ;
              sto:hasOfficialResource <http://www.iec.ch/functionalsafety/> ;
              sto:hasWikipediaArticle <https://en.wikipedia.org/wiki/IEC_61508> ;
              sto_iot:hasTargetConcern sto:Safety .


###  https://w3id.org/i40/sto#IEC_61511
sto:IEC_61511 rdf:type owl:NamedIndividual ,
                       sto:Standard ;
              dcterms:creator sto:irlan ;
              sto:hasClassification sto:IDSRAMCertification ;
              sto:hasDomain sto:FunctionalSafety ;
              sto:hasPublisher sto:IEC ;
              sto:relatedTo sto:IEC_61508 ,
                            sto:IEC_61511 ,
                            sto:IEC_62061 ,
                            sto:ISO_13849 ;
              sto:hasClassification sto:IDSRAMCertification ;
              sto_iot:hasTargetConcern sto:Safety;
              sto:hasPublicationDate "2016-02-24"^^xsd:date ;
              sto:hasTag "Functional safety - Safety instrumented systems for the process industry sector"@en ;
              dcterms:license sto:PrivateLicenseDocument ;
              rdfs:comment "IEC 61511 is a technical standard which sets out practices in the engineering of systems that ensure the safety of an industrial process through the use of instrumentation."@en ;
              rdfs:label "IEC 61511"^^xsd:string ;
              sto:hasDBpediaResource <http://dbpedia.org/resource/IEC_61511> ;
              sto:hasRelevantDomain sto:FunctionalSafety ;
              sto:hasMotivation "Defines the functional safety requirements established by IEC 61508 in process industry sector terminology"@en ;
              sto:hasOfficialResource <https://webstore.iec.ch/publication/24241> ;
              sto:hasWikipediaArticle <https://en.wikipedia.org/wiki/IEC_61511> ;
              sto_iot:hasTargetConcern sto:Safety .


###  https://w3id.org/i40/sto#IEC_61512
sto:IEC_61512 rdf:type owl:NamedIndividual ,
                       sto:Standard ;
              dcterms:creator sto:irlan ;
              sto:hasClassification sto:RamiControlDevice ,
                                    sto:RamiProduct ,
                                    sto:RamiStation ,
                                    sto:RamiWorkCenter ;
              sto:hasPublisher sto:IEC ;
              sto:hasMotivation "The standard sought to address the following problems: lack of a universal model for batch control, difficulty in communicating user requirement, integration among batch automation suppliers, difficulty in batch control configuration."@en ;
              sto:hasTag "ISA-88"@en ;
              rdfs:comment "Batch control - Models and terminology"@en ;
              rdfs:label "IEC 61512"@en ;
              sto:hasDBpediaResource <http://dbpedia.org/resource/ISA-88> ;
              sto:hasOfficialResource <https://webstore.iec.ch/publication/5528> ;
              sto:hasWikipediaArticle <https://en.wikipedia.org/wiki/ISA-88> .


###  https://w3id.org/i40/sto#IEC_61513
sto:IEC_61513 rdf:type owl:NamedIndividual ,
                       sto:Standard ;
              dcterms:creator sto:irlan ;
              sto:hasAvailableLanguage lang:eng ,
                                       lang:fra ;
              sto:hasClassification sto:Safety ;
              sto:hasPublisher sto:IEC ;
              rdfs:comment "IEC 61508 is intended to be a basic functional safety standard applicable to all kinds of industry. It defines functional safety as: “part of the overall safety relating to the EUC (Equipment Under Control) and the EUC control system which depends on the correct functioning of the E/E/PE safety-related systems, other technology safety-related systems and external risk reduction facilities.\""@en ;
              rdfs:label "IEC 61513"@en ;
              sto:hasDBpediaResource <http://dbpedia.org/resource/IEC_61508> ;
              sto:hasOfficialResource <https://webstore.iec.ch/publication/5532> ;
              sto:hasWikipediaArticle <https://en.wikipedia.org/wiki/IEC_61508> .

sto:IEC_61690 rdf:type owl:NamedIndividual ,
                             sto:Standard ;
                    sto:hasPublisher sto:IEC ;
                    dcterms:title "Electronic design interchange format (EDIF) "@en ;
                    rdfs:comment "IEC 61690 defines the syntax and semantics for EDIF "@en ;
                    rdfs:label "IEC 61690"@en .

###  https://w3id.org/i40/sto#IEC_61690_P1_E1
sto:IEC_61690_P1_E1 rdf:type owl:NamedIndividual ,
                             sto:Standard ;
                    dcterms:creator sto:irlan ;
                    sto:hasAvailableLanguage lang:eng ,
                                             lang:fra ;
                    sto:hasFileSize sto:FileSizeIEC_61690_P1 ;
                    sto:hasICS sto:ICS_35_240_50 ;
                    sto:hasPublisher sto:IEC ;
                    sto:hasTechnicalCommittee sto:TC_91 ;
                    sto:isPartOf sto:IEC_61690;
                    sto:hasEdition "1.0"^^xsd:float ;
                    sto:hasPublicationDate "2000-01-31"^^xsd:date ;
                    sto:hasStabilityDate "2018"^^xsd:gYear ;
                    dcterms:title "Electronic design interchange format (EDIF) - Part 1: Version 3 0 0. (This publication is available in electronic HTML format only)"@en ;
                    rdfs:comment "IEC 61690-1:2000 defines the syntax and semantics for EDIF Version 3 0 0. EDIF Version 3 0 0 addresses EDIF Level 0 and Level 1. EDIF Version 3 0 0 completely addresses the Connectivity and Schematic views, including at Level 1 the ability to represent frames. It includes capabilities formerly found in the Document and Graphics views. A series of releases is planned in the near future to address those views not completely addressed in this version."@en ;
                    rdfs:label "IEC 61690-1:2000"@en ;
                    sto:hasOfficialResource <https://webstore.iec.ch/publication/5723> .


###  https://w3id.org/i40/sto#IEC_61690_P2_E1
sto:IEC_61690_P2_E1 rdf:type owl:NamedIndividual ,
                             sto:Standard ;
                    dcterms:creator sto:irlan ;
                    sto:hasAvailableLanguage lang:eng ,
                                             lang:fra ;
                    sto:hasFileSize sto:FileSizeIEC_61690_P2 ;
                    sto:hasICS sto:ICS_35_240_50 ;
                    sto:hasPublisher sto:IEC ;
                    sto:hasTechnicalCommittee sto:TC_91 ;
                    sto:relatedTo sto:IEC_61690_P1_E1 ;
                    sto:isPartOf sto:IEC_61690;
                    sto:hasEdition "1.0"^^xsd:float ;
                    sto:hasPublicationDate "2000-01-31"^^xsd:date ;
                    sto:hasStabilityDate "2018"^^xsd:gYear ;
                    dcterms:title "Electronic design interchange format (EDIF) - Part 2: Version 4 0 0. (This publication is available in electronic HTML format only)"@en ;
                    rdfs:comment "IEC 61690-2:2000 defines the syntax and semantics for EDIF Version 4 0 0. EDIF Version 4 0 0 addresses EDIF Level 0 and Level 1. EDIF Version 3 0 0 provides support for Connectivity and Schematics; EDIF Version 4 0 0 offers additional capability by providing support for the representation of Printed Circuit Boards (PCBs) and Multi-chip Modules (MCMs) including technology rules and assembly drawings."@en ;
                    rdfs:label "IEC 61690-2:2000"@en ;
                    sto:hasOfficialResource <https://webstore.iec.ch/publication/5724> .

sto:IEC_61691 rdf:type owl:NamedIndividual ,
                             sto:Standard ;
                    sto:hasPublisher sto:IEC ;
                    dcterms:title "Behavioural languages "@en ;
                    rdfs:comment "Revises and enhances the VHDL language reference manual (LRM) by including a standard C language interface specification. The VHDL language was defined for use in the design and documentation of electronics systems."@en ;
                    rdfs:label "IEC 61691"@en  .

###  https://w3id.org/i40/sto#IEC_61691_P6_E1
sto:IEC_61691_P6_E1 rdf:type owl:NamedIndividual ,
                             sto:Standard ;
                    dcterms:creator sto:sebastian ;
                    sto:hasAvailableLanguage lang:eng ;
                    sto:hasFileSize sto:FileSizeIEC_61691_P6 ;
                    sto:hasICS sto:ICS_25_040_01 ,
                               sto:ICS_35_060 ;
                    sto:hasPublisher sto:IEC ;
                    sto:hasTechnicalCommittee sto:TC_91 ;
                    sto:relatedTo sto:IEC_61690_P1_E1 ;
                    sto:isPartOf sto:IEC_61691;
                    sto:hasEdition "1.0"^^xsd:float ;
                    sto:hasPages "332"^^xsd:int ;
                    sto:hasPublicationDate "2009-12-14"^^xsd:date ;
                    sto:hasStabilityDate "2018"^^xsd:gYear ;
                    dcterms:title "Behavioural languages - Part 6: VHDL Analog and Mixed-Signal Extensions"@en ;
                    rdfs:comment "IEC 61691-6:2009(E) Defines IEC 61691-6/IEEE Std 1076.1 language, a hardware description language for the description and the simulation of analog, digital, and mixed-signal systems. The language, also informally known as VHDLAMS, is built on the IEC 61691-1-1/IEEE 1076 (VHDL) language and extends it to provide capabilities of writing and simulating analog and mixed-signal models."@en ;
                    rdfs:label "IEC 61691-6:2009"@en ;
                    sto:hasOfficialResource <https://webstore.iec.ch/publication/5726> .


###  https://w3id.org/i40/sto#IEC_61784
sto:IEC_61784 rdf:type owl:NamedIndividual ,
                       sto:Standard ;
              dcterms:creator sto:irlan ;
              sto:hasClassification sto:RamiCommunicationlayer ,
                                    sto:RamiControlDevice ,
                                    sto:RamiFieldDevice ;
              sto:hasPublisher sto:IEC ;
              sto:relatedTo sto:IEC_29182_P1 ,
                            sto:IEC_61158 ,
                            sto:IEC_61784 ,
                            sto:OMG_DDS ;
              sto:hasMotivation "Information description and communication mapping for fieldbus profiles"@en ;
              sto:hasPublicationDate "2014-08-19"^^xsd:date ;
              sto:hasTag "IEC Fieldbus (Profibus)"@en ;
              dcterms:license sto:PrivateLicenseDocument ;
              rdfs:comment "Industrial communication networks - Profiles - Ethernet-real-time-enabled"@en ;
              rdfs:label "IEC 61784"@en ;
              sto:hasDBpediaResource <http://dbpedia.org/page/Profibus> ;
              sto:hasOfficialResource <https://webstore.iec.ch/publication/5878> .


###  https://w3id.org/i40/sto#IEC_61804
sto:IEC_61804 rdf:type owl:NamedIndividual ,
                       sto:Standard ;
              dcterms:creator sto:irlan ;
              sto:hasClassification sto:AsConfiguration ,
                                    sto:RamiControlDevice ,
                                    sto:RamiFieldDevice ;
              sto:hasPublisher sto:IEC ;
              sto:relatedTo sto:DIN_SPEC_16592 ,
                            sto:IEC_61131 ,
                            sto:IEC_61360 ,
                            sto:IEC_61499 ,
                            sto:IEC_61804 ,
                            sto:IEC_61850 ,
                            sto:IEC_61987_X ,
                            sto:IEC_62424 ,
                            sto:IEC_62453 ,
                            sto:IEC_62541 ,
                            sto:IEC_62714 ,
                            sto:ISO_13584 ,
                            sto:ISO_14306 ,
                            sto:ISO_15746 ,
                            sto:ISO_15926 ,
                            sto:ISO_18629 ,
                            sto:ISO_18828-2 ,
                            sto:ISO_20922 ,
                            sto:ISO_22400 ,
                            sto:ISO_29002 ,
                            sto:ISO_ASTM_52915 ,
                            sto:ISO_PAS_17506 ,
                            sto:MathML ,
                            sto:SysML ,
                            sto:eClass ;
              sto:hasTag "EDDL"@en ;
              rdfs:comment "Function blocks (FB) for process control - Overview of system aspects "@en ;
              rdfs:label "IEC 61804"@en ;
              sto:hasDBpediaResource <http://dbpedia.org/resource/Device_Description_Language> ;
              sto:hasOfficialResource <https://webstore.iec.ch/publication/5953> ;
              sto:hasWikipediaArticle <https://en.wikipedia.org/wiki/Device_Description_Language> .


###  https://w3id.org/i40/sto#IEC_61804_P3
sto:IEC_61804_P3 rdf:type owl:NamedIndividual ,
                          sto:Standard ;
                 dcterms:creator sto:irlan ;
                 sto:hasAvailableLanguage lang:eng ,
                                          lang:fra ;
                 sto:hasFileSize sto:FileSizeIEC_61804_P3 ;
                 sto:hasICS sto:ICS_25_040_40 ,
                            sto:ICS_35_240_50 ;
                 sto:hasPublisher sto:IEC ;
                 sto:hasTechnicalCommittee sto:TC_65 ;
                 sto_iot:frames sto:ThingDescription ;
                 sto:isPartOf sto:IEC_61804;
                 sto:hasEdition "3.0"^^xsd:float ;
                 sto:hasPages "694"^^xsd:int ;
                 sto:hasPublicationDate "2015-06-09"^^xsd:date ;
                 sto:hasStabilityDate "2019"^^xsd:gYear ;
                 sto:hasTag "IEC 61804-3:2015"@en ;
                 dcterms:title "Function Blocks (FB) for process control and Electronic Device Description Language (EDDL) - Part 3: EDDL syntax and semantics"@en ;
                 rdfs:comment "IEC 61804-3:2015 specifies the Electronic Device Description Language (EDDL) technology, which enables the integration of real product details using the tools of the engineering life cycle. It specifies EDDL as a generic language for describing the properties of automation system components. This third edition cancels and replaces the second edition published in 2010. This edition constitutes a technical revision. This edition includes the following significant technical changes with respect to the previous edition: Builtins and their profiles removed and relocated into IEC 61804-5. The following extensions are integrated in the EDDL specification to meet FDI requirements: - new contructs BLOB, PLUGIN; - component construct for communication server requirements (additional attributes); - extension of the class attribute; - new attributes PRIVATE, VISIBILITY, WRITE_MODE"@en ;
                 rdfs:label "IEC 61804-3:2015"@en ;
                 sto:hasOfficialResource <https://webstore.iec.ch/publication/22636> .


###  https://w3id.org/i40/sto#IEC_61804_P4
sto:IEC_61804_P4 rdf:type owl:NamedIndividual ,
                          sto:Standard ;
                 dcterms:creator sto:irlan ;
                 sto:hasAvailableLanguage lang:eng ,
                                          lang:fra ;
                 sto:hasFileSize sto:FileSizeIEC_61804_P4 ;
                 sto:hasICS sto:ICS_25_040_40 ,
                            sto:ICS_35_240_50 ;
                 sto:hasPublisher sto:IEC ;
                 sto:hasTechnicalCommittee sto:TC_65 ;
                 sto_iot:frames sto:ThingDescription ;
                 sto:isPartOf sto:IEC_61804;
                 sto:hasEdition "1.0"^^xsd:float ;
                 sto:hasPages "253"^^xsd:int ;
                 sto:hasPublicationDate "2015-10-07"^^xsd:date ;
                 sto:hasStabilityDate "2019"^^xsd:gYear ;
                 sto:hasTag "IEC 61804-4:2015"@en ;
                 dcterms:title "Function blocks (FB) for process control and electronic device description language (EDDL) - Part 4: EDD interpretation"@en ;
                 rdfs:comment "IEC 61804-4:2015 specifies EDD interpretation for EDD applications and EDDs to support EDD interoperability. This document is intended to ensure that field device developers use the EDDL constructs consistently and that the EDD applications have the same interpretations of the EDD. It supplements the EDDL specification to promote EDDL application interoperability and improve EDD portability between EDDL applications. This first edition cancels and replaces IEC TR 61804-4 published in 2006. This edition constitutes a technical revision. This edition includes the following significant technical changes with respect to the previous edition: - New paragraph: EDDL data description; - EDDL METHOD programming and usage of builtins; - Edit session; - Offline and online configuration; - EDDL communication description and Enhancements in paragraph EDDL user interface descriptions."@en ;
                 rdfs:label "IEC 61804-4:2015"@en ;
                 sto:hasOfficialResource <https://webstore.iec.ch/publication/23481> .


###  https://w3id.org/i40/sto#IEC_61804_P5
sto:IEC_61804_P5 rdf:type owl:NamedIndividual ,
                          sto:Standard ;
                 dcterms:creator sto:irlan ;
                 sto:hasAvailableLanguage lang:eng ,
                                          lang:fra ;
                 sto:hasFileSize sto:FileSizeIEC_61804_P5 ;
                 sto:hasICS sto:ICS_25_040_40 ,
                            sto:ICS_35_240_50 ;
                 sto:hasPublisher sto:IEC ;
                 sto:hasTechnicalCommittee sto:TC_65 ;
                 sto_iot:frames sto:ThingDescription ;
                 sto:isPartOf sto:IEC_61804;
                 sto:hasEdition "1.0"^^xsd:float ;
                 sto:hasPages "472"^^xsd:int ;
                 sto:hasPublicationDate "2015-06-09"^^xsd:date ;
                 sto:hasStabilityDate "2019"^^xsd:gYear ;
                 sto:hasTag "IEC 61804-5:2015 "@en ;
                 dcterms:title "Function blocks (FB) for process control and electronic device description language (EDDL) - Part 5: EDDL Builtin library"@en ;
                 rdfs:comment "IEC 61804-5:2015 specifies the EDDL Builtin library and provides the profiles of the various fieldbuses."@en ;
                 rdfs:label "IEC 61804-5:2015 "@en ;
                 sto:hasOfficialResource <https://webstore.iec.ch/publication/22637> .


###  https://w3id.org/i40/sto#IEC_61804_P6
sto:IEC_61804_P6 rdf:type owl:NamedIndividual ,
                          sto:TechnicalReport ;
                 dcterms:creator sto:irlan ;
                 sto:hasAvailableLanguage lang:eng ,
                                          lang:fra ;
                 sto:hasFileSize sto:FileSizeIEC_61804_P6 ;
                 sto:hasICS sto:ICS_25_040_40 ,
                            sto:ICS_35_240_50 ;
                 sto:hasPublisher sto:IEC ;
                 sto:hasTechnicalCommittee sto:TC_65 ;
                 sto_iot:frames sto:ThingDescription ;
                 sto:isPartOf sto:IEC_61804;
                 sto:hasEdition "1.0"^^xsd:float ;
                 sto:hasPages "15"^^xsd:int ;
                 sto:hasPublicationDate "2012-04-04"^^xsd:date ;
                 sto:hasStabilityDate "2022"^^xsd:gYear ;
                 sto:hasTag "IEC 61804-6:2012  "@en ;
                 dcterms:title "Function blocks (FB) for process control - Electronic device description language (EDDL) - Part 6: Meeting the requirements for integrating fieldbus devices in engineering tools for field devices"@en ;
                 rdfs:comment "IEC/TR 61804-6:2012(E) provides an evaluation and assessment of electronic device description language (EDDL) technology. It provides guidance to device and system manufacturers for how EDDL technology can help them meet user requirements. It provides guidance to system integrators, as well as instrumentation and maintenance practitioners at end-user companies, on how EDDL technology can help them integrate systems and incorporate device management in their work processes. It gives examples of requirements from the NAMUR NE 105 recommendation. It's intent is to illustrate how EDDL technology and products based on EDDL technology meet these requirements."@en ;
                 rdfs:label "IEC 61804-6:2012 "@en ;
                 sto:hasOfficialResource <https://webstore.iec.ch/publication/59577> .

sto:IEC_61810 rdf:type owl:NamedIndividual ,
                             sto:Standard ;
                    sto:hasPublisher sto:IEC ;
                    dcterms:title "Electromechanical elementary relays"@en ;
                    rdfs:comment "Electromechanical elementary relays."@en ;
                    rdfs:label "IEC 61810"@en  .

###  https://w3id.org/i40/sto#IEC_61810_P2_E3
sto:IEC_61810_P2_E3 rdf:type owl:NamedIndividual ,
                             sto:Standard ;
                    dcterms:creator sto:irlan ;
                    sto:hasAvailableLanguage lang:eng ,
                                             lang:fra ;
                    sto:hasFileSize sto:FileSizeIEC_61810_P2 ;
                    sto:hasICS sto:ICS_29_120_70 ;
                    sto:hasPublisher sto:IEC ;
                    sto:hasTechnicalCommittee sto:TC_94 ;
                    sto:hasPages "86"^^xsd:int ;
                    sto:hasStabilityDate "2020"^^xsd:gYear ;
                    sto:hasTag "IEC 61810-2:2017"@en ;
                    dcterms:title "Electromechanical elementary relays - Part 2: Reliability"@en ;
                    rdfs:comment """IEC 61810-2:2017 covers test conditions and provisions for the evaluation of endurance tests using appropriate statistical methods to obtain reliability characteristics for relays.
This document applies to electromechanical elementary relays considered as non-repaired items (i.e. items which are not repaired after failure).
This document does not cover procedures for electromechanical elementary relays where enhanced requirements for the verification of reliability apply.
This edition includes the following significant technical changes with respect to the previous edition:
- not only graphical but also numerical methods are added;
- reduction of number of samples in specified cases;
- new subclauses of confidence intervals are added;
- the WeiBayes approach is added to facilitate compliance tests (routine test) with lower effort;
- annexes have been restructured into an Annex A for data analysis (normative) and Annex B (informative) where various examples of the data analysis are given;
- the former Annex C has been incorporated into the modified Annex B;
- a new Annex C replaces the old Annex D."""@en ,
                                 "IEC 61810-2:2017 covers test conditions and provisions for the evaluation of endurance tests using appropriate statistical methods to obtain reliability characteristics for relays.nThis document applies to electromechanical elementary relays considered as non-repaired items (i.e. items which are not repaired after failure).nThis document does not cover procedures for electromechanical elementary relays where enhanced requirements for the verification of reliability apply.nThis edition includes the following significant technical changes with respect to the previous edition:n- not only graphical but also numerical methods are added;n- reduction of number of samples in specified cases;n- new subclauses of confidence intervals are added;n- the WeiBayes approach is added to facilitate compliance tests (routine test) with lower effort;n- annexes have been restructured into an Annex A for data analysis (normative) and Annex B (informative) where various examples of the data analysis are given;n- the former Annex C has been incorporated into the modified Annex B;n- a new Annex C replaces the old Annex D."@en ;
                    rdfs:label "IEC 61810-2:2017"@en ;
                    sto:hasOfficialResource <https://webstore.iec.ch/publication/33869> .


###  https://w3id.org/i40/sto#IEC_61810_P7_E2
sto:IEC_61810_P7_E2 rdf:type owl:NamedIndividual ,
                             sto:Standard ;
                    dcterms:creator sto:irlan ;
                    sto:hasAvailableLanguage lang:eng ,
                                             lang:fra ,
                                             lang:spa ;
                    sto:hasFileSize sto:FileSizeIEC_61810_P7 ;
                    sto:hasICS sto:ICS_29_120_70 ;
                    sto:hasPublisher sto:IEC ;
                    sto:hasTechnicalCommittee sto:TC_94 ;
                    sto:isPartOf sto:IEC_61810;
                    sto:hasEdition "2.0"^^xsd:float ;
                    sto:hasPages "176"^^xsd:int ;
                    sto:hasPublicationDate "2006-03-14"^^xsd:date ;
                    sto:hasStabilityDate "2018"^^xsd:gYear ;
                    sto:hasTag "IEC 61810-7:2006"@en ;
                    dcterms:title "Electromechanical elementary relays - Part 7: Test and measurement procedures"@en ;
                    rdfs:comment "IEC 61810-7:2006 Lays down the test and measurement procedures for electromechanical elementary relays. Covers basic considerations which are common to all types of electromechanical elementary relays. Supplementary requirements may be necessitated by specific designs or application."@en ;
                    rdfs:label "IEC 61810-7:2006"@en ;
                    sto:hasOfficialResource <https://webstore.iec.ch/publication/5963> .


###  https://w3id.org/i40/sto#IEC_61850
sto:IEC_61850 rdf:type owl:NamedIndividual ,
                       sto:Standard ;
              sto:hasPublisher sto:IEC ;
              rdfs:comment "IEC 61850 is a standard for vendor-agnostic engineering of the configuration of Intelligent Electronic Devices for electrical substation automation systems to be able to communicate with each other.."@en ;
              rdfs:label "IEC 61850"@en ;
              sto:hasDBpediaResource <http://dbpedia.org/page/IEC_61850> ;
              sto:hasOfficialResource <https://webstore.iec.ch/publication/4550> ;
              sto:hasWikipediaArticle <https://en.wikipedia.org/wiki/IEC_61850> .





###  https://w3id.org/i40/sto#IEC_61850_P10_E1
sto:IEC_61850_P10_E1 rdf:type owl:NamedIndividual ,
                              sto:Standard ;
                     sto:hasAvailableLanguage lang:eng ;
                     sto:hasFileSize sto:FileSizeIEC_61850_P10_E1 ;
                     sto:hasICS sto:ICS_33_200 ;
                     sto:hasPublisher sto:IEC ;
                     sto:hasTechnicalCommittee sto:TC_57 ;
                     sto:relatedTo sto:IEC_61850 ;
                     sto:isPartOf sto:IEC_61850;
                     sto:hasEdition "1.0"^^xsd:float ;
                     sto:hasPages "43"^^xsd:int ;
                     sto:hasPublicationDate "2005-05-30"^^xsd:date ;
                     sto:hasTag "IEC 61850-10:2005"@en ;
                     dcterms:title "Communication networks and systems in substations - Part 10: Conformance testing"@en ;
                     rdfs:comment "Specifies standard techniques for testing of conformance of implementations, as well as specific measurement techniques to be applied when declaring performance parameters. The use of these techniques will enhance the ability of the system integrator to integrate IEDs easily, operate IEDs correctly, and support the applications as intended.This publication is of core relevance for Smart Grid.."@en ;
                     rdfs:label "IEC 61850-10:2005"@en ;
                     sto:hasDBpediaResource <http://dbpedia.org/page/IEC_61850> ;
                     sto:hasOfficialResource <https://webstore.iec.ch/publication/20072> ;
                     sto:hasStatus "Withdrawn"@en ;
                     sto:hasWikipediaArticle <https://en.wikipedia.org/wiki/IEC_61850> .


###  https://w3id.org/i40/sto#IEC_61850_P10_E2
sto:IEC_61850_P10_E2 rdf:type owl:NamedIndividual ,
                              sto:Standard ;
                     sto:hasAvailableLanguage lang:eng ,
                                              lang:fra ;
                     sto:hasFileSize sto:FileSizeIEC_61850_P10_E2 ;
                     sto:hasICS sto:ICS_33_200 ;
                     sto:hasPublisher sto:IEC ;
                     sto:hasTechnicalCommittee sto:TC_57 ;
                     sto:relatedTo sto:IEC_61850 ;
                     sto:isPartOf sto:IEC_61850;
                     sto:hasEdition "2.0"^^xsd:float ;
                     sto:hasPages "170"^^xsd:int ;
                     sto:hasPublicationDate "2012-12-14"^^xsd:date ;
                     sto:hasStabilityDate "2020"^^xsd:gYear ;
                     sto:hasTag "IEC 61850-10:2012 "@en ;
                     dcterms:title "Communication networks and systems for power utility automation - Part 10: Conformance testing"@en ;
                     rdfs:comment "IEC 61850-10:2012 specifies standard techniques for testing of conformance of client, server and sampled value devices and engineering tools, as well as specific measurement techniques to be applied when declaring performance parameters. The use of these techniques will enhance the ability of the system integrator to integrate IEDs easily, operate IEDs correctly, and support the applications as intended. The major technical changes with regard to the previous edition are as follows:- updates to server device conformance test procedures;- additions of certain test procedures (client device conformance, sampled values device conformance, (engineering) tool related conformance, GOOSE performance).."@en ;
                     rdfs:label "IEC 61850-10:2012"@en ;
                     prov:wasRevisionOf sto:IEC_61850_P10_E1 ;
                     sto:hasDBpediaResource <http://dbpedia.org/page/IEC_61850> ;
                     sto:hasOfficialResource <https://webstore.iec.ch/publication/6008> ;
                     sto:hasStatus "Valid"@en ;
                     sto:hasWikipediaArticle <https://en.wikipedia.org/wiki/IEC_61850> .


###  https://w3id.org/i40/sto#IEC_61850_P4_E1
sto:IEC_61850_P4_E1 rdf:type owl:NamedIndividual ,
                             sto:Standard ;
                    sto:hasAvailableLanguage lang:eng ,
                                             lang:fra ;
                    sto:hasFileSize sto:FileSizeIEC_61850_P4_E1 ;
                    sto:hasICS sto:ICS_33_200 ;
                    sto:hasPublisher sto:IEC ;
                    sto:hasTechnicalCommittee sto:TC_57 ;
                    sto:relatedTo sto:IEC_61850 ;
                    sto:isPartOf sto:IEC_61850;
                    sto:hasEdition "1.0"^^xsd:float ;
                    sto:hasPages "59"^^xsd:int ;
                    sto:hasPublicationDate "2002-01-17"^^xsd:date ;
                    sto:hasTag "IEC 61850-4:2002"@en ;
                    dcterms:title "Communication networks and systems for power utility automation - Part 4: System and project management"@en ;
                    rdfs:comment "Describes the requirements of the system and project management process and of special supporting tools for engineering and testing.This publication is of core relevance for Smart Grid."@en ;
                    rdfs:label "IEC 61850-4:2002"@en ;
                    sto:hasOfficialResource <https://webstore.iec.ch/publication/20074> ;
                    sto:hasStatus "Withdrawn"@en .


###  https://w3id.org/i40/sto#IEC_61850_P4_E2
sto:IEC_61850_P4_E2 rdf:type owl:NamedIndividual ,
                             sto:Standard ;
                    sto:hasAvailableLanguage lang:eng ,
                                             lang:fra ;
                    sto:hasFileSize sto:FileSizeIEC_61850_P4_E2 ;
                    sto:hasICS sto:ICS_33_200 ;
                    sto:hasPublisher sto:IEC ;
                    sto:hasTechnicalCommittee sto:TC_57 ;
                    sto:relatedTo sto:IEC_61850 ;
                    sto:isPartOf sto:IEC_61850;
                    sto:hasEdition "2.0"^^xsd:float ;
                    sto:hasPages "74"^^xsd:int ;
                    sto:hasPublicationDate "2011-04-11"^^xsd:date ;
                    sto:hasStabilityDate "2020"^^xsd:gYear ;
                    sto:hasTag "IEC 61850-4:2011"@en ;
                    dcterms:title "Communication networks and systems for power utility automation - Part 4: System and project management"@en ;
                    rdfs:comment "IEC 61850-4:2011 applies to projects associated with process near automation systems of power utilities (UAS, utility automation system), like e.g. substation automation systems (SAS). It defines the system and project management for UAS systems with communication between intelligent electronic devices (IEDs) in the substation respective plant and the related system requirements. This second edition constitutes a technical revision to align the document more closely with the other parts of the IEC 61850 series, in addition to enlarging the scope from substation automation systems to all utility automation systems.This publication is of core relevance for Smart Grid."@en ;
                    rdfs:label "IEC 61850-4:2011"@en ;
                    prov:wasRevisionOf sto:IEC_61850_P4_E1 ;
                    sto:hasDBpediaResource <http://dbpedia.org/page/IEC_61850> ;
                    sto:hasOfficialResource <https://webstore.iec.ch/publication/6011> ;
                    sto:hasStatus "Valid"@en ;
                    sto:hasWikipediaArticle <https://en.wikipedia.org/wiki/IEC_61850> .


###  https://w3id.org/i40/sto#IEC_61850_P7_S1_E1
sto:IEC_61850_P7_S1_E1 rdf:type owl:NamedIndividual ,
                                sto:Standard ;
                       sto:hasAvailableLanguage lang:eng ;
                       sto:hasFileSize sto:FileSizeIEC_61850_P7_S1_E1 ;
                       sto:hasICS sto:ICS_33_200 ;
                       sto:hasPublisher sto:IEC ;
                       sto:hasTechnicalCommittee sto:TC_57 ;
                       sto:relatedTo sto:IEC_61850 ;
                     sto:isPartOf sto:IEC_61850;
                       sto:hasEdition "1.0"^^xsd:float ;
                       sto:hasPages "110"^^xsd:int ;
                       sto:hasPublicationDate "2003-07-23"^^xsd:date ;
                       sto:hasTag "IEC 61850-7-1:2003"@en ;
                       dcterms:title "Communication networks and systems for power utility automation - Part 7-1: Basic communication structure - Principles and models"@en ;
                       rdfs:comment "Provides an overview of the architecture for communication and interactions between substation devices such as protection devices, breakers, transformers, substation hosts, etc. Uses simple examples of functions to describe the concepts and methods applied in the IEC 61850 series. Also describes the relationships between other parts of the IEC 61850 series and defines how inter-operability is reached.This publication is of core relevance for Smart Grid."@en ;
                       rdfs:label "IEC 61850-7-1:2003"@en ;
                       sto:hasDBpediaResource <http://dbpedia.org/page/IEC_61850> ;
                       sto:hasOfficialResource <https://webstore.iec.ch/publication/20077> ;
                       sto:hasStatus "Withdrawn"@en ;
                       sto:hasWikipediaArticle <https://en.wikipedia.org/wiki/IEC_61850> .


###  https://w3id.org/i40/sto#IEC_61850_P7_S1_E2
sto:IEC_61850_P7_S1_E2 rdf:type owl:NamedIndividual ,
                                sto:Standard ;
                       sto:hasAvailableLanguage lang:eng ,
                                                lang:fra ;
                       sto:hasFileSize sto:FileSizeIEC_61850_P7_S1_E2 ;
                       sto:hasICS sto:ICS_33_200 ;
                       sto:hasPublisher sto:IEC ;
                       sto:hasTechnicalCommittee sto:TC_57 ;
                       sto:relatedTo sto:IEC_61850 ;
                       sto:isPartOf sto:IEC_61850;
                       sto:hasEdition "2.0"^^xsd:float ;
                       sto:hasPages "289"^^xsd:int ;
                       sto:hasPublicationDate "2011-07-15"^^xsd:date ;
                       sto:hasStabilityDate "2020"^^xsd:gYear ;
                       sto:hasTag "IEC 61850-7-1:2011"@en ;
                       dcterms:title "Communication networks and systems for power utility automation - Part 7-1: Basic communication structure - Principles and models"@en ;
                       rdfs:comment "IEC 61850-7-1:2011 introduces the modelling methods, communication principles, and information models that are used in the various parts of the IEC 61850-7 series. The purpose is to provide - from a conceptual point of view - assistance to understand the basic modelling concepts and description methods for:- substation-specific information models for power utility automation systems,- device functions used for power utility automation purposes, and- communication systems to provide interoperability within power utility facilities. Compared to the first edition, this second edition introduces:- the model for statistical and historical statistical data,- the concepts of proxies, gateways, LD hierarchy and LN inputs,- the model for time synchronisation,- the concepts behind different testing facilities,- the extended logging function. It also clarifies certain items."@en ;
                       rdfs:label "IEC 61850-7-1:2011"@en ;
                       prov:wasRevisionOf sto:IEC_61850_P7_S1_E1 ;
                       sto:hasDBpediaResource <http://dbpedia.org/page/IEC_61850> ;
                       sto:hasOfficialResource <https://webstore.iec.ch/publication/6011> ;
                       sto:hasStatus "Valid"@en ;
                       sto:hasWikipediaArticle <https://en.wikipedia.org/wiki/IEC_61850> .


###  https://w3id.org/i40/sto#IEC_61850_P7_S2_E1
sto:IEC_61850_P7_S2_E1 rdf:type owl:NamedIndividual ,
                                sto:Standard ;
                       sto:hasAvailableLanguage lang:eng ;
                       sto:hasFileSize sto:FileSizeIEC_61850_P7_S2_E1 ;
                       sto:hasICS sto:ICS_33_200 ;
                       sto:hasPublisher sto:IEC ;
                       sto:hasTechnicalCommittee sto:TC_57 ;
                       sto:relatedTo sto:IEC_61850 ;
                       sto:isPartOf sto:IEC_61850;
                       sto:hasEdition "1.0"^^xsd:float ;
                       sto:hasPages "171"^^xsd:int ;
                       sto:hasPublicationDate "2003-05-12"^^xsd:date ;
                       sto:hasTag "IEC 61850-7-2:2003"@en ;
                       dcterms:title "Communication networks and systems in substations - Part 7-2: Basic communication structure for substation and feeder equipment - Abstract communication service interface (ACSI)"@en ;
                       rdfs:comment "Applies to the ACSI communication in substations and feeder applications. The ACSI provides the abstract interface describing communications between a client and a remote server; and the abstract interface for fast and reliable system-wide event distribution between an application in one device and many remote applications in different devices and for transmission of sampled measured values."@en ;
                       rdfs:label "IEC 61850-7-2:2003"@en ;
                       sto:hasDBpediaResource <http://dbpedia.org/page/IEC_61850> ;
                       sto:hasOfficialResource <https://webstore.iec.ch/publication/20078> ;
                       sto:hasStatus "Withdrawn"@en ;
                       sto:hasWikipediaArticle <https://en.wikipedia.org/wiki/IEC_61850> .


###  https://w3id.org/i40/sto#IEC_61850_P7_S2_E2
sto:IEC_61850_P7_S2_E2 rdf:type owl:NamedIndividual ,
                                sto:Standard ;
                       sto:hasAvailableLanguage lang:eng ;
                       sto:hasFileSize sto:FileSizeIEC_61850_P7_S2_E2 ;
                       sto:hasICS sto:ICS_33_200 ;
                       sto:hasPublisher sto:IEC ;
                       sto:hasTechnicalCommittee sto:TC_57 ;
                       sto:relatedTo sto:IEC_61850 ;
                       sto:isPartOf sto:IEC_61850;
                       sto:hasEdition "2.0"^^xsd:float ;
                       sto:hasPages "213"^^xsd:int ;
                       sto:hasPublicationDate "2010-08-24"^^xsd:date ;
                       sto:hasStabilityDate "2020"^^xsd:gYear ;
                       sto:hasTag "IEC 61850-7-2:2010 "@en ;
                       dcterms:title "Communication networks and systems for power utility automation - Part 7-2: Basic information and communication structure - Abstract communication service interface (ACSI)"@en ;
                       rdfs:comment "IEC 61850-7-2:2010(E) applies to the ACSI communication for utility automation. The ACSI provides the following abstract communication service interfaces:- abstract interface describing communications between a client and a remote server;- and abstract interface for fast and reliable system-wide event distribution between an application in one device and many remote applications in different devices (publisher/sub-scriber) and for transmission of sampled measured values (publisher/subscriber).This publication is of core relevance for Smart Grid"@en ;
                       rdfs:label "IEC 61850-7-2:2010"@en ;
                       prov:wasRevisionOf sto:IEC_61850_P7_S2_E1 ;
                       sto:hasDBpediaResource <http://dbpedia.org/page/IEC_61850> ;
                       sto:hasOfficialResource <https://webstore.iec.ch/publication/6015> ;
                       sto:hasStatus "Valid"@en ;
                       sto:hasWikipediaArticle <https://en.wikipedia.org/wiki/IEC_61850> .


###  https://w3id.org/i40/sto#IEC_61850_P7_S3_E1
sto:IEC_61850_P7_S3_E1 rdf:type owl:NamedIndividual ,
                                sto:Standard ;
                       sto:hasAvailableLanguage lang:eng ;
                       sto:hasFileSize sto:FileSizeIEC_61850_P7_S3_E1 ;
                       sto:hasICS sto:ICS_33_200 ;
                       sto:hasPublisher sto:IEC ;
                       sto:hasTechnicalCommittee sto:TC_57 ;
                       sto:relatedTo sto:IEC_61850 ;
                       sto:isPartOf sto:IEC_61850;
                       sto:hasEdition "1.0"^^xsd:float ;
                       sto:hasPages "64"^^xsd:int ;
                       sto:hasPublicationDate "2003-05-12"^^xsd:date ;
                       sto:hasTag "61850-7-3:2003"@en ;
                       dcterms:title "Communication networks and systems in substations - Part 7-3: Basic communication structure for substation and feeder equipment - Common data classes"@en ;
                       rdfs:comment "Specifies common attribute types and common data classes related to substation applications. Specifies particularly: common data classes for status information, for measured information, for controllable status information, for controllable analogue set point information, for status settings, for analogue settings and attribute types used in these common data classes. Is applicable to the description of device models and functions of substations and feeder equipment. This publication is of core relevance for Smart Grid."@en ;
                       rdfs:label "IEC 61850-7-3:2003"@en ;
                       sto:hasDBpediaResource <http://dbpedia.org/page/IEC_61850> ;
                       sto:hasOfficialResource <https://webstore.iec.ch/publication/20079> ;
                       sto:hasStatus "Withdrawn"@en ;
                       sto:hasWikipediaArticle <https://en.wikipedia.org/wiki/IEC_61850> .


###  https://w3id.org/i40/sto#IEC_61850_P7_S3_E2
sto:IEC_61850_P7_S3_E2 rdf:type owl:NamedIndividual ,
                                sto:Standard ;
                       sto:hasAvailableLanguage lang:eng ,
                                                lang:fra ;
                       sto:hasFileSize sto:FileSizeIEC_61850_P7_S3_E2 ;
                       sto:hasICS sto:ICS_33_200 ;
                       sto:hasPublisher sto:IEC ;
                       sto:hasTechnicalCommittee sto:TC_57 ;
                       sto:relatedTo sto:IEC_61850 ;
                       sto:isPartOf sto:IEC_61850;
                       sto:hasEdition "2.0"^^xsd:float ;
                       sto:hasPages "182"^^xsd:int ;
                       sto:hasPublicationDate "2010-12-16"^^xsd:date ;
                       sto:hasStabilityDate "2020"^^xsd:gYear ;
                       sto:hasTag "IEC 61850-7-3:2010 "@en ;
                       dcterms:title "Communication networks and systems for power utility automation - Part 7-3: Basic communication structure - Common data classes"@en ;
                       rdfs:comment "IEC 61850-7-3:2010 is applicable to the description of device models and functions of substations and feeder equipment. It specifies constructed attribute classes and common data classes related to substation applications. In particular, it specifies common data classes for status information, common data classes for measured information, common data classes for control, common data classes for status settings, common data classes for analogue settings and attribute types used in these common data classes. This second edition defines new common data classes used for new standards defining object models for other domains based on IEC 61850 and for the representation of statistical and historical data. This publication is of core relevance for Smart Grid."@en ;
                       rdfs:label "IEC 61850-7-3:2010"@en ;
                       prov:wasRevisionOf sto:IEC_61850_P7_S3_E1 ;
                       sto:hasDBpediaResource <http://dbpedia.org/page/IEC_61850> ;
                       sto:hasOfficialResource <https://webstore.iec.ch/publication/6016> ;
                       sto:hasStatus "Valid"@en ;
                       sto:hasWikipediaArticle <https://en.wikipedia.org/wiki/IEC_61850> .


###  https://w3id.org/i40/sto#IEC_61850_P7_S420_E1
sto:IEC_61850_P7_S420_E1 rdf:type owl:NamedIndividual ,
                                  sto:Standard ;
                         sto:hasAvailableLanguage lang:eng ;
                         sto:hasFileSize sto:FileSizeIEC_61850_P7_S420_E1 ;
                         sto:hasICS sto:ICS_33_200 ;
                         sto:hasPublisher sto:IEC ;
                         sto:hasTechnicalCommittee sto:TC_57 ;
                         sto:isPartOf sto:IEC_61850;
                         sto:hasEdition "1.0"^^xsd:float ;
                         sto:hasPages "99"^^xsd:int ;
                         sto:hasPublicationDate "2009-03-10"^^xsd:date ;
                         sto:hasStabilityDate "2020"^^xsd:gYear ;
                         sto:hasTag " IEC 61850-7-420:2009 "@en ;
                         dcterms:title "Communication networks and systems for power utility automation - Part 7-420: Basic communication structure - Distributed energy resources logical nodes"@en ;
                         rdfs:comment "IEC 61850-7-420:2009(E) defines IEC 61850 information models to be used in the exchange of information with distributed energy resources (DER), which comprise dispersed generation devices and dispersed storage devices, including reciprocating engines, fuel cells, microturbines, photovoltaics, combined heat and power, and energy storage. Utilizes existing IEC 61850-7-4 logical nodes where possible, but also defines DER-specific logical nodes where needed."@en ;
                         rdfs:label " IEC 61850-7-420:2009"@en ;
                         sto:hasDBpediaResource <http://dbpedia.org/page/IEC_61850> ;
                         sto:hasOfficialResource <https://webstore.iec.ch/publication/6019> ;
                         sto:hasStatus "Valid"@en ;
                         sto:hasWikipediaArticle <https://en.wikipedia.org/wiki/IEC_61850> .


###  https://w3id.org/i40/sto#IEC_61850_P7_S4_E1
sto:IEC_61850_P7_S4_E1 rdf:type owl:NamedIndividual ,
                                sto:Standard ;
                       sto:hasAvailableLanguage lang:eng ;
                       sto:hasFileSize sto:FileSizeIEC_61850_P7_S4_E1 ;
                       sto:hasICS sto:ICS_33_200 ;
                       sto:hasPublisher sto:IEC ;
                       sto:relatedTo sto:IEC_61850 ;
                       sto:hasTechnicalCommittee sto:TC_57 ; 
                       sto:isPartOf sto:IEC_61850;
                       sto:hasEdition "1.0"^^xsd:float ;
                       sto:hasPages "104"^^xsd:int ;
                       sto:hasPublicationDate "2003-05-13"^^xsd:date ;
                       sto:hasTag "IEC 61850-7-4:2003"@en ;
                       dcterms:title "Communication networks and systems in substations - Part 7-4: Basic communication structure for substation and feeder equipment - Compatible logical node classes and data classes"@en ;
                       rdfs:comment "Specifies the information model of devices and functions related to substation applications. Specifies in particular the compatible logical node names and data names for communication between Intelligent Electronic Devices, which includes the relationship between Logical Nodes and Data.."@en ;
                       rdfs:label "IEC 61850-7-4:2003"@en ;
                       sto:hasDBpediaResource <http://dbpedia.org/page/IEC_61850> ;
                       sto:hasOfficialResource <https://webstore.iec.ch/publication/20080> ;
                       sto:hasStatus "Withdrawn"@en ;
                       sto:hasWikipediaArticle <https://en.wikipedia.org/wiki/IEC_61850> .


###  https://w3id.org/i40/sto#IEC_61850_P7_S4_E2
sto:IEC_61850_P7_S4_E2 rdf:type owl:NamedIndividual ,
                                sto:Standard ;
                       sto:hasAvailableLanguage lang:eng ,
                                                lang:fra ;
                        sto:hasFileSize sto:FileSizeIEC_61850_P7_S4_E2 ;
                       sto:hasICS sto:ICS_33_200 ;
                       sto:hasPublisher sto:IEC ;
                       sto:hasTechnicalCommittee sto:TC_57 ;
                       sto:relatedTo sto:IEC_61850 ;
                       sto:isPartOf sto:IEC_61850;
                       sto:hasEdition "2.0"^^xsd:float ;
                       sto:hasPages "421"^^xsd:int ;
                       sto:hasPublicationDate "2010-03-31"^^xsd:date ;
                       sto:hasStabilityDate "2020"^^xsd:gYear ;
                       sto:hasTag "IEC 61850-7-4:2010 "@en ;
                       dcterms:title "Communication networks and systems for power utility automation - Part 7-4: Basic communication structure - Compatible logical node classes and data object classes"@en ;
                       rdfs:comment "IEC 61850-7-4:2010 specifies the information model of devices and functions generally related to common use regarding applications in systems for power utility automation. It also contains the information model of devices and function-related applications in substations. In particular, it specifies the compatible logical node names and data object names for communication between intelligent electronic devices (IED). This includes the relationship between logical nodes and data objects. Major technical changes with regard to the previous edition are as follows:- corrections and clarifications according to technical issues raised by the users' community; extensions for new logical nodes for the power quality domain;- extensions for the model for statistical and historical statistical data;- extensions regarding IEC 61850-90-1;- extensions for new logical nodes for monitoring functions according to IEC 62271;- new logical nodes from IEC 61850-7-410 and IEC 61850-7-420 of general interest.This publication is of core relevance for Smart Grid."@en ;
                       rdfs:label "IEC 61850-7-4:2010"@en ;
                       prov:wasRevisionOf sto:IEC_61850_P7_S4_E1 ;
                       sto:hasDBpediaResource <http://dbpedia.org/page/IEC_61850> ;
                       sto:hasOfficialResource <https://webstore.iec.ch/publication/6017> ;
                       sto:hasStatus "Valid"@en ;
                       sto:hasWikipediaArticle <https://en.wikipedia.org/wiki/IEC_61850> .

sto:IEC_61850_P8_S1_E2 rdf:type owl:NamedIndividual ,
                          sto:Standard ;
                 dcterms:creator sto:priyanka;
                 sto:hasAvailableLanguage lang:eng ,
                                          lang:fra ;
                 sto:hasFileSize sto:FileSizeIEC_61850_P8_S1_E2 ;
                 sto:hasICS sto:ICS_33_200 ;
                 sto:hasPublisher sto:IEC ;
                 sto:hasTechnicalCommittee sto:TC_57 ;
                 sto:isPartOf sto:IEC_61850;
                 sto:hasEdition "2.0"^^xsd:float ;
                 sto:hasPages "386"^^xsd:int ;
                 sto:hasPublicationDate "2011-06-17"^^xsd:date ;
                 sto:hasStabilityDate "2020"^^xsd:gYear ;
                 sto:hasTag "IEC 61850-8-1:2011"@en ;
                 sto:hasStatus "Valid";
                 dcterms:title "Communication networks and systems for power utility automation - Part 7-4: Basic communication structure - Compatible logical node classes and data object classes"@en ;
                 rdfs:comment "IEC 61850-8-1:2011 specifies a method of exchanging time-critical and non-time-critical data through local-area networks by mapping ACSI to MMS and ISO/IEC 8802-3 frames. Defines a standardized method of using the ISO 9506 services to implement the exchange of data. For those ACSI services defined in IEC 61850-7-2 that are not mapped to MMS, this part defines additional protocols. It describes real utility devices with respect to their external visible data and behaviour using an object oriented approach. The objects are abstract in nature and may be used to a wide variety of applications. The use of this mapping goes far beyond the application in the utility communications. The main changes with respect to the previous edition are listed below: - the support of gigabit Ethernet, - the link layer redundancy, - the extension of the length of the object reference, - the extension of the reason for inclusion type for comprehensive logging, - the mapping of the tracking services, - a second mapping of the objectReference when used in the tracking services, or as linking, - the extension of the AdditionalCause enumeration, - the simulation of GOOSE telegram, - the so-called fixed-length encoded GOOSE, - the removal of the SCL Control Block."@en ;
                 rdfs:label "IEC 61850-8-1:2011"@en ;
                 sto:hasOfficialResource <https://webstore.iec.ch/publication/6021>;
                 sto:hasWikipediaArticle <https://en.wikipedia.org/wiki/IEC_61850> .


sto:IEC_61968 rdf:type owl:NamedIndividual ,
                             sto:Standard ;
                    sto:hasPublisher sto:IEC ;
                    dcterms:title "Application integration at electric utilities - System interfaces for distribution management "@en ;
                    rdfs:comment "IEC 61968 is a series of standards under development that will define standards for information exchanges between electrical distribution systems."@en ;
                    rdfs:label "IEC 61968"@en ;
                    sto:hasDBpediaResource <http://dbpedia.org/page/IEC_61968> ;
                    sto:hasWikipediaArticle <https://en.wikipedia.org/wiki/IEC_61968> .

###  https://w3id.org/i40/sto#IEC_61968_P3_E1
sto:IEC_61968_P3_E1 rdf:type owl:NamedIndividual ,
                             sto:Standard ;
                    sto:hasAvailableLanguage lang:eng ;
                    sto:hasFileSize sto:FileSizeIEC_61968_P3_E1 ;
                    sto:hasICS sto:ICS_33_200 ;
                    sto:hasPublisher sto:IEC ;
                    sto:hasTechnicalCommittee sto:TC_57 ;
                    sto:isPartOf sto:IEC_61968;
                    sto:hasEdition "1.0"^^xsd:float ;
                    sto:hasPages "36"^^xsd:int ;
                    sto:hasPublicationDate "2004-03-08"^^xsd:date ;
                    sto:hasTag "IEC 61968-3:2004"@en ;
                    dcterms:title "Application integration at electric utilities - System interfaces for distribution management - Part 3: Interface for network operations"@en ;
                    rdfs:comment "Specifies the information content of a set of message types that can be used to support many of the business functions related to network operations. Typical uses of the message types defined in this part include data acquisition by external systems, fault isolation, fault restoration, trouble management, maintenance of the plant, and the commissioning of the plant. This publication is of core relevance for Smart Grid."@en ;
                    rdfs:label "IEC 61968-3:2004"@en ;
                    sto:hasOfficialResource <https://webstore.iec.ch/publication/6202> ;
                    sto:hasStatus "Withdrawn"@en ;
                    sto:hasWikipediaArticle <https://en.wikipedia.org/wiki/IEC_61968> .

sto:IEEE_1815-2012 rdf:type owl:NamedIndividual ,
                            sto:Standard ; 
                            dcterms:creator sto:priyanka ;
                   sto:hasPublicationDate "2012-10-10"^^xsd:date ;
                    sto:hasPublisher sto:IEEE ;
                   rdfs:comment "IEEE Standard for Electric Power Systems Communications-Distributed Network Protocol (DNP3)"@en ;
                   rdfs:label "IEEE 1377-2012"@en ;
                   sto:hasTag "DNP3"@en;
                   sto:hasOfficialResource <https://standards.ieee.org/standard/1815-2012.html> .

###  https://w3id.org/i40/sto#IEC_61968_P3_E2
sto:IEC_61968_P3_E2 rdf:type owl:NamedIndividual ,
                             sto:Standard ;
                    sto:hasAvailableLanguage lang:eng ,
                                             lang:fra ;
                    sto:hasFileSize sto:FileSizeIEC_61968_P3_E2 ;
                    sto:hasICS sto:ICS_33_200 ;
                    sto:hasPublisher sto:IEC ;
                    sto:hasTechnicalCommittee sto:TC_57 ;
                    sto:relatedTo sto:IEC_61968_P3_E1 ;
                    sto:isPartOf sto:IEC_61968;
                    sto:hasEdition "2.0"^^xsd:float ;
                    sto:hasPages "322"^^xsd:int ;
                    sto:hasPublicationDate "2017-04-11"^^xsd:date ;
                    sto:hasStabilityDate "2019"^^xsd:gYear ;
                    sto:hasTag "IEC 61968-3:2017 "@en ;
                    dcterms:title "Application integration at electric utilities - System interfaces for distribution management - Part 3: Interface for network operations"@en ;
                    rdfs:comment "IEC 61968-3:2017 defines a Network Operations function which provides utilities the means to supervise main substation topology (breaker and switch state) and control equipment status. It also provides the means for handling network connectivity and loading conditions. Finally, it makes it possible for utilities to locate customer telephone complaints and supervise the location of field crews. IEC 61968-3 specifies the information content of a set of message payloads that can be used to support many of the business functions related to network operations. Typical uses of the message payloads defined in IEC 61968-3 include data acquisition by external systems, fault isolation, fault restoration, trouble management, maintenance of plant, and the commissioning of plant. This edition includes the following significant technical changes with respect to the previous edition: replacement of certain function names, addition of other function names."@en ;
                    rdfs:label "IEC 61968-3:2017"@en ;
                    prov:wasRevisionOf sto:IEC_61968_P3_E1 ;
                    sto:hasOfficialResource <https://webstore.iec.ch/publication/27527> ;
                    sto:hasStatus "Valid"@en ;
                    sto:hasWikipediaArticle <https://en.wikipedia.org/wiki/IEC_61968> .


###  https://w3id.org/i40/sto#IEC_61968_P4_E1
sto:IEC_61968_P4_E1 rdf:type owl:NamedIndividual ,
                             sto:Standard ;
                    sto:hasAvailableLanguage lang:eng ,
                                             lang:fra ;
                    sto:hasFileSize sto:FileSizeIEC_61968_P4_E1 ;
                    sto:hasICS sto:ICS_33_200 ;
                    sto:hasPublisher sto:IEC ;
                    sto:hasTechnicalCommittee sto:TC_57 ;
                    sto:relatedTo sto:IEC_61968_P3_E1 ;
                    sto:isPartOf sto:IEC_61968;
                    sto:hasEdition "1.0"^^xsd:float ;
                    sto:hasPages "101"^^xsd:int ;
                    sto:hasPublicationDate "2007-07-11"^^xsd:date ;
                    sto:hasStabilityDate "2020"^^xsd:gYear ;
                    sto:hasTag "IEC 61968-4:2007 "@en ;
                    dcterms:title "Application integration at electric utilities - System interfaces for distribution management - Part 4: Interfaces for records and asset management"@en ;
                    rdfs:comment "IEC 61968-4:2007 Specifies the information content of a set of message types that can be used to support many of the business functions related to records and asset management. Typical uses of the message types include network extension planning, copying feeder or other network data between systems, network or diagram edits and asset inspection.This publication is of core relevance for Smart Grid."@en ;
                    rdfs:label "IEC 61968-4:2007"@en ;
                    sto:hasOfficialResource <https://webstore.iec.ch/publication/6203> ;
                    sto:hasStatus "Valid"@en ;
                    sto:hasWikipediaArticle <https://en.wikipedia.org/wiki/IEC_61968> .


###  https://w3id.org/i40/sto#IEC_61968_P4_E2
sto:IEC_61968_P4_E2 rdf:type owl:NamedIndividual ,
                             sto:Standard ;
                    sto:hasAvailableLanguage lang:eng ,
                                             lang:fra ;
                    sto:hasFileSize sto:FileSizeIEC_61968_P4_E2 ;
                    sto:hasICS sto:ICS_33_200 ;
                    sto:hasPublisher sto:IEC ;
                    sto:hasTechnicalCommittee sto:TC_57 ;
                    sto:relatedTo sto:IEC_61968_P3_E1 ;
                    sto:isPartOf sto:IEC_61968;
                    sto:hasEdition "2.0"^^xsd:float ;
                    sto:hasPages "344"^^xsd:int ;
                    sto:hasPublicationDate "2018-12-14"^^xsd:date ;
                    sto:hasStabilityDate "2020"^^xsd:gYear ;
                    sto:hasTag "IEC 61968-4:2018 PRV "@en ;
                    dcterms:title "Application integration at electric utilities - System interfaces for distribution management - Part 4: Interfaces for records and asset management"@en ;
                    rdfs:comment "This Final Draft International Standard is an up to 6 weeks' pre-release of the official publication. It is available for sale during its voting period: 2018-12-14 to 2019-01-25. By purchasing this FDIS now, you will automatically receive, in addition, the final publication.IEC 61968:2019 specifies the information content of a set of message types that can be used to support many of the business functions related to records and asset management. Typical uses of the message types defined in this document include network extension planning, copying feeder or other network data between systems, network or diagram edits and asset inspection. Message types defined in other parts of IEC 61968 may also be relevant to these use cases.This second edition cancels and replaces the first edition published in 2007. This edition constitutes a technical revision. This edition includes the following significant technical changes with respect to the previous edition:a) removal of edition 1 profiles whose functionality has been superseded by other parts of IEC 61970 and IEC 61968 standards. In particular, NetworkDataSet and ChangeSet have been superseded by standards such as CDPSM (IEC 61968-13) and other ongoing efforts such as change modelling; and Presentation has been superseded by Diagram Layout Profile (IEC 61970-453);b) revision of the edition 1 profiles AssetList, AssetCatalogue and TypeAssetCatalogue to realign with current use cases and the latest CIM UML release. These profiles are based on an old version of CIM UML and many of the classes in these profiles are no longer in the recent CIM UMLs;c) addition of several new profiles to enable the exchange of asset condition data, analytics results and alerts, assets' physical, functional and lifecycle details, and assets' work;d) informative annexes on how this document can be used to enable strategic asset management;e) informative annexes with illustrative examples for the application of this document;f) scope coordinated with IEC 61968-13 where applicable;g) use cases in IEC 62559-2 use case template;h) traceability of use cases to IEC 62913-2-1 use cases."@en ;
                    rdfs:label "IEC 61968-4:2018 PRV"@en ;
                    prov:wasRevisionOf sto:IEC_61968_P4_E1 ;
                    sto:hasOfficialResource <https://webstore.iec.ch/publication/64397> ;
                    sto:hasStatus "Pre release version (PRV)"@en ;
                    sto:hasWikipediaArticle <https://en.wikipedia.org/wiki/IEC_61968> .


###  https://w3id.org/i40/sto#IEC_61968_P6_E1
sto:IEC_61968_P6_E1 rdf:type owl:NamedIndividual ,
                             sto:Standard ;
                    sto:hasAvailableLanguage lang:eng ,
                                             lang:fra ;
                    sto:hasFileSize sto:FileSizeIEC_61968_P6_E1 ;
                    sto:hasICS sto:ICS_33_200 ;
                    sto:hasPublisher sto:IEC ;
                    sto:hasTechnicalCommittee sto:TC_57 ;
                    sto:relatedTo sto:IEC_61968_P3_E1 ;
                    sto:isPartOf sto:IEC_61968;
                    sto:hasEdition "1.0"^^xsd:float ;
                    sto:hasPages "291"^^xsd:int ;
                    sto:hasPublicationDate "2015-07-07"^^xsd:date ;
                    sto:hasStabilityDate "2020"^^xsd:gYear ;
                    sto:hasTag "IEC 61968-6:2015 "@en ;
                    dcterms:title "Application integration at electric utilities - System interfaces for distribution management - Part 6: Interfaces for maintenance and construction"@en ;
                    rdfs:comment "IEC 61968-6:2015 specifies the information content of a set of message types that can be used to support business functions related to maintenance and construction. Typical uses of the message types defined in this part of IEC 61968 include planned maintenance, unplanned maintenance, conditional maintenance, work management, new service requests, etc. Message types defined in other parts of IEC 61968 may also be relevant to these use cases."@en ;
                    rdfs:label "IEC 61968-6:2015"@en ;
                    sto:hasOfficialResource <https://webstore.iec.ch/publication/22834> ;
                    sto:hasStatus "Valid"@en ;
                    sto:hasWikipediaArticle <https://en.wikipedia.org/wiki/IEC_61968> .


###  https://w3id.org/i40/sto#IEC_61968_P8_E1
sto:IEC_61968_P8_E1 rdf:type owl:NamedIndividual ,
                             sto:Standard ;
                    sto:hasAvailableLanguage lang:eng ,
                                             lang:fra ;
                    sto:hasFileSize sto:FileSizeIEC_61968_P8_E1 ;
                    sto:hasICS sto:ICS_33_200 ;
                    sto:hasPublisher sto:IEC ;
                    sto:hasTechnicalCommittee sto:TC_57 ;
                    sto:relatedTo sto:IEC_61968_P3_E1 ;
                    sto:isPartOf sto:IEC_61968;
                    sto:hasEdition "1.0"^^xsd:float ;
                    sto:hasPages "130"^^xsd:int ;
                    sto:hasPublicationDate "2015-05-27"^^xsd:date ;
                    sto:hasStabilityDate "2020"^^xsd:gYear ;
                    sto:hasTag "IEC 61968-8:2015  "@en ;
                    dcterms:title "Application integration at electric utilities - System interfaces for distribution management - Part 8: Interfaces for customer operations"@en ;
                    rdfs:comment "IEC 61968-8:2015 specifies the information content of a set of message types that can be used to support many of the business functions related to customer support. Typical uses of the message types include service request, customer agreement, and trouble management. The purpose is to define a standard for the integration of customer support (CS), which would include customer service, trouble management and point of sale related components integrated with other systems and business functions within the scope of IEC 61968. The scope of this standard is the exchange of information between a customer support system and other systems within the utility enterprise."@en ;
                    rdfs:label "IEC 61968-8:2015 "@en ;
                    sto:hasOfficialResource <https://webstore.iec.ch/publication/22537> ;
                    sto:hasStatus "Valid"@en ;
                    sto:hasWikipediaArticle <https://en.wikipedia.org/wiki/IEC_61968> .


###  https://w3id.org/i40/sto#IEC_61968_P9_E1
sto:IEC_61968_P9_E1 rdf:type owl:NamedIndividual ,
                             sto:Standard ;
                    sto:hasAvailableLanguage lang:eng ;
                    sto:hasFileSize sto:FileSizeIEC_61968_P9_E1 ;
                    sto:hasICS sto:ICS_33_200 ;
                    sto:hasPublisher sto:IEC ;
                    sto:hasTechnicalCommittee sto:TC_57 ;
                    sto:relatedTo sto:IEC_61968_P3_E1 ;
                    sto:isPartOf sto:IEC_61968;
                    sto:hasEdition "1.0"^^xsd:float ;
                    sto:hasPages "257"^^xsd:int ;
                    sto:hasPublicationDate "2009-09-16"^^xsd:date ;
                    sto:hasTag "IEC 61968-9:2009"@en ;
                    dcterms:title "Application integration at electric utilities - System interfaces for distribution management - Part 9: Interfaces for meter reading and control"@en ;
                    rdfs:comment "IEC 61968-9:2009(E) specifies the information content of a set of message types that can be used to support many of the business functions related to meter reading and control. Typical uses of the message types include meter reading, meter control, meter events, customer data synchronization and customer switching. Although intended primarily for electrical distribution networks, IEC 61968-9 can be used for other metering applications, including non-electrical metered quantities necessary to support gas and water networks. This publication is of core relevance for Smart Grid.."@en ;
                    rdfs:label "IEC 61968-9:2009"@en ;
                    sto:hasOfficialResource <https://webstore.iec.ch/publication/20183> ;
                    sto:hasStatus "Withdrawn"@en ;
                    sto:hasWikipediaArticle <https://en.wikipedia.org/wiki/IEC_61968> .


###  https://w3id.org/i40/sto#IEC_61968_P9_E2
sto:IEC_61968_P9_E2 rdf:type owl:NamedIndividual ,
                             sto:Standard ;
                    sto:hasAvailableLanguage lang:eng ,
                                             lang:fra ;
                    sto:hasFileSize sto:FileSizeIEC_61968_P9_E2 ;
                    sto:hasICS sto:ICS_33_200 ;
                    sto:hasPublisher sto:IEC ;
                    sto:hasTechnicalCommittee sto:TC_57 ;
                    sto:relatedTo sto:IEC_61968_P3_E1 ;
                    sto:isPartOf sto:IEC_61968;
                    sto:hasEdition "2.0"^^xsd:float ;
                    sto:hasPages "919"^^xsd:int ;
                    sto:hasPublicationDate "2013-10-16"^^xsd:date ;
                    sto:hasStabilityDate "2020"^^xsd:gYear ;
                    sto:hasTag "IEC 61968-9:2013 "@en ;
                    dcterms:title "Application integration at electric utilities - System interfaces for distribution management - Part 9: Interfaces for meter reading and control"@en ;
                    rdfs:comment "IEC 61968-9:2013 specifies the information content of a set of message types that can be used to support many of the business functions related to meter reading and control. Typical uses of the message types include meter reading, controls, events, customer data synchronization and customer switching. The purpose of IEC 61968-9 is to define a standard for the integration of metering systems (MS), which includes traditional manual systems, and (one or two-way) automated meter reading (AMR) systems, and meter data management (MDM) systems with other enterprise systems and business functions within the scope of IEC 61968. The scope of IEC 61968-9 is the exchange of information between metering systems, MDM systems and other systems within the utility enterprise. This new edition includes the following significant technical changes with respect to the previous edition:- changes to and addition of new profiles to support PAN and UsagePoints;- extensions to support PAN devices generically as EndDevices;- extensions to the MeterReading model and profiles to support richer descriptions of metered quantities and to accommodate coincident readings.."@en ;
                    rdfs:label "IEC 61968-9:2013"@en ;
                    prov:wasRevisionOf sto:IEC_61968_P9_E1 ;
                    sto:hasOfficialResource <https://webstore.iec.ch/publication/6204> ;
                    sto:hasStatus "Valid"@en ;
                    sto:hasWikipediaArticle <https://en.wikipedia.org/wiki/IEC_61968> .

sto:IEC_61970 rdf:type owl:NamedIndividual ,
                             sto:Standard ;
                    sto:hasPublisher sto:IEC ;
                    dcterms:title "Energy management system application program interface (EMS-API)"@en ;
                    rdfs:comment "Provides a set of guidelines and general infrastructure capabilities required for the application of the EMS-API interface standards."@en ;
                    rdfs:label "IEC 61970 "@en ;
                    sto:hasWikipediaArticle <https://en.wikipedia.org/wiki/IEC_61970> .

###  https://w3id.org/i40/sto#IEC_61970_P1_E1
sto:IEC_61970_P1_E1 rdf:type owl:NamedIndividual ,
                             sto:Standard ;
                    sto:hasAvailableLanguage lang:eng ,
                                             lang:fra ;
                    sto:hasFileSize sto:FileSizeIEC_61970_P1_E1 ;
                    sto:hasICS sto:ICS_33_200 ;
                    sto:hasPublisher sto:IEC ;
                    sto:hasTechnicalCommittee sto:TC_57 ;
                    sto:isPartOf sto:IEC_61970;
                    sto:hasEdition "1.0"^^xsd:float ;
                    sto:hasPages "81"^^xsd:int ;
                    sto:hasPublicationDate "2005-12-07"^^xsd:date ;
                    sto:hasStabilityDate "2020"^^xsd:gYear ;
                    sto:hasTag "IEC 61970-1:2005  "@en ;
                    dcterms:title "Energy management system application program interface (EMS-API) - Part 1: Guidelines and general requirements"@en ;
                    rdfs:comment "Provides a set of guidelines and general infrastructure capabilities required for the application of the EMS-API interface standards. Describes typical integration scenarios where these standards are to be applied and the types of applications to be integrated. Defines a reference model and provides a framework for the application of the other parts of these EMS-API standards.This publication is of core relevance for Smart Grid."@en ;
                    rdfs:label "IEC 61970-1:2005 "@en ;
                    sto:hasOfficialResource <https://webstore.iec.ch/publication/6208> ;
                    sto:hasStatus "Valid"@en ;
                    sto:hasWikipediaArticle <https://en.wikipedia.org/wiki/IEC_61970> .


###  https://w3id.org/i40/sto#IEC_61970_P301_E1
sto:IEC_61970_P301_E1 rdf:type owl:NamedIndividual ,
                               sto:Standard ;
                      sto:hasAvailableLanguage lang:eng ,
                                               lang:fra ;
                      sto:hasFileSize sto:FileSizeIEC_61970_P301_E1 ;
                      sto:hasICS sto:ICS_33_200 ;
                      sto:hasPublisher sto:IEC ;
                      sto:hasTechnicalCommittee sto:TC_57 ;
                      sto:isPartOf sto:IEC_61970;
                      sto:hasEdition "1.0"^^xsd:float ;
                      sto:hasPages "369"^^xsd:int ;
                      sto:hasPublicationDate "2003-11-26"^^xsd:date ;
                      sto:hasTag "IEC 61970-301:2003 "@en ;
                      dcterms:title "Energy management system application program interface (EMS-API) - Part 301: Common information model (CIM) base"@en ;
                      rdfs:comment "Defines the Common Information Model Base set of packages which provide a logical view of the physical aspects of Energy Management System information. Is part of the IEC 61970 series, which defines an Application Program Interface (API) for an Energy Management System (EMS)."@en ;
                      rdfs:label "IEC 61970-301:2003"@en ;
                      sto:hasOfficialResource <https://webstore.iec.ch/publication/20189> ;
                      sto:hasStatus "Withdrawn"@en ;
                      sto:hasWikipediaArticle <https://en.wikipedia.org/wiki/IEC_61970> .


###  https://w3id.org/i40/sto#IEC_61970_P301_E2
sto:IEC_61970_P301_E2 rdf:type owl:NamedIndividual ,
                               sto:Standard ;
                      sto:hasAvailableLanguage lang:eng ;
                      sto:hasFileSize sto:FileSizeIEC_61970_P301_E2 ;
                      sto:hasICS sto:ICS_33_200 ;
                      sto:hasPublisher sto:IEC ;
                      sto:hasTechnicalCommittee sto:TC_57 ;
                      sto:isPartOf sto:IEC_61970;
                      sto:hasEdition "2.0"^^xsd:float ;
                      sto:hasPages "211"^^xsd:int ;
                      sto:hasPublicationDate "2009-04-07"^^xsd:date ;
                      sto:hasTag "IEC 61970-301:2009 "@en ;
                      dcterms:title "Energy management system application program interface (EMS-API) - Part 301: Common information model (CIM) base"@en ;
                      rdfs:comment "IEC 61970-301:2009(E) defines the Common Information Model (CIM) base set of packages which provide a logical view of the physical aspects of an energy management system including SCADA (Supervisory Control and Data Acquisition). Whilst there are multiple IEC standards dealing with different parts of the CIM, there is a single, unified normalized information model comprising the CIM behind all these individual standards documents. This second edition contains the following main changes with respect to the previous edition:- change of the naming hierarchy,- replacement of several classes,- addition of several new classes,- many editorial corrections to resolve issues included in the first edition. This publication is of core relevance for Smart Grid."@en ;
                      rdfs:label "IEC 61970-301:2009"@en ;
                      prov:wasRevisionOf sto:IEC_61970_P301_E1 ;
                      sto:hasOfficialResource <https://webstore.iec.ch/publication/20190> ;
                      sto:hasStatus "Withdrawn"@en ;
                      sto:hasWikipediaArticle <https://en.wikipedia.org/wiki/IEC_61970> .


###  https://w3id.org/i40/sto#IEC_61970_P301_E3
sto:IEC_61970_P301_E3 rdf:type owl:NamedIndividual ,
                               sto:Standard ;
                      sto:hasAvailableLanguage lang:eng ,
                                               lang:fra ;
                      sto:hasFileSize sto:FileSizeIEC_61970_P301_E3 ;
                      sto:hasICS sto:ICS_33_200 ;
                      sto:hasPublisher sto:IEC ;
                      sto:hasTechnicalCommittee sto:TC_57 ;
                      sto:isPartOf sto:IEC_61970;
                      sto:hasEdition "3.0"^^xsd:float ;
                      sto:hasPages "533"^^xsd:int ;
                      sto:hasPublicationDate "2011-08-26"^^xsd:date ;
                      sto:hasTag "IEC 61970-301:2011 "@en ;
                      dcterms:title "Energy management system application program interface (EMS-API) - Part 301: Common information model (CIM) base"@en ;
                      rdfs:comment "IEC 61970-301:2011 deals with the common information model (CIM), an abstract model that represents all the major objects in an electric utility enterprise typically involved in utility operations. The object classes represented in the CIM are abstract in nature and may be used in a wide variety of applications. The use of the CIM goes far beyond its application in an EMS. This standard should be understood as a tool to enable integration in any domain where a common power system model is needed to facilitate interoperability and plug compatibility between applications and systems independent of any particular implementation. Major changes from the second edition include the following:- Addition of regulation control models;- new (OperationalLimits) package for equipment ratings;- addition of partial ownership specification;- enhancement of LoadResponseCharacteristic;- change from non-SI units to SI units."@en ;
                      rdfs:label "IEC 61970-301:2011"@en ;
                      prov:wasRevisionOf sto:IEC_61970_P301_E2 ;
                      sto:hasOfficialResource <https://webstore.iec.ch/publication/20191> ;
                      sto:hasStatus "Withdrawn"@en ;
                      sto:hasWikipediaArticle <https://en.wikipedia.org/wiki/IEC_61970> .


###  https://w3id.org/i40/sto#IEC_61970_P301_E4
sto:IEC_61970_P301_E4 rdf:type owl:NamedIndividual ,
                               sto:Standard ;
                      sto:hasAvailableLanguage lang:eng ,
                                               lang:fra ;
                      sto:hasFileSize sto:FileSizeIEC_61970_P301_E4 ;
                      sto:hasICS sto:ICS_33_200 ;
                      sto:hasPublisher sto:IEC ;
                      sto:hasTechnicalCommittee sto:TC_57 ;
                      sto:isPartOf sto:IEC_61970;
                      sto:hasEdition "4.0"^^xsd:float ;
                      sto:hasPages "644"^^xsd:int ;
                      sto:hasPublicationDate "2013-05-23"^^xsd:date ;
                      sto:hasTag "IEC 61970-301:2013 "@en ;
                      dcterms:title "Energy management system application program interface (EMS-API) - Part 301: Common information model (CIM) base"@en ;
                      rdfs:comment "IEC 61970-301:2013 deals with the common information model (CIM), an abstract model that represents all the major objects in an electric utility enterprise typically involved in utility operations. The object classes represented in the CIM are abstract in nature and may be used in a wide variety of applications. The use of the CIM goes far beyond its application in an EMS. This standard is to be understood as a tool to enable integration in any domain where a common power system model is needed to facilitate interoperability and plug compatibility between applications and systems independent of any particular implementation. Major changes from the third edition include the following:- extensions have been added to support UCTE exchange;- the transformer regulation model has been expanded to support phase shifting transformer models needed by ENTSO-E;- zero and negative sequence impedance terms have been added;- new StateVariables package has been added;- additional classes have been added."@en ;
                      rdfs:label "IEC 61970-301:2013"@en ;
                      prov:wasRevisionOf sto:IEC_61970_P301_E3 ;
                      sto:hasOfficialResource <https://webstore.iec.ch/publication/20192> ;
                      sto:hasStatus "Withdrawn"@en ;
                      sto:hasWikipediaArticle <https://en.wikipedia.org/wiki/IEC_61970> .


###  https://w3id.org/i40/sto#IEC_61970_P301_E5
sto:IEC_61970_P301_E5 rdf:type owl:NamedIndividual ,
                               sto:Standard ;
                      sto:hasAvailableLanguage lang:eng ,
                                               lang:fra ;
                      sto:hasFileSize sto:FileSizeIEC_61970_P301_E5 ;
                      sto:hasICS sto:ICS_33_200 ;
                      sto:hasPublisher sto:IEC ;
                      sto:hasTechnicalCommittee sto:TC_57 ;
                      sto:isPartOf sto:IEC_61970;
                      sto:hasEdition "5.0"^^xsd:float ;
                      sto:hasPages "766"^^xsd:int ;
                      sto:hasPublicationDate "2013-12-13"^^xsd:date ;
                      sto:hasTag "IEC 61970-301:2013 "@en ;
                      dcterms:title "Energy management system application program interface (EMS-API) - Part 301: Common information model (CIM) base"@en ;
                      rdfs:comment "IEC 61970-301:2013 defines the Common Information Model (CIM), that is an abstract model representing all the major objects in an electric utility enterprise typically involved in utility operations. By providing a standard way of representing power system resources as object classes and attributes, along with their relationships, the CIM facilitates the integration of Energy Management System (EMS) applications developed independently by different vendors, between entire EMS systems developed independently, or between an EMS system and other systems concerned with different aspects of power system operations, such as generation or distribution management. SCADA is modeled to the extent necessary to support power system simulation and inter-control center communication. The CIM facilitates integration by defining a common language (i.e. semantics) based on the CIM to enable these applications or systems to access public data and exchange information independent of how such information is represented internally. Major changes from the fourth edition include the following:- transformer models have been modified to be consistent for use by distribution and transmission purposes;- a more general and clear naming approach was added and several ambiguous attributes related to naming were dropped;- phase component wires models have been enhanced to describe internal phase specific attributes and connections;- addition of diagram layout models to facilitate the exchange of diagram layout information."@en ;
                      rdfs:label "IEC 61970-301:2013"@en ;
                      prov:wasRevisionOf sto:IEC_61970_P301_E4 ;
                      sto:hasOfficialResource <https://webstore.iec.ch/publication/6210> ;
                      sto:hasStatus "Withdrawn"@en ;
                      sto:hasWikipediaArticle <https://en.wikipedia.org/wiki/IEC_61970> .


###  https://w3id.org/i40/sto#IEC_61970_P301_E6
sto:IEC_61970_P301_E6 rdf:type owl:NamedIndividual ,
                               sto:Standard ;
                      sto:hasAvailableLanguage lang:eng ,
                                               lang:fra ;
                      sto:hasFileSize sto:FileSizeIEC_61970_P301_E6 ;
                      sto:hasICS sto:ICS_33_200 ;
                      sto:hasPublisher sto:IEC ;
                      sto:hasTechnicalCommittee sto:TC_57 ;
                      sto:isPartOf sto:IEC_61970;
                      sto:hasEdition "6.0"^^xsd:float ;
                      sto:hasPages "938"^^xsd:int ;
                      sto:hasPublicationDate "2016-12-16"^^xsd:date ;
                      sto:hasStabilityDate "2020"^^xsd:gYear ;
                      sto:hasTag "IEC 61970-301:2016 "@en ;
                      dcterms:title "Energy management system application program interface (EMS-API) - Part 301: Common information model (CIM) base"@en ;
                      rdfs:comment "IEC 61970-301:2016 is available as IEC 61970-301:2016 RLV which contains the International Standard and its Redline version, showing all changes of the technical content compared to the previous edition.IEC 61970-301:2016 lays down the common information model (CIM), which is an abstract model that represents all the major objects in an electric utility enterprise typically involved in utility operations. By providing a standard way of representing power system resources as object classes and attributes, along with their relationships, the CIM facilitates the integration of network applications developed independently by different vendors, between entire systems running network applications developed independently, or between a system running network applications and other systems concerned with different aspects of power system operations, such as generation or distribution management. SCADA is modeled to the extent necessary to support power system simulation and inter-control centre communication. The CIM facilitates integration by defining a common language (i.e. semantics) based on the CIM to enable these applications or systems to access public data and exchange information independent of how such information is represented internally. This new edition includes the following significant technical changes with respect to the previous edition:- new model for grounding including Petersen coils;- models for HVDC; addition of Static Var Compensation models;- phase shift transformer updates;- short circuit calculations based on IEC 60909;- addition of non-linear shunt compensator;- addition of model for steady state calculation inputs, Steady State Hypothesis;- addition of base frequency model;- Annex A with custom extensions added."@en ;
                      rdfs:label "IEC 61970-301:2016"@en ;
                      prov:wasRevisionOf sto:IEC_61970_P301_E5 ;
                      sto:hasOfficialResource <https://webstore.iec.ch/publication/31356> ;
                      sto:hasStatus "Valid"@en ;
                      sto:hasWikipediaArticle <https://en.wikipedia.org/wiki/IEC_61970> .


###  https://w3id.org/i40/sto#IEC_61970_P301_E6_RLV
sto:IEC_61970_P301_E6_RLV rdf:type owl:NamedIndividual ,
                                   sto:Standard ;
                          sto:hasAvailableLanguage lang:eng ,
                                                   lang:fra ;
                          sto:hasFileSize sto:FileSizeIEC_61970_P301_E6_RLV ;
                          sto:hasICS sto:ICS_33_200 ;
                          sto:hasPublisher sto:IEC ;
                          sto:hasTechnicalCommittee sto:TC_57 ;
                          sto:isPartOf sto:IEC_61970;
                          sto:hasEdition "6.0"^^xsd:float ;
                          sto:hasPages "1423"^^xsd:int ;
                          sto:hasPublicationDate "2016-12-16"^^xsd:date ;
                          sto:hasStabilityDate "2020"^^xsd:gYear ;
                          sto:hasTag "IEC 61970-301:2016 RLV Redline version "@en ;
                          dcterms:title "Energy management system application program interface (EMS-API) - Part 301: Common information model (CIM) base"@en ;
                          rdfs:comment "IEC 61970-301:2016 RLV contains both the official IEC International Standard and its Redline version. The Redline version is not an official document, it is available in English only and provides you with a quick and easy way to compare all the changes between the official IEC Standard and its previous edition.IEC 61970-301:2016 lays down the common information model (CIM), which is an abstract model that represents all the major objects in an electric utility enterprise typically involved in utility operations. By providing a standard way of representing power system resources as object classes and attributes, along with their relationships, the CIM facilitates the integration of network applications developed independently by different vendors, between entire systems running network applications developed independently, or between a system running network applications and other systems concerned with different aspects of power system operations, such as generation or distribution management. SCADA is modeled to the extent necessary to support power system simulation and inter-control centre communication. The CIM facilitates integration by defining a common language (i.e. semantics) based on the CIM to enable these applications or systems to access public data and exchange information independent of how such information is represented internally. This new edition includes the following significant technical changes with respect to the previous edition:- new model for grounding including Petersen coils;- models for HVDC; addition of Static Var Compensation models;- phase shift transformer updates;- short circuit calculations based on IEC 60909;- addition of non-linear shunt compensator;- addition of model for steady state calculation inputs, Steady State Hypothesis;- addition of base frequency model;- Annex A with custom extensions added."@en ;
                          rdfs:label "IEC 61970-301:2016 RLV Redline version "@en ;
                          prov:wasRevisionOf sto:IEC_61970_P301_E6 ;
                          sto:hasOfficialResource <https://webstore.iec.ch/publication/59669> ;
                          sto:hasStatus "RLV-Redline version"@en ;
                          sto:hasWikipediaArticle <https://en.wikipedia.org/wiki/IEC_61970> .


###  https://w3id.org/i40/sto#IEC_61970_P452_E1
sto:IEC_61970_P452_E1 rdf:type owl:NamedIndividual ,
                               sto:Standard ;
                      sto:hasAvailableLanguage lang:eng ,
                                               lang:fra ;
                      sto:hasFileSize sto:FileSizeIEC_61970_P452_E1 ;
                      sto:hasICS sto:ICS_33_200 ;
                      sto:hasPublisher sto:IEC ;
                      sto:hasTechnicalCommittee sto:TC_57 ;
                      sto:isPartOf sto:IEC_61970;
                      sto:hasEdition "1.0"^^xsd:float ;
                      sto:hasPages "244"^^xsd:int ;
                      sto:hasPublicationDate "2013-08-12"^^xsd:date ;
                      sto:hasTag "IEC 61970-452:2013 "@en ;
                      dcterms:title "Energy management system application program interface (EMS-API) - Part 452: CIM Static transmission network model profiles"@en ;
                      rdfs:comment "IEC 61970-452:2013 rigorously defines the subset of classes, class attributes, and roles from the CIM necessary to execute state estimation and power flow applications. This international standard is intended for two distinct audiences, data producers and data recipients, and may be read from two perspectives."@en ;
                      rdfs:label "IEC 61970-452:2013"@en ;
                      sto:hasOfficialResource <https://webstore.iec.ch/publication/6212> ;
                      sto:hasStatus "Withdrawn"@en ;
                      sto:hasWikipediaArticle <https://en.wikipedia.org/wiki/IEC_61970> .


###  https://w3id.org/i40/sto#IEC_61970_P452_E2
sto:IEC_61970_P452_E2 rdf:type owl:NamedIndividual ,
                               sto:Standard ;
                      sto:hasAvailableLanguage lang:eng ,
                                               lang:fra ;
                      sto:hasFileSize sto:FileSizeIEC_61970_P452_E2 ;
                      sto:hasICS sto:ICS_33_200 ;
                      sto:hasPublisher sto:IEC ;
                      sto:hasTechnicalCommittee sto:TC_57 ;
                      sto:isPartOf sto:IEC_61970;
                      sto:hasEdition "2.0"^^xsd:float ;
                      sto:hasPages "203"^^xsd:int ;
                      sto:hasPublicationDate "2015-04-09"^^xsd:date ;
                      sto:hasTag "IEC 61970-452:2015 "@en ;
                      dcterms:title "Energy management system application program interface (EMS-API) - Part 452: CIM model exchange specification"@en ;
                      rdfs:comment "IEC 61970-452:2015 rigorously defines the subset of classes, class attributes, and roles from the CIM necessary to execute state estimation and power flow applications. These requirements are based on prior industry practices for exchanging power system model data for use primarily in planning studies. This standard is intended for two distinct audiences, data producers and data recipients, and may be used from these two perspectives.."@en ;
                      rdfs:label "IEC 61970-452:2015"@en ;
                      prov:wasRevisionOf sto:IEC_61970_P452_E1 ;
                      sto:hasOfficialResource <https://webstore.iec.ch/publication/22090> ;
                      sto:hasStatus "Withdrawn"@en ;
                      sto:hasWikipediaArticle <https://en.wikipedia.org/wiki/IEC_61970> .


###  https://w3id.org/i40/sto#IEC_61970_P452_E3
sto:IEC_61970_P452_E3 rdf:type owl:NamedIndividual ,
                               sto:Standard ;
                      sto:hasAvailableLanguage lang:eng ,
                                               lang:fra ;
                      sto:hasFileSize sto:FileSizeIEC_61970_P452_E3 ;
                      sto:hasICS sto:ICS_33_200 ;
                      sto:hasPublisher sto:IEC ;
                      sto:hasTechnicalCommittee sto:TC_57 ;
                      sto:isPartOf sto:IEC_61970;
                      sto:hasRelevantDomain sto:Automation ,
                                        sto:CGMES ,
                                        sto:CyberSecurity ,
                                        sto:SmartCity ,
                                        sto:SmartEnergy ,
                                        sto:SmartGrid ;
                      sto:hasEdition "3.0"^^xsd:float ;
                      sto:hasPages "342"^^xsd:int ;
                      sto:hasPublicationDate "2017-07-26"^^xsd:date ;
                      sto:hasTag "IEC 61970-452:2017 "@en ;
                      dcterms:title "Energy management system application program interface (EMS-API) - Part 452: CIM static transmission network model profiles"@en ;
                      rdfs:comment "IEC 61970-452:2017 defines the subset of classes, class attributes, and roles from the CIM necessary to execute state estimation and power flow applications. This standard is intended for two distinct audiences, data producers and data recipients, and may be read from two perspectives. From the standpoint of model export software used by a data producer, the document describes a minimum subset of CIM classes, attributes, and associations which must be present in an XML formatted data file for model exchange. This new edition includes the following significant technical changes with respect to the previous edition: the Equipment profile has been split into three separate profiles, CoreEquipment, Operation and ShortCircuit; the HVDC model has been replaced with the new model defined in Edition 6 of 61970‑301."@en ;
                      rdfs:label "IEC 61970-452:2017"@en ;
                      prov:wasRevisionOf sto:IEC_61970_P452_E2 ;
                      sto:hasOfficialResource <https://webstore.iec.ch/publication/30444> ;
                      sto:hasStatus "Valid"@en ;
                      sto:hasWikipediaArticle <https://en.wikipedia.org/wiki/IEC_61970> .


###  https://w3id.org/i40/sto#IEC_61987_X
sto:IEC_61987_X rdf:type owl:NamedIndividual ,
                         sto:Standard ;
                dcterms:creator sto:irlan ,
                                sto:sebastian ;
                sto:hasClassification sto:AsEngineering ,
                                      sto:RamiControlDevice ,
                                      sto:RamiEnterprise ,
                                      sto:RamiFieldDevice ,
                                      sto:RamiProduct ,
                                      sto:RamiStation ,
                                      sto:RamiWorkCenter ;
                sto:hasPublisher sto:IEC ;
                sto:hasMotivation "Properties and LOPs as an informational representation of the features of measuring equipment. The referenced standards define general principles (e.g. part 11) as well as specific LOPs for specific device types. These international standards also may serve as examples for description of products."@en ;
                sto:hasTag "LOPs in PA"@en ;
                dcterms:license sto:PrivateLicenseDocument ;
                rdfs:comment "Industrial-process measurement and control - Data structures and elements in process equipment catalogs - Measuring equipment with analogue and digital output"@en ;
                rdfs:label "IEC 61987_X"@en ;
                sto:hasOfficialResource <https://webstore.iec.ch/publication/6225> .


###  https://w3id.org/i40/sto#IEC_62061
sto:IEC_62061 rdf:type owl:NamedIndividual ,
                       sto:Standard ;
              dcterms:creator sto:irlan ;
              sto:hasClassification sto:AsSafety  ;
              sto:hasPublisher sto:IEC ;
              sto:relatedTo sto:IEC_61508 ,
                            sto:IEC_61511 ,
                            sto:IEC_62061 ,
                            sto:ISO_13849 ;
              sto:hasTag "Safety of machinery"@en ;
              rdfs:comment "provides requirements that are applicable to the system level design of all types of machinery safety-related electrical control systems and also for the design of non-complex subsystems or devices."@en ;
              rdfs:label "IEC 60061"@en ;
              sto:hasDBpediaResource <http://dbpedia.org/resource/IEC_62061> ;
              sto:hasOfficialResource <https://webstore.iec.ch/publication/22797> ;
              sto:hasWikipediaArticle <https://en.wikipedia.org/wiki/IEC_62061> .


###  https://w3id.org/i40/sto#IEC_62237
sto:IEC_62237 rdf:type owl:NamedIndividual ,
                       sto:Standard ,
                       sto:TechnicalSpecification ;
              dcterms:creator sto:irlan;
              sto:hasClassification sto:AdminShellGeneral,
                                    sto:ProductionSystemModelData ,
                                    sto:RamiControlDevice ,
                                    sto:RamiFieldDevice ,
                                    sto:RamiStation ,
                                    sto:RamiWorkCenter ;
              sto:hasPublisher sto:IEC ;
              sto:relatedTo sto:IEC_62237 ,
                            sto:IEC_62337 ;
              sto:hasPublicationDate "2003-10-26"^^xsd:date ;
              rdfs:comment "Live working - Insulating hoses with fittings for use with hydraulic tools and equipment."@en ;
              rdfs:label "IEC 62237"@en ;
              sto:hasRelevantDomain sto:IndustrialAutomation ;
              sto:hasOfficialResource <https://webstore.iec.ch/publication/6626> .


###  https://w3id.org/i40/sto#IEC_62264
sto:IEC_62264 rdf:type owl:NamedIndividual ,
                       sto:Standard ;
              dcterms:creator sto:irlan ,
                              sto:sebastian ;
              sto:hasClassification sto:RamiFunctional ;
              sto:hasDeveloper sto:IEC ;
              sto:hasDomain sto:Enterprise_Control ;
              sto:hasPublisher sto:IEC ,
                               sto:MESA ;
              sto:relatedTo sto:ISA-95 ;
              sto:hasMotivation "Informational representation of MES and ERP models."@en ;
              sto:hasTag "Enterprise control systems"@en ,
                         "Enterprise-control system integration"@en ;
              dcterms:license sto:PrivateLicenseDocument ;
              rdfs:comment "Enterprise-control system integration - Models and terminology"@en ,
                           "IEC 62264 is an international standard for enterprise-control system integration. This standard is based upon ANSI/ISA-95."@en ;
              rdfs:label "IEC 62264"@en ;
              rdfs:seeAlso <https://en.wikipedia.org/wiki/B2MML> ;
              skos:altLabel "B2MML"^^xsd:string ;
              sto:hasDBpediaResource <http://dbpedia.org/resource/IEC_62264> ;
              sto:hasRelevantDomain sto:Enterprise_Control ;
              sto:hasMotivation "Informational representation of MES and ERP models."@en ;
              sto:hasOfficialResource <http://www.iso.org/iso/catalogue_detail.htm?csnumber=63740> ,
                                      <https://webstore.iec.ch/publication/6675> ,
                                      <https://www.iso.org/standard/57308.html> ;
              sto:hasWikipediaArticle <https://en.wikipedia.org/wiki/IEC_62264> .


###  https://w3id.org/i40/sto#IEC_62264_P6
sto:IEC_62264_P6 rdf:type owl:NamedIndividual ,
                          sto:Standard ;
                 sto:hasAvailableLanguage lang:eng ;
                 sto:hasFileSize sto:FileSizeIEC_62264_P6 ;
                 sto:hasICS sto:ICS_25_040_99 ,
                            sto:ICS_35_100 ,
                            sto:ICS_35_100_50 ;
                 sto:hasPublisher sto:IEC ;
                 sto:hasTechnicalCommittee sto:TC_65 ;
                 sto_iot:frames sto:Communication ;
                 sto:isPartOf sto:IEC_62264;
                 sto:hasEdition "1.0"^^xsd:float ;
                 sto:hasPages "50"^^xsd:int ;
                 sto:hasPublicationDate "2016-07-05"^^xsd:date ;
                 sto:hasTag "IEC PAS 62264-6:2016"@en ;
                 dcterms:title "Enterprise-control system integration - Part 6: Messaging Service Model"@en ;
                 rdfs:comment "IEC PAS 62264-6:2016(E) defines a model of a set of messaging services for information exchanges across Levels 3 and 4, and within Level 3, between applications performing business and manufacturing activities. It defines a standard interface for information exchange between systems."@en ;
                 rdfs:label " IEC PAS 62264-6:2016"@en ;
                 sto:hasOfficialResource <https://webstore.iec.ch/publication/25315> .


###  https://w3id.org/i40/sto#IEC_62279
sto:IEC_62279 rdf:type owl:NamedIndividual ,
                       sto:Standard ;
              dcterms:creator sto:irlan ;
              sto:hasClassification sto:Safety ;
              sto:hasDomain sto:ITSecurity ;
              sto:hasPublisher sto:IEC ;
              sto:hasPublicationDate "2015-06-25"^^xsd:date ;
              rdfs:comment "IEC 62279:2015 specifies the process and technical requirements for the development of software for programmable electronic systems for use in railway control and protection applications. It is aimed at use in any area where there are safety implications. These systems can be implemented using dedicated microprocessors, programmable logic controllers, multiprocessor distributed systems, larger scale central processor systems or other architectures."@en ;
              rdfs:label "IEC 62279"@en ;
              sto:hasRelevantDomain sto:ITSecurity ;
              sto:hasOfficialResource <https://webstore.iec.ch/publication/22781> .


###  https://w3id.org/i40/sto#IEC_62337
sto:IEC_62337 rdf:type owl:NamedIndividual ,
                       sto:Standard ;
              dcterms:creator sto:irlan ;
              sto:hasClassification sto:AsConditionMonitoring ,
                                    sto:AsLifecycle_Status ,
                                    sto:ProductionSystemModelData ,
                                    sto:RamiEnterprise ,
                                    sto:RamiFunctionalLayer ,
                                    sto:RamiWorkCenter ;
              sto:hasPublisher sto:IEC ;
              sto:relatedTo sto:IEC_62237 ,
                            sto:IEC_62337 ;
              sto:hasPublicationDate "2012-02-22"^^xsd:date ;
              rdfs:comment "Commissioning of electrical, instrumentation and control systems in the process industry - Specific phases and milestones."@en ;
              rdfs:label "IEC 62337"@en ;
              sto:hasRelevantDomain sto:IndustrialAutomation ;
              sto:hasOfficialResource <https://webstore.iec.ch/publication/6871> .


###  https://w3id.org/i40/sto#IEC_62424
sto:IEC_62424 rdf:type owl:NamedIndividual ,
                       sto:Standard ;
              dcterms:creator sto:irlan ;
              dul:isComponentOf sto:IEC_62714 ;
              sto:hasPublisher sto:IEC ;
              sto:hasTag "CAEX"@en ;
              dcterms:license sto:PrivateLicenseDocument ;
              rdfs:comment "CAEX (Computer Aided Engineering Exchange) is a neutral data format that allows storage of hierarchical object information, e.g. the hierarchical architecture of a plant. On a certain abstraction level, a plant consists in modules or components that are interconnected. CAEX allows storage of those modules or components by means of objects. Object oriented concepts as encapsulation, classes, class libraries, instances, instance hierarchies, inheritance, relations, attributes and interfaces are explicitly supported. CAEX bases on XML and is defined as XML schema (xsd file). The original intention of developing CAEX was the industrial lack of a common and established data exchange between process engineering tools and process control engineering tools. However, CAEX can be applied to all types of static object information, e.g. plant topologies, document topologies, product topologies, petri nets, but also for non-technical applications like phylogenetic trees."@en ;
              rdfs:label "IEC 62424"@en ;
              sto:hasDBpediaResource <http://dbpedia.org/resource/CAEX> ;
              sto:hasOfficialResource <https://webstore.iec.ch/publication/25442> ;
              sto:hasWikipediaArticle <https://en.wikipedia.org/wiki/CAEX> .


###  https://w3id.org/i40/sto#IEC_62443
sto:IEC_62443 rdf:type owl:NamedIndividual ,
                       sto:Standard ;
              dcterms:creator sto:irlan ,
                              sto:sebastian  ;
              sto_iot:hasTargetConcern sto:IdentityManagement;
              sto:hasClassification sto:RamiIdentification,
                                    sto:AsSecurity ,
                                    sto:ISA95CrossLevel ,
                                    sto:IDSRAMCertification ,
                                    sto:IIRASecurity ;
              sto:hasDeveloper sto:ANSI ,
                               sto:ISA ;
              sto:hasPublisher sto:ANSI ,
                               sto:IEC ,
                               sto:ISA ;
              sto:hasMotivation "Cyber attacks threat the industry and can cause damage to property and personal injury and affect the image of companies. The Standard allows to define procedures for implementing electronically secure Industrial Automation and Control Systems (IACS). This guidance applies to end-users, system integrators, security practitioners, and control systems manufacturers responsible for manufacturing, designing, implementing, or managing industrial automation and control systems"@en ;
              dcterms:license sto:PrivateLicenseDocument ;
              rdfs:comment "Electronically secure Industrial Automation and Control Systems. Defines procedures for implementing electronically secure Industrial Automation and Control Systems."@en ,
                           "ISA/IEC-62443 is a series of standards, technical reports, and related information that define procedures for implementing electronically secure Industrial Automation and Control Systems (IACS). This guidance applies to end-users (i.e. asset owner), system integrators, security practitioners, and control systems manufacturers responsible for manufacturing, designing, implementing, or managing industrial automation and control systems."@en ;
              rdfs:label "IEC 62443"@en ;
              skos:hasTag "ISA 99"@en ;
              sto:alignsWith sto:Identification ;
              sto:hasDBpediaResource <http://dbpedia.org/page/Cyber_security_standards#ISA/IEC-62443_(formerly_ISA-99)> ;
              sto:hasOfficialResource <https://webstore.iec.ch/publication/7029> ,
                                      <https://webstore.iec.ch/publication/7033> ;
              sto:hasWikipediaArticle <https://en.wikipedia.org/wiki/Cyber_security_standards#ISA.2FIEC-62443_.28formerly_ISA-99.29> .


###  https://w3id.org/i40/sto#IEC_62453
sto:IEC_62453 rdf:type owl:NamedIndividual ,
                       sto:Standard ;
              dcterms:creator sto:irlan ;
              sto:hasClassification sto:AsConfiguration ,
                                    sto:RamiControlDevice ,
                                    sto:RamiFieldDevice ,
                                    sto:RamiStation ;
              sto:hasPublisher sto:IEC ;
              sto:relatedTo sto:DIN_SPEC_16592 ,
                            sto:IEC_61131 ,
                            sto:IEC_61360 ,
                            sto:IEC_61499 ,
                            sto:IEC_61804 ,
                            sto:IEC_61850 ,
                            sto:IEC_61987_X ,
                            sto:IEC_62424 ,
                            sto:IEC_62453 ,
                            sto:IEC_62541 ,
                            sto:IEC_62714 ,
                            sto:ISO_13584 ,
                            sto:ISO_14306 ,
                            sto:ISO_15746 ,
                            sto:ISO_15926 ,
                            sto:ISO_18629 ,
                            sto:ISO_18828-2 ,
                            sto:ISO_20922 ,
                            sto:ISO_22400 ,
                            sto:ISO_29002 ,
                            sto:ISO_ASTM_52915 ,
                            sto:ISO_PAS_17506 ,
                            sto:MathML ,
                            sto:SysML ,
                            sto:eClass ;
              sto:hasMotivation "FDT is an interface for integration of devices into a system (e.g. control system or engineering system). The standard supports factory automation as well as process automation with a wide range of fieldbus protocols. The interface defines fieldbus-independent mechanisms for accessing data and functions of the devices."@en ;
              sto:hasTag "FDT"@en ;
              rdfs:comment "Field device tool (FDT) interface specification - Overview and guidance"@en ;
              rdfs:label "IEC 62453"@en ;
              sto:hasOfficialResource <https://webstore.iec.ch/publication/7040> .


###  https://w3id.org/i40/sto#IEC_62541
sto:IEC_62541 rdf:type owl:NamedIndividual ,
                       sto:Standard ;
              sto:hasAvailableLanguage lang:eng ;
              sto:hasClassification sto:RamiCommunicationlayer ,
                                    sto:RamiConnectedWorld ,
                                    sto:RamiControlDevice ,
                                    sto:RamiEnterprise ,
                                    sto:RamiFieldDevice ,
                                    sto:RamiStation ,
                                    sto:RamiWorkCenter ,
                                    sto:SCADALevel ;
              sto:hasDeveloper sto:OPC_Foundation ;
              sto:hasDomain sto:IndustrialAutomation ;
              sto:hasPublisher sto:IEC ;
              sto:relatedTo sto:DIN_SPEC_16592 ,
                            sto:IEC_61131 ,
                            sto:IEC_61360 ,
                            sto:IEC_61499 ,
                            sto:IEC_61804 ,
                            sto:IEC_61850 ,
                            sto:IEC_61987_X ,
                            sto:IEC_62424 ,
                            sto:IEC_62453 ,
                            sto:IEC_62541 ,
                            sto:IEC_62714 ,
                            sto:ISO_13584 ,
                            sto:ISO_14306 ,
                            sto:ISO_15746 ,
                            sto:ISO_15926 ,
                            sto:ISO_18629 ,
                            sto:ISO_18828-2 ,
                            sto:ISO_20922 ,
                            sto:ISO_22400 ,
                            sto:ISO_29002 ,
                            sto:ISO_ASTM_52915 ,
                            sto:ISO_PAS_17506 ,
                            sto:MathML ,
                            sto:SysML ,
                            sto:eClass ;
              sto:useStructureOf sto:IEC_61804 ;
              sto:hasTag "OPC UA"@en ;
              dcterms:license sto:GPLv2 ,
                              sto:OpenLicenseDocument ;
              rdfs:comment "OPC Unified Architecture (OPC UA) is an industrial M2M communication protocol for interoperability developed by the OPC Foundation. It is the successor to Open Platform Communications (OPC). Although developed by the same organization, OPC UA differs significantly from its predecessor. The Foundation's goal for this project was to provide a path forward from the original OPC communications model (namely the Microsoft Windows only process exchange COM/DCOM) to a cross-platform service-oriented architecture (SOA) for process control, while enhancing security and providing an information model."@en ;
              rdfs:label "IEC 62541"@en ;
              sto:hasDBpediaResource <http://dbpedia.org/resource/OPC_Unified_Architecture> ;
              sto:hasRelevantDomain sto:IndustrialAutomation ;
              sto:hasOfficialResource <https://opcfoundation.org/about/opc-technologies/opc-ua/> ;
              sto:hasWikipediaArticle <https://en.wikipedia.org/wiki/OPC_Unified_Architecture> ;
              sto_iot:hasTargetConcern sto:AutonomousCommunication .


###  https://w3id.org/i40/sto#IEC_62591
sto:IEC_62591 rdf:type owl:NamedIndividual ,
                       sto:Standard ;
              dcterms:creator sto:irlan ;
              sto:hasPublisher sto:IEC ;
              rdfs:comment "Industrial networks - Wireless communication network and communication profiles."@en ;
              rdfs:label "IEC 62591"@en ;
              sto:hasDBpediaResource <http://dbpedia.org/page/WirelessHART> ;
              sto:hasOfficialResource <https://webstore.iec.ch/publication/24433> ;
              sto:hasWikipediaArticle <https://en.wikipedia.org/wiki/WirelessHART> .


###  https://w3id.org/i40/sto#IEC_62656
sto:IEC_62656 rdf:type owl:NamedIndividual ,
                       sto:Standard ;
              dcterms:creator sto:irlan ;
              sto:hasPublisher sto:IEC ;
              rdfs:comment "Specifies the logical structure for a set of spreadsheets, used as data parcels, to define, transfer and register product ontologies"@en ;
              rdfs:label "IEC 62656"@en ;
              sto:hasOfficialResource <https://webstore.iec.ch/publication/7326> .


###  https://w3id.org/i40/sto#IEC_62714
sto:IEC_62714 rdf:type owl:NamedIndividual ,
                       sto:Standard ;
              dcterms:creator sto:irlan ;
              sto:hasClassification sto:AsEngineering ,
                                    sto:ProductionSystemEngineering ,
                                    sto:RamiControlDevice ,
                                    sto:RamiFieldDevice ,
                                    sto:RamiInformationLayer ,
                                    sto:RamiProduct ;
              sto:hasPublisher sto:IEC ;
              sto:relatedTo sto:DIN_SPEC_16592 ,
                            sto:IEC_61131 ,
                            sto:IEC_61360 ,
                            sto:IEC_61499 ,
                            sto:IEC_61804 ,
                            sto:IEC_61850 ,
                            sto:IEC_61987_X ,
                            sto:IEC_62424 ,
                            sto:IEC_62453 ,
                            sto:ISO_13584 ,
                            sto:ISO_14306 ,
                            sto:ISO_15746 ,
                            sto:ISO_15926 ,
                            sto:ISO_18629 ,
                            sto:ISO_18828-2 ,
                            sto:ISO_20922 ,
                            sto:ISO_22400 ,
                            sto:ISO_29002 ,
                            sto:ISO_ASTM_52915 ,
                            sto:ISO_PAS_17506 ,
                            sto:SysML ,
                            sto:eClass ;
              sto:uses sto:MathML ;
              sto:hasTag "AML"@en ,
                         "AutomationML"@en ;
              dcterms:license sto:OpenLicenseDocument ;
              rdfs:comment "Engineering data exchange format for use in industrial automation systems engineering - Automation markup language - Architecture and general requirements"@en ;
              rdfs:label "IEC 62714"@en ;
              sto:hasDBpediaResource <http://dbpedia.org/resource/AutomationML> ;
              sto:hasOfficialResource <https://www.automationml.org/> ;
              sto:hasWikipediaArticle <https://en.wikipedia.org/wiki/AutomationML> .

sto:IEC_62769 rdf:type owl:NamedIndividual ,
                          sto:Standard ;
                 sto:hasPublisher sto:IEC ;
                 dcterms:title "Field device integration (FDI) "@en ;
                 rdfs:comment "IEC 62769 describes the concepts of the Field Device Integration (FDI) specifications."@en ;
                 rdfs:label "IEC 62769 "@en  .

###  https://w3id.org/i40/sto#IEC_62769_P1
sto:IEC_62769_P1 rdf:type owl:NamedIndividual ,
                          sto:Standard ;
                 dcterms:creator sto:irlan ;
                 sto:hasAvailableLanguage lang:eng ,
                                          lang:fra ;
                 sto:hasFileSize sto:FileSizeIEC_62769_P1 ;
                 sto:hasICS sto:ICS_25_040_40 ,
                            sto:ICS_35_100_05 ;
                 sto:hasPublisher sto:IEC ;
                 sto:hasTechnicalCommittee sto:TC_65 ;
                 sto:isPartOf sto:IEC_62769;
                 sto:hasEdition "1.0"^^xsd:float ;
                 sto:hasPages "64"^^xsd:int ;
                 sto:hasPublicationDate "2015-05-12"^^xsd:date ;
                 sto:hasStabilityDate "2019"^^xsd:gYear ;
                 sto:hasTag "IEC 62769-1:2015   "@en ;
                 dcterms:title "Field device integration (FDI) - Part 1: Overview"@en ;
                 rdfs:comment "IEC 62769-1:2015 describes the concepts and overview of the Field Device Integration (FDI) specifications. The detailed motivation for the creation of this technology is also described. It helps to understand the other parts of this multi-part standard."@en ;
                 rdfs:label "IEC 62769-1:2015  "@en ;
                 sto:hasOfficialResource <https://webstore.iec.ch/publication/22453> .


###  https://w3id.org/i40/sto#IEC_62794
sto:IEC_62794 rdf:type owl:NamedIndividual ,
                       sto:Standard ,
                       sto:TechnicalReport ;
              dcterms:creator sto:irlan ;
              sto:hasClassification sto:AdminShellGeneral,
                                    sto:RamiControlDevice ,
                                    sto:RamiFieldDevice ,
                                    sto:RamiStation ,
                                    sto:RamiWorkCenter ;
              sto:hasPublisher sto:IEC ;
              sto:relatedTo sto:IEC_62794 ,
                            sto:IEC_62832 ;
              sto:hasMotivation "The standards for Digital Factory define methods and information models, which are required for self description of I40-components. "@en ;
              sto:hasTag "DF/TR"@en ;
              dcterms:license sto:PrivateLicenseDocument ;
              rdfs:comment "Industrial-process measurement, control and automation - Reference model for representation of production facilities (digital factory)"@en ;
              rdfs:label "IEC TR 62794"@en ;
              sto:hasOfficialResource <https://webstore.iec.ch/publication/7433> .


###  https://w3id.org/i40/sto#IEC_62832
sto:IEC_62832 rdf:type owl:NamedIndividual ,
                       sto:Standard ,
                       sto:TechnicalSpecification ;
              dcterms:creator sto:irlan ;
              sto:hasAvailableLanguage lang:eng ;
              sto:hasClassification sto:AdminShellGeneral,
                                    sto:RamiControlDevice ,
                                    sto:RamiFieldDevice ,
                                    sto:RamiStation ,
                                    sto:RamiWorkCenter ;
              sto:hasFileSize sto:FileSizeIEC_62832 ;
              sto:hasICS sto:ICS_25_040_40 ;
              sto:hasPublisher sto:IEC ;
              sto:hasTechnicalCommittee sto:TC_65 ;
              sto:relatedTo sto:IEC_62794 ,
                            sto:IEC_62832 ;
              sto:hasEdition "1.0"^^xsd:float ;
              sto:hasPages "47"^^xsd:int ;
              sto:hasPublicationDate "2016-12-16"^^xsd:date ;
              sto:hasStabilityDate "2020"^^xsd:gYear ;
              rdfs:comment "Industrial-process measurement, control and automation - Digital factory framework - Part 1: General principles"@en ;
              rdfs:label "IEC TS 62832-1:2016 "@en ;
              sto:hasOfficialResource <https://webstore.iec.ch/publication/33023> .


###  https://w3id.org/i40/sto#IEC_62837
sto:IEC_62837 rdf:type owl:NamedIndividual ,
                       sto:Standard ;
              dcterms:creator sto:irlan ;
              sto:hasAvailableLanguage lang:eng ;
              sto:hasPublisher sto:IEC ;
              rdfs:comment "Provides to the technical committees a framework for the development and adaptation of documents in order to improve energy efficiency in manufacturing, process control and industrial facility management."@en ;
              rdfs:label "IEC 62837"@en ;
              sto:hasOfficialResource <https://webstore.iec.ch/publication/7446> .


###  https://w3id.org/i40/sto#IEC_62890
sto:IEC_62890 rdf:type owl:NamedIndividual ,
                       sto:Standard ;
              dcterms:creator sto:irlan ;
              sto:hasClassification sto:AsLifecycle_Status ,
                                    sto:ProductionLifeCycleDataManagement ,
                                    sto:RamiStation ,
                                    sto:RamiWorkCenter ;
              sto:hasPublisher sto:IEC ;
              sto:hasMotivation "Stations need to describe their operational state and performance parameters towards superior I4.0-Components"@en ;
              sto:hasTag "IEC 62890"@en ;
              dcterms:license sto:PrivateLicenseDocument ;
              rdfs:comment "Defines standards for lifecycle management for systems and products used in industrial process measurement, control and automation"@en ,
                           "MES KPIs"@en ;
              rdfs:label "IEC 62890"@en ;
              sto:hasOfficialResource <http://www.iec.ch/dyn/www/f?p=103:38:16824039984463::::FSP_ORG_ID,FSP_APEX_PAGE,FSP_PROJECT_ID:1250,23,20929> .


###  https://w3id.org/i40/sto#IEC_81714
sto:IEC_81714 rdf:type owl:NamedIndividual ,
                       sto:Standard ;
              dcterms:creator sto:irlan ,
                              sto:sebastian ;
              sto:hasClassification sto:AsEngineering ,
                                    sto:AsIdentification ,
                                    sto:ModelingPractice ,
                                    sto:RamiAssetlayer ,
                                    sto:RamiProduct ;
              sto:hasPublisher sto:IEC ,
                               sto:ISO ;
              sto:hasPublicationDate "2004-10-01"^^xsd:date ;
              rdfs:comment "ISO/IEC 81714 Design of graphical symbols for use in the technical documentation of products -- Part 3: Classification of connect nodes, networks and their encoding-- specifies requirements concerning the classification of connect nodes assigned to graphical symbols, being a representation of functional and product concepts."@en ;
              rdfs:label "IEC 81714"@en ;
              sto:hasRelevantDomain sto:CAD ;
              sto:hasOfficialResource <https://www.iso.org/standard/40134.html> .


###  https://w3id.org/i40/sto#IEC_PAS_63088
sto:IEC_PAS_63088 rdf:type owl:NamedIndividual ,
                           sto:Standard ;
                  dcterms:creator sto:irlan ;
                  sto:hasPublisher sto:IEC ;
                  sto:hasPublicationDate "2017-03-07"^^xsd:date ;
                  sto:hasTag "RAMI 4.0"^^xsd:string ;
                  rdfs:comment "IEC PAS 63088:2017(E) describes a reference architecture model in the form of a cubic layer model, RAMI model"@en ;
                  rdfs:label "IEC PAS 63088"@en ;
                  sto:hasOfficialResource <https://webstore.iec.ch/publication/30082?lipi=urn%3Ali%3Apage%3Ad_flagship3_pulse_read%3B2vZf0%2FOGS2CeRjny8ARziQ%3D%3D> .


###  https://w3id.org/i40/sto#IEC_TS_62832
sto:IEC_TS_62832 rdf:type owl:NamedIndividual ,
                          sto:TechnicalSpecification ;
                 sto:hasClassification sto:AdminShellGeneral,
                                       sto:RamiControlDevice ,
                                       sto:RamiFieldDevice ,
                                       sto:RamiStation ,
                                       sto:RamiWorkCenter ;
                 sto:hasPublisher sto:IEC ;
                 sto:hasMotivation "The standards for Digital Factory define methods and information models, which are required for self description of I40-components. IEC TS 62832 defines methods, which allow to validate or plan connections between assets."@en ;
                 sto:hasTag "DF/TS"@en ;
                 dcterms:license sto:PrivateLicenseDocument ;
                 rdfs:comment "Digital Factory Reference model TS"@en ;
                 rdfs:label "IEC TS 62832"@en ;
                 sto:hasOfficialResource <https://webstore.iec.ch/publication/33023> .

    <http://www.w3.org/2000/01/rdf-schema#label> "IEC 61223-2-6:2006" ;
    <https://w3id.org/i40/sto#hasAvailableLanguage> <http://lexvo.org/id/iso639-3/en>, <http://lexvo.org/id/iso639-3/es>, <http://lexvo.org/id/iso639-3/fr> ;
    <https://w3id.org/i40/sto#hasEdition> "2"^^<http://www.w3.org/2001/XMLSchema#float> ;
    <https://w3id.org/i40/sto#hasOfficialResource> <https://webstore.iec.ch/publication/4934> ;
    <https://w3id.org/i40/sto#hasPages> "34"^^<http://www.w3.org/2001/XMLSchema#int>, "67"^^<http://www.w3.org/2001/XMLSchema#int> ;
    <https://w3id.org/i40/sto#hasPublicationDate> "2006-11-28"^^<http://www.w3.org/2001/XMLSchema#date> ;
    <https://w3id.org/i40/sto#hasPublisher> <https://w3id.org/i40/sto#IEC> ;
    <https://w3id.org/i40/sto#hasStabilityDate> "2019-12-31"^^<http://www.w3.org/2001/XMLSchema#date> ;
    <https://w3id.org/i40/sto#hasStatus> "REPLACED" ;
    <https://w3id.org/i40/sto#hasTechnicalCommittee> "TC 62/SC 62B" ;
    <https://w3id.org/i40/sto#hasVersion> "1"^^<http://www.w3.org/2001/XMLSchema#float> .

<https://w3id.org/i40/sto#ISO-IEC-IEEE_21840-2019>
    <http://purl.org/dc/terms/creator> <https://w3id.org/i40/sto#crawler> ;
    <http://purl.org/dc/terms/modified> "2019-12-09"^^<http://www.w3.org/2001/XMLSchema#date> ;
    <http://purl.org/dc/terms/title> "Systems and software engineering - Guidelines for the utilization of ISO/IEC/IEEE 15288 in the context of system of systems (SoS)" ;
    a <http://www.w3.org/2002/07/owl#NamedIndividual>, <https://w3id.org/i40/sto#Standard> ;
    <http://www.w3.org/2000/01/rdf-schema#comment> """
    text/html
    <p>This document provides guidance on the application of processes in ISO/IEC/IEEE 15288 to systems of systems (SoS). The scope of this document is the same as ISO/IEC/IEEE 15288, which addresses more than systems engineering activities.<br />
NOTE 1 Throughout the document, there is mixed use of &quot;system of systems&quot; and &quot;systems of systems&quot;. &quot;SoS&quot; could refer to a system of systems or systems of systems. Similarly, &quot;CS&quot; could refer to a constituent system or constituent systems.<br />
This document provides general guidance for each ISO/IEC/IEEE 15288 process and process outcome in the context of SoS, but it does not address specific activities, tasks, methods, or procedures. Additional processes and process outcomes unique to SoS can still be needed and are not covered by this document.<br />
This document explores the similarities and differences between systems and SoS and, by extension, the similarities and differences between engineering of systems and SoS. The guidance contained in this document is expected to evolve as the discipline matures.<br />
NOTE 2 In many cases, this document notes that ISO/IEC/IEEE 15288 processes or process outcomes &quot;applies as stated to SoS.&quot; Some interpretation within the context of SoS can still be needed.</p>
  """ ;
    <http://www.w3.org/2000/01/rdf-schema#label> "ISO/IEC/IEEE 21840:2019" ;
    <https://w3id.org/i40/sto#hasAvailableLanguage> <http://lexvo.org/id/iso639-3/en> ;
    <https://w3id.org/i40/sto#hasEdition> "1"^^<http://www.w3.org/2001/XMLSchema#float> ;
    <https://w3id.org/i40/sto#hasOfficialResource> <https://webstore.iec.ch/publication/66237> ;
    <https://w3id.org/i40/sto#hasPages> "58"^^<http://www.w3.org/2001/XMLSchema#int> ;
    <https://w3id.org/i40/sto#hasPublicationDate> "2019-12-06"^^<http://www.w3.org/2001/XMLSchema#date> ;
    <https://w3id.org/i40/sto#hasPublisher> <https://w3id.org/i40/sto#ISO> ;
    <https://w3id.org/i40/sto#hasStatus> "PUBLISHED" ;
    <https://w3id.org/i40/sto#hasTechnicalCommittee> "ISO/IEC JTC 1/SC 7" ;
    <https://w3id.org/i40/sto#hasVersion> "1"^^<http://www.w3.org/2001/XMLSchema#float> .

<https://w3id.org/i40/sto#ISO-IEC_10918-7-2019>
    <http://purl.org/dc/terms/creator> <https://w3id.org/i40/sto#crawler> ;
    <http://purl.org/dc/terms/modified> "2019-12-09"^^<http://www.w3.org/2001/XMLSchema#date> ;
    <http://purl.org/dc/terms/title> "Information technology - Digital compression and coding of continuous-tone still images - Part 7: Reference software" ;
    a <http://www.w3.org/2002/07/owl#NamedIndividual>, <https://w3id.org/i40/sto#Standard> ;
    <http://www.w3.org/2000/01/rdf-schema#comment> """
    text/html
    <p>This Specification provides reference software for the coding technology specified in Recommendation ITU-T T.81 | ISO/IEC 10918-1. While the reference implementations also provide an encoder, conformance testing of their encoding process is beyond the scope of this Specification.</p>
  """ ;
    <http://www.w3.org/2000/01/rdf-schema#label> "ISO/IEC 10918-7:2019" ;
    <https://w3id.org/i40/sto#hasAvailableLanguage> <http://lexvo.org/id/iso639-3/en> ;
    <https://w3id.org/i40/sto#hasEdition> "1"^^<http://www.w3.org/2001/XMLSchema#float> ;
    <https://w3id.org/i40/sto#hasOfficialResource> <https://webstore.iec.ch/publication/66236> ;
    <https://w3id.org/i40/sto#hasPages> "13"^^<http://www.w3.org/2001/XMLSchema#int> ;
    <https://w3id.org/i40/sto#hasPublicationDate> "2019-12-02"^^<http://www.w3.org/2001/XMLSchema#date> ;
    <https://w3id.org/i40/sto#hasPublisher> <https://w3id.org/i40/sto#ISO> ;
    <https://w3id.org/i40/sto#hasStatus> "PUBLISHED" ;
    <https://w3id.org/i40/sto#hasTechnicalCommittee> "ISO/IEC JTC 1/SC 29" ;
    <https://w3id.org/i40/sto#hasVersion> "1"^^<http://www.w3.org/2001/XMLSchema#float> .



###  https://w3id.org/i40/sto#IEEE
sto:IEEE rdf:type owl:NamedIndividual ,
                  foaf:Organization ,
                  sto:StandardOrganization ;
         sto:abbreviation "IEEE"@en ;
         sto:orgName "Institute of Electrical and Electronics Engineers"@en ;
         dcterms:description "IEEE and its members inspire a global community to innovate for a better tomorrow through highly cited publications, conferences, technology standards, and professional and educational activities. IEEE is the trusted “voice” for engineering, computing, and technology information around the globe."@en ;
         rdfs:seeAlso <https://www.ieee.org/> ;
         sto:hasWikipediaArticle <http://wikipedia.org/wiki/Institute_of_Electrical_and_Electronics_Engineers> .


###  https://w3id.org/i40/sto#IEEE_1377-2012
sto:IEEE_1377-2012 rdf:type owl:NamedIndividual ,
                            sto:Standard ;
                   dcterms:creator sto:sebastian ;
              sto:hasPublisher sto:IEEE ;
                   rdfs:comment "IEEE Standard for Utility Industry Metering Communication Protocol Application Layer (source: https://www.postscapes.com/internet-of-things-protocols/)"@en ;
                   rdfs:label "IEEE 1377-2012"@en ;
                   sto:hasOfficialResource <http://standards.ieee.org/findstds/standard/1377-2012.html> .


###  https://w3id.org/i40/sto#IEEE_1451
sto:IEEE_1451 rdf:type owl:NamedIndividual ,
                       sto:Standard ;
              dcterms:creator sto:sebastian ;
              rdfs:comment "The IEEE 1451, a family of Smart Transducer Interface Standards, describes a set of open, common, network-independent communication interfaces for connecting transducers (sensors or actuators) to microprocessors, instrumentation systems, and control/field networks. (source: https://www.postscapes.com/internet-of-things-protocols/)"@en ;
              rdfs:label "IEEE 1451"@en ;
              sto:hasPublisher sto:IEEE ;
              sto:hasOfficialResource <http://grouper.ieee.org/groups/1451/0/body%20frame_files/Family-of-1451_handout.htm> .


###  https://w3id.org/i40/sto#IEEE_1686
sto:IEEE_1686 rdf:type owl:NamedIndividual ,
                       sto:Standard ;
              dcterms:creator sto:irlan ,
                              sto:sebastian ;
              sto:hasClassification sto:IDSRAMSecurity ;
              sto:hasDeveloper sto:IEEE ;
              sto:hasPublisher sto:IEEE ;
              dcterms:title "Standard for Intelligent Electronic Devices Cyber Security Capabilities"@en ;
              rdfs:comment "The functions and features to be provided in intelligent electronic devices (IEDs) to accommodate critical infrastructure protection programs are defined in this standard. Security regarding the access, operation, configuration, firmware revision and data retrieval from an IED are addressed. Communications for the purpose of power system protection (teleprotection) are not addressed in this standard."@en ;
              rdfs:label "IEEE 1686"@en ;
              sto:hasDBpediaResource <http://dbpedia.org/resource/IEEE_Smart_Grid> ;
              sto:hasOfficialResource <https://standards.ieee.org/standard/1686-2007.html> ;
              sto:hasWikipediaArticle <https://en.wikipedia.org/wiki/IEEE_Smart_Grid> .


###  https://w3id.org/i40/sto#IEEE_1856
sto:IEEE_1856 rdf:type owl:NamedIndividual ,
                       sto:Standard ;
              dcterms:creator sto:sebastian ;
              sto:hasPublisher sto:IEEE ;
              rdfs:comment "Standard Framework for Prognostics and Health Management of Electronic Systems (source: https://www.postscapes.com/internet-of-things-protocols/)"@en ;
              rdfs:label "IEEE 1856"@en ;
              sto:hasOfficialResource <http://standards.ieee.org/develop/project/1856.html> .


###  https://w3id.org/i40/sto#IEEE_1888-3-2013
sto:IEEE_1888-3-2013 rdf:type owl:NamedIndividual ,
                              sto:Standard ;
                     dcterms:creator sto:sebastian ;
              sto:hasPublisher sto:IEEE ;
                     rdfs:comment " - IEEE Standard for Ubiquitous Green Community Control Network: Security (source: https://www.postscapes.com/internet-of-things-protocols/)"@en ;
                     rdfs:label "IEEE 1888.3-2013"@en ;
                     sto:hasOfficialResource <http://standards.ieee.org/findstds/standard/1888.3-2013.html> .


###  https://w3id.org/i40/sto#IEEE_1905_1-2013
sto:IEEE_1905_1-2013 rdf:type owl:NamedIndividual ,
                              sto:Standard ;
                     dcterms:creator sto:sebastian ;
              sto:hasPublisher sto:IEEE ;
                     rdfs:comment "IEEE Standard for a Convergent Digital Home Network for Heterogeneous Technologies (source: https://www.postscapes.com/internet-of-things-protocols/)"@en ;
                     rdfs:label "IEEE 1905.1-2013"@en ;
                     sto:hasOfficialResource <http://standards.ieee.org/findstds/standard/1905.1-2013.html> .


###  https://w3id.org/i40/sto#IEEE_2413
sto:IEEE_2413 rdf:type owl:NamedIndividual ,
                       sto:Standard ;
              dcterms:creator sto:sebastian ;
              sto:hasPublisher sto:IEEE ;
              rdfs:comment "IEEE P2413 - Standard for an Architectural Framework for the Internet of Things (IoT) (source: https://www.postscapes.com/internet-of-things-protocols/)"@en ;
              rdfs:label "IEEE 2413"@en ;
              sto:hasOfficialResource <https://standards.ieee.org/develop/project/2413.html> .


###  https://w3id.org/i40/sto#IEEE_42010
sto:IEEE_42010 rdf:type owl:NamedIndividual, 
               sto:Standard ;
               rdfs:label "IEEE 42010"^^xsd:string ;       
              sto:hasPublisher sto:IEEE ;       
               rdfs:comment "ISO/IEC/IEEE 42010:2011 defines requirements on the description of system, software and enterprise architectures. It aims to standardise the practice of architecture description by defining standard terms, presenting a conceptual foundation for expressing, communicating and reviewing architectures and specifying requirements that apply to architecture descriptions, architecture frameworks and architecture description languages."@en ;
               owl:sameAs sto:ISO_42010 .


###  https://w3id.org/i40/sto#IEEE_802
sto:IEEE_802 rdf:type owl:NamedIndividual ,
                      sto:Standard ;
             dcterms:creator sto:irlan ,
                             sto:sebastian ;
              sto:hasPublisher sto:IEEE ;
             rdfs:comment "IEEE 802.15.4 is a standard which specifies the physical layer and media access control for low-rate wireless personal area networks (LR-WPANs). It is maintained by the IEEE 802.15 working group. It is the basis for the ZigBee,ISA100.11a, WirelessHART, and MiWi specifications, each of which further extends the standard by developing the upper layers which are not defined in IEEE 802.15.4. Alternatively, it can be used with 6LoWPAN and standard Internet protocols to build a wireless embedded Internet. (source: https://www.postscapes.com/internet-of-things-protocols/)"@en ;
             rdfs:label "IEEE 802.15.4"@en ;
             sto:hasDBpediaResource <http://dbpedia.org/page/IEEE_802.15.4> ;
             sto:hasWikipediaArticle <https://en.wikipedia.org/wiki/IEEE_802.15.4> .


###  https://w3id.org/i40/sto#IEEE_802_16-2012
sto:IEEE_802_16-2012 rdf:type owl:NamedIndividual ,
                              sto:Standard ;
                     dcterms:creator sto:sebastian ;
              sto:hasPublisher sto:IEEE ;
                     rdfs:comment "IEEE Standard for Air Interface for Broadband Wireless Access Systems (source: https://www.postscapes.com/internet-of-things-protocols/)"@en ;
                     rdfs:label "IEEE 802.16p-2012"@en ;
                     sto:hasOfficialResource <http://standards.ieee.org/findstds/standard/802.16p-2012.html> .


###  https://w3id.org/i40/sto#IEEE_P1828
sto:IEEE_P1828 rdf:type owl:NamedIndividual ,
                        sto:Standard ;
               dcterms:creator sto:sebastian ;
              sto:hasPublisher sto:IEEE ;
               rdfs:comment "Standard for Systems With Virtual Components (source: https://www.postscapes.com/internet-of-things-protocols/)"@en ;
               rdfs:label "IEEE P1828"@en ;
               sto:hasOfficialResource <http://standards.ieee.org/develop/project/1828.html> .


###  https://w3id.org/i40/sto#IETF
sto:IETF rdf:type owl:NamedIndividual ,
                  sto:StandardOrganization ;
         sto:abbreviation "IETF"@en ;
         sto:orgName "Internet Engineering Task Force"@en ;
         rdfs:comment "TODO: complete annotations etc."@en ;
         rdfs:label "IETF"@en ;
         rdfs:seeAlso <http://wikipedia.org/wiki/Internet_Engineering_Task_Force> ,
                      <http://www.ietf.org/> ;
         sto:hasWikipediaArticle <http://wikipedia.org/wiki/Internet_Engineering_Task_Force> .


###  https://w3id.org/i40/sto#IIC
sto:IIC rdf:type owl:NamedIndividual ,
                 foaf:Organization ,
                 sto:IIoTConsortium ,
                 sto:StandardOrganization ;
        dcterms:creator sto:sebastian ;
        dul:associatedWith sto:IIRA ;
        rdfs:comment "Founded in 2014 to further development, adoption and wide-spread use of interconnected machines, intelligent analytics and people at work. (source: https://www.postscapes.com/internet-of-things-protocols/)"@en ;
        rdfs:label "IIC"@en ,
                   "Industrial Internet Consortium"@en ;
        sto:hasOfficialResource <http://www.iiconsortium.org/> .


###  https://w3id.org/i40/sto#IICF
sto:IICF rdf:type owl:NamedIndividual ,
                  foaf:Document ,
                  sto:Publication ;
         sto:hasClassification sto:IIRAConnectivity ;
         dcterms:title "Industrial Internet Connectivity Framework"@en ;
         rdfs:isDefinedBy <https://www.iiconsortium.org/IICF.htm> ;
         rdfs:label "IICF"@en ;
         rdfs:seeAlso <https://www.iiconsortium.org/pdf/IIC_PUB_G5_V1.01_PB_20180228.pdf> .


###  https://w3id.org/i40/sto#IICFFrameworkLayer
sto:IICFFrameworkLayer rdf:type owl:NamedIndividual ,
                                sto:IicfConnectivityLayer ,
                                sto:StandardClassification ;
                       dul:associatedWith sto:DDS ,
                                          sto:IDSRAMGovernance ,
                                          sto:IDSRAMSystemLayer ,
                                          sto:IEC_62541 ,
                                          sto:oneM2M ,
                                          <https://www.wikidata.org/wiki/Q1548249> ;
                       dul:isPartOf sto:IIRAConnectivity ;
                       sto_iot:alignsWith sto:IDSRAMGovernance ,
                                          sto:IDSRAMSystemLayer ;
                       sto_iot:frames sto:Authentication ,
                                      sto:Communication ,
                                      sto:DataAccess ,
                                      sto:DataDiscovery ,
                                      sto:Governance ,
                                      sto:Identification ,
                                      sto:IdentityManagement ,
                                      sto:IntegrityProtection ,
                                      sto:Interoperability ,
                                      sto:QualityOfService ,
                                      sto:SecureCommunication ,
                                      sto:Security ,
                                      sto:SemanticInteroperability ,
                                      sto:ServiceDescription ,
                                      sto:ServiceDiscovery ,
                                      sto:SyntacticInteroperability ,
                                      sto:Trustworthiness ;
                       rdfs:comment "IICF Framework Layer"@en ,
                                    "IICF Framework Layer an instance of the IICF Connectivity Layer"@en ;
                       rdfs:isDefinedBy <https://www.iiconsortium.org/pdf/IIC_PUB_G5_V1.01_PB_20180228.pdf> ;
                       rdfs:label "IICF Framework Layer"@en .


###  https://w3id.org/i40/sto#IICFFrameworkLayerAnno
sto:IICFFrameworkLayerAnno rdf:type owl:NamedIndividual ,
                                    oa:Annotation ;
                           oa:hasBody sto:IICFFrameworkLayer ;
                           oa:hasTarget [ rdf:type oa:SpecificResource ;
                                          dcterms:format "pdf" ;
                                          oa:hasSelector [ rdf:type oa:RangeSelector ;
                                                           oa:hasEndSelector [ rdf:type oa:XPathSelector ;
                                                                               rdf:value "Page 17"
                                                                             ] ;
                                                           oa:hasStartSelector [ rdf:type oa:XPathSelector ;
                                                                                 rdf:value "Page 14"
                                                                               ]
                                                         ] ;
                                          oa:hasSource sto:The_Industrial_Internet_of_Things_Volume_G5_Connectivity_Framework
                                        ] ,
                                        [ rdf:type oa:SpecificResource ;
                                          dcterms:format "pdf" ;
                                          oa:hasSelector [ rdf:type oa:RangeSelector ;
                                                           oa:hasEndSelector [ rdf:type oa:XPathSelector ;
                                                                               rdf:value "Page 17"
                                                                             ] ;
                                                           oa:hasStartSelector [ rdf:type oa:XPathSelector ;
                                                                                 rdf:value "Page 14"
                                                                               ]
                                                         ] ;
                                          oa:hasSource sto:The_Industrial_Internet_of_Things_Volume_G5_Connectivity_Framework
                                        ] .


###  https://w3id.org/i40/sto#IICFLinkLayer
sto:IICFLinkLayer rdf:type owl:NamedIndividual ,
                           sto:IicfConnectivityLayer ,
                           sto:StandardClassification ;
                  dul:associatedWith sto:IEEE_802 ,
                                     sto:IEEE_802_16-2012 ,
                                     sto:WiFi ;
                  dul:isPartOf sto:IIRAConnectivity ;
                  sto_iot:frames sto:Communication ;
                  rdfs:label "IICF Link Layer"@en .


###  https://w3id.org/i40/sto#IICFLinkLayerAnno
sto:IICFLinkLayerAnno rdf:type owl:NamedIndividual ,
                               oa:Annotation ;
                      oa:hasBody sto:IICFLinkLayer ;
                      oa:hasTarget [ rdf:type oa:SpecificResource ;
                                     dcterms:format "pdf" ;
                                     oa:hasSelector [ rdf:type oa:RangeSelector ;
                                                      oa:hasEndSelector [ rdf:type oa:XPathSelector ;
                                                                          rdf:value "Page 17"
                                                                        ] ;
                                                      oa:hasStartSelector [ rdf:type oa:XPathSelector ;
                                                                            rdf:value "Page 14"
                                                                          ]
                                                    ] ;
                                     oa:hasSource sto:The_Industrial_Internet_of_Things_Volume_G5_Connectivity_Framework
                                   ] ,
                                   [ rdf:type oa:SpecificResource ;
                                     dcterms:format "pdf" ;
                                     oa:hasSelector [ rdf:type oa:RangeSelector ;
                                                      oa:hasEndSelector [ rdf:type oa:XPathSelector ;
                                                                          rdf:value "Page 17"
                                                                        ] ;
                                                      oa:hasStartSelector [ rdf:type oa:XPathSelector ;
                                                                            rdf:value "Page 14"
                                                                          ]
                                                    ] ;
                                     oa:hasSource sto:The_Industrial_Internet_of_Things_Volume_G5_Connectivity_Framework
                                   ] .


###  https://w3id.org/i40/sto#IICFNetworkLayer
sto:IICFNetworkLayer rdf:type owl:NamedIndividual ,
                              sto:IicfConnectivityLayer ,
                              sto:StandardClassification ;
                     dul:associatedWith sto:IPv6 ;
                     dul:isPartOf sto:IIRAConnectivity ;
                     sto_iot:frames sto:Communication ,
                                    sto:IPv4Support ,
                                    sto:IPv6Support ,
                                    sto:Interoperability ,
                                    sto:SyntacticInteroperability ;
                     rdfs:label "IICF Network Layer"@en .


###  https://w3id.org/i40/sto#IICFNetworkLayerAnno
sto:IICFNetworkLayerAnno rdf:type owl:NamedIndividual ,
                                  oa:Annotation ;
                         oa:hasBody sto:IICFNetworkLayer ;
                         oa:hasTarget [ rdf:type oa:SpecificResource ;
                                        dcterms:format "pdf" ;
                                        oa:hasSelector [ rdf:type oa:RangeSelector ;
                                                         oa:hasEndSelector [ rdf:type oa:XPathSelector ;
                                                                             rdf:value "Page 17"
                                                                           ] ;
                                                         oa:hasStartSelector [ rdf:type oa:XPathSelector ;
                                                                               rdf:value "Page 14"
                                                                             ]
                                                       ] ;
                                        oa:hasSource sto:The_Industrial_Internet_of_Things_Volume_G5_Connectivity_Framework
                                      ] ,
                                      [ rdf:type oa:SpecificResource ;
                                        dcterms:format "pdf" ;
                                        oa:hasSelector [ rdf:type oa:RangeSelector ;
                                                         oa:hasEndSelector [ rdf:type oa:XPathSelector ;
                                                                             rdf:value "Page 17"
                                                                           ] ;
                                                         oa:hasStartSelector [ rdf:type oa:XPathSelector ;
                                                                               rdf:value "Page 14"
                                                                             ]
                                                       ] ;
                                        oa:hasSource sto:The_Industrial_Internet_of_Things_Volume_G5_Connectivity_Framework
                                      ] .


###  https://w3id.org/i40/sto#IICFPhysicalLayer
sto:IICFPhysicalLayer rdf:type owl:NamedIndividual ,
                               sto:IicfConnectivityLayer ,
                               sto:StandardClassification ;
                      dul:associatedWith sto:IEEE_802 ,
                                         sto:IEEE_802_16-2012 ;
                      dul:isPartOf sto:IIRAConnectivity ;
                      sto_iot:frames sto:Communication ;
                      rdfs:label "IICF Physical Layer" .


###  https://w3id.org/i40/sto#IICFPhysicalLayerAnno
sto:IICFPhysicalLayerAnno rdf:type owl:NamedIndividual ,
                                   oa:Annotation ;
                          oa:hasBody sto:IICFPhysicalLayer ;
                          oa:hasTarget [ rdf:type oa:SpecificResource ;
                                         dcterms:format "pdf" ;
                                         oa:hasSelector [ rdf:type oa:RangeSelector ;
                                                          oa:hasEndSelector [ rdf:type oa:XPathSelector ;
                                                                              rdf:value "Page 17"
                                                                            ] ;
                                                          oa:hasStartSelector [ rdf:type oa:XPathSelector ;
                                                                                rdf:value "Page 14"
                                                                              ]
                                                        ] ;
                                         oa:hasSource sto:The_Industrial_Internet_of_Things_Volume_G5_Connectivity_Framework
                                       ] ,
                                       [ rdf:type oa:SpecificResource ;
                                         dcterms:format "pdf" ;
                                         oa:hasSelector [ rdf:type oa:RangeSelector ;
                                                          oa:hasEndSelector [ rdf:type oa:XPathSelector ;
                                                                              rdf:value "Page 17"
                                                                            ] ;
                                                          oa:hasStartSelector [ rdf:type oa:XPathSelector ;
                                                                                rdf:value "Page 14"
                                                                              ]
                                                        ] ;
                                         oa:hasSource sto:The_Industrial_Internet_of_Things_Volume_G5_Connectivity_Framework
                                       ] .


###  https://w3id.org/i40/sto#IICFTansportLayer
sto:IICFTansportLayer rdf:type owl:NamedIndividual ,
                               sto:IicfConnectivityLayer ,
                               sto:StandardClassification ;
                      dul:associatedWith sto:HTTP ,
                                         sto:HTTP2 ,
                                         sto:IEC_61158 ,
                                         sto:ISO_20922 ,
                                         sto:RFC_2616 ,
                                         sto:RFC_793 ,
                                         sto:RFC_8323 ,
                                         sto:UDP ;
                      dul:isPartOf sto:IIRAConnectivity ;
                      sto_iot:frames sto:CardinalityOfDataSources ,
                                     sto:CardinalityOfParticipants ,
                                     sto:Communication ,
                                     sto:EndpointInvocation ,
                                     sto:Interoperability ,
                                     sto:Multilaterism ,
                                     sto:SecureCommunication ,
                                     sto:Security ,
                                     sto:ServiceComposition ,
                                     sto:SyntacticInteroperability ,
                                     sto:TimeSynchronization ,
                                     sto:Trustworthiness ,
                                     sto:Unicast ;
                      rdfs:label "IICF Transport Layer"@en .


###  https://w3id.org/i40/sto#IICFTansportLayerAnno
sto:IICFTansportLayerAnno rdf:type owl:NamedIndividual ,
                                   oa:Annotation ;
                          oa:hasBody sto:IICFTansportLayer ;
                          oa:hasTarget [ rdf:type oa:SpecificResource ;
                                         dcterms:format "pdf" ;
                                         oa:hasSelector [ rdf:type oa:RangeSelector ;
                                                          oa:hasEndSelector [ rdf:type oa:XPathSelector ;
                                                                              rdf:value "Page 17"
                                                                            ] ;
                                                          oa:hasStartSelector [ rdf:type oa:XPathSelector ;
                                                                                rdf:value "Page 14"
                                                                              ]
                                                        ] ;
                                         oa:hasSource sto:The_Industrial_Internet_of_Things_Volume_G5_Connectivity_Framework
                                       ] ,
                                       [ rdf:type oa:SpecificResource ;
                                         dcterms:format "pdf" ;
                                         oa:hasSelector [ rdf:type oa:RangeSelector ;
                                                          oa:hasEndSelector [ rdf:type oa:XPathSelector ;
                                                                              rdf:value "Page 17"
                                                                            ] ;
                                                          oa:hasStartSelector [ rdf:type oa:XPathSelector ;
                                                                                rdf:value "Page 14"
                                                                              ]
                                                        ] ;
                                         oa:hasSource sto:The_Industrial_Internet_of_Things_Volume_G5_Connectivity_Framework
                                       ] .


###  https://w3id.org/i40/sto#IICVocabulary
sto:IICVocabulary rdf:type owl:NamedIndividual ,
                           foaf:Document ,
                           sto:Publication ,
                           sto:StandardClassification ;
                  dcterms:creator sto:IIC ,
                                  sto:sebastian ;
                  dul:associatedWith sto:IDSRAMInformationLayer ;
                  foaf:maker sto:IIC ;
                  sto:hasPublisher sto:IIC ;
                  sto:isDescribedin sto:IIRA ;
                  sto_iot:alignsWith sto:IDSRAMInformationLayer ;
                  rdfs:label "IIC Vocabulary"@en .


###  https://w3id.org/i40/sto#IIC_PUB_G1_V1_80_20170131
sto:IIC_PUB_G1_V1_80_20170131 rdf:type owl:NamedIndividual ,
                                       oa:SpecificResource ;
                              rdfs:label "The Industrial Internet of Things Volume G1: Reference Architecture IIC:PUB:G1:V1.80:20170131"@en ;
                              sto:hasOpenResource <https://www.iiconsortium.org/IIC_PUB_G1_V1.80_2017-01-31.pdf> .


###  https://w3id.org/i40/sto#IIRA
sto:IIRA rdf:type owl:NamedIndividual ,
                  sto:ArchitectureDescription ,
                  sto:StandardizationFramework ;
         sto:hasPublisher sto:IIC ;
         rdfs:comment "The IIRA addresses the need for a common architecture framework to develop interoperable IIoT systems for diverse applications across a broad spectrum of industrial verticals in the public and private sectors to achieve the true promise of IIoT."@en ;
         rdfs:label "Industrial Internet Reference Architecture"@en ;
         skos:altLabel "IIRA" ;
         skos:note "Publications referred: 1. The Industrial Internet of Things Volume G1: Reference Architecture (IIC:PUB:G1:V1.80:20170131)" ;
         sto:hasOfficialResource <http://www.iiconsortium.org/IIRA.htm> ;
         sto_iot:hasTargetConcern <http://purl.oclc.org/NET/mvco.owl#EndUser> ,
                                  sto:BusinessValue ,
                                  sto:DecisionMaker ,
                                  sto:Developer ,
                                  sto:MaintenanceCost ,
                                  sto:ProductLiability ,
                                  sto:ProductManager ,
                                  sto:ReturnOnInvestment ,
                                  sto:SystemEngineer ,
                                  sto:SystemOperator ,
                                  <https://www.wikidata.org/wiki/Q1548249> .


###  https://w3id.org/i40/sto#IIRAApplicationDomain
sto:IIRAApplicationDomain rdf:type owl:NamedIndividual ,
                                   sto:IIRAFunctionalDomain ,
                                   sto:StandardClassification ;
                          dcterms:creator sto:sebastian ;
                          dul:associatedWith sto:BdvaCloudAndHighPerformanceComputing ,
                                             sto:EdgecrossItSystemsLayer ,
                                             sto:FiwareAdvancedUi ,
                                             sto:FiwareCloudHosting ,
                                             sto:IDSRAMProcessLayer ,
                                             sto:RAMIFunctionalLayer ,
                                             sto:RAMIInformationLayer ;
                          dul:isPartOf sto:IIRAFunctionalViewpoint ;
                          sto:isDescribedin sto:IIRA ;
                          sto_iot:alignsWith sto:BdvaCloudAndHighPerformanceComputing ,
                                             sto:EdgecrossItSystemsLayer ,
                                             sto:FiwareAdvancedUi ,
                                             sto:FiwareCloudHosting ,
                                             sto:IDSRAMProcessLayer ,
                                             sto:RAMIFunctionalLayer ,
                                             sto:RAMIInformationLayer ;
                          sto_iot:frames sto:BdvaDataViualisationAndUserInteraction ,
                                         sto:DataProcessing ,
                                         sto:EndpointInvocation ,
                                         sto:Interoperability ,
                                         sto:SyntacticInteroperability ;
                          rdfs:label "IIRA Application Domain"@en ;
                          skos:note "Publications referred: 'IIC:PUB:G1:V1.80:20170131' '6.4 THE APPLICATION DOMAIN' 'Page 34' " .


###  https://w3id.org/i40/sto#IIRAApplicationDomainAnno
sto:IIRAApplicationDomainAnno rdf:type owl:NamedIndividual ,
                                       oa:Annotation ;
                              oa:hasBody sto:IIRAApplicationDomain ;
                              oa:hasTarget [ rdf:type oa:SpecificResource ;
                                             dcterms:format "pdf" ;
                                             oa:hasSelector [ rdf:type oa:RangeSelector ;
                                                              oa:hasEndSelector [ rdf:type oa:XPathSelector ;
                                                                                  rdf:value "Page 35"
                                                                                ] ;
                                                              oa:hasStartSelector [ rdf:type oa:XPathSelector ;
                                                                                    rdf:value "Page 34"
                                                                                  ]
                                                            ] ;
                                             oa:hasSource sto:The_Industrial_Internet_of_Things_Volume_G1_Reference_Architecture
                                           ] ,
                                           [ rdf:type oa:SpecificResource ;
                                             dcterms:format "pdf" ;
                                             oa:hasSelector [ rdf:type oa:RangeSelector ;
                                                              oa:hasEndSelector [ rdf:type oa:XPathSelector ;
                                                                                  rdf:value "Page 35"
                                                                                ] ;
                                                              oa:hasStartSelector [ rdf:type oa:XPathSelector ;
                                                                                    rdf:value "Page 34"
                                                                                  ]
                                                            ] ;
                                             oa:hasSource sto:The_Industrial_Internet_of_Things_Volume_G1_Reference_Architecture
                                           ] .


###  https://w3id.org/i40/sto#IIRABusinessDomain
sto:IIRABusinessDomain rdf:type owl:NamedIndividual ,
                                sto:IIRAFunctionalDomain ,
                                sto:StandardClassification ;
                       dcterms:creator sto:sebastian ;
                       dul:associatedWith sto:IDSRAMBusinessLayer ,
                                          sto:OceanSystemViewpoint ,
                                          sto:RAMIBusinessLayer ;
                       dul:isPartOf sto:IIRAFunctionalViewpoint ;
                       sto:isDescribedin sto:IIRA ;
                       sto_iot:alignsWith sto:IDSRAMBusinessLayer ,
                                          sto:OceanSystemViewpoint ,
                                          sto:RAMIBusinessLayer ;
                       sto_iot:frames sto:AsProcessPlanning ;
                       rdfs:label "IIRA Business Domain"@en ;
                       skos:note "Publications referred: 'IIC:PUB:G1:V1.80:20170131' '6.5 THE BUSINESS DOMAIN' 'Page 34' " .


###  https://w3id.org/i40/sto#IIRABusinessDomainAnno
sto:IIRABusinessDomainAnno rdf:type owl:NamedIndividual ,
                                    oa:Annotation ;
                           oa:hasBody sto:IIRABusinessDomain ;
                           oa:hasTarget [ rdf:type oa:SpecificResource ;
                                          dcterms:format "pdf" ;
                                          oa:hasSelector [ rdf:type oa:RangeSelector ;
                                                           oa:hasEndSelector [ rdf:type oa:XPathSelector ;
                                                                               rdf:value "Page 35"
                                                                             ] ;
                                                           oa:hasStartSelector [ rdf:type oa:XPathSelector ;
                                                                                 rdf:value "Page 34"
                                                                               ]
                                                         ] ;
                                          oa:hasSource sto:The_Industrial_Internet_of_Things_Volume_G1_Reference_Architecture
                                        ] ,
                                        [ rdf:type oa:SpecificResource ;
                                          dcterms:format "pdf" ;
                                          oa:hasSelector [ rdf:type oa:RangeSelector ;
                                                           oa:hasEndSelector [ rdf:type oa:XPathSelector ;
                                                                               rdf:value "Page 35"
                                                                             ] ;
                                                           oa:hasStartSelector [ rdf:type oa:XPathSelector ;
                                                                                 rdf:value "Page 34"
                                                                               ]
                                                         ] ;
                                          oa:hasSource sto:The_Industrial_Internet_of_Things_Volume_G1_Reference_Architecture
                                        ] .


###  https://w3id.org/i40/sto#IIRABusinessViewpoint
sto:IIRABusinessViewpoint rdf:type owl:NamedIndividual ,
                                   sto:StandardClassification ,
                                   sto:Viewpoint ;
                          dcterms:creator sto:sebastian ;
                          dul:associatedWith sto:IviBusinessLayer ,
                                             sto:OceanBusinessViewpoint ,
                                             sto:OceanMarketplaceViewpoint ;
                          sto:isDescribedin sto:IIRA ;
                          sto_iot:alignsWith sto:IviBusinessLayer ,
                                             sto:OceanBusinessViewpoint ,
                                             sto:OceanMarketplaceViewpoint ;
                          sto_iot:frames sto:BusinessContext ,
                                         sto:BusinessValue ,
                                         sto:MaintenanceCost ,
                                         sto:ProductLiability ,
                                         sto:Resilience ,
                                         sto:ReturnOnInvestment ,
                                         sto:Safety ,
                                         sto:Security ,
                                         sto:Trustworthiness ;
                          rdfs:comment "The business viewpoint frames economic aspects and business relations regarded by the IIC Reference Architecture."@en ;
                          rdfs:label "IIRA Business Viewpoint"@en ;
                          skos:note "Publications referred: '(IIC:PUB:G1:V1.80:20170131' '3.5.1 BUSINESS VIEWPOINT' 'Page 15' " .


###  https://w3id.org/i40/sto#IIRABusinessViewpointAnno
sto:IIRABusinessViewpointAnno rdf:type owl:NamedIndividual ,
                                       oa:Annotation ;
                              oa:hasBody sto:IIRABusinessViewpoint ;
                              oa:hasTarget [ rdf:type oa:SpecificResource ;
                                             dcterms:format "pdf" ;
                                             oa:hasSelector [ rdf:type oa:RangeSelector ;
                                                              oa:hasEndSelector [ rdf:type oa:XPathSelector ;
                                                                                  rdf:value "Page 22"
                                                                                ] ;
                                                              oa:hasStartSelector [ rdf:type oa:XPathSelector ;
                                                                                    rdf:value "Page 20"
                                                                                  ]
                                                            ] ;
                                             oa:hasSource sto:The_Industrial_Internet_of_Things_Volume_G1_Reference_Architecture
                                           ] ,
                                           [ rdf:type oa:SpecificResource ;
                                             dcterms:format "pdf" ;
                                             oa:hasSelector [ rdf:type oa:RangeSelector ;
                                                              oa:hasEndSelector [ rdf:type oa:XPathSelector ;
                                                                                  rdf:value "Page 22"
                                                                                ] ;
                                                              oa:hasStartSelector [ rdf:type oa:XPathSelector ;
                                                                                    rdf:value "Page 20"
                                                                                  ]
                                                            ] ;
                                             oa:hasSource sto:The_Industrial_Internet_of_Things_Volume_G1_Reference_Architecture
                                           ] .


###  https://w3id.org/i40/sto#IIRAConnectivity
sto:IIRAConnectivity rdf:type owl:NamedIndividual ,
                              sto:IIRACrosscuttingFunction ,
                              sto:StandardClassification ;
                     dcterms:creator sto:sebastian ;
                     dul:associatedWith sto:BdvaDataProcessingArchitectures ,
                                        sto:DecisionMaker ,
                                        sto:DtpSystemView ,
                                        sto:FiwareApplicationsServicesAndDataDelivery ,
                                        sto:IEC_62541 ,
                                        sto:IICF ,
                                        sto:IotaEvolutionInteroperability ,
                                        sto:LinkLayer ,
                                        sto:NgsiLdApiOperation ,
                                        sto:RAMICommunicationlayer ,
                                        sto:REST ,
                                        sto:oneM2M ,
                                        <https://www.wikidata.org/wiki/Q1548249> ;
                     dul:isPartOf sto:IIRAFunctionalViewpoint ;
                     sto:isDescribedin sto:IIRA ;
                     sto_iot:alignsWith sto:BdvaDataProcessingArchitectures ,
                                        sto:DtpSystemView ,
                                        sto:FiwareApplicationsServicesAndDataDelivery ,
                                        sto:IotaEvolutionInteroperability ,
                                        sto:NgsiLdApiOperation ,
                                        sto:RAMICommunicationlayer ;
                     sto_iot:frames sto:Authentication ,
                                    sto:CardinalityOfDataSources ,
                                    sto:CardinalityOfParticipants ,
                                    sto:Communication ,
                                    sto:DataAccess ,
                                    sto:DataDiscovery ,
                                    sto:DynamicAdjustability ,
                                    sto:EndpointInvocation ,
                                    sto:Evolvability ,
                                    sto:Governance ,
                                    sto:IPv4Support ,
                                    sto:IPv6Support ,
                                    sto:Identification ,
                                    sto:IdentityManagement ,
                                    sto:IntegrityProtection ,
                                    sto:Interoperability ,
                                    sto:Multilaterism ,
                                    sto:NetworkPerformance ,
                                    sto:QualityOfService ,
                                    sto:Reliability ,
                                    sto:Resilience ,
                                    sto:Safety ,
                                    sto:Scalability ,
                                    sto:SecureCommunication ,
                                    sto:Security ,
                                    sto:SemanticInteroperability ,
                                    sto:ServiceChoreography ,
                                    sto:ServiceComposition ,
                                    sto:ServiceDeployment ,
                                    sto:ServiceDescription ,
                                    sto:ServiceDiscovery ,
                                    sto:ServiceLifecycleManagement ,
                                    sto:ServiceOrchestration ,
                                    sto:SyntacticInteroperability ,
                                    sto:TimeSynchronization ,
                                    sto:Trustworthiness ,
                                    sto:Unicast ;
                     rdfs:label "IIRA Connectivity"@en .


###  https://w3id.org/i40/sto#IIRAConnectivityAnno
sto:IIRAConnectivityAnno rdf:type owl:NamedIndividual ,
                                  oa:Annotation ;
                         oa:hasBody sto:IIRAConnectivity ;
                         oa:hasTarget [ rdf:type oa:SpecificResource ;
                                        dcterms:format "pdf" ;
                                        oa:hasSelector [ rdf:type oa:RangeSelector ;
                                                         oa:hasEndSelector [ rdf:type oa:XPathSelector ;
                                                                             rdf:value "Page 127"
                                                                           ] ;
                                                         oa:hasStartSelector [ rdf:type oa:XPathSelector ;
                                                                               rdf:value "Page 8"
                                                                             ]
                                                       ] ;
                                        oa:hasSource sto:The_Industrial_Internet_of_Things_Volume_G5_Connectivity_Framework
                                      ] ,
                                      [ rdf:type oa:SpecificResource ;
                                        dcterms:format "pdf" ;
                                        oa:hasSelector [ rdf:type oa:RangeSelector ;
                                                         oa:hasEndSelector [ rdf:type oa:XPathSelector ;
                                                                             rdf:value "Page 127"
                                                                           ] ;
                                                         oa:hasStartSelector [ rdf:type oa:XPathSelector ;
                                                                               rdf:value "Page 8"
                                                                             ]
                                                       ] ;
                                        oa:hasSource sto:The_Industrial_Internet_of_Things_Volume_G5_Connectivity_Framework
                                      ] .


###  https://w3id.org/i40/sto#IIRAControlDomain
sto:IIRAControlDomain rdf:type owl:NamedIndividual ,
                               sto:IIRAFunctionalDomain ,
                               sto:StandardClassification ;
                      dcterms:creator sto:sebastian ;
                      dul:associatedWith sto:EdgecrossEdgeComputingLayer ,
                                         sto:FiwareIotServicesEnablement ,
                                         sto:IDSRAMSystemLayer ,
                                         sto:IotaInformationViewpoint ,
                                         sto:NgsiLdApiOperation ,
                                         sto:RAMIIntegrationLayer ,
                                         sto:xRoadProtocolsInterfaces ;
                      dul:isPartOf sto:IIRAFunctionalViewpoint ;
                      sto:isDescribedin sto:IIRA ;
                      sto_iot:alignsWith sto:EdgecrossEdgeComputingLayer ,
                                         sto:FiwareIotServicesEnablement ,
                                         sto:IDSRAMSystemLayer ,
                                         sto:IotaInformationViewpoint ,
                                         sto:NgsiLdApiOperation ,
                                         sto:RAMIIntegrationLayer ,
                                         sto:xRoadProtocolsInterfaces ;
                      sto_iot:frames sto:Actuation ,
                                     sto:AssetManagement ,
                                     sto:Communication ,
                                     sto:EdgeAnalytics ,
                                     sto:IoT ,
                                     sto:Sensing ,
                                     sto:VirtualEntity ;
                      rdfs:label "IIRA Control Domain"@en ;
                      skos:note "Publications referred: 'IIC:PUB:G1:V1.80:20170131' '6.1 THE CONTROL DOMAIN' 'Page 27' " .


###  https://w3id.org/i40/sto#IIRAControlDomainAnno
sto:IIRAControlDomainAnno rdf:type owl:NamedIndividual ,
                                   oa:Annotation ;
                          oa:hasBody sto:IIRAControlDomain ;
                          oa:hasTarget [ rdf:type oa:SpecificResource ;
                                         dcterms:format "pdf" ;
                                         oa:hasSelector [ rdf:type oa:RangeSelector ;
                                                          oa:hasEndSelector [ rdf:type oa:XPathSelector ;
                                                                              rdf:value "Page 30"
                                                                            ] ;
                                                          oa:hasStartSelector [ rdf:type oa:XPathSelector ;
                                                                                rdf:value "Page 27"
                                                                              ]
                                                        ] ;
                                         oa:hasSource sto:The_Industrial_Internet_of_Things_Volume_G1_Reference_Architecture
                                       ] ,
                                       [ rdf:type oa:SpecificResource ;
                                         dcterms:format "pdf" ;
                                         oa:hasSelector [ rdf:type oa:RangeSelector ;
                                                          oa:hasEndSelector [ rdf:type oa:XPathSelector ;
                                                                              rdf:value "Page 30"
                                                                            ] ;
                                                          oa:hasStartSelector [ rdf:type oa:XPathSelector ;
                                                                                rdf:value "Page 27"
                                                                              ]
                                                        ] ;
                                         oa:hasSource sto:The_Industrial_Internet_of_Things_Volume_G1_Reference_Architecture
                                       ] .


###  https://w3id.org/i40/sto#IIRACrosscuttingFunction
sto:IIRACrosscuttingFunction rdf:type owl:NamedIndividual ;
                             dcterms:creator sto:sebastian .


###  https://w3id.org/i40/sto#IIRACrosscuttingFunctionAnno
sto:IIRACrosscuttingFunctionAnno rdf:type owl:NamedIndividual ,
                                          oa:Annotation ;
                                 oa:hasBody sto:IIRACrosscuttingFunction ;
                                 oa:hasTarget [ rdf:type oa:SpecificResource ;
                                                dcterms:format "pdf" ;
                                                oa:hasSelector [ rdf:type oa:RangeSelector ;
                                                                 oa:hasEndSelector [ rdf:type oa:XPathSelector ;
                                                                                     rdf:value "Page 36"
                                                                                   ] ;
                                                                 oa:hasStartSelector [ rdf:type oa:XPathSelector ;
                                                                                       rdf:value "Page 34"
                                                                                     ]
                                                               ] ;
                                                oa:hasSource sto:The_Industrial_Internet_of_Things_Volume_G1_Reference_Architecture
                                              ] ,
                                              [ rdf:type oa:SpecificResource ;
                                                dcterms:format "pdf" ;
                                                oa:hasSelector [ rdf:type oa:RangeSelector ;
                                                                 oa:hasEndSelector [ rdf:type oa:XPathSelector ;
                                                                                     rdf:value "Page 36"
                                                                                   ] ;
                                                                 oa:hasStartSelector [ rdf:type oa:XPathSelector ;
                                                                                       rdf:value "Page 34"
                                                                                     ]
                                                               ] ;
                                                oa:hasSource sto:The_Industrial_Internet_of_Things_Volume_G1_Reference_Architecture
                                              ] .


###  https://w3id.org/i40/sto#IIRADistributedDataManagement
sto:IIRADistributedDataManagement rdf:type owl:NamedIndividual ,
                                           sto:IIRACrosscuttingFunction ,
                                           sto:StandardClassification ;
                                  dcterms:creator sto:sebastian ;
                                  dul:associatedWith sto:FiwareCloudHosting ,
                                                     sto:RAMICommunicationlayer ;
                                  dul:isPartOf sto:IIRAFunctionalViewpoint ;
                                  sto:isDescribedin sto:IIRA ;
                                  sto_iot:alignsWith sto:FiwareCloudHosting ,
                                                     sto:RAMICommunicationlayer ;
                                  sto_iot:frames sto:Interoperability ,
                                                 sto:SemanticInteroperability ;
                                  rdfs:label "IIRA Distributed Data Management"@en .


###  https://w3id.org/i40/sto#IIRAFunctionalDomain
sto:IIRAFunctionalDomain rdf:type owl:NamedIndividual ;
                         dcterms:creator sto:sebastian .


###  https://w3id.org/i40/sto#IIRAFunctionalViewpoint
sto:IIRAFunctionalViewpoint rdf:type owl:NamedIndividual ,
                                     sto:StandardClassification ,
                                     sto:Viewpoint ;
                            dcterms:creator sto:sebastian ;
                            dul:associatedWith sto:IDSRAMReferenceArchitectureModel ,
                                               sto:IotaFunctionalViewpoint ,
                                               sto:OceanSystemViewpoint ;
                            sto:isDescribedin sto:IIRA ;
                            sto_iot:alignsWith sto:IDSRAMReferenceArchitectureModel ,
                                               sto:IotaFunctionalViewpoint ,
                                               sto:OceanSystemViewpoint ;
                            sto_iot:frames sto:AsProcessPlanning ,
                                           sto:AccessPolicy ,
                                           sto:Actuation ,
                                           sto:Authentication ,
                                           sto:Authorization ,
                                           sto:Availability ,
                                           sto:BdvaDataViualisationAndUserInteraction ,
                                           sto:CardinalityOfDataSources ,
                                           sto:CardinalityOfParticipants ,
                                           sto:CloudComputing ,
                                           sto:Communication ,
                                           sto:DataAccess ,
                                           sto:DataAccessControl ,
                                           sto:DataAnalytics ,
                                           sto:DataAtRest ,
                                           sto:DataDiscovery ,
                                           sto:DataInMotion ,
                                           sto:DataProcessing ,
                                           sto:DataProtection ,
                                           sto:DataSovereignty ,
                                           sto:DynamicAdjustability ,
                                           sto:EndpointInvocation ,
                                           sto:Evolvability ,
                                           sto:Governance ,
                                           sto:IPv4Support ,
                                           sto:IPv6Support ,
                                           sto:Identification ,
                                           sto:IdentityManagement ,
                                           sto:IntegrityProtection ,
                                           sto:Interoperability ,
                                           sto:IoT ,
                                           sto:Multilaterism ,
                                           sto:NetworkPerformance ,
                                           sto:Privacy ,
                                           sto:QualityOfService ,
                                           sto:RealTimeAnalytics ,
                                           sto:Reliability ,
                                           sto:Resilience ,
                                           sto:Safety ,
                                           sto:Scalability ,
                                           sto:SecureCommunication ,
                                           sto:Security ,
                                           sto:SecurityConfiguration ,
                                           sto:SemanticInteroperability ,
                                           sto:Sensing ,
                                           sto:ServiceAccessControl ,
                                           sto:ServiceChoreography ,
                                           sto:ServiceComposition ,
                                           sto:ServiceDeployment ,
                                           sto:ServiceDescription ,
                                           sto:ServiceDiscovery ,
                                           sto:ServiceIsolation ,
                                           sto:ServiceLevelAgreements ,
                                           sto:ServiceLifecycleManagement ,
                                           sto:ServiceOrchestration ,
                                           sto:StreamProcessing ,
                                           sto:SyntacticInteroperability ,
                                           sto:TimeSynchronization ,
                                           sto:Trustworthiness ,
                                           sto:Unicast ;
                            rdfs:comment "The IIRA Functional Viewpoint contains the IIRA Domains in order to describe technical relations and communications between the several dimensions of IoT devices."@en ;
                            rdfs:label "IIRA Functional Viewpoint"@en ;
                            skos:note "Publications referred: '(IIC:PUB:G1:V1.80:20170131' '3.5.3 FUNCTIONAL VIEWPOINT' 'Page 16' " .


###  https://w3id.org/i40/sto#IIRAFunctionalViewpointAnno
sto:IIRAFunctionalViewpointAnno rdf:type owl:NamedIndividual ,
                                         oa:Annotation ;
                                oa:hasBody sto:IIRAFunctionalViewpoint ;
                                oa:hasTarget [ rdf:type oa:SpecificResource ;
                                               dcterms:format "pdf" ;
                                               oa:hasSelector [ rdf:type oa:RangeSelector ;
                                                                oa:hasEndSelector [ rdf:type oa:XPathSelector ;
                                                                                    rdf:value "Page 38"
                                                                                  ] ;
                                                                oa:hasStartSelector [ rdf:type oa:XPathSelector ;
                                                                                      rdf:value "Page 25"
                                                                                    ]
                                                              ] ;
                                               oa:hasSource sto:The_Industrial_Internet_of_Things_Volume_G1_Reference_Architecture
                                             ] ,
                                             [ rdf:type oa:SpecificResource ;
                                               dcterms:format "pdf" ;
                                               oa:hasSelector [ rdf:type oa:RangeSelector ;
                                                                oa:hasEndSelector [ rdf:type oa:XPathSelector ;
                                                                                    rdf:value "Page 38"
                                                                                  ] ;
                                                                oa:hasStartSelector [ rdf:type oa:XPathSelector ;
                                                                                      rdf:value "Page 25"
                                                                                    ]
                                                              ] ;
                                               oa:hasSource sto:The_Industrial_Internet_of_Things_Volume_G1_Reference_Architecture
                                             ] .


###  https://w3id.org/i40/sto#IIRAImplementationViewpoint
sto:IIRAImplementationViewpoint rdf:type owl:NamedIndividual ,
                                         sto:StandardClassification ,
                                         sto:Viewpoint ;
                                dul:associatedWith sto:ControlDomain ,
                                                   sto:DtpDeploymentView ,
                                                   sto:FIWARE ,
                                                   sto:IDSRAMSystemLayer ,
                                                   sto:IIRAApplicationDomain ,
                                                   sto:IIRABusinessDomain ,
                                                   sto:IIRAOperationsDomain ,
                                                   sto:InformationDomain ,
                                                   sto:IotaDeploymentOperationViewpoint ,
                                                   sto:NgsiLdArchitecture ,
                                                   sto:xRoadDeploymentView ;
                                sto:isDescribedin sto:IIRA ;
                                sto_iot:alignsWith sto:DtpDeploymentView ,
                                                   sto:FIWARE ,
                                                   sto:IotaDeploymentOperationViewpoint ,
                                                   sto:NgsiLdArchitecture ,
                                                   sto:xRoadDeploymentView ;
                                sto_iot:frames sto:CloudComputing ,
                                               sto:Communication ,
                                               sto:DataProcessing ,
                                               sto:EdgeComputing ,
                                               sto:EndpointDescription ,
                                               sto:Interoperability ,
                                               sto:SemanticInteroperability ;
                                rdfs:label "IIRA Implementation Viewpoint"@en ;
                                skos:note "Publications referred: '(IIC:PUB:G1:V1.80:20170131' '3.5.4 IMPLEMENTATION VIEWPOINT' 'Page 16' " .


###  https://w3id.org/i40/sto#IIRAImplementationViewpointAnno
sto:IIRAImplementationViewpointAnno rdf:type owl:NamedIndividual ,
                                             oa:Annotation ;
                                    oa:hasBody sto:IIRAImplementationViewpoint ;
                                    oa:hasTarget [ rdf:type oa:SpecificResource ;
                                                   dcterms:format "pdf" ;
                                                   oa:hasSelector [ rdf:type oa:RangeSelector ;
                                                                    oa:hasEndSelector [ rdf:type oa:XPathSelector ;
                                                                                        rdf:value "Page 47"
                                                                                      ] ;
                                                                    oa:hasStartSelector [ rdf:type oa:XPathSelector ;
                                                                                          rdf:value "Page 38"
                                                                                        ]
                                                                  ] ;
                                                   oa:hasSource sto:The_Industrial_Internet_of_Things_Volume_G1_Reference_Architecture
                                                 ] ,
                                                 [ rdf:type oa:SpecificResource ;
                                                   dcterms:format "pdf" ;
                                                   oa:hasSelector [ rdf:type oa:RangeSelector ;
                                                                    oa:hasEndSelector [ rdf:type oa:XPathSelector ;
                                                                                        rdf:value "Page 47"
                                                                                      ] ;
                                                                    oa:hasStartSelector [ rdf:type oa:XPathSelector ;
                                                                                          rdf:value "Page 38"
                                                                                        ]
                                                                  ] ;
                                                   oa:hasSource sto:The_Industrial_Internet_of_Things_Volume_G1_Reference_Architecture
                                                 ] .


###  https://w3id.org/i40/sto#IIRAIndustrialAnalytics
sto:IIRAIndustrialAnalytics rdf:type owl:NamedIndividual ,
                                     sto:IIRACrosscuttingFunction ,
                                     sto:StandardClassification ;
                            dul:isPartOf sto:IIRAFunctionalViewpoint ;
                            sto:isDescribedin sto:IIRA .


###  https://w3id.org/i40/sto#IIRAInformationDomain
sto:IIRAInformationDomain rdf:type owl:NamedIndividual ,
                                   sto:IIRAFunctionalDomain ,
                                   sto:StandardClassification ;
                          dul:associatedWith sto:BdvaDataAnalytics ,
                                             sto:BdvaDataProcessingArchitectures ,
                                             sto:DtpSystemView ,
                                             sto:EdgecrossEdgeComputingLayer ,
                                             sto:IDSRAMInformationLayer ,
                                             sto:IDSRAMProcessLayer ,
                                             sto:IotaInformationViewpoint ,
                                             sto:NgsiLdInformationModel ,
                                             sto:RAMIInformationLayer ;
                          dul:isPartOf sto:IIRAFunctionalViewpoint ;
                          sto:isDescribedin sto:IIRA ;
                          sto_iot:alignsWith sto:BdvaDataAnalytics ,
                                             sto:BdvaDataProcessingArchitectures ,
                                             sto:DtpSystemView ,
                                             sto:EdgecrossEdgeComputingLayer ,
                                             sto:IDSRAMInformationLayer ,
                                             sto:IDSRAMProcessLayer ,
                                             sto:IotaInformationViewpoint ,
                                             sto:NgsiLdInformationModel ,
                                             sto:RAMIInformationLayer ;
                          sto_iot:frames sto:DataAnalytics ,
                                         sto:DataProcessing ,
                                         sto:Interoperability ,
                                         sto:SemanticInteroperability ,
                                         sto:StreamProcessing ,
                                         sto:SyntacticInteroperability ;
                          rdfs:label "IIRA Information Domain"@en ;
                          skos:note "Publications referred: 'IIC:PUB:G1:V1.80:20170131' '6.3 THE INFORMATION DOMAIN' 'Page 32' " .


###  https://w3id.org/i40/sto#IIRAInformationDomainAnno
sto:IIRAInformationDomainAnno rdf:type owl:NamedIndividual ,
                                       oa:Annotation ;
                              oa:hasBody sto:IIRAInformationDomain ;
                              oa:hasTarget [ rdf:type oa:SpecificResource ;
                                             dcterms:format "pdf" ;
                                             oa:hasSelector [ rdf:type oa:RangeSelector ;
                                                              oa:hasEndSelector [ rdf:type oa:XPathSelector ;
                                                                                  rdf:value "Page 34"
                                                                                ] ;
                                                              oa:hasStartSelector [ rdf:type oa:XPathSelector ;
                                                                                    rdf:value "Page 32"
                                                                                  ]
                                                            ] ;
                                             oa:hasSource sto:The_Industrial_Internet_of_Things_Volume_G1_Reference_Architecture
                                           ] ,
                                           [ rdf:type oa:SpecificResource ;
                                             dcterms:format "pdf" ;
                                             oa:hasSelector [ rdf:type oa:RangeSelector ;
                                                              oa:hasEndSelector [ rdf:type oa:XPathSelector ;
                                                                                  rdf:value "Page 34"
                                                                                ] ;
                                                              oa:hasStartSelector [ rdf:type oa:XPathSelector ;
                                                                                    rdf:value "Page 32"
                                                                                  ]
                                                            ] ;
                                             oa:hasSource sto:The_Industrial_Internet_of_Things_Volume_G1_Reference_Architecture
                                           ] .


###  https://w3id.org/i40/sto#IIRAIntelligentAndResilientControl
sto:IIRAIntelligentAndResilientControl rdf:type owl:NamedIndividual ,
                                                sto:IIRACrosscuttingFunction ,
                                                sto:StandardClassification ;
                                       dul:isPartOf sto:IIRAFunctionalViewpoint ;
                                       sto:isDescribedin sto:IIRA ;
                                       rdfs:comment """There is a renewed movement to distribute computational capability toward the network peripheries, away from concentrated computation centers, to benefit from a reduction in movement of data and communication latency, and enhancement in local intelligent control and, more importantly, resilience.
source: Industrial Internet Reference Archietcture"""@en ;
                                       rdfs:label "IIRA Intelligent and Resilient Control"@en .


###  https://w3id.org/i40/sto#IIRAOperationsDomain
sto:IIRAOperationsDomain rdf:type owl:NamedIndividual ,
                                  sto:IIRAFunctionalDomain ,
                                  sto:StandardClassification ;
                         dul:associatedWith sto:DtpSystemView ,
                                            sto:EdgecrossEdgeComputingLayer ,
                                            sto:IDSRAMProcessLayer ,
                                            sto:IotaInformationViewpoint ,
                                            sto:IviActivityView ,
                                            sto:RAMIFunctionalLayer ;
                         dul:isPartOf sto:IIRAFunctionalViewpoint ;
                         sto:isDescribedin sto:IIRA ;
                         sto_iot:alignsWith sto:DtpSystemView ,
                                            sto:EdgecrossEdgeComputingLayer ,
                                            sto:IDSRAMProcessLayer ,
                                            sto:IotaInformationViewpoint ,
                                            sto:IviActivityView ,
                                            sto:RAMIFunctionalLayer ;
                         sto_iot:frames sto:DataAnalytics ,
                                        sto:RealTimeAnalytics ,
                                        sto:ServiceDeployment ,
                                        sto:ServiceLifecycleManagement ;
                         rdfs:label "IIRA Operation Domain"@en ;
                         skos:note "Publications referred: 'IIC:PUB:G1:V1.80:20170131' '6.2 THE OPERATIONS DOMAIN' 'Page 30' " .


###  https://w3id.org/i40/sto#IIRAOperationsDomainAnno
sto:IIRAOperationsDomainAnno rdf:type owl:NamedIndividual ,
                                      oa:Annotation ;
                             oa:hasBody sto:IIRAOperationsDomain ;
                             oa:hasTarget [ rdf:type oa:SpecificResource ;
                                            dcterms:format "pdf" ;
                                            oa:hasSelector [ rdf:type oa:RangeSelector ;
                                                             oa:hasEndSelector [ rdf:type oa:XPathSelector ;
                                                                                 rdf:value "Page 32"
                                                                               ] ;
                                                             oa:hasStartSelector [ rdf:type oa:XPathSelector ;
                                                                                   rdf:value "Page 30"
                                                                                 ]
                                                           ] ;
                                            oa:hasSource sto:The_Industrial_Internet_of_Things_Volume_G1_Reference_Architecture
                                          ] ,
                                          [ rdf:type oa:SpecificResource ;
                                            dcterms:format "pdf" ;
                                            oa:hasSelector [ rdf:type oa:RangeSelector ;
                                                             oa:hasEndSelector [ rdf:type oa:XPathSelector ;
                                                                                 rdf:value "Page 32"
                                                                               ] ;
                                                             oa:hasStartSelector [ rdf:type oa:XPathSelector ;
                                                                                   rdf:value "Page 30"
                                                                                 ]
                                                           ] ;
                                            oa:hasSource sto:The_Industrial_Internet_of_Things_Volume_G1_Reference_Architecture
                                          ] .


###  https://w3id.org/i40/sto#IIRAPhysicalSystems
sto:IIRAPhysicalSystems rdf:type owl:NamedIndividual ,
                                 sto:StandardClassification ;
                        dcterms:creator sto:sebastian ;
                        dul:associatedWith sto:EdgecrossFacilityLayer ,
                                           sto:IDSRAMSystemLayer ,
                                           sto:IviAssetView ,
                                           sto:RAMIAssetlayer ;
                        dul:isPartOf sto:IIRAFunctionalViewpoint ;
                        sto:isDescribedin sto:IIRA ;
                        sto_iot:alignsWith sto:EdgecrossFacilityLayer ,
                                           sto:IDSRAMSystemLayer ,
                                           sto:IviAssetView ,
                                           sto:RAMIAssetlayer ;
                        rdfs:comment "Computational capabilities ranging from very limited (e.g. in a smart sensor) to reasonably rich (e.g. a cluster of servers) are placed in, attached to or collocated with physical systems (e.g. in smart sensors, devices or machines). These capabilities are connected through a variety of connectivity technologies including wireless."@en ;
                        rdfs:label "IIRA Physical Systems"@en ;
                        sto:hasOfficialResource <https://www.iiconsortium.org/IIRA.htm> .


###  https://w3id.org/i40/sto#IIRAPrivacy
sto:IIRAPrivacy rdf:type owl:NamedIndividual ,
                         sto:IIRASystemCharacteristics ,
                         sto:StandardClassification ;
                dul:associatedWith sto:DtpSecurityPrivacy ;
                dul:isPartOf sto:IIRAFunctionalViewpoint ;
                sto:isDescribedin sto:IIRA ;
                sto_iot:alignsWith sto:DtpSecurityPrivacy ;
                sto_iot:frames sto:DataSovereignty ,
                               sto:Privacy ,
                               sto:Trustworthiness ;
                rdfs:label "IIRA Privacy"@en .


###  https://w3id.org/i40/sto#IIRAReliability
sto:IIRAReliability rdf:type owl:NamedIndividual ,
                             sto:IIRASystemCharacteristics ,
                             sto:StandardClassification ;
                    dul:isPartOf sto:IIRAFunctionalViewpoint ;
                    sto:isDescribedin sto:IIRA ;
                    sto_iot:frames sto:Reliability ,
                                   sto:Trustworthiness ;
                    rdfs:label "IIRA Reliability"@en ;
                    skos:note "Publications referred: '<https://www.iiconsortium.org/pdf/IIC_PUB_G4_V1.00_PB-3.pdf IIC:PUB:G4:V1.0:PB:20160926>' '3.4 RELIABILITY' 'Page 18'" .


###  https://w3id.org/i40/sto#IIRAReliabilityAnno
sto:IIRAReliabilityAnno rdf:type owl:NamedIndividual ,
                                 oa:Annotation ;
                        oa:hasBody sto:IIRAReliability ;
                        oa:hasTarget [ rdf:type oa:SpecificResource ;
                                       dcterms:format "pdf" ;
                                       oa:hasSelector [ rdf:type oa:RangeSelector ;
                                                        oa:hasEndSelector [ rdf:type oa:XPathSelector ;
                                                                            rdf:value "Page 19"
                                                                          ] ;
                                                        oa:hasStartSelector [ rdf:type oa:XPathSelector ;
                                                                              rdf:value "Page 18"
                                                                            ]
                                                      ] ;
                                       oa:hasSource sto:Industrial_Internet_of_Things_Volume_G4_Security_Framework
                                     ] ,
                                     [ rdf:type oa:SpecificResource ;
                                       dcterms:format "pdf" ;
                                       oa:hasSelector [ rdf:type oa:RangeSelector ;
                                                        oa:hasEndSelector [ rdf:type oa:XPathSelector ;
                                                                            rdf:value "Page 19"
                                                                          ] ;
                                                        oa:hasStartSelector [ rdf:type oa:XPathSelector ;
                                                                              rdf:value "Page 18"
                                                                            ]
                                                      ] ;
                                       oa:hasSource sto:Industrial_Internet_of_Things_Volume_G4_Security_Framework
                                     ] .


###  https://w3id.org/i40/sto#IIRAResilience
sto:IIRAResilience rdf:type owl:NamedIndividual ,
                            sto:IIRASystemCharacteristics ,
                            sto:StandardClassification ;
                   dul:isPartOf sto:IIRAFunctionalViewpoint ;
                   sto:isDescribedin sto:IIRA ;
                   rdfs:label "IIRA Resilience"@en .


###  https://w3id.org/i40/sto#IIRAResilienceAnno
sto:IIRAResilienceAnno rdf:type owl:NamedIndividual ,
                                oa:Annotation ;
                       oa:hasBody sto:IIRAResilience ;
                       oa:hasTarget [ rdf:type oa:SpecificResource ;
                                      dcterms:format "pdf" ;
                                      oa:hasSelector [ rdf:type oa:RangeSelector ;
                                                       oa:hasEndSelector [ rdf:type oa:XPathSelector ;
                                                                           rdf:value "Page 20"
                                                                         ] ;
                                                       oa:hasStartSelector [ rdf:type oa:XPathSelector ;
                                                                             rdf:value "Page 19"
                                                                           ]
                                                     ] ;
                                      oa:hasSource sto:Industrial_Internet_of_Things_Volume_G4_Security_Framework
                                    ] ,
                                    [ rdf:type oa:SpecificResource ;
                                      dcterms:format "pdf" ;
                                      oa:hasSelector [ rdf:type oa:RangeSelector ;
                                                       oa:hasEndSelector [ rdf:type oa:XPathSelector ;
                                                                           rdf:value "Page 19"
                                                                         ] ;
                                                       oa:hasStartSelector [ rdf:type oa:XPathSelector ;
                                                                             rdf:value "Page 18"
                                                                           ]
                                                     ] ;
                                      oa:hasSource sto:Industrial_Internet_of_Things_Volume_G4_Security_Framework
                                    ] ,
                                    [ rdf:type oa:SpecificResource ;
                                      dcterms:format "pdf" ;
                                      oa:hasSelector [ rdf:type oa:RangeSelector ;
                                                       oa:hasEndSelector [ rdf:type oa:XPathSelector ;
                                                                           rdf:value "Page 19"
                                                                         ] ;
                                                       oa:hasStartSelector [ rdf:type oa:XPathSelector ;
                                                                             rdf:value "Page 18"
                                                                           ]
                                                     ] ;
                                      oa:hasSource sto:Industrial_Internet_of_Things_Volume_G4_Security_Framework
                                    ] ,
                                    [ rdf:type oa:SpecificResource ;
                                      dcterms:format "pdf" ;
                                      oa:hasSelector [ rdf:type oa:RangeSelector ;
                                                       oa:hasEndSelector [ rdf:type oa:XPathSelector ;
                                                                           rdf:value "Page 20"
                                                                         ] ;
                                                       oa:hasStartSelector [ rdf:type oa:XPathSelector ;
                                                                             rdf:value "Page 19"
                                                                           ]
                                                     ] ;
                                      oa:hasSource sto:Industrial_Internet_of_Things_Volume_G4_Security_Framework
                                    ] .


###  https://w3id.org/i40/sto#IIRASafety
sto:IIRASafety rdf:type owl:NamedIndividual ,
                        sto:IIRASystemCharacteristics ,
                        sto:StandardClassification ;
               dul:isPartOf sto:IIRAFunctionalViewpoint ;
               sto:isDescribedin sto:IIRA ;
               rdfs:label "IIRA Safety"@en .


###  https://w3id.org/i40/sto#IIRASafetyAnno
sto:IIRASafetyAnno rdf:type owl:NamedIndividual ,
                            oa:Annotation ;
                   oa:hasBody sto:IIRASafety ;
                   oa:hasTarget [ rdf:type oa:SpecificResource ;
                                  dcterms:format "pdf" ;
                                  oa:hasSelector [ rdf:type oa:RangeSelector ;
                                                   oa:hasEndSelector [ rdf:type oa:XPathSelector ;
                                                                       rdf:value "Page 18"
                                                                     ] ;
                                                   oa:hasStartSelector [ rdf:type oa:XPathSelector ;
                                                                         rdf:value "Page 17"
                                                                       ]
                                                 ] ;
                                  oa:hasSource sto:Industrial_Internet_of_Things_Volume_G4_Security_Framework
                                ] ,
                                [ rdf:type oa:SpecificResource ;
                                  dcterms:format "pdf" ;
                                  oa:hasSelector [ rdf:type oa:RangeSelector ;
                                                   oa:hasEndSelector [ rdf:type oa:XPathSelector ;
                                                                       rdf:value "Page 18"
                                                                     ] ;
                                                   oa:hasStartSelector [ rdf:type oa:XPathSelector ;
                                                                         rdf:value "Page 17"
                                                                       ]
                                                 ] ;
                                  oa:hasSource sto:Industrial_Internet_of_Things_Volume_G4_Security_Framework
                                ] .


###  https://w3id.org/i40/sto#IIRAScalability
sto:IIRAScalability rdf:type owl:NamedIndividual ,
                             sto:IIRASystemCharacteristics ,
                             sto:StandardClassification ;
                    dul:associatedWith sto:FiwareCloudHosting ;
                    dul:isPartOf sto:IIRAFunctionalViewpoint ;
                    sto:isDescribedin sto:IIRA ;
                    sto_iot:alignsWith sto:FiwareCloudHosting ;
                    sto_iot:frames sto:Scalability ;
                    rdfs:label "IIRA Scalability"@en .


###  https://w3id.org/i40/sto#IIRASecurity
sto:IIRASecurity rdf:type owl:NamedIndividual ,
                          sto:IIRASystemCharacteristics ,
                          sto:StandardClassification ;
                 dcterms:creator sto:sebastian ;
                 dul:associatedWith sto:DataOwner ,
                                    sto:DecisionMaker ,
                                    sto:DtpSecurityPrivacy ,
                                    sto:FiwareSecurity ,
                                    sto:IDSRAMSecurity ,
                                    sto:IotaAvailabilityResilience ,
                                    sto:IotaTrustSecurityPrivacy ,
                                    <https://www.wikidata.org/wiki/Q1548249> ;
                 dul:isPartOf sto:IIRAFunctionalViewpoint ;
                 sto:isDescribedin sto:IIRA ;
                 sto_iot:alignsWith sto:DtpSecurityPrivacy ,
                                    sto:FiwareSecurity ,
                                    sto:IDSRAMSecurity ,
                                    sto:IotaAvailabilityResilience ,
                                    sto:IotaTrustSecurityPrivacy ;
                 sto_iot:frames sto:AccessPolicy ,
                                sto:Authorization ,
                                sto:Availability ,
                                sto:CloudComputing ,
                                sto:Communication ,
                                sto:DataAccessControl ,
                                sto:DataAtRest ,
                                sto:DataInMotion ,
                                sto:DataProcessing ,
                                sto:DataProtection ,
                                sto:DataSovereignty ,
                                sto:Identification ,
                                sto:IdentityManagement ,
                                sto:IntegrityProtection ,
                                sto:Privacy ,
                                sto:Reliability ,
                                sto:Resilience ,
                                sto:Safety ,
                                sto:SecureCommunication ,
                                sto:Security ,
                                sto:SecurityConfiguration ,
                                sto:ServiceAccessControl ,
                                sto:ServiceIsolation ,
                                sto:ServiceLevelAgreements ,
                                sto:ServiceLifecycleManagement ,
                                sto:Trustworthiness ;
                 rdfs:label "IIRA Security"@en .


###  https://w3id.org/i40/sto#IIRASecurityAnno
sto:IIRASecurityAnno rdf:type owl:NamedIndividual ,
                              oa:Annotation ;
                     oa:hasBody sto:IIRASecurity ;
                     oa:hasTarget [ rdf:type oa:SpecificResource ;
                                    dcterms:format "pdf" ;
                                    oa:hasSelector [ rdf:type oa:RangeSelector ;
                                                     oa:hasEndSelector [ rdf:type oa:XPathSelector ;
                                                                         rdf:value "Page 121"
                                                                       ] ;
                                                     oa:hasStartSelector [ rdf:type oa:XPathSelector ;
                                                                           rdf:value "Page 11"
                                                                         ]
                                                   ] ;
                                    oa:hasSource sto:Industrial_Internet_of_Things_Volume_G4_Security_Framework
                                  ] ,
                                  [ rdf:type oa:SpecificResource ;
                                    dcterms:format "pdf" ;
                                    oa:hasSelector [ rdf:type oa:RangeSelector ;
                                                     oa:hasEndSelector [ rdf:type oa:XPathSelector ;
                                                                         rdf:value "Page 121"
                                                                       ] ;
                                                     oa:hasStartSelector [ rdf:type oa:XPathSelector ;
                                                                           rdf:value "Page 11"
                                                                         ]
                                                   ] ;
                                    oa:hasSource sto:Industrial_Internet_of_Things_Volume_G4_Security_Framework
                                  ] .


###  https://w3id.org/i40/sto#IIRASecurityFramework
sto:IIRASecurityFramework rdf:type owl:NamedIndividual ,
                                   sto:StandardClassification ;
                          dcterms:creator sto:sebastian ;
                          dul:associatedWith sto:BdvaCyberSecurityTrust ,
                                             sto:BdvaDataProtection ,
                                             sto:IDSRAMSecurity ,
                                             sto:xRoadSystemComponents ;
                          sto_iot:alignsWith sto:BdvaCyberSecurityTrust ,
                                             sto:BdvaDataProtection ,
                                             sto:IDSRAMSecurity ,
                                             sto:xRoadSystemComponents ;
                          rdfs:label "IIC Security Framework"@en ;
                          skos:note "Publications referred: '<https://www.iiconsortium.org/pdf/IIC_PUB_G4_V1.00_PB-3.pdf IIC:PUB:G4:V1.0:PB:20160926>'" ;
                          sto:hasOfficialResource <https://www.iiconsortium.org/IISF.htm> .


###  https://w3id.org/i40/sto#IIRASecurityFrameworkAnno
sto:IIRASecurityFrameworkAnno rdf:type owl:NamedIndividual ,
                                       oa:Annotation ;
                              oa:hasBody sto:IIRASecurityFramework ;
                              oa:hasTarget [ rdf:type oa:SpecificResource ;
                                             dcterms:format "pdf" ;
                                             oa:hasSelector [ rdf:type oa:RangeSelector ;
                                                              oa:hasEndSelector [ rdf:type oa:XPathSelector ;
                                                                                  rdf:value "Page 121"
                                                                                ] ;
                                                              oa:hasStartSelector [ rdf:type oa:XPathSelector ;
                                                                                    rdf:value "Page 11"
                                                                                  ]
                                                            ] ;
                                             oa:hasSource sto:Industrial_Internet_of_Things_Volume_G4_Security_Framework
                                           ] ,
                                           [ rdf:type oa:SpecificResource ;
                                             dcterms:format "pdf" ;
                                             oa:hasSelector [ rdf:type oa:RangeSelector ;
                                                              oa:hasEndSelector [ rdf:type oa:XPathSelector ;
                                                                                  rdf:value "Page 121"
                                                                                ] ;
                                                              oa:hasStartSelector [ rdf:type oa:XPathSelector ;
                                                                                    rdf:value "Page 11"
                                                                                  ]
                                                            ] ;
                                             oa:hasSource sto:Industrial_Internet_of_Things_Volume_G4_Security_Framework
                                           ] ,
                                           [ rdf:type oa:SpecificResource ;
                                             dcterms:format "pdf" ;
                                             oa:hasSelector [ rdf:type oa:RangeSelector ;
                                                              oa:hasEndSelector [ rdf:type oa:XPathSelector ;
                                                                                  rdf:value "Page 121"
                                                                                ] ;
                                                              oa:hasStartSelector [ rdf:type oa:XPathSelector ;
                                                                                    rdf:value "Page 11"
                                                                                  ]
                                                            ] ;
                                             oa:hasSource sto:Industrial_Internet_of_Things_Volume_G4_Security_Framework
                                           ] ,
                                           [ rdf:type oa:SpecificResource ;
                                             dcterms:format "pdf" ;
                                             oa:hasSelector [ rdf:type oa:RangeSelector ;
                                                              oa:hasEndSelector [ rdf:type oa:XPathSelector ;
                                                                                  rdf:value "Page 121"
                                                                                ] ;
                                                              oa:hasStartSelector [ rdf:type oa:XPathSelector ;
                                                                                    rdf:value "Page 11"
                                                                                  ]
                                                            ] ;
                                             oa:hasSource sto:Industrial_Internet_of_Things_Volume_G4_Security_Framework
                                           ] .


###  https://w3id.org/i40/sto#IIRASystemCharacteristics
sto:IIRASystemCharacteristics rdf:type owl:NamedIndividual ;
                              dcterms:creator sto:sebastian .


###  https://w3id.org/i40/sto#IIRAUsageViewpoint
sto:IIRAUsageViewpoint rdf:type owl:NamedIndividual ,
                                sto:StandardClassification ,
                                sto:Viewpoint ;
                       dul:associatedWith sto:BdvaDataViualisationAndUserInteraction ,
                                          sto:DtpEcosystemView ,
                                          sto:FiwareAdvancedUi ,
                                          sto:IviManagementView ;
                       sto:isDescribedin sto:IIRA ;
                       sto_iot:alignsWith sto:BdvaDataViualisationAndUserInteraction ,
                                          sto:DtpEcosystemView ,
                                          sto:FiwareAdvancedUi ,
                                          sto:IviManagementView ;
                       sto_iot:frames sto:AsProcessPlanning ,
                                      sto:DynamicAdjustability ,
                                      sto:Evolvability ,
                                      sto:RoleCategorization ,
                                      sto:ServiceChoreography ,
                                      sto:ServiceComposition ,
                                      sto:ServiceDeployment ,
                                      sto:ServiceLifecycleManagement ,
                                      sto:ServiceOrchestration ;
                       rdfs:label "IIRA Usage Viewpoint"@en ;
                       skos:note "Publications referred: '(IIC:PUB:G1:V1.80:20170131' '3.5.2 USAGE VIEWPOINT' 'Page 16' " .


###  https://w3id.org/i40/sto#IIRAUsageViewpointAnno
sto:IIRAUsageViewpointAnno rdf:type owl:NamedIndividual ,
                                    oa:Annotation ;
                           oa:hasBody sto:IIRAUsageViewpoint ;
                           oa:hasTarget [ rdf:type oa:SpecificResource ;
                                          dcterms:format "pdf" ;
                                          oa:hasSelector [ rdf:type oa:RangeSelector ;
                                                           oa:hasEndSelector [ rdf:type oa:XPathSelector ;
                                                                               rdf:value "Page 25"
                                                                             ] ;
                                                           oa:hasStartSelector [ rdf:type oa:XPathSelector ;
                                                                                 rdf:value "Page 22"
                                                                               ]
                                                         ] ;
                                          oa:hasSource sto:The_Industrial_Internet_of_Things_Volume_G1_Reference_Architecture
                                        ] ,
                                        [ rdf:type oa:SpecificResource ;
                                          dcterms:format "pdf" ;
                                          oa:hasSelector [ rdf:type oa:RangeSelector ;
                                                           oa:hasEndSelector [ rdf:type oa:XPathSelector ;
                                                                               rdf:value "Page 25"
                                                                             ] ;
                                                           oa:hasStartSelector [ rdf:type oa:XPathSelector ;
                                                                                 rdf:value "Page 22"
                                                                               ]
                                                         ] ;
                                          oa:hasSource sto:The_Industrial_Internet_of_Things_Volume_G1_Reference_Architecture
                                        ] .


###  https://w3id.org/i40/sto#IIRC
sto:IIRC rdf:type owl:NamedIndividual ,
                  sto:StandardizationFramework ;
         rdfs:comment "Industrial Internet Connectivity Framework"@en ;
         rdfs:isDefinedBy <https://www.iiconsortium.org/IICF.htm> ;
         rdfs:label "IICF"@en ;
         rdfs:seeAlso <https://www.iiconsortium.org/pdf/IIC_PUB_G5_V1.01_PB_20180228.pdf> .


###  https://w3id.org/i40/sto#IIoTConsortium
sto:IIoTConsortium rdf:type owl:NamedIndividual ;
                   dcterms:creator sto:sebastian .


###  https://w3id.org/i40/sto#IPSO
sto:IPSO rdf:type owl:NamedIndividual ,
                  foaf:Organization ,
                  sto:IIoTConsortium ;
         dcterms:creator sto:sebastian ;
         rdfs:comment "The Alliance is a global non-profit organization serving the various communities seeking to establish the Internet Protocol as the network for the connection of Smart Objects by providing coordinated marketing efforts available to the general public. (source: https://www.postscapes.com/internet-of-things-protocols/)"@en ;
         rdfs:label "IPSO"@en ;
         sto:hasOfficialResource <http://www.ipso-alliance.org/> .


###  https://w3id.org/i40/sto#IPv4Support
sto:IPv4Support rdf:type owl:NamedIndividual ,
                         sto_iot:Concern ;
                dcterms:creator sto:sebastian ;
                sto_iot:supports sto:SyntacticInteroperability ;
                rdfs:comment "Communication with non-IPv6 networks must be possible (IPv4, others)."@en ;
                rdfs:label "IPv4 Support"@en ;
                rdfs:seeAlso "IoT-A Requirement UNI.313" ;
                sto:hasDBpediaResource <http://dbpedia.org/resource/Internet_Protocol> ;
                sto:hasStakeholder "System Architect"@en .


###  https://w3id.org/i40/sto#IPv6
sto:IPv6 rdf:type owl:NamedIndividual ,
                  foaf:Document ,
                  sto:Publication ,
                  sto:TechnicalSpecification ;
         dcterms:creator sto:sebastian ;
         rdfs:comment "IPv6, is an Internet Layer protocol for packet-switched internetworking and provides end-to-end datagram transmission across multiple IP networks. (source: https://www.postscapes.com/internet-of-things-protocols/)"@en ;
         rdfs:label "IPv6"@en ;
         sto:hasWikipediaArticle <https://en.wikipedia.org/wiki/IPv6> ;
         sto_iot:hasTargetConcern sto:SyntacticInteroperability .


###  https://w3id.org/i40/sto#IPv6Support
sto:IPv6Support rdf:type owl:NamedIndividual ,
                         sto_iot:Concern ;
                dcterms:creator sto:sebastian ;
                sto_iot:supports sto:SyntacticInteroperability ;
                rdfs:comment "A system built using the ARM shall use/support common-addressing-schemes such as IPv6."@en ;
                rdfs:label "IPv6 Support"@en ;
                rdfs:seeAlso "IoT-A Requirement UNI.312" ;
                sto:hasDBpediaResource <http://dbpedia.org/resource/Internet_Protocol> ;
                sto:hasStakeholder "System Architect"@en .


###  https://w3id.org/i40/sto#ISA
sto:ISA rdf:type owl:NamedIndividual ,
                 foaf:Organization ,
                 sto:StandardOrganization ;
        sto:hasHeadquaterIn dbr:_North_Carolina ;
        sto:abbreviation "ISA"^^xsd:string ;
        sto:formationDate "1945-04-28"^^xsd:date ;
        sto:orgName "International Society of Automation"@en ;
        rdfs:comment "The International Society of Automation (www.isa.org) is a nonprofit professional association that sets the standard for those who apply engineering and technology to improve the management, safety, and cybersecurity of modern automation and control systems used across industry and critical infrastructure. Founded in 1945, ISA develops widely used global standards; certifies industry professionals; provides education and training; publishes books and technical articles; hosts conferences and exhibits; and provides networking and career development programs for its 40,000 members and 400,000 customers around the world."@en ;
        sto:hasDBpediaResource <http://dbpedia.org/resource/International_Society_of_Automation> ;
        sto:hasOfficialResource <https://www.isa.org/> ;
        sto:hasWikipediaArticle <https://en.wikipedia.org/wiki/International_Society_of_Automation> .


###  https://w3id.org/i40/sto#ISA-95
sto:ISA-95 rdf:type owl:NamedIndividual ,
                    sto:Standard ;
           dcterms:creator sto:irlan ;
           sto:hasDeveloper sto:ANSI ,
                            sto:ISA ;
           sto:hasPublisher sto:ANSI ,
                            sto:ISA ;
           sto:relatedTo sto:B2MML ,
                         sto:IEC_62264 ,
                         sto:ISA-95 ;
           rdfs:comment "ANSI/ISA-95, or ISA-95 as it is more commonly referred, is an international standard from the International Society of Automation for developing an automated interface between enterprise and control systems. This standard has been developed for global manufacturers. It was developed to be applied in all industries, and in all sorts of processes, like batch processes, continuous and repetitive processes.There are 5 parts of the ISA-95 standard.ISA-95 Models"@en ;
           rdfs:label "ISA 95"@en ;
           sto:hasDBpediaResource <http://dbpedia.org/resource/ANSI/ISA-95> ;
           sto:hasOfficialResource <https://www.isa.org/isa95/> ;
           sto:hasWikipediaArticle <https://en.wikipedia.org/wiki/ANSI/ISA-95> .


###  https://w3id.org/i40/sto#ISA10011a
sto:ISA10011a rdf:type owl:NamedIndividual ,
                       sto:TechnicalSpecification ;
              dcterms:creator sto:irlan ,
                              sto:sebastian ;
              rdfs:comment "ISA100.11a is a wireless networking technology standard developed by the International Society of Automation (ISA). The official description is Wireless Systems for Industrial Automation: Process Control and Related Application. (source: https://www.postscapes.com/internet-of-things-protocols/)"@en ;
              rdfs:label "ISA100.11a"@en ;
              sto:hasDBpediaResource <http://dbpedia.org/resource/ISA100.11a> ;
              sto:hasWikipediaArticle <https://en.wikipedia.org/wiki/ISA100.11a> .


###  https://w3id.org/i40/sto#ISA95
sto:ISA95 rdf:type owl:NamedIndividual ,
                   sto:StandardizationFramework ;
          sto:isDescribedin sto:IotaReferenceArchitecture ;
          rdfs:comment "Describes the ISA95 as a Standarization Initiative that classifies Standards"@en ;
          rdfs:label "ISA 95"@en .


###  https://w3id.org/i40/sto#ISA_62443
sto:ISA_62443 rdf:type owl:NamedIndividual ,
                       sto:Standard ;
           sto:hasPublisher sto:ISA ;
              rdfs:comment "Security for industrial automation and control systems"@en ;
              rdfs:label "ISA_62443"@en ;
              sto:publisher sto:ISA .


###  https://w3id.org/i40/sto#ISO
sto:ISO rdf:type owl:NamedIndividual ,
                 dul:Collection ,
                 sto:StandardOrganization ;
        sto:belongsTo dbr:Switzerland ;
        sto:hasHeadquaterIn dbr:Geneva ;
        sto:abbreviation "ISO"^^xsd:string ;
        sto:formationDate "1947-02-23"^^xsd:date ;
        sto:orgName "International Organization for Standardization"@en ,
                    "Internationale Organisation für Normung"@de ,
                    "Organisation internationale de normalisation"@fr ,
                    "The International Organization for Standardization"@en ,
                    "Международная организация по стандартизации"@ru ;
        rdfs:comment "Is an independent, non-governmental organization, the members of which are the standards organizations of the 162 member countries. It is the world's largest developer of voluntary international standards and facilitates world trade by providing common standards between nations. Nearly twenty thousand standards have been set covering everything from manufactured products and technology to food safety, agriculture and healthcare."@en ,
                     "The International Organization for Standardization (ISO) is an international standard-setting body composed of representatives from various national standards organizations."@en ;
        sto:hasDBpediaResource <http://dbpedia.org/page/International_Organization_for_Standardization> ;
        sto:hasOfficialResource <https://www.iso.org> ,
                                <https://www.iso.org/about-us.html> ;
        sto:hasWikipediaArticle <https://en.wikipedia.org/wiki/International_Organization_for_Standardization> .


###  https://w3id.org/i40/sto#ISO_10303
sto:ISO_10303 rdf:type owl:NamedIndividual ,
                       sto:Standard ;
              dcterms:creator sto:irlan ;
              sto:hasClassification sto:ProductLifeCycleManagement ;
              sto:hasPublisher sto:ISO ;
              sto:relatedTo sto:ISO_10303 ,
                            sto:ISO_8062-4 ;
              rdfs:comment "Standard for the Exchange of Product model data. ISO 10303 can represent 3D objects in Computer-aided design (CAD) and related information."@en ;
              rdfs:label "ISO 10303"@en ;
              skos:note "TODO - Split properly and classify it - check the NIST paper"@en ;
              sto:hasDBpediaResource <http://dbpedia.org/page/ISO_10303> ;
              sto:hasOfficialResource <https://www.steptools.com/stds/step/> ;
              sto:hasWikipediaArticle <https://en.wikipedia.org/wiki/ISO_10303> .


###  https://w3id.org/i40/sto#ISO_1101
sto:ISO_1101 rdf:type owl:NamedIndividual ,
                      sto:Standard ;
             dcterms:creator sto:irlan ;
             sto:hasClassification sto:ModelingPractice ,
                                   sto:RamiAssetlayer ,
                                   sto:RamiProduct ;
             sto:hasPublisher sto:ISO ;
             sto:hasPublicationDate "2017-02-01"^^xsd:date ;
             rdfs:comment "Geometrical product specifications (GPS) -- Geometrical tolerancing -- Tolerances of form, orientation, location and run-out"@en ;
             rdfs:label "ISO 1101"@en ;
             sto:hasOfficialResource <https://www.iso.org/standard/66777.html> .


###  https://w3id.org/i40/sto#ISO_11404
sto:ISO_11404 rdf:type owl:NamedIndividual ,
                       sto:Standard ;
              sto:hasDeveloper sto:IEC ,
                               sto:ISO ;
              sto:hasPublisher sto:ISO ;
              sto:hasPublicationDate "2007-12-01"^^xsd:date ;
              rdfs:comment "Information technology -- General-Purpose Datatypes (GPD)"@en ;
              rdfs:label "ISO/IEC 11404"@en ;
              sto:hasDBpediaResource <http://dbpedia.org/page/ISO/IEC_11404> ;
              sto:hasOfficialResource <https://webstore.iec.ch/publication/9602> ,
                                      <https://www.iso.org/standard/39479.html> ;
              sto:hasOpenResource <http://www.open-std.org/jtc1/sc22/open/n3620.pdf> ;
              sto:hasWikipediaArticle <https://en.wikipedia.org/wiki/ISO/IEC_11404> .


###  https://w3id.org/i40/sto#ISO_11783
sto:ISO_11783 rdf:type owl:NamedIndividual ,
                       sto:Standard ;
              dcterms:creator sto:irlan ;
              sto:hasPublisher sto:ISO ;
              sto:relatedTo sto:ISO_11783 ,
                            sto:ISO_11898-1 ;
              sto:hasTag "ISOBUS"@en ;
              rdfs:comment "ISO 11783, known as Tractors and machinery for agriculture and forestry—Serial control and communications data network is a communication protocol for the agriculture industry based on the SAE J1939 protocol (which includes CANbus)."@en ;
              rdfs:label "ISO 11783"@en ;
              sto:hasDBpediaResource <http://dbpedia.org/resource/ISO_11783> ;
              sto:hasOfficialResource <https://www.iso.org/standard/61646.html> ;
              sto:hasWikipediaArticle <https://en.wikipedia.org/wiki/ISO_11783> .


###  https://w3id.org/i40/sto#ISO_11898-1
sto:ISO_11898-1 rdf:type owl:NamedIndividual ,
                         sto:Standard ;
                dcterms:creator sto:irlan ;
                sto:hasClassification sto:AsEngineering ,
                                      sto:AsSafety  ,
                                      sto:RamiCommunicationlayer ;
                sto:hasPublisher sto:ISO ;
                sto:relatedTo sto:ISO_11783 ,
                              sto:ISO_11898-1 ;
                sto:hasPublicationDate "2015-12-01"^^xsd:date ;
                sto:hasTag "CAN Bus"@en ;
                rdfs:comment "Used mainly for Road vehicles Controller area network (CAN) Data link layer and physical signalling."@en ;
                rdfs:label "ISO 11898-1"@en ;
                sto:hasDBpediaResource <http://dbpedia.org/page/CAN_bus> ;
                sto:hasRelevantDomain sto:IndustrialAutomation ;
                sto:hasOfficialResource <https://www.iso.org/standard/63648.html> .


###  https://w3id.org/i40/sto#ISO_1302
sto:ISO_1302 rdf:type owl:NamedIndividual ,
                      sto:Standard ;
             sto:hasClassification sto:ModelingPractice ;
             sto:hasPublicationDate "2002-02-01"^^xsd:date ;
             rdfs:comment "Geometrical product specifications Standards"@en ;
             rdfs:label "ISO 1302"@en ;
                sto:hasPublisher sto:ISO ;
             sto:hasOfficialResource <https://www.iso.org/standard/28089.html> .


###  https://w3id.org/i40/sto#ISO_13374
sto:ISO_13374 rdf:type owl:NamedIndividual ,
                       sto:Standard ;
              dcterms:creator sto:irlan ;
              sto:hasClassification sto:AsConditionMonitoring ,
                                    sto:ProductionSystemEngineering ,
                                    sto:RamiBusinessLayer ,
                                    sto:RamiEnterprise ;
                sto:hasPublisher sto:ISO ;
              sto:hasPublisher sto:ISO ;
              sto:relatedTo sto:ISO_13374 ,
                            sto:ISO_15704 ,
                            sto:ISO_19439 ;
              sto:hasPublicationDate "2012-02-01"^^xsd:date ;
              rdfs:comment "Condition monitoring and diagnostics of machines -- Data processing, communication and presentation"@en ;
              rdfs:label "ISO 13374"@en ;
              sto:hasRelevantDomain sto:IndustrialAutomation ;
              sto:hasOfficialResource <https://www.iso.org/standard/61131.html> .


###  https://w3id.org/i40/sto#ISO_13485
sto:ISO_13485 rdf:type owl:NamedIndividual ,
                       sto:Standard ;
              dcterms:creator sto:irlan ;
              sto:hasClassification sto:AsSafety  ;
               sto_iot:hasTargetConcern sto:QualityOfService;
              sto:hasPublisher sto:ISO ;
              rdfs:comment "Medical devices -- Quality management systems -- Requirements for regulatory purposes."@en ;
              rdfs:label "ISO 13485"@en ;
              sto:hasDBpediaResource <http://dbpedia.org/page/ISO_13485> ;
              sto:hasOfficialResource <https://www.iso.org/iso-9001-quality-management.html> ;
              sto_iot:hasTargetConcern sto:QualityOfService .


###  https://w3id.org/i40/sto#ISO_13584
sto:ISO_13584 rdf:type owl:NamedIndividual ,
                       sto:Standard ;
              dcterms:creator sto:irlan ;
              sto:hasClassification sto:ProductCatalogData ;
              sto:hasPublisher sto:ISO ;
              sto:relatedTo sto:DIN_SPEC_16592 ,
                            sto:IEC_61131 ,
                            sto:IEC_61360 ,
                            sto:IEC_61499 ,
                            sto:IEC_61804 ,
                            sto:IEC_61850 ,
                            sto:IEC_61987_X ,
                            sto:IEC_62424 ,
                            sto:IEC_62453 ,
                            sto:IEC_62541 ,
                            sto:IEC_62714 ,
                            sto:ISO_13584 ,
                            sto:ISO_14306 ,
                            sto:ISO_15746 ,
                            sto:ISO_15926 ,
                            sto:ISO_18629 ,
                            sto:ISO_18828-2 ,
                            sto:ISO_20922 ,
                            sto:ISO_22400 ,
                            sto:ISO_29002 ,
                            sto:ISO_ASTM_52915 ,
                            sto:ISO_PAS_17506 ,
                            sto:MathML ,
                            sto:SysML ,
                            sto:eClass ;
              sto:hasMotivation "Standard data elements (properties) are used as elements in administration shell"@en ;
              sto:hasTag "Industrial automation systems and integration"@en ;
              dcterms:license sto:PrivateLicenseDocument ;
              rdfs:comment "ISO 13584 is a series of International Standards for the computer-sensible representation and exchange of parts library data. The objective is to provide a mechanism capable of transferring parts library data, independent from any particular system. The nature of this description makes it suitable not only for the exchange of files containing parts libraries, but also as a basis for implementing and sharing databases of parts library data, and archiving"@en ;
              rdfs:label "ISO 13584"@en ;
              sto:hasDBpediaResource <http://dbpedia.org/resource/ISO_13584> ;
              sto:hasOfficialResource <https://webstore.iec.ch/publication/5380%0Ahttp://www.iso.org/iso/catalogue_detail.htm?csnumber=43423> ;
              sto:hasWikipediaArticle <https://en.wikipedia.org/wiki/ISO_13584> .


###  https://w3id.org/i40/sto#ISO_13849
sto:ISO_13849 rdf:type owl:NamedIndividual ,
                       sto:Standard ;
              dcterms:creator sto:irlan ;
              sto:hasClassification sto:AsSafety ,
                                    sto:IDSRAMCertification ,
                                    sto:IIRASecurity ;
              sto:hasDomain sto:Safety_Machinery ;
              sto:hasPublisher sto:ISO ;
              sto:relatedTo sto:IEC_61508 ,
                            sto:IEC_61511 ,
                            sto:IEC_62061 ,
                            sto:ISO_13849 ;
              rdfs:comment "Provides safety requirements and guidance on the principles for the design and integration of safety-related parts of control systems (SRP/CS), including the design of software."@en ;
              rdfs:label "ISO 13849"@en ;
              sto:hasDBpediaResource <http://dbpedia.org/resource/ISO_13849> ;
              sto:hasOfficialResource <http://www.iso.org/iso/home/store/catalogue_tc/catalogue_detail.htm?csnumber=69883> ;
              sto:hasWikipediaArticle <https://en.wikipedia.org/wiki/ISO_13849> ;
              sto_iot:hasTargetConcern sto:Safety .


###  https://w3id.org/i40/sto#ISO_14306
sto:ISO_14306 rdf:type owl:NamedIndividual ,
                       foaf:Document ,
                       sto:Publication ,
                       sto:Standard ;
              dcterms:creator sto:irlan ;
              sto:hasClassification sto:AsEngineering ,
                                    sto:AsIdentification ,
                                    sto:AsProcessPlanning ,
                                    sto:ProductionSystemModelData ,
                                    sto:RamiAssetlayer ,
                                    sto:RamiProduct ;
              sto:hasPublisher sto:ISO ;
              sto:relatedTo sto:DIN_SPEC_16592 ,
                            sto:IEC_61131 ,
                            sto:IEC_61360 ,
                            sto:IEC_61499 ,
                            sto:IEC_61804 ,
                            sto:IEC_61850 ,
                            sto:IEC_61987_X ,
                            sto:IEC_62424 ,
                            sto:IEC_62453 ,
                            sto:IEC_62541 ,
                            sto:IEC_62714 ,
                            sto:ISO_13584 ,
                            sto:ISO_14306 ,
                            sto:ISO_15746 ,
                            sto:ISO_15926 ,
                            sto:ISO_18629 ,
                            sto:ISO_18828-2 ,
                            sto:ISO_20922 ,
                            sto:ISO_22400 ,
                            sto:ISO_29002 ,
                            sto:ISO_ASTM_52915 ,
                            sto:ISO_PAS_17506 ,
                            sto:MathML ,
                            sto:SysML ,
                            sto:eClass ;
              sto:hasPublicationDate "2017-07-01"^^xsd:date ;
              rdfs:comment "It provides the description of the structure and content for a binary file having the extension of .jt. A binary file with the .jt extension is generally referred to as a JT file. The JT format described in ISO 14306:2012 is used primarily in industrial use cases as the means for capturing and repurposing lightweight 3D product definition data"@en ;
              rdfs:label "ISO 14306"@en ;
              sto:hasRelevantDomain sto:CAD ;
              sto:hasOfficialResource <https://www.iso.org/standard/60572.html> .


###  https://w3id.org/i40/sto#ISO_14443
sto:ISO_14443 rdf:type owl:NamedIndividual ,
                       foaf:Document ,
                       sto:Publication ,
                       sto:Standard ;
              dcterms:creator sto:irlan ;
              foaf:maker sto:IEC ,
                         sto:ISO ;
              sto:hasPublisher sto:IEC ,
                               sto:ISO ;
              rdfs:comment "ISO 14443 Identification cards -- Contactless integrated circuit cards -- Proximity cards is an international standard that defines proximity cards used for identification, and the transmission protocols for communicating with it"@en ;
              rdfs:label "ISO 14443"@en .


###  https://w3id.org/i40/sto#ISO_14739-1
sto:ISO_14739-1 rdf:type owl:NamedIndividual ,
                         foaf:Document ,
                         sto:Publication ,
                         sto:Standard ;
                dcterms:creator sto:irlan ;
                sto:hasClassification sto:NISTProductModelDataExchange ;
                sto:hasPublisher sto:ISO ;
                sto:hasPublicationDate "2014-12-01"^^xsd:date ;
                rdfs:comment "Document management -- 3D use of Product Representation Compact (PRC) format-ISO 14739-1:2014 describes PRC 10001 of a product representation compact (PRC) file format for three dimensional (3D) content data. This format is designed to be included in PDF (ISO 32000) and other similar document formats for the purpose of 3D visualization and exchange. "@en ;
                rdfs:label "ISO 14739-1"@en ;
                skos:altLabel "STEP"@en ;
                sto:hasRelevantDomain sto:CAD ;
                sto:hasOfficialResource <https://www.iso.org/standard/54948.html> .


###  https://w3id.org/i40/sto#ISO_15408
sto:ISO_15408 rdf:type owl:NamedIndividual ,
                       foaf:Document ,
                       sto:Publication ,
                       sto:Standard ;
              dcterms:creator sto:irlan ;
              sto:hasClassification sto:IIRASecurity ;
              sto:hasPublisher sto:ISO ;
              dc:title "Common Criteria for Information Technology Security Evaluation"@en ;
              rdfs:comment "The Common Criteria for Information Technology Security Evaluation (abbreviated as Common Criteria or CC) is an international standard (ISO/IEC 15408) for computer security certification"@en ;
              rdfs:label "ISO/IEC 15408"@en ;
              sto:hasOfficialResource <https://webstore.iec.ch/publication/10255> ,
                                      <https://www.iso.org/standard/50341.html> ,
                                      <https://www.niap-ccevs.org/Documents_and_Guidance/cc_docs.cfm> ;
              sto:hasOpenResource <http://comsec.spb.ru/matherials/is/iso15408-1.pdf> ,
                                  <http://www.comsec.spb.ru/matherials/is/iso15408-3.pdf> ;
              sto:hasWikipediaArticle <http://wikipedia.org/wiki/Common_Criteria_for_Information_Technology_Security_Evaluation> .


###  https://w3id.org/i40/sto#ISO_15459
sto:ISO_15459 rdf:type owl:NamedIndividual ,
                       sto:Standard ;
              rdfs:label "ISO 15459"^^xsd:string ;              
              rdfs:comment "ISO/IEC 15459-1:2014 specifies a unique string of characters for the identification of individual transport units. The character string is intended to be represented in a bar code label or other AIDC media attached to the entity to meet management needs. To address management needs, different types of entities are recognized in the various parts of ISO/IEC 15459, which allows different requirements to be met by the identities associated with each type. The rules for the unique identification for individual transport units, to identify physical logistical transfers, with the identity relevant for the duration of one or more items in the load being held or transported as part of that load, are defined and supported by example."@en ;
              dcterms:creator sto:irlan ;
              sto:hasPublisher sto:IEC ,
                               sto:ISO ;
              rdfs:label "ISO 15459" .


###  https://w3id.org/i40/sto#ISO_15531
sto:ISO_15531 rdf:type owl:NamedIndividual ,
                       sto:Standard ;
              dcterms:creator sto:irlan ;
              sto:hasDomain sto:IndustrialProcessMeasurementControl ;
              sto:hasPublisher sto:ISO ;
              sto:relatedTo sto:ISO_15531 ,
                            sto:ISO_15531-2x ,
                            sto:ISO_15531-3x ,
                            sto:ISO_15531-4x ;
              sto:hasTag "MANDATE"@en ;
              rdfs:comment "This Standard models manufacturing management data such as, Resources management data (Resource model); Time related features (Time model); Flow management data in manufacturing (Flow management model)."@en ;
              rdfs:isDefinedBy <https://www.researchgate.net/publication/220171079_ISO_15531_MANDATE_a_standardised_data_model_for_manufacturing_management> ;
              rdfs:label "ISO 15531"@en ;
              sto:hasRelevantDomain sto:IndustrialProcessMeasurementControl ;
              sto:hasOfficialResource <https://www.iso.org/standard/28144.html> .


###  https://w3id.org/i40/sto#ISO_15531-2x
sto:ISO_15531-2x rdf:type owl:NamedIndividual ,
                          foaf:Document ,
                          sto:Publication ,
                          sto:Standard ,
                          sto:StandardPart ;
                 dul:isComponentOf sto:ISO_15531 ;
              sto:hasPublisher sto:ISO ;
                 sto:relatedTo sto:ISO_15531 ,
                               sto:ISO_15531-2x ,
                               sto:ISO_15531-3x ,
                               sto:ISO_15531-4x ;
                 rdfs:comment "Production data for external exchanges. refering to the representation of product information to be exchanged with the external environment (customers and suppliers), with the aim to model the main production information exchanged between industrial companies, in order to improve exchanges and integration through the use of EDI protocols."@en ;
                 rdfs:isDefinedBy <https://www.researchgate.net/publication/220171079_ISO_15531_MANDATE_a_standardised_data_model_for_manufacturing_management> ;
                 rdfs:label "ISO 15531 2x series"@en .


###  https://w3id.org/i40/sto#ISO_15531-3x
sto:ISO_15531-3x rdf:type owl:NamedIndividual ,
                          foaf:Document ,
                          sto:Publication ,
                          sto:Standard ,
                          sto:StandardPart ;
                 dul:isComponentOf sto:ISO_15531 ;
                 sto:hasPublisher sto:ISO ;
                 sto:relatedTo sto:ISO_15531 ,
                               sto:ISO_15531-2x ,
                               sto:ISO_15531-3x ,
                               sto:ISO_15531-4x ;
                 rdfs:comment "Manufacturing resource usage management data sto: refering to the way of managing the use of resources, such as resource configuration and capabilities, operation management of manufacturing devices, installations and facilities."@en ;
                 rdfs:isDefinedBy <https://www.researchgate.net/publication/220171079_ISO_15531_MANDATE_a_standardised_data_model_for_manufacturing_management> ;
                 rdfs:label "ISO 15531 3x series"@en .


###  https://w3id.org/i40/sto#ISO_15531-4x
sto:ISO_15531-4x rdf:type owl:NamedIndividual ,
                          foaf:Document ,
                          sto:Publication ,
                          sto:Standard ,
                          sto:StandardPart ;
                 dul:isComponentOf sto:ISO_15531 ;
              sto:hasPublisher sto:ISO ;
                 sto:relatedTo sto:ISO_15531 ,
                               sto:ISO_15531-2x ,
                               sto:ISO_15531-3x ,
                               sto:ISO_15531-4x ;
                 rdfs:comment "Manufacturing flow management data sto: refering to the material flow control and aiming at the representation of data and elements supporting the control and monitoring of the flow of materials in manufacturing processes."@en ;
                 rdfs:isDefinedBy <https://www.researchgate.net/publication/220171079_ISO_15531_MANDATE_a_standardised_data_model_for_manufacturing_management> ;
                 rdfs:label "ISO 15531 4x series"@en .


###  https://w3id.org/i40/sto#ISO_15704
sto:ISO_15704 rdf:type owl:NamedIndividual ,
                       sto:Standard ;
              dcterms:creator sto:irlan ;
              sto:hasClassification sto:RamiBusinessLayer ,
                                    sto:RamiEnterprise ;
              sto:hasPublisher sto:ISO ;
              sto:relatedTo sto:ISO_13374 ,
                            sto:ISO_15704 ,
                            sto:ISO_19439 ;
              sto:hasPublicationDate "2000-06-01"^^xsd:date ;
              rdfs:comment "Identifies requirements for enterprise-reference architectures and methodologies"@en ;
              rdfs:label "ISO 15704"@en ;
              sto:hasRelevantDomain sto:IndustrialAutomation ;
              sto:hasOfficialResource <https://www.iso.org/standard/28777.html> .


###  https://w3id.org/i40/sto#ISO_15746
sto:ISO_15746 rdf:type owl:NamedIndividual ,
                       sto:Standard ;
              dcterms:creator sto:irlan ;
              sto:hasClassification sto:AsEngineering ,
                                    sto:ProductLifeCycleManagement ,
                                    sto:RamiCommunicationlayer ,
                                    sto:RamiControlDevice ,
                                    sto:RamiFieldDevice ,
                                    sto:RamiFunctional ,
                                    sto:RamiInformationLayer ,
                                    sto:RamiIntegrationLayer ,
                                    sto:RamiProduct ;
              sto:hasPublisher sto:ISO ;
              sto:relatedTo sto:DIN_SPEC_16592 ,
                            sto:IEC_61131 ,
                            sto:IEC_61360 ,
                            sto:IEC_61499 ,
                            sto:IEC_61804 ,
                            sto:IEC_61850 ,
                            sto:IEC_61987_X ,
                            sto:IEC_62424 ,
                            sto:IEC_62453 ,
                            sto:IEC_62541 ,
                            sto:IEC_62714 ,
                            sto:ISO_13584 ,
                            sto:ISO_14306 ,
                            sto:ISO_15746 ,
                            sto:ISO_15926 ,
                            sto:ISO_18629 ,
                            sto:ISO_18828-2 ,
                            sto:ISO_20922 ,
                            sto:ISO_22400 ,
                            sto:ISO_29002 ,
                            sto:ISO_ASTM_52915 ,
                            sto:ISO_PAS_17506 ,
                            sto:MathML ,
                            sto:SysML ,
                            sto:eClass ;
              sto:hasPublicationDate "2015-04-01"^^xsd:date ;
              rdfs:comment "Automation systems and integration -- Integration of advanced process control and optimization capabilities for manufacturing systems."@en ;
              rdfs:label "ISO 15746"@en ;
              sto:hasRelevantDomain sto:IndustrialAutomation ;
              sto:hasOfficialResource <https://www.iso.org/standard/61131.html> .


###  https://w3id.org/i40/sto#ISO_15926
sto:ISO_15926 rdf:type owl:NamedIndividual ,
                       sto:Standard ;
              dcterms:creator sto:irlan ;
              sto:hasClassification sto:AsEngineering ,
                                    sto:AsConfiguration ,
                                    sto:ProductLifeCycleManagement ,
                                    sto:RamiIntegrationLayer ,
                                    sto:RamiProduct ;
              sto:hasPublisher sto:ISO ;
              sto:relatedTo sto:DIN_SPEC_16592 ,
                            sto:IEC_61131 ,
                            sto:IEC_61360 ,
                            sto:IEC_61499 ,
                            sto:IEC_61804 ,
                            sto:IEC_61850 ,
                            sto:IEC_61987_X ,
                            sto:IEC_62424 ,
                            sto:IEC_62453 ,
                            sto:IEC_62541 ,
                            sto:IEC_62714 ,
                            sto:ISO_13584 ,
                            sto:ISO_14306 ,
                            sto:ISO_15746 ,
                            sto:ISO_15926 ,
                            sto:ISO_18629 ,
                            sto:ISO_18828-2 ,
                            sto:ISO_20922 ,
                            sto:ISO_22400 ,
                            sto:ISO_29002 ,
                            sto:ISO_ASTM_52915 ,
                            sto:ISO_PAS_17506 ,
                            sto:MathML ,
                            sto:SysML ,
                            sto:eClass ;
              sto:hasPublicationDate "2003-12-01"^^xsd:date ;
              rdfs:comment "Industrial automation systems and integration -- Integration of life-cycle data for process plants including oil and gas production facilities."@en ;
              rdfs:label "ISO 15926"@en ;
              sto:hasRelevantDomain sto:IndustrialAutomation ;
              sto:hasOfficialResource <https://www.iso.org/standard/29557.html> .


###  https://w3id.org/i40/sto#ISO_16739
sto:ISO_16739 rdf:type owl:NamedIndividual ,
                       sto:Standard ;
              dcterms:creator sto:irlan ;
              sto:hasClassification sto:AsLifecycle_Status ,
                                    sto:ProductLifeCycleManagement ,
                                    sto:RamiStation ,
                                    sto:RamiWorkCenter ;
              sto:hasPublisher sto:ISO ;
              sto:relatedTo sto:IEC_62890 ,
                            sto:ISO_16739 ;
              sto:hasPublicationDate "2013-04-01"^^xsd:date ;
              rdfs:comment "Industry Foundation Classes (IFC) for data sharing in the construction and facility management industries."@en ;
              rdfs:label "ISO 16739"@en ;
              sto:hasRelevantDomain sto:IndustrialAutomation ;
              sto:hasOfficialResource <https://www.iso.org/standard/51622.html> .


###  https://w3id.org/i40/sto#ISO_16792
sto:ISO_16792 rdf:type owl:NamedIndividual ,
                       sto:Standard ;
              dcterms:creator sto:irlan ;
              sto:hasClassification sto:ModelingPractice ,
                                    sto:RamiAssetlayer ,
                                    sto:RamiProduct ;
              sto:hasPublisher sto:ISO ;
              sto:hasPublicationDate "2015-12-01"^^xsd:date ;
              rdfs:comment "ISO 16792 Technical product documentation -- Digital product definition data practices-It supports two methods of application: model-only and model and drawing in digital format."@en ;
              rdfs:label "ISO 16792"@en ;
              sto:hasRelevantDomain sto:CAD ;
              sto:hasOfficialResource <https://www.iso.org/standard/56865.html> .


###  https://w3id.org/i40/sto#ISO_18629
sto:ISO_18629 rdf:type owl:NamedIndividual ,
                       sto:Standard ;
              dcterms:creator sto:irlan ;
              sto:hasClassification sto:AsConfiguration ,
                                    sto:NISTProductModelDataExchange ,
                                    sto:RamiCommunicationlayer ,
                                    sto:RamiControlDevice ,
                                    sto:RamiFieldDevice ,
                                    sto:RamiFunctionalLayer ,
                                    sto:RamiInformationLayer ,
                                    sto:RamiIntegrationLayer ,
                                    sto:RamiProduct ;
              sto:hasPublisher sto:ISO ;
              sto:relatedTo sto:DIN_SPEC_16592 ,
                            sto:IEC_61131 ,
                            sto:IEC_61360 ,
                            sto:IEC_61499 ,
                            sto:IEC_61804 ,
                            sto:IEC_61850 ,
                            sto:IEC_61987_X ,
                            sto:IEC_62424 ,
                            sto:IEC_62453 ,
                            sto:IEC_62541 ,
                            sto:IEC_62714 ,
                            sto:ISO_13584 ,
                            sto:ISO_14306 ,
                            sto:ISO_15746 ,
                            sto:ISO_15926 ,
                            sto:ISO_18629 ,
                            sto:ISO_18828-2 ,
                            sto:ISO_20922 ,
                            sto:ISO_22400 ,
                            sto:ISO_29002 ,
                            sto:ISO_ASTM_52915 ,
                            sto:ISO_PAS_17506 ,
                            sto:MathML ,
                            sto:SysML ,
                            sto:eClass ;
              sto:hasPublicationDate "2004-11-01"^^xsd:date ;
              sto:hasTag "PSL"@en ;
              rdfs:comment "ISO 18629-1:2004 provides a general overview of the different series of parts of ISO 18629, which defines a process specification language aimed at identifying, formally defining and structuring the semantic concepts intrinsic to the capture and exchange of process information related to discrete manufacturing."@en ;
              rdfs:label "ISO 19629"@en ;
              sto:hasRelevantDomain sto:IndustrialAutomation ;
              sto:hasOfficialResource <https://www.iso.org/standard/35431.html> ;
              sto:hasWikipediaArticle <https://en.wikipedia.org/wiki/Process_Specification_Language> .


###  https://w3id.org/i40/sto#ISO_18828-2
sto:ISO_18828-2 rdf:type owl:NamedIndividual ,
                         sto:Standard ;
                dcterms:creator sto:irlan ;
                sto:hasClassification sto:AsEngineering ,
                                      sto:RamiControlDevice ,
                                      sto:RamiEnterprise ,
                                      sto:RamiFieldDevice ,
                                      sto:RamiProduct ,
                                      sto:RamiStation ,
                                      sto:RamiWorkCenter ;
                sto:hasPublisher sto:ISO ;
                sto:relatedTo sto:DIN_SPEC_16592 ,
                              sto:IEC_61131 ,
                              sto:IEC_61360 ,
                              sto:IEC_61499 ,
                              sto:IEC_61804 ,
                              sto:IEC_61850 ,
                              sto:IEC_61987_X ,
                              sto:IEC_62424 ,
                              sto:IEC_62453 ,
                              sto:IEC_62541 ,
                              sto:IEC_62714 ,
                              sto:ISO_13584 ,
                              sto:ISO_14306 ,
                              sto:ISO_15746 ,
                              sto:ISO_15926 ,
                              sto:ISO_18629 ,
                              sto:ISO_18828-2 ,
                              sto:ISO_20922 ,
                              sto:ISO_22400 ,
                              sto:ISO_29002 ,
                              sto:ISO_ASTM_52915 ,
                              sto:ISO_PAS_17506 ,
                              sto:MathML ,
                              sto:SysML ,
                              sto:eClass ;
                sto:hasPublicationDate "2016-10-01"^^xsd:date ;
                rdfs:comment "Industrial automation systems and integration -- Standardized procedures for production systems engineering."@en ;
                rdfs:label "ISO 18828-2"@en ;
                sto:hasRelevantDomain sto:IndustrialAutomation ;
                sto:hasOfficialResource <https://www.iso.org/standard/63505.html> .


###  https://w3id.org/i40/sto#ISO_19439
sto:ISO_19439 rdf:type owl:NamedIndividual ,
                       sto:Standard ;
              dcterms:creator sto:irlan ;
              dul:associatedWith sto:Certification ;
              sto:hasClassification sto:RamiBusinessLayer ;
              sto:hasPublisher sto:ISO ;
              sto:relatedTo sto:ISO_13374 ,
                            sto:ISO_15704 ,
                            sto:ISO_19439 ;
              rdfs:comment "Provides a unified conceptual basis for model-based enterprise engineering that enables consistency, convergence and interoperability of the various modelling methodologies and supporting tools."@en ;
              rdfs:label "ISO 19439"@en ;
              sto:hasDBpediaResource <http://dbpedia.org/page/ISO_19439> ;
              sto:hasOfficialResource <https://www.iso.org/standard/33833.html> ;
              sto:hasWikipediaArticle <https://en.wikipedia.org/wiki/ISO_19439> .


###  https://w3id.org/i40/sto#ISO_19440
sto:ISO_19440 rdf:type owl:NamedIndividual ,
                       sto:TechnicalSpecification ;
              dcterms:creator sto:irlan ;
              sto:hasClassification sto:AsEngineering ,
                                    sto:EnterpriseLevel ,
                                    sto:RamiEnterprise ,
                                    sto:RamiIntegrationLayer ,
                                    sto:RamiProduct ;
              sto:hasPublisher sto:ISO ;
              sto:relatedTo sto:BPMN ,
                            sto:ISO_19440 ;
              sto:hasPublicationDate "2007-12-01"^^xsd:date ;
              rdfs:comment "Enterprise integration -- Constructs for enterprise modelling-specifies the characteristics of the core constructs necessary for computer-supported modelling of enterprises conforming to ISO 19439.."@en ;
              rdfs:label "ISO 19440"@en ;
              sto:hasRelevantDomain sto:EnterpriseIntegration ;
              sto:hasOfficialResource <https://www.iso.org/standard/33834.html> .


###  https://w3id.org/i40/sto#ISO_19770
sto:ISO_19770 rdf:type owl:NamedIndividual ,
                       sto:Standard ;
              dcterms:creator sto:irlan ;
              sto:hasClassification sto:IIRASecurity ;
              sto:hasDeveloper sto:ISO ;
              sto:hasPublisher sto:IEC ,
                               sto:ISO ;
              sto:hasPublicationDate "2017-12-01"^^xsd:date ;
              dcterms:title "Information technology — Software asset management"@en ;
              rdfs:comment "International standards in the ISO/IEC 19770 family of standards for IT asset management (ITAM) address both the processes and technology for managing software assets and related IT assets. Broadly speaking, the standard family belongs to the set of Software Asset Management (or SAM) standards and is integrated with other Management System Standards."@en ;
              rdfs:label "ISO/IEC 19770"@en ;
              sto:hasDBpediaResource <http://dbpedia.org/resource/ISO/IEC_19770> ;
              sto:hasWikipediaArticle <https://en.wikipedia.org/wiki/ISO/IEC_19770> .


###  https://w3id.org/i40/sto#ISO_19941
sto:ISO_19941 rdf:type owl:NamedIndividual ,
                       sto:Standard ;
              dcterms:creator sto:sebastian ;
              dcterms:title "Cloud Computing - Interoperability and Portability"@en ;
              sto_iot:hasTargetConcern sto:CloudComputing;
              rdfs:comment "Description of the ecosystem of devices and cloud services and the related flows of data between cloud services, cloud service customers, cloud service users and their devices. These are necessary to provide guidance about how data is used on the devices in the context of the cloud computing ecosystem and the associated location and identity issues that emerge from such use."@en ;
              rdfs:label "ISO/IEC 19941:2017"@en ;
              sto:hasPublisher sto:IEC ,
                               sto:ISO ;
              sto:hasOfficialResource <http://standards.iso.org/ittf/PubliclyAvailableStandards/c066639_ISO_IEC_19941_2017.zip> ;
              sto_iot:hasTargetConcern sto:CloudComputing .



###  https://w3id.org/i40/sto#ISO_20140_5
sto:ISO_20140_5 rdf:type owl:NamedIndividual ,
                         sto:Standard ;
                dcterms:creator sto:irlan ;
                sto:hasPublisher sto:ISO ;
                sto:hasTag "Energy Efficiency"@en ;
                rdfs:comment "Automation systems and integration -- Evaluating energy efficiency and other factors of manufacturing systems that influence the environment"@en ;
                rdfs:label "ISO 20140-5"@en ;
                sto:hasOfficialResource <http://www.iso.org/iso/catalogue_detail.htm?csnumber=54809> .



###  https://w3id.org/i40/sto#ISO_20140_P1
sto:ISO_20140_P1 rdf:type owl:NamedIndividual ,
                          sto:Standard ;
                 dcterms:creator sto:irlan ;
                 sto:hasClassification sto:IIRASecurity ;
                 sto:hasDeveloper sto:ISO ;
                 sto:hasPublisher sto:ISO ;
                 sto_iot:frames sto:EnergyEfficiency ;
                 sto:isPartOf sto:ISO_20140_5;
                 sto:hasPublicationDate "2013-05-01"^^xsd:date ;
                 dcterms:title "Automation systems and integration -- Evaluating energy efficiency and other factors of manufacturing systems that influence the environment -- Part 1: Overview and general principles"@en ;
                 rdfs:comment "Evaluating the energy efficiency of a manufacturing system and other factors, e.g. energy consumption, waste and release, etc., that influence the environment. The evaluation method provides guidelines to analyse the usage of energy by the manufacturing system and the effects of the manufacturing system on the environment. ISO 20140 systematically evaluates the environmental influence through analysing the manufacturing activities and the manufacturing system. (source: iso.org)"@en ;
                 rdfs:label "ISO 20140-1:2013"@en ;
                 sto:hasOfficialResource <https://www.iso.org/standard/54809.html> .


###  https://w3id.org/i40/sto#ISO_20546
sto:ISO_20546 rdf:type owl:NamedIndividual ,
                       sto:Standard ;
              dcterms:creator sto:irlan ;
              sto:hasPublisher sto:IEC ,
                               sto:ISO ;
              dcterms:title "Big data -- Overview and vocabulary"@en ;
              rdfs:comment "TODO: check with other reference architecture standards"@en ;
              rdfs:label "ISO/IEC 20546"@en .


###  https://w3id.org/i40/sto#ISO_20547-3
sto:ISO_20547-3 rdf:type owl:NamedIndividual ,
                         sto:Standard ;
                dcterms:creator sto:irlan ;
                sto:hasPublisher sto:IEC ,
                                 sto:ISO ;
                dcterms:title "Big data reference architecture -- Part 3: Reference architecture"@en ;
                rdfs:comment "TODO: how is this standard related to other reference architecture description formats?"@en ,
                             "under development (as from 2018-07-23)"@en ;
                rdfs:label "ISO/IEC DIS 20547-3"@en ;
                sto:hasOfficialResource <https://www.iso.org/standard/71277.html> .


###  https://w3id.org/i40/sto#ISO_20547-4
sto:ISO_20547-4 rdf:type owl:NamedIndividual ,
                         sto:Standard ;
                dcterms:creator sto:irlan ;
                sto:hasPublisher sto:IEC ,
                                 sto:ISO ;
                dcterms:title "Big data reference architecture -- Part 4: Security and privacy"@en ;
                rdfs:comment "TODO: check with other reference architecture description frameworks"@en ,
                             "under development (as from 2018-07-23)"@en ;
                rdfs:label "ISO/IEC AWI 20547-4"@en ;
                sto:hasOfficialResource <https://www.iso.org/standard/71278.html> .


###  https://w3id.org/i40/sto#ISO_20922
sto:ISO_20922 rdf:type owl:NamedIndividual ,
                       sto:Standard ;
              dcterms:creator sto:irlan ;
              sto:hasClassification sto:InformationDomain ;
              sto:hasDeveloper sto:IBM ,
                               sto:OASIS ;
              sto:hasDomain sto:M2M ;
              sto:hasPublisher sto:IEC ,
                               sto:ISO ;
              sto:relatedTo sto:DIN_SPEC_16592 ,
                            sto:IEC_61131 ,
                            sto:IEC_61360 ,
                            sto:IEC_61499 ,
                            sto:IEC_61804 ,
                            sto:IEC_61850 ,
                            sto:IEC_61987_X ,
                            sto:IEC_62424 ,
                            sto:IEC_62453 ,
                            sto:IEC_62541 ,
                            sto:IEC_62714 ,
                            sto:ISO_13584 ,
                            sto:ISO_14306 ,
                            sto:ISO_15746 ,
                            sto:ISO_15926 ,
                            sto:ISO_18629 ,
                            sto:ISO_18828-2 ,
                            sto:ISO_20922 ,
                            sto:ISO_22400 ,
                            sto:ISO_29002 ,
                            sto:ISO_ASTM_52915 ,
                            sto:ISO_PAS_17506 ,
                            sto:MathML ,
                            sto:SysML ,
                            sto:eClass ;
              sto:hasPublicationDate "2016-06-01"^^xsd:date ;
              sto:hasTag "MQTT"@en ,
                         "Message Queue Telemetry Transport"@en ;
              rdfs:comment "ISO/IEC 20922:2016 is a Client Server publish/subscribe messaging transport protocol. It is light weight, open, simple, and designed so as to be easy to implement. These characteristics make it ideal for use in many situations, including constrained environments such as for communication in Machine to Machine (M2M) and Internet of Things (IoT) contexts where a small code footprint is required and/or network bandwidth is at a premium."@en ;
              rdfs:label "ISO 20922"@en ;
              sto:hasDBpediaResource <http://dbpedia.org/resource/MQTT> ;
              sto:hasRelevantDomain sto:M2M ;
              sto:hasOfficialResource <http://mqtt.org/> ,
                                      <https://www.iso.org/standard/69466.html> ;
              sto:hasWikipediaArticle <https://en.wikipedia.org/wiki/MQTT> .


###  https://w3id.org/i40/sto#ISO_22400
sto:ISO_22400 rdf:type owl:NamedIndividual ,
                       sto:Standard ;
              dcterms:creator sto:irlan ;
              sto:hasClassification sto:AsConditionMonitoring ,
                                    sto:AsLifecycle_Status ,
                                    sto:RamiBusinessLayer ,
                                    sto:RamiConnectedWorld ,
                                    sto:RamiControlDevice ,
                                    sto:RamiEnterprise ,
                                    sto:RamiFieldDevice ,
                                    sto:RamiStation ,
                                    sto:RamiWorkCenter ;
              sto:hasPublisher sto:ISO ;
              sto:relatedTo sto:DIN_SPEC_16592 ,
                            sto:IEC_61131 ,
                            sto:IEC_61360 ,
                            sto:IEC_61499 ,
                            sto:IEC_61804 ,
                            sto:IEC_61850 ,
                            sto:IEC_61987_X ,
                            sto:IEC_62424 ,
                            sto:IEC_62453 ,
                            sto:IEC_62541 ,
                            sto:IEC_62714 ,
                            sto:ISO_13584 ,
                            sto:ISO_14306 ,
                            sto:ISO_15746 ,
                            sto:ISO_15926 ,
                            sto:ISO_18629 ,
                            sto:ISO_18828-2 ,
                            sto:ISO_20922 ,
                            sto:ISO_22400 ,
                            sto:ISO_29002 ,
                            sto:ISO_ASTM_52915 ,
                            sto:ISO_PAS_17506 ,
                            sto:MathML ,
                            sto:SysML ,
                            sto:eClass ;
              sto:hasPublicationDate "2014-01-01"^^xsd:date ;
              rdfs:comment "Automation systems and integration -- Key performance indicators (KPIs) for manufacturing operations management."@en ;
              rdfs:label "ISO 22400"@en ;
              sto:hasRelevantDomain sto:IndustrialAutomation ;
              sto:hasOfficialResource <https://www.iso.org/standard/54497.html> .


###  https://w3id.org/i40/sto#ISO_22745-11
sto:ISO_22745-11 rdf:type owl:NamedIndividual ,
                          sto:Standard ;
                 dcterms:creator sto:irlan ;
                 sto:hasAvailableLanguage lang:eng ;
                 sto:hasClassification sto:ProductCatalogData ,
                                       sto:RamiAssetlayer ,
                                       sto:RamiProduct ;
                 sto:hasPublisher sto:ISO ;
                 sto:hasPublicationDate "2010-02-01"^^xsd:date ;
                 rdfs:comment "ISO 22745-11:2010 provides guidelines that are recommended for the development of terminology for concepts in an open technical dictionary (OTD).Compliance with these guidelines is not required in order for a term or definition to be included in an OTD. These guidelines are provided as a framework for developers of industrial terminology to ensure that definitions are consistent and understandable. Terminology that complies with these guidelines will be marked as such in the OTD. This will allow a user to perform a search that filters terminology based on compliance with ISO 22745-11:2010."@en ;
                 rdfs:label "ISO 22745-11"@en ;
                 sto:hasRelevantDomain sto:IndustrialAutomation ;
                 sto:hasAvailableLanguage lang:eng;
                 sto:hasOfficialResource <https://www.iso.org/standard/53999.html> .


###  https://w3id.org/i40/sto#ISO_24760
sto:ISO_24760 rdf:type owl:NamedIndividual ,
                       sto:Standard  ;
              dcterms:creator sto:irlan ;
              rdfs:label "ISO 24760"@en ;
              rdfs:comment """ISO/IEC 24760-1:2011

    defines terms for identity management, and
    specifies core concepts of identity and identity management and their relationships.

It is applicable to any information system that processes identity information.

A bibliography of documents describing various aspects of identity information management is provided."""@en ;
              sto:hasClassification sto:AsIdentification,
                                    sto:AsSafety  ,
                                    sto:AsSecurity ,
                                    sto:IIRASecurity ,
                                    sto:NISTProductModelDataExchange ,
                                    sto:RamiControlDevice ,
                                    sto:RamiFieldDevice ,
                                    sto:RamiInformationLayer ,
                                    sto:RamiProduct ,
                                    sto:RamiStation ;
              sto:hasPublisher sto:IEC ;
              sto:hasStatus "Withdrawn"@en ;
              sto:relatedTo sto:IEC_24760 ,
                            sto:IEC_62443 ,
                            sto:ISO_24760 ;
              sto:hasPublicationDate "2011-12-01"^^xsd:date ;
              sto:hasRelevantDomain sto:ITSecurity ;
              sto:hasOfficialResource <https://www.iso.org/standard/57914.html>;
              .


###  https://w3id.org/i40/sto#ISO_26262
sto:ISO_26262 rdf:type owl:NamedIndividual ,
                       sto:Standard ;
              dcterms:creator sto:irlan ;
              sto:hasClassification sto:IDSRAMCertification ,
                                    sto:Safety ;
              sto:hasDomain sto:ITSecurity ;
              sto:hasPublisher sto:ISO ;
              dcterms:title "Road vehicles – Functional safety"@en ;
              rdfs:comment "ISO 26262, titled \"Road vehicles – Functional safety\", is an international standard for functional safety of electrical and/or electronic systems in production automobiles defined by the International Organization for Standardization (ISO) in 2011."@en ;
              rdfs:label "ISO 26262"@en ;
              sto:hasDBpediaResource <http://dbpedia.org/resource/ISO_26262> ;
              sto:hasRelevantDomain sto:ITSecurity ;
              sto:hasOfficialResource <https://www.iso.org/obp/ui/#iso:std:iso:26262:-1:ed-1:v1:en> ;
              sto:hasWikipediaArticle <https://en.wikipedia.org/wiki/ISO_26262> .


###  https://w3id.org/i40/sto#ISO_27000
sto:ISO_27000 rdf:type owl:NamedIndividual ,
                       sto:Standard ;
              dcterms:creator sto:irlan ;
              sto:hasClassification sto:IDSRAMSecurity ;
              sto:hasPublisher sto:ISO ;
              sto:hasMotivation "Provides best practices for information security management. A critical issue for Industry 4.0 "@en ;
              sto:hasTag "Information Security Management Systems"@en ;
              rdfs:comment "The ISO/IEC 27000 family of standards helps organizations keep information assets secure. Using this family of standards will help your organization manage the security of assets such as financial information, intellectual property, employee details or information entrusted to you by third parties."@en ;
              rdfs:label "IEC 27000"@en ,
                         "ISO/IEC 27000"@en ;
              sto:hasDBpediaResource <http://dbpedia.org/resource/IEC_27000> ;
              sto:hasOfficialResource <http://www.27000.org/> ;
              sto:hasWikipediaArticle <https://en.wikipedia.org/wiki/ISO/IEC_27000> .


###  https://w3id.org/i40/sto#ISO_27001
sto:ISO_27001 rdf:type owl:NamedIndividual ,
                       sto:Standard ;
              dcterms:creator sto:sebastian ;
              sto:hasClassification sto:IDSRAMCertification ,
                                    sto:IDSRAMSecurity ,
                                    sto:IIRASecurity ;
              sto:hasDomain sto:ITSecurity ;
              sto:hasPublisher sto:IEC ,
                               sto:ISO ;
              rdfs:comment "ISO/IEC 27001 is an information security standard, part of the ISO/IEC 27000 family of standards."@en ;
              rdfs:label "ISO 27001"@en ,
                         "ISO/IEC 27001"@en ;
              sto:hasDBpediaResource <http://dbpedia.org/resource/ISO/IEC_27001> ;
              sto:hasRelevantDomain sto:ITSecurity ;
              sto:hasOfficialResource <https://www.iso.org/isoiec-27001-information-security.html> ;
              sto:hasWikipediaArticle <https://en.wikipedia.org/wiki/ISO/IEC_27001> .


###  https://w3id.org/i40/sto#ISO_27017
sto:ISO_27017 rdf:type owl:NamedIndividual ,
                       sto:Standard ;
              dcterms:creator sto:irlan ;
              sto:hasClassification sto:IIRASecurity ;
              sto:hasDomain sto:ITSecurity ;
              sto:hasPublisher sto:IEC ,
                               sto:ISO ;
              sto:hasPublicationDate "2015-12-01"^^xsd:date ;
              dc:title "Code of practice for information security controls based on ISO/IEC 27002 for cloud services"@en ;
              rdfs:comment "The ISO/IEC 270172 standard provides guidance on the information security elements of cloud computing. It assists with the implementation of cloud-specific information security controls, supplementing the guidance in ISO 27000 series standards."@en ;
              rdfs:label "ISO/IEC 27017"@en ;
              sto:hasDBpediaResource <http://dbpedia.org/resource/ISO/IEC_27000-series> ;
              sto:hasRelevantDomain sto:ITSecurity ;
              sto:hasOfficialResource <https://www.iso.org/standard/43757.html> ;
              sto:hasWikipediaArticle <https://en.wikipedia.org/wiki/ISO/IEC_27000-series> .


###  https://w3id.org/i40/sto#ISO_27018
sto:ISO_27018 rdf:type owl:NamedIndividual ,
                       sto:Standard ;
              dcterms:creator sto:irlan ,
                              sto:sebastian ;
              foaf:maker sto:IEC ,
                         sto:ISO ;
              sto:hasClassification sto:IIRAPrivacy ,
                                    sto:IIRASecurity ;
              sto:hasPublisher sto:IEC ,
                               sto:ISO ;
              sto:hasPublicationDate "2014-08-01"^^xsd:date ;
              dc:title "Information technology -- Security techniques -- Code of practice for protection of personally identifiable information (PII) in public clouds acting as PII processors"@en ;
              rdfs:comment "ISO/IEC 27018:2014 establishes commonly accepted control objectives, controls and guidelines for implementing measures to protect Personally Identifiable Information (PII) in accordance with the privacy principles in ISO/IEC 29100 for the public cloud computing environment."@en ;
              rdfs:label "IEC 27018"@en ;
              sto:hasDBpediaResource <http://dbpedia.org/resource/ISO/IEC_27000-series> ;
              sto:hasOfficialResource <https://webstore.iec.ch/publication/11302> ,
                                      <https://www.iso.org/standard/61498.html> ;
              sto:hasOpenResource <https://ciostrategycouncil.com/wp-content/uploads/2018/04/W_ISO-IEC-27018-2014.pdf> ;
              sto:hasWikipediaArticle <https://en.wikipedia.org/wiki/ISO/IEC_27000-series> .


###  https://w3id.org/i40/sto#ISO_27019
sto:ISO_27019 rdf:type owl:NamedIndividual ,
                       sto:Standard ;
              dcterms:creator sto:irlan ;
              sto:hasClassification sto:IDSRAMCertification ;
              sto:hasPublisher sto:ISO ;
              dcterms:title "Guidance for information security management of power supply control systems based on ISO/IEC 27002"@en ;
              rdfs:comment "The specification serves as a guidance for introducing ISO/IEC 27002 into the energy domain."@en ;
              rdfs:label "ISO 27019"@en ;
              sto:hasOfficialResource <https://www.beuth.de/de/technische-regel/din-iso-iec-tr-27019/223679647> .


###  https://w3id.org/i40/sto#ISO_27031
sto:ISO_27031 rdf:type owl:NamedIndividual ,
                       sto:Standard ;
              dcterms:creator sto:irlan ,
                              sto:sebastian ;
              foaf:maker sto:IEC ,
                         sto:ISO ;
              sto:hasClassification sto:IIRASecurity ;
              sto:hasPublisher sto:IEC ,
                               sto:ISO ;
              sto:domainName "Business Continuity"@en ;
              sto:hasPublicationDate "2011-03-01"^^xsd:date ;
              dc:title "Guidelines for information and communication technology readiness for business continuity"@en ;
              rdfs:comment "ISO/IEC 27031:2011 describes the concepts and principles of information and comunication technology (ICT) readiness for business continuity, and provides a framework of methods and processes to identify and specify all aspects (such as performance criteria, design, and implementation) for improving an organization's ICT readiness to ensure business continuity."@en ;
              rdfs:label "ISO 27031"@en ;
              sto:hasOfficialResource <https://webstore.iec.ch/publication/11304> ,
                                      <https://www.iso.org/standard/44374.html> .


###  https://w3id.org/i40/sto#ISO_27036
sto:ISO_27036 rdf:type owl:NamedIndividual ,
                       sto:Standard ;
              dcterms:creator sto:irlan ,
                              sto:sebastian ;
              sto:hasClassification sto:IIRASecurity ;
              sto:hasPublisher sto:IEC ,
                               sto:ISO ;
              sto:hasPublicationDate "2016-10-01"^^xsd:date ;
              dc:title "Information security for supplier relationships"@en ;
              rdfs:comment """ISO/IEC 27036-4:2016 provides cloud service customers and cloud service providers with guidance on

a) gaining visibility into the information security risks associated with the use of cloud services and managing those risks effectively, and

b) responding to risks specific to the acquisition or provision of cloud services that can have an information security impact on organizations using these services."""@en ;
              rdfs:label "ISO/IEC 27036"@en ;
              sto:hasDBpediaResource <http://dbpedia.org/resource/ISO/IEC_27000-series> ;
              sto:hasOfficialResource <https://webstore.iec.ch/publication/11314> ,
                                      <https://www.iso.org/standard/59689.html> ;
              sto:hasOpenResource <https://wodzinski.waw.pl/data/_uploaded/file/c059648_ISO_IEC_27036-1_2014.pdf> ;
              sto:hasWikipediaArticle <https://en.wikipedia.org/wiki/ISO/IEC_27000-series> .


###  https://w3id.org/i40/sto#ISO_29002
sto:ISO_29002 rdf:type owl:NamedIndividual ,
                       sto:Standard ;
              dcterms:creator sto:irlan ;
              sto:hasDomain sto:IndustrialProcessMeasurementControl ;
              sto:hasPublisher sto:ISO ;
              sto:relatedTo sto:DIN_SPEC_16592 ,
                            sto:IEC_61131 ,
                            sto:IEC_61360 ,
                            sto:IEC_61499 ,
                            sto:IEC_61804 ,
                            sto:IEC_61850 ,
                            sto:IEC_61987_X ,
                            sto:IEC_62424 ,
                            sto:IEC_62453 ,
                            sto:IEC_62541 ,
                            sto:IEC_62714 ,
                            sto:ISO_13584 ,
                            sto:ISO_14306 ,
                            sto:ISO_15746 ,
                            sto:ISO_15926 ,
                            sto:ISO_18629 ,
                            sto:ISO_18828-2 ,
                            sto:ISO_20922 ,
                            sto:ISO_22400 ,
                            sto:ISO_29002 ,
                            sto:ISO_ASTM_52915 ,
                            sto:ISO_PAS_17506 ,
                            sto:MathML ,
                            sto:SysML ,
                            sto:eClass ;
              sto:hasPublicationDate "2010-04-01"^^xsd:date ;
              rdfs:comment "ISO 29002 is an interoperability standard, which provides a repository to be used in various ISO XML formats. It is used in ontoML."@en ;
              rdfs:label "ISO 29002"@en ;
              sto:hasRelevantDomain sto:IndustrialProcessMeasurementControl ;
              sto:hasOfficialResource <https://www.iso.org/standard/53617.html> .


###  https://w3id.org/i40/sto#ISO_29100
sto:ISO_29100 rdf:type owl:NamedIndividual ,
                       foaf:Document ,
                       sto:Publication ,
                       sto:Standard ;
              foaf:maker sto:IEC ,
                         sto:ISO ;
              sto:hasClassification sto:IIRAPrivacy ,
                                    sto:IIRASecurity ;
              sto:hasPublisher sto:IEC ,
                               sto:ISO ;
              sto:hasPublicationDate "2011-12-01"^^xsd:date ;
              dcterms:title "Privacy framework"@en ;
              rdfs:comment """‘Privacy framework’1 provides a guideline that specifies a common privacy terminology, defines actors and roles in processing PII, describes privacy safeguarding considerations, and includes references to known privacy principles for Information technology.
source: IIC SF"""@en ;
              rdfs:label "ISO/IEC 29100"@en ;
              sto:hasOfficialResource <https://webstore.iec.ch/publication/11322> ,
                                      <https://www.iso.org/standard/45123.html> ;
              sto:hasOpenResource <https://pecb.com/pdf/whitepapers/30-Whitepapers-iso-29100-how-can-organizations-secure-its-privacy-network.pdf> .


###  https://w3id.org/i40/sto#ISO_29101
sto:ISO_29101 rdf:type owl:NamedIndividual ,
                       sto:Standard ;
              dcterms:creator sto:irlan ;
              sto:hasClassification sto:IIRAPrivacy ;
              sto:hasPublisher sto:IEC ,
                               sto:ISO ;
              sto:hasPublicationDate "2013-10-01"^^xsd:date ;
              dcterms:title "Privacy architecture framework"@en ,
                            "Privacy impact assessment–Guidelines"@en ;
              rdfs:comment "Code of practice for protection of personally identifiable information (PII) in public clouds acting as PII processors"@en ;
              rdfs:label "ISO/IEC 29101"@en ;
              sto:hasOfficialResource <https://www.iso.org/standard/45124.html> .





###  https://w3id.org/i40/sto#ISO_29134
sto:ISO_29134 rdf:type owl:NamedIndividual ,
                       foaf:Document ,
                       sto:Publication ,
                       sto:Standard ;
              dcterms:creator sto:ISO ,
                              sto:irlan ;
              foaf:maker sto:IEC ,
                         sto:ISO ;
              sto:hasClassification sto:IIRAPrivacy ;
              sto:hasDomain sto:ITSecurity ;
              sto:hasPublisher sto:IEC ,
                               sto:ISO ;
              sto:hasPublicationDate "2017-06-01"^^xsd:date ;
              dc:title "Privacy impact assessment–Guidelines"@en ;
              rdfs:comment "‘Privacy impact assessment–Guidelines’ proposes a methodology to conduct assessments on the impact of privacy."@en ;
              rdfs:label "ISO/IEC 29134"@en ;
              sto:hasRelevantDomain sto:ITSecurity ;
              sto:hasOfficialResource <https://www.iso.org/standard/62289.html> .


###  https://w3id.org/i40/sto#ISO_29161
sto:ISO_29161 rdf:type owl:NamedIndividual ,
                       foaf:Document ,
                       sto:Publication ,
                       sto:Standard ;
              dcterms:creator sto:irlan ;
              sto:hasPublisher sto:IEC ,
                               sto:ISO ;
              sto:hasPublicationDate "2016-08-01"^^xsd:date ;
              rdfs:comment "ISO/IEC 29161:2016 establishes a unique identification scheme for the Internet of Things (IoT), based on existing and evolving data structures."@en ;
              rdfs:label "ISO 29161"^^xsd:string ;
              sto:hasOfficialResource <https://www.iso.org/standard/45240.html> .


###  https://w3id.org/i40/sto#ISO_29190
sto:ISO_29190 rdf:type owl:NamedIndividual ,
                       foaf:Document ,
                       sto:Publication ,
                       sto:Standard ;
              dcterms:creator sto:irlan ;
              foaf:maker sto:IEC ,
                         sto:ISO ;
              sto:hasClassification sto:IIRAPrivacy ,
                                    sto:IIRASecurity ;
              sto_iot:hasTargetConcern sto:Privacy;
              sto:hasPublisher sto:IEC ,
                               sto:ISO ;
              sto:hasPublicationDate "2015-08-01"^^xsd:date ;
              dcterms:title "Privacy capability assessment model"@en ;
              rdfs:comment "‘Privacy capability assessment model’ provides high-level guidance to organizations about assessing their capability to manage privacy-related processes."@en ;
              rdfs:label "ISO/IEC 29190"@en ;
              sto:hasOfficialResource <https://webstore.iec.ch/publication/23118> ,
                                      <https://www.iso.org/standard/45269.html> ;
              sto:hasOpenResource <https://www.sis.se/api/document/preview/919384/> .


###  https://w3id.org/i40/sto#ISO_42010
sto:ISO_42010 rdf:type owl:NamedIndividual ,
                       sto:Standard ;
              dcterms:creator sto:irlan ;
              sto:hasPublisher sto:IEC ,
                               sto:ISO ;
              rdfs:label "ISO 42010"^^xsd:string ;
              sto:domainName "Reference Architecture Description"@en ;
              dcterms:title "Systems and software engineering — Architecture description"@en ;
              rdfs:comment """ISO/IEC/IEEE 42010:2011 defines requirements on the description of system, software and enterprise architectures. It aims to standardise the practice of architecture description by defining standard terms, presenting a conceptual foundation for expressing, communicating and reviewing architectures and specifying requirements that apply to architecture descriptions, architecture frameworks and architecture description languages.

Following its predecessor, IEEE Std 1471, the standard makes a strict distinction between Architectures and Architecture Descriptions.

The description of ISO/IEC/IEEE 42010 in this article is based upon the standard published in 2011."""@en ;
              rdfs:label "ISO/IEC 42010"@en ;
              sto:hasDBpediaResource <http://dbpedia.org/resource/ISO/IEC_42010> ;
              sto:hasOfficialResource <https://www.iso.org/standard/50508.html> ;
              sto:hasWikipediaArticle <https://en.wikipedia.org/wiki/ISO/IEC_42010> .


###  https://w3id.org/i40/sto#ISO_50001
sto:ISO_50001 rdf:type owl:NamedIndividual ,
                       foaf:Document ,
                       sto:Publication ,
                       sto:Standard ;
              dcterms:creator sto:irlan ;
              sto:hasClassification sto:ISA95CrossLevel ;
              sto:hasPublisher sto:ISO ;
              rdfs:comment "Energy management systems – Requirements with guidance for use is a specification created by the International Organization for Standardization (ISO) for an energy management system."@en ;
              rdfs:label "ISO 50001"@en ;
              sto:hasDBpediaResource <http://dbpedia.org/page/ISO_50001> ;
              sto:hasOfficialResource <https://www.iso.org/iso-50001-energy-management.html> ;
              sto_iot:hasTargetConcern sto:Energy_management .


###  https://w3id.org/i40/sto#ISO_5459
sto:ISO_5459 rdf:type owl:NamedIndividual ,
                      sto:Standard ;
             dcterms:creator sto:irlan ;
             sto:hasClassification sto:ModelingPractice ,
                                   sto:RamiAssetlayer ,
                                   sto:RamiProduct ;
             sto:hasPublisher sto:ISO ;
             sto:hasPublicationDate "2011-08-01"^^xsd:date ;
             rdfs:comment "Geometrical product specifications (GPS) -- Geometrical tolerancing -- Datums and datum systems--ISO 5459:2011 specifies terminology, rules and methodology for the indication and understanding of datums and datum systems in technical product documentation"@en ;
             rdfs:label "ISO 5459"@en ;
             sto:hasRelevantDomain sto:M2M ;
             sto:hasOfficialResource <https://www.iso.org/standard/40358.html> .


###  https://w3id.org/i40/sto#ISO_61508
sto:ISO_61508 rdf:type owl:NamedIndividual ,
                       sto:Standard ;
              owl:sameAs sto:IEC_61508 ;
             sto:hasPublisher sto:ISO ;
              rdfs:label "ISO 61508"@en ;
             rdfs:comment "Functional safety is a concept applicable across all industry sectors. It is fundamental to the enabling of complex technology used for safety-related systems. It provides the assurance that the safety-related systems will offer the necessary risk reduction required to achieve safety for the equipment. The oil and gas industry, nuclear plants and the machinery sector, to name but a few, all rely heavily on functional safety to achieve safety for the equipment giving rise to the hazards."@en ;
                       .


###  https://w3id.org/i40/sto#ISO_8062-4
sto:ISO_8062-4 rdf:type owl:NamedIndividual ,
                        sto:Standard ;
               dcterms:creator sto:irlan ;
               sto:hasClassification sto:ProductionSystemModelData ,
                                     sto:RamiAssetlayer ,
                                     sto:RamiProduct ;
               sto:hasPublisher sto:ISO ;
               sto:relatedTo sto:ISO_10303 ,
                             sto:ISO_8062-4 ;
               sto:hasPublicationDate "2017-07-01"^^xsd:date ;
               sto:hasTag "Automation systems and integration"@en ;
               rdfs:comment "Geometrical product specifications (GPS) -- Dimensional and geometrical tolerances for moulded parts -- General tolerances for castings using profile tolerancing in a general datum system"@en ;
               rdfs:label "ISO 8062-4"@en ;
               sto:hasOfficialResource <https://www.iso.org/standard/60774.html> .


###  https://w3id.org/i40/sto#ISO_9000
sto:ISO_9000 rdf:type owl:NamedIndividual ,
                      sto:Standard ;
             dcterms:creator sto:irlan ;
             sto:hasClassification sto:ISA95CrossLevel ;
             sto:hasPublisher sto:ISO ;
             rdfs:comment "The ISO 9000 family of quality management systems standards is designed to help organizations ensure that they meet the needs of customers and other stakeholders while meeting statutory and regulatory requirements related to a product or program."@en ;
             rdfs:label "ISO 9000"@en ;
             sto:hasDBpediaResource <http://dbpedia.org/page/ISO_9000> ;
             sto:hasOfficialResource <https://www.iso.org/iso-9001-quality-management.html> ;
             sto:hasWikipediaArticle <https://en.wikipedia.org/wiki/ISO_9000> ;
             sto_iot:hasTargetConcern sto:QualityOfService .


###  https://w3id.org/i40/sto#ISO_9594
sto:ISO_9594 rdf:type owl:NamedIndividual ,
                      sto:Standard ;
             dcterms:creator sto:irlan ;
             sto:hasClassification sto:DataSovereignty ,
                                   sto:IDSRAMCertification ,
                                   sto:IDSRAMSecurity ;
             sto:hasPublisher sto:ISO ;               
             rdfs:comment """ISO/IEC 9594-8:2017 addresses some of the security requirements in the areas of authentication and other security services through the provision of a set of frameworks upon which full services can be based. Specifically, this Recommendation | International Standard defines frameworks for:
- public-key certificates; and
- attribute certificates."""@en ;
             rdfs:label "ISO/IEC 9594"@en ,
                        "X.509"@en ;
             sto:hasOfficialResource <https://tools.ietf.org/html/rfc5280> .


###  https://w3id.org/i40/sto#ISO_9594-8
sto:ISO_9594-8 rdf:type owl:NamedIndividual ,
                        sto:Standard ;
               dcterms:creator sto:irlan ;
               sto:hasClassification sto:DataSovereignty ,
                                     sto:IDSRAMCertification ,
                                     sto:IDSRAMSecurity ;
               sto:hasPublisher sto:ISO ;
               dcterms:title "Information technology -- Open Systems Interconnection -- The Directory -- Part 8: Public-key and attribute certificate frameworks"@en ;
               rdfs:comment """ISO/IEC 9594-8:2017 addresses some of the security requirements in the areas of authentication and other security services through the provision of a set of frameworks upon which full services can be based. Specifically, this Recommendation | International Standard defines frameworks for:
- public-key certificates; and
- attribute certificates."""@en ;
               rdfs:label "ISO/IEC 9594-8"@en ;
               rdfs:seeAlso <https://tools.ietf.org/html/rfc5280> ;
               sto:hasOfficialResource <https://tools.ietf.org/html/rfc5280> ,
                                       <https://www.iso.org/standard/72557.html> .


###  https://w3id.org/i40/sto#ISO_ASTM_52915
sto:ISO_ASTM_52915 rdf:type owl:NamedIndividual ,
                            sto:Standard ;
                   dcterms:creator sto:irlan ;
                   sto:hasClassification sto:AsEngineering ,
                                         sto:AsIdentification ,
                                         sto:ProductionSystemEngineering ,
                                         sto:RamiAssetlayer ,
                                         sto:RamiProduct ;
                   sto:hasPublisher sto:ISO ;
                   sto:relatedTo sto:DIN_SPEC_16592 ,
                                 sto:IEC_61131 ,
                                 sto:IEC_61360 ,
                                 sto:IEC_61499 ,
                                 sto:IEC_61804 ,
                                 sto:IEC_61850 ,
                                 sto:IEC_61987_X ,
                                 sto:IEC_62424 ,
                                 sto:IEC_62453 ,
                                 sto:IEC_62541 ,
                                 sto:IEC_62714 ,
                                 sto:ISO_13584 ,
                                 sto:ISO_14306 ,
                                 sto:ISO_15746 ,
                                 sto:ISO_15926 ,
                                 sto:ISO_18629 ,
                                 sto:ISO_18828-2 ,
                                 sto:ISO_20922 ,
                                 sto:ISO_22400 ,
                                 sto:ISO_29002 ,
                                 sto:ISO_ASTM_52915 ,
                                 sto:ISO_PAS_17506 ,
                                 sto:MathML ,
                                 sto:SysML ,
                                 sto:eClass ;
                   sto:hasPublicationDate "2016-02-01"^^xsd:date ;
                   rdfs:comment "ISO ASTM 52915:2016 provides the specification for the Additive Manufacturing File Format (AMF), an interchange format to address the current and future needs of additive manufacturing technology."@en ;
                   rdfs:label "ISO ASTM 52915"@en ;
                   sto:hasRelevantDomain sto:IndustrialAutomation ;
                   sto:hasOfficialResource <https://www.iso.org/standard/60572.html> .


###  https://w3id.org/i40/sto#ISO_PAS_17506
sto:ISO_PAS_17506 rdf:type owl:NamedIndividual ,
                           sto:Standard ;
                  dcterms:creator sto:irlan ;
                  dul:isComponentOf sto:IEC_62714 ;
                  sto:hasDeveloper sto:ISO ;
                  sto:hasPublisher sto:ISO ;
                  sto:relatedTo sto:DIN_SPEC_16592 ,
                                sto:IEC_61131 ,
                                sto:IEC_61360 ,
                                sto:IEC_61499 ,
                                sto:IEC_61804 ,
                                sto:IEC_61850 ,
                                sto:IEC_61987_X ,
                                sto:IEC_62424 ,
                                sto:IEC_62453 ,
                                sto:IEC_62541 ,
                                sto:IEC_62714 ,
                                sto:ISO_13584 ,
                                sto:ISO_14306 ,
                                sto:ISO_15746 ,
                                sto:ISO_15926 ,
                                sto:ISO_18629 ,
                                sto:ISO_18828-2 ,
                                sto:ISO_20922 ,
                                sto:ISO_22400 ,
                                sto:ISO_29002 ,
                                sto:ISO_ASTM_52915 ,
                                sto:ISO_PAS_17506 ,
                                sto:MathML ,
                                sto:SysML ,
                                sto:eClass ;
                  sto:hasTag "COLLADA"@en ;
                  rdfs:comment "ISO-PAS 17506-2012 describes the COLLADA schema. COLLADA is a COLLAborative Design Activity that defines an XML-based schema to enable 3D authoring applications to freely exchange digital assets without loss of information, enabling multiple software packages to be combined into extremely powerful tool chains."@en ,
                               "SO/PAS 17506:2012 describes the COLLADA schema. COLLADA is a COLLAborative Design Activity that defines an XML-based schema to enable 3D authoring applications to freely exchange digital assets without loss of information, enabling multiple software packages to be combined into extremely powerful tool chains. The purpose of ISO/PAS 17506:2012 is to provide a specification for the COLLADA schema in sufficient detail to enable software developers to create tools to process COLLADA resources. In particular, it is relevant to those who import to or export from digital content creation (DCC) applications, 3D interactive applications and tool chains, prototyping tools, real-time visualization applications such as those used in the video game and movie industries, and CAD tools. ISO/PAS 17506:2012 covers the initial design and specifications of the COLLADA schema, as well as a minimal set of requirements for COLLADA exporters. "@en ;
                  rdfs:label "ISO PAS 17506"@en ;
                  sto:hasDBpediaResource <http://dbpedia.org/resource/COLLADA> ;
                  sto:hasOfficialResource <https://www.iso.org/standard/59902.html> ;
                  sto:hasWikipediaArticle <https://en.wikipedia.org/wiki/COLLADA> .


###  https://w3id.org/i40/sto#ISO_TS_14649-201
sto:ISO_TS_14649-201 rdf:type owl:NamedIndividual ,
                              sto:Standard ;
                     dcterms:creator sto:irlan ;
                     sto:hasClassification sto:AsEngineering ,
                                           sto:AsConfiguration,
                                           sto:AsSafety  ,
                                           sto:ProductionSystemModelData ,
                                           sto:RamiAssetlayer ,
                                           sto:RamiIntegrationLayer ,
                                           sto:RamiProduct ;
                     sto:hasPublisher sto:ISO ;
                     sto:hasPublicationDate "2011-12-01"^^xsd:date ;
                     rdfs:comment "SO/TS 14649-201:2011 specifies the technology-specific machine tool description data elements needed as process data for manufacturing and machine characteristics. The machine tool descriptions covered in this schema are, initially, milling machines, machining centres, turning machines and multi-tasking machines.ISO/TS 14649-201:2011 is not intended to replace existing machine tool description standards, but to cover the specific needs of manufacturing resource description for manufacturing needs in the technologies described in ISO 14649."@en ;
                     rdfs:label "ISO TS 14649-201"@en ;
                     sto:hasRelevantDomain sto:IndustrialAutomation ;
                     sto:hasOfficialResource <https://www.iso.org/standard/60042.html> .


###  https://w3id.org/i40/sto#ITSecurity
sto:ITSecurity rdf:type owl:NamedIndividual ,
                        sto:RelevantDomain;
               rdfs:label "IT Security"@en ;
               skos:altLabel "Information Security Management"@en .


###  https://w3id.org/i40/sto#Safety_Machinery
sto:Safety_Machinery 
a owl:NamedIndividual ;
  a sto:RelevantDomain;
  rdfs:label "Safety of Machinery"@en ;
  rdfs:comment "Safety of Machinery domain"@en ;
  sto:domainName "Safety of Machinery"@en ;
.


###  https://w3id.org/i40/sto#Identification
sto:Identification rdf:type owl:NamedIndividual ,
                            sto:StandardClassification ,
                            sto_iot:Concern ;
                   dul:associatedWith sto:AsIdentification ,
                                      sto:IEC_24760 ,
                                      sto:IEC_62443 ,
                                      sto:ISO_24760 ;
                   sto_iot:alignsWith sto:AsIdentification ,
                                      sto:IEC_24760 ,
                                      sto:IEC_62443 ,
                                      sto:ISO_24760 ;
                   sto_iot:supports sto:IdentityManagement ;
                   rdfs:comment "The concern how to identify a participant (client, endpoint etc.) in the internet."@en ;
                   rdfs:label "Identification"@en ;
                   rdfs:seeAlso "IoT-A Requirement UNI.030" ,
                                "IoT-A Requirement UNI.425" ,
                                "IoT-A Requirement UNI.428" ,
                                "IoT-A Requirement UNI.622" ;
                   skos:note "Publications referred: '<https://doi.org/10.1016/j.jksuci.2016.10.003>' 'Survey on domain specific IoT architectures' 'Page 299'" ;
                   sto:hasDBpediaResource <http://dbpedia.org/resource/Identification_(information)> .

###  https://w3id.org/i40/sto#Automatic_Id_Data_Capture_Techniques
sto:Automatic_Id_Data_Capture_Techniques 
a owl:NamedIndividual ;
  a sto:RelevantDomain;
  rdfs:label "Automatic Id Data Capture Techniques"@en ;
  rdfs:comment "Automatic Id Data Capture Techniques domain"@en ;
  sto:domainName "Automatic Id Data Capture Techniques"@en ;
.

###  https://w3id.org/i40/sto#IicfConnectivityLayer
sto:IicfConnectivityLayer rdf:type owl:NamedIndividual ;
                          dcterms:creator sto:sebastian .


###  https://w3id.org/i40/sto#IicfConnectivityLayerAnno
sto:IicfConnectivityLayerAnno rdf:type owl:NamedIndividual ,
                                       oa:Annotation ;
                              oa:hasBody sto:IicfConnectivityLayer ;
                              oa:hasTarget [ rdf:type oa:SpecificResource ;
                                             dcterms:format "pdf" ;
                                             oa:hasSelector [ rdf:type oa:RangeSelector ;
                                                              oa:hasEndSelector [ rdf:type oa:XPathSelector ;
                                                                                  rdf:value "Page 17"
                                                                                ] ;
                                                              oa:hasStartSelector [ rdf:type oa:XPathSelector ;
                                                                                    rdf:value "Page 14"
                                                                                  ]
                                                            ] ;
                                             oa:hasSource sto:The_Industrial_Internet_of_Things_Volume_G5_Connectivity_Framework
                                           ] ,
                                           [ rdf:type oa:SpecificResource ;
                                             dcterms:format "pdf" ;
                                             oa:hasSelector [ rdf:type oa:RangeSelector ;
                                                              oa:hasEndSelector [ rdf:type oa:XPathSelector ;
                                                                                  rdf:value "Page 17"
                                                                                ] ;
                                                              oa:hasStartSelector [ rdf:type oa:XPathSelector ;
                                                                                    rdf:value "Page 14"
                                                                                  ]
                                                            ] ;
                                             oa:hasSource sto:The_Industrial_Internet_of_Things_Volume_G5_Connectivity_Framework
                                           ] .


###  https://w3id.org/i40/sto#Electrotechnical
sto:Electrotechnical 
 a owl:NamedIndividual ;
  a sto:RelevantDomain;
  rdfs:label "Electrotechnical"@en ;
  rdfs:comment "Electrotechnical domain"@en;
  sto:domainName "Electrotechnical"@en;
 .
 

###  https://w3id.org/i40/sto#IndustrialAutomation
sto:IndustrialAutomation rdf:type owl:NamedIndividual ,
                                  sto:RelevantDomain;
                         sto:domainName "Industrial Automation"@en ;
                         rdfs:comment "Industrial automation deals primarily with the automation of manufacturing, quality control and material handling processes. General purpose controllers for industrial processes include Programmable logic controllers, stand-alone I/O modules, and computers. Industrial automation is to replace the decision making of humans and manual command-response activities with the use of mechanized equipment and logical programming commands. One trend is increased use of Machine vision to provide automatic inspection and robot guidance functions, another is a continuing increase in the use of robots. Industrial automation is simply done at the industrial level."@en ;
                         rdfs:label "Industrial Automation"@en ;
                         sto:hasDBpediaResource <http://dbpedia.org/resource/Category:IndustrialAutomation> ;
                         sto:hasWikipediaArticle <https://en.wikipedia.org/wiki/Automation> .


###  https://w3id.org/i40/sto#IndustrialDataSpace
sto:IndustrialDataSpace rdf:type owl:NamedIndividual ,
                                 sto:StandardizationFramework .


###  https://w3id.org/i40/sto#IndustrialInternetArchitecture
sto:IndustrialInternetArchitecture rdf:type owl:NamedIndividual ,
                                            sto:ArchitectureDescription ;
                                   sto:hasPublisher sto:AllianceOfIndustrialInternet ;
                                   rdfs:label "AII Industrial Internet Architecture"@en ;
                                   sto:hasOfficialResource <http://en.aii-alliance.org/uploadfile/2017/0307/Industrial.pdf> .


###  https://w3id.org/i40/sto#IndustrialInternetStandardSystem
sto:IndustrialInternetStandardSystem rdf:type owl:NamedIndividual ,
                                              sto:Publication ;
                                     sto:hasPublisher sto:AllianceOfIndustrialInternet ;
                                     rdfs:comment "Industrial Internet involves all industrial segment and all entities of industry field and ICT field, and it’s forming a complicated and total new ecological system. With industrial system networking and collaboration increasing, lots of new standardization requirements rise. While considering about the problems for Industrial Internet such as standard lacking, standard lagging, and standard duplicated, under the guidance of the Ministry of Industry and Information Technology (MIIT), Alliance of Industrial Internet (referred to as AII hereinafter) launched the study on the Industrial Internet standard system. Based on Industrial Internet Architecture (Version 1.0) and research on Industrial Internet standard requirements, AII drafted the Report on Industrial Internet Standard System (Version 1.0). In this Report, we propose the general idea, basic principles, standard system framework, key standardization directions and promotion suggestions. It aims to provide a systemized guidance of Industrial  Internet standardization for the industrial communities, to provide references and basis for development and amendment of Industrial Internet national standards, industrial standards and group standards, and to provide support for Industrial Internet development."@en ;
                                     rdfs:label "Industrial Internet Standard System"@en .


###  https://w3id.org/i40/sto#IndustrialProcessMeasurementControl
sto:IndustrialProcessMeasurementControl rdf:type owl:NamedIndividual ,
                                                 sto:RelevantDomain;
                                        sto:domainName "Industrial process measurement and control"@en ;
                                        rdfs:comment "Industrial process measurement and control"@en .


###  https://w3id.org/i40/sto#InformationDomain
sto:InformationDomain rdf:type owl:NamedIndividual .


###  https://w3id.org/i40/sto#InternationalClassificationForStandards
sto:InternationalClassificationForStandards sto:abbreviation "ICS"@en .


###  https://w3id.org/i40/sto#Italy
sto:Italy rdf:type owl:NamedIndividual ,
                   dbo:Country .


###  https://w3id.org/i40/sto#Japan
sto:Japan rdf:type owl:NamedIndividual ,
                   dbo:Country .


###  https://w3id.org/i40/sto#KATS
sto:KATS rdf:type owl:NamedIndividual ,
                  foaf:Organization ,
                  sto:StandardOrganization ;
         dul:associatedWith sto:IEC ,
                            sto:ISO ;
         dul:isMemberOf sto:IEC ,
                        sto:ISO ;
         sto:belongsTo dbr:South_Korea ;
         sto:hasHeadquaterIn dbr:Eumseong ;
         sto:abbreviation "KATS"@de ;
         sto:orgName "Korean Agency for Technology and Standards"@en ;
         rdfs:comment "Korean Agency for Technology and Standards is the government standards organization for South Korea. It is part of the Ministry of Knowledge Economy. It is authorized to regulate and manage the legal measures of South Korea by the current Measures Act."@en ;
         rdfs:label "Korean Agency for Technology and Standards"@en ;
         sto:hasDBpediaResource <http://dbpedia.org/page/Korean_Agency_for_Technology_and_Standards> ;
         sto:hasWikipediaArticle <https://en.wikipedia.org/wiki/Korean_Agency_for_Technology_and_Standards> .


###  https://w3id.org/i40/sto#KeyRock
sto:KeyRock rdf:type owl:NamedIndividual ,
                     foaf:Document ,
                     sto:Publication ,
                     sto:TechnicalSpecification ;
            dul:associatedWith sto:FiwareDataContextManagement ,
                               sto:FiwareSecurity ;
            sto_iot:hasTargetConcern sto:IdentityManagement .


###  https://w3id.org/i40/sto#LLAP
sto:LLAP rdf:type owl:NamedIndividual ,
                  foaf:Document ,
                  sto:Publication ,
                  sto:TechnicalSpecification ;
         dcterms:creator sto:sebastian ;
         rdfs:comment "LLAP (lightweight local automation protocol): is a simple short message that is sent between inteligent objects using normal text, it's not like TCP/IP, bluetooth, zigbee, 6lowpan, WiFi etc which achieve at a low level 'how' to move data around. This means LLAP can run over any communication medium. The three strengths of LLAP are, it'll run on anything now, anything in the future and it's easily understandable by humans. (source: https://www.postscapes.com/internet-of-things-protocols/)"@en ;
         rdfs:label "LLAP"@en ;
         sto:hasOfficialResource <http://openkontrol.org/llap/index.php/openkontrol/69-LLAP%20-%20Lightweight%20Local%20Automation%20Protocol> .


###  https://w3id.org/i40/sto#LWM2M
sto:LWM2M rdf:type owl:NamedIndividual ,
                   foaf:Document ,
                   sto:Publication ,
                   sto:TechnicalSpecification ;
          dcterms:creator sto:sebastian ;
          rdfs:comment "LWM2M (Lightweight M2M) is a system standard in the Open Mobile Alliance. It includes DTLS, CoAP, Block, Observe, SenML and Resource Directory and weaves them into a device-server interface along with an Object structure. (source: https://www.postscapes.com/internet-of-things-protocols/)"@en ;
          rdfs:label "LWM2M"@en ;
          sto:hasOfficialResource <http://yucianga.info/?p=786> .


###  https://w3id.org/i40/sto#LinkedData
sto:LinkedData rdf:type owl:NamedIndividual ,
                        foaf:Document ,
                        sto:Publication ,
                        sto:TechnicalSpecification .


###  https://w3id.org/i40/sto#LoRaWAN
sto:LoRaWAN rdf:type owl:NamedIndividual ,
                     foaf:Document ,
                     sto:Publication ,
                     sto:TechnicalSpecification ;
            dcterms:creator sto:sebastian ;
            rdfs:comment "LoRaWAN - Network protocol intended for wireless battery operated Things in regional, national or global network. (source: https://www.postscapes.com/internet-of-things-protocols/)"@en ;
            rdfs:label "LoRaWAN"@en ;
            sto:hasOfficialResource <https://www.lora-alliance.org/What-Is-LoRa/Technology> .


###  https://w3id.org/i40/sto#LoWPAN
sto:LoWPAN rdf:type owl:NamedIndividual ,
                    foaf:Document ,
                    sto:Publication ,
                    sto:TechnicalSpecification ;
           dcterms:creator sto:IETF ,
                           sto:sebastian ;
           foaf:maker sto:IETF ;
           sto:hasClassification sto:IIRAConnectivity ,
                                 sto:RAMICommunicationlayer ;
           sto:hasDeveloper sto:IETF ;
           sto:hasPublisher sto:IETF ;
           rdfs:comment "6LoWPAN is an acronym of IPv6 over Low power Wireless Personal Area Networks. It is an adaption layer for IPv6 over IEEE802.15.4 links. This protocol operates only in the 2.4 GHz frequency range with 250 kbps transfer rate. (source: https://www.postscapes.com/internet-of-things-protocols/)"@en ;
           rdfs:label "6LoWPAN"@en ;
           sto:hasDBpediaResource <http://dbpedia.org/resource/6LoWPAN> ;
           sto:hasWikipediaArticle <https://en.wikipedia.org/wiki/6LoWPAN> ;
           sto_iot:hasTargetConcern sto:Communication .


###  https://w3id.org/i40/sto#LowPowerWiFi
sto:LowPowerWiFi rdf:type owl:NamedIndividual ,
                          foaf:Document ,
                          sto:Publication ,
                          sto:TechnicalSpecification .


###  https://w3id.org/i40/sto#LsDL
sto:LsDL rdf:type owl:NamedIndividual ,
                  sto:TechnicalSpecification ;
         dcterms:creator sto:sebastian ;
         rdfs:comment "LsDL (Lemonbeat smart Device Language) - XML-based device language for service oriented devices. (source: https://www.postscapes.com/internet-of-things-protocols/)"@en ;
         rdfs:label "LsDL"@en ;
         sto:hasOfficialResource <http://www.lemonbeat.com/lsdl/> .


###  https://w3id.org/i40/sto#LteMtc
sto:LteMtc rdf:type owl:NamedIndividual ,
                    sto:TechnicalSpecification ;
           dcterms:creator sto:sebastian ;
           rdfs:comment "LTE-MTC (LTE-Machine Type Communication) - Standards-based family of technologies supports several technology categories, such as Cat-1 and CatM1, suitable for the IoT. (source: https://www.postscapes.com/internet-of-things-protocols/)"@en ;
           rdfs:label "LTE-MTC"@en ;
           sto:hasOfficialResource <http://www.gsma.com/connectedliving/long-term-evolution-machine-type-communication-lte-mtc-cat-m1/> .


###  https://w3id.org/i40/sto#M2M
sto:M2M rdf:type owl:NamedIndividual ,
                 sto:RelevantDomain;
        sto:domainName "Machine to machine Communication"@en ;
        rdfs:comment "Machine to machine refers to direct communication between devices using any communications channel, including wired and wireless"@en ;
        rdfs:label "Machine to Machine"@en ;
        sto:hasDBpediaResource <http://dbpedia.org/resource/Machine_to_machine> ;
        sto:hasWikipediaArticle <https://en.wikipedia.org/wiki/Machine_to_machine> .


###  https://w3id.org/i40/sto#MESA
sto:MESA rdf:type owl:NamedIndividual ,
                  foaf:Organization ,
                  sto:StandardOrganization ;
         sto:hasHeadquaterIn dbr:_Arizona ;
         sto:abbreviation "MESA"^^xsd:string ;
         sto:formationDate "1992-01-01"^^xsd:date ;
         sto:orgName "Manufacturing Enterprise Solutions Association"@en ;
         rdfs:comment "The Manufacturing Enterprise Solutions Association International is a global community of manufacturers, producers, industry leaders, and solution providers who are focused on driving business results from manufacturing information."@en ;
         sto:hasDBpediaResource <http://dbpedia.org/page/Manufacturing_Enterprise_Solutions_Association> ;
         sto:hasOfficialResource <http://www.mesa.org/en/index.asp> ;
         sto:hasWikipediaArticle <https://en.wikipedia.org/wiki/Manufacturing_Enterprise_Solutions_Association> .


###  https://w3id.org/i40/sto#MIIT
sto:MIIT rdf:type owl:NamedIndividual ,
                  sto:StandardOrganization ;
         sto:belongsTo dbr:China ;
         sto:hasHeadquaterIn dbr:Beijing ;
         sto:abbreviation "MIIT"^^xsd:string ;
         sto:formationDate "2008-03-01"^^xsd:date ;
         sto:orgName "Ministry of Industry and Information Technology"@en ;
         rdfs:comment "Ministry of Industry and Information Technology (MIIT) of the Chinese government, established in March 2008, is the state agency of the People's Republic of China responsible for regulation and development of the postal service, Internet, wireless, broadcasting, communications, production of electronic and information goods, software industry and the promotion of the national knowledge economy."@en ;
         sto:hasDBpediaResource <http://dbpedia.org/page/Ministry_of_Industry_and_Information_Technology> ;
         sto:hasOfficialResource <http://www.miit.gov.cn/> ;
         sto:hasWikipediaArticle <https://en.wikipedia.org/wiki/Ministry_of_Industry_and_Information_Technology> .


###  https://w3id.org/i40/sto#MOMLevel
sto:ISA95MOMLevel rdf:type owl:NamedIndividual ,
                      sto:ISA95Level ,
                      sto:StandardClassification ;
             rdfs:comment "Describes the MOM level according to the ISA95 level classification."@en ;
             rdfs:label "MOM Level"@en ;
             sto:isDescribedin sto:ISA95 ;
             skos:definition "Manufacturing Operation Management Level according to ISA 95"@en .


###  https://w3id.org/i40/sto#MTConnect
sto:MTConnect rdf:type owl:NamedIndividual ,
                       sto:Standard ;
              dcterms:creator sto:MTConnect_Institute ;
              foaf:maker sto:MTConnect_Institute ;
              sto:hasClassification sto:DeviceLevel ;
              sto:hasDeveloper sto:MTConnect_Institute ;
              sto:hasPublisher sto:MTConnect_Institute ;
              sto:hasTag "MTConnect"@en ;
              rdfs:comment "MTConnect is a protocol designed for the exchange of data between shop floor equipment and software applications used for monitoring and data analysis. MTConnect is referred to as a read-only standard, meaning that it only defines the extraction (reading) of data from control devices, not the writing of data to a control device. Freely available, open standards are used for all aspects of MTConnect. Data from shop floor devices is presented in XML format, and is retrieved from information providers, called Agents, using Hypertext Transfer Protocol (HTTP) as the underlying transport protocol. MTConnect provides a RESTful interface, which means the interface is stateless. No session must be established to retrieve data from an MTConnect Agent, and no logon or logoff sequence is required (unless overlying security protocols are added which do). Lightweight Directory Access Protocol (LDAP) is recommended for discovery services."@en ;
              rdfs:label "MTConnect"@en ;
              sto:relatedTo sto:IEC_62541;
              sto:hasDBpediaResource <http://dbpedia.org/resource/MTConnect> ;
              sto:hasOfficialResource <http://www.mtconnect.org/standard-documents> ;
              sto:hasWikipediaArticle <https://en.wikipedia.org/wiki/MTConnect> ;
              rdfs:seeAlso <https://www.mmsonline.com/columns/the-difference-between-mtconnect-and-opc-ua>;
              .


###  https://w3id.org/i40/sto#MTConnect_Institute
sto:MTConnect_Institute rdf:type owl:NamedIndividual ,
                                 sto:StandardOrganization ;
                        sto:abbreviation "MTC"^^xsd:string ;
                        sto:formationDate "2006-01-01"^^xsd:date ;
                        sto:orgName "MTConnect Institute"@en ;
                        rdfs:comment "MTConnect Institute is a collaborative effort to develop technical standards and specifications intended to foster greater interoperability between automation/control applications, field systems/devices, and business/office applications in the manufacturing industry (\"MTConnect Specifications\"), as well as schema, prototype software examples, and related documentation in order to facilitate the implementation of the MTConnect Specifications in compliant applications, drivers, and other services"@en ;
                        sto:hasOfficialResource <https://w3id.org/i40/www.mtconnect.org> .


###  https://w3id.org/i40/sto#Manufacturing
sto:IVRAManufacturing rdf:type owl:NamedIndividual ,
                           sto:StandardClassification ;
                  dul:associatedWith sto:IviActivityLayer ;
                  sto:alignsWith sto:IviActivityLayer;
                  sto:isDescribedin sto:IVRA .


###  https://w3id.org/i40/sto#NISTManufacturingModelData
sto:NISTManufacturingModelData rdf:type owl:NamedIndividual ,
                                    sto:ProductDevelopmentLifeCycle ,
                                    sto:StandardClassification ;
                           sto:isDescribedin sto:NISTInitiative ;
                           rdfs:comment "Manufacturing Model Data Standards define the data needed to manufacture a product from a design."@en ;
                           rdfs:label "Manufacturing Model Data"@en .


###  https://w3id.org/i40/sto#MathML
sto:MathML rdf:type owl:NamedIndividual ,
                    sto:Standard ;
           dcterms:creator sto:irlan ;
           sto:hasPublisher sto:W3C ;
           sto:relatedTo sto:DIN_SPEC_16592 ,
                         sto:IEC_61131 ,
                         sto:IEC_61360 ,
                         sto:IEC_61499 ,
                         sto:IEC_61804 ,
                         sto:IEC_61850 ,
                         sto:IEC_61987_X ,
                         sto:IEC_62424 ,
                         sto:IEC_62453 ,
                         sto:IEC_62541 ,
                         sto:IEC_62714 ,
                         sto:ISO_13584 ,
                         sto:ISO_14306 ,
                         sto:ISO_15746 ,
                         sto:ISO_15926 ,
                         sto:ISO_18629 ,
                         sto:ISO_18828-2 ,
                         sto:ISO_20922 ,
                         sto:ISO_22400 ,
                         sto:ISO_29002 ,
                         sto:ISO_ASTM_52915 ,
                         sto:ISO_PAS_17506 ,
                         sto:MathML ,
                         sto:SysML ,
                         sto:eClass ;
           rdfs:comment "MathML is a low-level specification for mathematical and scientific content on the Web and beyond"@en ;
           rdfs:label "MathML"@en ;
           sto:hasDBpediaResource <http://dbpedia.org/page/MathML> ;
           sto:hasOfficialResource <https://www.w3.org/Math/> ;
           sto:hasWikipediaArticle <https://en.wikipedia.org/wiki/MathML> .


###  https://w3id.org/i40/sto#Mihini
sto:Mihini rdf:type owl:NamedIndividual ,
                    sto:TechnicalSpecification ;
           dcterms:creator sto:sebastian ;
           rdfs:comment "Mihini/M3DA: The Mihini agent is a software component that acts as a mediator between an M2M server and the applications running on an embedded gateway. M3DA is a protocol optimized for the transport of binary M2M data. It is made available in the Mihini project both for means of Device Management, by easing the manipulation and synchronization of a device's data model, and for means of Asset Management, by allowing user applications to exchange typed data/commands back and forth with an M2M server, in a way that optimizes the use of bandwidth (source: https://www.postscapes.com/internet-of-things-protocols/)"@en ;
           rdfs:label "Mihini"@en ;
           sto:hasOfficialResource <https://wiki.eclipse.org/Mihini/M3DA_Specification> .


###  https://w3id.org/i40/sto#ModBus
sto:ModBus rdf:type owl:NamedIndividual ,
                    sto:TechnicalSpecification ;
           dcterms:creator sto:SE ;
           foaf:maker sto:SE ;
           sto:hasClassification sto:RamiIntegrationLayer ;
           sto:hasPublisher sto:SE ;
           sto:hasTag "Modbus"@en ;
           rdfs:comment "Modbus is a serial communications protocol to be used in Programmable logic controllers (PLCs)."@en ;
           rdfs:label "ModBus"@en ;
           sto:hasDBpediaResource <http://dbpedia.org/page/Modbus> ;
           sto:hasOfficialResource <http://www.modbus.org/> ;
           sto:hasWikipediaArticle <https://en.wikipedia.org/wiki/Modbus> .


###  https://w3id.org/i40/sto#ModelingPractice
sto:NISTModelingPractice rdf:type owl:NamedIndividual ,
                              sto:ProductDevelopmentLifeCycle ,
                              sto:StandardClassification ;
                     sto:isDescribedin sto:NISTInitiative ;
                     rdfs:comment "Modeling practice standards define digital product-definition data practices for both two-dimensional (2D) drawings and three-dimensional (3D) models."@en ;
                     rdfs:label "Modeling Practice"@en .


###  https://w3id.org/i40/sto#NERC
sto:NERC rdf:type owl:NamedIndividual ,
                  sto:StandardOrganization ;
         sto:abbreviation "NERC"@en ;
         sto:orgName "North American Electric Reliability Corporation"@en ;
         dcterms:description "The North American Electric Reliability Corporation (NERC) is a not-for-profit international regulatory authority whose mission is to assure the effective and efficient reduction of risks to the reliability and security of the grid. NERC develops and enforces Reliability Standards; annually assesses seasonal and long‐term reliability; monitors the bulk power system through system awareness; and educates, trains, and certifies industry personnel. NERC’s area of responsibility spans the continental United States, Canada, and the northern portion of Baja California, Mexico. NERC is the electric reliability organization (ERO) for North America, subject to oversight by the Federal Energy Regulatory Commission (FERC) and governmental authorities in Canada. NERC's jurisdiction includes users, owners, and operators of the bulk power system, which serves more than 334 million people."@en ;
         rdfs:seeAlso <https://www.nerc.com/Pages/default.aspx> ;
         sto:hasWikipediaArticle <https://wikipedia.org/wiki/North_American_Electric_Reliability_Corporation> .


###  https://w3id.org/i40/sto#NFC
sto:NFC rdf:type owl:NamedIndividual ,
                 sto:TechnicalSpecification ;
        dcterms:creator sto:sebastian ;
        sto:hasClassification sto:OpenFogNodeView ;
        rdfs:comment "Based on the standard ISO/IEC 18092:2004, using inductive coupled devices at a center frequency of13.56 MHz. The data rate is up to 424 kbps and the rangeis with a few meters short compared to the wireless sensornetworks. (source: https://www.postscapes.com/internet-of-things-protocols/)"@en ;
        rdfs:label "NFC"@en ;
        sto:hasOfficialResource <http://www.nfc-forum.org/home/> .


###  https://w3id.org/i40/sto#NIST
sto:NIST rdf:type owl:NamedIndividual ,
                  sto:StandardOrganization ;
         sto:belongsTo dbr:United_States ;
         sto:hasHeadquaterIn dbr:_Maryland ;
         sto:abbreviation "NIST"^^xsd:string ;
         sto:formationDate "1901-01-01"^^xsd:date ;
         sto:orgName "National Institute of Standards and Technology"@en ;
         rdfs:comment "The National Institute of Standards and Technology (NIST) is a measurement standards laboratory, and a non-regulatory agency of the United States Department of Commerce."@en ;
         sto:hasDBpediaResource <http://dbpedia.org/page/National_Institute_of_Standards_and_Technology> ;
         sto:hasOfficialResource <https://www.nist.gov/> ;
         sto:hasWikipediaArticle <https://en.wikipedia.org/wiki/National_Institute_of_Standards_and_Technology> .


###  https://w3id.org/i40/sto#NISTIR_8062
sto:NISTIR_8062 rdf:type owl:NamedIndividual ,
                         sto:Standard ;
                dcterms:creator sto:irlan ;
                sto:hasClassification sto:IIRAPrivacy ;
                sto:hasPublisher sto:NIST ;
                sto:hasPublicationDate "2017-04-01"^^xsd:date ;
                dc:title "Privacy Risk Management for Federal Information Systems"@en ;
                rdfs:comment "This document provides an introduction to the concepts of privacy engineering and risk management for federal information systems. These concepts establish the basis for a common vocabulary to facilitate better understanding and communication of privacy risk within federal information systems, and the effective implementation of privacy principles. This publication introduces two key components to support the application of privacy engineering and risk management: privacy engineering objectives and a privacy risk model."@en ;
                rdfs:label "NIST Internal Report (NISTIR) 8062"@en ,
                           "NISTIR 8062"@en ;
                sto:hasOfficialResource <https://doi.org/10.6028/NIST.IR.8062> .


###  https://w3id.org/i40/sto#NISTIR_8107
sto:NISTIR_8107 rdf:type owl:NamedIndividual ,
                         sto:Standard  ;
                sto:isDescribedin sto:NISTBusinessProcessExecution ,
                                  sto:SCM ;
                sto:hasPublisher sto:NIST ;
                rdfs:comment "Describes the NIST Initiative"@en ;
                rdfs:isDefinedBy <http://nvlpubs.nist.gov/nistpubs/ir/2016/NIST.IR.8107.pdf> ;
                rdfs:label "NISTIR_8107"@en ;
                skos:note "TODO - improve this classification"@en .


###  https://w3id.org/i40/sto#NISTInitiative
sto:NISTInitiative rdf:type owl:NamedIndividual ,
                            sto:StandardizationFramework ;
                   sto:hasPublisher sto:NIST ;
                   rdfs:comment "Describes the National Institute of Standards and Technology Initiative, i.e., NIST which provides a standard landascape"@en ;
                   rdfs:isDefinedBy <http://nvlpubs.nist.gov/nistpubs/ir/2016/NIST.IR.8107.pdf> ;
                   rdfs:label "NIST Initiative"@en .


###  https://w3id.org/i40/sto#NIST_500-291
sto:NIST_500-291 rdf:type owl:NamedIndividual ,
                          sto:RelevantDomain,
                          sto:Standard ;
                 dcterms:creator sto:irlan ;
                 sto:hasClassification sto:IIRASecurity ;
                 sto:hasPublisher sto:NIST ;
                 #sto:hasRelevantDomain
                 sto:hasPublicationDate "2011-08-10"^^xsd:date ;
                 dcterms:title "NIST Cloud Computing Standards Roadmap"@en ;
                 rdfs:comment "The NIST Cloud Computing Standards Roadmap Working Group has surveyed the existing standards landscape for security, portability, and interoperability standards/models/studies/use cases, etc., relevant to cloud computing. Using this available information, current standards, standards gaps, and standardization priorities are identified in this document. The NIST Definition of Cloud Computing identified cloud computing as a model for enabling ubiquitous, convenient, on-demand network access to a shared pool of configurable computing resources (e.g., networks, servers, storage, applications, and services) that can be rapidly provisioned and released with minimal management effort or service provider interaction."@en ;
                 rdfs:label "NIST 500-291"@en ;
                 sto:hasOfficialResource <https://www.nist.gov/publications/nist-sp-500-291-nist-cloud-computing-standards-roadmap> .


###  https://w3id.org/i40/sto#NIST_500-292
sto:NIST_500-292 rdf:type owl:NamedIndividual ,
                          sto:RelevantDomain,
                          sto:Standard ;
                 sto:hasClassification sto:IIRASecurity ,
                                       sto:Security ;
                 sto:hasDomain sto:CloudComputing ;
                 sto:hasPublisher sto:NIST ;
                 sto:hasRelevantDomain sto:CloudComputing;
                 sto:hasPublicationDate "2011-09-09"^^xsd:date ;
                 dc:title "NIST Cloud Computing Reference Architecture"@en ;
                 rdfs:comment "The adoption of cloud computing into the Federal Government and its implementation depend upon a variety of technical and non-technical factors. A fundamental reference point, based on the NIST definition of Cloud Computing, is needed to describe an overall framework that can be used government-wide. This document presents the NIST Cloud Computing Reference Architecture (RA) and Taxonomy (Tax) that will accurately communicate the components and offerings of cloud computing."@en ;
                 rdfs:label "NIST 500-292"@en ;
                 sto:hasOfficialResource <https://www.nist.gov/publications/nist-cloud-computing-reference-architecture> .


###  https://w3id.org/i40/sto#NIST_500-293
sto:NIST_500-293 rdf:type owl:NamedIndividual ,
                          sto:RelevantDomain,
                          sto:Standard ;
                 dcterms:creator sto:irlan ,
                                 sto:sebastian ;
                 sto:hasAvailableLanguage lang:eng ;
                 sto:hasClassification sto:IIRASecurity ;
                 sto:hasPublisher sto:NIST ;
                 sto:hasRelevantDomain sto:CloudComputing ;
                 sto:hasPublicationDate "2014-10-21"^^xsd:date ;
                 dcterms:title "US Government Cloud Computing Technology Roadmap"@en ;
                 rdfs:comment "The National Institute of Standards and Technology (NIST), consistent with its mission, has a technology leadership role in support of United States Government (USG) secure and effective adoption of the Cloud Computing model to reduce costs and improve services. This role is described in the 2011 Federal Cloud Computing Strategy as “... a central one in defining and advancing standards, and collaborating with USG Agency CIOs, private sector experts, and international bodies to identify and reach consensus on cloud computing technology & standardization priorities.” This NIST Cloud Computing program and initiative to develop a USG Cloud Computing Technology Roadmap is one of several complementary and parallel USG initiatives defined in the broader Federal Cloud Computing Strategy referenced above. The Federal Cloud Computing Strategy characterizes cloud computing as a “profound economic and technical shift (with) great potential to reduce the cost of federal Information Technology (IT) systems while … improving IT capabilities and stimulating innovation in IT solutions.” In the technology vision of Federal Cloud Computing Strategy success, USG agencies will be able to easily locate desired IT services in a mature and competitive marketplace, rapidly procure access to these services, and use them to deliver innovative mission solutions. Cloud services will be secure, interoperable, and reliable. Agencies will be able to switch between providers easily and with minimal cost, and receive equal or superior service."@en ;
                 rdfs:label "NIST 500-293"@en ;
                 sto:hasOfficialResource <https://www.nist.gov/publications/us-government-cloud-computing-technology-roadmap-volume-i-high-priority-requirements?pub_id=915112> .


###  https://w3id.org/i40/sto#NIST_800-144
sto:NIST_800-144 rdf:type owl:NamedIndividual ,
                          foaf:Document ,
                          sto:RelevantDomain,
                          sto:Publication ,
                          sto:Standard ;
                 dcterms:creator sto:NIST ;
                 foaf:maker sto:NIST ;
                 sto:hasClassification sto:IIRASecurity ;
                 sto:hasPublisher sto:NIST ;
                 sto:hasRelevantDomain sto:CloudComputing ;
                 sto:hasPublicationDate "2011-12-01"^^xsd:date ;
                 dcterms:title "Guidelines on Security and Privacy in Public Cloud Computing"@en ;
                 rdfs:comment "Cloud computing can and does mean different things to different people. The common characteristics most interpretations share are on-demand scalability of highly available and reliable pooled computing resources, secure access to metered services from nearly anywhere, and displacement of data and services from inside to outside the organization. While aspects of these characteristics have been realized to a certain extent, cloud computing remains a work in progress. This publication provides an overview of the security and privacy challenges pertinent to public cloud computing and points out considerations organizations should take when outsourcing data, applications, and infrastructure to a public cloud environment."@en ;
                 rdfs:label "NIST 800-144"@en ;
                 sto:hasOfficialResource <https://csrc.nist.gov/publications/detail/sp/800-144/final> .


###  https://w3id.org/i40/sto#NIST_800-146
sto:NIST_800-146 rdf:type owl:NamedIndividual ,
                          sto:Standard ;
                 dcterms:creator sto:irlan ;
                 sto:hasClassification sto:IIRASecurity ;
                 sto:hasDomain sto:CloudComputing ;
                 sto:hasPublisher sto:NIST ;
                 sto:hasPublicationDate "2012-05-01"^^xsd:date ;
                 dc:title "Cloud Computing Synopsis and Recommendations"@en ;
                 rdfs:comment "This document reprises the NIST-established definition of cloud computing, describes cloud computing benefits and open issues, presents an overview of major classes of cloud technology, and provides guidelines and recommendations on how organizations should consider the relative opportunities and risks of cloud computing."@en ;
                 rdfs:label "NIST 800-146"@en ;
                 sto:hasRelevantDomain sto:CloudComputing ;
                 sto:hasOfficialResource <https://csrc.nist.gov/publications/detail/sp/800-146/final> .


###  https://w3id.org/i40/sto#NanoIP
sto:NanoIP rdf:type owl:NamedIndividual ,
                    sto:TechnicalSpecification ;
           dcterms:creator sto:sebastian ;
           rdfs:comment "NanoIP, which stands for the nano Internet Protocol, is a concept that was created to bring Internet-like networking services to embedded and sensor devices, without the overhead of TCP/IP. NanoIP was designed with minimal overheads, wireless networking, and local addressing in mind. (source: https://www.postscapes.com/internet-of-things-protocols/)"@en ;
           rdfs:label "NanoIP"@en ;
           sto:hasOfficialResource <http://www.cwc.oulu.fi/nanoip/> .


###  https://w3id.org/i40/sto#NbIoT
sto:NbIoT rdf:type owl:NamedIndividual ,
                   sto:TechnicalSpecification ;
          dcterms:creator sto:sebastian ;
          rdfs:comment "NB-IoT (Narrow-Band IoT) A technology being standardized by the 3GPP standards body. (source: https://www.postscapes.com/internet-of-things-protocols/)"@en ;
          rdfs:label "NB-IoT"@en ;
          sto:hasWikipediaArticle <https://en.wikipedia.org/wiki/NarrowBand_IOT> .


###  https://w3id.org/i40/sto#NetworkLayer
sto:NetworkLayer rdf:type owl:NamedIndividual .


###  https://w3id.org/i40/sto#OAGIS
sto:OAGIS rdf:type owl:NamedIndividual ,
                   sto:Standard ;
          dcterms:creator sto:sebastian ;
          sto:hasPublisher sto:OAGi ;
          sto:hasTag "Open Applications Group Integration Specification"@en ;
          rdfs:comment "The Open Applications Group Integration Specification (OAGIS) is an effort to provide a canonical business language for information integration. It uses XML as the common alphabet for defining business messages, and for identifying business processes (scenarios) that allow businesses and business applications to communicate."@en ;
          rdfs:label "OAGIS"@en ;
          sto:hasOfficialResource <http://www.oagi.org/dnn2/DownloadsandResources/OAGIS100PublicDownload.aspx> ;
          sto:hasWikipediaArticle <https://de.wikipedia.org/wiki/Open_Application_Group_Integration_Specification> .


###  https://w3id.org/i40/sto#OAGi
sto:OAGi rdf:type owl:NamedIndividual ,
                  sto:StandardOrganization ;
         sto:hasHeadquaterIn dbr:_Georgia ;
         sto:abbreviation "OAGi"^^xsd:string ;
         sto:formationDate "1994-01-01"^^xsd:date ;
         sto:orgName "Open Applications Group"@en ;
         rdfs:comment "The Open Applications Group is a not-for-profit standards development organization. Founded in 1994, is focused on building enterprise ready process-based data exchange standards for both B2B and A2A integration."@en ;
         rdfs:label "OAGi"@en ;
         sto:hasOfficialResource <http://www.oagi.org/dnn2/Home.aspx> .


###  https://w3id.org/i40/sto#OASIS
sto:OASIS rdf:type owl:NamedIndividual ,
                   sto:StandardOrganization ;
          sto:hasHeadquaterIn dbr:Boston ;
          sto:abbreviation "OASIS"^^xsd:string ;
          sto:formationDate "1993-01-01"^^xsd:date ;
          sto:orgName "Organization for the Advancement of Structured Information Standards"@en ;
          rdfs:comment "The Organization for the Advancement of Structured Information Standards (OASIS) is a global nonprofit consortium that works on the development, convergence, and adoption of standards for security, Internet of Things, energy, content technologies, emergency management, and other areas."@en ;
          sto:hasDBpediaResource <http://dbpedia.org/page/OASIS_(organization)> ;
          sto:hasOfficialResource <https://www.oasis-open.org/> ;
          sto:hasWikipediaArticle <https://en.wikipedia.org/wiki/OASIS_(organization)> .


###  https://w3id.org/i40/sto#OCF_Core_Specification_VERSION_2_0_1
sto:OCF_Core_Specification_VERSION_2_0_1 rdf:type owl:NamedIndividual ,
                                                  oa:SpecificResource ;
                                         rdfs:label "OCF Core Specification VERSION 2.0.1 | February 11, 2019"@en ;
                                         sto:hasOpenResource <https://openconnectivity.org/specs/OCF_Core_Specification_v2.0.1.pdf> .


###  https://w3id.org/i40/sto#ODRL
sto:ODRL rdf:type owl:NamedIndividual ,
                  foaf:Document ,
                  sto:Publication ,
                  sto:Standard ;
         dcterms:creator sto:W3C ;
         foaf:maker sto:W3C ;
         sto:hasClassification sto:IDSRAMInformationLayer ,
                               sto:IDSRAMSecurity ;
         sto:hasPublisher sto:W3C ;
         rdfs:comment """The Open Digital Rights Language (ODRL) is a policy expression language that provides a flexible and interoperable information model, vocabulary, and encoding mechanisms for representing statements about the usage of content and services. The ODRL Information Model describes the underlying concepts, entities, and relationships that form the foundational basis for the semantics of the ODRL policies.
Policies are used to represent permitted and prohibited actions over a certain asset, as well as the obligations required to be meet by stakeholders. In addition, policies may be limited by constraints (e.g., temporal or spatial constraints) and duties (e.g. payments) may be imposed on permissions."""@en ;
         rdfs:label "ODRL"@en ,
                    "Open Digital Rights Language"@en ;
         sto:hasOfficialResource <https://www.w3.org/TR/odrl-model/> .


###  https://w3id.org/i40/sto#ODVA
sto:ODVA rdf:type owl:NamedIndividual ,
                  sto:StandardOrganization ;
         sto:hasHeadquaterIn dbr:_Michigan ;
         sto:abbreviation "ODVA"^^xsd:string ;
         sto:formationDate "1995-01-01"^^xsd:date ;
         sto:orgName "ODVA, Inc"@en ;
         rdfs:comment "Founded in 1995, ODVA is a global association whose members comprise the world’s leading automation companies. ODVA’s mission is to advance open, interoperable information and communication technologies in industrial automation. ODVA recognizes its media independent network protocol, the Common Industrial Protocol or “CIP” — and the network adaptations of CIP — EtherNet/IP, DeviceNet, CompoNet and ControlNet — as its core technology and the primary common interest of its membership. For future interoperability of production systems and the integration of the production systems with other systems, ODVA embraces the adoption of commercial-off-the-shelf (COTS) and standard, unmodified Internet and Ethernet technologies as a guiding principle wherever possible. This principle is exemplified by EtherNet/IP — the world’s number one industrial Ethernet network."@en ;
         sto:hasDBpediaResource <http://dbpedia.org/resource/ODVA_(company)> ;
         sto:hasOfficialResource <https://www.odva.org> ;
         sto:hasWikipediaArticle <https://en.wikipedia.org/wiki/ODVA_(company)> .


###  https://w3id.org/i40/sto#OMG
sto:OMG rdf:type owl:NamedIndividual ,
                 sto:StandardOrganization ;
        sto:hasHeadquaterIn dbr:_Massachusetts ;
        sto:abbreviation "OMG"^^xsd:string ;
        sto:formationDate "1989-01-01"^^xsd:date ;
        sto:orgName "Object Management Group"@en ;
        rdfs:comment "The Object Management Group (OMG) is an international, open membership, not-for-profit technology standards consortium. OMG Task Forces develop enterprise integration standards for a wide range of technologies and industries. OMG modeling standards enable visual design, execution and maintenance of software and other processes. Originally aimed at standardizing distributed object-oriented systems, the company now focuses on modeling (programs, systems and business processes) and model-based standards."@en ;
        sto:hasDBpediaResource <http://dbpedia.org/resource/Object_Management_Group> ;
        sto:hasOfficialResource <http://www.omg.org/> ;
        sto:hasWikipediaArticle <https://en.wikipedia.org/wiki/Object_Management_Group> .


###  https://w3id.org/i40/sto#OMG_DDS
sto:OMG_DDS rdf:type owl:NamedIndividual ,
                     foaf:Document ,
                     sto:Publication ,
                     sto:Standard ;
            dcterms:creator sto:OMG ;
            foaf:maker sto:OMG ;
            sto:hasClassification sto:IICFFrameworkLayer ,
                                  sto:IIRAConnectivity ;
            sto:hasPublisher sto:OMG ;
            sto:relatedTo sto:IEC_29182_P1 ,
                          sto:IEC_61158 ,
                          sto:IEC_61784 ,
                          sto:OMG_DDS ;
            sto:hasTag "Data Distribution Service for real-time systems"@en ;
            rdfs:comment "The Data Distribution Service for real-time systems (DDS) is an Object Management Group (OMG) machine-to-machine (sometimes called middleware) standard that aims to enable scalable, real-time, dependable, high-performance and interoperable data exchanges using a publish–subscribe pattern. DDS addresses the needs of applications like financial trading, air-traffic control, smart grid management, and other big data applications. The standard is used in applications such as smartphone operating systems, transportation systems and vehicles, software-defined radio, and by healthcare providers. DDS was promoted for use in the Internet of things."@en ;
            rdfs:label "OMG DDS"@en ;
            sto:hasDBpediaResource <http://dbpedia.org/page/Data_Distribution_Service> ;
            sto:hasOfficialResource <http://portals.omg.org/dds/> ;
            sto:hasWikipediaArticle <https://en.wikipedia.org/wiki/Data_Distribution_Service> .


###  https://w3id.org/i40/sto#OPC_Foundation
sto:OPC_Foundation rdf:type owl:NamedIndividual ,
                            sto:StandardOrganization ;
                   sto:hasHeadquaterIn dbr:_Arizona ;
                   sto:abbreviation "OPC"^^xsd:string ;
                   sto:formationDate "1994-01-01"^^xsd:date ;
                   sto:orgName "OPC Foundation"@en ;
                   rdfs:comment "Is an industry consortium that creates and maintains standards for open connectivity of industrial automation devices and systems, such as industrial control systems and process control generally"@en ;
                   rdfs:label "OPC Foundation"@en ;
                   sto:hasDBpediaResource <http://dbpedia.org/page/OPC_Foundation> ;
                   sto:hasOfficialResource <https://opcfoundation.org/> ;
                   sto:hasWikipediaArticle <https://en.wikipedia.org/wiki/OPC_Foundation> .


###  https://w3id.org/i40/sto#OTrP
sto:OTrP rdf:type owl:NamedIndividual ,
                  foaf:Document ,
                  sto:Publication ,
                  sto:TechnicalSpecification ;
         dcterms:creator sto:sebastian ;
         rdfs:comment "Open Trust Protocol (OTrP) - A protocol to install, update, and delete applications and to manage security configuration in a Trusted Execution Environment (TEE). (source: https://www.postscapes.com/internet-of-things-protocols/)"@en ;
         rdfs:label "Open Trust Protocol"@en ;
         sto:hasOfficialResource <https://www.ietf.org/id/draft-pei-opentrustprotocol-01.txt> .


###  https://w3id.org/i40/sto#OpenDaylight
sto:OpenDaylight rdf:type owl:NamedIndividual ,
                          foaf:Document ,
                          sto:Publication ,
                          sto:TechnicalSpecification ;
                 dcterms:creator sto:sebastian .





###  https://w3id.org/i40/sto#ISO_50001
sto:ISO_50001 rdf:type owl:NamedIndividual ,
                       sto:Standard ;
              sto_iot:hasTargetConcern sto:Energy_management ;
              rdfs:label "ISO 50001"@en .


###  https://w3id.org/i40/sto#ISO_9000
sto:ISO_9000 rdf:type owl:NamedIndividual ,
                      sto:Standard ;
             sto:hasClassification sto:ISA95CrossLevel ,
                                   sto:IDSRAMCertification ;
             sto_iot:hasTargetConcern sto:QualityOfService ;
             rdfs:label "ISO 9000"@en .

###  https://w3id.org/i40/sto#ISO_9594
sto:ISO_9594 rdf:type owl:NamedIndividual ,
                      sto:Standard ;
             sto:hasClassification sto:IDSRAMCertification ,
                                   sto:IDSRAMSecurity ;
             sto_iot:hasTargetConcern sto:DataSovereignty ;
             rdfs:label "ISO/IEC 9594"@en ,
                        "X.509"@en .


###  https://w3id.org/i40/sto#ISO_9594-8
sto:ISO_9594-8 rdf:type owl:NamedIndividual ,
                        sto:Standard ;
               sto:hasClassification sto:IDSRAMCertification ,
                                     sto:IDSRAMSecurity ;
               sto_iot:hasTargetConcern sto:DataSovereignty ;
               rdfs:label "ISO/IEC 9594-8"@en .


###  https://w3id.org/i40/sto#KeyRock
sto:KeyRock rdf:type owl:NamedIndividual ,
                     foaf:Document ,
                     sto:Publication ,
                     sto:TechnicalSpecification ;
            dul:associatedWith sto:FiwareDataContextManagement ,
                               sto:FiwareSecurity ;
            sto_iot:hasTargetConcern sto:IdentityManagement .


        
###  https://w3id.org/i40/sto#ID4me
sto:ID4me rdf:type owl:NamedIndividual ,
                   sto:TechnicalSpecification ;
          sto_iot:hasTargetConcern sto:Identification ,
                               sto:IdentityManagement .




###  https://w3id.org/i40/sto#IEC_62541
sto:IEC_62541 rdf:type owl:NamedIndividual ,
                       sto:Standard ;
              sto:hasClassification sto:IDSRAMSystemLayer ,
                                    sto:IICFFrameworkLayer ,
                                    sto:IIRAApplicationDomain ,
                                    sto:IIRAOperationsDomain ,
                                    sto:InformationDomain ,
                                    sto:RamiCommunicationlayer ,
                                    sto:RamiConnectedWorld ,
                                    sto:RamiControlDevice ,
                                    sto:RamiEnterprise ,
                                    sto:RamiFieldDevice ,
                                    sto:RamiStation ,
                                    sto:RamiWorkCenter ,
                                    sto:SCADALevel ;
              sto_iot:hasTargetConcern sto:AutonomousCommunication,
                                       sto:Communication ,
                                       sto:DataSovereignty;.


###  https://w3id.org/i40/sto#IPv6
sto:IPv6 rdf:type owl:NamedIndividual ,
                  foaf:Document ,
                  sto:Publication ,
                  sto:TechnicalSpecification ;
         dcterms:creator sto:sebastian ;
         sto_iot:hasTargetConcern sto:SyntacticInteroperability ;
         rdfs:comment "IPv6, is an Internet Layer protocol for packet-switched internetworking and provides end-to-end datagram transmission across multiple IP networks. (source: https://www.postscapes.com/internet-of-things-protocols/)"@en ;
         rdfs:label "IPv6"@en ;
         sto:hasWikipediaArticle <https://en.wikipedia.org/wiki/IPv6> .


###  https://w3id.org/i40/sto#DIN_SPEC_16593_P1
sto:DIN_SPEC_16593_P1 rdf:type owl:NamedIndividual ,
                               sto:Standard ;
                      sto_iot:hasTargetConcern sto:ServiceDescription .


###  https://w3id.org/i40/sto#DIN_SPEC_92222
sto:DIN_SPEC_92222 rdf:type owl:NamedIndividual ,
                            sto:Standard ;
                   sto_iot:hasTargetConcern sto:CloudComputing ,
                              sto:communication ,
                              sto:Interoperability .


###  https://w3id.org/i40/sto#IEC_61804_P3
sto:IEC_61804_P3 rdf:type owl:NamedIndividual ,
                          sto:Standard ;
                 sto_iot:hasTargetConcern sto:ThingDescription .


###  https://w3id.org/i40/sto#IEC_61804_P4
sto:IEC_61804_P4 rdf:type owl:NamedIndividual ,
                          sto:Standard ;
                 sto_iot:hasTargetConcern sto:ThingDescription .


###  https://w3id.org/i40/sto#IEC_61804_P5
sto:IEC_61804_P5 rdf:type owl:NamedIndividual ,
                          sto:Standard ;
                 sto_iot:hasTargetConcern sto:ThingDescription .


###  https://w3id.org/i40/sto#IEC_61804_P6
sto:IEC_61804_P6 rdf:type owl:NamedIndividual ,
                          sto:TechnicalReport ;
                sto_iot:hasTargetConcern sto:ThingDescription .


###  https://w3id.org/i40/sto#IEC_62264_P6
sto:IEC_62264_P6 rdf:type owl:NamedIndividual ,
                          sto:Standard ;
                 sto_iot:hasTargetConcern sto:Communication .


###  https://w3id.org/i40/sto#ISO_20140_P1
sto:ISO_20140_P1 rdf:type owl:NamedIndividual ,
                          sto:Standard ;
                 sto_iot:hasTargetConcern sto:EnergyEfficiency .


###  https://w3id.org/i40/sto#OpenLicenseDocument
sto:OpenLicenseDocument rdf:type owl:NamedIndividual ,
                                 dcterms:LicenseDocument ;
                        rdfs:comment "Open or Free License"@en ;
                        rdfs:label "Open or Free License"@en ;
                        rdfs:seeAlso <https://en.wikipedia.org/wiki/Free_license> .


###  https://w3id.org/i40/sto#OpenWSN
sto:OpenWSN rdf:type owl:NamedIndividual ,
                     foaf:Document ,
                     sto:Publication ,
                     sto:TechnicalSpecification ;
            dcterms:creator sto:sebastian ;
            rdfs:comment "OpenWSN Serves as a repository for open-source implementations of protocol stacks based on Internet of Things standards, using a variety of hardware and software platforms. (source: https://www.postscapes.com/internet-of-things-protocols/)"@en ;
            rdfs:label "OpenWSN"@en ;
            sto:hasOfficialResource <https://openwsn.atlassian.net/wiki/pages/viewpage.action?pageId=688187> .


###  https://w3id.org/i40/sto#PrivateLicenseDocument
sto:PrivateLicenseDocument rdf:type owl:NamedIndividual ,
                                    dcterms:LicenseDocument ;
                           rdfs:comment "Published under a Private License."@en ;
                           rdfs:label "Private License"@en ;
                           rdfs:seeAlso <https://en.wikipedia.org/wiki/Trade_secret> .


###  https://w3id.org/i40/sto#Priyanka
sto:Priyanka rdf:type owl:NamedIndividual ,
                      foaf:Person ;
             rdfs:label "Priyanka Nanjappa"@en ;
             foaf:familyName "Nanjappa"^^xsd:string ;
             foaf:name sto:Priyanka ,
                       "Priyanka"^^xsd:string .


###  https://w3id.org/i40/sto#ProductCatalogData
sto:ProductCatalogData rdf:type owl:NamedIndividual ,
                                sto:ProductDevelopmentLifeCycle  ;
                       sto:isDescribedin sto:NISTInitiative ;
                       rdfs:comment "Product catalog data standards support the description of particular instances of products or parts in a uniform, vendor-neutral way."@en ;
                       rdfs:label "Product Catalog Data"@en .


###  https://w3id.org/i40/sto#ProductLifeCycleManagement
sto:ProductLifeCycleManagement rdf:type owl:NamedIndividual ,
                                        sto:ProductDevelopmentLifeCycle  ;
                               sto:isDescribedin sto:NISTInitiative ;
                               rdfs:comment "Product lifecycle data management focuses on the needs of long-term retention and access to data consistently throughout the product lifecycle."@en ;
                               rdfs:label "Production Life Cycle Management"@en .


###  https://w3id.org/i40/sto#ProductModelDataExchange
sto:NISTProductModelDataExchange rdf:type owl:NamedIndividual ,
                                      sto:ProductDevelopmentLifeCycle  ;
                             sto:isDescribedin sto:NISTInitiative ;
                             rdfs:comment "These standards capture the representation of product and engineering information to enable data exchange between CAD software from different vendors."@en ;
                             rdfs:label "Product Model Data Exchange"@en .


###  https://w3id.org/i40/sto#ProductionLifeCycleDataManagement
sto:ProductionLifeCycleDataManagement rdf:type owl:NamedIndividual ,
                                               sto:ProductionSystemLifeCycle  ;
                                      sto:isDescribedin sto:NISTInitiative ;
                                      rdfs:comment "Production lifecycle data management standards define general models of data integration, sharing, exchange, and hand-over for lifecycle support of production facilities."@en ;
                                      rdfs:label "Production Life Cycle Data Management"@en .


###  https://w3id.org/i40/sto#ProductionSystemEngineering
sto:ProductionSystemEngineering rdf:type owl:NamedIndividual ,
                                         sto:ProductionSystemLifeCycle  ;
                                sto:isDescribedin sto:NISTInitiative ;
                                rdfs:comment "Standards can interconnect engineering tools from different disciplines, e.g., system engineering, mechanical plant engineering, electrical design, process engineering, process control engineering, Human Machine Interface (HMI) development, PLC programming, and robotic programming."@en ;
                                rdfs:label "Production System Engineering"@en .


###  https://w3id.org/i40/sto#ProductionSystemMaintenance
sto:ProductionSystemMaintenance rdf:type owl:NamedIndividual ,
                                         sto:ProductionSystemLifeCycle ;
                                sto:isDescribedin sto:NISTInitiative ;
                                rdfs:comment "Classifies standards define data processing, communication, and presentation standards for condition monitoring and diagnostics of machines, for maintaining the adequate performance of the system, and for searching ways to improve performance"@en ;
                                rdfs:label "Production System Maintenance"@en .


###  https://w3id.org/i40/sto#ProductionSystemModelData
sto:ProductionSystemModelData rdf:type owl:NamedIndividual ,
                                       sto:ProductionSystemLifeCycle ;
                              sto:isDescribedin sto:NISTInitiative ;
                              rdfs:comment "Provide information models for factory and production system design. They enhance information exchange among stakeholders, and enable virtual commissioning, which can improve manufacturing agility and reduce manufacturing cost."@en ;
                              rdfs:label "Production System Model Data"@en .


###  https://w3id.org/i40/sto#PublicLicenseDocument
sto:PublicLicenseDocument rdf:type owl:NamedIndividual ,
                                   dcterms:LicenseDocument ;
                          rdfs:comment "Published under a Public License."@en ;
                          rdfs:label "Public License"@en ;
                          rdfs:seeAlso <https://en.wikipedia.org/wiki/Public_copyright_license> .


###  https://w3id.org/i40/sto#QIF
sto:QIF rdf:type owl:NamedIndividual ,
                 foaf:Document ,
                 sto:Publication ,
                 sto:Standard ;
        dcterms:creator sto:DMSC ;
        foaf:maker sto:DMSC ;
        sto:hasPublisher sto:DMSC ;
        rdfs:comment " Quality Information Framework (QIF) standard defines an integrated set of information models which enable the effective exchange of metrology data throughout the entire manufacturing quality measurement process"@en ;
        rdfs:isDefinedBy <http://qifstandards.org/about-qif/> ;
        rdfs:label "Quality Information Framework"@en ;
        skos:note "Is implemented in XML"@en ;
        sto:hasOfficialResource <http://qifstandards.org/> .


###  https://w3id.org/i40/sto#QUIC
sto:QUIC rdf:type owl:NamedIndividual ,
                  foaf:Document ,
                  sto:Publication ,
                  sto:TechnicalSpecification ;
         dcterms:creator sto:sebastian ;
         rdfs:comment "QUIC (Quick UDP Internet Connections, pronounced quick) supports a set of multiplexed connections between two endpoints over User Datagram Protocol (UDP), and was designed to provide security protection equivalent to TLS/SSL, along with reduced connection and transport latency, and bandwidth estimation in each direction to avoid congestion. (source: https://www.postscapes.com/internet-of-things-protocols/)"@en ;
         rdfs:label "QUIC"@en ;
         sto:hasOfficialResource <https://en.wikipedia.org/wiki/QUIC> .




###  https://w3id.org/i40/sto#RuralElectrification
sto:RuralElectrification rdf:type owl:NamedIndividual ,
                                  sto:RelevantDomain ;
                         rdfs:comment "Bringing electricity into remote areas"@en ;
                         rdfs:label "Rural Electrification"@en ;
                         sto:hasWikipediaArticle <https://en.wikipedia.org/wiki/Rural_electrification> .


###  https://w3id.org/i40/sto#SCADALevel
sto:SCADALevel rdf:type owl:NamedIndividual ,
                        sto:ISA95Level ,
                        sto:StandardClassification ;
               sto:isDescribedin sto:ISA95 ;
               rdfs:comment "Describes the SCADA level according to the ISA95 level classification."@en ;
               rdfs:label "SCADA Level"@en ;
               skos:definition "Supervisory control and data acquisition according to ISA 95"@en .


###  https://w3id.org/i40/sto#SCIM
sto:SCIM rdf:type owl:NamedIndividual ,
                  foaf:Document ,
                  sto:Publication ,
                  sto:TechnicalSpecification ;
         dcterms:creator sto:irlan ,
                         sto:sebastian ;
         dul:associatedWith sto:FiwareSecurity ,
                            sto:RFC_7642 ,
                            sto:RFC_7643 ,
                            sto:RFC_7644 ;
         foaf:maker sto:IETF ;
         sto:hasPublisher sto:IETF ;
         dcterms:title "IETF System for Cross-domain Identity Management (SCIM) 2.0"@en ;
         rdfs:comment "The System for Cross-domain Identity Management (SCIM) specification is designed to make managing user identities in cloud-based applications and services easier. The specification suite seeks to build upon experience with existing schemas and deployments, placing specific emphasis on simplicity of development and integration, while applying existing authentication, authorization, and privacy models. Its intent is to reduce the cost and complexity of user management operations by providing a common user schema and extension model, as well as binding documents to provide patterns for exchanging this schema using standard protocols. In essence: make it fast, cheap, and easy to move users in to, out of, and around the cloud."@en ;
         rdfs:label "SCIM"@en ;
         sto:hasDBpediaResource <http://dbpedia.org/resource/System_for_Cross-domain_Identity_Management> ;
         sto:hasWikipediaArticle <https://en.wikipedia.org/wiki/System_for_Cross-domain_Identity_Management> ;
         sto_iot:hasTargetConcern sto:CrossDomainIdentityManagement .


###  https://w3id.org/i40/sto#SCM
sto:SCM rdf:type owl:NamedIndividual ,
                 sto:BusinessCycleSCM ;
        sto:isDescribedin sto:NISTInitiative ;
        rdfs:comment "Describes Plan-Source-Make-Deliver-Return cycle for managing the manufacturing supply chain."@en ;
        rdfs:label "Supply Chain Management"@en .


###  https://w3id.org/i40/sto#SCOR
sto:SCOR rdf:type owl:NamedIndividual ,
                  foaf:Document ,
                  sto:Publication ,
                  sto:TechnicalSpecification ;
         dcterms:creator sto:APICS ;
         foaf:maker sto:APICS ;
         sto:hasClassification sto:SCM ;
         sto:hasDeveloper sto:APICS ;
         sto:hasTag "SCOR"@en ;
         rdfs:comment "APICS Supply Chain Operations Reference."@en ;
         rdfs:label "SCOR"@en ;
         sto:hasDBpediaResource <http://dbpedia.org/page/Supply-chain_operations_reference> ;
         sto:hasOfficialResource <http://www.apics.org/apics-for-business/products-and-services/apics-scc-frameworks/scor> ;
         sto:hasWikipediaArticle <https://en.wikipedia.org/wiki/Supply-chain_operations_reference> .


###  https://w3id.org/i40/sto#SE
sto:SE rdf:type owl:NamedIndividual ;
       sto:hasHeadquaterIn dbr:Paris ;
       sto:abbreviation "SE"^^xsd:string ;
       sto:formationDate "1936-01-01"^^xsd:date ;
       sto:orgName "Schneider Electric"@en ;
       rdfs:comment "Schneider Electric SE is a European multinational corporation that specializes in energy management and automation solutions, spanning hardware, software, and services."@en ;
       sto:hasDBpediaResource <http://dbpedia.org/page/Schneider_Electric> ;
       sto:hasOfficialResource <http://www.schneider-electric.com/ww/en/> ;
       sto:hasWikipediaArticle <https://en.wikipedia.org/wiki/Schneider_Electric> .


###  https://w3id.org/i40/sto#SENML
sto:SENML rdf:type owl:NamedIndividual ,
                   sto:TechnicalSpecification ;
          dcterms:creator sto:irlan ,
                          sto:sebastian ;
          rdfs:comment "SENML (Media Types for Sensor Markup Language) - A simple sensor, such as a temperature sensor, could use this media type in protocols such as HTTP or CoAP to transport the measurements of the sensor or to be configured.  (source: https://www.postscapes.com/internet-of-things-protocols/)"@en ;
          rdfs:label "SENML"@en ;
          sto:hasOfficialResource <https://tools.ietf.org/html/draft-jennings-senml-08> .


###  https://w3id.org/i40/sto#SMCP
sto:SMCP rdf:type owl:NamedIndividual ,
                  sto:TechnicalSpecification ;
         dcterms:creator sto:irlan ,
                         sto:sebastian ;
         rdfs:comment "SMCP — A C-based CoAP stack which is suitable for embedded environments. Features include: Support draft-ietf-core-coap-13, Fully asynchronous I/O, Supports both BSD sockets and UIP. (source: https://www.postscapes.com/internet-of-things-protocols/)"@en ;
         rdfs:label "SMCP"@en ;
         sto:hasOfficialResource <https://github.com/darconeous/smcp/tree/smcp-0.6> .


###  https://w3id.org/i40/sto#SOAP
sto:SOAP rdf:type owl:NamedIndividual ,
                  sto:TechnicalSpecification ;
         dcterms:creator sto:irlan ,
                         sto:sebastian ;
         rdfs:comment "SOAP (Simple Object Access Protocol) (source: https://www.postscapes.com/internet-of-things-protocols/)"@en ;
         rdfs:label "SOAP"@en ;
         sto:hasDBpediaResource <http://dbpedia.org/page/Service-oriented_architecture> ;
         sto:hasWikipediaArticle <https://en.wikipedia.org/wiki/SOAP> .


###  https://w3id.org/i40/sto#SSI
sto:SSI rdf:type owl:NamedIndividual ,
                 sto:TechnicalSpecification ;
        dcterms:creator sto:irlan ,
                        sto:sebastian ;
        rdfs:comment "SSI (Simple Sensor Interface) is a simple communications protocol designed for data transfer between computers or user terminals and smart sensors. (source: https://www.postscapes.com/internet-of-things-protocols/)"@en ;
        rdfs:label "SSI"@en ;
        sto:hasDBpediaResource <http://dbpedia.org/page/Simple_Sensor_Interface_protocol> ;
        sto:hasWikipediaArticle <https://en.wikipedia.org/wiki/Simple_Sensor_Interface_protocol> .


###  https://w3id.org/i40/sto#SSN
sto:SSN rdf:type owl:NamedIndividual ,
                 sto:TechnicalSpecification ;
        dcterms:creator sto:irlan ,
                        sto:sebastian ;
        rdfs:comment "Semantic Sensor Net Ontology - W3C This ontology describes sensors and observations, and related concepts. It does not describe domain concepts, time, locations, etc. these are intended to be included from other ontologies via OWL imports. (source: https://www.postscapes.com/internet-of-things-protocols/)"@en ;
        rdfs:label "SSN"@en ;
        sto:hasOfficialResource <https://www.w3.org/2005/Incubator/ssn/wiki/Semantic_Sensor_Net_Ontology> .


###  https://w3id.org/i40/sto#STOMP
sto:STOMP rdf:type owl:NamedIndividual ,
                   foaf:Document ,
                   sto:Publication ,
                   sto:TechnicalSpecification ;
          dcterms:creator sto:sebastian ;
          rdfs:comment "STOMP - The Simple Text Oriented Messaging Protocol (source: https://www.postscapes.com/internet-of-things-protocols/)"@en ;
          rdfs:label "STOMP"@en ;
          sto:hasOfficialResource <https://stomp.github.io/implementations.html> .


###  https://w3id.org/i40/sto#SensorML
sto:SensorML rdf:type owl:NamedIndividual ,
                      foaf:Document ,
                      sto:Publication ,
                      sto:TechnicalSpecification ;
             dcterms:creator sto:sebastian ;
             rdfs:comment "SensorML provides standard models and an XML encoding for describing sensors and measurement processes. (source: https://www.postscapes.com/internet-of-things-protocols/)"@en ;
             rdfs:label "SensorML"@en ;
             sto:hasWikipediaArticle <https://en.wikipedia.org/wiki/SensorML> .


###  https://w3id.org/i40/sto#SmartCity
sto:SmartCity rdf:type owl:NamedIndividual ,
                       sto:RelevantDomain ;
              rdfs:comment " A city that collects data which is used for better Maintenance of it's resources"@en ;
              rdfs:label " Smart City"@en ;
              sto:hasWikipediaArticle <https://en.wikipedia.org/wiki/Smart_city> .


###  https://w3id.org/i40/sto#SmartEnergy
sto:SmartEnergy rdf:type owl:NamedIndividual ,
                         sto:RelevantDomain ;
                rdfs:comment " Intelligent technologies in value chain of energy industry"@en ;
                rdfs:label " Smart Energy"@en ;
                sto:hasWikipediaArticle <https://translate.google.com/translate?hl=en&sl=de&u=https://de.wikipedia.org/wiki/Smart_Energy&prev=search> .


###  https://w3id.org/i40/sto#SmartGrid
sto:SmartGrid rdf:type owl:NamedIndividual ,
                       sto:RelevantDomain ;
              rdfs:comment "An electrical grid having smart appliances"@en ;
              rdfs:label "Smart Grid"@en ;
              sto:hasWikipediaArticle <https://en.wikipedia.org/wiki/Smart_grid> .


###  https://w3id.org/i40/sto#StandardClassification
sto:StandardClassification rdf:type owl:NamedIndividual ;
                           dcterms:creator sto:irlan .


###  https://w3id.org/i40/sto#StandardizationFramework
sto:StandardizationFramework rdf:type owl:NamedIndividual ;
                             dcterms:creator sto:irlan .


###  https://w3id.org/i40/sto#SysML
sto:SysML rdf:type owl:NamedIndividual ,
                   foaf:Document ,
                   sto:Publication ,
                   sto:Standard ;
          dcterms:creator sto:OMG ;
          foaf:maker sto:OMG ;
          sto:hasDeveloper sto:OMG ;
          sto:hasPublisher sto:OMG ;
          sto:relatedTo sto:DIN_SPEC_16592 ,
                        sto:IEC_61131 ,
                        sto:IEC_61360 ,
                        sto:IEC_61499 ,
                        sto:IEC_61804 ,
                        sto:IEC_61850 ,
                        sto:IEC_61987_X ,
                        sto:IEC_62424 ,
                        sto:IEC_62453 ,
                        sto:IEC_62541 ,
                        sto:IEC_62714 ,
                        sto:ISO_13584 ,
                        sto:ISO_14306 ,
                        sto:ISO_15746 ,
                        sto:ISO_15926 ,
                        sto:ISO_18629 ,
                        sto:ISO_18828-2 ,
                        sto:ISO_20922 ,
                        sto:ISO_22400 ,
                        sto:ISO_29002 ,
                        sto:ISO_ASTM_52915 ,
                        sto:ISO_PAS_17506 ,
                        sto:MathML ,
                        sto:SysML ,
                        sto:eClass ;
          rdfs:comment "The OMG Systems Modeling Language (OMG SysML) is a general-purpose graphical modeling language for specifying, analyzing, designing, and verifying complex systems that may include hardware, software, information, personnel, procedures, and facilities. In particular, the language provides graphical representations with a semantic foundation for modeling system requirements, behavior, structure, and parametrics, which is used to integrate with other engineering analysis models. It represents a subset of UML 2 with extensions needed to satisfy the requirements of the UML for Systems Engineering RFP as indicated in Figure 1. SysML leverages the OMG XML Metadata Interchange (XMI®) to exchange modeling data between tools, and is also intended to be compatible with the evolving ISO 10303-233 systems engineering data interchange standard."@en ;
          rdfs:label "Systems Modeling Language"@en ;
          sto:hasDBpediaResource <http://dbpedia.org/resource/Systems_Modeling_Language> ;
          sto:hasOfficialResource <http://sysml.org/> ,
                                  <http://www.omgsysml.org/what-is-sysml.htm> ;
          sto:hasWikipediaArticle <https://en.wikipedia.org/wiki/Systems_Modeling_Language> .


###  https://w3id.org/i40/sto#TC_1
sto:TC_1 rdf:type owl:NamedIndividual ,
                  sto:TechnicalCommittee ;
         dcterms:title "Terminology"@en ;
         rdfs:comment "To sanction the terms and definitions used in the different electrotechnical fields and to determine the equivalence of the terms used in the different languages. As a consequence, to prepare an International Electrotechnical Vocabulary aiming at the standardization and coordination of the terms relating to electrical sciences and techniques for use in the technical language and literature, in teaching, in technical specifications and in commercial exchanges, and at giving their equivalents in the different languages."@en ;
         rdfs:label "TC 1"@en .


###  https://w3id.org/i40/sto#TC_103
sto:TC_103 rdf:type owl:NamedIndividual ,
                    sto:TechnicalCommittee ;
           dcterms:title "Transmitting equipment for radiocommunication"@en ;
           rdfs:comment """Standardization of transmitting equipment for radiocommunications purposes and electronic devices employing similar
techniques. The standardization work deals with methods of measurement, safety requirements and transmitter control and Interconnection"""@en ;
           rdfs:label "TC 103"@en .


###  https://w3id.org/i40/sto#TC_25
sto:TC_25 rdf:type owl:NamedIndividual ,
                   sto:TechnicalCommittee ;
          dcterms:title "Quantities and units"@en ;
          rdfs:comment "To prepare international standards on quantities and units to be used in electrical technology. Such standards may relate to their definitions, names, letter symbols and use; to the relations in which they appear; and to the signs and symbols used with them."@en ;
          rdfs:label "TC 25"@en .


###  https://w3id.org/i40/sto#TC_3
sto:TC_3 rdf:type owl:NamedIndividual ,
                  sto:TechnicalCommittee ;
         dcterms:title "Information structures and elements, identification and marking principles, documentation and graphical symbols"@en ;
         rdfs:comment "To prepare standards for the electrotechnical and related fields regarding:1) methods and rules associated with the human interpretation of information. This refers to:- presentation of information in technical documentation,- graphical symbols for use in technical documentation,- graphical symbols for the human interaction with equipment,2) methods and rules associated with the handling of information in computer sensible form. This refers to:- information models for the purpose of technical documentation and the exchange of technical information, and the identification of further needs for such models,- definition of data element types and data sets for use in information models and technical documentation, and for exchange of technical information.It includes definition and co-ordination of the information required during the whole life cycle of a device, system, or plant.3) General and safety application concerning the man-machine interface, marking and identification in electrical installations and equipment, marking systems and general rules for:- the meanings of colours and alternative means, when used for marking and identification,- the arrangement of indicating devices and actuators,- coding principles for indicating and actuating devices,- terminal designation of electrical and electronic components, apparatus and equipment,- the termination designation of certain designated conductors,- marking of electrical and electronic equipment with ratings related to supply and to its properties,- marking of bare and insulated conductors.These standards are principally intended for use by technical committees in the preparation of standards in accordance with the principles laid down in IEC Guide 104: Guide to the drafting of Safety Standards, and the role of committees with Safety Pilot Functions and Safety Group Functions, and in ISO/IEC Guide 51: Guidelines for the inclusion of safety aspects in standards."@en ;
         rdfs:label "TC 3"@en .


###  https://w3id.org/i40/sto#TC_40
sto:TC_40 rdf:type owl:NamedIndividual ,
                   sto:TechnicalCommittee ;
          dcterms:title "Capacitors and resistors for electronic equipment"@en ;
          rdfs:comment "To prepare international standards for:a) Capacitors, resistors, thermistors and varistors intended for use in electronic equipment.b) Capacitors, resistors and inductors and complete electromagnetic interference (EMI) suppression filter units for EMI suppression (see note).c) Passive integrated circuits or networks containing resistors, capacitors, inductors or their combinations. For the dimensional standardization of the final package, requirements laid down by TC 47 shall be adopted whenever possible.d) Packaging of electronic components for automatic handling, which is an activity undertaken on behalf of all relevant component technical committees.e) Electric double layer capacitors for use in electric and electronic equipment.Note: In this work, use has to be made as far as possible of any relevant work of TC 51 on inductors, the CISPR on the measurement of EMI suppression characteristics and TC 77 on electromagnetic compatibility (EMC). Liaison has also to be maintained with TC 61, TC 66, TC 108 and other appropriate IEC Technical Committees on the safety aspects of EMI suppression components and filter units."@en ;
          rdfs:label "TC 40"@en .


###  https://w3id.org/i40/sto#TC_44
sto:TC_44 rdf:type owl:NamedIndividual ,
                   sto:TechnicalCommittee ;
          dcterms:title "Safety of machinery - Electrotechnical aspects"@en ;
          rdfs:comment "Standardization in the field of the application of electro-technical equipment and systems to machinery (including a group of machines working together in a coordinated manner, excluding higher-level systems aspects) not portable by hand while working, but which may include mobile equipment. The equipment covered commences at the point of connection of the electrical supply to the machinery.Standardization of interfaces (excluding local area networks and fieldbus) between control equipment and the electro-technical equipment of machinery.Standardization of electrotechnical equipment and systems relating to the safeguarding of persons from hazards of the machinery, its associated equipment and the environment.To coordinate with ISO all matters concerning the safety of machinery.."@en ;
          rdfs:label "TC 44"@en .


###  https://w3id.org/i40/sto#TC_56
sto:TC_56 rdf:type owl:NamedIndividual ,
                   sto:TechnicalCommittee ;
          dcterms:title "Dependability"@en ;
          rdfs:comment """To prepare international standards in the field of dependability, in all appropriate technological areas, including those not normally dealt with by IEC Technical Committees. Dependability covers the availability performance and its influencing factors: reliability performance, maintainability performance and maintenance support performance (including management of obsolescence). The standards provide systematic methods and tools for the dependability assessment and management of equipment, services and systems throughout their life cycles.
The standards cover generic aspects on reliability and maintainability programme management, testing and analytical techniques, software and system dependability, life cycle costing, technical risk analysis and project risk management. This includes standards related to product issues from component reliability to guidance for engineering dependability of systems, standards related to process issues from technological risk analysis to integrated logistics support and standards related to management issues from dependability program management to managing for obsolescence.
The application of these standards may raise safety related issues, though the standards themselves do not cover safety. They may be applied to business risk analysis but these risk areas are not dealt with by TC 56."""@en ;
          rdfs:label "TC 56"@en .


###  https://w3id.org/i40/sto#TC_57
sto:TC_57 rdf:type owl:NamedIndividual ,
                   sto:TechnicalCommittee ;
          dcterms:title "Power systems management and associated information exchange"@en ;
          rdfs:comment """To prepare international standards for power systems control equipment and systems including EMS (Energy Management Systems), SCADA (Supervisory Control And Data Acquisition), distribution automation, teleprotection, and associated information exchange for real-time and non-real-time information, used in the planning, operation and maintenance of power systems. Power systems management comprises control within control centres, substations and individual pieces of primary equipment including telecontrol and interfaces to equipment, systems and databases, which may be outside the scope of TC 57. The special conditions in a high voltage environment have to be taken into consideration.
Note 1: Standards prepared by other technical committees of the IEC and organizations such as ITU and ISO shall be used where applicable.
Note 2: Although the work of TC 57 is chiefly concerned with standards for electric power systems, these standards may also be useful for application by the relevant bodies to other geographical widespread processes.
Note 3: Whereas standards related to measuring and protection relays and to the control and monitoring equipment used with these systems are treated by TC 95, TC 57 deals with the interface to the control systems and the transmission aspects for teleprotection systems. Whereas standards related to equipment for electrical measurement and load control are treated by TC 13, TC 57 deals with the interface of equipment for interconnection lines and industrial consumers and producers requiring energy management type interfaces to the control system."""@en ;
          rdfs:label "TC 57"@en .


###  https://w3id.org/i40/sto#TC_65
sto:TC_65 rdf:type owl:NamedIndividual ,
                   sto:TechnicalCommittee ;
          dcterms:title "Industrial-process measurement, control and automation"@en ;
          rdfs:comment "To prepare international standards for systems and elements used for industrial-process measurement and control concerning continuous and batch processes."@en ;
          rdfs:label "TC 65"@en .


###  https://w3id.org/i40/sto#TC_66
sto:TC_66 rdf:type owl:NamedIndividual ,
                   sto:TechnicalCommittee ;
          dcterms:title "Safety of measuring"@en ,
                        "control and laboratory equipment"@en ;
          rdfs:comment """To prepare safety standards for test and measurement equipment, industrial-process control equipment, and laboratory equipment wherever they are used.
Such equipment includes:
a) equipment and systems to measure, test, generate, and analyse, simple and complex electromagnetic quantities and equipment that by electromagnetic means measure physical quantities.
Note: Aspects of this equipment other than safety are covered by other technical committees.
b) equipment and systems for industrial-process measurement and control.
Note: Aspects of this equipment other than safety are covered by TC 65 except that SC 65A has a Horizontal Safety Function relating to the functional safety of electrical/electronic/ programmable electronic systems and SC 65B is responsible for the functional safety of programmable controllers.
c) laboratory equipment for analysis, handling and preparation of materials.
Note: This equipment includes measuring instruments, systems and their accessories, for preparation, treatment and analysis of materials in the fields of research, medicine, industry and education, and for environmental monitoring.
TC 66 has a Group Safety Function in accordance with IEC Guide 104 for the equipment in categories a) to c) above."""@en ;
          rdfs:label "TC 66"@en .


###  https://w3id.org/i40/sto#TC_77
sto:TC_77 rdf:type owl:NamedIndividual ,
                   sto:TechnicalCommittee ;
          dcterms:title "Electromagnetic compatibility"@en ;
          rdfs:comment """Standardization - to prepare standards and technical reports - in the field of electromagnetic compatibility (EMC), with
particular emphasis on general application and use by product committees. (Horizontal function). The scope covers the following aspects of EMC:
- Immunity and related items, over the whole frequency range: basic and generic standards, - emission in the low frequency range (f <= 9 kHz, e.g. harmonics and voltage fluctuations): basic, generic and product (family) standards,
- emission in the high frequency range (f > 9 kHz): disturbances not covered by CISPR 10 (1992), in co-ordination with CISPR (e.g. mains signalling).
Product immunity standards are not included. However, at the request of product committees, TC 77 may also prepare such standards under the co-ordination of ACEC.
Horizontal Safety Function: Electromagnetic compatibility in so far as safety aspects are involved."""@en ;
          rdfs:label "TC 77"@en .


###  https://w3id.org/i40/sto#TC_79
sto:TC_79 rdf:type owl:NamedIndividual ,
                   sto:TechnicalCommittee ;
          dcterms:title "Alarm and electronic security systems"@en ;
          rdfs:comment "To prepare international standards for the protection of buildings, persons, areas and properties against fraudulent actions having the purpose to enter in a place or to take or to use something without permission and other threat related to persons.The scope includes, but is not limited to equipment and systems, either used by ordinary persons or by trained people in the following residential and non residential applications:- Access control systems- Alarm transmission systems- Video surveillance systems- Combined and/or integrated systems even including fire alarm systems*- Fire detection and fire alarm systems*- Intruder and hold-up alarm systems- Remote receiving and/or surveillance centres- Social alarm systems.These systems can be used for providing a local or remote alarm; they can be used for calling private guards, social assistance, fire brigade or police force. They can be used for recording and transmission of dated or undated information, sounds, pictures of places and people for surveillance purposes. The standards cover:- terminology;- technical characteristics regarding performance criteria, reliable operation, installation, maintenance;- testing for detection, monitoring, recording, triggering an alarm and transmission to a remote centre including procedures and protocols for communication.Electrical safety, environmental conditions and behaviour of alarm systems regarding electromagnetic compatibility are also considered with reference to the appropriate standards (e.g. Guide ISO/IEC 51).* ISO/TC21/SC3 is in charge of the production of standards for \"Fire detection and alarm systems\"."@en ;
          rdfs:label "TC 79"@en .


###  https://w3id.org/i40/sto#TC_8
sto:TC_8 rdf:type owl:NamedIndividual ,
                  sto:TechnicalCommittee ;
         dcterms:title "Systems aspects of electrical energy supply"@en ;
         rdfs:comment "To prepare and coordinate, in co-operation with other TC/SCs, the development of international standards and other deliverables with emphasis on overall system aspects of electricity supply systems and acceptable balance between cost and quality for the users of electrical energy. Electricity supply system encompasses transmission and distribution networks, generators and loads with their network interfaces."@en ;
         rdfs:label "TC 8"@en .


###  https://w3id.org/i40/sto#TC_88
sto:TC_88 rdf:type owl:NamedIndividual ,
                   sto:TechnicalCommittee ;
          dcterms:title "Wind energy generation systems"@en ;
          rdfs:comment """TC 88 standardization in the field of wind energy generation systems including wind turbines, wind power plants onshore and offshore and interaction with the electrical system(s) to which energy is supplied.

These standards address site suitability and resource assessment, design
requirements, engineering integrity, modeling requirements, measurement techniques, test procedures, operation and maintenance. Their purpose is to provide a basis for design, quality assurance and technical aspects for certification. The standards address site-specific conditions, all systems and subsystems of wind turbines and wind power plants, such as mechanical, and electrical systems, support structures, control and protection as well as communication systems for monitoring, centralized and distributed control and evaluation, implementation of grid connection requirements for wind power plants, and environmental aspects of wind power development. The TC 88 standards will be developed based on and in agreement with appropriate IEC/ISO standards."""@en ;
          rdfs:label "TC 88"@en .


###  https://w3id.org/i40/sto#TC_91
sto:TC_91 rdf:type owl:NamedIndividual ,
                   sto:TechnicalCommittee ;
          dcterms:title "Electronics assembly technology"@en ;
          rdfs:comment "To prepare international standards on design, manufacturing and testing of electronic assemblies including the requirements and tests for materials and components used to manufacture circuit boards and electronic assemblies, as well as the formats of electronic data and libraries for describing these products and processes."@en ;
          rdfs:label "TC 91"@en .


###  https://w3id.org/i40/sto#TC_94
sto:TC_94 rdf:type owl:NamedIndividual ,
                   sto:TechnicalCommittee ;
          dcterms:title "All-or-nothing electrical relays"@en ;
          rdfs:comment """To prepare international standards applicable to all-or-nothing electrical relays used in the various fields of Electrical Engineering covered by the IEC, normally produced in very large
numbers as components of electromechanical or electronic
equipment and eventually submitted to Quality Assurance requirements based on sampling techniques."""@en ;
          rdfs:label "TC 94"@en .


###  https://w3id.org/i40/sto#TC_95
sto:TC_95 rdf:type owl:NamedIndividual ,
                   sto:TechnicalCommittee ;
          dcterms:title "Measuring relays and protection equipment"@en ;
          rdfs:comment "Standardisation of measuring relays and protection equipment used in various fields of electrical engineering covered by IEC, taking into a ccount combinations of devices to form schemes for power system protection including the control, monitoring and process interface equipment used with those systems.Excluded are the following:All devices covered by standards prepared by other IEC Technical Committees, for example instrument transformers (TC 38)."@en ;
          rdfs:label "TC 95"@en .


###  https://w3id.org/i40/sto#TS-0009
sto:TS-0009 rdf:type owl:NamedIndividual ,
                     foaf:Document ,
                     sto:Publication ,
                     sto:Standard ;
            dcterms:creator sto:oneM2M ;
            foaf:maker sto:oneM2M ;
            sto:hasClassification sto:IICFFrameworkLayer ;
            sto:hasPublisher sto:oneM2M ;
            dcterms:title "HTTP Protocol Binding"@en ;
            rdfs:comment """The present document will cover the protocol specific part of communication protocol used by oneM2M compliant systems as RESTful HTTP binding.
The scope of the present document is (not limited to as shown below):
• Binding oneM2M Protocol primitive types to HTTP method.
• Binding oneM2M response status codes (successful/unsuccessful) to HTTP response codes.
• Binding oneM2M RESTful resources to HTTP resources.
The present document is depending on Core Protocol specification (oneM2M TS-0004) for data types."""@en ;
            rdfs:label "TS-0009"@en ;
            sto:hasOfficialResource <https://w3id.org/i40/www.onem2m.org/images/files/deliverables/Release2A/TS-0009-HTTP_Protocol_Binding-v_2_13_1.pdf> .


###  https://w3id.org/i40/sto#TSMP
sto:TSMP rdf:type owl:NamedIndividual ,
                  foaf:Document ,
                  sto:Publication ,
                  sto:TechnicalSpecification ;
         dcterms:creator sto:sebastian ;
         rdfs:comment "Time Synchronized Mesh Protocol (TSMP): A communications protocol for self-organizing networks of wireless devices called motes. TSMP devices stay synchronized to each other and communicate in timeslots, similar to other TDM (time-division multiplexing) systems. (source: https://www.postscapes.com/internet-of-things-protocols/)"@en ;
         rdfs:label "TSMP"@en ;
         sto:hasWikipediaArticle <https://en.wikipedia.org/wiki/TSMP> .

###  https://w3id.org/i40/sto#TechnicalCommittee
sto:TechnicalCommittee rdf:type owl:Class ;
                       sto:abbreviation "TC"^^xsd:string ;
                       rdfs:label "Technical Committee"@en ;
                       skos:note "A property explaining that TC and SC are managed by SMB (Standardization Management Board) needs to be added"@en ;
                       rdfs:comment "Specifies the representitive code name of the Technical Committee that covers a Standard for e.g, TC 1, SC 3C. Many thousand experts carry out standardization work in the IEC in TCs (technical committees) and SCs (subcommittees), in hundreds of working groups, project and maintenance teams. They represent the national electrotechnical needs of IEC Member countries and of many Affiliates at the global level in the IEC. These technical experts are sent by industry, governments, test and research laboratories, academia and even consumer groups to work on the global, neutral and independent platform of the IEC. That's where they develop globally relevant, voluntary, consensus based IEC International Standards."@en ;
                       rdfs:seeAlso <http://www.iec.ch/dyn/www/f?p=103:62:9979528650478:::62:FSP_ORG_ID,FSP_LANG_ID:,25> ;
                       rdfs:isDefinedBy sto:IEC .


###  https://w3id.org/i40/sto#TechnicalReport
sto:TechnicalReport rdf:type owl:Class ;
                    cc:attributionURL <http://www.iec.ch> ;
                    rdfs:isDefinedBy sto:IEC ;
                    rdfs:comment "Technical Reports contain collected data of a kind different from that normally published as an International Standard, for example data obtained from a survey carried out among national committees, data of work in other international organizations or data on \"the state of the art\" in relation to standards of national committees on a particular subject.Technical Reports are entirely informative in nature and shall not contain matter implying that they are normative"@en ;
                    rdfs:label "Technical Report"@en ;
                    rdfs:seeAlso <http://www.iec.ch/standardsdev/publications/tr.htm> ;
                    rdfs:comment "Specifies that a given Publication is a Technical Report"@en .


###  https://w3id.org/i40/sto#TechnicalSpecification
sto:TechnicalSpecification rdf:type owl:Class ;
                           rdfs:comment "Specifies that a given Publication is a Technical Specification"@en ;
                           rdfs:label "Technical Specification"@en ;
                           rdfs:comment "Technical Specifications are often published when the subject under question is still under development or when insufficient consensus for approval of an International Standard is available.Technical Specifications approach International Standards in terms of detail and completeness, but have not yet passed through all approval stages either because consensus has not been reached or because standardization is seen to be premature."@en ;
                           cc:attributionURL <http://www.iec.ch> ;
                           rdfs:isDefinedBy sto:IEC ;
                           rdfs:seeAlso <http://www.iec.ch/standardsdev/publications/ts.htm> .

###  https://w3id.org/i40/sto#Technology
sto:Technology rdf:type owl:NamedIndividual ;
               dcterms:creator sto:sebastian .


###  https://w3id.org/i40/sto#Telehash
sto:Telehash rdf:type owl:NamedIndividual ,
                      sto:TechnicalSpecification ;
             dcterms:creator sto:sebastian ;
             rdfs:comment "Telehash - JSON+UDP+DHT=Freedom: A secure wire protocol powering a decentralized overlay network for apps and devices. (source: https://www.postscapes.com/internet-of-things-protocols/)"@en ;
             rdfs:label "Telehash"@en ;
             sto:hasOfficialResource <http://telehash.org/> .


###  https://w3id.org/i40/sto#Thread
sto:Thread rdf:type owl:NamedIndividual ,
                    sto:Standard ;
           dcterms:creator sto:sebastian ;
           rdfs:comment "Thread - Built on open standards and IPv6 technology with 6LoWPAN as its foundation. (source: https://www.postscapes.com/internet-of-things-protocols/)"@en ;
           rdfs:label "Thread"@en ;
           sto:hasPublisher <https://www.threadgroup.org/thread-group> ;
           sto:hasOfficialResource <http://www.threadgroup.org/About.aspx> .


###  https://w3id.org/i40/sto#UDP
sto:UDP rdf:type owl:NamedIndividual ,
                 foaf:Document ,
                 sto:Publication ,
                 sto:Standard ;
        dcterms:creator sto:sebastian ;
         sto:hasPublisher sto:IETF ;
        rdfs:comment "UDP (User Datagram Protocol) - A simple OSI transport layer protocol for client/server network applications based on Internet Protocol (IP). UDP is the main alternative to TCP and one of the oldest network protocols in existence, introduced in 1980. UDP is often used in applications specially tuned for real-time performance."@en ;
        rdfs:label "UDP"@en ;
        sto:hasOfficialResource <https://tools.ietf.org/html/rfc768> .


###  https://w3id.org/i40/sto#UN-CEFACT
sto:UN-CEFACT rdf:type owl:NamedIndividual ,
                       foaf:Organization ,
                       sto:StandardOrganization ;
              sto:hasHeadquaterIn dbr:Geneva ;
              sto:abbreviation "UN/CEFACT"^^xsd:string ;
              sto:orgName "United Nations Centre for Trade Facilitation and Electronic Business"@en ;
              rdfs:comment "UN/CEFACT is the United Nations Centre for Trade Facilitation and Electronic Business. It was established as an intergovernmental body of the United Nations Economic Commission for Europe (UNECE) in 1996 and evolved from UNECE’s long tradition of work in trade facilitation."@en ;
              sto:hasDBpediaResource <http://dbpedia.org/page/UN/CEFACT> ;
              sto:hasOfficialResource <https://www.unece.org/cefact/> ;
              sto:hasWikipediaArticle <https://en.wikipedia.org/wiki/UN/CEFACT> .


###  https://w3id.org/i40/sto#UPnP
sto:UPnP rdf:type owl:NamedIndividual ,
                  foaf:Document ,
                  sto:Publication ,
                  sto:TechnicalSpecification ;
         dcterms:creator sto:sebastian ;
         rdfs:comment "UPnP (Universal Plug and Play) - Now managed by the Open Connectivity Foundation is a set of networking protocols that permits networked devices to seamlessly discover each other's presence on the network and establish functional network services for data sharing, communications, and entertainment.(source: https://www.postscapes.com/internet-of-things-protocols/)"@en ;
         rdfs:label "UPnP"@en ;
         sto:hasOfficialResource <https://openconnectivity.org/upnp> .


###  https://w3id.org/i40/sto#URI
sto:URI rdf:type owl:NamedIndividual ,
                 foaf:Document ,
                 sto:Publication ,
                 sto:TechnicalSpecification .


###  https://w3id.org/i40/sto#VDE_2182
sto:VDE_2182 rdf:type owl:NamedIndividual ,
                      sto:Standard ;
             dcterms:creator sto:VDI ,
                             sto:sebastian ;
             foaf:maker sto:VDI ;
             sto:hasClassification sto:AsSecurity ;
             sto:hasDeveloper sto:VDI ;
             sto:hasPublisher sto:VDI ;
             dcterms:license "private"@en ;
             dcterms:title "IT-security for industrial automation"@en ,
                           "Informationssicherheit in der industriellen Automatisierung"@de ;
             rdfs:comment "This guideline describes how specific measures can be implemented in order to guarantee the IT security of automated machines and plant; aspects of the automation devices, automation systems, and automation applications used are considered. A uniform, feasible procedure for ensuring IT security throughout the entire life cycle of automation devices, systems, and applications is described, based on common terms and definitions agreed by the manufacturers of automation devices and systems and their users (e.g., machine manufacturers, integrators, operators). The life cycle covers the development, integration, operation, migration, and decommissioning phases.This guideline defines a simple procedure model for the development and description of IT Security. The model consists of eight steps."@en ;
             rdfs:label "VDI/VDE 2182"@en ;
             sto:hasOfficialResource <http://www.vdi.eu/nc/guidelines/vdivde_2182_blatt_1-informationssicherheit_in_der_industriellen_automatisierung_allgemeines_vorgehensmode/> .


###  https://w3id.org/i40/sto#VDI
sto:VDI rdf:type owl:NamedIndividual ,
                 foaf:Organization ,
                 sto:StandardOrganization ;
        dcterms:creator sto:sebastian ;
        sto:hasHeadquaterIn dbr:Berlin ;
        sto:abbreviation "VDI"@en ;
        sto:formationDate "1856-05-12"^^xsd:date ;
        sto:orgName "Association of German Engineers"@en ,
                    "Verein Deutscher Ingenieure"@de ;
        rdfs:comment "Verein Deutscher Ingenieure (VDI) (English: Association of German Engineers) is an organization with over 150,000 engineers and natural scientists. More than 12,000 honorary experts process the latest findings every year to promote the technology location. Established in 1856, the VDI is today the largest engineering association in Western Europe. The role of the VDI in Germany is comparable to that of the American Society of Civil Engineers (ASCE) in the United States or Engineers Australia (EA) in Australia barring the broader field of work of the VDI. The VDI is not a union. The association promotes the advancement of technology and represents the interests of engineers and of engineering businesses in Germany."@en ;
        rdfs:label "VDI"@en ;
        sto:hasDBpediaResource <http://dbpedia.org/resource/VDI> ;
        sto:hasOfficialResource <http://www.vdi.eu/> ;
        sto:hasWikipediaArticle <https://en.wikipedia.org/wiki/VDI> .


###  https://w3id.org/i40/sto#VDI_VDE_2182
sto:VDI_VDE_2182 rdf:type owl:NamedIndividual ,
                          sto:Standard ;
                 dcterms:creator sto:VDI ,
                                 sto:sebastian ;
                 foaf:maker sto:VDI ;
                 sto:hasClassification sto:AsSecurity ;
                 sto:hasDeveloper sto:VDI ;
                 sto:hasPublisher sto:VDI ;
                 dcterms:license sto:PrivateLicenseDocument ;
                 dcterms:title "IT-security for industrial automation"@en ,
                               "Informationssicherheit in der industriellen Automatisierung"@de ;
                 rdfs:comment "This guideline describes how specific measures can be implemented in order to guarantee the IT security of automated machines and plant; aspects of the automation devices, automation systems, and automation applications used are considered. A uniform, feasible procedure for ensuring IT security throughout the entire life cycle of automation devices, systems, and applications is described, based on common terms and definitions agreed by the manufacturers of automation devices and systems and their users (e.g., machine manufacturers, integrators, operators). The life cycle covers the development, integration, operation, migration, and decommissioning phases.This guideline defines a simple procedure model for the development and description of IT Security. The model consists of eight steps."@en ;
                 rdfs:label "VDI/VDE 2182"@en ;
                 sto:hasOfficialResource <http://www.vdi.eu/nc/guidelines/vdivde_2182_blatt_1-informationssicherheit_in_der_industriellen_automatisierung_allgemeines_vorgehensmode/> .


###  https://w3id.org/i40/sto#VDMA
sto:VDMA rdf:type owl:NamedIndividual ,
                  foaf:Organization ,
                  sto:StandardOrganization ;
         sto:hasHeadquaterIn dbr:Frankfurt ;
         sto:abbreviation "VDMA"^^xsd:string ;
         sto:formationDate "1892-11-15"^^xsd:date ;
         sto:orgName "Mechanical Engineering Industry Association"@en ,
                     "Verband Deutscher Maschinen- und Anlagenbau"@de ;
         rdfs:comment "The Mechanical Engineering Industry Association (Verband Deutscher Maschinen- und Anlagenbau – VDMA) has its headquarters in Frankfurt am Main, Germany, and represents around 3,200 members, making it the largest industry association in Europe. The Association represents the interests of the predominantly medium-sized companies in the mechanical engineering industry towards policymakers and society, as well as towards business, the scientific community, public authorities and the media. With more than one million employees and a turnover of around EUR 218 billion (2015), mechanical and plant engineering is Germany’s largest employer in the industrial sector.In addition, VDMA sees itself as a platform that provides its member companies with various networks where they can discuss technological challenges, interdisciplinary issues and many other topics."@en ;
         sto:hasDBpediaResource <http://dbpedia.org/resource/VDMA> ;
         sto:hasOfficialResource <http://www.vdma.org> ;
         sto:hasWikipediaArticle <https://en.wikipedia.org/wiki/Mechanical_Engineering_Industry_Association> .


###  https://w3id.org/i40/sto#VDMA_24582
sto:VDMA_24582 rdf:type owl:NamedIndividual ,
                        foaf:Document ,
                        sto:Publication ,
                        sto:Standard ;
               dcterms:creator sto:VDMA ;
               foaf:maker sto:VDMA ;
               sto:hasClassification sto:AsConditionMonitoring ;
               sto:hasPublisher sto:VDMA ;
               rdfs:comment "Fieldbus neutral reference architecture for Condition Monitoring in production automation"@en ;
               rdfs:label "VDMA 24582"@en ;
               sto:hasOfficialResource <https://www.vdma.org/documents/105628/2244593/Inhalt+VDMA+24582_en.pdf/> .


###  https://w3id.org/i40/sto#Vocabulary
sto:Vocabulary rdf:type owl:NamedIndividual .


###  https://w3id.org/i40/sto#W3C
sto:W3C rdf:type owl:NamedIndividual ,
                 foaf:Organization ,
                 sto:StandardOrganization ;
        sto:hasHeadquaterIn dbr:_Massachusetts ;
        sto:abbreviation "W3C"^^xsd:string ;
        sto:formationDate "1994-10-01"^^xsd:date ;
        sto:orgName "World Wide Web Consortium"@en ;
        rdfs:comment "The World Wide Web Consortium (W3C) is the main international standards organization for the World Wide Web (abbreviated WWW or W3). Founded and currently led by Tim Berners-Lee, the consortium is made up of member organizations which maintain full-time staff for the purpose of working together in the development of standards for the World Wide Web. As of 4 November 2015, the World Wide Web Consortium (W3C) has 408 members. The W3C also engages in education and outreach, develops software and serves as an open forum for discussion about the Web."@en ;
        rdfs:label "W3C"@en ;
        sto:hasDBpediaResource <http://dbpedia.org/resource/World_Wide_Web_Consortium> ;
        sto:hasOfficialResource <https://www.w3.org/> ;
        sto:hasWikipediaArticle <https://en.wikipedia.org/wiki/World_Wide_Web_Consortium> .


###  https://w3id.org/i40/sto#W3C_DCAT
sto:W3C_DCAT rdf:type owl:NamedIndividual ,
                      foaf:Document ,
                      sto:Publication ,
                      sto:Standard ;
             dcterms:creator sto:W3C ,
                             sto:sebastian ;
             foaf:maker sto:W3C ;
             sto:hasDeveloper sto:W3C ;
             sto:hasPublisher sto:W3C ;
             rdfs:comment """DCAT is an RDF vocabulary designed to facilitate interoperability between data catalogs published on the Web. This document defines the schema and provides examples for its use.

By using DCAT to describe datasets in data catalogs, publishers increase discoverability and enable applications easily to consume metadata from multiple catalogs. It further enables decentralized publishing of catalogs and facilitates federated dataset search across sites. Aggregated DCAT metadata can serve as a manifest file to facilitate digital preservation."""@en ;
             rdfs:label "DCAT"@en ;
             sto:hasDBpediaResource <http://dbpedia.org/resource/Data_Catalog_Vocabulary> ;
             sto:hasOfficialResource <https://www.w3.org/TR/vocab-dcat/> ;
             sto:hasWikipediaArticle <https://en.wikipedia.org/wiki/Data_Catalog_Vocabulary> .


###  https://w3id.org/i40/sto#W3C_OWL
sto:W3C_OWL rdf:type owl:NamedIndividual ,
                     foaf:Document ,
                     sto:Publication ,
                     sto:Standard ;
            dcterms:creator sto:W3C ;
            foaf:maker sto:W3C ;
            sto:hasPublisher sto:W3C ;
            sto:relatedTo sto:W3C_RDF ;
            sto:hasTag "OWL"@en ;
            dcterms:license sto:PublicLicenseDocument ;
            rdfs:comment "The W3C Web Ontology Language (OWL) is a Semantic Web language designed to represent rich and complex knowledge about things, groups of things, and relations between things. OWL is a computational logic-based language such that knowledge expressed in OWL can be exploited by computer programs, e.g., to verify the consistency of that knowledge or to make implicit knowledge explicit. OWL documents, known as ontologies, can be published in the World Wide Web and may refer to or be referred from other OWL ontologies. OWL is part of the W3C’s Semantic Web technology stack, which includes RDF, RDFS, SPARQL, etc."@en ;
            rdfs:label "Web Ontology Language"@en ;
            sto:hasDBpediaResource <http://dbpedia.org/resource/Web_Ontology_Language> ;
            sto:hasOfficialResource <https://www.w3.org/OWL/> ;
            sto:hasWikipediaArticle <https://en.wikipedia.org/wiki/Web_Ontology_Language?oldformat=true> .


###  https://w3id.org/i40/sto#W3C_RDF
sto:W3C_RDF rdf:type owl:NamedIndividual ,
                     foaf:Document ,
                     sto:Publication ,
                     sto:Standard ;
            dcterms:creator sto:W3C ;
            foaf:maker sto:W3C ;
            sto:hasPublisher sto:W3C ;
            sto:hasTag "RDF"@en ;
            dcterms:license sto:PublicLicenseDocument ;
            rdfs:comment "RDF is a standard model for data interchange on the Web. RDF has features that facilitate data merging even if the underlying schemas differ, and it specifically supports the evolution of schemas over time without requiring all the data consumers to be changed. "@en ;
            rdfs:label "Resource Description Framework"@en ;
            sto:hasDBpediaResource <http://dbpedia.org/resource/Resource_Description_Framework> ;
            sto:hasOfficialResource <https://www.w3.org/RDF/> ;
            sto:hasWikipediaArticle <https://en.wikipedia.org/wiki/Resource_Description_Framework> .


###  https://w3id.org/i40/sto#W3C_RIF
sto:W3C_RIF rdf:type owl:NamedIndividual ,
                     foaf:Document ,
                     sto:Publication ,
                     sto:Standard ;
            dcterms:creator sto:W3C ;
            foaf:maker sto:W3C ;
            sto:hasPublisher sto:W3C ;
            sto:relatedTo sto:W3C_OWL ;
            sto:hasTag "RIF"@en ;
            dcterms:license sto:PublicLicenseDocument ;
            rdfs:comment "The Rule Interchange Format (RIF) is a W3C Recommendation. RIF is part of the infrastructure for the semantic web, along with (principally) SPARQL, RDF and OWL. Although originally envisioned by many as a rules layer for the semantic web, in reality the design of RIF is based on the observation that there are many rules languages in existence, and what is needed is to exchange rules between them."@en ;
            rdfs:label "Rule Interchange Format"@en ;
            sto:hasDBpediaResource <http://dbpedia.org/resource/Rule_Interchange_Format> ;
            sto:hasOfficialResource <https://www.w3.org/TR/rif-overview/> ;
            sto:hasWikipediaArticle <https://en.wikipedia.org/wiki/Rule_Interchange_Format> .


###  https://w3id.org/i40/sto#W3C_SPARQL
sto:W3C_SPARQL rdf:type owl:NamedIndividual ,
                        foaf:Document ,
                        sto:Publication ,
                        sto:Standard ;
               dcterms:creator sto:W3C ;
               foaf:maker sto:W3C ;
               sto:hasPublisher sto:W3C ;
               sto:relatedTo sto:W3C_RDF ;
               sto:hasTag "SPARQL"@en ;
               dcterms:license sto:PublicLicenseDocument ;
               rdfs:comment "The SPARQL Protocol and RDF Query Language (SPARQL) is a query language and protocol for RDF. This document specifies the SPARQL Protocol; it describes a means for conveying SPARQL queries and updates to a SPARQL processing service and returning the results via HTTP to the entity that requested them. This protocol was developed by the W3C SPARQL Working Group, part of the Semantic Web Activity as described in the activity statement ."@en ;
               rdfs:label "SPARQL"@en ;
               sto:hasDBpediaResource <http://dbpedia.org/resource/SPARQL> ;
               sto:hasOfficialResource <https://www.w3.org/SPARQL> ;
               sto:hasWikipediaArticle <https://en.wikipedia.org/wiki/SPARQL> .


###  https://w3id.org/i40/sto#Weave
sto:Weave rdf:type owl:NamedIndividual ,
                   foaf:Document ,
                   sto:Publication ,
                   sto:TechnicalSpecification ;
          dcterms:creator sto:sebastian ;
          rdfs:comment "A communications platform for IoT devices that enables device setup, phone-to-device-to-cloud communication, and user interaction from mobile devices and the web. (source: https://www.postscapes.com/internet-of-things-protocols/)"@en ;
          rdfs:label "Weave"@en ;
          sto:hasOfficialResource <https://developers.google.com/weave/> .


###  https://w3id.org/i40/sto#WebSocket
sto:WebSocket rdf:type owl:NamedIndividual ,
                       foaf:Document ,
                       sto:Publication ,
                       sto:TechnicalSpecification ;
              dcterms:creator sto:sebastian ;
              rdfs:comment "The WebSocket specification — developed as part of the HTML5 initiative — introduced the WebSocket JavaScript interface, which defines a full-duplex single socket connection over which messages can be sent between client and server. The WebSocket standard simplifies much of the complexity around bi-directional web communication and connection management. (source: https://www.postscapes.com/internet-of-things-protocols/)"@en ;
              rdfs:label "WebSocket"@en ;
              sto:hasOfficialResource <https://websocket.org/> .


###  https://w3id.org/i40/sto#Weightless
sto:Weightless rdf:type owl:NamedIndividual ,
                        foaf:Document ,
                        sto:Publication ,
                        sto:TechnicalSpecification ;
               dcterms:creator sto:sebastian ;
               rdfs:comment "Weightless is a proposed proprietary open wireless technology standard for exchanging data between a base station and thousands of machines around it (using wavelength radio transmissions in unoccupied TV transmission channels) with high levels of security.  (source: https://www.postscapes.com/internet-of-things-protocols/)"@en ;
               rdfs:label "Weightless"@en ;
               sto:hasOfficialResource <http://www.weightless.org/> .


###  https://w3id.org/i40/sto#WiFi
sto:WiFi rdf:type owl:NamedIndividual ,
                  foaf:Document ,
                  sto:Publication ,
                  sto:TechnicalSpecification ;
         dcterms:creator sto:sebastian ;
         sto:hasClassification sto:OpenFogNodeView ;
         rdfs:label "WiFi"@en ;
         sto:hasOfficialResource <https://www.wi-fi.org/> .


###  https://w3id.org/i40/sto#WiMax
sto:WiMax rdf:type owl:NamedIndividual ,
                   foaf:Document ,
                   sto:Publication ,
                   sto:TechnicalSpecification ;
          dcterms:creator sto:sebastian ;
          rdfs:comment "WiMax is based on the standard IEEE 802.16 and is intended for wireless metropolitan area networks. The range is different for fixed stations, where it can go up to 50 km and mobile devices with 5 to 15 km. WiMAx operates at frequencies between 2.5 GHz to 5.8 GHz with a transferrate of 40 Mbps.  (source: https://www.postscapes.com/internet-of-things-protocols/)"@en ;
          rdfs:label "WiMax"@en ;
          sto:hasWikipediaArticle <https://en.wikipedia.org/wiki/WiMAX> .


###  https://w3id.org/i40/sto#WiSunAlliance
sto:WiSunAlliance rdf:type owl:NamedIndividual ,
                           foaf:Organization ,
                           sto:IIoTConsortium ;
                  dcterms:creator sto:sebastian ;
                  rdfs:comment "The Wi-SUN Alliance seeks to advance seamless connectivity by promoting IEEE 802.15.4g standard based interoperability for global regional markets. (source: https://www.postscapes.com/internet-of-things-protocols/)"@en ;
                  rdfs:label "Wi-SUN Alliance"@en ;
                  sto:hasOfficialResource <http://www.wi-sun.org/> .


###  https://w3id.org/i40/sto#WirelessHart
sto:WirelessHart rdf:type owl:NamedIndividual ,
                          foaf:Document ,
                          sto:Publication ,
                          sto:TechnicalSpecification ;
                 dcterms:creator sto:sebastian ;
                 rdfs:comment "WirelessHART technology provides a robust wireless protocol for the full range of process measurement, control, and asset management applications. (source: https://www.postscapes.com/internet-of-things-protocols/)"@en ;
                 rdfs:label "WirelessHart"@en ;
                 sto:hasOfficialResource <http://www.hartcomm.org/protocol/wihart/wireless_technology.html> .


###  https://w3id.org/i40/sto#WolframLanguage
sto:WolframLanguage rdf:type owl:NamedIndividual ,
                             foaf:Document ,
                             sto:Publication ,
                             sto:TechnicalSpecification ;
                    dcterms:creator sto:sebastian ;
                    rdfs:comment "A symbolic representation of each device. Then there are a standard set of Wolfram Language functions like DeviceRead, DeviceExecute, DeviceReadBuffer and DeviceReadTimeSeries that perform operations related to the device. (source: https://www.postscapes.com/internet-of-things-protocols/)"@en ;
                    rdfs:label "Wolfram Language"@en ;
                    sto:hasOfficialResource <https://reference.wolfram.com/language/guide/ConnectingToDevices.html> .


###  https://w3id.org/i40/sto#X509
sto:X509 rdf:type owl:NamedIndividual ,
                  sto:Standard ;
         dcterms:creator sto:sebastian ;
         rdfs:comment "Standard for public key infrastructure (PKI) to manage digital certificates and public-key encryption. A key part of the Transport Layer Security protocol used to secure web and email communication.  (source: https://www.postscapes.com/internet-of-things-protocols/)"@en ;
         rdfs:label "X.509"@en ;
         sto:hasPublisher <http://dbpedia.org/resource/International_Telecommunication_Union> ;
         sto:hasOfficialResource <https://www.itu.int/rec/T-REC-X.509> ;
         sto:hasWikipediaArticle <https://en.wikipedia.org/wiki/X.509> .


###  https://w3id.org/i40/sto#XACML
sto:XACML rdf:type owl:NamedIndividual ,
                   foaf:Document ,
                   sto:Publication ,
                   sto:TechnicalSpecification ;
          dul:associatedWith sto:FiwareSecurity ;
          sto_iot:hasTargetConcern sto:Authorization ,
                                   sto:DataAccessControl .


###  https://w3id.org/i40/sto#XMPP
sto:XMPP rdf:type owl:NamedIndividual ,
                  sto:TechnicalSpecification ;
         dcterms:creator sto:sebastian ;
         rdfs:comment "XMPP (Extensible Messaging and Presence Protocol): An open technology for real-time communication, which powers a wide range of applications including instant messaging, presence, multi-party chat, voice and video calls, collaboration, lightweight middleware, content syndication, and generalized routing of XML data. (source: https://www.postscapes.com/internet-of-things-protocols/)"@en ;
         rdfs:label "XMPP"@en ;
         sto:hasOfficialResource <https://xmpp.org/> .


###  https://w3id.org/i40/sto#XMPP-IoT
sto:XMPP-IoT rdf:type owl:NamedIndividual ,
                      sto:TechnicalSpecification ;
             dcterms:creator sto:sebastian ;
             rdfs:comment "XMPP-IoT: In the same manor as XMPP silently has created people to people communication interoperable. We are aiming to make communication machine to people and machine to machine interoperable. (source: https://www.postscapes.com/internet-of-things-protocols/)"@en ;
             rdfs:label "XMPP-IoT"@en ;
             sto:hasOfficialResource <https://github.com/joachimlindborg/XMPP-IoT> .


###  https://w3id.org/i40/sto#ZVEI
sto:ZVEI rdf:type owl:NamedIndividual ,
                  sto:StandardOrganization ;
         dcterms:title "German Electrical and Electronic Manufacturers' Association"@en ,
                       "Zentralverband Elektrotechnik- und Elektronikindustrie"@de ;
         rdfs:comment "The ZVEI is one of the most important manufacturers' associations in Germany. It represents the interests of a high-tech branch with a very widely varied and extremely dynamic product portfolio."@en ;
         rdfs:label "ZVEI"@en ;
         sto:hasOfficialResource <https://www.zvei.org/> ;
         .


###  https://w3id.org/i40/sto#ZigBee
sto:ZigBee rdf:type owl:NamedIndividual ,
                    sto:TechnicalSpecification ;
           dcterms:creator sto:irlan ,
                           sto:sebastian ;
           rdfs:comment "The ZigBee protocol uses the 802.15.4 standard and operates in the 2.4 GHz frequency range with 250 kbps. The maximum number of nodes in the network is 1024 with a range up to 200 meter. ZigBee can use 128 bit AES encryption. (source: https://www.postscapes.com/internet-of-things-protocols/)"@en ;
           rdfs:label "ZigBee"@en ;
           sto:hasOfficialResource <http://www.zigbee.org/> .


###  https://w3id.org/i40/sto#bitkom
sto:bitkom rdf:type owl:NamedIndividual ,
                    foaf:Organization ,
                    sto:StandardOrganization ;
           dcterms:creator sto:sebastian ;
           dcterms:title "Bundesverband Informationswirtschaft, Telekommunikation und neue Medien"@de ,
                         "German Association for IT, Telecommunications and New Media"@en ;
           rdfs:label "Bitkom"@en ;
           sto:hasOfficialResource <https://www.bitkom.org/> ;
           sto:hasWikipediaArticle <https://de.wikipedia.org/wiki/Bundesverband_Informationswirtschaft,_Telekommunikation_und_neue_Medien'> .


###  https://w3id.org/i40/sto#communication
sto:communication rdf:type owl:NamedIndividual .


###  https://w3id.org/i40/sto#eClass
sto:eClass rdf:type owl:NamedIndividual ,
                    sto:Standard ;
           dcterms:creator sto:eClassAssoc ;
           foaf:maker sto:eClassAssoc ;
           sto:hasClassification sto:AsEngineering ,
                                 sto:RamiConnectedWorld ,
                                 sto:RamiControlDevice ,
                                 sto:RamiEnterprise ,
                                 sto:RamiProduct ,
                                 sto:RamiStation ,
                                 sto:RamiWorkCenter ;
           sto:hasDeveloper sto:eClassAssoc ;
           sto:hasPublisher sto:eClassAssoc ;
           sto:relatedTo sto:DIN_SPEC_16592 ,
                         sto:IEC_61131 ,
                         sto:IEC_61360 ,
                         sto:IEC_61499 ,
                         sto:IEC_61804 ,
                         sto:IEC_61850 ,
                         sto:IEC_61987_X ,
                         sto:IEC_62424 ,
                         sto:IEC_62453 ,
                         sto:IEC_62541 ,
                         sto:IEC_62714 ,
                         sto:ISO_13584 ,
                         sto:ISO_14306 ,
                         sto:ISO_15746 ,
                         sto:ISO_15926 ,
                         sto:ISO_18629 ,
                         sto:ISO_18828-2 ,
                         sto:ISO_20922 ,
                         sto:ISO_22400 ,
                         sto:ISO_29002 ,
                         sto:ISO_ASTM_52915 ,
                         sto:ISO_PAS_17506 ,
                         sto:MathML ,
                         sto:SysML ,
                         sto:eClass ;
           sto:hasMotivation "Global identification, semantic description and automatic product classification"@en ;
           rdfs:comment "eCl@ss is the cross-industry product data standard for classification and clear description of products and services."@en ;
           rdfs:label "eClass"@en ;
           sto:hasDBpediaResource <http://de.dbpedia.org/page/ECl@ss> ;
           sto:hasOfficialResource <https://www.eclass.eu/eclasscontent/standard/overview.html.en> ;
           sto:hasWikipediaArticle <https://de.wikipedia.org/wiki/ECl@ss> .


###  https://w3id.org/i40/sto#eClassAssoc
sto:eClassAssoc rdf:type owl:NamedIndividual ,
                         foaf:Organization ,
                         sto:StandardOrganization ;
                sto:hasHeadquaterIn dbr:Cologne ;
                sto:abbreviation "eCl@ss"^^xsd:string ,
                                 "eClass"^^xsd:string ;
                sto:formationDate "2000-11-14"^^xsd:date ;
                sto:orgName "eCl@ss e. V."@de ;
                rdfs:comment "Der eCl@ss e. V. ist eine Non-Profit-Organisation, die den gleichnamigen Klassifikationsstandard branchenübergreifend international definiert, weiterentwickelt und verbreitet. Der Verein wird getragen von ordentlichen und fördernden Mitgliedern aus Unternehmen, Verbänden und Institutionen."@de ;
                sto:hasOfficialResource <https://www.eclass.eu> ;
                sto:hasWikipediaArticle <https://www.wikiwand.com/de/ECl@ss> .


###  https://w3id.org/i40/sto#ebXML
sto:ebXML rdf:type owl:NamedIndividual ,
                   sto:Standard ;
          dcterms:creator sto:irlan ,
                          sto:sebastian ;
          sto:hasClassification sto:NISTBusinessProcessExecution ;
          sto:hasPublisher sto:OASIS ,
                           sto:UN-CEFACT ;
          sto:hasTag "ebXML"@en ;
          rdfs:comment "Electronic Business using eXtensible Markup Language, commonly known as e-business XML, or ebXML is a family of XML based standards whose mission is to provide an open, XML-based infrastructure that enables the global use of electronic business information in an interoperable, secure, and consistent manner by all trading partners."@en ;
          rdfs:label "ebXML"@en ;
          sto:hasDBpediaResource <http://dbpedia.org/resource/EbXML> ;
          sto:hasOfficialResource <https://webstore.iec.ch/publication/24433> ;
          sto:hasWikipediaArticle <https://en.wikipedia.org/wiki/EbXML> .


###  https://w3id.org/i40/sto#irlan
sto:irlan rdf:type owl:NamedIndividual ,
                   foaf:Person ;
          rdfs:label "Irlan Grangel"^^xsd:string ;
          foaf:familyName "Grangel"^^xsd:string ;
          foaf:mbox "irlangrangel2003@gmail.com"^^xsd:string ;
          foaf:name "Irlan"^^xsd:string .


###  https://w3id.org/i40/sto#mDNS
sto:mDNS rdf:type owl:NamedIndividual ,
                  sto:TechnicalSpecification ;
         dcterms:creator sto:sebastian ;
         rdfs:comment "mDNS (multicast Domain Name System) - Resolves host names to IP addresses within small networks that do not include a local name server. (source: https://www.postscapes.com/internet-of-things-protocols/)"@en ;
         rdfs:label "mDNS"@en ;
         sto:hasDBpediaResource <http://dbpedia.org/page/Multicast_DNS> ;
         sto:hasWikipediaArticle <https://en.wikipedia.org/wiki/Multicast_DNS> .


###  https://w3id.org/i40/sto#oneM2M
sto:oneM2M rdf:type owl:NamedIndividual ,
                    sto:StandardOrganization ;
           rdfs:comment "The purpose and goal of oneM2M is to develop technical specifications which address the need for a common M2M Service Layer that can be readily embedded within various hardware and software, and relied upon to connect the myriad of devices in the field with M2M application servers worldwide. A critical objective of oneM2M is to attract and actively involve organizations from M2M-related business domains such as: telematics and intelligent transportation, healthcare, utilities, industrial automation, smart homes, etc."@en ;
           rdfs:label "oneM2M"@en ;
           sto:hasOfficialResource <http://www.onem2m.org/about-onem2m/why-onem2m> .


###  https://w3id.org/i40/sto#openAAS
sto:openAAS rdf:type owl:NamedIndividual ,
                     sto:TechnicalSpecification ;
            dcterms:creator sto:sebastian ;
            dul:associatedWith sto:AdministrationShell ;
            rdfs:comment """Im Open Source Projekt „openAAS“ – die Abkürzung „AAS“ steht für den englischen Begriff „Asset Administration Shell“, zu Deutsch „Verwaltungsschale“ – arbeitet der ZVEI gemeinsam mit der RWTH Aachen und Unternehmen aus Maschinenbau und Elektroindustrie daran, Industrie 4.0 in die Praxis
umzusetzen. Die Veranschaulichung und Erprobung einer Industrie-4.0-konformen Verwaltungsschale stehen im Mittelpunkt. Dies ist Voraussetzung für eine international erfolgreiche Technologieverifikation
und Standardisierung."""@de ,
                         "openAAS is an open source project to establish a Platform Industry 4.0 conform Administration Shell with open software."@en ;
            rdfs:label "openAAS"@en .


###  https://w3id.org/i40/sto#sebastian
sto:sebastian rdf:type owl:NamedIndividual ,
                       foaf:Person ;
              rdfs:label "Sebastian Bader"^^xsd:string ;
              foaf:familyName "Bader"^^xsd:string ;
              foaf:name "Sebastian"^^xsd:string ;
              sto:hasOfficialResource <https://sebastianrbader.de> .


###  https://w3id.org/i40/sto#uIP
sto:uIP rdf:type owl:NamedIndividual ,
                 sto:TechnicalSpecification ;
        dcterms:creator sto:sebastian ;
        rdfs:comment "The uIP is an open source TCP/IP stack capable of being used with tiny 8- and 16-bit microcontrollers. It was initially developed by Adam Dunkels of the 'Networked Embedded Systems' group at the Swedish Institute of Computer Science, licensed under a BSD style license, and further developed by a wide group of developers. (source: https://www.postscapes.com/internet-of-things-protocols/)"@en ;
        rdfs:label "uIP"@en ;
        sto:hasWikipediaArticle <https://en.wikipedia.org/wiki/UIP_%28micro_IP%29> .


###  https://www.linkedin.com/in/paul-baptista-601177b2
<https://www.linkedin.com/in/paul-baptista-601177b2> rdf:type owl:NamedIndividual ,
                                                              foaf:Person ;
                                                     rdfs:label "Paul Baptista"^^xsd:string .


###  https://www.wikidata.org/wiki/Q1548249
<https://www.wikidata.org/wiki/Q1548249> rdf:type owl:NamedIndividual ,
                                                  sto_iot:hasStakeholder ;
                                         rdfs:label "System Architect"@en .


#################################################################
#    Annotations
#################################################################


